<?xml version="1.0"?>
<rdf:RDF xmlns="http://www.ontologyrepository.com/CommonCoreOntologies/Domain/CyberOntology#"
     xml:base="http://www.ontologyrepository.com/CommonCoreOntologies/Domain/CyberOntology"
     xmlns:dc="http://purl.org/dc/elements/1.1/"
     xmlns:obo="http://purl.obolibrary.org/obo/"
     xmlns:owl="http://www.w3.org/2002/07/owl#"
     xmlns:rdf="http://www.w3.org/1999/02/22-rdf-syntax-ns#"
     xmlns:xml="http://www.w3.org/XML/1998/namespace"
     xmlns:xsd="http://www.w3.org/2001/XMLSchema#"
     xmlns:cco2="https://www.commoncoreontologies.org/"
     xmlns:rdfs="http://www.w3.org/2000/01/rdf-schema#"
     xmlns:skos="http://www.w3.org/2004/02/skos/core#"
     xmlns:terms="http://purl.org/dc/terms/">
    <owl:Ontology rdf:about="http://www.ontologyrepository.com/CommonCoreOntologies/Domain/CyberOntology">
        <owl:versionIRI rdf:resource="http://www.ontologyrepository.com/CommonCoreOntologies/Domain/2024-04-17/CyberOntology"/>
        <owl:imports rdf:resource="https://www.commoncoreontologies.org/AllCoreOntology"/>
        <terms:license xml:lang="en">Copyright 2024 CUBRC Inc.

https://opensource.org/license/bsd-3-clause

Redistribution and use in source and binary forms, with or without modification, are permitted provided that the following conditions are met:

1. Redistributions of source code must retain the above copyright notice, this list of conditions and the following disclaimer.

2. Redistributions in binary form must reproduce the above copyright notice, this list of conditions and the following disclaimer in the documentation and/or other materials provided with the distribution.

3. Neither the name of the copyright holder nor the names of its contributors may be used to endorse or promote products derived from this software without specific prior written permission.

THIS SOFTWARE IS PROVIDED BY THE COPYRIGHT HOLDERS AND CONTRIBUTORS “AS IS” AND ANY EXPRESS OR IMPLIED WARRANTIES, INCLUDING, BUT NOT LIMITED TO, THE IMPLIED WARRANTIES OF MERCHANTABILITY AND FITNESS FOR A PARTICULAR PURPOSE ARE DISCLAIMED. IN NO EVENT SHALL THE COPYRIGHT HOLDER OR CONTRIBUTORS BE LIABLE FOR ANY DIRECT, INDIRECT, INCIDENTAL, SPECIAL, EXEMPLARY, OR CONSEQUENTIAL DAMAGES (INCLUDING, BUT NOT LIMITED TO, PROCUREMENT OF SUBSTITUTE GOODS OR SERVICES; LOSS OF USE, DATA, OR PROFITS; OR BUSINESS INTERRUPTION) HOWEVER CAUSED AND ON ANY THEORY OF LIABILITY, WHETHER IN CONTRACT, STRICT LIABILITY, OR TORT (INCLUDING NEGLIGENCE OR OTHERWISE) ARISING IN ANY WAY OUT OF THE USE OF THIS SOFTWARE, EVEN IF ADVISED OF THE POSSIBILITY OF SUCH DAMAGE.</terms:license>
        <rdfs:comment xml:lang="en">The Cyber Ontology is designed to serve as a domain-level reference for representing entities relevant to the digitization, manipulation, and transfer of information using telecommunication networks, especially as they pertain to activities in cyberspace. Examples include: information processing artifacts and their functions, networks and their components, software, protocols and standards, users and their permissions, data transformation and encoding, cyber attacks and their objectives.</rdfs:comment>
        <rdfs:comment xml:lang="en">There are at least three unique senses of &apos;cyberspace&apos;: the interconnected physical devices that make up a telecommunication network; a space within those systems, presumably where electromagnetic energy flows; and the logical space of sequences and patterns of structured information carriers within that flow of energy. This last sense is analogous to the propagation of sound waves through the air or ripples in a pond and is closest to the view referred to within the defining elements of this ontology. However, all three may be applicable to articulate enties relevant to the cyber domain. Thus, we do not attempt to define &apos;cyberspace&apos; formally and leave it as primitive. See Here: https://csrc.nist.gov/glossary/term/cyberspace.</rdfs:comment>
        <rdfs:label xml:lang="en">Cyber Ontology</rdfs:label>
        <owl:versionInfo xml:lang="en">Compatible with CCO version 1.5</owl:versionInfo>
    </owl:Ontology>
    


    <!-- 
    ///////////////////////////////////////////////////////////////////////////////////////
    //
    // Annotation properties
    //
    ///////////////////////////////////////////////////////////////////////////////////////
     -->

    


    <!-- http://purl.org/dc/elements/1.1/contributor -->

    <owl:AnnotationProperty rdf:about="http://purl.org/dc/elements/1.1/contributor"/>
    


    <!-- http://purl.org/dc/terms/creator -->

    <owl:AnnotationProperty rdf:about="http://purl.org/dc/terms/creator"/>
    


    <!-- http://purl.org/dc/terms/license -->

    <owl:AnnotationProperty rdf:about="http://purl.org/dc/terms/license"/>
    


    <!-- https://www.commoncoreontologies.org/ont00001753 -->

    <owl:AnnotationProperty rdf:about="https://www.commoncoreontologies.org/ont00001753"/>
    


    <!-- https://www.commoncoreontologies.org/ont00001754 -->

    <owl:AnnotationProperty rdf:about="https://www.commoncoreontologies.org/ont00001754"/>
    


    <!-- https://www.commoncoreontologies.org/ont00001760 -->

    <owl:AnnotationProperty rdf:about="https://www.commoncoreontologies.org/ont00001760"/>
    


    <!-- 
    ///////////////////////////////////////////////////////////////////////////////////////
    //
    // Object Properties
    //
    ///////////////////////////////////////////////////////////////////////////////////////
     -->

    


    <!-- http://purl.obolibrary.org/obo/BFO_0000054 -->

    <owl:ObjectProperty rdf:about="http://purl.obolibrary.org/obo/BFO_0000054"/>
    


    <!-- http://purl.obolibrary.org/obo/BFO_0000055 -->

    <owl:ObjectProperty rdf:about="http://purl.obolibrary.org/obo/BFO_0000055"/>
    


    <!-- http://purl.obolibrary.org/obo/BFO_0000056 -->

    <owl:ObjectProperty rdf:about="http://purl.obolibrary.org/obo/BFO_0000056"/>
    


    <!-- http://purl.obolibrary.org/obo/BFO_0000057 -->

    <owl:ObjectProperty rdf:about="http://purl.obolibrary.org/obo/BFO_0000057"/>
    


    <!-- http://purl.obolibrary.org/obo/BFO_0000066 -->

    <owl:ObjectProperty rdf:about="http://purl.obolibrary.org/obo/BFO_0000066"/>
    


    <!-- http://purl.obolibrary.org/obo/BFO_0000171 -->

    <owl:ObjectProperty rdf:about="http://purl.obolibrary.org/obo/BFO_0000171"/>
    


    <!-- http://purl.obolibrary.org/obo/BFO_0000176 -->

    <owl:ObjectProperty rdf:about="http://purl.obolibrary.org/obo/BFO_0000176"/>
    


    <!-- http://purl.obolibrary.org/obo/BFO_0000178 -->

    <owl:ObjectProperty rdf:about="http://purl.obolibrary.org/obo/BFO_0000178"/>
    


    <!-- http://purl.obolibrary.org/obo/BFO_0000196 -->

    <owl:ObjectProperty rdf:about="http://purl.obolibrary.org/obo/BFO_0000196"/>
    


    <!-- http://purl.obolibrary.org/obo/BFO_0000197 -->

    <owl:ObjectProperty rdf:about="http://purl.obolibrary.org/obo/BFO_0000197"/>
    


    <!-- http://www.ontologyrepository.com/CommonCoreOntologies/file_attachment_of -->

    <owl:ObjectProperty rdf:about="http://www.ontologyrepository.com/CommonCoreOntologies/file_attachment_of">
        <rdfs:subPropertyOf rdf:resource="http://purl.obolibrary.org/obo/BFO_0000176"/>
        <owl:inverseOf rdf:resource="http://www.ontologyrepository.com/CommonCoreOntologies/has_file_attachment"/>
        <rdfs:label xml:lang="en">file attachment of</rdfs:label>
        <cco2:ont00001760 rdf:datatype="http://www.w3.org/2001/XMLSchema#anyURI">http://www.ontologyrepository.com/CommonCoreOntologies/Domain/CyberOntology</cco2:ont00001760>
    </owl:ObjectProperty>
    


    <!-- http://www.ontologyrepository.com/CommonCoreOntologies/format_used_in -->

    <owl:ObjectProperty rdf:about="http://www.ontologyrepository.com/CommonCoreOntologies/format_used_in">
        <rdfs:subPropertyOf rdf:resource="https://www.commoncoreontologies.org/ont00001942"/>
        <owl:inverseOf rdf:resource="http://www.ontologyrepository.com/CommonCoreOntologies/uses_format"/>
        <rdfs:label xml:lang="en">format used in</rdfs:label>
        <cco2:ont00001760 rdf:datatype="http://www.w3.org/2001/XMLSchema#anyURI">http://www.ontologyrepository.com/CommonCoreOntologies/Domain/CyberOntology</cco2:ont00001760>
    </owl:ObjectProperty>
    


    <!-- http://www.ontologyrepository.com/CommonCoreOntologies/has_causal_factor -->

    <owl:ObjectProperty rdf:about="http://www.ontologyrepository.com/CommonCoreOntologies/has_causal_factor">
        <rdfs:subPropertyOf rdf:resource="http://purl.obolibrary.org/obo/BFO_0000057"/>
        <owl:inverseOf rdf:resource="http://www.ontologyrepository.com/CommonCoreOntologies/is_causal_factor_in"/>
        <rdfs:label xml:lang="en">has causal factor</rdfs:label>
        <cco2:ont00001760 rdf:datatype="http://www.w3.org/2001/XMLSchema#anyURI">http://www.ontologyrepository.com/CommonCoreOntologies/Domain/CyberOntology</cco2:ont00001760>
    </owl:ObjectProperty>
    


    <!-- http://www.ontologyrepository.com/CommonCoreOntologies/has_child_node -->

    <owl:ObjectProperty rdf:about="http://www.ontologyrepository.com/CommonCoreOntologies/has_child_node">
        <owl:inverseOf rdf:resource="http://www.ontologyrepository.com/CommonCoreOntologies/has_parent_node"/>
        <rdfs:label xml:lang="en">has child node</rdfs:label>
        <cco2:ont00001760 rdf:datatype="http://www.w3.org/2001/XMLSchema#anyURI">http://www.ontologyrepository.com/CommonCoreOntologies/Domain/CyberOntology</cco2:ont00001760>
    </owl:ObjectProperty>
    


    <!-- http://www.ontologyrepository.com/CommonCoreOntologies/has_file_attachment -->

    <owl:ObjectProperty rdf:about="http://www.ontologyrepository.com/CommonCoreOntologies/has_file_attachment">
        <rdfs:subPropertyOf rdf:resource="http://purl.obolibrary.org/obo/BFO_0000178"/>
        <rdfs:label xml:lang="en">has file attachment</rdfs:label>
        <cco2:ont00001760 rdf:datatype="http://www.w3.org/2001/XMLSchema#anyURI">http://www.ontologyrepository.com/CommonCoreOntologies/Domain/CyberOntology</cco2:ont00001760>
    </owl:ObjectProperty>
    


    <!-- http://www.ontologyrepository.com/CommonCoreOntologies/has_node_attribute -->

    <owl:ObjectProperty rdf:about="http://www.ontologyrepository.com/CommonCoreOntologies/has_node_attribute">
        <owl:inverseOf rdf:resource="http://www.ontologyrepository.com/CommonCoreOntologies/node_attribute_of"/>
        <rdfs:label xml:lang="en">has node attribute</rdfs:label>
        <cco2:ont00001760 rdf:datatype="http://www.w3.org/2001/XMLSchema#anyURI">http://www.ontologyrepository.com/CommonCoreOntologies/Domain/CyberOntology</cco2:ont00001760>
    </owl:ObjectProperty>
    


    <!-- http://www.ontologyrepository.com/CommonCoreOntologies/has_parent_node -->

    <owl:ObjectProperty rdf:about="http://www.ontologyrepository.com/CommonCoreOntologies/has_parent_node">
        <rdfs:label xml:lang="en">has parent node</rdfs:label>
        <cco2:ont00001760 rdf:datatype="http://www.w3.org/2001/XMLSchema#anyURI">http://www.ontologyrepository.com/CommonCoreOntologies/Domain/CyberOntology</cco2:ont00001760>
    </owl:ObjectProperty>
    


    <!-- http://www.ontologyrepository.com/CommonCoreOntologies/is_causal_factor_in -->

    <owl:ObjectProperty rdf:about="http://www.ontologyrepository.com/CommonCoreOntologies/is_causal_factor_in">
        <rdfs:subPropertyOf rdf:resource="http://purl.obolibrary.org/obo/BFO_0000056"/>
        <rdfs:label xml:lang="en">is causal factor in</rdfs:label>
        <cco2:ont00001760 rdf:datatype="http://www.w3.org/2001/XMLSchema#anyURI">http://www.ontologyrepository.com/CommonCoreOntologies/Domain/CyberOntology</cco2:ont00001760>
    </owl:ObjectProperty>
    


    <!-- http://www.ontologyrepository.com/CommonCoreOntologies/node_attribute_of -->

    <owl:ObjectProperty rdf:about="http://www.ontologyrepository.com/CommonCoreOntologies/node_attribute_of">
        <rdfs:label xml:lang="en">node attribute of</rdfs:label>
        <cco2:ont00001760 rdf:datatype="http://www.w3.org/2001/XMLSchema#anyURI">http://www.ontologyrepository.com/CommonCoreOntologies/Domain/CyberOntology</cco2:ont00001760>
    </owl:ObjectProperty>
    


    <!-- http://www.ontologyrepository.com/CommonCoreOntologies/uses_format -->

    <owl:ObjectProperty rdf:about="http://www.ontologyrepository.com/CommonCoreOntologies/uses_format">
        <rdfs:subPropertyOf rdf:resource="https://www.commoncoreontologies.org/ont00001920"/>
        <rdfs:label xml:lang="en">uses format</rdfs:label>
        <cco2:ont00001760 rdf:datatype="http://www.w3.org/2001/XMLSchema#anyURI">http://www.ontologyrepository.com/CommonCoreOntologies/Domain/CyberOntology</cco2:ont00001760>
    </owl:ObjectProperty>
    


    <!-- https://www.commoncoreontologies.org/ont00001778 -->

    <owl:ObjectProperty rdf:about="https://www.commoncoreontologies.org/ont00001778"/>
    


    <!-- https://www.commoncoreontologies.org/ont00001787 -->

    <owl:ObjectProperty rdf:about="https://www.commoncoreontologies.org/ont00001787"/>
    


    <!-- https://www.commoncoreontologies.org/ont00001803 -->

    <owl:ObjectProperty rdf:about="https://www.commoncoreontologies.org/ont00001803"/>
    


    <!-- https://www.commoncoreontologies.org/ont00001816 -->

    <owl:ObjectProperty rdf:about="https://www.commoncoreontologies.org/ont00001816"/>
    


    <!-- https://www.commoncoreontologies.org/ont00001819 -->

    <owl:ObjectProperty rdf:about="https://www.commoncoreontologies.org/ont00001819"/>
    


    <!-- https://www.commoncoreontologies.org/ont00001841 -->

    <owl:ObjectProperty rdf:about="https://www.commoncoreontologies.org/ont00001841"/>
    


    <!-- https://www.commoncoreontologies.org/ont00001899 -->

    <owl:ObjectProperty rdf:about="https://www.commoncoreontologies.org/ont00001899"/>
    


    <!-- https://www.commoncoreontologies.org/ont00001920 -->

    <owl:ObjectProperty rdf:about="https://www.commoncoreontologies.org/ont00001920"/>
    


    <!-- https://www.commoncoreontologies.org/ont00001925 -->

    <owl:ObjectProperty rdf:about="https://www.commoncoreontologies.org/ont00001925"/>
    


    <!-- https://www.commoncoreontologies.org/ont00001933 -->

    <owl:ObjectProperty rdf:about="https://www.commoncoreontologies.org/ont00001933"/>
    


    <!-- https://www.commoncoreontologies.org/ont00001942 -->

    <owl:ObjectProperty rdf:about="https://www.commoncoreontologies.org/ont00001942"/>
    


    <!-- https://www.commoncoreontologies.org/ont00001959 -->

    <owl:ObjectProperty rdf:about="https://www.commoncoreontologies.org/ont00001959">
        <owl:inverseOf rdf:resource="https://www.commoncoreontologies.org/ont00001970"/>
        <rdfs:domain rdf:resource="http://purl.obolibrary.org/obo/BFO_0000015"/>
        <rdfs:range rdf:resource="http://purl.obolibrary.org/obo/BFO_0000015"/>
        <owl:propertyChainAxiom rdf:parseType="Collection">
            <rdf:Description rdf:about="https://www.commoncoreontologies.org/ont00001803"/>
            <rdf:Description rdf:about="http://purl.obolibrary.org/obo/BFO_0000057"/>
            <rdf:Description rdf:about="http://purl.obolibrary.org/obo/BFO_0000054"/>
        </owl:propertyChainAxiom>
        <skos:definition xml:lang="en">x inhibits y iff x and y are non-identical Processes, d is a Decrease of Realizable Entity, and x is_cause_of d, and r is a Realizable Entity, and d has_participant r, and r realized_in y.</skos:definition>
        <rdfs:comment xml:lang="en">This term has a super property chain that caused a logical inconsistency when &apos;inhibits&apos; was asserted as a subproperty of &apos;is cause of&apos;. Discussion during the IEEE Cyber Ontology Working Group meeting April 17, 2024 identified multiple proposed changes to &apos;inhibits&apos; and its inverse &apos;inhibited by&apos;. Possible resolutions include:

1. Delete the super property chain.
2. Alter the super property chain.
3. Move &apos;inhibits&apos; so it is no longer a subproperty of &apos;is caused by&apos;.

Doubts were raised regarding the utility of the super property chain.

Regardless of possible changes to the super property chain, doubts were raised as to whether &apos;inhibits&apos; should be a subproperty of &apos;is caused by&apos;. Two possible locations to move &apos;inhibits&apos; to were proposed. First, &apos;inhibits&apos; might be a subproperty of &apos;disrupts&apos; as its current definition aligns with the second type of &quot;disruption&quot; described. Second, &apos;inhibits&apos; might be better asserted under owl:topObjectProperty with its definition and range altered. It was noted that doing so may require deprecating the current IRI.

The group agreed that the immediate solution is to leave the definitions and super property axioms as-is and move &apos;inhibits&apos; and &apos;inhibited by&apos; under owl:topObjectProperty.

It is also suggested that these properties be brought to the CCO WG to address since their scope is larger than just the cyber domain.</rdfs:comment>
        <rdfs:label xml:lang="en">inhibits</rdfs:label>
        <cco2:ont00001760 rdf:datatype="http://www.w3.org/2001/XMLSchema#anyURI">http://www.ontologyrepository.com/CommonCoreOntologies/Domain/CyberOntology</cco2:ont00001760>
    </owl:ObjectProperty>
    


    <!-- https://www.commoncoreontologies.org/ont00001962 -->

    <owl:ObjectProperty rdf:about="https://www.commoncoreontologies.org/ont00001962"/>
    


    <!-- https://www.commoncoreontologies.org/ont00001970 -->

    <owl:ObjectProperty rdf:about="https://www.commoncoreontologies.org/ont00001970">
        <owl:propertyChainAxiom rdf:parseType="Collection">
            <rdf:Description rdf:about="http://purl.obolibrary.org/obo/BFO_0000055"/>
            <rdf:Description rdf:about="http://purl.obolibrary.org/obo/BFO_0000056"/>
            <rdf:Description rdf:about="https://www.commoncoreontologies.org/ont00001819"/>
        </owl:propertyChainAxiom>
        <skos:definition xml:lang="en">y inhibited_by x iff x and y are non-identical Processes, d is a Decrease of Realizable Entity, and x is_cause_of d, and r is a Realizable Entity, and d has_participant r, and r realized_in y.</skos:definition>
        <rdfs:comment xml:lang="en">See comment on &apos;inhibits&apos; for an update on the status of this object property.</rdfs:comment>
        <rdfs:label xml:lang="en">inhibited by</rdfs:label>
        <cco2:ont00001760 rdf:datatype="http://www.w3.org/2001/XMLSchema#anyURI">http://www.ontologyrepository.com/CommonCoreOntologies/Domain/CyberOntology</cco2:ont00001760>
    </owl:ObjectProperty>
    


    <!-- 
    ///////////////////////////////////////////////////////////////////////////////////////
    //
    // Classes
    //
    ///////////////////////////////////////////////////////////////////////////////////////
     -->

    


    <!-- http://purl.obolibrary.org/obo/BFO_0000015 -->

    <owl:Class rdf:about="http://purl.obolibrary.org/obo/BFO_0000015"/>
    


    <!-- http://purl.obolibrary.org/obo/BFO_0000023 -->

    <owl:Class rdf:about="http://purl.obolibrary.org/obo/BFO_0000023"/>
    


    <!-- http://purl.obolibrary.org/obo/BFO_0000027 -->

    <owl:Class rdf:about="http://purl.obolibrary.org/obo/BFO_0000027"/>
    


    <!-- http://purl.obolibrary.org/obo/BFO_0000040 -->

    <owl:Class rdf:about="http://purl.obolibrary.org/obo/BFO_0000040"/>
    


    <!-- http://www.ontologyrepository.com/CommonCoreOntologies/AccessReader -->

    <owl:Class rdf:about="http://www.ontologyrepository.com/CommonCoreOntologies/AccessReader">
        <rdfs:subClassOf rdf:resource="https://www.commoncoreontologies.org/ont00000117"/>
        <skos:definition xml:lang="en">An Information Processing Artifact that is designed to process whether a prospective user has the creditials to access some resource.</skos:definition>
        <rdfs:comment xml:lang="en">Access may be to a physical resource (e.g., a room) or to a virtual resource.</rdfs:comment>
        <rdfs:label xml:lang="en">Access Reader</rdfs:label>
        <cco2:ont00001754>https://en.wikipedia.org/wiki/Card_reader#Access_control_card_reader</cco2:ont00001754>
        <cco2:ont00001760 rdf:datatype="http://www.w3.org/2001/XMLSchema#anyURI">http://www.ontologyrepository.com/CommonCoreOntologies/Domain/CyberOntology</cco2:ont00001760>
    </owl:Class>
    


    <!-- http://www.ontologyrepository.com/CommonCoreOntologies/ActOfArtifactCreation -->

    <owl:Class rdf:about="http://www.ontologyrepository.com/CommonCoreOntologies/ActOfArtifactCreation">
        <rdfs:subClassOf rdf:resource="https://www.commoncoreontologies.org/ont00000908"/>
        <skos:definition xml:lang="en">An Act of Artifact Processing that consists of bringing a new Artifact into existence.</skos:definition>
        <rdfs:label xml:lang="en">Act of Artifact Creation</rdfs:label>
        <cco2:ont00001760 rdf:datatype="http://www.w3.org/2001/XMLSchema#anyURI">http://www.ontologyrepository.com/CommonCoreOntologies/Domain/CyberOntology</cco2:ont00001760>
    </owl:Class>
    


    <!-- http://www.ontologyrepository.com/CommonCoreOntologies/ActOfArtifactDestruction -->

    <owl:Class rdf:about="http://www.ontologyrepository.com/CommonCoreOntologies/ActOfArtifactDestruction">
        <rdfs:subClassOf rdf:resource="https://www.commoncoreontologies.org/ont00000908"/>
        <skos:definition xml:lang="en">An Act of Artifact Processing that consists of destroying some Artifact.</skos:definition>
        <rdfs:label xml:lang="en">Act of Artifact Destruction</rdfs:label>
        <cco2:ont00001760 rdf:datatype="http://www.w3.org/2001/XMLSchema#anyURI">http://www.ontologyrepository.com/CommonCoreOntologies/Domain/CyberOntology</cco2:ont00001760>
    </owl:Class>
    


    <!-- http://www.ontologyrepository.com/CommonCoreOntologies/ActOfComputerProgramCreation -->

    <owl:Class rdf:about="http://www.ontologyrepository.com/CommonCoreOntologies/ActOfComputerProgramCreation">
        <rdfs:subClassOf rdf:resource="http://www.ontologyrepository.com/CommonCoreOntologies/ActOfArtifactCreation"/>
        <skos:definition xml:lang="en">An Intentional Act wherin some Agent develops a Computer Program.</skos:definition>
        <rdfs:label xml:lang="en">Act Of Computer Software Creation</rdfs:label>
        <cco2:ont00001760 rdf:datatype="http://www.w3.org/2001/XMLSchema#anyURI">http://www.ontologyrepository.com/CommonCoreOntologies/Domain/CyberOntology</cco2:ont00001760>
    </owl:Class>
    


    <!-- http://www.ontologyrepository.com/CommonCoreOntologies/ActOfCyberExploitation -->

    <owl:Class rdf:about="http://www.ontologyrepository.com/CommonCoreOntologies/ActOfCyberExploitation">
        <rdfs:subClassOf rdf:resource="https://www.commoncoreontologies.org/ont00000228"/>
        <skos:definition xml:lang="en">An Intentional Act that is part of a Cyber Attack wherein a Cyber Attacker uses a Cyber Exploit Artifact to realize a Cyber Vulnerability.</skos:definition>
        <rdfs:label xml:lang="en">Act of Cyber Exploitation</rdfs:label>
        <cco2:ont00001760 rdf:datatype="http://www.w3.org/2001/XMLSchema#anyURI">http://www.ontologyrepository.com/CommonCoreOntologies/Domain/CyberOntology</cco2:ont00001760>
    </owl:Class>
    


    <!-- http://www.ontologyrepository.com/CommonCoreOntologies/ActOfCyberThreatDetection -->

    <owl:Class rdf:about="http://www.ontologyrepository.com/CommonCoreOntologies/ActOfCyberThreatDetection">
        <rdfs:subClassOf rdf:resource="https://www.commoncoreontologies.org/ont00001251"/>
        <skos:definition xml:lang="en">An Act of Intelligence Gathering wherein an Agent attempts to detect cyber threats.</skos:definition>
        <rdfs:label xml:lang="en">Act Of Cyber Threat Detection</rdfs:label>
        <cco2:ont00001760 rdf:datatype="http://www.w3.org/2001/XMLSchema#anyURI">http://www.ontologyrepository.com/CommonCoreOntologies/Domain/CyberOntology</cco2:ont00001760>
    </owl:Class>
    


    <!-- http://www.ontologyrepository.com/CommonCoreOntologies/ActOfCyberThreatMitigation -->

    <owl:Class rdf:about="http://www.ontologyrepository.com/CommonCoreOntologies/ActOfCyberThreatMitigation">
        <owl:equivalentClass>
            <owl:Class>
                <owl:intersectionOf rdf:parseType="Collection">
                    <rdf:Description rdf:about="http://www.ontologyrepository.com/CommonCoreOntologies/ActOfInhibiting"/>
                    <owl:Restriction>
                        <owl:onProperty rdf:resource="https://www.commoncoreontologies.org/ont00001959"/>
                        <owl:someValuesFrom rdf:resource="http://www.ontologyrepository.com/CommonCoreOntologies/CyberAttack"/>
                    </owl:Restriction>
                </owl:intersectionOf>
            </owl:Class>
        </owl:equivalentClass>
        <rdfs:subClassOf rdf:resource="http://www.ontologyrepository.com/CommonCoreOntologies/ActOfInhibiting"/>
        <skos:definition xml:lang="en">An Intentional Act which inhibits a Cyber Attack.</skos:definition>
        <rdfs:label xml:lang="en">Act of Cyber Threat Mitigation</rdfs:label>
        <cco2:ont00001760 rdf:datatype="http://www.w3.org/2001/XMLSchema#anyURI">http://www.ontologyrepository.com/CommonCoreOntologies/Domain/CyberOntology</cco2:ont00001760>
    </owl:Class>
    


    <!-- http://www.ontologyrepository.com/CommonCoreOntologies/ActOfEvasion -->

    <owl:Class rdf:about="http://www.ontologyrepository.com/CommonCoreOntologies/ActOfEvasion">
        <rdfs:subClassOf rdf:resource="https://www.commoncoreontologies.org/ont00000228"/>
        <skos:definition xml:lang="en">An Intentional Act of attempting to avoid an entity.</skos:definition>
        <rdfs:label xml:lang="en">Act of Evasion</rdfs:label>
        <cco2:ont00001760 rdf:datatype="http://www.w3.org/2001/XMLSchema#anyURI">http://www.ontologyrepository.com/CommonCoreOntologies/Domain/CyberOntology</cco2:ont00001760>
    </owl:Class>
    


    <!-- http://www.ontologyrepository.com/CommonCoreOntologies/ActOfExperimentation -->

    <owl:Class rdf:about="http://www.ontologyrepository.com/CommonCoreOntologies/ActOfExperimentation">
        <rdfs:subClassOf rdf:resource="https://www.commoncoreontologies.org/ont00000228"/>
        <skos:definition xml:lang="en">An Intentional Act wherein an Agent tests new ideas, methods, or activities, in an attempt to discover new information or knowledge.</skos:definition>
        <rdfs:label xml:lang="en">Act of Experimentation</rdfs:label>
        <cco2:ont00001754 xml:lang="en">https://www.lexico.com/en/definition/experimentation</cco2:ont00001754>
        <cco2:ont00001760 rdf:datatype="http://www.w3.org/2001/XMLSchema#anyURI">http://www.ontologyrepository.com/CommonCoreOntologies/Domain/CyberOntology</cco2:ont00001760>
    </owl:Class>
    


    <!-- http://www.ontologyrepository.com/CommonCoreOntologies/ActOfInhibiting -->

    <owl:Class rdf:about="http://www.ontologyrepository.com/CommonCoreOntologies/ActOfInhibiting">
        <owl:equivalentClass>
            <owl:Class>
                <owl:intersectionOf rdf:parseType="Collection">
                    <rdf:Description rdf:about="https://www.commoncoreontologies.org/ont00000228"/>
                    <owl:Restriction>
                        <owl:onProperty rdf:resource="https://www.commoncoreontologies.org/ont00001959"/>
                        <owl:someValuesFrom rdf:resource="http://purl.obolibrary.org/obo/BFO_0000015"/>
                    </owl:Restriction>
                </owl:intersectionOf>
            </owl:Class>
        </owl:equivalentClass>
        <rdfs:subClassOf rdf:resource="https://www.commoncoreontologies.org/ont00000228"/>
        <skos:altLabel xml:lang="en">Act of Mitigation</skos:altLabel>
        <skos:definition xml:lang="en">An Intentional Act that inhibits some Process.</skos:definition>
        <rdfs:label xml:lang="en">Act of Inhibiting</rdfs:label>
        <cco2:ont00001760 rdf:datatype="http://www.w3.org/2001/XMLSchema#anyURI">http://www.ontologyrepository.com/CommonCoreOntologies/Domain/CyberOntology</cco2:ont00001760>
    </owl:Class>
    


    <!-- http://www.ontologyrepository.com/CommonCoreOntologies/ActOfSearching -->

    <owl:Class rdf:about="http://www.ontologyrepository.com/CommonCoreOntologies/ActOfSearching">
        <rdfs:subClassOf rdf:resource="https://www.commoncoreontologies.org/ont00000228"/>
        <skos:definition xml:lang="en">An Intentional Act of trying to find an entity.</skos:definition>
        <rdfs:label xml:lang="en">Act of Searching</rdfs:label>
        <cco2:ont00001760 rdf:datatype="http://www.w3.org/2001/XMLSchema#anyURI">http://www.ontologyrepository.com/CommonCoreOntologies/Domain/CyberOntology</cco2:ont00001760>
    </owl:Class>
    


    <!-- http://www.ontologyrepository.com/CommonCoreOntologies/Adware -->

    <owl:Class rdf:about="http://www.ontologyrepository.com/CommonCoreOntologies/Adware">
        <rdfs:subClassOf rdf:resource="http://www.ontologyrepository.com/CommonCoreOntologies/ComputerProgram"/>
        <skos:definition xml:lang="en">A Computer Program that is designed to generate revenue for its developer by automatically generating online advertisements in the user interface of the software or on a screen presented to the user during the installation process.</skos:definition>
        <rdfs:label xml:lang="en">Adware</rdfs:label>
        <cco2:ont00001754>https://en.wikipedia.org/wiki/Adware</cco2:ont00001754>
        <cco2:ont00001760 rdf:datatype="http://www.w3.org/2001/XMLSchema#anyURI">http://www.ontologyrepository.com/CommonCoreOntologies/Domain/CyberOntology</cco2:ont00001760>
    </owl:Class>
    


    <!-- http://www.ontologyrepository.com/CommonCoreOntologies/AggregationFunction -->

    <owl:Class rdf:about="http://www.ontologyrepository.com/CommonCoreOntologies/AggregationFunction">
        <rdfs:subClassOf rdf:resource="https://www.commoncoreontologies.org/ont00000653"/>
        <skos:definition xml:lang="en">An Algorithm in which the values of multiple rows are grouped together to form a single value of more significant meaning.</skos:definition>
        <rdfs:label xml:lang="en">Aggregation Function</rdfs:label>
        <cco2:ont00001754>https://en.wikipedia.org/wiki/Aggregate_function</cco2:ont00001754>
        <cco2:ont00001760 rdf:datatype="http://www.w3.org/2001/XMLSchema#anyURI">http://www.ontologyrepository.com/CommonCoreOntologies/Domain/CyberOntology</cco2:ont00001760>
    </owl:Class>
    


    <!-- http://www.ontologyrepository.com/CommonCoreOntologies/AggregationProcess -->

    <owl:Class rdf:about="http://www.ontologyrepository.com/CommonCoreOntologies/AggregationProcess">
        <rdfs:subClassOf rdf:resource="http://www.ontologyrepository.com/CommonCoreOntologies/ComputerProgramExecution"/>
        <skos:definition xml:lang="en">A Computer Program Execution in which the values of multiple rows are grouped together to form a single value of more significant meaning.</skos:definition>
        <rdfs:label xml:lang="en">Aggregation Process</rdfs:label>
        <cco2:ont00001760 rdf:datatype="http://www.w3.org/2001/XMLSchema#anyURI">http://www.ontologyrepository.com/CommonCoreOntologies/Domain/CyberOntology</cco2:ont00001760>
    </owl:Class>
    


    <!-- http://www.ontologyrepository.com/CommonCoreOntologies/AnimationSoftwareApplication -->

    <owl:Class rdf:about="http://www.ontologyrepository.com/CommonCoreOntologies/AnimationSoftwareApplication">
        <rdfs:subClassOf rdf:resource="http://www.ontologyrepository.com/CommonCoreOntologies/MultimediaSoftwareApplication"/>
        <skos:definition xml:lang="en">A Multimedia Software Application that is designed to enable a user to create and edit animations.</skos:definition>
        <rdfs:label xml:lang="en">Animation Software Application</rdfs:label>
        <cco2:ont00001760 rdf:datatype="http://www.w3.org/2001/XMLSchema#anyURI">http://www.ontologyrepository.com/CommonCoreOntologies/Domain/CyberOntology</cco2:ont00001760>
    </owl:Class>
    


    <!-- http://www.ontologyrepository.com/CommonCoreOntologies/AnonymityNetwork -->

    <owl:Class rdf:about="http://www.ontologyrepository.com/CommonCoreOntologies/AnonymityNetwork">
        <rdfs:subClassOf rdf:resource="http://www.ontologyrepository.com/CommonCoreOntologies/DarkNetwork"/>
        <skos:definition xml:lang="en">A Dark Network that enables users to access the Internet while blocking any tracking or tracing of their identity.</skos:definition>
        <rdfs:label xml:lang="en">Anonymity Network</rdfs:label>
        <cco2:ont00001754>https://www.techopedia.com/definition/25187/anonymity-network</cco2:ont00001754>
        <cco2:ont00001760 rdf:datatype="http://www.w3.org/2001/XMLSchema#anyURI">http://www.ontologyrepository.com/CommonCoreOntologies/Domain/CyberOntology</cco2:ont00001760>
    </owl:Class>
    


    <!-- http://www.ontologyrepository.com/CommonCoreOntologies/Anonymization -->

    <owl:Class rdf:about="http://www.ontologyrepository.com/CommonCoreOntologies/Anonymization">
        <rdfs:subClassOf rdf:resource="http://www.ontologyrepository.com/CommonCoreOntologies/ComputerProgramExecution"/>
        <skos:definition xml:lang="en">A Computer Program Execution that encrypts or removes personally identifiable information from data sets in order to maintain the anonymity of the people described by the data.</skos:definition>
        <rdfs:label xml:lang="en">Anonymization</rdfs:label>
        <cco2:ont00001754 rdf:datatype="http://www.w3.org/2001/XMLSchema#anyURI">https://en.wikipedia.org/wiki/Data_anonymization</cco2:ont00001754>
        <cco2:ont00001760 rdf:datatype="http://www.w3.org/2001/XMLSchema#anyURI">http://www.ontologyrepository.com/CommonCoreOntologies/Domain/CyberOntology</cco2:ont00001760>
    </owl:Class>
    


    <!-- http://www.ontologyrepository.com/CommonCoreOntologies/Anonymizer -->

    <owl:Class rdf:about="http://www.ontologyrepository.com/CommonCoreOntologies/Anonymizer">
        <rdfs:subClassOf rdf:resource="http://www.ontologyrepository.com/CommonCoreOntologies/ApplicationSoftware"/>
        <skos:definition xml:lang="en">Application Software that is designed to conceal the identity of some client from some Computer Network.</skos:definition>
        <rdfs:label xml:lang="en">Anonymizer</rdfs:label>
        <cco2:ont00001760 rdf:datatype="http://www.w3.org/2001/XMLSchema#anyURI">http://www.ontologyrepository.com/CommonCoreOntologies/Domain/CyberOntology</cco2:ont00001760>
    </owl:Class>
    


    <!-- http://www.ontologyrepository.com/CommonCoreOntologies/AntivirusApplication -->

    <owl:Class rdf:about="http://www.ontologyrepository.com/CommonCoreOntologies/AntivirusApplication">
        <rdfs:subClassOf rdf:resource="http://www.ontologyrepository.com/CommonCoreOntologies/UtilityProgram"/>
        <skos:altLabel xml:lang="en">Anti-malware Software</skos:altLabel>
        <skos:definition xml:lang="en">A Utility Program that is designed to prevent, detect, and remove malicious software.</skos:definition>
        <rdfs:label xml:lang="en">Antivirus Application</rdfs:label>
        <cco2:ont00001754>https://en.wikipedia.org/wiki/Antivirus_software</cco2:ont00001754>
        <cco2:ont00001760 rdf:datatype="http://www.w3.org/2001/XMLSchema#anyURI">http://www.ontologyrepository.com/CommonCoreOntologies/Domain/CyberOntology</cco2:ont00001760>
    </owl:Class>
    


    <!-- http://www.ontologyrepository.com/CommonCoreOntologies/ApplicationBinaryInterface -->

    <owl:Class rdf:about="http://www.ontologyrepository.com/CommonCoreOntologies/ApplicationBinaryInterface">
        <rdfs:subClassOf rdf:resource="https://www.commoncoreontologies.org/ont00000319"/>
        <skos:altLabel xml:lang="en">ABI</skos:altLabel>
        <skos:definition xml:lang="en">An Artifact Design that is a specification for how to enable a Computer Library and/or Operating System to interact with a Computer Program.</skos:definition>
        <rdfs:label xml:lang="en">Application Binary Interface</rdfs:label>
        <cco2:ont00001754>https://en.wikipedia.org/wiki/Application_binary_interface</cco2:ont00001754>
        <cco2:ont00001760 rdf:datatype="http://www.w3.org/2001/XMLSchema#anyURI">http://www.ontologyrepository.com/CommonCoreOntologies/Domain/CyberOntology</cco2:ont00001760>
    </owl:Class>
    


    <!-- http://www.ontologyrepository.com/CommonCoreOntologies/ApplicationManager -->

    <owl:Class rdf:about="http://www.ontologyrepository.com/CommonCoreOntologies/ApplicationManager">
        <rdfs:subClassOf rdf:resource="http://www.ontologyrepository.com/CommonCoreOntologies/UtilityProgram"/>
        <skos:definition xml:lang="en">A Utility Program that is designed to oversee the installation, patching, updating, and accessibility of software applications.</skos:definition>
        <rdfs:label xml:lang="en">Application Manager</rdfs:label>
        <cco2:ont00001760 rdf:datatype="http://www.w3.org/2001/XMLSchema#anyURI">http://www.ontologyrepository.com/CommonCoreOntologies/Domain/CyberOntology</cco2:ont00001760>
    </owl:Class>
    


    <!-- http://www.ontologyrepository.com/CommonCoreOntologies/ApplicationProgrammingInterface -->

    <owl:Class rdf:about="http://www.ontologyrepository.com/CommonCoreOntologies/ApplicationProgrammingInterface">
        <rdfs:subClassOf rdf:resource="https://www.commoncoreontologies.org/ont00000798"/>
        <skos:altLabel xml:lang="en">API</skos:altLabel>
        <rdfs:label xml:lang="en">Application Programming Interface</rdfs:label>
        <cco2:ont00001754>https://en.wikipedia.org/wiki/Application_programming_interface</cco2:ont00001754>
        <cco2:ont00001760 rdf:datatype="http://www.w3.org/2001/XMLSchema#anyURI">http://www.ontologyrepository.com/CommonCoreOntologies/Domain/CyberOntology</cco2:ont00001760>
    </owl:Class>
    


    <!-- http://www.ontologyrepository.com/CommonCoreOntologies/ApplicationSoftware -->

    <owl:Class rdf:about="http://www.ontologyrepository.com/CommonCoreOntologies/ApplicationSoftware">
        <rdfs:subClassOf rdf:resource="http://www.ontologyrepository.com/CommonCoreOntologies/ComputerProgram"/>
        <skos:altLabel xml:lang="en">App</skos:altLabel>
        <skos:altLabel xml:lang="en">Application</skos:altLabel>
        <skos:altLabel xml:lang="en">Application Program</skos:altLabel>
        <skos:altLabel xml:lang="en">Software</skos:altLabel>
        <skos:altLabel xml:lang="en">Software Application</skos:altLabel>
        <skos:altLabel xml:lang="en">Software Program</skos:altLabel>
        <skos:definition xml:lang="en">A Computer Prgoram that is designed to execute a group of coordinated Computer Functions for the benefit of a user.</skos:definition>
        <rdfs:label xml:lang="en">Application Software</rdfs:label>
        <cco2:ont00001754>https://en.wikipedia.org/wiki/Application_software</cco2:ont00001754>
        <cco2:ont00001760 rdf:datatype="http://www.w3.org/2001/XMLSchema#anyURI">http://www.ontologyrepository.com/CommonCoreOntologies/Domain/CyberOntology</cco2:ont00001760>
    </owl:Class>
    


    <!-- http://www.ontologyrepository.com/CommonCoreOntologies/Array -->

    <owl:Class rdf:about="http://www.ontologyrepository.com/CommonCoreOntologies/Array">
        <rdfs:subClassOf rdf:resource="https://www.commoncoreontologies.org/ont00000798"/>
        <skos:definition xml:lang="en">An Information Bearing Artifact that is the bearer of a finite ordered list of Information Content Entities.</skos:definition>
        <rdfs:label xml:lang="en">Array</rdfs:label>
        <cco2:ont00001760 rdf:datatype="http://www.w3.org/2001/XMLSchema#anyURI">http://www.ontologyrepository.com/CommonCoreOntologies/Domain/CyberOntology</cco2:ont00001760>
    </owl:Class>
    


    <!-- http://www.ontologyrepository.com/CommonCoreOntologies/AssemblyLanguage -->

    <owl:Class rdf:about="http://www.ontologyrepository.com/CommonCoreOntologies/AssemblyLanguage">
        <rdfs:subClassOf rdf:resource="http://www.ontologyrepository.com/CommonCoreOntologies/LowLevelProgrammingLanguage"/>
        <skos:definition xml:lang="en">A Programming Language that prescribes a canonical form of communicating instructions which have been translated from a High-Level Programming Language and which can be translated into some Machine Language.</skos:definition>
        <rdfs:label xml:lang="en">Assembly Language</rdfs:label>
        <cco2:ont00001760 rdf:datatype="http://www.w3.org/2001/XMLSchema#anyURI">http://www.ontologyrepository.com/CommonCoreOntologies/Domain/CyberOntology</cco2:ont00001760>
    </owl:Class>
    


    <!-- http://www.ontologyrepository.com/CommonCoreOntologies/AudioEditingSoftwareApplication -->

    <owl:Class rdf:about="http://www.ontologyrepository.com/CommonCoreOntologies/AudioEditingSoftwareApplication">
        <rdfs:subClassOf rdf:resource="http://www.ontologyrepository.com/CommonCoreOntologies/MultimediaSoftwareApplication"/>
        <skos:definition xml:lang="en">A Multimedia Software Application that is designed to enable a user to create and edit audio files.</skos:definition>
        <rdfs:label xml:lang="en">Audio Editing Software Application</rdfs:label>
        <cco2:ont00001760 rdf:datatype="http://www.w3.org/2001/XMLSchema#anyURI">http://www.ontologyrepository.com/CommonCoreOntologies/Domain/CyberOntology</cco2:ont00001760>
    </owl:Class>
    


    <!-- http://www.ontologyrepository.com/CommonCoreOntologies/Authentication -->

    <owl:Class rdf:about="http://www.ontologyrepository.com/CommonCoreOntologies/Authentication">
        <rdfs:subClassOf rdf:resource="http://www.ontologyrepository.com/CommonCoreOntologies/ComputerProgramExecution"/>
        <skos:definition xml:lang="en">A Computer Program Execution in which the identity of a user is verified.</skos:definition>
        <rdfs:label xml:lang="en">Authentication</rdfs:label>
        <cco2:ont00001754 rdf:datatype="http://www.w3.org/2000/01/rdf-schema#Literal">https://en.wikipedia.org/wiki/Authentication</cco2:ont00001754>
        <cco2:ont00001760 rdf:datatype="http://www.w3.org/2001/XMLSchema#anyURI">http://www.ontologyrepository.com/CommonCoreOntologies/Domain/CyberOntology</cco2:ont00001760>
    </owl:Class>
    


    <!-- http://www.ontologyrepository.com/CommonCoreOntologies/Authorization -->

    <owl:Class rdf:about="http://www.ontologyrepository.com/CommonCoreOntologies/Authorization">
        <rdfs:subClassOf rdf:resource="http://www.ontologyrepository.com/CommonCoreOntologies/ComputerProgramExecution"/>
        <skos:altLabel xml:lang="en">Access Control</skos:altLabel>
        <skos:definition xml:lang="en">A Computer Program Execution that bestows a user account with File Permissions.</skos:definition>
        <rdfs:label xml:lang="en">Authorization</rdfs:label>
        <cco2:ont00001754 rdf:datatype="http://www.w3.org/2001/XMLSchema#anyURI">https://www.okta.com/identity-101/authentication-vs-authorization/</cco2:ont00001754>
        <cco2:ont00001760 rdf:datatype="http://www.w3.org/2001/XMLSchema#anyURI">http://www.ontologyrepository.com/CommonCoreOntologies/Domain/CyberOntology</cco2:ont00001760>
    </owl:Class>
    


    <!-- http://www.ontologyrepository.com/CommonCoreOntologies/AutomatedTellerMachine -->

    <owl:Class rdf:about="http://www.ontologyrepository.com/CommonCoreOntologies/AutomatedTellerMachine">
        <rdfs:subClassOf rdf:resource="https://www.commoncoreontologies.org/ont00000690"/>
        <skos:altLabel xml:lang="en">ATM</skos:altLabel>
        <skos:definition xml:lang="en">A Telecommunication Instrument which is designed to enable the customers of a financial institution to perform financial transactions, particularly cash withdrawal, without the need for a human cashier, clerk, or bank teller.</skos:definition>
        <rdfs:label xml:lang="en">Automated Teller Machine</rdfs:label>
        <cco2:ont00001754>https://en.wikipedia.org/wiki/Automated_teller_machine</cco2:ont00001754>
        <cco2:ont00001760 rdf:datatype="http://www.w3.org/2001/XMLSchema#anyURI">http://www.ontologyrepository.com/CommonCoreOntologies/Domain/CyberOntology</cco2:ont00001760>
    </owl:Class>
    


    <!-- http://www.ontologyrepository.com/CommonCoreOntologies/BackdoorProgram -->

    <owl:Class rdf:about="http://www.ontologyrepository.com/CommonCoreOntologies/BackdoorProgram">
        <rdfs:subClassOf rdf:resource="http://www.ontologyrepository.com/CommonCoreOntologies/Malware"/>
        <skos:definition xml:lang="en">Malware that is designed to bypass normal authentication or encryption in a computer system in order to secure remote access to that system.</skos:definition>
        <rdfs:label xml:lang="en">Backdoor Program</rdfs:label>
        <cco2:ont00001754>https://en.wikipedia.org/wiki/Backdoor_(computing)</cco2:ont00001754>
        <cco2:ont00001760 rdf:datatype="http://www.w3.org/2001/XMLSchema#anyURI">http://www.ontologyrepository.com/CommonCoreOntologies/Domain/CyberOntology</cco2:ont00001760>
    </owl:Class>
    


    <!-- http://www.ontologyrepository.com/CommonCoreOntologies/BackupFile -->

    <owl:Class rdf:about="http://www.ontologyrepository.com/CommonCoreOntologies/BackupFile">
        <rdfs:subClassOf rdf:resource="http://www.ontologyrepository.com/CommonCoreOntologies/DigitalFile"/>
        <skos:definition xml:lang="en">A Digital File that that is designed to preserve the content of the original digital file in the case of destruction of the original.</skos:definition>
        <rdfs:label xml:lang="en">Backup File</rdfs:label>
        <cco2:ont00001760 rdf:datatype="http://www.w3.org/2001/XMLSchema#anyURI">http://www.ontologyrepository.com/CommonCoreOntologies/Domain/CyberOntology</cco2:ont00001760>
    </owl:Class>
    


    <!-- http://www.ontologyrepository.com/CommonCoreOntologies/BackupSoftware -->

    <owl:Class rdf:about="http://www.ontologyrepository.com/CommonCoreOntologies/BackupSoftware">
        <rdfs:subClassOf rdf:resource="http://www.ontologyrepository.com/CommonCoreOntologies/UtilityProgram"/>
        <skos:definition xml:lang="en">A Utility Program that is designed to supplementary, exact copies of Digital Files, Databases, or of all the data on a Computer, which can be accessed later to restore the original contents in the event of data loss.</skos:definition>
        <rdfs:label xml:lang="en">Backup Software</rdfs:label>
        <cco2:ont00001754>https://en.wikipedia.org/wiki/Backup_software</cco2:ont00001754>
        <cco2:ont00001760 rdf:datatype="http://www.w3.org/2001/XMLSchema#anyURI">http://www.ontologyrepository.com/CommonCoreOntologies/Domain/CyberOntology</cco2:ont00001760>
    </owl:Class>
    


    <!-- http://www.ontologyrepository.com/CommonCoreOntologies/BasebandBandwidthMeasurement -->

    <owl:Class rdf:about="http://www.ontologyrepository.com/CommonCoreOntologies/BasebandBandwidthMeasurement">
        <rdfs:subClassOf rdf:resource="http://www.ontologyrepository.com/CommonCoreOntologies/SignalBandwidthMeasurement"/>
        <skos:definition xml:lang="en">A Signal Bandwidth Measurement that is a measurement of the range of continuous Frequencies between zero and some upper cutoff Frequency.</skos:definition>
        <rdfs:label xml:lang="en">Baseband Bandwidth Measurement</rdfs:label>
        <cco2:ont00001760 rdf:datatype="http://www.w3.org/2001/XMLSchema#anyURI">http://www.ontologyrepository.com/CommonCoreOntologies/Domain/CyberOntology</cco2:ont00001760>
    </owl:Class>
    


    <!-- http://www.ontologyrepository.com/CommonCoreOntologies/BattlefieldSimulator -->

    <owl:Class rdf:about="http://www.ontologyrepository.com/CommonCoreOntologies/BattlefieldSimulator">
        <rdfs:subClassOf rdf:resource="http://www.ontologyrepository.com/CommonCoreOntologies/SimulationSoftware"/>
        <skos:definition xml:lang="en">Simulation Software that is designed to enable a user to model a battle.</skos:definition>
        <rdfs:label xml:lang="en">Battlefield Simulator</rdfs:label>
        <cco2:ont00001760 rdf:datatype="http://www.w3.org/2001/XMLSchema#anyURI">http://www.ontologyrepository.com/CommonCoreOntologies/Domain/CyberOntology</cco2:ont00001760>
    </owl:Class>
    


    <!-- http://www.ontologyrepository.com/CommonCoreOntologies/Bit -->

    <owl:Class rdf:about="http://www.ontologyrepository.com/CommonCoreOntologies/Bit">
        <rdfs:subClassOf rdf:resource="https://www.commoncoreontologies.org/ont00000798"/>
        <skos:definition xml:lang="en">An Information Bearing Artifact that is the bearer of one of two values (exclusive) which can be concretized within a two-state device.</skos:definition>
        <skos:example>1, 0</skos:example>
        <skos:example>On, Off</skos:example>
        <skos:example>True, False</skos:example>
        <rdfs:label xml:lang="en">Bit</rdfs:label>
        <cco2:ont00001754>https://en.wikipedia.org/wiki/Bit</cco2:ont00001754>
        <cco2:ont00001760 rdf:datatype="http://www.w3.org/2001/XMLSchema#anyURI">http://www.ontologyrepository.com/CommonCoreOntologies/Domain/CyberOntology</cco2:ont00001760>
    </owl:Class>
    


    <!-- http://www.ontologyrepository.com/CommonCoreOntologies/Blog -->

    <owl:Class rdf:about="http://www.ontologyrepository.com/CommonCoreOntologies/Blog">
        <rdfs:subClassOf rdf:resource="http://www.ontologyrepository.com/CommonCoreOntologies/Website"/>
        <skos:definition xml:lang="en">A Website that consists of discrete, often informal diary-style entries (&quot;posts&quot;).</skos:definition>
        <rdfs:label xml:lang="en">Blog</rdfs:label>
        <cco2:ont00001760 rdf:datatype="http://www.w3.org/2001/XMLSchema#anyURI">http://www.ontologyrepository.com/CommonCoreOntologies/Domain/CyberOntology</cco2:ont00001760>
    </owl:Class>
    


    <!-- http://www.ontologyrepository.com/CommonCoreOntologies/Bootkit -->

    <owl:Class rdf:about="http://www.ontologyrepository.com/CommonCoreOntologies/Bootkit">
        <rdfs:subClassOf rdf:resource="http://www.ontologyrepository.com/CommonCoreOntologies/Rootkit"/>
        <skos:definition xml:lang="en">Rootkit that is designed to replace a Computer&apos;s legitimate boot loader.</skos:definition>
        <rdfs:label xml:lang="en">Bootkit</rdfs:label>
        <cco2:ont00001754>https://en.wikipedia.org/wiki/Rootkit#bootkit</cco2:ont00001754>
        <cco2:ont00001760 rdf:datatype="http://www.w3.org/2001/XMLSchema#anyURI">http://www.ontologyrepository.com/CommonCoreOntologies/Domain/CyberOntology</cco2:ont00001760>
    </owl:Class>
    


    <!-- http://www.ontologyrepository.com/CommonCoreOntologies/Botnet -->

    <owl:Class rdf:about="http://www.ontologyrepository.com/CommonCoreOntologies/Botnet">
        <rdfs:subClassOf rdf:resource="https://www.commoncoreontologies.org/ont00000700"/>
        <skos:definition xml:lang="en">A Computer Network which is composed of two or more Internet-connected devices, each of which is running one or more Internet Bots.</skos:definition>
        <rdfs:label xml:lang="en">Botnet</rdfs:label>
        <cco2:ont00001754 rdf:datatype="http://www.w3.org/2001/XMLSchema#anyURI">https://en.wikipedia.org/wiki/Botnet</cco2:ont00001754>
        <cco2:ont00001760 rdf:datatype="http://www.w3.org/2001/XMLSchema#anyURI">http://www.ontologyrepository.com/CommonCoreOntologies/Domain/CyberOntology</cco2:ont00001760>
    </owl:Class>
    


    <!-- http://www.ontologyrepository.com/CommonCoreOntologies/BroadbandCommunicationArtifactFunction -->

    <owl:Class rdf:about="http://www.ontologyrepository.com/CommonCoreOntologies/BroadbandCommunicationArtifactFunction">
        <rdfs:subClassOf rdf:resource="https://www.commoncoreontologies.org/ont00000727"/>
        <rdfs:subClassOf>
            <owl:Restriction>
                <owl:onProperty rdf:resource="http://purl.obolibrary.org/obo/BFO_0000197"/>
                <owl:someValuesFrom rdf:resource="https://www.commoncoreontologies.org/ont00000998"/>
            </owl:Restriction>
        </rdfs:subClassOf>
        <skos:definition xml:lang="en">A Communication Artifact Function that is realized in relatively high Bit transfer rates.</skos:definition>
        <rdfs:label xml:lang="en">Broadband Communication Artifact Function</rdfs:label>
        <cco2:ont00001760 rdf:datatype="http://www.w3.org/2001/XMLSchema#anyURI">http://www.ontologyrepository.com/CommonCoreOntologies/Domain/CyberOntology</cco2:ont00001760>
    </owl:Class>
    


    <!-- http://www.ontologyrepository.com/CommonCoreOntologies/BrowserHijackingProgram -->

    <owl:Class rdf:about="http://www.ontologyrepository.com/CommonCoreOntologies/BrowserHijackingProgram">
        <rdfs:subClassOf rdf:resource="http://www.ontologyrepository.com/CommonCoreOntologies/Malware"/>
        <skos:definition xml:lang="en">Malware that is designed to modify a Web Browser&apos;s settings without a user&apos;s permission in order to inject unwanted advertising into that Browser.</skos:definition>
        <rdfs:label xml:lang="en">Browser Hijacking Program</rdfs:label>
        <cco2:ont00001754>https://en.wikipedia.org/wiki/Browser_hijacking</cco2:ont00001754>
        <cco2:ont00001760 rdf:datatype="http://www.w3.org/2001/XMLSchema#anyURI">http://www.ontologyrepository.com/CommonCoreOntologies/Domain/CyberOntology</cco2:ont00001760>
    </owl:Class>
    


    <!-- http://www.ontologyrepository.com/CommonCoreOntologies/Byte -->

    <owl:Class rdf:about="http://www.ontologyrepository.com/CommonCoreOntologies/Byte">
        <rdfs:subClassOf rdf:resource="https://www.commoncoreontologies.org/ont00000798"/>
        <skos:definition xml:lang="en">An Information Bearing Artifact that consists of an ordered collection of eight or fewer Bits.</skos:definition>
        <rdfs:comment xml:lang="en">Bytes are almost ubiquitously understood as ordered collections of eight Bits, but there are exceptions where Bytes are understood as ordered collections of fewer than eight Bits.</rdfs:comment>
        <rdfs:label xml:lang="en">Byte</rdfs:label>
        <cco2:ont00001754>https://en.wikipedia.org/wiki/Byte</cco2:ont00001754>
        <cco2:ont00001760 rdf:datatype="http://www.w3.org/2001/XMLSchema#anyURI">http://www.ontologyrepository.com/CommonCoreOntologies/Domain/CyberOntology</cco2:ont00001760>
    </owl:Class>
    


    <!-- http://www.ontologyrepository.com/CommonCoreOntologies/CVEVulnerability -->

    <owl:Class rdf:about="http://www.ontologyrepository.com/CommonCoreOntologies/CVEVulnerability">
        <owl:equivalentClass>
            <owl:Class>
                <owl:intersectionOf rdf:parseType="Collection">
                    <rdf:Description rdf:about="http://www.ontologyrepository.com/CommonCoreOntologies/CyberVulnerability"/>
                    <owl:Restriction>
                        <owl:onProperty rdf:resource="http://purl.obolibrary.org/obo/BFO_0000197"/>
                        <owl:someValuesFrom>
                            <owl:Class>
                                <owl:intersectionOf rdf:parseType="Collection">
                                    <rdf:Description rdf:about="https://www.commoncoreontologies.org/ont00000117"/>
                                    <owl:Restriction>
                                        <owl:onProperty rdf:resource="https://www.commoncoreontologies.org/ont00001920"/>
                                        <owl:someValuesFrom rdf:resource="http://www.ontologyrepository.com/CommonCoreOntologies/ComputerProgramArtifactModel"/>
                                    </owl:Restriction>
                                </owl:intersectionOf>
                            </owl:Class>
                        </owl:someValuesFrom>
                    </owl:Restriction>
                </owl:intersectionOf>
            </owl:Class>
        </owl:equivalentClass>
        <rdfs:subClassOf rdf:resource="http://www.ontologyrepository.com/CommonCoreOntologies/CyberVulnerability"/>
        <skos:altLabel xml:lang="en">Common Vulnerability or Exposure</skos:altLabel>
        <skos:definition xml:lang="en">A Cyber Vulnerability that inheres in an Information Processing Artifact prescribed by a known Computer Program Artifact Model.</skos:definition>
        <rdfs:label xml:lang="en">CVE Vulnerability</rdfs:label>
        <rdfs:seeAlso rdf:datatype="http://www.w3.org/2001/XMLSchema#anyURI">https://cve.mitre.org/about/index.html</rdfs:seeAlso>
        <cco2:ont00001760 rdf:datatype="http://www.w3.org/2001/XMLSchema#anyURI">http://www.ontologyrepository.com/CommonCoreOntologies/Domain/CyberOntology</cco2:ont00001760>
    </owl:Class>
    


    <!-- http://www.ontologyrepository.com/CommonCoreOntologies/CacheMemory -->

    <owl:Class rdf:about="http://www.ontologyrepository.com/CommonCoreOntologies/CacheMemory">
        <rdfs:subClassOf rdf:resource="http://www.ontologyrepository.com/CommonCoreOntologies/ComputerMemory"/>
        <skos:definition xml:lang="en">Computer Memory that is fast, relatively small, not visible to software, is completely handled by the hardware, and stores the most recently used main memory data.</skos:definition>
        <rdfs:label xml:lang="en">Cache Memory</rdfs:label>
        <cco2:ont00001754>https://en.wikipedia.org/wiki/Cache_memory</cco2:ont00001754>
        <cco2:ont00001760 rdf:datatype="http://www.w3.org/2001/XMLSchema#anyURI">http://www.ontologyrepository.com/CommonCoreOntologies/Domain/CyberOntology</cco2:ont00001760>
    </owl:Class>
    


    <!-- http://www.ontologyrepository.com/CommonCoreOntologies/CallCenter -->

    <owl:Class rdf:about="http://www.ontologyrepository.com/CommonCoreOntologies/CallCenter">
        <rdfs:subClassOf rdf:resource="https://www.commoncoreontologies.org/ont00000531"/>
        <skos:definition xml:lang="en">A Communications Facility that is designed to house Groups of Agents who respond to inquiries for an Organization.</skos:definition>
        <rdfs:label xml:lang="en">Call Center</rdfs:label>
        <cco2:ont00001760 rdf:datatype="http://www.w3.org/2001/XMLSchema#anyURI">http://www.ontologyrepository.com/CommonCoreOntologies/Domain/CyberOntology</cco2:ont00001760>
    </owl:Class>
    


    <!-- http://www.ontologyrepository.com/CommonCoreOntologies/CentralProcessingUnit -->

    <owl:Class rdf:about="http://www.ontologyrepository.com/CommonCoreOntologies/CentralProcessingUnit">
        <rdfs:subClassOf rdf:resource="http://www.ontologyrepository.com/CommonCoreOntologies/ProcessingUnit"/>
        <skos:definition xml:lang="en">A Processing Unit that is designed to execute the basic arithmetic, logical, control, and input/output operations prescribed by some Computer Program.</skos:definition>
        <rdfs:label xml:lang="en">Central Processing Unit</rdfs:label>
        <cco2:ont00001754>https://en.wikipedia.org/wiki/Central_processing_unit</cco2:ont00001754>
        <cco2:ont00001760 rdf:datatype="http://www.w3.org/2001/XMLSchema#anyURI">http://www.ontologyrepository.com/CommonCoreOntologies/Domain/CyberOntology</cco2:ont00001760>
    </owl:Class>
    


    <!-- http://www.ontologyrepository.com/CommonCoreOntologies/ChecksumMeasurement -->

    <owl:Class rdf:about="http://www.ontologyrepository.com/CommonCoreOntologies/ChecksumMeasurement">
        <rdfs:subClassOf rdf:resource="https://www.commoncoreontologies.org/ont00001022"/>
        <skos:definition xml:lang="en">A Ratio Measurement Information Content Entity that is a measurement of the number of bits in a transmission unit that is included with the unit so that the receiver can check to see whether the same number of bits arrived.</skos:definition>
        <rdfs:label xml:lang="en">Checksum Measurement</rdfs:label>
        <cco2:ont00001754>http://searchsecurity.techtarget.com/definition/checksum</cco2:ont00001754>
        <cco2:ont00001760 rdf:datatype="http://www.w3.org/2001/XMLSchema#anyURI">http://www.ontologyrepository.com/CommonCoreOntologies/Domain/CyberOntology</cco2:ont00001760>
    </owl:Class>
    


    <!-- http://www.ontologyrepository.com/CommonCoreOntologies/ChildComputerProgramExecution -->

    <owl:Class rdf:about="http://www.ontologyrepository.com/CommonCoreOntologies/ChildComputerProgramExecution">
        <owl:equivalentClass>
            <owl:Class>
                <owl:intersectionOf rdf:parseType="Collection">
                    <rdf:Description rdf:about="http://www.ontologyrepository.com/CommonCoreOntologies/ComputerProgramExecution"/>
                    <owl:Restriction>
                        <owl:onProperty rdf:resource="https://www.commoncoreontologies.org/ont00001962"/>
                        <owl:someValuesFrom rdf:resource="http://www.ontologyrepository.com/CommonCoreOntologies/ComputerProgramExecution"/>
                    </owl:Restriction>
                </owl:intersectionOf>
            </owl:Class>
        </owl:equivalentClass>
        <rdfs:subClassOf rdf:resource="http://www.ontologyrepository.com/CommonCoreOntologies/ComputerProgramExecution"/>
        <skos:altLabel xml:lang="en">Child Computer Process</skos:altLabel>
        <skos:definition xml:lang="en">A Computer Program Execution that is started by some other Computer Program Execution.</skos:definition>
        <rdfs:label xml:lang="en">Child Computer Program Execution</rdfs:label>
        <cco2:ont00001760 rdf:datatype="http://www.w3.org/2001/XMLSchema#anyURI">http://www.ontologyrepository.com/CommonCoreOntologies/Domain/CyberOntology</cco2:ont00001760>
    </owl:Class>
    


    <!-- http://www.ontologyrepository.com/CommonCoreOntologies/CodeCompilation -->

    <owl:Class rdf:about="http://www.ontologyrepository.com/CommonCoreOntologies/CodeCompilation">
        <rdfs:subClassOf rdf:resource="http://www.ontologyrepository.com/CommonCoreOntologies/ComputerProgramExecution"/>
        <rdfs:subClassOf>
            <owl:Restriction>
                <owl:onProperty rdf:resource="http://www.ontologyrepository.com/CommonCoreOntologies/has_causal_factor"/>
                <owl:someValuesFrom rdf:resource="http://www.ontologyrepository.com/CommonCoreOntologies/CodeCompiler"/>
            </owl:Restriction>
        </rdfs:subClassOf>
        <skos:definition xml:lang="en">A Computer Program Execution in which some Information Bearing Entity that uses a Compiled Language is translated into some Information Bearing Entity that uses a Low-Level Programming Language.</skos:definition>
        <rdfs:label xml:lang="en">Code Compilation</rdfs:label>
        <cco2:ont00001760 rdf:datatype="http://www.w3.org/2001/XMLSchema#anyURI">http://www.ontologyrepository.com/CommonCoreOntologies/Domain/CyberOntology</cco2:ont00001760>
    </owl:Class>
    


    <!-- http://www.ontologyrepository.com/CommonCoreOntologies/CodeCompiler -->

    <owl:Class rdf:about="http://www.ontologyrepository.com/CommonCoreOntologies/CodeCompiler">
        <rdfs:subClassOf rdf:resource="http://www.ontologyrepository.com/CommonCoreOntologies/SoftwareEngineeringSoftware"/>
        <skos:definition xml:lang="en">A Software Engineering Application that translates another Computer Program written in one Programming Language into another Programming Language, most often to create an Executable Program.</skos:definition>
        <rdfs:label xml:lang="en">Code Compiler</rdfs:label>
        <cco2:ont00001760 rdf:datatype="http://www.w3.org/2001/XMLSchema#anyURI">http://www.ontologyrepository.com/CommonCoreOntologies/Domain/CyberOntology</cco2:ont00001760>
    </owl:Class>
    


    <!-- http://www.ontologyrepository.com/CommonCoreOntologies/CodeInterpreter -->

    <owl:Class rdf:about="http://www.ontologyrepository.com/CommonCoreOntologies/CodeInterpreter">
        <rdfs:subClassOf rdf:resource="http://www.ontologyrepository.com/CommonCoreOntologies/SoftwareEngineeringSoftware"/>
        <skos:definition xml:lang="en">A Software Engineering Application that directly executes the instructions of some Executable Program without compiling those instructions into some Machine Language.</skos:definition>
        <rdfs:label xml:lang="en">Code Interpreter</rdfs:label>
        <cco2:ont00001760 rdf:datatype="http://www.w3.org/2001/XMLSchema#anyURI">http://www.ontologyrepository.com/CommonCoreOntologies/Domain/CyberOntology</cco2:ont00001760>
    </owl:Class>
    


    <!-- http://www.ontologyrepository.com/CommonCoreOntologies/CompiledLanguage -->

    <owl:Class rdf:about="http://www.ontologyrepository.com/CommonCoreOntologies/CompiledLanguage">
        <rdfs:subClassOf rdf:resource="http://www.ontologyrepository.com/CommonCoreOntologies/HighLevelProgrammingLanguage"/>
        <rdfs:subClassOf>
            <owl:Restriction>
                <owl:onProperty rdf:resource="https://www.commoncoreontologies.org/ont00001899"/>
                <owl:someValuesFrom>
                    <owl:Class>
                        <owl:intersectionOf rdf:parseType="Collection">
                            <rdf:Description rdf:about="http://www.ontologyrepository.com/CommonCoreOntologies/ComputerProgram"/>
                            <owl:Restriction>
                                <owl:onProperty rdf:resource="https://www.commoncoreontologies.org/ont00001816"/>
                                <owl:someValuesFrom rdf:resource="http://www.ontologyrepository.com/CommonCoreOntologies/CodeCompilation"/>
                            </owl:Restriction>
                        </owl:intersectionOf>
                    </owl:Class>
                </owl:someValuesFrom>
            </owl:Restriction>
        </rdfs:subClassOf>
        <owl:disjointWith rdf:resource="http://www.ontologyrepository.com/CommonCoreOntologies/InterpretedLanguage"/>
        <owl:disjointWith rdf:resource="http://www.ontologyrepository.com/CommonCoreOntologies/MachineLanguage"/>
        <skos:definition xml:lang="en">A Programming Language that prescribes a canonical form of communicating instructions to be executed by a Processing Unit in such a way that the Information Bearing Entity that uses this Programming Language must first be the input of some Code Compilation.</skos:definition>
        <rdfs:label xml:lang="en">Compiled Language</rdfs:label>
        <cco2:ont00001754>https://en.wikipedia.org/wiki/Compiled_language</cco2:ont00001754>
        <cco2:ont00001760 rdf:datatype="http://www.w3.org/2001/XMLSchema#anyURI">http://www.ontologyrepository.com/CommonCoreOntologies/Domain/CyberOntology</cco2:ont00001760>
    </owl:Class>
    


    <!-- http://www.ontologyrepository.com/CommonCoreOntologies/CompressedDataFormat -->

    <owl:Class rdf:about="http://www.ontologyrepository.com/CommonCoreOntologies/CompressedDataFormat">
        <rdfs:subClassOf rdf:resource="http://www.ontologyrepository.com/CommonCoreOntologies/FileFormat"/>
        <skos:definition xml:lang="en">A File Format that prescribes a way of encoding information which uses fewer Bits than the original encoding of that information.</skos:definition>
        <skos:example>A .zip file format</skos:example>
        <rdfs:label xml:lang="en">Compressed Data Format</rdfs:label>
        <cco2:ont00001754>https://en.wikipedia.org/wiki/Data_compression</cco2:ont00001754>
        <cco2:ont00001760 rdf:datatype="http://www.w3.org/2001/XMLSchema#anyURI">http://www.ontologyrepository.com/CommonCoreOntologies/Domain/CyberOntology</cco2:ont00001760>
    </owl:Class>
    


    <!-- http://www.ontologyrepository.com/CommonCoreOntologies/ComputerAggregate -->

    <owl:Class rdf:about="http://www.ontologyrepository.com/CommonCoreOntologies/ComputerAggregate">
        <rdfs:subClassOf rdf:resource="http://purl.obolibrary.org/obo/BFO_0000027"/>
        <skos:definition xml:lang="en">An Object Aggregate that consists of Computers.</skos:definition>
        <rdfs:label xml:lang="en">Computer Aggregate</rdfs:label>
        <cco2:ont00001760 rdf:datatype="http://www.w3.org/2001/XMLSchema#anyURI">http://www.ontologyrepository.com/CommonCoreOntologies/Domain/CyberOntology</cco2:ont00001760>
    </owl:Class>
    


    <!-- http://www.ontologyrepository.com/CommonCoreOntologies/ComputerComponent -->

    <owl:Class rdf:about="http://www.ontologyrepository.com/CommonCoreOntologies/ComputerComponent">
        <rdfs:subClassOf rdf:resource="https://www.commoncoreontologies.org/ont00000995"/>
        <skos:altLabel xml:lang="en">Computer Hardware</skos:altLabel>
        <skos:definition xml:lang="en">An Artifact designed to be a component of a Computer.</skos:definition>
        <rdfs:label xml:lang="en">Computer Component</rdfs:label>
        <cco2:ont00001754 rdf:datatype="http://www.w3.org/2001/XMLSchema#anyURI">https://en.wikipedia.org/wiki/Computer_hardware</cco2:ont00001754>
        <cco2:ont00001760 rdf:datatype="http://www.w3.org/2001/XMLSchema#anyURI">http://www.ontologyrepository.com/CommonCoreOntologies/Domain/CyberOntology</cco2:ont00001760>
    </owl:Class>
    


    <!-- http://www.ontologyrepository.com/CommonCoreOntologies/ComputerKeyboard -->

    <owl:Class rdf:about="http://www.ontologyrepository.com/CommonCoreOntologies/ComputerKeyboard">
        <rdfs:subClassOf rdf:resource="http://www.ontologyrepository.com/CommonCoreOntologies/InputDevice"/>
        <skos:definition xml:lang="en">An Input Device designed to enable users to input text and control a Computer via a standardized arrangement of keys.</skos:definition>
        <rdfs:label xml:lang="en">Computer Keyboard</rdfs:label>
        <cco2:ont00001754 rdf:datatype="http://www.w3.org/2001/XMLSchema#anyURI">https://en.wikipedia.org/wiki/Computer_keyboard</cco2:ont00001754>
        <cco2:ont00001760 rdf:datatype="http://www.w3.org/2001/XMLSchema#anyURI">http://www.ontologyrepository.com/CommonCoreOntologies/Domain/CyberOntology</cco2:ont00001760>
    </owl:Class>
    


    <!-- http://www.ontologyrepository.com/CommonCoreOntologies/ComputerLanguage -->

    <owl:Class rdf:about="http://www.ontologyrepository.com/CommonCoreOntologies/ComputerLanguage">
        <rdfs:subClassOf rdf:resource="https://www.commoncoreontologies.org/ont00000146"/>
        <skos:definition xml:lang="en">An Artificial Language that prescribes a canonical form of communiction within or between Computers.</skos:definition>
        <rdfs:label xml:lang="en">Computer Language</rdfs:label>
        <cco2:ont00001760 rdf:datatype="http://www.w3.org/2001/XMLSchema#anyURI">http://www.ontologyrepository.com/CommonCoreOntologies/Domain/CyberOntology</cco2:ont00001760>
    </owl:Class>
    


    <!-- http://www.ontologyrepository.com/CommonCoreOntologies/ComputerLogFile -->

    <owl:Class rdf:about="http://www.ontologyrepository.com/CommonCoreOntologies/ComputerLogFile">
        <rdfs:subClassOf rdf:resource="http://www.ontologyrepository.com/CommonCoreOntologies/DigitalFile"/>
        <skos:definition xml:lang="en">An Information Bearing Artifact that bears information recording the activity of a device or process within some Computer.</skos:definition>
        <rdfs:label xml:lang="en">Computer Log File</rdfs:label>
        <cco2:ont00001760 rdf:datatype="http://www.w3.org/2001/XMLSchema#anyURI">http://www.ontologyrepository.com/CommonCoreOntologies/Domain/CyberOntology</cco2:ont00001760>
    </owl:Class>
    


    <!-- http://www.ontologyrepository.com/CommonCoreOntologies/ComputerMemory -->

    <owl:Class rdf:about="http://www.ontologyrepository.com/CommonCoreOntologies/ComputerMemory">
        <rdfs:subClassOf rdf:resource="https://www.commoncoreontologies.org/ont00001179"/>
        <skos:definition xml:lang="en">A Digital Storage Device that stores some Information Content Entity for immediate use in a Computer.</skos:definition>
        <rdfs:label xml:lang="en">Computer Memory</rdfs:label>
        <cco2:ont00001754>https://en.wikipedia.org/wiki/Computer_memory</cco2:ont00001754>
        <cco2:ont00001760 rdf:datatype="http://www.w3.org/2001/XMLSchema#anyURI">http://www.ontologyrepository.com/CommonCoreOntologies/Domain/CyberOntology</cco2:ont00001760>
    </owl:Class>
    


    <!-- http://www.ontologyrepository.com/CommonCoreOntologies/ComputerMemoryLocation -->

    <owl:Class rdf:about="http://www.ontologyrepository.com/CommonCoreOntologies/ComputerMemoryLocation">
        <rdfs:subClassOf rdf:resource="https://www.commoncoreontologies.org/ont00000798"/>
        <skos:definition xml:lang="en">An Information Bearing Artifact that is part of some Computer Memory and bears some Information Content Entity.</skos:definition>
        <rdfs:label xml:lang="en">Computer Memory Location</rdfs:label>
        <cco2:ont00001760 rdf:datatype="http://www.w3.org/2001/XMLSchema#anyURI">http://www.ontologyrepository.com/CommonCoreOntologies/Domain/CyberOntology</cco2:ont00001760>
    </owl:Class>
    


    <!-- http://www.ontologyrepository.com/CommonCoreOntologies/ComputerMonitor -->

    <owl:Class rdf:about="http://www.ontologyrepository.com/CommonCoreOntologies/ComputerMonitor">
        <rdfs:subClassOf rdf:resource="http://www.ontologyrepository.com/CommonCoreOntologies/OutputDevice"/>
        <skos:definition xml:lang="en">An Output Device that displays information in pictorial form</skos:definition>
        <rdfs:label xml:lang="en">Computer Monitor</rdfs:label>
        <cco2:ont00001754 rdf:datatype="http://www.w3.org/2001/XMLSchema#anyURI">https://en.wikipedia.org/wiki/Computer_monitor</cco2:ont00001754>
        <cco2:ont00001760 rdf:datatype="http://www.w3.org/2001/XMLSchema#anyURI">http://www.ontologyrepository.com/CommonCoreOntologies/Domain/CyberOntology</cco2:ont00001760>
    </owl:Class>
    


    <!-- http://www.ontologyrepository.com/CommonCoreOntologies/ComputerMouse -->

    <owl:Class rdf:about="http://www.ontologyrepository.com/CommonCoreOntologies/ComputerMouse">
        <rdfs:subClassOf rdf:resource="http://www.ontologyrepository.com/CommonCoreOntologies/PointingDevice"/>
        <skos:definition xml:lang="en">A Pointing Device that detects two-dimensional motion relative to a surface and typically translates this motion of a pointer on a display, which allows a smooth control of the graphical user interface of a computer.</skos:definition>
        <rdfs:label xml:lang="en">Computer Mouse</rdfs:label>
        <cco2:ont00001754 rdf:datatype="http://www.w3.org/2001/XMLSchema#anyURI">https://en.wikipedia.org/wiki/Computer_mouse</cco2:ont00001754>
        <cco2:ont00001760 rdf:datatype="http://www.w3.org/2001/XMLSchema#anyURI">http://www.ontologyrepository.com/CommonCoreOntologies/Domain/CyberOntology</cco2:ont00001760>
    </owl:Class>
    


    <!-- http://www.ontologyrepository.com/CommonCoreOntologies/ComputerNetworkingDevice -->

    <owl:Class rdf:about="http://www.ontologyrepository.com/CommonCoreOntologies/ComputerNetworkingDevice">
        <rdfs:subClassOf rdf:resource="https://www.commoncoreontologies.org/ont00000315"/>
        <skos:altLabel xml:lang="en">Networking Hardware</skos:altLabel>
        <skos:definition xml:lang="en">A Telecommunication Switching Node that is designed to send and receive data over a Computer Network.</skos:definition>
        <skos:example>Router</skos:example>
        <skos:example>Switch</skos:example>
        <rdfs:label xml:lang="en">Computer Networking Device</rdfs:label>
        <cco2:ont00001754>https://en.wikipedia.org/wiki/Networking_hardware</cco2:ont00001754>
        <cco2:ont00001760 rdf:datatype="http://www.w3.org/2001/XMLSchema#anyURI">http://www.ontologyrepository.com/CommonCoreOntologies/Domain/CyberOntology</cco2:ont00001760>
    </owl:Class>
    


    <!-- http://www.ontologyrepository.com/CommonCoreOntologies/ComputerNetworkingPort -->

    <owl:Class rdf:about="http://www.ontologyrepository.com/CommonCoreOntologies/ComputerNetworkingPort">
        <rdfs:subClassOf rdf:resource="https://www.commoncoreontologies.org/ont00001247"/>
        <skos:definition xml:lang="en">A Telecommunication Endpoint that is used to provide or receive specified services over a Computer Network.</skos:definition>
        <rdfs:label xml:lang="en">Computer Networking Port</rdfs:label>
        <cco2:ont00001754>https://en.wikipedia.org/wiki/Port_(computer_networking)</cco2:ont00001754>
        <cco2:ont00001760 rdf:datatype="http://www.w3.org/2001/XMLSchema#anyURI">http://www.ontologyrepository.com/CommonCoreOntologies/Domain/CyberOntology</cco2:ont00001760>
    </owl:Class>
    


    <!-- http://www.ontologyrepository.com/CommonCoreOntologies/ComputerObject -->

    <owl:Class rdf:about="http://www.ontologyrepository.com/CommonCoreOntologies/ComputerObject">
        <rdfs:subClassOf rdf:resource="http://www.ontologyrepository.com/CommonCoreOntologies/ComputerMemoryLocation"/>
        <skos:definition xml:lang="en">A Computer Memory Location that consists of a variable, function, or data structure that can be manipulated by a Computer Program or Subroutine.</skos:definition>
        <rdfs:label xml:lang="en">Computer Object</rdfs:label>
        <cco2:ont00001760 rdf:datatype="http://www.w3.org/2001/XMLSchema#anyURI">http://www.ontologyrepository.com/CommonCoreOntologies/Domain/CyberOntology</cco2:ont00001760>
    </owl:Class>
    


    <!-- http://www.ontologyrepository.com/CommonCoreOntologies/ComputerPrinter -->

    <owl:Class rdf:about="http://www.ontologyrepository.com/CommonCoreOntologies/ComputerPrinter">
        <rdfs:subClassOf rdf:resource="http://www.ontologyrepository.com/CommonCoreOntologies/OutputDevice"/>
        <skos:definition xml:lang="en">An Output Device which makes a persistent representation of graphics or text, usually on paper.</skos:definition>
        <rdfs:label xml:lang="en">Computer Printer</rdfs:label>
        <cco2:ont00001754 rdf:datatype="http://www.w3.org/2001/XMLSchema#anyURI">https://en.wikipedia.org/wiki/Printer_(computing)</cco2:ont00001754>
        <cco2:ont00001760 rdf:datatype="http://www.w3.org/2001/XMLSchema#anyURI">http://www.ontologyrepository.com/CommonCoreOntologies/Domain/CyberOntology</cco2:ont00001760>
    </owl:Class>
    


    <!-- http://www.ontologyrepository.com/CommonCoreOntologies/ComputerPrinterFunction -->

    <owl:Class rdf:about="http://www.ontologyrepository.com/CommonCoreOntologies/ComputerPrinterFunction">
        <rdfs:subClassOf rdf:resource="http://www.ontologyrepository.com/CommonCoreOntologies/InformationProcessingArtifactFunction"/>
        <skos:definition xml:lang="en">An Information Processing Artifact Function that when realized is in a process of transforming a Digital File into a persistent Document or Image.</skos:definition>
        <rdfs:label xml:lang="en">Computer Printer Function</rdfs:label>
        <cco2:ont00001760 rdf:datatype="http://www.w3.org/2001/XMLSchema#anyURI">http://www.ontologyrepository.com/CommonCoreOntologies/Domain/CyberOntology</cco2:ont00001760>
    </owl:Class>
    


    <!-- http://www.ontologyrepository.com/CommonCoreOntologies/ComputerProgram -->

    <owl:Class rdf:about="http://www.ontologyrepository.com/CommonCoreOntologies/ComputerProgram">
        <rdfs:subClassOf rdf:resource="https://www.commoncoreontologies.org/ont00000117"/>
        <skos:definition xml:lang="en">An Information Processing Artifact that consists of a collection of Computer Functions that are designed to be executed by a Processing Unit to perform a specific task.</skos:definition>
        <rdfs:label xml:lang="en">Computer Program</rdfs:label>
        <cco2:ont00001754>https://en.wikipedia.org/wiki/Computer_program</cco2:ont00001754>
        <cco2:ont00001760 rdf:datatype="http://www.w3.org/2001/XMLSchema#anyURI">http://www.ontologyrepository.com/CommonCoreOntologies/Domain/CyberOntology</cco2:ont00001760>
    </owl:Class>
    


    <!-- http://www.ontologyrepository.com/CommonCoreOntologies/ComputerProgramArtifactModel -->

    <owl:Class rdf:about="http://www.ontologyrepository.com/CommonCoreOntologies/ComputerProgramArtifactModel">
        <rdfs:subClassOf rdf:resource="https://www.commoncoreontologies.org/ont00001045"/>
        <rdfs:subClassOf>
            <owl:Restriction>
                <owl:onProperty rdf:resource="https://www.commoncoreontologies.org/ont00001942"/>
                <owl:someValuesFrom rdf:resource="http://www.ontologyrepository.com/CommonCoreOntologies/ComputerProgram"/>
            </owl:Restriction>
        </rdfs:subClassOf>
        <skos:definition xml:lang="en">An Artifact Model that prescribes a Computer Program.</skos:definition>
        <skos:example xml:lang="en">Vim v8.1</skos:example>
        <rdfs:label xml:lang="en">Computer Program Artifact Model</rdfs:label>
        <cco2:ont00001760 rdf:datatype="http://www.w3.org/2001/XMLSchema#anyURI">http://www.ontologyrepository.com/CommonCoreOntologies/Domain/CyberOntology</cco2:ont00001760>
    </owl:Class>
    


    <!-- http://www.ontologyrepository.com/CommonCoreOntologies/ComputerProgramExecution -->

    <owl:Class rdf:about="http://www.ontologyrepository.com/CommonCoreOntologies/ComputerProgramExecution">
        <rdfs:subClassOf rdf:resource="https://www.commoncoreontologies.org/ont00000110"/>
        <rdfs:subClassOf>
            <owl:Restriction>
                <owl:onProperty rdf:resource="https://www.commoncoreontologies.org/ont00001920"/>
                <owl:someValuesFrom rdf:resource="https://www.commoncoreontologies.org/ont00000653"/>
            </owl:Restriction>
        </rdfs:subClassOf>
        <skos:altLabel xml:lang="en">Computer Process</skos:altLabel>
        <skos:definition xml:lang="en">A Mechanical Process that is comprised of a sequence of simple operations performed by a Central Processing Unit or some Computer Program according to the instructions of some Algorithm.</skos:definition>
        <rdfs:label xml:lang="en">Computer Program Execution</rdfs:label>
        <cco2:ont00001760 rdf:datatype="http://www.w3.org/2001/XMLSchema#anyURI">http://www.ontologyrepository.com/CommonCoreOntologies/Domain/CyberOntology</cco2:ont00001760>
    </owl:Class>
    


    <!-- http://www.ontologyrepository.com/CommonCoreOntologies/ComputerSystem -->

    <owl:Class rdf:about="http://www.ontologyrepository.com/CommonCoreOntologies/ComputerSystem">
        <rdfs:subClassOf rdf:resource="http://purl.obolibrary.org/obo/BFO_0000027"/>
        <skos:definition xml:lang="en">An Object Aggregate that has a Computer and some Computer Peripheral Device as members.</skos:definition>
        <rdfs:label xml:lang="en">Computer System</rdfs:label>
        <cco2:ont00001760 rdf:datatype="http://www.w3.org/2001/XMLSchema#anyURI">http://www.ontologyrepository.com/CommonCoreOntologies/Domain/CyberOntology</cco2:ont00001760>
    </owl:Class>
    


    <!-- http://www.ontologyrepository.com/CommonCoreOntologies/ComputerTablet -->

    <owl:Class rdf:about="http://www.ontologyrepository.com/CommonCoreOntologies/ComputerTablet">
        <rdfs:subClassOf rdf:resource="https://www.commoncoreontologies.org/ont00000420"/>
        <skos:definition xml:lang="en">A Computer that is designed to be portable, has a touchscreen, and does not have a fixed hardware keyboard.</skos:definition>
        <rdfs:label xml:lang="en">Computer Tablet</rdfs:label>
        <cco2:ont00001760 rdf:datatype="http://www.w3.org/2001/XMLSchema#anyURI">http://www.ontologyrepository.com/CommonCoreOntologies/Domain/CyberOntology</cco2:ont00001760>
    </owl:Class>
    


    <!-- http://www.ontologyrepository.com/CommonCoreOntologies/ComputerVirus -->

    <owl:Class rdf:about="http://www.ontologyrepository.com/CommonCoreOntologies/ComputerVirus">
        <rdfs:subClassOf rdf:resource="http://www.ontologyrepository.com/CommonCoreOntologies/Malware"/>
        <skos:definition xml:lang="en">Malware that is designed to replicate itself by modifying existent Computer Programs and inserting its own code.</skos:definition>
        <rdfs:label xml:lang="en">Computer Virus</rdfs:label>
        <cco2:ont00001754>https://en.wikipedia.org/wiki/Computer_virus</cco2:ont00001754>
        <cco2:ont00001760 rdf:datatype="http://www.w3.org/2001/XMLSchema#anyURI">http://www.ontologyrepository.com/CommonCoreOntologies/Domain/CyberOntology</cco2:ont00001760>
    </owl:Class>
    


    <!-- http://www.ontologyrepository.com/CommonCoreOntologies/ComputerWorm -->

    <owl:Class rdf:about="http://www.ontologyrepository.com/CommonCoreOntologies/ComputerWorm">
        <rdfs:subClassOf rdf:resource="http://www.ontologyrepository.com/CommonCoreOntologies/Malware"/>
        <skos:definition xml:lang="en">Malware that is designed to replicate itself in order to spread to other Computers.</skos:definition>
        <rdfs:label xml:lang="en">Computer Worm</rdfs:label>
        <cco2:ont00001754>https://en.wikipedia.org/wiki/Computer_worm</cco2:ont00001754>
        <cco2:ont00001760 rdf:datatype="http://www.w3.org/2001/XMLSchema#anyURI">http://www.ontologyrepository.com/CommonCoreOntologies/Domain/CyberOntology</cco2:ont00001760>
    </owl:Class>
    


    <!-- http://www.ontologyrepository.com/CommonCoreOntologies/ComputingBandwidthMeasurement -->

    <owl:Class rdf:about="http://www.ontologyrepository.com/CommonCoreOntologies/ComputingBandwidthMeasurement">
        <rdfs:subClassOf rdf:resource="https://www.commoncoreontologies.org/ont00001022"/>
        <skos:definition xml:lang="en">A Ratio Measurement Information Content Entity that is a measurement of the rate of Bit transfer over time.</skos:definition>
        <rdfs:label xml:lang="en">Computing Bandwidth Measurement</rdfs:label>
        <cco2:ont00001760 rdf:datatype="http://www.w3.org/2001/XMLSchema#anyURI">http://www.ontologyrepository.com/CommonCoreOntologies/Domain/CyberOntology</cco2:ont00001760>
    </owl:Class>
    


    <!-- http://www.ontologyrepository.com/CommonCoreOntologies/Constraint -->

    <owl:Class rdf:about="http://www.ontologyrepository.com/CommonCoreOntologies/Constraint">
        <rdfs:subClassOf rdf:resource="https://www.commoncoreontologies.org/ont00000965"/>
        <skos:definition xml:lang="en">A Directive Information Content Entity that prescribes a limitation of an entity.</skos:definition>
        <rdfs:label xml:lang="en">Constraint</rdfs:label>
        <cco2:ont00001760 rdf:datatype="http://www.w3.org/2001/XMLSchema#anyURI">http://www.ontologyrepository.com/CommonCoreOntologies/Domain/CyberOntology</cco2:ont00001760>
    </owl:Class>
    


    <!-- http://www.ontologyrepository.com/CommonCoreOntologies/ContentAccessSoftware -->

    <owl:Class rdf:about="http://www.ontologyrepository.com/CommonCoreOntologies/ContentAccessSoftware">
        <rdfs:subClassOf rdf:resource="http://www.ontologyrepository.com/CommonCoreOntologies/ApplicationSoftware"/>
        <skos:definition xml:lang="en">Application Software that is designed to enable a user to access some information content without editing.</skos:definition>
        <rdfs:label xml:lang="en">Content Access Software</rdfs:label>
        <cco2:ont00001754>https://en.wikipedia.org/wiki/Application_software</cco2:ont00001754>
        <cco2:ont00001760 rdf:datatype="http://www.w3.org/2001/XMLSchema#anyURI">http://www.ontologyrepository.com/CommonCoreOntologies/Domain/CyberOntology</cco2:ont00001760>
    </owl:Class>
    


    <!-- http://www.ontologyrepository.com/CommonCoreOntologies/CryptanalystRole -->

    <owl:Class rdf:about="http://www.ontologyrepository.com/CommonCoreOntologies/CryptanalystRole">
        <rdfs:subClassOf rdf:resource="http://www.ontologyrepository.com/CommonCoreOntologies/CyberSecurityRole"/>
        <skos:definition xml:lang="en">A Cyber Security Role that inheres in an Agent by virtue of its responsibility to decipher secret codes and write codes that cannot be cracked by hackers</skos:definition>
        <rdfs:label xml:lang="en">Cryptanalyst Role</rdfs:label>
        <cco2:ont00001754 rdf:datatype="http://www.w3.org/2001/XMLSchema#anyURI">https://www.careerexplorer.com/careers/cryptanalyst/</cco2:ont00001754>
        <cco2:ont00001760 rdf:datatype="http://www.w3.org/2001/XMLSchema#anyURI">http://www.ontologyrepository.com/CommonCoreOntologies/Domain/CyberOntology</cco2:ont00001760>
    </owl:Class>
    


    <!-- http://www.ontologyrepository.com/CommonCoreOntologies/CryptographerRole -->

    <owl:Class rdf:about="http://www.ontologyrepository.com/CommonCoreOntologies/CryptographerRole">
        <rdfs:subClassOf rdf:resource="http://www.ontologyrepository.com/CommonCoreOntologies/CyberSecurityRole"/>
        <skos:definition xml:lang="en">A Cyber Security Role that inheres in an Agent by virtue of its responsibility to develop algorithms, ciphers and security systems to encrypt sensitive information and provide privacy for people and corporations.</skos:definition>
        <rdfs:label xml:lang="en">Cryptographer Role</rdfs:label>
        <cco2:ont00001754 rdf:datatype="http://www.w3.org/2001/XMLSchema#anyURI">https://www.careerexplorer.com/careers/cryptographer/</cco2:ont00001754>
    </owl:Class>
    


    <!-- http://www.ontologyrepository.com/CommonCoreOntologies/CyberAct -->

    <owl:Class rdf:about="http://www.ontologyrepository.com/CommonCoreOntologies/CyberAct">
        <owl:equivalentClass>
            <owl:Class>
                <owl:intersectionOf rdf:parseType="Collection">
                    <rdf:Description rdf:about="https://www.commoncoreontologies.org/ont00000005"/>
                    <owl:Restriction>
                        <owl:onProperty rdf:resource="http://purl.obolibrary.org/obo/BFO_0000066"/>
                        <owl:someValuesFrom rdf:resource="https://www.commoncoreontologies.org/ont00000700"/>
                    </owl:Restriction>
                </owl:intersectionOf>
            </owl:Class>
        </owl:equivalentClass>
        <rdfs:subClassOf rdf:resource="https://www.commoncoreontologies.org/ont00000005"/>
        <dc:contributor xml:lang="en">CUBRC Inc</dc:contributor>
        <skos:altLabel xml:lang="en">Cyber Event</skos:altLabel>
        <skos:definition xml:lang="en">A Cyber Act is an Act that occurs through cyberspace.</skos:definition>
        <rdfs:comment xml:lang="en">Roughly, anything that happens “within” a Computer Network (a.k.a. Cyber System or Information System) is a Cyber Act.</rdfs:comment>
        <rdfs:comment xml:lang="en">Change definition to: &quot;An Act that occurs in or through a Computer Network.&quot;</rdfs:comment>
        <rdfs:label xml:lang="en">Cyber Act</rdfs:label>
        <cco2:ont00001760 rdf:datatype="http://www.w3.org/2001/XMLSchema#anyURI">http://www.ontologyrepository.com/CommonCoreOntologies/Domain/CyberOntology</cco2:ont00001760>
    </owl:Class>
    


    <!-- http://www.ontologyrepository.com/CommonCoreOntologies/CyberAttack -->

    <owl:Class rdf:about="http://www.ontologyrepository.com/CommonCoreOntologies/CyberAttack">
        <rdfs:subClassOf rdf:resource="http://www.ontologyrepository.com/CommonCoreOntologies/CyberAct"/>
        <skos:definition xml:lang="en">Cyber Attack is a Cyber Act that is malicious and directed at a portion of cyber space.</skos:definition>
        <rdfs:comment xml:lang="en">An act that is intended to caused harm and is wrongful against another without legal justification or excuse.</rdfs:comment>
        <rdfs:label xml:lang="en">Cyber Attack</rdfs:label>
        <cco2:ont00001760 rdf:datatype="http://www.w3.org/2001/XMLSchema#anyURI">http://www.ontologyrepository.com/CommonCoreOntologies/Domain/CyberOntology</cco2:ont00001760>
    </owl:Class>
    


    <!-- http://www.ontologyrepository.com/CommonCoreOntologies/CyberAttackerRole -->

    <owl:Class rdf:about="http://www.ontologyrepository.com/CommonCoreOntologies/CyberAttackerRole">
        <owl:equivalentClass>
            <owl:Restriction>
                <owl:onProperty rdf:resource="https://www.commoncoreontologies.org/ont00001787"/>
                <owl:someValuesFrom rdf:resource="http://www.ontologyrepository.com/CommonCoreOntologies/CyberAttack"/>
            </owl:Restriction>
        </owl:equivalentClass>
        <rdfs:subClassOf rdf:resource="https://www.commoncoreontologies.org/ont00001017"/>
        <skos:definition xml:lang="en">A Material Entity that is agent in a Cyber Attack.</skos:definition>
        <rdfs:label xml:lang="en">Cyber Attacker</rdfs:label>
        <cco2:ont00001760 rdf:datatype="http://www.w3.org/2001/XMLSchema#anyURI">http://www.ontologyrepository.com/CommonCoreOntologies/Domain/CyberOntology</cco2:ont00001760>
    </owl:Class>
    


    <!-- http://www.ontologyrepository.com/CommonCoreOntologies/CyberDefenderRole -->

    <owl:Class rdf:about="http://www.ontologyrepository.com/CommonCoreOntologies/CyberDefenderRole">
        <rdfs:subClassOf rdf:resource="http://www.ontologyrepository.com/CommonCoreOntologies/CyberSecurityRole"/>
        <skos:definition xml:lang="en">A Cyber Security Role that inheres in an Agent by virtue of its responsibility for preventing, detecting and providing timely responses to attacks or threats against computers or computer networks.</skos:definition>
        <rdfs:label xml:lang="en">Cyber Defender Role</rdfs:label>
        <cco2:ont00001754 rdf:datatype="http://www.w3.org/2001/XMLSchema#anyURI">https://www.techopedia.com/definition/6705/cyber-defense</cco2:ont00001754>
        <cco2:ont00001760 rdf:datatype="http://www.w3.org/2001/XMLSchema#anyURI">http://www.ontologyrepository.com/CommonCoreOntologies/Domain/CyberOntology</cco2:ont00001760>
    </owl:Class>
    


    <!-- http://www.ontologyrepository.com/CommonCoreOntologies/CyberExploit -->

    <owl:Class rdf:about="http://www.ontologyrepository.com/CommonCoreOntologies/CyberExploit">
        <owl:equivalentClass>
            <owl:Class>
                <owl:intersectionOf rdf:parseType="Collection">
                    <owl:Class>
                        <owl:unionOf rdf:parseType="Collection">
                            <rdf:Description rdf:about="https://www.commoncoreontologies.org/ont00000117"/>
                            <rdf:Description rdf:about="https://www.commoncoreontologies.org/ont00000798"/>
                        </owl:unionOf>
                    </owl:Class>
                    <owl:Restriction>
                        <owl:onProperty rdf:resource="https://www.commoncoreontologies.org/ont00001925"/>
                        <owl:someValuesFrom>
                            <owl:Class>
                                <owl:intersectionOf rdf:parseType="Collection">
                                    <rdf:Description rdf:about="http://purl.obolibrary.org/obo/BFO_0000040"/>
                                    <owl:Restriction>
                                        <owl:onProperty rdf:resource="https://www.commoncoreontologies.org/ont00001787"/>
                                        <owl:someValuesFrom rdf:resource="http://www.ontologyrepository.com/CommonCoreOntologies/CyberAttack"/>
                                    </owl:Restriction>
                                </owl:intersectionOf>
                            </owl:Class>
                        </owl:someValuesFrom>
                    </owl:Restriction>
                </owl:intersectionOf>
            </owl:Class>
        </owl:equivalentClass>
        <rdfs:subClassOf rdf:resource="https://www.commoncoreontologies.org/ont00000995"/>
        <skos:definition xml:lang="en">An Artifact that is used by an Agent in a Cyber Attack to facilitate the realization of a Cyber Vulnerability.</skos:definition>
        <rdfs:label xml:lang="en">Cyber Exploit Artifact</rdfs:label>
        <cco2:ont00001760 rdf:datatype="http://www.w3.org/2001/XMLSchema#anyURI">http://www.ontologyrepository.com/CommonCoreOntologies/Domain/CyberOntology</cco2:ont00001760>
    </owl:Class>
    


    <!-- http://www.ontologyrepository.com/CommonCoreOntologies/CyberObjectiveSpecification -->

    <owl:Class rdf:about="http://www.ontologyrepository.com/CommonCoreOntologies/CyberObjectiveSpecification">
        <rdfs:subClassOf rdf:resource="https://www.commoncoreontologies.org/ont00000476"/>
        <skos:definition xml:lang="en">An Objective that prescribes a projected state that some Agent intends to achieve in cyberspace.</skos:definition>
        <skos:example xml:lang="en">Escalated privileges, Updated password.</skos:example>
        <rdfs:label xml:lang="en">Cyber Objective Specification</rdfs:label>
    </owl:Class>
    


    <!-- http://www.ontologyrepository.com/CommonCoreOntologies/CyberPlatform -->

    <owl:Class rdf:about="http://www.ontologyrepository.com/CommonCoreOntologies/CyberPlatform">
        <rdfs:subClassOf rdf:resource="http://purl.obolibrary.org/obo/BFO_0000027"/>
        <skos:definition xml:lang="en">An Object Aggregate which consists of an operating system and underlying hardware determining the physical environment in which software executes.</skos:definition>
        <rdfs:label xml:lang="en">Cyber Platform</rdfs:label>
        <cco2:ont00001760 rdf:datatype="http://www.w3.org/2001/XMLSchema#anyURI">http://www.ontologyrepository.com/CommonCoreOntologies/Domain/CyberOntology</cco2:ont00001760>
    </owl:Class>
    


    <!-- http://www.ontologyrepository.com/CommonCoreOntologies/CyberSecurityAdministratorRole -->

    <owl:Class rdf:about="http://www.ontologyrepository.com/CommonCoreOntologies/CyberSecurityAdministratorRole">
        <rdfs:subClassOf rdf:resource="http://www.ontologyrepository.com/CommonCoreOntologies/CyberSecurityRole"/>
        <skos:definition xml:lang="en">A Cyber Security Role that inheres in an Agent by virtue of its responsibility to ensure the network&apos;s security, protect against unauthorized access, modification, or destruction, and troubleshoot any access problems.</skos:definition>
        <rdfs:label xml:lang="en">Cyber Security Administrator Role</rdfs:label>
        <cco2:ont00001754 rdf:datatype="http://www.w3.org/2001/XMLSchema#anyURI">https://www.betterteam.com/security-administrator-job-description</cco2:ont00001754>
        <cco2:ont00001760 rdf:datatype="http://www.w3.org/2001/XMLSchema#anyURI">http://www.ontologyrepository.com/CommonCoreOntologies/Domain/CyberOntology</cco2:ont00001760>
    </owl:Class>
    


    <!-- http://www.ontologyrepository.com/CommonCoreOntologies/CyberSecurityAnalystRole -->

    <owl:Class rdf:about="http://www.ontologyrepository.com/CommonCoreOntologies/CyberSecurityAnalystRole">
        <rdfs:subClassOf rdf:resource="http://www.ontologyrepository.com/CommonCoreOntologies/CyberSecurityRole"/>
        <skos:definition xml:lang="en">A Cyber Security Role that inheres in an Agent by virtue of its responsibility to design and implement security systems to protect a company or organization’s computer networks from cyber attacks, and help set and maintain security standards.</skos:definition>
        <rdfs:label xml:lang="en">Cyber Security Analyst Role</rdfs:label>
        <cco2:ont00001754 rdf:datatype="http://www.w3.org/2001/XMLSchema#anyURI">https://www.betterteam.com/information-security-analyst-job-description</cco2:ont00001754>
        <cco2:ont00001760 rdf:datatype="http://www.w3.org/2001/XMLSchema#anyURI">http://www.ontologyrepository.com/CommonCoreOntologies/Domain/CyberOntology</cco2:ont00001760>
    </owl:Class>
    


    <!-- http://www.ontologyrepository.com/CommonCoreOntologies/CyberSecurityArchitectRole -->

    <owl:Class rdf:about="http://www.ontologyrepository.com/CommonCoreOntologies/CyberSecurityArchitectRole">
        <rdfs:subClassOf rdf:resource="http://www.ontologyrepository.com/CommonCoreOntologies/CyberSecurityRole"/>
        <skos:definition xml:lang="en">A Cyber Security Role that inheres in an Agent by virtue of its responsibility to design, build and oversee the implementation of network and computer security for an organization.</skos:definition>
        <rdfs:label xml:lang="en">Cyber Security Architect Role</rdfs:label>
        <cco2:ont00001754 rdf:datatype="http://www.w3.org/2001/XMLSchema#anyURI">https://www.cyberdegrees.org/jobs/security-architect/</cco2:ont00001754>
        <cco2:ont00001760 rdf:datatype="http://www.w3.org/2001/XMLSchema#anyURI">http://www.ontologyrepository.com/CommonCoreOntologies/Domain/CyberOntology</cco2:ont00001760>
    </owl:Class>
    


    <!-- http://www.ontologyrepository.com/CommonCoreOntologies/CyberSecurityConsultantRole -->

    <owl:Class rdf:about="http://www.ontologyrepository.com/CommonCoreOntologies/CyberSecurityConsultantRole">
        <rdfs:subClassOf rdf:resource="http://www.ontologyrepository.com/CommonCoreOntologies/CyberSecurityRole"/>
        <skos:definition xml:lang="en">A Cyber Security Role that inheres in an Agent by virtue of its responsibility to design and implement the best security solutions for an organization’s needs as well as talk to stakeholders, draw up budgets, supervise teams, and conduct research.</skos:definition>
        <rdfs:label xml:lang="en">Cyber Security Consultant Role</rdfs:label>
        <cco2:ont00001754 rdf:datatype="http://www.w3.org/2001/XMLSchema#anyURI">https://www.cyberdegrees.org/jobs/security-consultant/</cco2:ont00001754>
        <cco2:ont00001760 rdf:datatype="http://www.w3.org/2001/XMLSchema#anyURI">http://www.ontologyrepository.com/CommonCoreOntologies/Domain/CyberOntology</cco2:ont00001760>
    </owl:Class>
    


    <!-- http://www.ontologyrepository.com/CommonCoreOntologies/CyberSecurityEngineerRole -->

    <owl:Class rdf:about="http://www.ontologyrepository.com/CommonCoreOntologies/CyberSecurityEngineerRole">
        <rdfs:subClassOf rdf:resource="http://www.ontologyrepository.com/CommonCoreOntologies/CyberSecurityRole"/>
        <skos:definition xml:lang="en">A Cyber Security Role that inheres in an Agent by virtue of its responsibility to help businesses by protecting their computer and networking systems from potential hackers and cyber-attacks.</skos:definition>
        <rdfs:label xml:lang="en">Cyber Security Engineer Role</rdfs:label>
        <cco2:ont00001754 rdf:datatype="http://www.w3.org/2001/XMLSchema#anyURI">https://www.betterteam.com/cyber-security-engineer-job-description</cco2:ont00001754>
        <cco2:ont00001760 rdf:datatype="http://www.w3.org/2001/XMLSchema#anyURI">http://www.ontologyrepository.com/CommonCoreOntologies/Domain/CyberOntology</cco2:ont00001760>
    </owl:Class>
    


    <!-- http://www.ontologyrepository.com/CommonCoreOntologies/CyberSecurityProtectionPlan -->

    <owl:Class rdf:about="http://www.ontologyrepository.com/CommonCoreOntologies/CyberSecurityProtectionPlan">
        <rdfs:subClassOf rdf:resource="https://www.commoncoreontologies.org/ont00000974"/>
        <skos:altLabel xml:lang="en">Cyber Security Standard</skos:altLabel>
        <skos:definition xml:lang="en">A Plan that prescribes Acts which protect the cyber environment of a user or organization.</skos:definition>
        <rdfs:comment xml:lang="en">This environment includes users themselves, networks, devices, all software, processes, information in storage or transit, applications, services, and systems that can be connected directly or indirectly to networks.</rdfs:comment>
        <rdfs:label xml:lang="en">Cyber Security Protection Plan</rdfs:label>
        <cco2:ont00001754 rdf:datatype="http://www.w3.org/2001/XMLSchema#anyURI">https://en.wikipedia.org/wiki/Cyber_security_standards</cco2:ont00001754>
        <cco2:ont00001760 rdf:datatype="http://www.w3.org/2001/XMLSchema#anyURI">http://www.ontologyrepository.com/CommonCoreOntologies/Domain/CyberOntology</cco2:ont00001760>
    </owl:Class>
    


    <!-- http://www.ontologyrepository.com/CommonCoreOntologies/CyberSecurityRole -->

    <owl:Class rdf:about="http://www.ontologyrepository.com/CommonCoreOntologies/CyberSecurityRole">
        <rdfs:subClassOf rdf:resource="http://purl.obolibrary.org/obo/BFO_0000023"/>
        <skos:definition xml:lang="en">A Role that is realized in an Act wherein its bearer attempts to prevent and mitigate Cyber Attacks.</skos:definition>
        <rdfs:label xml:lang="en">Cyber Security Role</rdfs:label>
        <cco2:ont00001760 rdf:datatype="http://www.w3.org/2001/XMLSchema#anyURI">http://www.ontologyrepository.com/CommonCoreOntologies/Domain/CyberOntology</cco2:ont00001760>
    </owl:Class>
    


    <!-- http://www.ontologyrepository.com/CommonCoreOntologies/CyberSecuritySoftwareDeveloperRole -->

    <owl:Class rdf:about="http://www.ontologyrepository.com/CommonCoreOntologies/CyberSecuritySoftwareDeveloperRole">
        <rdfs:subClassOf rdf:resource="http://www.ontologyrepository.com/CommonCoreOntologies/CyberSecurityRole"/>
        <skos:definition xml:lang="en">A Cyber Security Role that inheres in an Agent by virtue of its responsibility to develop security software and integrates security into applications software during the course of design and development.</skos:definition>
        <rdfs:label xml:lang="en">Cyber Security Software Developer Role</rdfs:label>
        <cco2:ont00001754 rdf:datatype="http://www.w3.org/2001/XMLSchema#anyURI">https://www.cyberdegrees.org/jobs/security-software-developer/</cco2:ont00001754>
        <cco2:ont00001760 rdf:datatype="http://www.w3.org/2001/XMLSchema#anyURI">http://www.ontologyrepository.com/CommonCoreOntologies/Domain/CyberOntology</cco2:ont00001760>
    </owl:Class>
    


    <!-- http://www.ontologyrepository.com/CommonCoreOntologies/CyberThreatNominalMeasurement -->

    <owl:Class rdf:about="http://www.ontologyrepository.com/CommonCoreOntologies/CyberThreatNominalMeasurement">
        <rdfs:subClassOf rdf:resource="https://www.commoncoreontologies.org/ont00000293"/>
        <skos:definition xml:lang="en">A Nominal Measurement Information Content Entity that is about the potential impact of a Cyber Vulnerability when realized in a Cyber Attack.</skos:definition>
        <rdfs:label xml:lang="en">Cyber Threat Nominal Measurement</rdfs:label>
        <cco2:ont00001760 rdf:datatype="http://www.w3.org/2001/XMLSchema#anyURI">http://www.ontologyrepository.com/CommonCoreOntologies/Domain/CyberOntology</cco2:ont00001760>
    </owl:Class>
    


    <!-- http://www.ontologyrepository.com/CommonCoreOntologies/CyberVulnerability -->

    <owl:Class rdf:about="http://www.ontologyrepository.com/CommonCoreOntologies/CyberVulnerability">
        <rdfs:subClassOf rdf:resource="https://www.commoncoreontologies.org/ont00000548"/>
        <rdfs:subClassOf>
            <owl:Class>
                <owl:intersectionOf rdf:parseType="Collection">
                    <owl:Restriction>
                        <owl:onProperty rdf:resource="http://purl.obolibrary.org/obo/BFO_0000054"/>
                        <owl:someValuesFrom rdf:resource="http://www.ontologyrepository.com/CommonCoreOntologies/CyberAttack"/>
                    </owl:Restriction>
                    <owl:Restriction>
                        <owl:onProperty rdf:resource="http://purl.obolibrary.org/obo/BFO_0000054"/>
                        <owl:allValuesFrom rdf:resource="http://www.ontologyrepository.com/CommonCoreOntologies/CyberAttack"/>
                    </owl:Restriction>
                </owl:intersectionOf>
            </owl:Class>
        </rdfs:subClassOf>
        <skos:altLabel xml:lang="en">Common Software Weakness</skos:altLabel>
        <skos:definition xml:lang="en">A Vulnerability that is realized by a Cyber Attack interfering with or destroying a device&apos;s ability to function normally.</skos:definition>
        <rdfs:label xml:lang="en">Cyber Vulnerability</rdfs:label>
        <rdfs:seeAlso rdf:datatype="http://www.w3.org/2001/XMLSchema#anyURI">https://cwe.mitre.org/about/index.html</rdfs:seeAlso>
        <cco2:ont00001760 rdf:datatype="http://www.w3.org/2001/XMLSchema#anyURI">http://www.ontologyrepository.com/CommonCoreOntologies/Domain/CyberOntology</cco2:ont00001760>
    </owl:Class>
    


    <!-- http://www.ontologyrepository.com/CommonCoreOntologies/CybersecurityAct -->

    <owl:Class rdf:about="http://www.ontologyrepository.com/CommonCoreOntologies/CybersecurityAct">
        <rdfs:subClassOf rdf:resource="http://www.ontologyrepository.com/CommonCoreOntologies/CyberAct"/>
        <terms:creator xml:lang="en">CUBRC Inc</terms:creator>
        <skos:altLabel xml:lang="en">Cybersecurity Event</skos:altLabel>
        <skos:definition xml:lang="en">A Cyber Act that affects the security of a Computer Network or the information residing therein.</skos:definition>
        <rdfs:comment xml:lang="en">‘Security’ is most likely a realizable entity that inheres in its bearer (in this case, a Computer Network) and gets realized by various processes. NOTE: defining &apos;Security&apos; or &apos;Cybersecurity&apos; is necessary in order to create an equivalency axiom for &apos;Cybersecurity Act&apos;.</rdfs:comment>
        <rdfs:label xml:lang="en">Cybersecurity Act</rdfs:label>
        <cco2:ont00001754 rdf:datatype="http://www.w3.org/2001/XMLSchema#anyURI">https://csrc.nist.gov/glossary/term/cybersecurity_event</cco2:ont00001754>
        <cco2:ont00001754 rdf:datatype="http://www.w3.org/2001/XMLSchema#anyURI">https://www.bitlyft.com/resources/security-incident-vs-event-what-is-the-difference</cco2:ont00001754>
        <cco2:ont00001760 rdf:datatype="http://www.w3.org/2001/XMLSchema#anyURI">http://www.ontologyrepository.com/CommonCoreOntologies/Domain/CyberOntology</cco2:ont00001760>
    </owl:Class>
    


    <!-- http://www.ontologyrepository.com/CommonCoreOntologies/CybersecurityIncident -->

    <owl:Class rdf:about="http://www.ontologyrepository.com/CommonCoreOntologies/CybersecurityIncident">
        <owl:equivalentClass>
            <owl:Class>
                <owl:intersectionOf rdf:parseType="Collection">
                    <rdf:Description rdf:about="http://www.ontologyrepository.com/CommonCoreOntologies/CybersecurityAct"/>
                    <owl:Restriction>
                        <owl:onProperty rdf:resource="https://www.commoncoreontologies.org/ont00001803"/>
                        <owl:someValuesFrom rdf:resource="https://www.commoncoreontologies.org/ont00001289"/>
                    </owl:Restriction>
                </owl:intersectionOf>
            </owl:Class>
        </owl:equivalentClass>
        <rdfs:subClassOf rdf:resource="http://www.ontologyrepository.com/CommonCoreOntologies/CybersecurityAct"/>
        <terms:creator xml:lang="en">CUBRC Inc</terms:creator>
        <skos:altLabel xml:lang="en">Cyber Attack Consequence</skos:altLabel>
        <skos:definition xml:lang="en">A Cybersecurity Act that causes an adverse effect to a Computer Network, the information residing therein, or its authorized users or owners.</skos:definition>
        <skos:example xml:lang="en">a data breach or data spill</skos:example>
        <skos:example xml:lang="en">the outcome of a successful cyber attack</skos:example>
        <rdfs:comment xml:lang="en">TO DO: Add a term(s) for Confidentiality, Integrity, and Accessibility (CIA) of data. Then use these terms to refine the definition of Cybersecurity Incident.

This is needed because scoping the range of consequences that make a Cyber Act qualify as a Cybersecurity Incident is challenging. For example, consider a scenario where a major credit reporting agency experiences a data breach/spill that affects millions of people but at least some of those people are not owners/users/etc. of that database. Damage is done and this should be typed as a Cybersecurity Incident, but how do we capture these &quot;outside&quot; agents without making the definition too broad? For example, we probably don&apos;t want to include cyber bullying that causes real world harm as Cybersecurity Incidents.</rdfs:comment>
        <rdfs:label xml:lang="en">Cybersecurity Incident</rdfs:label>
        <cco2:ont00001754 rdf:datatype="http://www.w3.org/2001/XMLSchema#anyURI">https://csrc.nist.gov/glossary/term/cyber_incident</cco2:ont00001754>
        <cco2:ont00001754 rdf:datatype="http://www.w3.org/2001/XMLSchema#anyURI">https://www.bitlyft.com/resources/security-incident-vs-event-what-is-the-difference</cco2:ont00001754>
        <cco2:ont00001760 rdf:datatype="http://www.w3.org/2001/XMLSchema#anyURI">http://www.ontologyrepository.com/CommonCoreOntologies/Domain/CyberOntology</cco2:ont00001760>
    </owl:Class>
    


    <!-- http://www.ontologyrepository.com/CommonCoreOntologies/CybersecurityInfraction -->

    <owl:Class rdf:about="http://www.ontologyrepository.com/CommonCoreOntologies/CybersecurityInfraction">
        <owl:equivalentClass>
            <owl:Class>
                <owl:intersectionOf rdf:parseType="Collection">
                    <rdf:Description rdf:about="http://www.ontologyrepository.com/CommonCoreOntologies/CybersecurityAct"/>
                    <owl:Restriction>
                        <owl:onProperty rdf:resource="https://www.commoncoreontologies.org/ont00001803"/>
                        <owl:someValuesFrom>
                            <owl:Class>
                                <owl:intersectionOf rdf:parseType="Collection">
                                    <owl:Class>
                                        <owl:unionOf rdf:parseType="Collection">
                                            <rdf:Description rdf:about="https://www.commoncoreontologies.org/ont00000609"/>
                                            <rdf:Description rdf:about="https://www.commoncoreontologies.org/ont00001356"/>
                                        </owl:unionOf>
                                    </owl:Class>
                                    <owl:Restriction>
                                        <owl:onProperty rdf:resource="https://www.commoncoreontologies.org/ont00001778"/>
                                        <owl:someValuesFrom rdf:resource="http://www.ontologyrepository.com/CommonCoreOntologies/CyberVulnerability"/>
                                    </owl:Restriction>
                                </owl:intersectionOf>
                            </owl:Class>
                        </owl:someValuesFrom>
                    </owl:Restriction>
                </owl:intersectionOf>
            </owl:Class>
        </owl:equivalentClass>
        <rdfs:subClassOf rdf:resource="http://www.ontologyrepository.com/CommonCoreOntologies/CybersecurityAct"/>
        <terms:creator xml:lang="en">CUBRC Inc</terms:creator>
        <skos:altLabel xml:lang="en">Cybersecurity Escape</skos:altLabel>
        <skos:definition xml:lang="en">A Cybersecurity Act that decreases the security of a Computer Network by creating a new Cyber Vulnerability or increasing an existing Cyber Vulnerability that inheres in that Computer Network.</skos:definition>
        <rdfs:comment xml:lang="en">This class is designed to disambiguate between Cyber Acts that MIGHT cause damage (i.e., Cybersecurity Infraction) from Cyber Acts that DO cause damage (i.e., Cybersecurity Incident).</rdfs:comment>
        <skos:example xml:lang="en">creating a weak password or reusing passwords</skos:example>
        <skos:example xml:lang="en">failing to set appropriate network access permissions</skos:example>
        <skos:example xml:lang="en">leaving a networked device unlocked and unattended in a public space</skos:example>
        <rdfs:label xml:lang="en">Cybersecurity Infraction</rdfs:label>
        <cco2:ont00001760 rdf:datatype="http://www.w3.org/2001/XMLSchema#anyURI">http://www.ontologyrepository.com/CommonCoreOntologies/Domain/CyberOntology</cco2:ont00001760>
    </owl:Class>
    


    <!-- http://www.ontologyrepository.com/CommonCoreOntologies/CybersecurityProcess -->

    <owl:Class rdf:about="http://www.ontologyrepository.com/CommonCoreOntologies/CybersecurityProcess">
        <owl:equivalentClass>
            <owl:Class>
                <owl:intersectionOf rdf:parseType="Collection">
                    <rdf:Description rdf:about="http://www.ontologyrepository.com/CommonCoreOntologies/CybersecurityAct"/>
                    <owl:Restriction>
                        <owl:onProperty rdf:resource="https://www.commoncoreontologies.org/ont00001803"/>
                        <owl:someValuesFrom>
                            <owl:Class>
                                <owl:intersectionOf rdf:parseType="Collection">
                                    <owl:Class>
                                        <owl:unionOf rdf:parseType="Collection">
                                            <rdf:Description rdf:about="https://www.commoncoreontologies.org/ont00000543"/>
                                            <rdf:Description rdf:about="https://www.commoncoreontologies.org/ont00001066"/>
                                        </owl:unionOf>
                                    </owl:Class>
                                    <owl:Restriction>
                                        <owl:onProperty rdf:resource="https://www.commoncoreontologies.org/ont00001778"/>
                                        <owl:someValuesFrom rdf:resource="http://www.ontologyrepository.com/CommonCoreOntologies/CyberVulnerability"/>
                                    </owl:Restriction>
                                </owl:intersectionOf>
                            </owl:Class>
                        </owl:someValuesFrom>
                    </owl:Restriction>
                </owl:intersectionOf>
            </owl:Class>
        </owl:equivalentClass>
        <rdfs:subClassOf rdf:resource="http://www.ontologyrepository.com/CommonCoreOntologies/CybersecurityAct"/>
        <terms:creator xml:lang="en">CUBRC Inc</terms:creator>
        <skos:definition xml:lang="en">A Cybersecurity Act that is performed to increase the security of a Computer Network.</skos:definition>
        <skos:example xml:lang="en">a password verification process intended to prevent the creation of weak passwords</skos:example>
        <skos:example xml:lang="en">deploying a firewall for a computer network</skos:example>
        <skos:example xml:lang="en">running a malware scan</skos:example>
        <rdfs:label xml:lang="en">Cybersecurity Process</rdfs:label>
        <cco2:ont00001754 rdf:datatype="http://www.w3.org/2001/XMLSchema#anyURI">https://csrc.nist.gov/glossary/term/cybersecurity</cco2:ont00001754>
        <cco2:ont00001754 rdf:datatype="http://www.w3.org/2001/XMLSchema#anyURI">https://nvlpubs.nist.gov/nistpubs/CSWP/NIST.CSWP.04162018.pdf</cco2:ont00001754>
        <cco2:ont00001760 rdf:datatype="http://www.w3.org/2001/XMLSchema#anyURI">http://www.ontologyrepository.com/CommonCoreOntologies/Domain/CyberOntology</cco2:ont00001760>
    </owl:Class>
    


    <!-- http://www.ontologyrepository.com/CommonCoreOntologies/CybersecurityViolation -->

    <owl:Class rdf:about="http://www.ontologyrepository.com/CommonCoreOntologies/CybersecurityViolation">
        <rdfs:subClassOf rdf:resource="http://www.ontologyrepository.com/CommonCoreOntologies/CybersecurityAct"/>
        <terms:creator xml:lang="en">CUBRC Inc</terms:creator>
        <skos:definition xml:lang="en">A Cybersecurity Act that violates the Computer Network owner&apos;s Cybersecurity Policy.</skos:definition>
        <rdfs:comment xml:lang="en">Cybersecurity Violations are differentiated from Cybersecurity Infractions because violations are specific to organizational policies. Not every act that violates a Cybersecurity Policy necessarily has a negative effect on the security of a Computer Network. Similarly, it is unlikely that any given Cybersecurity Policy is capable of documenting every possible action that would negatively affect a Computer Network. Hence, these classes are distinct despite having many instances in common.</rdfs:comment>
        <skos:example xml:lang="en">failing to follow the exact steps outlined by the security policy for a procedure</skos:example>
        <skos:example xml:lang="en">plugging an unapproved device into a company computer</skos:example>
        <skos:example xml:lang="en">using a secure information system to access a personal social media account</skos:example>
        <rdfs:comment xml:lang="en">Creating an equivalency axiom for Cybersecurity Violation requires creating a term such as &apos;Cybersecurity Policy&apos;.</rdfs:comment>
        <rdfs:label xml:lang="en">Cybersecurity Violation</rdfs:label>
        <cco2:ont00001760 rdf:datatype="http://www.w3.org/2001/XMLSchema#anyURI">http://www.ontologyrepository.com/CommonCoreOntologies/Domain/CyberOntology</cco2:ont00001760>
    </owl:Class>
    


    <!-- http://www.ontologyrepository.com/CommonCoreOntologies/DHCPServiceFunction -->

    <owl:Class rdf:about="http://www.ontologyrepository.com/CommonCoreOntologies/DHCPServiceFunction">
        <rdfs:subClassOf rdf:resource="http://www.ontologyrepository.com/CommonCoreOntologies/NetworkServiceFunction"/>
        <skos:altLabel xml:lang="en">DHCP Service</skos:altLabel>
        <skos:definition xml:lang="en">A Network Service Function that when realized is in a process of dynamically assigning an Internet Protocol Address and other network configuration parameters to devices on a Computer Network.</skos:definition>
        <rdfs:label xml:lang="en">DHCP Service Function</rdfs:label>
        <cco2:ont00001754>https://en.wikipedia.org/wiki/Dynamic_Host_Configuration_Protocol</cco2:ont00001754>
        <cco2:ont00001760 rdf:datatype="http://www.w3.org/2001/XMLSchema#anyURI">http://www.ontologyrepository.com/CommonCoreOntologies/Domain/CyberOntology</cco2:ont00001760>
    </owl:Class>
    


    <!-- http://www.ontologyrepository.com/CommonCoreOntologies/DNSServiceFunction -->

    <owl:Class rdf:about="http://www.ontologyrepository.com/CommonCoreOntologies/DNSServiceFunction">
        <rdfs:subClassOf rdf:resource="http://www.ontologyrepository.com/CommonCoreOntologies/NetworkServiceFunction"/>
        <skos:altLabel xml:lang="en">DNS Service</skos:altLabel>
        <skos:definition xml:lang="en">A Network Service Function that when relized is in a process of translating Domain Names to the Internet Protocol Addresses needed for locating and identifying computer services and devices on a Computer Network.</skos:definition>
        <rdfs:label xml:lang="en">DNS Service Function</rdfs:label>
        <cco2:ont00001754>https://en.wikipedia.org/wiki/Domain_Name_System</cco2:ont00001754>
        <cco2:ont00001760 rdf:datatype="http://www.w3.org/2001/XMLSchema#anyURI">http://www.ontologyrepository.com/CommonCoreOntologies/Domain/CyberOntology</cco2:ont00001760>
    </owl:Class>
    


    <!-- http://www.ontologyrepository.com/CommonCoreOntologies/DarkNetwork -->

    <owl:Class rdf:about="http://www.ontologyrepository.com/CommonCoreOntologies/DarkNetwork">
        <rdfs:subClassOf rdf:resource="http://www.ontologyrepository.com/CommonCoreOntologies/OverlayNetwork"/>
        <rdfs:subClassOf>
            <owl:Restriction>
                <owl:onProperty rdf:resource="http://purl.obolibrary.org/obo/BFO_0000056"/>
                <owl:someValuesFrom rdf:resource="http://www.ontologyrepository.com/CommonCoreOntologies/Authentication"/>
            </owl:Restriction>
        </rdfs:subClassOf>
        <skos:definition xml:lang="en">An Overlay Network that can be accessed only with specific software, configurations, or authorization, often using non-standard communications protocols or ports.</skos:definition>
        <rdfs:label xml:lang="en">Dark Network</rdfs:label>
        <cco2:ont00001754>https://en.wikipedia.org/wiki/Darknet</cco2:ont00001754>
        <cco2:ont00001760 rdf:datatype="http://www.w3.org/2001/XMLSchema#anyURI">http://www.ontologyrepository.com/CommonCoreOntologies/Domain/CyberOntology</cco2:ont00001760>
    </owl:Class>
    


    <!-- http://www.ontologyrepository.com/CommonCoreOntologies/DataBuffer -->

    <owl:Class rdf:about="http://www.ontologyrepository.com/CommonCoreOntologies/DataBuffer">
        <rdfs:subClassOf rdf:resource="http://www.ontologyrepository.com/CommonCoreOntologies/ComputerMemoryLocation"/>
        <skos:definition xml:lang="en">A Computer Memory Location that is designed to temporarily store data while it is being moved from one place to another.</skos:definition>
        <rdfs:label xml:lang="en">Data Buffer</rdfs:label>
        <cco2:ont00001754>https://en.wikipedia.org/wiki/Data_buffer</cco2:ont00001754>
        <cco2:ont00001760 rdf:datatype="http://www.w3.org/2001/XMLSchema#anyURI">http://www.ontologyrepository.com/CommonCoreOntologies/Domain/CyberOntology</cco2:ont00001760>
    </owl:Class>
    


    <!-- http://www.ontologyrepository.com/CommonCoreOntologies/DataColumn -->

    <owl:Class rdf:about="http://www.ontologyrepository.com/CommonCoreOntologies/DataColumn">
        <rdfs:subClassOf rdf:resource="http://www.ontologyrepository.com/CommonCoreOntologies/Tuple"/>
        <skos:definition xml:lang="en">A Tuple that structures information vertically within a Matrix.</skos:definition>
        <rdfs:label xml:lang="en">Data Column</rdfs:label>
        <cco2:ont00001760 rdf:datatype="http://www.w3.org/2001/XMLSchema#anyURI">http://www.ontologyrepository.com/CommonCoreOntologies/Domain/CyberOntology</cco2:ont00001760>
    </owl:Class>
    


    <!-- http://www.ontologyrepository.com/CommonCoreOntologies/DataDestructionAttack -->

    <owl:Class rdf:about="http://www.ontologyrepository.com/CommonCoreOntologies/DataDestructionAttack">
        <rdfs:subClassOf rdf:resource="http://www.ontologyrepository.com/CommonCoreOntologies/CyberAttack"/>
        <skos:definition xml:lang="en">A Cyber Attack that results in the modification of tapes, hard disks, and other forms of electronic media, such that the Information Content Entities encoded on them cannot be accessed, read, or used.</skos:definition>
        <rdfs:label xml:lang="en">Data Destruction Attack</rdfs:label>
        <cco2:ont00001754 rdf:datatype="http://www.w3.org/2001/XMLSchema#anyURI">https://searchstorage.techtarget.com/definition/data-destruction</cco2:ont00001754>
        <cco2:ont00001760 rdf:datatype="http://www.w3.org/2001/XMLSchema#anyURI">http://www.ontologyrepository.com/CommonCoreOntologies/Domain/CyberOntology</cco2:ont00001760>
    </owl:Class>
    


    <!-- http://www.ontologyrepository.com/CommonCoreOntologies/DataExchangeLanguage -->

    <owl:Class rdf:about="http://www.ontologyrepository.com/CommonCoreOntologies/DataExchangeLanguage">
        <rdfs:subClassOf rdf:resource="http://www.ontologyrepository.com/CommonCoreOntologies/ComputerLanguage"/>
        <skos:definition xml:lang="en">A Computer Language that prescribes a way of communicating information between multiple Computer Programs in a common format.</skos:definition>
        <rdfs:label xml:lang="en">Data Exchange Language</rdfs:label>
        <cco2:ont00001754>https://en.wikipedia.org/wiki/Data_exchange</cco2:ont00001754>
        <cco2:ont00001760 rdf:datatype="http://www.w3.org/2001/XMLSchema#anyURI">http://www.ontologyrepository.com/CommonCoreOntologies/Domain/CyberOntology</cco2:ont00001760>
    </owl:Class>
    


    <!-- http://www.ontologyrepository.com/CommonCoreOntologies/DataOffsetDesignator -->

    <owl:Class rdf:about="http://www.ontologyrepository.com/CommonCoreOntologies/DataOffsetDesignator">
        <rdfs:subClassOf rdf:resource="https://www.commoncoreontologies.org/ont00001022"/>
        <skos:definition xml:lang="en">A Ratio Measurement Content Entity that is a measurement of the size of an Information Header in number of Bits.</skos:definition>
        <rdfs:label xml:lang="en">Data Offset Measurement</rdfs:label>
        <cco2:ont00001760 rdf:datatype="http://www.w3.org/2001/XMLSchema#anyURI">http://www.ontologyrepository.com/CommonCoreOntologies/Domain/CyberOntology</cco2:ont00001760>
    </owl:Class>
    


    <!-- http://www.ontologyrepository.com/CommonCoreOntologies/DataProcessingStack -->

    <owl:Class rdf:about="http://www.ontologyrepository.com/CommonCoreOntologies/DataProcessingStack">
        <rdfs:subClassOf rdf:resource="http://www.ontologyrepository.com/CommonCoreOntologies/SoftwareStack"/>
        <skos:definition xml:lang="en">A Software Stack that enables the validation, sorting, summation, aggregation, analysis, reporting, and classification of Information Content Entities.</skos:definition>
        <rdfs:label xml:lang="en">Data Processing Stack</rdfs:label>
        <cco2:ont00001754>https://en.wikipedia.org/wiki/Data_processing</cco2:ont00001754>
        <cco2:ont00001760 rdf:datatype="http://www.w3.org/2001/XMLSchema#anyURI">http://www.ontologyrepository.com/CommonCoreOntologies/Domain/CyberOntology</cco2:ont00001760>
    </owl:Class>
    


    <!-- http://www.ontologyrepository.com/CommonCoreOntologies/DataRequest -->

    <owl:Class rdf:about="http://www.ontologyrepository.com/CommonCoreOntologies/DataRequest">
        <rdfs:subClassOf rdf:resource="http://www.ontologyrepository.com/CommonCoreOntologies/DataTransfer"/>
        <skos:definition xml:lang="en">A Data Transfer in which a sender requests some data from the receiver of that request.</skos:definition>
        <rdfs:label xml:lang="en">Data Request</rdfs:label>
        <cco2:ont00001760 rdf:datatype="http://www.w3.org/2001/XMLSchema#anyURI">http://www.ontologyrepository.com/CommonCoreOntologies/Domain/CyberOntology</cco2:ont00001760>
    </owl:Class>
    


    <!-- http://www.ontologyrepository.com/CommonCoreOntologies/DataRequestAcknowledgement -->

    <owl:Class rdf:about="http://www.ontologyrepository.com/CommonCoreOntologies/DataRequestAcknowledgement">
        <rdfs:subClassOf rdf:resource="http://www.ontologyrepository.com/CommonCoreOntologies/DataTransfer"/>
        <skos:definition xml:lang="en">A Data Transfer in which the receiver of a Data Request sends an acknowledgment that the request has been received.</skos:definition>
        <rdfs:label xml:lang="en">Data Request Acknowledgement</rdfs:label>
        <cco2:ont00001760 rdf:datatype="http://www.w3.org/2001/XMLSchema#anyURI">http://www.ontologyrepository.com/CommonCoreOntologies/Domain/CyberOntology</cco2:ont00001760>
    </owl:Class>
    


    <!-- http://www.ontologyrepository.com/CommonCoreOntologies/DataRow -->

    <owl:Class rdf:about="http://www.ontologyrepository.com/CommonCoreOntologies/DataRow">
        <rdfs:subClassOf rdf:resource="http://www.ontologyrepository.com/CommonCoreOntologies/Tuple"/>
        <skos:definition xml:lang="en">A Tuple that structures information horizontally within a Matrix.</skos:definition>
        <rdfs:label xml:lang="en">Data Row</rdfs:label>
        <cco2:ont00001760 rdf:datatype="http://www.w3.org/2001/XMLSchema#anyURI">http://www.ontologyrepository.com/CommonCoreOntologies/Domain/CyberOntology</cco2:ont00001760>
    </owl:Class>
    


    <!-- http://www.ontologyrepository.com/CommonCoreOntologies/DataSynchronizationUtility -->

    <owl:Class rdf:about="http://www.ontologyrepository.com/CommonCoreOntologies/DataSynchronizationUtility">
        <rdfs:subClassOf rdf:resource="http://www.ontologyrepository.com/CommonCoreOntologies/UtilityProgram"/>
        <skos:definition xml:lang="en">A Utility Program that is designed to establish consistency among data from a source to a target data storage and vice versa, and the continuous harmonization of the data over time</skos:definition>
        <rdfs:label xml:lang="en">Data Synchronization Utility</rdfs:label>
        <cco2:ont00001754>https://en.wikipedia.org/wiki/Data_synchronization</cco2:ont00001754>
        <cco2:ont00001760 rdf:datatype="http://www.w3.org/2001/XMLSchema#anyURI">http://www.ontologyrepository.com/CommonCoreOntologies/Domain/CyberOntology</cco2:ont00001760>
    </owl:Class>
    


    <!-- http://www.ontologyrepository.com/CommonCoreOntologies/DataTable -->

    <owl:Class rdf:about="http://www.ontologyrepository.com/CommonCoreOntologies/DataTable">
        <rdfs:subClassOf rdf:resource="http://www.ontologyrepository.com/CommonCoreOntologies/Matrix"/>
        <rdfs:subClassOf>
            <owl:Restriction>
                <owl:onProperty rdf:resource="http://purl.obolibrary.org/obo/BFO_0000178"/>
                <owl:someValuesFrom rdf:resource="http://www.ontologyrepository.com/CommonCoreOntologies/DataColumn"/>
            </owl:Restriction>
        </rdfs:subClassOf>
        <skos:definition xml:lang="en">A Matrix which consists of Data Rows and Data Columns.</skos:definition>
        <rdfs:label xml:lang="en">Data Table</rdfs:label>
        <cco2:ont00001760 rdf:datatype="http://www.w3.org/2001/XMLSchema#anyURI">http://www.ontologyrepository.com/CommonCoreOntologies/Domain/CyberOntology</cco2:ont00001760>
    </owl:Class>
    


    <!-- http://www.ontologyrepository.com/CommonCoreOntologies/DataTransfer -->

    <owl:Class rdf:about="http://www.ontologyrepository.com/CommonCoreOntologies/DataTransfer">
        <rdfs:subClassOf rdf:resource="http://www.ontologyrepository.com/CommonCoreOntologies/ComputerProgramExecution"/>
        <skos:definition xml:lang="en">A Computer Program Execution in which an Information Content Entity inhering in some Information Bearing Entity is sent to some other Information Bearing Entity, which now bears that Information Content Entity.</skos:definition>
        <rdfs:label xml:lang="en">Data Transfer</rdfs:label>
        <cco2:ont00001760 rdf:datatype="http://www.w3.org/2001/XMLSchema#anyURI">http://www.ontologyrepository.com/CommonCoreOntologies/Domain/CyberOntology</cco2:ont00001760>
    </owl:Class>
    


    <!-- http://www.ontologyrepository.com/CommonCoreOntologies/DatabaseSoftwareApplication -->

    <owl:Class rdf:about="http://www.ontologyrepository.com/CommonCoreOntologies/DatabaseSoftwareApplication">
        <rdfs:subClassOf rdf:resource="http://www.ontologyrepository.com/CommonCoreOntologies/InformationWorkerSoftware"/>
        <skos:altLabel xml:lang="en">Database Management System</skos:altLabel>
        <skos:definition xml:lang="en">An Information Worker Software Application that is designed to enable a user to create, edit, and query a Database.</skos:definition>
        <rdfs:label xml:lang="en">Database Software Application</rdfs:label>
        <cco2:ont00001760 rdf:datatype="http://www.w3.org/2001/XMLSchema#anyURI">http://www.ontologyrepository.com/CommonCoreOntologies/Domain/CyberOntology</cco2:ont00001760>
    </owl:Class>
    


    <!-- http://www.ontologyrepository.com/CommonCoreOntologies/DatabaseSoftwareApplicationModel -->

    <owl:Class rdf:about="http://www.ontologyrepository.com/CommonCoreOntologies/DatabaseSoftwareApplicationModel">
        <rdfs:subClassOf rdf:resource="http://www.ontologyrepository.com/CommonCoreOntologies/ComputerProgramArtifactModel"/>
        <rdfs:subClassOf>
            <owl:Restriction>
                <owl:onProperty rdf:resource="https://www.commoncoreontologies.org/ont00001942"/>
                <owl:someValuesFrom rdf:resource="http://www.ontologyrepository.com/CommonCoreOntologies/DatabaseSoftwareApplication"/>
            </owl:Restriction>
        </rdfs:subClassOf>
        <skos:definition xml:lang="en">A Computer Program Artifact Model that prescribes some Database Software Application.</skos:definition>
        <rdfs:label xml:lang="en">Database Software Application Model</rdfs:label>
        <cco2:ont00001760 rdf:datatype="http://www.w3.org/2001/XMLSchema#anyURI">http://www.ontologyrepository.com/CommonCoreOntologies/Domain/CyberOntology</cco2:ont00001760>
    </owl:Class>
    


    <!-- http://www.ontologyrepository.com/CommonCoreOntologies/DefaultStasis -->

    <owl:Class rdf:about="http://www.ontologyrepository.com/CommonCoreOntologies/DefaultStasis">
        <rdfs:subClassOf rdf:resource="https://www.commoncoreontologies.org/ont00001213"/>
        <skos:definition xml:lang="en">A Stasis of Artifact Operationality in which an Artifact&apos;s functions are configured to some preselected settings.</skos:definition>
        <rdfs:label xml:lang="en">Default Stasis</rdfs:label>
        <cco2:ont00001760 rdf:datatype="http://www.w3.org/2001/XMLSchema#anyURI">http://www.ontologyrepository.com/CommonCoreOntologies/Domain/CyberOntology</cco2:ont00001760>
    </owl:Class>
    


    <!-- http://www.ontologyrepository.com/CommonCoreOntologies/DenialOfService -->

    <owl:Class rdf:about="http://www.ontologyrepository.com/CommonCoreOntologies/DenialOfService">
        <rdfs:subClassOf rdf:resource="http://www.ontologyrepository.com/CommonCoreOntologies/CyberAttack"/>
        <skos:altLabel xml:lang="en">DoS</skos:altLabel>
        <skos:definition xml:lang="en">A Cyber Attack in which some Agent seeks to make a machine or network resource unavailable to its intended users by temporarily or indefinitely disrupting services of a host connected to a Computer Network.</skos:definition>
        <rdfs:label xml:lang="en">Denial of Service</rdfs:label>
        <cco2:ont00001754>https://en.wikipedia.org/wiki/Denial-of-service_attack</cco2:ont00001754>
        <cco2:ont00001760 rdf:datatype="http://www.w3.org/2001/XMLSchema#anyURI">http://www.ontologyrepository.com/CommonCoreOntologies/Domain/CyberOntology</cco2:ont00001760>
    </owl:Class>
    


    <!-- http://www.ontologyrepository.com/CommonCoreOntologies/DesignationSpecification -->

    <owl:Class rdf:about="http://www.ontologyrepository.com/CommonCoreOntologies/DesignationSpecification">
        <rdfs:subClassOf rdf:resource="https://www.commoncoreontologies.org/ont00000965"/>
        <skos:definition xml:lang="en">A Directive Information Content Entity that prescribes how some entities should be designated.</skos:definition>
        <skos:example>Domain Name System</skos:example>
        <rdfs:label xml:lang="en">Designation Specification</rdfs:label>
        <cco2:ont00001760 rdf:datatype="http://www.w3.org/2001/XMLSchema#anyURI">http://www.ontologyrepository.com/CommonCoreOntologies/Domain/CyberOntology</cco2:ont00001760>
    </owl:Class>
    


    <!-- http://www.ontologyrepository.com/CommonCoreOntologies/DesktopComputer -->

    <owl:Class rdf:about="http://www.ontologyrepository.com/CommonCoreOntologies/DesktopComputer">
        <rdfs:subClassOf rdf:resource="https://www.commoncoreontologies.org/ont00000420"/>
        <skos:definition xml:lang="en">A Computer that is designed not to be portable.</skos:definition>
        <rdfs:label xml:lang="en">Desktop Computer</rdfs:label>
        <cco2:ont00001760 rdf:datatype="http://www.w3.org/2001/XMLSchema#anyURI">http://www.ontologyrepository.com/CommonCoreOntologies/Domain/CyberOntology</cco2:ont00001760>
    </owl:Class>
    


    <!-- http://www.ontologyrepository.com/CommonCoreOntologies/Digit -->

    <owl:Class rdf:about="http://www.ontologyrepository.com/CommonCoreOntologies/Digit">
        <rdfs:subClassOf rdf:resource="http://www.ontologyrepository.com/CommonCoreOntologies/Grapheme"/>
        <skos:definition xml:lang="en">A Grapheme that is used either in isolation or combination to represent a number in positional numeral systems.</skos:definition>
        <rdfs:label xml:lang="en">Digit</rdfs:label>
        <cco2:ont00001754>https://en.wikipedia.org/wiki/Numerical_digit</cco2:ont00001754>
        <cco2:ont00001760 rdf:datatype="http://www.w3.org/2001/XMLSchema#anyURI">http://www.ontologyrepository.com/CommonCoreOntologies/Domain/CyberOntology</cco2:ont00001760>
    </owl:Class>
    


    <!-- http://www.ontologyrepository.com/CommonCoreOntologies/DigitalClipboard -->

    <owl:Class rdf:about="http://www.ontologyrepository.com/CommonCoreOntologies/DigitalClipboard">
        <rdfs:subClassOf rdf:resource="http://www.ontologyrepository.com/CommonCoreOntologies/DataBuffer"/>
        <skos:altLabel xml:lang="en">Paste Buffer</skos:altLabel>
        <skos:definition xml:lang="en">A Data Buffer that is designed to temporarily store data which is being transferred between Documents or Software Applications.</skos:definition>
        <rdfs:label xml:lang="en">Digital Clipboard</rdfs:label>
        <cco2:ont00001760 rdf:datatype="http://www.w3.org/2001/XMLSchema#anyURI">http://www.ontologyrepository.com/CommonCoreOntologies/Domain/CyberOntology</cco2:ont00001760>
    </owl:Class>
    


    <!-- http://www.ontologyrepository.com/CommonCoreOntologies/DigitalFile -->

    <owl:Class rdf:about="http://www.ontologyrepository.com/CommonCoreOntologies/DigitalFile">
        <rdfs:subClassOf rdf:resource="https://www.commoncoreontologies.org/ont00000798"/>
        <rdfs:subClassOf>
            <owl:Restriction>
                <owl:onProperty rdf:resource="http://purl.obolibrary.org/obo/BFO_0000171"/>
                <owl:someValuesFrom rdf:resource="https://www.commoncoreontologies.org/ont00001179"/>
            </owl:Restriction>
        </rdfs:subClassOf>
        <skos:definition xml:lang="en">An Information Bearing Artifact that consist of a one-dimensional array of bytes on a Digital Storage Device, and which is designed to be easily opened, read, changed, and closed by an Information Processing Artifact.</skos:definition>
        <rdfs:label xml:lang="en">Digital File</rdfs:label>
        <cco2:ont00001760 rdf:datatype="http://www.w3.org/2001/XMLSchema#anyURI">http://www.ontologyrepository.com/CommonCoreOntologies/Domain/CyberOntology</cco2:ont00001760>
    </owl:Class>
    


    <!-- http://www.ontologyrepository.com/CommonCoreOntologies/DigitalFileHeader -->

    <owl:Class rdf:about="http://www.ontologyrepository.com/CommonCoreOntologies/DigitalFileHeader">
        <rdfs:subClassOf rdf:resource="http://www.ontologyrepository.com/CommonCoreOntologies/InformationHeader"/>
        <rdfs:subClassOf>
            <owl:Restriction>
                <owl:onProperty rdf:resource="http://purl.obolibrary.org/obo/BFO_0000176"/>
                <owl:someValuesFrom rdf:resource="http://www.ontologyrepository.com/CommonCoreOntologies/DigitalFile"/>
            </owl:Restriction>
        </rdfs:subClassOf>
        <skos:definition xml:lang="en">An Information Header that is part of a Digital File.</skos:definition>
        <rdfs:label xml:lang="en">Digital File Header</rdfs:label>
        <cco2:ont00001760 rdf:datatype="http://www.w3.org/2001/XMLSchema#anyURI">http://www.ontologyrepository.com/CommonCoreOntologies/Domain/CyberOntology</cco2:ont00001760>
    </owl:Class>
    


    <!-- http://www.ontologyrepository.com/CommonCoreOntologies/DigitalFileManagementFunction -->

    <owl:Class rdf:about="http://www.ontologyrepository.com/CommonCoreOntologies/DigitalFileManagementFunction">
        <rdfs:subClassOf rdf:resource="http://www.ontologyrepository.com/CommonCoreOntologies/InformationProcessingArtifactFunction"/>
        <skos:definition xml:lang="en">An Information Processing Artifact Function that when realized is in a process of creating, accessing, and managing Digital Files.</skos:definition>
        <rdfs:label xml:lang="en">Digital File Management Function</rdfs:label>
        <cco2:ont00001760 rdf:datatype="http://www.w3.org/2001/XMLSchema#anyURI">http://www.ontologyrepository.com/CommonCoreOntologies/Domain/CyberOntology</cco2:ont00001760>
    </owl:Class>
    


    <!-- http://www.ontologyrepository.com/CommonCoreOntologies/DigitalFileProcess -->

    <owl:Class rdf:about="http://www.ontologyrepository.com/CommonCoreOntologies/DigitalFileProcess">
        <rdfs:subClassOf rdf:resource="http://www.ontologyrepository.com/CommonCoreOntologies/ComputerProgramExecution"/>
        <skos:definition xml:lang="en">A Computer Program Execution that opens, closes, reads, or writes a Digital File.</skos:definition>
        <rdfs:label xml:lang="en">Digital File Process</rdfs:label>
        <cco2:ont00001760 rdf:datatype="http://www.w3.org/2001/XMLSchema#anyURI">http://www.ontologyrepository.com/CommonCoreOntologies/Domain/CyberOntology</cco2:ont00001760>
    </owl:Class>
    


    <!-- http://www.ontologyrepository.com/CommonCoreOntologies/DigitalFileSystem -->

    <owl:Class rdf:about="http://www.ontologyrepository.com/CommonCoreOntologies/DigitalFileSystem">
        <rdfs:subClassOf rdf:resource="http://purl.obolibrary.org/obo/BFO_0000027"/>
        <skos:altLabel xml:lang="en">Physical File System</skos:altLabel>
        <rdfs:label xml:lang="en">Digital File System</rdfs:label>
        <cco2:ont00001754>https://en.wikipedia.org/wiki/File_system</cco2:ont00001754>
        <cco2:ont00001760 rdf:datatype="http://www.w3.org/2001/XMLSchema#anyURI">http://www.ontologyrepository.com/CommonCoreOntologies/Domain/CyberOntology</cco2:ont00001760>
    </owl:Class>
    


    <!-- http://www.ontologyrepository.com/CommonCoreOntologies/DigitalObject -->

    <owl:Class rdf:about="http://www.ontologyrepository.com/CommonCoreOntologies/DigitalObject">
        <rdfs:subClassOf rdf:resource="https://www.commoncoreontologies.org/ont00000798"/>
        <skos:definition xml:lang="en">An Information Bearing Artifact that is designed to bear a collection of related values.</skos:definition>
        <rdfs:label xml:lang="en">Digital Object</rdfs:label>
        <cco2:ont00001760 rdf:datatype="http://www.w3.org/2001/XMLSchema#anyURI">http://www.ontologyrepository.com/CommonCoreOntologies/Domain/CyberOntology</cco2:ont00001760>
    </owl:Class>
    


    <!-- http://www.ontologyrepository.com/CommonCoreOntologies/DiskChecker -->

    <owl:Class rdf:about="http://www.ontologyrepository.com/CommonCoreOntologies/DiskChecker">
        <rdfs:subClassOf rdf:resource="http://www.ontologyrepository.com/CommonCoreOntologies/UtilityProgram"/>
        <skos:definition xml:lang="en">A Utility Program that is designed to scan a Hard Disk Drive to file Digital Files that are corrupted in some way.</skos:definition>
        <rdfs:label xml:lang="en">Disk Checker</rdfs:label>
        <cco2:ont00001754>https://en.wikipedia.org/wiki/Disk_utility#Disk_checkers</cco2:ont00001754>
        <cco2:ont00001760 rdf:datatype="http://www.w3.org/2001/XMLSchema#anyURI">http://www.ontologyrepository.com/CommonCoreOntologies/Domain/CyberOntology</cco2:ont00001760>
    </owl:Class>
    


    <!-- http://www.ontologyrepository.com/CommonCoreOntologies/DiskCleaner -->

    <owl:Class rdf:about="http://www.ontologyrepository.com/CommonCoreOntologies/DiskCleaner">
        <rdfs:subClassOf rdf:resource="http://www.ontologyrepository.com/CommonCoreOntologies/UtilityProgram"/>
        <skos:definition xml:lang="en">A Utility Program that is designed to find and delete potentially unnecessary or potentially unwanted Digital Files from a Hard Disk Drive.</skos:definition>
        <rdfs:label xml:lang="en">Disk Cleaner</rdfs:label>
        <cco2:ont00001754>https://en.wikipedia.org/wiki/Disk_utility#Disk_cleaners</cco2:ont00001754>
        <cco2:ont00001760 rdf:datatype="http://www.w3.org/2001/XMLSchema#anyURI">http://www.ontologyrepository.com/CommonCoreOntologies/Domain/CyberOntology</cco2:ont00001760>
    </owl:Class>
    


    <!-- http://www.ontologyrepository.com/CommonCoreOntologies/DiskCompressionUtility -->

    <owl:Class rdf:about="http://www.ontologyrepository.com/CommonCoreOntologies/DiskCompressionUtility">
        <rdfs:subClassOf rdf:resource="http://www.ontologyrepository.com/CommonCoreOntologies/UtilityProgram"/>
        <skos:definition xml:lang="en">A Utility Program that is designed to increases the amount of information that can be stored on a Hard Disk Drive.</skos:definition>
        <rdfs:label xml:lang="en">Disk Compression Utility</rdfs:label>
        <cco2:ont00001754>https://en.wikipedia.org/wiki/Disk_compression</cco2:ont00001754>
        <cco2:ont00001760 rdf:datatype="http://www.w3.org/2001/XMLSchema#anyURI">http://www.ontologyrepository.com/CommonCoreOntologies/Domain/CyberOntology</cco2:ont00001760>
    </owl:Class>
    


    <!-- http://www.ontologyrepository.com/CommonCoreOntologies/DiskDefragmenter -->

    <owl:Class rdf:about="http://www.ontologyrepository.com/CommonCoreOntologies/DiskDefragmenter">
        <rdfs:subClassOf rdf:resource="http://www.ontologyrepository.com/CommonCoreOntologies/UtilityProgram"/>
        <skos:definition xml:lang="en">A Utility Program that is designed to reduce the extent to which Digital Files are stored non-contiguously on a Hard Disk Drive.</skos:definition>
        <rdfs:label xml:lang="en">Disk Defragmenter</rdfs:label>
        <cco2:ont00001754>https://en.wikipedia.org/wiki/Defragmentation</cco2:ont00001754>
        <cco2:ont00001760 rdf:datatype="http://www.w3.org/2001/XMLSchema#anyURI">http://www.ontologyrepository.com/CommonCoreOntologies/Domain/CyberOntology</cco2:ont00001760>
    </owl:Class>
    


    <!-- http://www.ontologyrepository.com/CommonCoreOntologies/DiskPartitionEditor -->

    <owl:Class rdf:about="http://www.ontologyrepository.com/CommonCoreOntologies/DiskPartitionEditor">
        <rdfs:subClassOf rdf:resource="http://www.ontologyrepository.com/CommonCoreOntologies/UtilityProgram"/>
        <skos:definition xml:lang="en">A Utility Program that is designed to divide an individual Hard Disk Drive into multiple logical drives, each with its own Digital File System which can be mounted by the Operating System and treated as an individual drive.</skos:definition>
        <rdfs:label xml:lang="en">Disk Partition Editor</rdfs:label>
        <cco2:ont00001754>https://en.wikipedia.org/wiki/Disk_partitioning</cco2:ont00001754>
        <cco2:ont00001760 rdf:datatype="http://www.w3.org/2001/XMLSchema#anyURI">http://www.ontologyrepository.com/CommonCoreOntologies/Domain/CyberOntology</cco2:ont00001760>
    </owl:Class>
    


    <!-- http://www.ontologyrepository.com/CommonCoreOntologies/DiskSpaceAnalyzer -->

    <owl:Class rdf:about="http://www.ontologyrepository.com/CommonCoreOntologies/DiskSpaceAnalyzer">
        <rdfs:subClassOf rdf:resource="http://www.ontologyrepository.com/CommonCoreOntologies/UtilityProgram"/>
        <skos:definition xml:lang="en">A Utility Program that is designed to visualize disk space usage by getting the size for each folder (including sub-folders) and files in a folder or drive.</skos:definition>
        <rdfs:label xml:lang="en">Disk Space Analyzer</rdfs:label>
        <cco2:ont00001754>https://en.wikipedia.org/wiki/Disk_utility#Disk_space_analyzers</cco2:ont00001754>
        <cco2:ont00001760 rdf:datatype="http://www.w3.org/2001/XMLSchema#anyURI">http://www.ontologyrepository.com/CommonCoreOntologies/Domain/CyberOntology</cco2:ont00001760>
    </owl:Class>
    


    <!-- http://www.ontologyrepository.com/CommonCoreOntologies/DistributedControlSystem -->

    <owl:Class rdf:about="http://www.ontologyrepository.com/CommonCoreOntologies/DistributedControlSystem">
        <rdfs:subClassOf rdf:resource="https://www.commoncoreontologies.org/ont00000781"/>
        <skos:definition xml:lang="en">A Control System in which autonomous controllers are distributed throughout the system, but there is a central operator supervisory control.</skos:definition>
        <rdfs:label xml:lang="en">Distributed Control System</rdfs:label>
        <cco2:ont00001754>https://en.wikipedia.org/wiki/Distributed_control_system</cco2:ont00001754>
        <cco2:ont00001760 rdf:datatype="http://www.w3.org/2001/XMLSchema#anyURI">http://www.ontologyrepository.com/CommonCoreOntologies/Domain/CyberOntology</cco2:ont00001760>
    </owl:Class>
    


    <!-- http://www.ontologyrepository.com/CommonCoreOntologies/DocumentStoreDatabaseSoftwareApplicationModel -->

    <owl:Class rdf:about="http://www.ontologyrepository.com/CommonCoreOntologies/DocumentStoreDatabaseSoftwareApplicationModel">
        <rdfs:subClassOf rdf:resource="http://www.ontologyrepository.com/CommonCoreOntologies/KeyValueDatabaseSoftwareApplicationModel"/>
        <skos:definition xml:lang="en">A Key-Value Database Software Application Model that prescribes some Database Software Application where the stored values are documents whose contents are accesible via the sructure of the document itself.</skos:definition>
        <rdfs:label xml:lang="en">Document Store Database Software Application Model</rdfs:label>
        <cco2:ont00001760 rdf:datatype="http://www.w3.org/2001/XMLSchema#anyURI">http://www.ontologyrepository.com/CommonCoreOntologies/Domain/CyberOntology</cco2:ont00001760>
    </owl:Class>
    


    <!-- http://www.ontologyrepository.com/CommonCoreOntologies/DomainName -->

    <owl:Class rdf:about="http://www.ontologyrepository.com/CommonCoreOntologies/DomainName">
        <rdfs:subClassOf rdf:resource="https://www.commoncoreontologies.org/ont00000077"/>
        <skos:definition xml:lang="en">A Code Identifier that designates a resource on a Computer Network according to the rules of the Domain Name System.</skos:definition>
        <rdfs:comment xml:lang="en">A domain name might designate a personal computer, a server, a web site, or other web service. Generally, one of the purposes of a domain name is designate a computer resource while hiding the (less human friendly) IP address from end users.</rdfs:comment>
        <skos:example>www.google.com</skos:example>
        <rdfs:label xml:lang="en">Domain Name</rdfs:label>
        <cco2:ont00001754>https://en.wikipedia.org/wiki/Domain_name</cco2:ont00001754>
        <cco2:ont00001760 rdf:datatype="http://www.w3.org/2001/XMLSchema#anyURI">http://www.ontologyrepository.com/CommonCoreOntologies/Domain/CyberOntology</cco2:ont00001760>
    </owl:Class>
    


    <!-- http://www.ontologyrepository.com/CommonCoreOntologies/DomainNameRegistrar -->

    <owl:Class rdf:about="http://www.ontologyrepository.com/CommonCoreOntologies/DomainNameRegistrar">
        <rdfs:subClassOf rdf:resource="https://www.commoncoreontologies.org/ont00001180"/>
        <skos:definition xml:lang="en">An Organization that manages the reservation of Internet Domain Names.</skos:definition>
        <rdfs:label xml:lang="en">Domain Name Registrar</rdfs:label>
        <cco2:ont00001754>https://en.wikipedia.org/wiki/Domain_name_registrar</cco2:ont00001754>
        <cco2:ont00001760 rdf:datatype="http://www.w3.org/2001/XMLSchema#anyURI">http://www.ontologyrepository.com/CommonCoreOntologies/Domain/CyberOntology</cco2:ont00001760>
    </owl:Class>
    


    <!-- http://www.ontologyrepository.com/CommonCoreOntologies/DomainWatchlist -->

    <owl:Class rdf:about="http://www.ontologyrepository.com/CommonCoreOntologies/DomainWatchlist">
        <rdfs:subClassOf rdf:resource="http://www.ontologyrepository.com/CommonCoreOntologies/Watchlist"/>
        <skos:definition xml:lang="en">A Watchlist which prescribes which Domain Names require close surveillance.</skos:definition>
        <rdfs:label xml:lang="en">Domain Watchlist</rdfs:label>
        <cco2:ont00001760 rdf:datatype="http://www.w3.org/2001/XMLSchema#anyURI">http://www.ontologyrepository.com/CommonCoreOntologies/Domain/CyberOntology</cco2:ont00001760>
    </owl:Class>
    


    <!-- http://www.ontologyrepository.com/CommonCoreOntologies/DownloadingProcess -->

    <owl:Class rdf:about="http://www.ontologyrepository.com/CommonCoreOntologies/DownloadingProcess">
        <rdfs:subClassOf rdf:resource="http://www.ontologyrepository.com/CommonCoreOntologies/FileTransfer"/>
        <skos:definition xml:lang="en">A File Transfer in which a Computer File is retrieved from some remote Computer and stored on some user&apos;s local Computer.</skos:definition>
        <rdfs:label xml:lang="en">Downloading Process</rdfs:label>
        <cco2:ont00001760 rdf:datatype="http://www.w3.org/2001/XMLSchema#anyURI">http://www.ontologyrepository.com/CommonCoreOntologies/Domain/CyberOntology</cco2:ont00001760>
    </owl:Class>
    


    <!-- http://www.ontologyrepository.com/CommonCoreOntologies/DrivingSimulator -->

    <owl:Class rdf:about="http://www.ontologyrepository.com/CommonCoreOntologies/DrivingSimulator">
        <rdfs:subClassOf rdf:resource="http://www.ontologyrepository.com/CommonCoreOntologies/VehicleSimulator"/>
        <skos:definition xml:lang="en">A Vehicle Simulator that is designed to enable a user to model the process of driving an Automobile.</skos:definition>
        <rdfs:label xml:lang="en">Driving Simulator</rdfs:label>
        <cco2:ont00001760 rdf:datatype="http://www.w3.org/2001/XMLSchema#anyURI">http://www.ontologyrepository.com/CommonCoreOntologies/Domain/CyberOntology</cco2:ont00001760>
    </owl:Class>
    


    <!-- http://www.ontologyrepository.com/CommonCoreOntologies/DynamicDNSService -->

    <owl:Class rdf:about="http://www.ontologyrepository.com/CommonCoreOntologies/DynamicDNSService">
        <rdfs:subClassOf rdf:resource="http://www.ontologyrepository.com/CommonCoreOntologies/UtilityProgram"/>
        <rdfs:subClassOf>
            <owl:Restriction>
                <owl:onProperty rdf:resource="http://purl.obolibrary.org/obo/BFO_0000196"/>
                <owl:someValuesFrom rdf:resource="http://www.ontologyrepository.com/CommonCoreOntologies/NetworkServiceFunction"/>
            </owl:Restriction>
        </rdfs:subClassOf>
        <skos:altLabel xml:lang="en">DDNS</skos:altLabel>
        <skos:definition xml:lang="en">A Utility Program that automatically updates a Domain Name in the Domain Name System with a new IP Address.</skos:definition>
        <rdfs:label xml:lang="en">Dynamic DNS Service</rdfs:label>
        <cco2:ont00001754>https://en.wikipedia.org/wiki/Dynamic_DNS</cco2:ont00001754>
        <cco2:ont00001760 rdf:datatype="http://www.w3.org/2001/XMLSchema#anyURI">http://www.ontologyrepository.com/CommonCoreOntologies/Domain/CyberOntology</cco2:ont00001760>
    </owl:Class>
    


    <!-- http://www.ontologyrepository.com/CommonCoreOntologies/ElectromagneticPulseVulnerability -->

    <owl:Class rdf:about="http://www.ontologyrepository.com/CommonCoreOntologies/ElectromagneticPulseVulnerability">
        <rdfs:subClassOf rdf:resource="https://www.commoncoreontologies.org/ont00000548"/>
        <rdfs:subClassOf>
            <owl:Restriction>
                <owl:onProperty rdf:resource="http://purl.obolibrary.org/obo/BFO_0000054"/>
                <owl:allValuesFrom rdf:resource="https://www.commoncoreontologies.org/ont00000812"/>
            </owl:Restriction>
        </rdfs:subClassOf>
        <skos:altLabel xml:lang="en">EMP Vulnerability</skos:altLabel>
        <skos:definition xml:lang="en">A Vulnerability that is realized by an Electromagnetic Pulse disrupting, damaging, or destroying one or more capabilities of an Artifact.</skos:definition>
        <rdfs:label xml:lang="en">Electromagnetic Pulse Vulnerability</rdfs:label>
        <cco2:ont00001760 rdf:datatype="http://www.w3.org/2001/XMLSchema#anyURI">http://www.ontologyrepository.com/CommonCoreOntologies/Domain/CyberOntology</cco2:ont00001760>
    </owl:Class>
    


    <!-- http://www.ontologyrepository.com/CommonCoreOntologies/EmailMessageHeader -->

    <owl:Class rdf:about="http://www.ontologyrepository.com/CommonCoreOntologies/EmailMessageHeader">
        <rdfs:subClassOf rdf:resource="http://www.ontologyrepository.com/CommonCoreOntologies/InformationHeader"/>
        <skos:definition xml:lang="en">An Information Header that is part of some Email Message.</skos:definition>
        <rdfs:label xml:lang="en">Email Message Header</rdfs:label>
        <cco2:ont00001760 rdf:datatype="http://www.w3.org/2001/XMLSchema#anyURI">http://www.ontologyrepository.com/CommonCoreOntologies/Domain/CyberOntology</cco2:ont00001760>
    </owl:Class>
    


    <!-- http://www.ontologyrepository.com/CommonCoreOntologies/EmailSoftwareApplication -->

    <owl:Class rdf:about="http://www.ontologyrepository.com/CommonCoreOntologies/EmailSoftwareApplication">
        <rdfs:subClassOf rdf:resource="http://www.ontologyrepository.com/CommonCoreOntologies/InformationWorkerSoftware"/>
        <skos:definition xml:lang="en">An Information Worker Software Application that is designed to enable a user to compose, edit, send, and receive Email Messages.</skos:definition>
        <rdfs:label xml:lang="en">Email Software Application</rdfs:label>
        <cco2:ont00001760 rdf:datatype="http://www.w3.org/2001/XMLSchema#anyURI">http://www.ontologyrepository.com/CommonCoreOntologies/Domain/CyberOntology</cco2:ont00001760>
    </owl:Class>
    


    <!-- http://www.ontologyrepository.com/CommonCoreOntologies/EmergencySimulator -->

    <owl:Class rdf:about="http://www.ontologyrepository.com/CommonCoreOntologies/EmergencySimulator">
        <rdfs:subClassOf rdf:resource="http://www.ontologyrepository.com/CommonCoreOntologies/SimulationSoftware"/>
        <skos:definition xml:lang="en">Simulation Software that is designed to enable a user to model an emergency situation.</skos:definition>
        <rdfs:label xml:lang="en">Emergency Simulator</rdfs:label>
        <cco2:ont00001760 rdf:datatype="http://www.w3.org/2001/XMLSchema#anyURI">http://www.ontologyrepository.com/CommonCoreOntologies/Domain/CyberOntology</cco2:ont00001760>
    </owl:Class>
    


    <!-- http://www.ontologyrepository.com/CommonCoreOntologies/Emulator -->

    <owl:Class rdf:about="http://www.ontologyrepository.com/CommonCoreOntologies/Emulator">
        <rdfs:subClassOf rdf:resource="https://www.commoncoreontologies.org/ont00000117"/>
        <skos:definition xml:lang="en">An Information Processing Artifact that is designed to use some combination of hardware and software to simulate the behavior of another Information Processing Artifact.</skos:definition>
        <rdfs:label xml:lang="en">Emulator</rdfs:label>
        <cco2:ont00001760 rdf:datatype="http://www.w3.org/2001/XMLSchema#anyURI">http://www.ontologyrepository.com/CommonCoreOntologies/Domain/CyberOntology</cco2:ont00001760>
    </owl:Class>
    


    <!-- http://www.ontologyrepository.com/CommonCoreOntologies/EncodingScheme -->

    <owl:Class rdf:about="http://www.ontologyrepository.com/CommonCoreOntologies/EncodingScheme">
        <rdfs:subClassOf rdf:resource="https://www.commoncoreontologies.org/ont00000653"/>
        <skos:definition xml:lang="en">An Algorithm that prescribes how an Information Content Entity in one format can be converted into another format.</skos:definition>
        <rdfs:label xml:lang="en">Encoding Scheme</rdfs:label>
        <cco2:ont00001754>https://en.wikipedia.org/wiki/Code</cco2:ont00001754>
        <cco2:ont00001760 rdf:datatype="http://www.w3.org/2001/XMLSchema#anyURI">http://www.ontologyrepository.com/CommonCoreOntologies/Domain/CyberOntology</cco2:ont00001760>
    </owl:Class>
    


    <!-- http://www.ontologyrepository.com/CommonCoreOntologies/EncryptedFile -->

    <owl:Class rdf:about="http://www.ontologyrepository.com/CommonCoreOntologies/EncryptedFile">
        <rdfs:subClassOf rdf:resource="http://www.ontologyrepository.com/CommonCoreOntologies/DigitalFile"/>
        <skos:definition xml:lang="en">A Digital File that has been encoded using some Encryption Algorithm.</skos:definition>
        <rdfs:label xml:lang="en">Encrypted File</rdfs:label>
        <cco2:ont00001760 rdf:datatype="http://www.w3.org/2001/XMLSchema#anyURI">http://www.ontologyrepository.com/CommonCoreOntologies/Domain/CyberOntology</cco2:ont00001760>
    </owl:Class>
    


    <!-- http://www.ontologyrepository.com/CommonCoreOntologies/Encryption -->

    <owl:Class rdf:about="http://www.ontologyrepository.com/CommonCoreOntologies/Encryption">
        <rdfs:subClassOf rdf:resource="http://www.ontologyrepository.com/CommonCoreOntologies/ComputerProgramExecution"/>
        <skos:definition xml:lang="en">A Computer Program Execution in which the content of an Information Bearing Entity is rendered unintelligible to unauthorized accessors.</skos:definition>
        <rdfs:label xml:lang="en">Encryption</rdfs:label>
        <cco2:ont00001760 rdf:datatype="http://www.w3.org/2001/XMLSchema#anyURI">http://www.ontologyrepository.com/CommonCoreOntologies/Domain/CyberOntology</cco2:ont00001760>
    </owl:Class>
    


    <!-- http://www.ontologyrepository.com/CommonCoreOntologies/EncryptionAlgorithm -->

    <owl:Class rdf:about="http://www.ontologyrepository.com/CommonCoreOntologies/EncryptionAlgorithm">
        <rdfs:subClassOf rdf:resource="http://www.ontologyrepository.com/CommonCoreOntologies/EncodingScheme"/>
        <skos:definition xml:lang="en">An Encoding Scheme that prescribes how an Information Content Entity in some intelligible format can be converted into a format in such a way that only authorizes parties can access it.</skos:definition>
        <rdfs:label xml:lang="en">Encryption Algorithm</rdfs:label>
        <cco2:ont00001754>https://en.wikipedia.org/wiki/Encryption</cco2:ont00001754>
        <cco2:ont00001760 rdf:datatype="http://www.w3.org/2001/XMLSchema#anyURI">http://www.ontologyrepository.com/CommonCoreOntologies/Domain/CyberOntology</cco2:ont00001760>
    </owl:Class>
    


    <!-- http://www.ontologyrepository.com/CommonCoreOntologies/EthernetCord -->

    <owl:Class rdf:about="http://www.ontologyrepository.com/CommonCoreOntologies/EthernetCord">
        <rdfs:subClassOf rdf:resource="https://www.commoncoreontologies.org/ont00000825"/>
        <skos:definition xml:lang="en">A Telecommunication Network Line that is designed to support connections over a Computer Network by means of coaxial cables as a shared medium, or twisted pair and fiber optic links in conjunction with Hubs or Switches.</skos:definition>
        <rdfs:label xml:lang="en">Ethernet Cord</rdfs:label>
        <cco2:ont00001754>https://en.wikipedia.org/wiki/Ethernet</cco2:ont00001754>
        <cco2:ont00001760 rdf:datatype="http://www.w3.org/2001/XMLSchema#anyURI">http://www.ontologyrepository.com/CommonCoreOntologies/Domain/CyberOntology</cco2:ont00001760>
    </owl:Class>
    


    <!-- http://www.ontologyrepository.com/CommonCoreOntologies/ExecutableFile -->

    <owl:Class rdf:about="http://www.ontologyrepository.com/CommonCoreOntologies/ExecutableFile">
        <rdfs:subClassOf rdf:resource="http://www.ontologyrepository.com/CommonCoreOntologies/DigitalFile"/>
        <skos:definition xml:lang="en">A Digital File that can be directly executed by a Processing Unit.</skos:definition>
        <rdfs:comment xml:lang="en">An executable file does not need to be parsed by a computer program in order to be meaningful (e.g., because it has been compiled).</rdfs:comment>
        <skos:example>A .exe file</skos:example>
        <skos:example>A .jar file</skos:example>
        <rdfs:label xml:lang="en">Executable File</rdfs:label>
        <cco2:ont00001754>https://en.wikipedia.org/wiki/Executable</cco2:ont00001754>
        <cco2:ont00001760 rdf:datatype="http://www.w3.org/2001/XMLSchema#anyURI">http://www.ontologyrepository.com/CommonCoreOntologies/Domain/CyberOntology</cco2:ont00001760>
    </owl:Class>
    


    <!-- http://www.ontologyrepository.com/CommonCoreOntologies/ExecuteFilePermission -->

    <owl:Class rdf:about="http://www.ontologyrepository.com/CommonCoreOntologies/ExecuteFilePermission">
        <rdfs:subClassOf rdf:resource="http://www.ontologyrepository.com/CommonCoreOntologies/FilePermission"/>
        <skos:definition xml:lang="en">A File Permission that prescribes the operating system to run program code for a user account.</skos:definition>
        <rdfs:label xml:lang="en">Execute File Permission</rdfs:label>
        <cco2:ont00001754 rdf:datatype="http://www.w3.org/2001/XMLSchema#anyURI">https://en.wikipedia.org/wiki/File_system_permissions</cco2:ont00001754>
        <cco2:ont00001760 rdf:datatype="http://www.w3.org/2001/XMLSchema#anyURI">http://www.ontologyrepository.com/CommonCoreOntologies/Domain/CyberOntology</cco2:ont00001760>
    </owl:Class>
    


    <!-- http://www.ontologyrepository.com/CommonCoreOntologies/FileAppending -->

    <owl:Class rdf:about="http://www.ontologyrepository.com/CommonCoreOntologies/FileAppending">
        <rdfs:subClassOf rdf:resource="http://www.ontologyrepository.com/CommonCoreOntologies/DigitalFileProcess"/>
        <skos:definition xml:lang="en">A Digital File Process that adds content to an existing Digital File.</skos:definition>
        <rdfs:label xml:lang="en">File Appending</rdfs:label>
        <cco2:ont00001760 rdf:datatype="http://www.w3.org/2001/XMLSchema#anyURI">http://www.ontologyrepository.com/CommonCoreOntologies/Domain/CyberOntology</cco2:ont00001760>
    </owl:Class>
    


    <!-- http://www.ontologyrepository.com/CommonCoreOntologies/FileArchiver -->

    <owl:Class rdf:about="http://www.ontologyrepository.com/CommonCoreOntologies/FileArchiver">
        <rdfs:subClassOf rdf:resource="http://www.ontologyrepository.com/CommonCoreOntologies/UtilityProgram"/>
        <skos:definition xml:lang="en">A Utility Program that combines a number of files together into one archive file, or a series of archive files, for easier transportation or storage.</skos:definition>
        <rdfs:label xml:lang="en">File Archiver</rdfs:label>
        <cco2:ont00001754>https://en.wikipedia.org/wiki/File_archiver</cco2:ont00001754>
        <cco2:ont00001760 rdf:datatype="http://www.w3.org/2001/XMLSchema#anyURI">http://www.ontologyrepository.com/CommonCoreOntologies/Domain/CyberOntology</cco2:ont00001760>
    </owl:Class>
    


    <!-- http://www.ontologyrepository.com/CommonCoreOntologies/FileClosing -->

    <owl:Class rdf:about="http://www.ontologyrepository.com/CommonCoreOntologies/FileClosing">
        <rdfs:subClassOf rdf:resource="http://www.ontologyrepository.com/CommonCoreOntologies/DigitalFileProcess"/>
        <skos:definition xml:lang="en">A Digital File Process that makes a Digital File unavailable for modification.</skos:definition>
        <rdfs:label xml:lang="en">File Closing</rdfs:label>
        <cco2:ont00001760 rdf:datatype="http://www.w3.org/2001/XMLSchema#anyURI">http://www.ontologyrepository.com/CommonCoreOntologies/Domain/CyberOntology</cco2:ont00001760>
    </owl:Class>
    


    <!-- http://www.ontologyrepository.com/CommonCoreOntologies/FileCompressor -->

    <owl:Class rdf:about="http://www.ontologyrepository.com/CommonCoreOntologies/FileCompressor">
        <rdfs:subClassOf rdf:resource="http://www.ontologyrepository.com/CommonCoreOntologies/FileArchiver"/>
        <skos:definition xml:lang="en">A File Archiver that is designed to encode the information in a Digital File in a way which uses fewer Bits than its original encoding.</skos:definition>
        <skos:example>A gzip application</skos:example>
        <rdfs:label xml:lang="en">File Compressor</rdfs:label>
        <cco2:ont00001760 rdf:datatype="http://www.w3.org/2001/XMLSchema#anyURI">http://www.ontologyrepository.com/CommonCoreOntologies/Domain/CyberOntology</cco2:ont00001760>
    </owl:Class>
    


    <!-- http://www.ontologyrepository.com/CommonCoreOntologies/FileFormat -->

    <owl:Class rdf:about="http://www.ontologyrepository.com/CommonCoreOntologies/FileFormat">
        <rdfs:subClassOf rdf:resource="https://www.commoncoreontologies.org/ont00000965"/>
        <skos:definition xml:lang="en">A Directive Information Content Entity that prescribes how Bits are used to encode some Information Content Entity in some Digital Storage Device.</skos:definition>
        <rdfs:label xml:lang="en">File Format</rdfs:label>
        <cco2:ont00001754>https://en.wikipedia.org/wiki/File_format</cco2:ont00001754>
        <cco2:ont00001760 rdf:datatype="http://www.w3.org/2001/XMLSchema#anyURI">http://www.ontologyrepository.com/CommonCoreOntologies/Domain/CyberOntology</cco2:ont00001760>
    </owl:Class>
    


    <!-- http://www.ontologyrepository.com/CommonCoreOntologies/FileManager -->

    <owl:Class rdf:about="http://www.ontologyrepository.com/CommonCoreOntologies/FileManager">
        <rdfs:subClassOf rdf:resource="http://www.ontologyrepository.com/CommonCoreOntologies/UtilityProgram"/>
        <skos:definition xml:lang="en">A Utility Program that is designed to provide a user interface to manage Digital Files and File System Directories.</skos:definition>
        <rdfs:label xml:lang="en">File Manager</rdfs:label>
        <cco2:ont00001760 rdf:datatype="http://www.w3.org/2001/XMLSchema#anyURI">http://www.ontologyrepository.com/CommonCoreOntologies/Domain/CyberOntology</cco2:ont00001760>
    </owl:Class>
    


    <!-- http://www.ontologyrepository.com/CommonCoreOntologies/FileOpening -->

    <owl:Class rdf:about="http://www.ontologyrepository.com/CommonCoreOntologies/FileOpening">
        <rdfs:subClassOf rdf:resource="http://www.ontologyrepository.com/CommonCoreOntologies/DigitalFileProcess"/>
        <skos:definition xml:lang="en">A Digital File Process that makes a Digital File available for modification.</skos:definition>
        <rdfs:label xml:lang="en">File Opening</rdfs:label>
        <cco2:ont00001760 rdf:datatype="http://www.w3.org/2001/XMLSchema#anyURI">http://www.ontologyrepository.com/CommonCoreOntologies/Domain/CyberOntology</cco2:ont00001760>
    </owl:Class>
    


    <!-- http://www.ontologyrepository.com/CommonCoreOntologies/FilePermission -->

    <owl:Class rdf:about="http://www.ontologyrepository.com/CommonCoreOntologies/FilePermission">
        <rdfs:subClassOf rdf:resource="https://www.commoncoreontologies.org/ont00000751"/>
        <skos:definition xml:lang="en">An Action Permission that prescribes the file system access of user accounts.</skos:definition>
        <rdfs:label xml:lang="en">File Permission</rdfs:label>
        <cco2:ont00001754 rdf:datatype="http://www.w3.org/2001/XMLSchema#anyURI">https://en.wikipedia.org/wiki/File_system_permissions</cco2:ont00001754>
        <cco2:ont00001760 rdf:datatype="http://www.w3.org/2001/XMLSchema#anyURI">http://www.ontologyrepository.com/CommonCoreOntologies/Domain/CyberOntology</cco2:ont00001760>
    </owl:Class>
    


    <!-- http://www.ontologyrepository.com/CommonCoreOntologies/FileReading -->

    <owl:Class rdf:about="http://www.ontologyrepository.com/CommonCoreOntologies/FileReading">
        <rdfs:subClassOf rdf:resource="http://www.ontologyrepository.com/CommonCoreOntologies/DigitalFileProcess"/>
        <skos:definition xml:lang="en">A Digital File Process in which the content of a Digital File serves as input to an Information Processing Artifact.</skos:definition>
        <rdfs:label xml:lang="en">File Reading</rdfs:label>
        <cco2:ont00001760 rdf:datatype="http://www.w3.org/2001/XMLSchema#anyURI">http://www.ontologyrepository.com/CommonCoreOntologies/Domain/CyberOntology</cco2:ont00001760>
    </owl:Class>
    


    <!-- http://www.ontologyrepository.com/CommonCoreOntologies/FileServer -->

    <owl:Class rdf:about="http://www.ontologyrepository.com/CommonCoreOntologies/FileServer">
        <rdfs:subClassOf rdf:resource="http://www.ontologyrepository.com/CommonCoreOntologies/NetworkServer"/>
        <skos:definition xml:lang="en">A Network Server that enables clients to access a Digital File Management Function.</skos:definition>
        <rdfs:label xml:lang="en">File Server</rdfs:label>
        <cco2:ont00001754 rdf:datatype="http://www.w3.org/2001/XMLSchema#anyURI">https://en.wikipedia.org/wiki/File_server</cco2:ont00001754>
        <cco2:ont00001760 rdf:datatype="http://www.w3.org/2001/XMLSchema#anyURI">http://www.ontologyrepository.com/CommonCoreOntologies/Domain/CyberOntology</cco2:ont00001760>
    </owl:Class>
    


    <!-- http://www.ontologyrepository.com/CommonCoreOntologies/FileSynchronizationUtility -->

    <owl:Class rdf:about="http://www.ontologyrepository.com/CommonCoreOntologies/FileSynchronizationUtility">
        <rdfs:subClassOf rdf:resource="http://www.ontologyrepository.com/CommonCoreOntologies/DataSynchronizationUtility"/>
        <skos:definition xml:lang="en">A Data Synchronization Utility that is designed to establish that Digital Files in two or more locations are updated in tandem.</skos:definition>
        <rdfs:label xml:lang="en">File Synchronization Utility</rdfs:label>
        <cco2:ont00001754>https://en.wikipedia.org/wiki/File_synchronization</cco2:ont00001754>
        <cco2:ont00001760 rdf:datatype="http://www.w3.org/2001/XMLSchema#anyURI">http://www.ontologyrepository.com/CommonCoreOntologies/Domain/CyberOntology</cco2:ont00001760>
    </owl:Class>
    


    <!-- http://www.ontologyrepository.com/CommonCoreOntologies/FileSystemDirectory -->

    <owl:Class rdf:about="http://www.ontologyrepository.com/CommonCoreOntologies/FileSystemDirectory">
        <rdfs:subClassOf rdf:resource="http://purl.obolibrary.org/obo/BFO_0000027"/>
        <skos:altLabel xml:lang="en">Directory</skos:altLabel>
        <skos:altLabel xml:lang="en">Folder</skos:altLabel>
        <skos:definition xml:lang="en">An Object Aggregate that consists of an aggregate of Digital Files within the context of a Digital File System.</skos:definition>
        <rdfs:label xml:lang="en">File System Directory</rdfs:label>
        <cco2:ont00001754>https://en.wikipedia.org/wiki/Directory_(computing)</cco2:ont00001754>
        <cco2:ont00001760 rdf:datatype="http://www.w3.org/2001/XMLSchema#anyURI">http://www.ontologyrepository.com/CommonCoreOntologies/Domain/CyberOntology</cco2:ont00001760>
    </owl:Class>
    


    <!-- http://www.ontologyrepository.com/CommonCoreOntologies/FileTransfer -->

    <owl:Class rdf:about="http://www.ontologyrepository.com/CommonCoreOntologies/FileTransfer">
        <rdfs:subClassOf rdf:resource="http://www.ontologyrepository.com/CommonCoreOntologies/DataTransfer"/>
        <skos:definition xml:lang="en">A Data Transfer in which a Computer File is transmitted from one Computer to another.</skos:definition>
        <rdfs:label xml:lang="en">File Transfer</rdfs:label>
        <cco2:ont00001760 rdf:datatype="http://www.w3.org/2001/XMLSchema#anyURI">http://www.ontologyrepository.com/CommonCoreOntologies/Domain/CyberOntology</cco2:ont00001760>
    </owl:Class>
    


    <!-- http://www.ontologyrepository.com/CommonCoreOntologies/FileWriting -->

    <owl:Class rdf:about="http://www.ontologyrepository.com/CommonCoreOntologies/FileWriting">
        <rdfs:subClassOf rdf:resource="http://www.ontologyrepository.com/CommonCoreOntologies/DigitalFileProcess"/>
        <skos:definition xml:lang="en">A Digital File Process that outputs information to a new Digital File.</skos:definition>
        <rdfs:label xml:lang="en">File Writing</rdfs:label>
        <cco2:ont00001760 rdf:datatype="http://www.w3.org/2001/XMLSchema#anyURI">http://www.ontologyrepository.com/CommonCoreOntologies/Domain/CyberOntology</cco2:ont00001760>
    </owl:Class>
    


    <!-- http://www.ontologyrepository.com/CommonCoreOntologies/Firewall -->

    <owl:Class rdf:about="http://www.ontologyrepository.com/CommonCoreOntologies/Firewall">
        <rdfs:subClassOf rdf:resource="http://www.ontologyrepository.com/CommonCoreOntologies/NetworkSecurityApplication"/>
        <skos:definition xml:lang="en">A Network Security Application that uses defined rules to allow or block traffic between a trusted internal Computer Network and an untrusted outside Computer Network.</skos:definition>
        <rdfs:label xml:lang="en">Firewall</rdfs:label>
        <cco2:ont00001754>http://www.cisco.com/c/en/us/products/security/what-is-network-security.html</cco2:ont00001754>
        <cco2:ont00001760 rdf:datatype="http://www.w3.org/2001/XMLSchema#anyURI">http://www.ontologyrepository.com/CommonCoreOntologies/Domain/CyberOntology</cco2:ont00001760>
    </owl:Class>
    


    <!-- http://www.ontologyrepository.com/CommonCoreOntologies/Firmware -->

    <owl:Class rdf:about="http://www.ontologyrepository.com/CommonCoreOntologies/Firmware">
        <rdfs:subClassOf rdf:resource="http://www.ontologyrepository.com/CommonCoreOntologies/SystemSoftware"/>
        <skos:definition xml:lang="en">A System Software that enables low-level control for components of an Information Processing Artifact.</skos:definition>
        <rdfs:label xml:lang="en">Firmware</rdfs:label>
        <cco2:ont00001754>https://en.wikipedia.org/wiki/Firmware</cco2:ont00001754>
        <cco2:ont00001760 rdf:datatype="http://www.w3.org/2001/XMLSchema#anyURI">http://www.ontologyrepository.com/CommonCoreOntologies/Domain/CyberOntology</cco2:ont00001760>
    </owl:Class>
    


    <!-- http://www.ontologyrepository.com/CommonCoreOntologies/FirmwareVulnerability -->

    <owl:Class rdf:about="http://www.ontologyrepository.com/CommonCoreOntologies/FirmwareVulnerability">
        <rdfs:subClassOf rdf:resource="http://www.ontologyrepository.com/CommonCoreOntologies/CyberVulnerability"/>
        <skos:definition xml:lang="en">A Cyber Vulnerability realized by a Cyber Attack that prevents an Information Processing Artifact&apos;s firmware from functioning properly.</skos:definition>
        <rdfs:label xml:lang="en">Firmware Vulnerability</rdfs:label>
        <cco2:ont00001760 rdf:datatype="http://www.w3.org/2001/XMLSchema#anyURI">http://www.ontologyrepository.com/CommonCoreOntologies/Domain/CyberOntology</cco2:ont00001760>
    </owl:Class>
    


    <!-- http://www.ontologyrepository.com/CommonCoreOntologies/FlashDrive -->

    <owl:Class rdf:about="http://www.ontologyrepository.com/CommonCoreOntologies/FlashDrive">
        <rdfs:subClassOf rdf:resource="https://www.commoncoreontologies.org/ont00001179"/>
        <skos:definition xml:lang="en">A Digital Storage Device that is designed to store information using flash memory, have an integrated USB interface, and be removable and rewritable.</skos:definition>
        <rdfs:label xml:lang="en">Flash Drive</rdfs:label>
        <cco2:ont00001754>https://en.wikipedia.org/wiki/USB_flash_drive</cco2:ont00001754>
        <cco2:ont00001760 rdf:datatype="http://www.w3.org/2001/XMLSchema#anyURI">http://www.ontologyrepository.com/CommonCoreOntologies/Domain/CyberOntology</cco2:ont00001760>
    </owl:Class>
    


    <!-- http://www.ontologyrepository.com/CommonCoreOntologies/FlightSimulator -->

    <owl:Class rdf:about="http://www.ontologyrepository.com/CommonCoreOntologies/FlightSimulator">
        <rdfs:subClassOf rdf:resource="http://www.ontologyrepository.com/CommonCoreOntologies/VehicleSimulator"/>
        <skos:definition xml:lang="en">A Vehicle Simulator that is designed to enable a user to model the process of flying an Aircraft or Spacecraft.</skos:definition>
        <rdfs:label xml:lang="en">Flight Simulator</rdfs:label>
        <cco2:ont00001760 rdf:datatype="http://www.w3.org/2001/XMLSchema#anyURI">http://www.ontologyrepository.com/CommonCoreOntologies/Domain/CyberOntology</cco2:ont00001760>
    </owl:Class>
    


    <!-- http://www.ontologyrepository.com/CommonCoreOntologies/FlowControlDirective -->

    <owl:Class rdf:about="http://www.ontologyrepository.com/CommonCoreOntologies/FlowControlDirective">
        <rdfs:subClassOf rdf:resource="https://www.commoncoreontologies.org/ont00000965"/>
        <skos:definition xml:lang="en">A Directive Information Content Entity that prescribes the rate of data transmission between two nodes to prevent a fast sender from overwhelming a slow receiver.</skos:definition>
        <rdfs:label xml:lang="en">Flow Control Directive</rdfs:label>
        <cco2:ont00001754>https://en.wikipedia.org/wiki/Flow_control_(data)</cco2:ont00001754>
        <cco2:ont00001760 rdf:datatype="http://www.w3.org/2001/XMLSchema#anyURI">http://www.ontologyrepository.com/CommonCoreOntologies/Domain/CyberOntology</cco2:ont00001760>
    </owl:Class>
    


    <!-- http://www.ontologyrepository.com/CommonCoreOntologies/GraphDatabaseSoftwareApplicationModel -->

    <owl:Class rdf:about="http://www.ontologyrepository.com/CommonCoreOntologies/GraphDatabaseSoftwareApplicationModel">
        <rdfs:subClassOf rdf:resource="http://www.ontologyrepository.com/CommonCoreOntologies/DatabaseSoftwareApplicationModel"/>
        <skos:definition xml:lang="en">A Database Software Application Model that prescribes a Database Software Application where the data is stored as sets of nodes, or vertices, linked via edges, or relationships.</skos:definition>
        <rdfs:label xml:lang="en">Graph Database Software Application Model</rdfs:label>
        <cco2:ont00001760 rdf:datatype="http://www.w3.org/2001/XMLSchema#anyURI">http://www.ontologyrepository.com/CommonCoreOntologies/Domain/CyberOntology</cco2:ont00001760>
    </owl:Class>
    


    <!-- http://www.ontologyrepository.com/CommonCoreOntologies/Grapheme -->

    <owl:Class rdf:about="http://www.ontologyrepository.com/CommonCoreOntologies/Grapheme">
        <rdfs:subClassOf rdf:resource="http://www.ontologyrepository.com/CommonCoreOntologies/WrittenSymbol"/>
        <skos:definition xml:lang="en">A Written Symbol that is the smallest unit of a writing system of any given language.</skos:definition>
        <skos:example>Alphabetic letters</skos:example>
        <skos:example>Chinese characters</skos:example>
        <skos:example>Numerical digits</skos:example>
        <skos:example>Typographic ligatures</skos:example>
        <rdfs:label xml:lang="en">Grapheme</rdfs:label>
        <cco2:ont00001754>https://en.wikipedia.org/wiki/Grapheme</cco2:ont00001754>
        <cco2:ont00001760 rdf:datatype="http://www.w3.org/2001/XMLSchema#anyURI">http://www.ontologyrepository.com/CommonCoreOntologies/Domain/CyberOntology</cco2:ont00001760>
    </owl:Class>
    


    <!-- http://www.ontologyrepository.com/CommonCoreOntologies/GraphicArtSoftwareApplication -->

    <owl:Class rdf:about="http://www.ontologyrepository.com/CommonCoreOntologies/GraphicArtSoftwareApplication">
        <rdfs:subClassOf rdf:resource="http://www.ontologyrepository.com/CommonCoreOntologies/MultimediaSoftwareApplication"/>
        <skos:definition xml:lang="en">A Multimedia Software Application that is designed to enable a user to create and edit graphic files.</skos:definition>
        <rdfs:label xml:lang="en">Graphic Art Software Application</rdfs:label>
        <cco2:ont00001760 rdf:datatype="http://www.w3.org/2001/XMLSchema#anyURI">http://www.ontologyrepository.com/CommonCoreOntologies/Domain/CyberOntology</cco2:ont00001760>
    </owl:Class>
    


    <!-- http://www.ontologyrepository.com/CommonCoreOntologies/GraphicsProcessingUnit -->

    <owl:Class rdf:about="http://www.ontologyrepository.com/CommonCoreOntologies/GraphicsProcessingUnit">
        <rdfs:subClassOf rdf:resource="http://www.ontologyrepository.com/CommonCoreOntologies/ProcessingUnit"/>
        <skos:definition xml:lang="en">A Processing Unit that is designed to accelerate the execution of some Computer Program pertaining to the display of some Image on a Screen.</skos:definition>
        <rdfs:label xml:lang="en">Graphics Processing Unit</rdfs:label>
        <cco2:ont00001754>https://en.wikipedia.org/wiki/Graphics_processing_unit</cco2:ont00001754>
        <cco2:ont00001760 rdf:datatype="http://www.w3.org/2001/XMLSchema#anyURI">http://www.ontologyrepository.com/CommonCoreOntologies/Domain/CyberOntology</cco2:ont00001760>
    </owl:Class>
    


    <!-- http://www.ontologyrepository.com/CommonCoreOntologies/HardDiskDrive -->

    <owl:Class rdf:about="http://www.ontologyrepository.com/CommonCoreOntologies/HardDiskDrive">
        <rdfs:subClassOf rdf:resource="https://www.commoncoreontologies.org/ont00001179"/>
        <skos:definition xml:lang="en">A Digital Storage Device that is designed to provide long-term storage and retrieval of digital information using one or more rigid rapidly rotating disks coated with magnetic material.</skos:definition>
        <rdfs:label xml:lang="en">Hard Disk Drive</rdfs:label>
        <cco2:ont00001754>https://en.wikipedia.org/wiki/Hard_disk_drive</cco2:ont00001754>
        <cco2:ont00001760 rdf:datatype="http://www.w3.org/2001/XMLSchema#anyURI">http://www.ontologyrepository.com/CommonCoreOntologies/Domain/CyberOntology</cco2:ont00001760>
    </owl:Class>
    


    <!-- http://www.ontologyrepository.com/CommonCoreOntologies/HashBucket -->

    <owl:Class rdf:about="http://www.ontologyrepository.com/CommonCoreOntologies/HashBucket">
        <rdfs:subClassOf rdf:resource="http://www.ontologyrepository.com/CommonCoreOntologies/Tuple"/>
        <skos:definition xml:lang="en">A Tuple that partitions Key-Value Pairs in a Hash Table.</skos:definition>
        <rdfs:label xml:lang="en">Hash Bucket</rdfs:label>
        <cco2:ont00001760 rdf:datatype="http://www.w3.org/2001/XMLSchema#anyURI">http://www.ontologyrepository.com/CommonCoreOntologies/Domain/CyberOntology</cco2:ont00001760>
    </owl:Class>
    


    <!-- http://www.ontologyrepository.com/CommonCoreOntologies/HashFunction -->

    <owl:Class rdf:about="http://www.ontologyrepository.com/CommonCoreOntologies/HashFunction">
        <rdfs:subClassOf rdf:resource="http://www.ontologyrepository.com/CommonCoreOntologies/Subroutine"/>
        <skos:definition xml:lang="en">A Subroutine that has some variable as input and which outputs a fixed-length string or number.</skos:definition>
        <rdfs:label xml:lang="en">Hash Function</rdfs:label>
        <cco2:ont00001760 rdf:datatype="http://www.w3.org/2001/XMLSchema#anyURI">http://www.ontologyrepository.com/CommonCoreOntologies/Domain/CyberOntology</cco2:ont00001760>
    </owl:Class>
    


    <!-- http://www.ontologyrepository.com/CommonCoreOntologies/HashTable -->

    <owl:Class rdf:about="http://www.ontologyrepository.com/CommonCoreOntologies/HashTable">
        <rdfs:subClassOf rdf:resource="http://www.ontologyrepository.com/CommonCoreOntologies/DataTable"/>
        <skos:altLabel xml:lang="en">Hash Map</skos:altLabel>
        <skos:definition xml:lang="en">A Matrix that uses a Hash Function to efficiently store non-contiguous Key-Value Pairs in Hash Buckets.</skos:definition>
        <rdfs:label xml:lang="en">Hash Table</rdfs:label>
        <cco2:ont00001754>https://en.wikipedia.org/wiki/Hash_table</cco2:ont00001754>
        <cco2:ont00001760 rdf:datatype="http://www.w3.org/2001/XMLSchema#anyURI">http://www.ontologyrepository.com/CommonCoreOntologies/Domain/CyberOntology</cco2:ont00001760>
    </owl:Class>
    


    <!-- http://www.ontologyrepository.com/CommonCoreOntologies/HashValue -->

    <owl:Class rdf:about="http://www.ontologyrepository.com/CommonCoreOntologies/HashValue">
        <rdfs:subClassOf rdf:resource="https://www.commoncoreontologies.org/ont00000798"/>
        <skos:altLabel xml:lang="en">Hash</skos:altLabel>
        <skos:definition xml:lang="en">An Information Bearing Artifact that is the output of a Hash Function.</skos:definition>
        <rdfs:label xml:lang="en">Hash Value</rdfs:label>
        <cco2:ont00001760 rdf:datatype="http://www.w3.org/2001/XMLSchema#anyURI">http://www.ontologyrepository.com/CommonCoreOntologies/Domain/CyberOntology</cco2:ont00001760>
    </owl:Class>
    


    <!-- http://www.ontologyrepository.com/CommonCoreOntologies/HighLevelProgrammingLanguage -->

    <owl:Class rdf:about="http://www.ontologyrepository.com/CommonCoreOntologies/HighLevelProgrammingLanguage">
        <rdfs:subClassOf rdf:resource="http://www.ontologyrepository.com/CommonCoreOntologies/ProgrammingLanguage"/>
        <skos:definition xml:lang="en">A Programming Language with strong abstraction from the language necessary for a set of instructions to be executed by a Processing Unit.</skos:definition>
        <rdfs:label xml:lang="en">High-Level Programming Language</rdfs:label>
        <cco2:ont00001760 rdf:datatype="http://www.w3.org/2001/XMLSchema#anyURI">http://www.ontologyrepository.com/CommonCoreOntologies/Domain/CyberOntology</cco2:ont00001760>
    </owl:Class>
    


    <!-- http://www.ontologyrepository.com/CommonCoreOntologies/HypervisorProgram -->

    <owl:Class rdf:about="http://www.ontologyrepository.com/CommonCoreOntologies/HypervisorProgram">
        <rdfs:subClassOf rdf:resource="http://www.ontologyrepository.com/CommonCoreOntologies/UtilityProgram"/>
        <skos:definition xml:lang="en">An Utility Program that creates and runs Virtual Machines.</skos:definition>
        <rdfs:label xml:lang="en">Hypervisor Program</rdfs:label>
        <cco2:ont00001754 rdf:datatype="http://www.w3.org/2001/XMLSchema#anyURI">https://en.wikipedia.org/wiki/Hypervisor</cco2:ont00001754>
        <cco2:ont00001760 rdf:datatype="http://www.w3.org/2001/XMLSchema#anyURI">http://www.ontologyrepository.com/CommonCoreOntologies/Domain/CyberOntology</cco2:ont00001760>
    </owl:Class>
    


    <!-- http://www.ontologyrepository.com/CommonCoreOntologies/ImageScanner -->

    <owl:Class rdf:about="http://www.ontologyrepository.com/CommonCoreOntologies/ImageScanner">
        <rdfs:subClassOf rdf:resource="https://www.commoncoreontologies.org/ont00000771"/>
        <skos:definition xml:lang="en">An Imaging Instrument that optically scans an image, document, or object, and converts it to a digital image.</skos:definition>
        <rdfs:label xml:lang="en">Image Scanner</rdfs:label>
        <cco2:ont00001754 rdf:datatype="http://www.w3.org/2001/XMLSchema#anyURI">https://en.wikipedia.org/wiki/Image_scanner</cco2:ont00001754>
        <cco2:ont00001760 rdf:datatype="http://www.w3.org/2001/XMLSchema#anyURI">http://www.ontologyrepository.com/CommonCoreOntologies/Domain/CyberOntology</cco2:ont00001760>
    </owl:Class>
    


    <!-- http://www.ontologyrepository.com/CommonCoreOntologies/InformationAggregateSpecification -->

    <owl:Class rdf:about="http://www.ontologyrepository.com/CommonCoreOntologies/InformationAggregateSpecification">
        <rdfs:subClassOf rdf:resource="https://www.commoncoreontologies.org/ont00000965"/>
        <skos:definition xml:lang="en">A Directive Information Content Entity that prescribes some ordering (sequence, arrangement) of Information Content Entities.</skos:definition>
        <rdfs:label xml:lang="en">Information Aggregate Specification</rdfs:label>
        <cco2:ont00001760 rdf:datatype="http://www.w3.org/2001/XMLSchema#anyURI">http://www.ontologyrepository.com/CommonCoreOntologies/Domain/CyberOntology</cco2:ont00001760>
    </owl:Class>
    


    <!-- http://www.ontologyrepository.com/CommonCoreOntologies/InformationHeader -->

    <owl:Class rdf:about="http://www.ontologyrepository.com/CommonCoreOntologies/InformationHeader">
        <rdfs:subClassOf rdf:resource="https://www.commoncoreontologies.org/ont00000798"/>
        <skos:definition xml:lang="en">An Information Bearing Artifact that bears supplementary information describing the contents of the some other information bearer.</skos:definition>
        <skos:example>A TCP packet header</skos:example>
        <skos:example>An email message header</skos:example>
        <skos:example>Page headers in a novel</skos:example>
        <rdfs:label xml:lang="en">Information Header</rdfs:label>
        <cco2:ont00001760 rdf:datatype="http://www.w3.org/2001/XMLSchema#anyURI">http://www.ontologyrepository.com/CommonCoreOntologies/Domain/CyberOntology</cco2:ont00001760>
    </owl:Class>
    


    <!-- http://www.ontologyrepository.com/CommonCoreOntologies/InformationProcessingArtifactFunction -->

    <owl:Class rdf:about="http://www.ontologyrepository.com/CommonCoreOntologies/InformationProcessingArtifactFunction">
        <rdfs:subClassOf rdf:resource="https://www.commoncoreontologies.org/ont00000727"/>
        <skos:altLabel xml:lang="en">Service</skos:altLabel>
        <skos:definition xml:lang="en">A Communication Artifact Function that inheres in some Information Processing Artifact.</skos:definition>
        <rdfs:label xml:lang="en">Information Processing Artifact Function</rdfs:label>
        <cco2:ont00001760 rdf:datatype="http://www.w3.org/2001/XMLSchema#anyURI">http://www.ontologyrepository.com/CommonCoreOntologies/Domain/CyberOntology</cco2:ont00001760>
    </owl:Class>
    


    <!-- http://www.ontologyrepository.com/CommonCoreOntologies/InformationTransferProtocol -->

    <owl:Class rdf:about="http://www.ontologyrepository.com/CommonCoreOntologies/InformationTransferProtocol">
        <rdfs:subClassOf rdf:resource="https://www.commoncoreontologies.org/ont00000965"/>
        <skos:definition xml:lang="en">A Directive Information Content Entity that prescribes the format in which some Information Content Entity should be transferred between two Computers or other devices.</skos:definition>
        <rdfs:label xml:lang="en">Information Transfer Protocol</rdfs:label>
        <cco2:ont00001760 rdf:datatype="http://www.w3.org/2001/XMLSchema#anyURI">http://www.ontologyrepository.com/CommonCoreOntologies/Domain/CyberOntology</cco2:ont00001760>
    </owl:Class>
    


    <!-- http://www.ontologyrepository.com/CommonCoreOntologies/InformationWorkerSoftware -->

    <owl:Class rdf:about="http://www.ontologyrepository.com/CommonCoreOntologies/InformationWorkerSoftware">
        <rdfs:subClassOf rdf:resource="http://www.ontologyrepository.com/CommonCoreOntologies/ApplicationSoftware"/>
        <skos:definition xml:lang="en">Application Software that is designed to enable users to create and manage Information Bearing Artifacts.</skos:definition>
        <rdfs:label xml:lang="en">Information Worker Software</rdfs:label>
        <cco2:ont00001754>https://en.wikipedia.org/wiki/Application_software#Information_worker_software</cco2:ont00001754>
        <cco2:ont00001760 rdf:datatype="http://www.w3.org/2001/XMLSchema#anyURI">http://www.ontologyrepository.com/CommonCoreOntologies/Domain/CyberOntology</cco2:ont00001760>
    </owl:Class>
    


    <!-- http://www.ontologyrepository.com/CommonCoreOntologies/InputDevice -->

    <owl:Class rdf:about="http://www.ontologyrepository.com/CommonCoreOntologies/InputDevice">
        <rdfs:subClassOf rdf:resource="http://www.ontologyrepository.com/CommonCoreOntologies/ComputerComponent"/>
        <skos:definition xml:lang="en">A Computer Component used to provide data and control signals to an Information Processing Artifact</skos:definition>
        <rdfs:label xml:lang="en">Input Device</rdfs:label>
        <cco2:ont00001754 rdf:datatype="http://www.w3.org/2001/XMLSchema#anyURI">https://en.wikipedia.org/wiki/Input_device</cco2:ont00001754>
        <cco2:ont00001760 rdf:datatype="http://www.w3.org/2001/XMLSchema#anyURI">http://www.ontologyrepository.com/CommonCoreOntologies/Domain/CyberOntology</cco2:ont00001760>
    </owl:Class>
    


    <!-- http://www.ontologyrepository.com/CommonCoreOntologies/IntegratedDevelopmentEnvironment -->

    <owl:Class rdf:about="http://www.ontologyrepository.com/CommonCoreOntologies/IntegratedDevelopmentEnvironment">
        <rdfs:subClassOf rdf:resource="http://www.ontologyrepository.com/CommonCoreOntologies/SoftwareEngineeringSoftware"/>
        <skos:definition xml:lang="en">Software Engineering Sotware that is designed to facilitate authoring, modifying, compiling, deploying and debugging software.</skos:definition>
        <rdfs:label xml:lang="en">Integrated Development Environment</rdfs:label>
        <cco2:ont00001754>https://en.wikipedia.org/wiki/Integrated_development_environment</cco2:ont00001754>
        <cco2:ont00001760 rdf:datatype="http://www.w3.org/2001/XMLSchema#anyURI">http://www.ontologyrepository.com/CommonCoreOntologies/Domain/CyberOntology</cco2:ont00001760>
    </owl:Class>
    


    <!-- http://www.ontologyrepository.com/CommonCoreOntologies/InternationalizedResourceIdentifier -->

    <owl:Class rdf:about="http://www.ontologyrepository.com/CommonCoreOntologies/InternationalizedResourceIdentifier">
        <rdfs:subClassOf rdf:resource="http://www.ontologyrepository.com/CommonCoreOntologies/UniformResourceIdentifier"/>
        <skos:definition xml:lang="en">A Uniform Resource Identifier that may contain characters from the Universal Character Set (Unicode/ISO 10646).</skos:definition>
        <rdfs:label xml:lang="en">Internationalized Resource Identifier</rdfs:label>
        <cco2:ont00001753>IRI</cco2:ont00001753>
        <cco2:ont00001754>https://en.wikipedia.org/wiki/Internationalized_Resource_Identifier</cco2:ont00001754>
        <cco2:ont00001760 rdf:datatype="http://www.w3.org/2001/XMLSchema#anyURI">http://www.ontologyrepository.com/CommonCoreOntologies/Domain/CyberOntology</cco2:ont00001760>
    </owl:Class>
    


    <!-- http://www.ontologyrepository.com/CommonCoreOntologies/InternetBot -->

    <owl:Class rdf:about="http://www.ontologyrepository.com/CommonCoreOntologies/InternetBot">
        <rdfs:subClassOf rdf:resource="http://www.ontologyrepository.com/CommonCoreOntologies/ApplicationSoftware"/>
        <skos:definition xml:lang="en">Application Software that runs automated tasks (scripts) over the Internet.</skos:definition>
        <rdfs:label xml:lang="en">Internet Bot</rdfs:label>
        <cco2:ont00001754>https://en.wikipedia.org/wiki/Internet_bot</cco2:ont00001754>
        <cco2:ont00001760 rdf:datatype="http://www.w3.org/2001/XMLSchema#anyURI">http://www.ontologyrepository.com/CommonCoreOntologies/Domain/CyberOntology</cco2:ont00001760>
    </owl:Class>
    


    <!-- http://www.ontologyrepository.com/CommonCoreOntologies/InternetForum -->

    <owl:Class rdf:about="http://www.ontologyrepository.com/CommonCoreOntologies/InternetForum">
        <rdfs:subClassOf rdf:resource="http://www.ontologyrepository.com/CommonCoreOntologies/Website"/>
        <skos:definition xml:lang="en">A Website on which people can hold conversations in the form of posted messages that are typically longer than one sentence and that are at least temporarily archived.</skos:definition>
        <rdfs:label xml:lang="en">Internet Forum</rdfs:label>
        <cco2:ont00001754>https://en.wikipedia.org/wiki/Internet_forum</cco2:ont00001754>
        <cco2:ont00001760 rdf:datatype="http://www.w3.org/2001/XMLSchema#anyURI">http://www.ontologyrepository.com/CommonCoreOntologies/Domain/CyberOntology</cco2:ont00001760>
    </owl:Class>
    


    <!-- http://www.ontologyrepository.com/CommonCoreOntologies/InternetProtocolAddress -->

    <owl:Class rdf:about="http://www.ontologyrepository.com/CommonCoreOntologies/InternetProtocolAddress">
        <rdfs:subClassOf rdf:resource="https://www.commoncoreontologies.org/ont00000077"/>
        <skos:altLabel xml:lang="en">IP Address</skos:altLabel>
        <skos:definition xml:lang="en">A Code Identifier that designates a Computer or other device that is connected to the Internet Protocol Suite.</skos:definition>
        <rdfs:label xml:lang="en">Internet Protocol Address</rdfs:label>
        <cco2:ont00001754>https://en.wikipedia.org/wiki/Internet_protocol_suite</cco2:ont00001754>
        <cco2:ont00001760 rdf:datatype="http://www.w3.org/2001/XMLSchema#anyURI">http://www.ontologyrepository.com/CommonCoreOntologies/Domain/CyberOntology</cco2:ont00001760>
    </owl:Class>
    


    <!-- http://www.ontologyrepository.com/CommonCoreOntologies/InternetRelayChatService -->

    <owl:Class rdf:about="http://www.ontologyrepository.com/CommonCoreOntologies/InternetRelayChatService">
        <rdfs:subClassOf rdf:resource="http://www.ontologyrepository.com/CommonCoreOntologies/InternetBot"/>
        <skos:altLabel xml:lang="en">IRC Service</skos:altLabel>
        <skos:definition xml:lang="en">An Internet Bot that manages access to an IRC network.</skos:definition>
        <rdfs:label xml:lang="en">Internet Relay Chat Service</rdfs:label>
        <cco2:ont00001754>https://en.wikipedia.org/wiki/Internet_Relay_Chat_services</cco2:ont00001754>
        <cco2:ont00001760 rdf:datatype="http://www.w3.org/2001/XMLSchema#anyURI">http://www.ontologyrepository.com/CommonCoreOntologies/Domain/CyberOntology</cco2:ont00001760>
    </owl:Class>
    


    <!-- http://www.ontologyrepository.com/CommonCoreOntologies/InternetServiceProvider -->

    <owl:Class rdf:about="http://www.ontologyrepository.com/CommonCoreOntologies/InternetServiceProvider">
        <rdfs:subClassOf rdf:resource="https://www.commoncoreontologies.org/ont00000509"/>
        <skos:definition xml:lang="en">A Service Provider that provides services for accessing and using the Internet.</skos:definition>
        <rdfs:label xml:lang="en">Internet Service Provider</rdfs:label>
        <cco2:ont00001754>https://en.wikipedia.org/wiki/Internet_service_provider</cco2:ont00001754>
        <cco2:ont00001760 rdf:datatype="http://www.w3.org/2001/XMLSchema#anyURI">http://www.ontologyrepository.com/CommonCoreOntologies/Domain/CyberOntology</cco2:ont00001760>
    </owl:Class>
    


    <!-- http://www.ontologyrepository.com/CommonCoreOntologies/InterpretedLanguage -->

    <owl:Class rdf:about="http://www.ontologyrepository.com/CommonCoreOntologies/InterpretedLanguage">
        <rdfs:subClassOf rdf:resource="http://www.ontologyrepository.com/CommonCoreOntologies/HighLevelProgrammingLanguage"/>
        <owl:disjointWith rdf:resource="http://www.ontologyrepository.com/CommonCoreOntologies/MachineLanguage"/>
        <skos:definition xml:lang="en">A Programming Language that prescribes a canonical form of communicating instructions to be executed by a Processing Unit in such a way that those instructions do not need to be compiled into Machine Language instructions.</skos:definition>
        <rdfs:label xml:lang="en">Interpreted Language</rdfs:label>
        <cco2:ont00001754>https://en.wikipedia.org/wiki/Interpreted_language</cco2:ont00001754>
        <cco2:ont00001760 rdf:datatype="http://www.w3.org/2001/XMLSchema#anyURI">http://www.ontologyrepository.com/CommonCoreOntologies/Domain/CyberOntology</cco2:ont00001760>
    </owl:Class>
    


    <!-- http://www.ontologyrepository.com/CommonCoreOntologies/JSONFile -->

    <owl:Class rdf:about="http://www.ontologyrepository.com/CommonCoreOntologies/JSONFile">
        <rdfs:subClassOf rdf:resource="http://www.ontologyrepository.com/CommonCoreOntologies/TextFile"/>
        <skos:definition xml:lang="en">A Text File that uses JavaScript Object Notation as a Data Exchange Language.</skos:definition>
        <rdfs:label xml:lang="en">JSON File</rdfs:label>
        <cco2:ont00001760 rdf:datatype="http://www.w3.org/2001/XMLSchema#anyURI">http://www.ontologyrepository.com/CommonCoreOntologies/Domain/CyberOntology</cco2:ont00001760>
    </owl:Class>
    


    <!-- http://www.ontologyrepository.com/CommonCoreOntologies/KeyValueDatabaseSoftwareApplicationModel -->

    <owl:Class rdf:about="http://www.ontologyrepository.com/CommonCoreOntologies/KeyValueDatabaseSoftwareApplicationModel">
        <rdfs:subClassOf rdf:resource="http://www.ontologyrepository.com/CommonCoreOntologies/DatabaseSoftwareApplicationModel"/>
        <skos:definition xml:lang="en">A Database Software Application Model that prescribes some Database Software Application where the data is stored as a collection of records, or objects, each of which is associated with a distinct key.</skos:definition>
        <rdfs:label xml:lang="en">Key-Value Database Software Application Model</rdfs:label>
        <cco2:ont00001760 rdf:datatype="http://www.w3.org/2001/XMLSchema#anyURI">http://www.ontologyrepository.com/CommonCoreOntologies/Domain/CyberOntology</cco2:ont00001760>
    </owl:Class>
    


    <!-- http://www.ontologyrepository.com/CommonCoreOntologies/KeyValuePair -->

    <owl:Class rdf:about="http://www.ontologyrepository.com/CommonCoreOntologies/KeyValuePair">
        <rdfs:subClassOf rdf:resource="http://www.ontologyrepository.com/CommonCoreOntologies/OrderedPair"/>
        <skos:altLabel xml:lang="en">Attribute-Value Pair</skos:altLabel>
        <skos:altLabel xml:lang="en">Field-Value Pair</skos:altLabel>
        <skos:altLabel xml:lang="en">Value Pair</skos:altLabel>
        <skos:definition xml:lang="en">A Pair whose first element is some Information Bearing Artifact which bears some unique designator for some entity and whose second element is some Information Bearing Artifact which represents either the designated entity or some other designator which designates the location of information about that entity.</skos:definition>
        <rdfs:label xml:lang="en">Key-Value Pair</rdfs:label>
        <cco2:ont00001760 rdf:datatype="http://www.w3.org/2001/XMLSchema#anyURI">http://www.ontologyrepository.com/CommonCoreOntologies/Domain/CyberOntology</cco2:ont00001760>
    </owl:Class>
    


    <!-- http://www.ontologyrepository.com/CommonCoreOntologies/Keylogger -->

    <owl:Class rdf:about="http://www.ontologyrepository.com/CommonCoreOntologies/Keylogger">
        <rdfs:subClassOf rdf:resource="http://www.ontologyrepository.com/CommonCoreOntologies/Malware"/>
        <skos:definition xml:lang="en">Malware that is designed to record the keys struck on a keyboard.</skos:definition>
        <rdfs:label xml:lang="en">Keylogger</rdfs:label>
        <cco2:ont00001754>https://en.wikipedia.org/wiki/Keystroke_logging</cco2:ont00001754>
        <cco2:ont00001760 rdf:datatype="http://www.w3.org/2001/XMLSchema#anyURI">http://www.ontologyrepository.com/CommonCoreOntologies/Domain/CyberOntology</cco2:ont00001760>
    </owl:Class>
    


    <!-- http://www.ontologyrepository.com/CommonCoreOntologies/LaptopComputer -->

    <owl:Class rdf:about="http://www.ontologyrepository.com/CommonCoreOntologies/LaptopComputer">
        <rdfs:subClassOf rdf:resource="https://www.commoncoreontologies.org/ont00000420"/>
        <skos:altLabel xml:lang="en">Notebook Computer</skos:altLabel>
        <skos:definition xml:lang="en">A Computer that is designed to be portable with a screen and keyboard included in a single clamshell housing.</skos:definition>
        <rdfs:label xml:lang="en">Laptop Computer</rdfs:label>
        <cco2:ont00001760 rdf:datatype="http://www.w3.org/2001/XMLSchema#anyURI">http://www.ontologyrepository.com/CommonCoreOntologies/Domain/CyberOntology</cco2:ont00001760>
    </owl:Class>
    


    <!-- http://www.ontologyrepository.com/CommonCoreOntologies/Letter -->

    <owl:Class rdf:about="http://www.ontologyrepository.com/CommonCoreOntologies/Letter">
        <rdfs:subClassOf rdf:resource="http://www.ontologyrepository.com/CommonCoreOntologies/Grapheme"/>
        <skos:definition xml:lang="en">A Grapheme that consists of a single mark which is conventionally used in writing and printing to represent a speech sound and that is part of some alphabet.</skos:definition>
        <rdfs:label xml:lang="en">Letter</rdfs:label>
        <cco2:ont00001760 rdf:datatype="http://www.w3.org/2001/XMLSchema#anyURI">http://www.ontologyrepository.com/CommonCoreOntologies/Domain/CyberOntology</cco2:ont00001760>
    </owl:Class>
    


    <!-- http://www.ontologyrepository.com/CommonCoreOntologies/LocalAreaNetwork -->

    <owl:Class rdf:about="http://www.ontologyrepository.com/CommonCoreOntologies/LocalAreaNetwork">
        <rdfs:subClassOf rdf:resource="https://www.commoncoreontologies.org/ont00000700"/>
        <skos:altLabel xml:lang="en">LAN</skos:altLabel>
        <skos:definition xml:lang="en">A Computer Network that is designed to connect several resources within a small area (e.g., a building).</skos:definition>
        <rdfs:label xml:lang="en">Local Area Network</rdfs:label>
        <cco2:ont00001754>https://kb.iu.edu/d/agki</cco2:ont00001754>
        <cco2:ont00001760 rdf:datatype="http://www.w3.org/2001/XMLSchema#anyURI">http://www.ontologyrepository.com/CommonCoreOntologies/Domain/CyberOntology</cco2:ont00001760>
    </owl:Class>
    


    <!-- http://www.ontologyrepository.com/CommonCoreOntologies/LowLevelProgrammingLanguage -->

    <owl:Class rdf:about="http://www.ontologyrepository.com/CommonCoreOntologies/LowLevelProgrammingLanguage">
        <rdfs:subClassOf rdf:resource="http://www.ontologyrepository.com/CommonCoreOntologies/ProgrammingLanguage"/>
        <skos:definition xml:lang="en">A Programming Language that provides little or no abstraction from the language necessary for a set of instructions to be executed by a Processing Unit.</skos:definition>
        <rdfs:label xml:lang="en">Low-Level Programming Language</rdfs:label>
        <cco2:ont00001760 rdf:datatype="http://www.w3.org/2001/XMLSchema#anyURI">http://www.ontologyrepository.com/CommonCoreOntologies/Domain/CyberOntology</cco2:ont00001760>
    </owl:Class>
    


    <!-- http://www.ontologyrepository.com/CommonCoreOntologies/MacOperatingSystemSoftwareModel -->

    <owl:Class rdf:about="http://www.ontologyrepository.com/CommonCoreOntologies/MacOperatingSystemSoftwareModel">
        <rdfs:subClassOf rdf:resource="http://www.ontologyrepository.com/CommonCoreOntologies/UnixOperatingSystemModel"/>
        <skos:altLabel xml:lang="en">MacOS</skos:altLabel>
        <skos:altLabel xml:lang="en">Windows</skos:altLabel>
        <skos:definition xml:lang="en">A Unix Operating System Software Model that is developed and marketed by Apple Inc for its Mac personal computers.</skos:definition>
        <rdfs:label xml:lang="en">Mac Operating System Software Model</rdfs:label>
        <cco2:ont00001754 rdf:datatype="http://www.w3.org/2001/XMLSchema#anyURI">https://en.wikipedia.org/wiki/MacOS</cco2:ont00001754>
        <cco2:ont00001760 rdf:datatype="http://www.w3.org/2001/XMLSchema#anyURI">http://www.ontologyrepository.com/CommonCoreOntologies/Domain/CyberOntology</cco2:ont00001760>
    </owl:Class>
    


    <!-- http://www.ontologyrepository.com/CommonCoreOntologies/MachineLanguage -->

    <owl:Class rdf:about="http://www.ontologyrepository.com/CommonCoreOntologies/MachineLanguage">
        <rdfs:subClassOf rdf:resource="http://www.ontologyrepository.com/CommonCoreOntologies/LowLevelProgrammingLanguage"/>
        <skos:definition xml:lang="en">A Programming Language that prescribes a canonical form of communicating instructions to be executed directly by a Processing Unit.</skos:definition>
        <rdfs:label xml:lang="en">Machine Language</rdfs:label>
        <cco2:ont00001754>https://en.wikipedia.org/wiki/Machine_code</cco2:ont00001754>
        <cco2:ont00001760 rdf:datatype="http://www.w3.org/2001/XMLSchema#anyURI">http://www.ontologyrepository.com/CommonCoreOntologies/Domain/CyberOntology</cco2:ont00001760>
    </owl:Class>
    


    <!-- http://www.ontologyrepository.com/CommonCoreOntologies/MainframeComputer -->

    <owl:Class rdf:about="http://www.ontologyrepository.com/CommonCoreOntologies/MainframeComputer">
        <rdfs:subClassOf rdf:resource="https://www.commoncoreontologies.org/ont00000420"/>
        <skos:definition xml:lang="en">A Computer that is designed to be used primarily by large organizations for critical applications, bulk data processing, enterprise resource planning, and transaction processing.</skos:definition>
        <rdfs:label xml:lang="en">Mainframe Computer</rdfs:label>
        <cco2:ont00001754>https://en.wikipedia.org/wiki/Mainframe_computer</cco2:ont00001754>
        <cco2:ont00001760 rdf:datatype="http://www.w3.org/2001/XMLSchema#anyURI">http://www.ontologyrepository.com/CommonCoreOntologies/Domain/CyberOntology</cco2:ont00001760>
    </owl:Class>
    


    <!-- http://www.ontologyrepository.com/CommonCoreOntologies/MaliciousAdware -->

    <owl:Class rdf:about="http://www.ontologyrepository.com/CommonCoreOntologies/MaliciousAdware">
        <owl:equivalentClass>
            <owl:Class>
                <owl:intersectionOf rdf:parseType="Collection">
                    <rdf:Description rdf:about="http://www.ontologyrepository.com/CommonCoreOntologies/Adware"/>
                    <owl:Restriction>
                        <owl:onProperty rdf:resource="https://www.commoncoreontologies.org/ont00001787"/>
                        <owl:someValuesFrom rdf:resource="http://www.ontologyrepository.com/CommonCoreOntologies/CyberAttack"/>
                    </owl:Restriction>
                </owl:intersectionOf>
            </owl:Class>
        </owl:equivalentClass>
        <rdfs:subClassOf rdf:resource="http://www.ontologyrepository.com/CommonCoreOntologies/Adware"/>
        <skos:definition xml:lang="en">Adware that is an agent in some Cyber Attack..</skos:definition>
        <rdfs:label xml:lang="en">Malicious Adware</rdfs:label>
        <cco2:ont00001760 rdf:datatype="http://www.w3.org/2001/XMLSchema#anyURI">http://www.ontologyrepository.com/CommonCoreOntologies/Domain/CyberOntology</cco2:ont00001760>
    </owl:Class>
    


    <!-- http://www.ontologyrepository.com/CommonCoreOntologies/MaliciousCode -->

    <owl:Class rdf:about="http://www.ontologyrepository.com/CommonCoreOntologies/MaliciousCode">
        <owl:equivalentClass>
            <owl:Class>
                <owl:intersectionOf rdf:parseType="Collection">
                    <rdf:Description rdf:about="http://www.ontologyrepository.com/CommonCoreOntologies/Subroutine"/>
                    <owl:Restriction>
                        <owl:onProperty rdf:resource="https://www.commoncoreontologies.org/ont00001841"/>
                        <owl:someValuesFrom rdf:resource="http://www.ontologyrepository.com/CommonCoreOntologies/CyberAttack"/>
                    </owl:Restriction>
                </owl:intersectionOf>
            </owl:Class>
        </owl:equivalentClass>
        <rdfs:subClassOf rdf:resource="http://www.ontologyrepository.com/CommonCoreOntologies/Subroutine"/>
        <skos:definition xml:lang="en">A Subroutine that is input of a Cyber Attack.</skos:definition>
        <rdfs:label xml:lang="en">Malicious Code</rdfs:label>
        <cco2:ont00001760 rdf:datatype="http://www.w3.org/2001/XMLSchema#anyURI">http://www.ontologyrepository.com/CommonCoreOntologies/Domain/CyberOntology</cco2:ont00001760>
    </owl:Class>
    


    <!-- http://www.ontologyrepository.com/CommonCoreOntologies/MaliciousSpyware -->

    <owl:Class rdf:about="http://www.ontologyrepository.com/CommonCoreOntologies/MaliciousSpyware">
        <owl:equivalentClass>
            <owl:Class>
                <owl:intersectionOf rdf:parseType="Collection">
                    <rdf:Description rdf:about="http://www.ontologyrepository.com/CommonCoreOntologies/Spyware"/>
                    <owl:Restriction>
                        <owl:onProperty rdf:resource="https://www.commoncoreontologies.org/ont00001787"/>
                        <owl:someValuesFrom rdf:resource="http://www.ontologyrepository.com/CommonCoreOntologies/CyberAttack"/>
                    </owl:Restriction>
                </owl:intersectionOf>
            </owl:Class>
        </owl:equivalentClass>
        <rdfs:subClassOf rdf:resource="http://www.ontologyrepository.com/CommonCoreOntologies/Spyware"/>
        <skos:definition xml:lang="en">Spyware that is an agent in a Cyber Attack.</skos:definition>
        <rdfs:label xml:lang="en">Malicious Spyware</rdfs:label>
        <cco2:ont00001760 rdf:datatype="http://www.w3.org/2001/XMLSchema#anyURI">http://www.ontologyrepository.com/CommonCoreOntologies/Domain/CyberOntology</cco2:ont00001760>
    </owl:Class>
    


    <!-- http://www.ontologyrepository.com/CommonCoreOntologies/Malware -->

    <owl:Class rdf:about="http://www.ontologyrepository.com/CommonCoreOntologies/Malware">
        <owl:equivalentClass>
            <owl:Class>
                <owl:intersectionOf rdf:parseType="Collection">
                    <rdf:Description rdf:about="http://www.ontologyrepository.com/CommonCoreOntologies/ComputerProgram"/>
                    <owl:Restriction>
                        <owl:onProperty rdf:resource="https://www.commoncoreontologies.org/ont00001787"/>
                        <owl:someValuesFrom rdf:resource="http://www.ontologyrepository.com/CommonCoreOntologies/CyberAttack"/>
                    </owl:Restriction>
                </owl:intersectionOf>
            </owl:Class>
        </owl:equivalentClass>
        <rdfs:subClassOf rdf:resource="http://www.ontologyrepository.com/CommonCoreOntologies/ComputerProgram"/>
        <rdfs:subClassOf>
            <owl:Restriction>
                <owl:onProperty rdf:resource="http://purl.obolibrary.org/obo/BFO_0000178"/>
                <owl:someValuesFrom rdf:resource="http://www.ontologyrepository.com/CommonCoreOntologies/MaliciousCode"/>
            </owl:Restriction>
        </rdfs:subClassOf>
        <skos:definition xml:lang="en">A Computer Program that is an agent in a Cyber Attack.</skos:definition>
        <rdfs:label xml:lang="en">Malware</rdfs:label>
        <cco2:ont00001760 rdf:datatype="http://www.w3.org/2001/XMLSchema#anyURI">http://www.ontologyrepository.com/CommonCoreOntologies/Domain/CyberOntology</cco2:ont00001760>
    </owl:Class>
    


    <!-- http://www.ontologyrepository.com/CommonCoreOntologies/MarkupLanguage -->

    <owl:Class rdf:about="http://www.ontologyrepository.com/CommonCoreOntologies/MarkupLanguage">
        <rdfs:subClassOf rdf:resource="http://www.ontologyrepository.com/CommonCoreOntologies/ComputerLanguage"/>
        <skos:definition xml:lang="en">A Computer Language that prescribes a canonical form of annotating the structure of some text.</skos:definition>
        <rdfs:label xml:lang="en">Markup Language</rdfs:label>
        <cco2:ont00001754>https://en.wikipedia.org/wiki/Markup_language</cco2:ont00001754>
        <cco2:ont00001760 rdf:datatype="http://www.w3.org/2001/XMLSchema#anyURI">http://www.ontologyrepository.com/CommonCoreOntologies/Domain/CyberOntology</cco2:ont00001760>
    </owl:Class>
    


    <!-- http://www.ontologyrepository.com/CommonCoreOntologies/Matrix -->

    <owl:Class rdf:about="http://www.ontologyrepository.com/CommonCoreOntologies/Matrix">
        <rdfs:subClassOf rdf:resource="http://www.ontologyrepository.com/CommonCoreOntologies/Array"/>
        <skos:definition xml:lang="en">An Array which orders its elements along two dimensions.</skos:definition>
        <rdfs:label xml:lang="en">Matrix</rdfs:label>
        <cco2:ont00001760 rdf:datatype="http://www.w3.org/2001/XMLSchema#anyURI">http://www.ontologyrepository.com/CommonCoreOntologies/Domain/CyberOntology</cco2:ont00001760>
    </owl:Class>
    


    <!-- http://www.ontologyrepository.com/CommonCoreOntologies/MediaAccessControlAddress -->

    <owl:Class rdf:about="http://www.ontologyrepository.com/CommonCoreOntologies/MediaAccessControlAddress">
        <rdfs:subClassOf rdf:resource="https://www.commoncoreontologies.org/ont00000077"/>
        <skos:altLabel xml:lang="en">MAC Address</skos:altLabel>
        <skos:definition xml:lang="en">A Code Identifier that designates a Computer and is assigned to network interfaces for communications at the data link layer of a network segment.</skos:definition>
        <rdfs:label xml:lang="en">Media Access Control Address</rdfs:label>
        <cco2:ont00001754>https://en.wikipedia.org/wiki/MAC_address</cco2:ont00001754>
        <cco2:ont00001760 rdf:datatype="http://www.w3.org/2001/XMLSchema#anyURI">http://www.ontologyrepository.com/CommonCoreOntologies/Domain/CyberOntology</cco2:ont00001760>
    </owl:Class>
    


    <!-- http://www.ontologyrepository.com/CommonCoreOntologies/MemoryCorruption -->

    <owl:Class rdf:about="http://www.ontologyrepository.com/CommonCoreOntologies/MemoryCorruption">
        <rdfs:subClassOf rdf:resource="http://www.ontologyrepository.com/CommonCoreOntologies/CyberVulnerability"/>
        <skos:definition xml:lang="en">A Cyber Vulnerability that is realized by a Cyber Attack which writes to memory outside the bounds of a buffer, when the root cause is something other than a sequential copies of excessive data from a fixed starting location.</skos:definition>
        <rdfs:comment xml:lang="en">This may include issues such as incorrect pointer arithmetic, accessing invalid pointers due to incomplete initialization or memory release, etc</rdfs:comment>
        <rdfs:label xml:lang="en">Memory Corruption</rdfs:label>
        <cco2:ont00001760 rdf:datatype="http://www.w3.org/2001/XMLSchema#anyURI">http://www.ontologyrepository.com/CommonCoreOntologies/Domain/CyberOntology</cco2:ont00001760>
    </owl:Class>
    


    <!-- http://www.ontologyrepository.com/CommonCoreOntologies/MemoryTester -->

    <owl:Class rdf:about="http://www.ontologyrepository.com/CommonCoreOntologies/MemoryTester">
        <rdfs:subClassOf rdf:resource="http://www.ontologyrepository.com/CommonCoreOntologies/UtilityProgram"/>
        <skos:definition xml:lang="en">A Utility Program that is designed to test and verify modules of Computer Memory.</skos:definition>
        <rdfs:label xml:lang="en">Memory Tester</rdfs:label>
        <cco2:ont00001754>https://en.wikipedia.org/wiki/Memory_tester</cco2:ont00001754>
        <cco2:ont00001760 rdf:datatype="http://www.w3.org/2001/XMLSchema#anyURI">http://www.ontologyrepository.com/CommonCoreOntologies/Domain/CyberOntology</cco2:ont00001760>
    </owl:Class>
    


    <!-- http://www.ontologyrepository.com/CommonCoreOntologies/MetropolitanAreaNetwork -->

    <owl:Class rdf:about="http://www.ontologyrepository.com/CommonCoreOntologies/MetropolitanAreaNetwork">
        <rdfs:subClassOf rdf:resource="https://www.commoncoreontologies.org/ont00000700"/>
        <skos:altLabel xml:lang="en">MAN</skos:altLabel>
        <skos:definition xml:lang="en">A Computer Network that is designed to connect several resources within a City.</skos:definition>
        <rdfs:label xml:lang="en">Metropolitan Area Network</rdfs:label>
        <cco2:ont00001754>https://kb.iu.edu/d/agki</cco2:ont00001754>
        <cco2:ont00001760 rdf:datatype="http://www.w3.org/2001/XMLSchema#anyURI">http://www.ontologyrepository.com/CommonCoreOntologies/Domain/CyberOntology</cco2:ont00001760>
    </owl:Class>
    


    <!-- http://www.ontologyrepository.com/CommonCoreOntologies/Microblog -->

    <owl:Class rdf:about="http://www.ontologyrepository.com/CommonCoreOntologies/Microblog">
        <rdfs:subClassOf rdf:resource="http://www.ontologyrepository.com/CommonCoreOntologies/Blog"/>
        <skos:definition xml:lang="en">A Blog that consists of short posts which can be shared online by other users.</skos:definition>
        <rdfs:label xml:lang="en">Microblog</rdfs:label>
        <cco2:ont00001760 rdf:datatype="http://www.w3.org/2001/XMLSchema#anyURI">http://www.ontologyrepository.com/CommonCoreOntologies/Domain/CyberOntology</cco2:ont00001760>
    </owl:Class>
    


    <!-- http://www.ontologyrepository.com/CommonCoreOntologies/Morpheme -->

    <owl:Class rdf:about="http://www.ontologyrepository.com/CommonCoreOntologies/Morpheme">
        <rdfs:subClassOf rdf:resource="http://www.ontologyrepository.com/CommonCoreOntologies/WrittenSymbol"/>
        <skos:definition xml:lang="en">A Written Symbol that is the smallest meaningful unit of a writing system and which may or may not be freestanding.</skos:definition>
        <skos:example>The morpheme &apos;cat&apos;</skos:example>
        <skos:example>The prefix &apos;ante&apos;</skos:example>
        <skos:example>The word &apos;unbreakable&apos; consists of 3 morphemes: &apos;un-&apos;, &apos;-break-&apos; and &apos;-able&apos;.</skos:example>
        <rdfs:label xml:lang="en">Morpheme</rdfs:label>
        <cco2:ont00001760 rdf:datatype="http://www.w3.org/2001/XMLSchema#anyURI">http://www.ontologyrepository.com/CommonCoreOntologies/Domain/CyberOntology</cco2:ont00001760>
    </owl:Class>
    


    <!-- http://www.ontologyrepository.com/CommonCoreOntologies/MultiModelDatabaseSoftwareApplicationModel -->

    <owl:Class rdf:about="http://www.ontologyrepository.com/CommonCoreOntologies/MultiModelDatabaseSoftwareApplicationModel">
        <rdfs:subClassOf rdf:resource="http://www.ontologyrepository.com/CommonCoreOntologies/DatabaseSoftwareApplicationModel"/>
        <skos:definition xml:lang="en">A Database Software Application Model that prescribes a Database Software Application where the data is stored using more than one data model.</skos:definition>
        <rdfs:label xml:lang="en">Multi-Model Database Software Application Model</rdfs:label>
        <cco2:ont00001760 rdf:datatype="http://www.w3.org/2001/XMLSchema#anyURI">http://www.ontologyrepository.com/CommonCoreOntologies/Domain/CyberOntology</cco2:ont00001760>
    </owl:Class>
    


    <!-- http://www.ontologyrepository.com/CommonCoreOntologies/MultimediaSoftwareApplication -->

    <owl:Class rdf:about="http://www.ontologyrepository.com/CommonCoreOntologies/MultimediaSoftwareApplication">
        <rdfs:subClassOf rdf:resource="http://www.ontologyrepository.com/CommonCoreOntologies/InformationWorkerSoftware"/>
        <skos:definition xml:lang="en">An Information Worker Software Application that is designed to enable a user to create and edit Images, Audio Files, and Videos.</skos:definition>
        <rdfs:label xml:lang="en">Multimedia Software Application</rdfs:label>
        <cco2:ont00001760 rdf:datatype="http://www.w3.org/2001/XMLSchema#anyURI">http://www.ontologyrepository.com/CommonCoreOntologies/Domain/CyberOntology</cco2:ont00001760>
    </owl:Class>
    


    <!-- http://www.ontologyrepository.com/CommonCoreOntologies/NetworkCommunicationWaitingStatus -->

    <owl:Class rdf:about="http://www.ontologyrepository.com/CommonCoreOntologies/NetworkCommunicationWaitingStatus">
        <rdfs:subClassOf rdf:resource="https://www.commoncoreontologies.org/ont00000847"/>
        <skos:definition xml:lang="en">An Active Stasis in which some resource on a network is waiting to receive messages from other resources it is connected to on that network.</skos:definition>
        <rdfs:comment xml:lang="en">Instances of this class can be combined with instances of other classes to represent various TCP states, including: CLOSE WAIT, CLOSING, FIN-WAIT-1, FIN-WAIT-2, LAST ACK, SYN RECEIVED, SYN SENT, and TIME WAIT.</rdfs:comment>
        <rdfs:label xml:lang="en">Network Communication Waiting Status</rdfs:label>
        <cco2:ont00001760 rdf:datatype="http://www.w3.org/2001/XMLSchema#anyURI">http://www.ontologyrepository.com/CommonCoreOntologies/Domain/CyberOntology</cco2:ont00001760>
    </owl:Class>
    


    <!-- http://www.ontologyrepository.com/CommonCoreOntologies/NetworkConnectionClosed -->

    <owl:Class rdf:about="http://www.ontologyrepository.com/CommonCoreOntologies/NetworkConnectionClosed">
        <rdfs:subClassOf rdf:resource="https://www.commoncoreontologies.org/ont00000936"/>
        <skos:definition xml:lang="en">A Deactivated Stasis in which multiple resources connected over a network are not connected via their designed communication functions.</skos:definition>
        <rdfs:label xml:lang="en">Network Connection Closed</rdfs:label>
        <cco2:ont00001760 rdf:datatype="http://www.w3.org/2001/XMLSchema#anyURI">http://www.ontologyrepository.com/CommonCoreOntologies/Domain/CyberOntology</cco2:ont00001760>
    </owl:Class>
    


    <!-- http://www.ontologyrepository.com/CommonCoreOntologies/NetworkConnectionEstablished -->

    <owl:Class rdf:about="http://www.ontologyrepository.com/CommonCoreOntologies/NetworkConnectionEstablished">
        <rdfs:subClassOf rdf:resource="https://www.commoncoreontologies.org/ont00000847"/>
        <skos:definition xml:lang="en">An Active Stasis in which multiple resources connected over a network are connected via their designed communication functions.</skos:definition>
        <rdfs:label xml:lang="en">Network Connection Established</rdfs:label>
        <cco2:ont00001760 rdf:datatype="http://www.w3.org/2001/XMLSchema#anyURI">http://www.ontologyrepository.com/CommonCoreOntologies/Domain/CyberOntology</cco2:ont00001760>
    </owl:Class>
    


    <!-- http://www.ontologyrepository.com/CommonCoreOntologies/NetworkConnectionExecution -->

    <owl:Class rdf:about="http://www.ontologyrepository.com/CommonCoreOntologies/NetworkConnectionExecution">
        <rdfs:subClassOf rdf:resource="http://www.ontologyrepository.com/CommonCoreOntologies/ComputerProgramExecution"/>
        <skos:definition xml:lang="en">A Computer Program Execution in which two resources are connected or unconnected on a network.</skos:definition>
        <rdfs:label xml:lang="en">Network Connection Execution</rdfs:label>
        <cco2:ont00001760 rdf:datatype="http://www.w3.org/2001/XMLSchema#anyURI">http://www.ontologyrepository.com/CommonCoreOntologies/Domain/CyberOntology</cco2:ont00001760>
    </owl:Class>
    


    <!-- http://www.ontologyrepository.com/CommonCoreOntologies/NetworkConnectionInitiated -->

    <owl:Class rdf:about="http://www.ontologyrepository.com/CommonCoreOntologies/NetworkConnectionInitiated">
        <rdfs:subClassOf rdf:resource="http://www.ontologyrepository.com/CommonCoreOntologies/NetworkConnectionExecution"/>
        <skos:definition xml:lang="en">A Computer Program Execution in which two previously unconnected resources become connected on a network.</skos:definition>
        <rdfs:comment xml:lang="en">For the state of two resources being connected see Network Connection Established.</rdfs:comment>
        <rdfs:label xml:lang="en">Network Connection Initiation</rdfs:label>
        <cco2:ont00001760 rdf:datatype="http://www.w3.org/2001/XMLSchema#anyURI">http://www.ontologyrepository.com/CommonCoreOntologies/Domain/CyberOntology</cco2:ont00001760>
    </owl:Class>
    


    <!-- http://www.ontologyrepository.com/CommonCoreOntologies/NetworkConnectionTermination -->

    <owl:Class rdf:about="http://www.ontologyrepository.com/CommonCoreOntologies/NetworkConnectionTermination">
        <rdfs:subClassOf rdf:resource="http://www.ontologyrepository.com/CommonCoreOntologies/NetworkConnectionExecution"/>
        <skos:definition xml:lang="en">A Computer Program Execution in which two previously connected resources on a network become unconnected.</skos:definition>
        <rdfs:label xml:lang="en">Network Connection Termination</rdfs:label>
        <cco2:ont00001760 rdf:datatype="http://www.w3.org/2001/XMLSchema#anyURI">http://www.ontologyrepository.com/CommonCoreOntologies/Domain/CyberOntology</cco2:ont00001760>
    </owl:Class>
    


    <!-- http://www.ontologyrepository.com/CommonCoreOntologies/NetworkHost -->

    <owl:Class rdf:about="http://www.ontologyrepository.com/CommonCoreOntologies/NetworkHost">
        <rdfs:subClassOf rdf:resource="https://www.commoncoreontologies.org/ont00000117"/>
        <skos:definition xml:lang="en">An Information Processing Artifact that is part of a Computer Network.</skos:definition>
        <rdfs:label xml:lang="en">Network Host</rdfs:label>
        <cco2:ont00001754 rdf:datatype="http://www.w3.org/2001/XMLSchema#anyURI">https://en.wikipedia.org/wiki/Host_(network)</cco2:ont00001754>
        <cco2:ont00001760 rdf:datatype="http://www.w3.org/2001/XMLSchema#anyURI">http://www.ontologyrepository.com/CommonCoreOntologies/Domain/CyberOntology</cco2:ont00001760>
    </owl:Class>
    


    <!-- http://www.ontologyrepository.com/CommonCoreOntologies/NetworkHub -->

    <owl:Class rdf:about="http://www.ontologyrepository.com/CommonCoreOntologies/NetworkHub">
        <rdfs:subClassOf rdf:resource="http://www.ontologyrepository.com/CommonCoreOntologies/ComputerNetworkingDevice"/>
        <skos:definition xml:lang="en">A Computer Networking Device that connects multiple Ethernet devices together and making them act as a single network segment.</skos:definition>
        <rdfs:label xml:lang="en">Network Hub</rdfs:label>
        <cco2:ont00001754>https://en.wikipedia.org/wiki/Ethernet_hub</cco2:ont00001754>
        <cco2:ont00001760 rdf:datatype="http://www.w3.org/2001/XMLSchema#anyURI">http://www.ontologyrepository.com/CommonCoreOntologies/Domain/CyberOntology</cco2:ont00001760>
    </owl:Class>
    


    <!-- http://www.ontologyrepository.com/CommonCoreOntologies/NetworkIntrusionDetectionApplication -->

    <owl:Class rdf:about="http://www.ontologyrepository.com/CommonCoreOntologies/NetworkIntrusionDetectionApplication">
        <rdfs:subClassOf rdf:resource="http://www.ontologyrepository.com/CommonCoreOntologies/NetworkSecurityApplication"/>
        <skos:definition xml:lang="en">A Network Security Application that is designed to detect and alert users or administrators about successful or failed attempts from unauthorized agents to gain access to some Computer Network.</skos:definition>
        <rdfs:label xml:lang="en">Network Intrusion Detection Application</rdfs:label>
        <cco2:ont00001760 rdf:datatype="http://www.w3.org/2001/XMLSchema#anyURI">http://www.ontologyrepository.com/CommonCoreOntologies/Domain/CyberOntology</cco2:ont00001760>
    </owl:Class>
    


    <!-- http://www.ontologyrepository.com/CommonCoreOntologies/NetworkPacket -->

    <owl:Class rdf:about="http://www.ontologyrepository.com/CommonCoreOntologies/NetworkPacket">
        <rdfs:subClassOf rdf:resource="https://www.commoncoreontologies.org/ont00000798"/>
        <rdfs:subClassOf>
            <owl:Restriction>
                <owl:onProperty rdf:resource="http://purl.obolibrary.org/obo/BFO_0000178"/>
                <owl:someValuesFrom rdf:resource="http://www.ontologyrepository.com/CommonCoreOntologies/PacketHeader"/>
            </owl:Restriction>
        </rdfs:subClassOf>
        <skos:definition xml:lang="en">An Information Bearing Artifact that bears some collection of data that is meant to be communicated over some Computer Network.</skos:definition>
        <rdfs:label xml:lang="en">Network Packet</rdfs:label>
        <cco2:ont00001760 rdf:datatype="http://www.w3.org/2001/XMLSchema#anyURI">http://www.ontologyrepository.com/CommonCoreOntologies/Domain/CyberOntology</cco2:ont00001760>
    </owl:Class>
    


    <!-- http://www.ontologyrepository.com/CommonCoreOntologies/NetworkRouter -->

    <owl:Class rdf:about="http://www.ontologyrepository.com/CommonCoreOntologies/NetworkRouter">
        <rdfs:subClassOf rdf:resource="http://www.ontologyrepository.com/CommonCoreOntologies/ComputerNetworkingDevice"/>
        <skos:altLabel xml:lang="en">Router</skos:altLabel>
        <skos:definition xml:lang="en">A Computer Networking Device that connects multiple Computer Networks by forwarding data packets between them.</skos:definition>
        <rdfs:label xml:lang="en">Network Router</rdfs:label>
        <cco2:ont00001754>https://en.wikipedia.org/wiki/Router_(computing)</cco2:ont00001754>
        <cco2:ont00001760 rdf:datatype="http://www.w3.org/2001/XMLSchema#anyURI">http://www.ontologyrepository.com/CommonCoreOntologies/Domain/CyberOntology</cco2:ont00001760>
    </owl:Class>
    


    <!-- http://www.ontologyrepository.com/CommonCoreOntologies/NetworkSecurityApplication -->

    <owl:Class rdf:about="http://www.ontologyrepository.com/CommonCoreOntologies/NetworkSecurityApplication">
        <rdfs:subClassOf rdf:resource="http://www.ontologyrepository.com/CommonCoreOntologies/UtilityProgram"/>
        <skos:definition xml:lang="en">A Utility Program that is designed to protect the usability and integrity of some Computer Network and its data.</skos:definition>
        <rdfs:label xml:lang="en">Network Security Application</rdfs:label>
        <cco2:ont00001754>http://www.cisco.com/c/en/us/products/security/what-is-network-security.html</cco2:ont00001754>
        <cco2:ont00001760 rdf:datatype="http://www.w3.org/2001/XMLSchema#anyURI">http://www.ontologyrepository.com/CommonCoreOntologies/Domain/CyberOntology</cco2:ont00001760>
    </owl:Class>
    


    <!-- http://www.ontologyrepository.com/CommonCoreOntologies/NetworkServer -->

    <owl:Class rdf:about="http://www.ontologyrepository.com/CommonCoreOntologies/NetworkServer">
        <rdfs:subClassOf rdf:resource="http://www.ontologyrepository.com/CommonCoreOntologies/ComputerProgram"/>
        <skos:altLabel xml:lang="en">Server</skos:altLabel>
        <skos:definition xml:lang="en">A Computer Program that enables clients to access a Computer Service Function over a Computer Network.</skos:definition>
        <rdfs:label xml:lang="en">Network Server</rdfs:label>
        <cco2:ont00001760 rdf:datatype="http://www.w3.org/2001/XMLSchema#anyURI">http://www.ontologyrepository.com/CommonCoreOntologies/Domain/CyberOntology</cco2:ont00001760>
    </owl:Class>
    


    <!-- http://www.ontologyrepository.com/CommonCoreOntologies/NetworkServiceFunction -->

    <owl:Class rdf:about="http://www.ontologyrepository.com/CommonCoreOntologies/NetworkServiceFunction">
        <rdfs:subClassOf rdf:resource="http://www.ontologyrepository.com/CommonCoreOntologies/InformationProcessingArtifactFunction"/>
        <skos:altLabel xml:lang="en">Network Service</skos:altLabel>
        <skos:definition xml:lang="en">An Information Processing Artifact Function that when realized is in a process of a client accessing some other Information Processing Artifact Function, called a service, over a Computer Network.</skos:definition>
        <rdfs:comment xml:lang="en">&apos;Service&apos; typically refers to the functionality of some program, or other resource, e.g., file management. The ability for a server to provide that functionality requires the existence of an additional function, which is what these classes are designed to represent. However, the service-enabling function is different from the service itself. Since many types of programs and other information processing artifacts can be offered as services, it doesn’t make sense to create duplicate terms for when an application is a service vs. when it isn’t. By analogy, consider a pizza restaurant that offers dine-in, take-out, and delivery options. These three modes of getting your pizza don’t make for three different kinds of pizza. Same pizza, same restaurant, different ways of accessing.</rdfs:comment>
        <rdfs:label xml:lang="en">Network Service Function</rdfs:label>
        <cco2:ont00001760 rdf:datatype="http://www.w3.org/2001/XMLSchema#anyURI">http://www.ontologyrepository.com/CommonCoreOntologies/Domain/CyberOntology</cco2:ont00001760>
    </owl:Class>
    


    <!-- http://www.ontologyrepository.com/CommonCoreOntologies/NetworkSwitch -->

    <owl:Class rdf:about="http://www.ontologyrepository.com/CommonCoreOntologies/NetworkSwitch">
        <rdfs:subClassOf rdf:resource="http://www.ontologyrepository.com/CommonCoreOntologies/ComputerNetworkingDevice"/>
        <skos:altLabel xml:lang="en">Switch</skos:altLabel>
        <skos:definition xml:lang="en">A Computer Networking Device that connects devices together on a single Computer Network by using packet switching to receive, process, and forward data to the destination device.</skos:definition>
        <rdfs:label xml:lang="en">Network Switch</rdfs:label>
        <cco2:ont00001754>https://en.wikipedia.org/wiki/Network_switch</cco2:ont00001754>
        <cco2:ont00001760 rdf:datatype="http://www.w3.org/2001/XMLSchema#anyURI">http://www.ontologyrepository.com/CommonCoreOntologies/Domain/CyberOntology</cco2:ont00001760>
    </owl:Class>
    


    <!-- http://www.ontologyrepository.com/CommonCoreOntologies/NetworkUtility -->

    <owl:Class rdf:about="http://www.ontologyrepository.com/CommonCoreOntologies/NetworkUtility">
        <rdfs:subClassOf rdf:resource="http://www.ontologyrepository.com/CommonCoreOntologies/UtilityProgram"/>
        <skos:definition xml:lang="en">A Utility Program that is designed to analyze and configure various aspects of a Computer Network.</skos:definition>
        <rdfs:label xml:lang="en">Network Utility</rdfs:label>
        <cco2:ont00001754>https://en.wikipedia.org/wiki/Network_utility</cco2:ont00001754>
        <cco2:ont00001760 rdf:datatype="http://www.w3.org/2001/XMLSchema#anyURI">http://www.ontologyrepository.com/CommonCoreOntologies/Domain/CyberOntology</cco2:ont00001760>
    </owl:Class>
    


    <!-- http://www.ontologyrepository.com/CommonCoreOntologies/Node -->

    <owl:Class rdf:about="http://www.ontologyrepository.com/CommonCoreOntologies/Node">
        <rdfs:subClassOf rdf:resource="https://www.commoncoreontologies.org/ont00000798"/>
        <skos:altLabel xml:lang="en">Vertex</skos:altLabel>
        <skos:definition xml:lang="en">An Information Bearing Artifact that is a basic element in a graph data structure, which can be connected to other such elements by edges.</skos:definition>
        <rdfs:label xml:lang="en">Node</rdfs:label>
        <cco2:ont00001760 rdf:datatype="http://www.w3.org/2001/XMLSchema#anyURI">http://www.ontologyrepository.com/CommonCoreOntologies/Domain/CyberOntology</cco2:ont00001760>
    </owl:Class>
    


    <!-- http://www.ontologyrepository.com/CommonCoreOntologies/NodeAttribute -->

    <owl:Class rdf:about="http://www.ontologyrepository.com/CommonCoreOntologies/NodeAttribute">
        <rdfs:subClassOf rdf:resource="https://www.commoncoreontologies.org/ont00000798"/>
        <skos:definition xml:lang="en">An Information Bearing Artifact that is attached to a Node, and which typically bears information about that Node or what it represents.</skos:definition>
        <rdfs:label xml:lang="en">Node Attribute</rdfs:label>
        <cco2:ont00001760 rdf:datatype="http://www.w3.org/2001/XMLSchema#anyURI">http://www.ontologyrepository.com/CommonCoreOntologies/Domain/CyberOntology</cco2:ont00001760>
    </owl:Class>
    


    <!-- http://www.ontologyrepository.com/CommonCoreOntologies/NodeTrack -->

    <owl:Class rdf:about="http://www.ontologyrepository.com/CommonCoreOntologies/NodeTrack">
        <rdfs:subClassOf rdf:resource="https://www.commoncoreontologies.org/ont00000798"/>
        <skos:definition xml:lang="en">An Information Bearing Artifact that is an ordered sequence of Nodes.</skos:definition>
        <rdfs:label xml:lang="en">Node Track</rdfs:label>
        <cco2:ont00001760 rdf:datatype="http://www.w3.org/2001/XMLSchema#anyURI">http://www.ontologyrepository.com/CommonCoreOntologies/Domain/CyberOntology</cco2:ont00001760>
    </owl:Class>
    


    <!-- http://www.ontologyrepository.com/CommonCoreOntologies/NodeTree -->

    <owl:Class rdf:about="http://www.ontologyrepository.com/CommonCoreOntologies/NodeTree">
        <rdfs:subClassOf rdf:resource="https://www.commoncoreontologies.org/ont00000798"/>
        <skos:definition xml:lang="en">An Information Bearing Entity that consists of a hierarchy of Nodes with exactly one root Node.</skos:definition>
        <rdfs:label xml:lang="en">Node Tree</rdfs:label>
        <cco2:ont00001760 rdf:datatype="http://www.w3.org/2001/XMLSchema#anyURI">http://www.ontologyrepository.com/CommonCoreOntologies/Domain/CyberOntology</cco2:ont00001760>
    </owl:Class>
    


    <!-- http://www.ontologyrepository.com/CommonCoreOntologies/NoteManagementSoftwareApplication -->

    <owl:Class rdf:about="http://www.ontologyrepository.com/CommonCoreOntologies/NoteManagementSoftwareApplication">
        <rdfs:subClassOf rdf:resource="http://www.ontologyrepository.com/CommonCoreOntologies/InformationWorkerSoftware"/>
        <skos:definition xml:lang="en">An Information Worker Software Application that is designed to enable a user to record information captured from another source.</skos:definition>
        <rdfs:label xml:lang="en">Note Management Software Application</rdfs:label>
        <cco2:ont00001760 rdf:datatype="http://www.w3.org/2001/XMLSchema#anyURI">http://www.ontologyrepository.com/CommonCoreOntologies/Domain/CyberOntology</cco2:ont00001760>
    </owl:Class>
    


    <!-- http://www.ontologyrepository.com/CommonCoreOntologies/Ontology -->

    <owl:Class rdf:about="http://www.ontologyrepository.com/CommonCoreOntologies/Ontology">
        <rdfs:subClassOf rdf:resource="https://www.commoncoreontologies.org/ont00000798"/>
        <skos:definition xml:lang="en">An Information Bearing Artifact that is designed to represent types of entities and the relationships between them, and which can be encoded in a Computer Language.</skos:definition>
        <rdfs:label xml:lang="en">Ontology</rdfs:label>
        <cco2:ont00001754>R. Arp, B. Smith, and A.D. Spear, &quot;Building Ontologies with Basic Formal Ontology,&quot; Cambridge, MA: MIT Press, 2015</cco2:ont00001754>
        <cco2:ont00001760 rdf:datatype="http://www.w3.org/2001/XMLSchema#anyURI">http://www.ontologyrepository.com/CommonCoreOntologies/Domain/CyberOntology</cco2:ont00001760>
    </owl:Class>
    


    <!-- http://www.ontologyrepository.com/CommonCoreOntologies/OntologyEditingSoftwareApplication -->

    <owl:Class rdf:about="http://www.ontologyrepository.com/CommonCoreOntologies/OntologyEditingSoftwareApplication">
        <rdfs:subClassOf rdf:resource="http://www.ontologyrepository.com/CommonCoreOntologies/InformationWorkerSoftware"/>
        <skos:definition xml:lang="en">An Information Worker Software Application that is designed to enable a user to create and manage an Ontology.</skos:definition>
        <rdfs:label xml:lang="en">Ontology Editing Software Application</rdfs:label>
        <cco2:ont00001760 rdf:datatype="http://www.w3.org/2001/XMLSchema#anyURI">http://www.ontologyrepository.com/CommonCoreOntologies/Domain/CyberOntology</cco2:ont00001760>
    </owl:Class>
    


    <!-- http://www.ontologyrepository.com/CommonCoreOntologies/OpenSystemsInterconnectionCategory -->

    <owl:Class rdf:about="http://www.ontologyrepository.com/CommonCoreOntologies/OpenSystemsInterconnectionCategory">
        <rdfs:subClassOf rdf:resource="https://www.commoncoreontologies.org/ont00000293"/>
        <skos:altLabel xml:lang="en">OSI Category</skos:altLabel>
        <skos:definition xml:lang="en">A Nominal Measurement Information Content Entity that categorizes pieces of hardware or software based on their communication functionality.</skos:definition>
        <rdfs:label xml:lang="en">Open Systems Interconnection Category</rdfs:label>
        <cco2:ont00001754>https://en.wikipedia.org/wiki/OSI_model</cco2:ont00001754>
        <cco2:ont00001760 rdf:datatype="http://www.w3.org/2001/XMLSchema#anyURI">http://www.ontologyrepository.com/CommonCoreOntologies/Domain/CyberOntology</cco2:ont00001760>
    </owl:Class>
    


    <!-- http://www.ontologyrepository.com/CommonCoreOntologies/OperatingSystem -->

    <owl:Class rdf:about="http://www.ontologyrepository.com/CommonCoreOntologies/OperatingSystem">
        <rdfs:subClassOf rdf:resource="http://www.ontologyrepository.com/CommonCoreOntologies/SystemSoftware"/>
        <skos:altLabel xml:lang="en">OS</skos:altLabel>
        <skos:definition xml:lang="en">System Software that is designed to manage Computer hardware and software resources and provides common services for Computer Programs.</skos:definition>
        <rdfs:comment xml:lang="en">With the exception of firmware, all computer programs require an operating system to function.</rdfs:comment>
        <rdfs:label xml:lang="en">Operating System</rdfs:label>
        <cco2:ont00001754>https://en.wikipedia.org/wiki/Operating_system</cco2:ont00001754>
        <cco2:ont00001760 rdf:datatype="http://www.w3.org/2001/XMLSchema#anyURI">http://www.ontologyrepository.com/CommonCoreOntologies/Domain/CyberOntology</cco2:ont00001760>
    </owl:Class>
    


    <!-- http://www.ontologyrepository.com/CommonCoreOntologies/OperatingSystemSoftwareModel -->

    <owl:Class rdf:about="http://www.ontologyrepository.com/CommonCoreOntologies/OperatingSystemSoftwareModel">
        <rdfs:subClassOf rdf:resource="http://www.ontologyrepository.com/CommonCoreOntologies/ComputerProgramArtifactModel"/>
        <rdfs:subClassOf>
            <owl:Restriction>
                <owl:onProperty rdf:resource="https://www.commoncoreontologies.org/ont00001942"/>
                <owl:someValuesFrom rdf:resource="http://www.ontologyrepository.com/CommonCoreOntologies/OperatingSystem"/>
            </owl:Restriction>
        </rdfs:subClassOf>
        <skos:definition xml:lang="en">A Computer Program Artifact Model that prescribes some Operating System.</skos:definition>
        <rdfs:comment xml:lang="en">Subclasses of Operating System Model are fiat collections that group families of related models based on the developer or a shared evolutionary history. It is reasonable to assume these classes are best considered as enumerations of all the known models that belong in that family or developmental history.</rdfs:comment>
        <rdfs:label xml:lang="en">Operating System Software Model</rdfs:label>
        <cco2:ont00001760 rdf:datatype="http://www.w3.org/2001/XMLSchema#anyURI">http://www.ontologyrepository.com/CommonCoreOntologies/Domain/CyberOntology</cco2:ont00001760>
    </owl:Class>
    


    <!-- http://www.ontologyrepository.com/CommonCoreOntologies/OrderedPair -->

    <owl:Class rdf:about="http://www.ontologyrepository.com/CommonCoreOntologies/OrderedPair">
        <rdfs:subClassOf rdf:resource="http://www.ontologyrepository.com/CommonCoreOntologies/Tuple"/>
        <skos:definition xml:lang="en">A Tuple which consists of exactly two ordered elements.</skos:definition>
        <rdfs:label xml:lang="en">Ordered Pair</rdfs:label>
        <cco2:ont00001760 rdf:datatype="http://www.w3.org/2001/XMLSchema#anyURI">http://www.ontologyrepository.com/CommonCoreOntologies/Domain/CyberOntology</cco2:ont00001760>
    </owl:Class>
    


    <!-- http://www.ontologyrepository.com/CommonCoreOntologies/OrphanComputerProgramExecution -->

    <owl:Class rdf:about="http://www.ontologyrepository.com/CommonCoreOntologies/OrphanComputerProgramExecution">
        <rdfs:subClassOf rdf:resource="http://www.ontologyrepository.com/CommonCoreOntologies/ChildComputerProgramExecution"/>
        <skos:altLabel xml:lang="en">Orphan Computer Process</skos:altLabel>
        <skos:definition xml:lang="en">A Child Computer Program Execution whose Parent Computer Process has terminated.</skos:definition>
        <rdfs:comment xml:lang="en">Shall be axiomatized as an equivalency, eg. Child Program Execution and process started by some (Computer Program Execution and participates in some Terminated Stasis).</rdfs:comment>
        <rdfs:label xml:lang="en">Orphan Computer Program Execution</rdfs:label>
        <cco2:ont00001754 rdf:datatype="http://www.w3.org/2001/XMLSchema#anyURI">https://en.wikipedia.org/wiki/Orphan_process</cco2:ont00001754>
        <cco2:ont00001760 rdf:datatype="http://www.w3.org/2001/XMLSchema#anyURI">http://www.ontologyrepository.com/CommonCoreOntologies/Domain/CyberOntology</cco2:ont00001760>
    </owl:Class>
    


    <!-- http://www.ontologyrepository.com/CommonCoreOntologies/OutputDevice -->

    <owl:Class rdf:about="http://www.ontologyrepository.com/CommonCoreOntologies/OutputDevice">
        <rdfs:subClassOf rdf:resource="http://www.ontologyrepository.com/CommonCoreOntologies/ComputerComponent"/>
        <skos:definition xml:lang="en">A Computer Component that converts information into human-understandable form</skos:definition>
        <rdfs:label xml:lang="en">Output Device</rdfs:label>
        <cco2:ont00001754 rdf:datatype="http://www.w3.org/2001/XMLSchema#anyURI">https://en.wikipedia.org/wiki/Output_device</cco2:ont00001754>
        <cco2:ont00001760 rdf:datatype="http://www.w3.org/2001/XMLSchema#anyURI">http://www.ontologyrepository.com/CommonCoreOntologies/Domain/CyberOntology</cco2:ont00001760>
    </owl:Class>
    


    <!-- http://www.ontologyrepository.com/CommonCoreOntologies/OverlayNetwork -->

    <owl:Class rdf:about="http://www.ontologyrepository.com/CommonCoreOntologies/OverlayNetwork">
        <rdfs:subClassOf rdf:resource="https://www.commoncoreontologies.org/ont00000700"/>
        <skos:definition xml:lang="en">A Computer Network that is built on top of another Computer Network.</skos:definition>
        <rdfs:label xml:lang="en">Overlay Network</rdfs:label>
        <cco2:ont00001754>https://en.wikipedia.org/wiki/Overlay_network</cco2:ont00001754>
        <cco2:ont00001760 rdf:datatype="http://www.w3.org/2001/XMLSchema#anyURI">http://www.ontologyrepository.com/CommonCoreOntologies/Domain/CyberOntology</cco2:ont00001760>
    </owl:Class>
    


    <!-- http://www.ontologyrepository.com/CommonCoreOntologies/PackageManager -->

    <owl:Class rdf:about="http://www.ontologyrepository.com/CommonCoreOntologies/PackageManager">
        <rdfs:subClassOf rdf:resource="http://www.ontologyrepository.com/CommonCoreOntologies/UtilityProgram"/>
        <skos:definition xml:lang="en">A Utility Program that is designed to automate the process of installing, upgrading, configuring, and removing Computer Programs for a Computer&apos;s Operating System.</skos:definition>
        <rdfs:label xml:lang="en">Package Manager</rdfs:label>
        <cco2:ont00001754>https://en.wikipedia.org/wiki/Package_manager</cco2:ont00001754>
        <cco2:ont00001760 rdf:datatype="http://www.w3.org/2001/XMLSchema#anyURI">http://www.ontologyrepository.com/CommonCoreOntologies/Domain/CyberOntology</cco2:ont00001760>
    </owl:Class>
    


    <!-- http://www.ontologyrepository.com/CommonCoreOntologies/PacketHeader -->

    <owl:Class rdf:about="http://www.ontologyrepository.com/CommonCoreOntologies/PacketHeader">
        <rdfs:subClassOf rdf:resource="http://www.ontologyrepository.com/CommonCoreOntologies/InformationHeader"/>
        <rdfs:subClassOf>
            <owl:Restriction>
                <owl:onProperty rdf:resource="http://purl.obolibrary.org/obo/BFO_0000176"/>
                <owl:someValuesFrom rdf:resource="http://www.ontologyrepository.com/CommonCoreOntologies/NetworkPacket"/>
            </owl:Restriction>
        </rdfs:subClassOf>
        <skos:definition xml:lang="en">A Information Header that is part of some Computer Packet.</skos:definition>
        <rdfs:label xml:lang="en">Packet Header</rdfs:label>
        <cco2:ont00001760 rdf:datatype="http://www.w3.org/2001/XMLSchema#anyURI">http://www.ontologyrepository.com/CommonCoreOntologies/Domain/CyberOntology</cco2:ont00001760>
    </owl:Class>
    


    <!-- http://www.ontologyrepository.com/CommonCoreOntologies/PacketTransfer -->

    <owl:Class rdf:about="http://www.ontologyrepository.com/CommonCoreOntologies/PacketTransfer">
        <rdfs:subClassOf rdf:resource="http://www.ontologyrepository.com/CommonCoreOntologies/DataTransfer"/>
        <skos:definition xml:lang="en">A Data Transfer in which a Network Packet is transmitted from one Computer to another.</skos:definition>
        <rdfs:label xml:lang="en">Packet Transfer</rdfs:label>
        <cco2:ont00001760 rdf:datatype="http://www.w3.org/2001/XMLSchema#anyURI">http://www.ontologyrepository.com/CommonCoreOntologies/Domain/CyberOntology</cco2:ont00001760>
    </owl:Class>
    


    <!-- http://www.ontologyrepository.com/CommonCoreOntologies/ParentComputerProgramExecution -->

    <owl:Class rdf:about="http://www.ontologyrepository.com/CommonCoreOntologies/ParentComputerProgramExecution">
        <owl:equivalentClass>
            <owl:Class>
                <owl:intersectionOf rdf:parseType="Collection">
                    <rdf:Description rdf:about="http://www.ontologyrepository.com/CommonCoreOntologies/ComputerProgramExecution"/>
                    <owl:Restriction>
                        <owl:onProperty rdf:resource="https://www.commoncoreontologies.org/ont00001933"/>
                        <owl:someValuesFrom rdf:resource="http://www.ontologyrepository.com/CommonCoreOntologies/ComputerProgramExecution"/>
                    </owl:Restriction>
                </owl:intersectionOf>
            </owl:Class>
        </owl:equivalentClass>
        <rdfs:subClassOf rdf:resource="http://www.ontologyrepository.com/CommonCoreOntologies/ComputerProgramExecution"/>
        <skos:altLabel xml:lang="en">Parent Computer Process</skos:altLabel>
        <skos:definition xml:lang="en">A Computer Program Execution that starts some other Computer Program Execution.</skos:definition>
        <rdfs:label xml:lang="en">Parent Computer Program Execution</rdfs:label>
        <cco2:ont00001760 rdf:datatype="http://www.w3.org/2001/XMLSchema#anyURI">http://www.ontologyrepository.com/CommonCoreOntologies/Domain/CyberOntology</cco2:ont00001760>
    </owl:Class>
    


    <!-- http://www.ontologyrepository.com/CommonCoreOntologies/PassbandBandwidthMeasurement -->

    <owl:Class rdf:about="http://www.ontologyrepository.com/CommonCoreOntologies/PassbandBandwidthMeasurement">
        <rdfs:subClassOf rdf:resource="http://www.ontologyrepository.com/CommonCoreOntologies/SignalBandwidthMeasurement"/>
        <skos:definition xml:lang="en">A Signal Bandwidth Measurement that is a measurement of the range of continuous Frequencies between some upper and lower cutoff Frequencies.</skos:definition>
        <rdfs:label xml:lang="en">Passband Bandwidth Measurement</rdfs:label>
        <cco2:ont00001760 rdf:datatype="http://www.w3.org/2001/XMLSchema#anyURI">http://www.ontologyrepository.com/CommonCoreOntologies/Domain/CyberOntology</cco2:ont00001760>
    </owl:Class>
    


    <!-- http://www.ontologyrepository.com/CommonCoreOntologies/Pathname -->

    <owl:Class rdf:about="http://www.ontologyrepository.com/CommonCoreOntologies/Pathname">
        <rdfs:subClassOf rdf:resource="https://www.commoncoreontologies.org/ont00000077"/>
        <skos:definition xml:lang="en">A Code Identifier that designates a Digital File or File System Directory by specifying where that item is located within a hierarchy of File System Directories.</skos:definition>
        <skos:example>C:/john.doe/Documents/myDocument.doc</skos:example>
        <rdfs:label xml:lang="en">Pathname</rdfs:label>
        <cco2:ont00001760 rdf:datatype="http://www.w3.org/2001/XMLSchema#anyURI">http://www.ontologyrepository.com/CommonCoreOntologies/Domain/CyberOntology</cco2:ont00001760>
    </owl:Class>
    


    <!-- http://www.ontologyrepository.com/CommonCoreOntologies/PeerToPeerNetwork -->

    <owl:Class rdf:about="http://www.ontologyrepository.com/CommonCoreOntologies/PeerToPeerNetwork">
        <rdfs:subClassOf rdf:resource="http://www.ontologyrepository.com/CommonCoreOntologies/OverlayNetwork"/>
        <skos:altLabel xml:lang="en">P2P Network</skos:altLabel>
        <skos:definition xml:lang="en">An Overlay Network that partitions tasks or workloads between equally privileged peers on the network.</skos:definition>
        <rdfs:label xml:lang="en">Peer-to-Peer Network</rdfs:label>
        <cco2:ont00001754>https://en.wikipedia.org/wiki/Peer-to-peer</cco2:ont00001754>
        <cco2:ont00001760 rdf:datatype="http://www.w3.org/2001/XMLSchema#anyURI">http://www.ontologyrepository.com/CommonCoreOntologies/Domain/CyberOntology</cco2:ont00001760>
    </owl:Class>
    


    <!-- http://www.ontologyrepository.com/CommonCoreOntologies/PersonalAreaNetwork -->

    <owl:Class rdf:about="http://www.ontologyrepository.com/CommonCoreOntologies/PersonalAreaNetwork">
        <rdfs:subClassOf rdf:resource="https://www.commoncoreontologies.org/ont00000700"/>
        <skos:altLabel xml:lang="en">PAN</skos:altLabel>
        <skos:definition xml:lang="en">A Computer Network that is designed to connect several personal devices such as Computers, Telephones, and Tablets.</skos:definition>
        <rdfs:label xml:lang="en">Personal Area Network</rdfs:label>
        <cco2:ont00001754>https://en.wikipedia.org/wiki/Personal_area_network</cco2:ont00001754>
        <cco2:ont00001760 rdf:datatype="http://www.w3.org/2001/XMLSchema#anyURI">http://www.ontologyrepository.com/CommonCoreOntologies/Domain/CyberOntology</cco2:ont00001760>
    </owl:Class>
    


    <!-- http://www.ontologyrepository.com/CommonCoreOntologies/Phishing -->

    <owl:Class rdf:about="http://www.ontologyrepository.com/CommonCoreOntologies/Phishing">
        <rdfs:subClassOf rdf:resource="http://www.ontologyrepository.com/CommonCoreOntologies/CyberAttack"/>
        <skos:definition xml:lang="en">A Cyber Attack wherein an Agent sends an electronic message purporting to be from a reputable sender in order to induce its recipients to reveal sensitive information.</skos:definition>
        <rdfs:label xml:lang="en">Phishing</rdfs:label>
        <cco2:ont00001754>https://en.wikipedia.org/wiki/Phishing</cco2:ont00001754>
        <cco2:ont00001760 rdf:datatype="http://www.w3.org/2001/XMLSchema#anyURI">http://www.ontologyrepository.com/CommonCoreOntologies/Domain/CyberOntology</cco2:ont00001760>
    </owl:Class>
    


    <!-- http://www.ontologyrepository.com/CommonCoreOntologies/PointingDevice -->

    <owl:Class rdf:about="http://www.ontologyrepository.com/CommonCoreOntologies/PointingDevice">
        <rdfs:subClassOf rdf:resource="http://www.ontologyrepository.com/CommonCoreOntologies/InputDevice"/>
        <skos:definition xml:lang="en">An Input Device that allows a user to input spatial data to Information Processing Artficat..</skos:definition>
        <rdfs:label xml:lang="en">Pointing Device</rdfs:label>
        <cco2:ont00001754 rdf:datatype="http://www.w3.org/2001/XMLSchema#anyURI">https://en.wikipedia.org/wiki/Pointing_device</cco2:ont00001754>
        <cco2:ont00001760 rdf:datatype="http://www.w3.org/2001/XMLSchema#anyURI">http://www.ontologyrepository.com/CommonCoreOntologies/Domain/CyberOntology</cco2:ont00001760>
    </owl:Class>
    


    <!-- http://www.ontologyrepository.com/CommonCoreOntologies/PresentationSoftwareApplication -->

    <owl:Class rdf:about="http://www.ontologyrepository.com/CommonCoreOntologies/PresentationSoftwareApplication">
        <rdfs:subClassOf rdf:resource="http://www.ontologyrepository.com/CommonCoreOntologies/InformationWorkerSoftware"/>
        <skos:definition xml:lang="en">An Information Worker Software Application that is designed to enable a user to create, edit, and present a series of Images or Videos.</skos:definition>
        <rdfs:label xml:lang="en">Presentation Software Application</rdfs:label>
        <cco2:ont00001760 rdf:datatype="http://www.w3.org/2001/XMLSchema#anyURI">http://www.ontologyrepository.com/CommonCoreOntologies/Domain/CyberOntology</cco2:ont00001760>
    </owl:Class>
    


    <!-- http://www.ontologyrepository.com/CommonCoreOntologies/PrintServer -->

    <owl:Class rdf:about="http://www.ontologyrepository.com/CommonCoreOntologies/PrintServer">
        <rdfs:subClassOf rdf:resource="http://www.ontologyrepository.com/CommonCoreOntologies/NetworkServer"/>
        <skos:altLabel xml:lang="en">Printer Server</skos:altLabel>
        <skos:definition xml:lang="en">A Network Server that enables clients to access a Computer Printer Function.</skos:definition>
        <rdfs:label xml:lang="en">Print Server</rdfs:label>
        <cco2:ont00001754 rdf:datatype="http://www.w3.org/2001/XMLSchema#anyURI">https://en.wikipedia.org/wiki/Print_server</cco2:ont00001754>
        <cco2:ont00001760 rdf:datatype="http://www.w3.org/2001/XMLSchema#anyURI">http://www.ontologyrepository.com/CommonCoreOntologies/Domain/CyberOntology</cco2:ont00001760>
    </owl:Class>
    


    <!-- http://www.ontologyrepository.com/CommonCoreOntologies/PrivateComputerNetwork -->

    <owl:Class rdf:about="http://www.ontologyrepository.com/CommonCoreOntologies/PrivateComputerNetwork">
        <owl:equivalentClass>
            <owl:Class>
                <owl:intersectionOf rdf:parseType="Collection">
                    <rdf:Description rdf:about="https://www.commoncoreontologies.org/ont00000700"/>
                    <owl:Restriction>
                        <owl:onProperty rdf:resource="http://purl.obolibrary.org/obo/BFO_0000056"/>
                        <owl:someValuesFrom rdf:resource="http://www.ontologyrepository.com/CommonCoreOntologies/Authentication"/>
                    </owl:Restriction>
                </owl:intersectionOf>
            </owl:Class>
        </owl:equivalentClass>
        <rdfs:subClassOf rdf:resource="https://www.commoncoreontologies.org/ont00000700"/>
        <skos:definition xml:lang="en">A Computer Network which requires authentication in order to access it.</skos:definition>
        <rdfs:label xml:lang="en">Private Computer Network</rdfs:label>
        <cco2:ont00001760 rdf:datatype="http://www.w3.org/2001/XMLSchema#anyURI">http://www.ontologyrepository.com/CommonCoreOntologies/Domain/CyberOntology</cco2:ont00001760>
    </owl:Class>
    


    <!-- http://www.ontologyrepository.com/CommonCoreOntologies/ProcessVirtualMachine -->

    <owl:Class rdf:about="http://www.ontologyrepository.com/CommonCoreOntologies/ProcessVirtualMachine">
        <rdfs:subClassOf rdf:resource="http://www.ontologyrepository.com/CommonCoreOntologies/VirtualMachine"/>
        <skos:definition xml:lang="en">A Virtual Machine that executes Computer Programs in a platform-independent environment.</skos:definition>
        <rdfs:label xml:lang="en">Process Virtual Machine</rdfs:label>
        <cco2:ont00001754>https://en.wikipedia.org/wiki/Virtual_machine</cco2:ont00001754>
        <cco2:ont00001760 rdf:datatype="http://www.w3.org/2001/XMLSchema#anyURI">http://www.ontologyrepository.com/CommonCoreOntologies/Domain/CyberOntology</cco2:ont00001760>
    </owl:Class>
    


    <!-- http://www.ontologyrepository.com/CommonCoreOntologies/ProcessingUnit -->

    <owl:Class rdf:about="http://www.ontologyrepository.com/CommonCoreOntologies/ProcessingUnit">
        <rdfs:subClassOf rdf:resource="https://www.commoncoreontologies.org/ont00000117"/>
        <skos:definition xml:lang="en">An Information Processing Artifact that is designed to execute the instructions of some Computer Program.</skos:definition>
        <rdfs:label xml:lang="en">Processing Unit</rdfs:label>
        <cco2:ont00001760 rdf:datatype="http://www.w3.org/2001/XMLSchema#anyURI">http://www.ontologyrepository.com/CommonCoreOntologies/Domain/CyberOntology</cco2:ont00001760>
    </owl:Class>
    


    <!-- http://www.ontologyrepository.com/CommonCoreOntologies/ProgrammableLogicController -->

    <owl:Class rdf:about="http://www.ontologyrepository.com/CommonCoreOntologies/ProgrammableLogicController">
        <rdfs:subClassOf rdf:resource="https://www.commoncoreontologies.org/ont00000420"/>
        <skos:altLabel xml:lang="en">PLC</skos:altLabel>
        <skos:definition xml:lang="en">A Computer that is designed to be rugged and adaptable for the control of manufacturing processes.</skos:definition>
        <rdfs:label xml:lang="en">Programmable Logic Controller</rdfs:label>
        <cco2:ont00001754>https://en.wikipedia.org/wiki/Programmable_logic_controller</cco2:ont00001754>
        <cco2:ont00001760 rdf:datatype="http://www.w3.org/2001/XMLSchema#anyURI">http://www.ontologyrepository.com/CommonCoreOntologies/Domain/CyberOntology</cco2:ont00001760>
    </owl:Class>
    


    <!-- http://www.ontologyrepository.com/CommonCoreOntologies/ProgrammingLanguage -->

    <owl:Class rdf:about="http://www.ontologyrepository.com/CommonCoreOntologies/ProgrammingLanguage">
        <rdfs:subClassOf rdf:resource="http://www.ontologyrepository.com/CommonCoreOntologies/ComputerLanguage"/>
        <skos:definition xml:lang="en">A Computer Language that prescribes a canonical form of communicating instructions to be executed by some Processing Unit or by a Computer Program.</skos:definition>
        <rdfs:label xml:lang="en">Programming Language</rdfs:label>
        <cco2:ont00001760 rdf:datatype="http://www.w3.org/2001/XMLSchema#anyURI">http://www.ontologyrepository.com/CommonCoreOntologies/Domain/CyberOntology</cco2:ont00001760>
    </owl:Class>
    


    <!-- http://www.ontologyrepository.com/CommonCoreOntologies/ProgrammingMethod -->

    <owl:Class rdf:about="http://www.ontologyrepository.com/CommonCoreOntologies/ProgrammingMethod">
        <rdfs:subClassOf rdf:resource="http://www.ontologyrepository.com/CommonCoreOntologies/Subroutine"/>
        <skos:altLabel xml:lang="en">Method</skos:altLabel>
        <skos:definition xml:lang="en">A Subroutine that is part of a Computer Object.</skos:definition>
        <rdfs:label xml:lang="en">Programming Method</rdfs:label>
        <cco2:ont00001754>https://en.wikipedia.org/wiki/Method_(computer_programming)</cco2:ont00001754>
        <cco2:ont00001760 rdf:datatype="http://www.w3.org/2001/XMLSchema#anyURI">http://www.ontologyrepository.com/CommonCoreOntologies/Domain/CyberOntology</cco2:ont00001760>
    </owl:Class>
    


    <!-- http://www.ontologyrepository.com/CommonCoreOntologies/ProxyFirewall -->

    <owl:Class rdf:about="http://www.ontologyrepository.com/CommonCoreOntologies/ProxyFirewall">
        <rdfs:subClassOf rdf:resource="http://www.ontologyrepository.com/CommonCoreOntologies/Firewall"/>
        <skos:altLabel xml:lang="en">Application Firewall</skos:altLabel>
        <skos:altLabel xml:lang="en">Gateway Firewall</skos:altLabel>
        <skos:definition xml:lang="en">A Firewall that protects network resources by filtering messages at the application layer using stateful inspection technology and deep packet inspection.</skos:definition>
        <rdfs:label xml:lang="en">Proxy Firewall</rdfs:label>
        <cco2:ont00001754>http://searchsecurity.techtarget.com/definition/proxy-firewall</cco2:ont00001754>
        <cco2:ont00001760 rdf:datatype="http://www.w3.org/2001/XMLSchema#anyURI">http://www.ontologyrepository.com/CommonCoreOntologies/Domain/CyberOntology</cco2:ont00001760>
    </owl:Class>
    


    <!-- http://www.ontologyrepository.com/CommonCoreOntologies/QueryLanguage -->

    <owl:Class rdf:about="http://www.ontologyrepository.com/CommonCoreOntologies/QueryLanguage">
        <rdfs:subClassOf rdf:resource="http://www.ontologyrepository.com/CommonCoreOntologies/ComputerLanguage"/>
        <skos:definition xml:lang="en">A Computer language used to make queries in databases and information systems.</skos:definition>
        <rdfs:label xml:lang="en">Query Language</rdfs:label>
        <cco2:ont00001754 rdf:datatype="http://www.w3.org/2001/XMLSchema#anyURI">https://en.wikipedia.org/wiki/Query_language</cco2:ont00001754>
        <cco2:ont00001760 rdf:datatype="http://www.w3.org/2001/XMLSchema#anyURI">http://www.ontologyrepository.com/CommonCoreOntologies/Domain/CyberOntology</cco2:ont00001760>
    </owl:Class>
    


    <!-- http://www.ontologyrepository.com/CommonCoreOntologies/RandomAccessMemory -->

    <owl:Class rdf:about="http://www.ontologyrepository.com/CommonCoreOntologies/RandomAccessMemory">
        <rdfs:subClassOf rdf:resource="http://www.ontologyrepository.com/CommonCoreOntologies/ComputerMemory"/>
        <skos:definition xml:lang="en">Computer Memory that stores frequently used Computer Programs to increase the general speed of a Computer.</skos:definition>
        <rdfs:label xml:lang="en">Random-Access Memory</rdfs:label>
        <cco2:ont00001753>RAM</cco2:ont00001753>
        <cco2:ont00001754>https://en.wikipedia.org/wiki/Random-access_memory</cco2:ont00001754>
        <cco2:ont00001760 rdf:datatype="http://www.w3.org/2001/XMLSchema#anyURI">http://www.ontologyrepository.com/CommonCoreOntologies/Domain/CyberOntology</cco2:ont00001760>
    </owl:Class>
    


    <!-- http://www.ontologyrepository.com/CommonCoreOntologies/Ransomware -->

    <owl:Class rdf:about="http://www.ontologyrepository.com/CommonCoreOntologies/Ransomware">
        <rdfs:subClassOf rdf:resource="http://www.ontologyrepository.com/CommonCoreOntologies/Malware"/>
        <skos:definition xml:lang="en">Malware that is designed to lock a user out of a computer system, and threaten to publish the victim&apos;s data or perpetually block system access unless a ransom is paid.</skos:definition>
        <rdfs:label xml:lang="en">Ransomware</rdfs:label>
        <cco2:ont00001754>https://en.wikipedia.org/wiki/Ransomware</cco2:ont00001754>
        <cco2:ont00001760 rdf:datatype="http://www.w3.org/2001/XMLSchema#anyURI">http://www.ontologyrepository.com/CommonCoreOntologies/Domain/CyberOntology</cco2:ont00001760>
    </owl:Class>
    


    <!-- http://www.ontologyrepository.com/CommonCoreOntologies/ReadFilePermission -->

    <owl:Class rdf:about="http://www.ontologyrepository.com/CommonCoreOntologies/ReadFilePermission">
        <rdfs:subClassOf rdf:resource="http://www.ontologyrepository.com/CommonCoreOntologies/FilePermission"/>
        <skos:definition xml:lang="en">A File Permission that prescribes the reading of a file by a user account.</skos:definition>
        <rdfs:label xml:lang="en">Read File Permission</rdfs:label>
        <cco2:ont00001754 rdf:datatype="http://www.w3.org/2001/XMLSchema#anyURI">https://en.wikipedia.org/wiki/File_system_permissions</cco2:ont00001754>
        <cco2:ont00001760 rdf:datatype="http://www.w3.org/2001/XMLSchema#anyURI">http://www.ontologyrepository.com/CommonCoreOntologies/Domain/CyberOntology</cco2:ont00001760>
    </owl:Class>
    


    <!-- http://www.ontologyrepository.com/CommonCoreOntologies/RelationalDatabaseSoftwareApplicationModel -->

    <owl:Class rdf:about="http://www.ontologyrepository.com/CommonCoreOntologies/RelationalDatabaseSoftwareApplicationModel">
        <rdfs:subClassOf rdf:resource="http://www.ontologyrepository.com/CommonCoreOntologies/DatabaseSoftwareApplicationModel"/>
        <skos:definition xml:lang="en">A Database Software Application Model that prescribes a Database Software Application where the data is stored as a set of linked tables, or relations, that contain attributes, or columns, along with identifying keys that can be use to write queries to return joined and trimmed subsets of the database contents.</skos:definition>
        <rdfs:label xml:lang="en">Relational Database Software Application Model</rdfs:label>
        <cco2:ont00001754 rdf:datatype="http://www.w3.org/2001/XMLSchema#anyURI">https://searchdatamanagement.techtarget.com/definition/relational-database</cco2:ont00001754>
        <cco2:ont00001760 rdf:datatype="http://www.w3.org/2001/XMLSchema#anyURI">http://www.ontologyrepository.com/CommonCoreOntologies/Domain/CyberOntology</cco2:ont00001760>
    </owl:Class>
    


    <!-- http://www.ontologyrepository.com/CommonCoreOntologies/RemoteAccess -->

    <owl:Class rdf:about="http://www.ontologyrepository.com/CommonCoreOntologies/RemoteAccess">
        <rdfs:subClassOf rdf:resource="http://www.ontologyrepository.com/CommonCoreOntologies/ComputerProgramExecution"/>
        <skos:definition xml:lang="en">A Computer Program Execution in which an Information Processing Artifact at one location connects with some other Information Processing Artifact at some other, remote location.</skos:definition>
        <rdfs:label xml:lang="en">Remote Access</rdfs:label>
        <cco2:ont00001754>https://en.wikipedia.org/wiki/Remote_access</cco2:ont00001754>
        <cco2:ont00001760 rdf:datatype="http://www.w3.org/2001/XMLSchema#anyURI">http://www.ontologyrepository.com/CommonCoreOntologies/Domain/CyberOntology</cco2:ont00001760>
    </owl:Class>
    


    <!-- http://www.ontologyrepository.com/CommonCoreOntologies/RemoteAccessServiceFunction -->

    <owl:Class rdf:about="http://www.ontologyrepository.com/CommonCoreOntologies/RemoteAccessServiceFunction">
        <rdfs:subClassOf rdf:resource="http://www.ontologyrepository.com/CommonCoreOntologies/NetworkServiceFunction"/>
        <skos:altLabel xml:lang="en">Remote Access Service</skos:altLabel>
        <skos:definition xml:lang="en">A Network Service Function that when realized is in a process of a Computer remotely accessing and controling another Computer on a Computer Network.</skos:definition>
        <rdfs:label xml:lang="en">Remote Access Service Function</rdfs:label>
        <cco2:ont00001760 rdf:datatype="http://www.w3.org/2001/XMLSchema#anyURI">http://www.ontologyrepository.com/CommonCoreOntologies/Domain/CyberOntology</cco2:ont00001760>
    </owl:Class>
    


    <!-- http://www.ontologyrepository.com/CommonCoreOntologies/RemoteAccessTool -->

    <owl:Class rdf:about="http://www.ontologyrepository.com/CommonCoreOntologies/RemoteAccessTool">
        <rdfs:subClassOf rdf:resource="http://www.ontologyrepository.com/CommonCoreOntologies/ApplicationSoftware"/>
        <skos:altLabel xml:lang="en">RAT</skos:altLabel>
        <skos:altLabel xml:lang="en">Remote Administration Software</skos:altLabel>
        <skos:definition xml:lang="en">Application Software that allows a remote operator to control a system.</skos:definition>
        <rdfs:label xml:lang="en">Remote Access Tool</rdfs:label>
        <cco2:ont00001760 rdf:datatype="http://www.w3.org/2001/XMLSchema#anyURI">http://www.ontologyrepository.com/CommonCoreOntologies/Domain/CyberOntology</cco2:ont00001760>
    </owl:Class>
    


    <!-- http://www.ontologyrepository.com/CommonCoreOntologies/RemoteTerminalUnit -->

    <owl:Class rdf:about="http://www.ontologyrepository.com/CommonCoreOntologies/RemoteTerminalUnit">
        <rdfs:subClassOf rdf:resource="https://www.commoncoreontologies.org/ont00000420"/>
        <skos:altLabel xml:lang="en">RTU</skos:altLabel>
        <skos:definition xml:lang="en">A Computer that is designed to interface objects in the physical world to a Distributed Control System or a SCADA System by transmitting telemetry data to a master system, and by using messages from the master supervisory system to control connected objects.</skos:definition>
        <rdfs:label xml:lang="en">Remote Terminal Unit</rdfs:label>
        <cco2:ont00001754>https://en.wikipedia.org/wiki/Remote_terminal_unit</cco2:ont00001754>
        <cco2:ont00001760 rdf:datatype="http://www.w3.org/2001/XMLSchema#anyURI">http://www.ontologyrepository.com/CommonCoreOntologies/Domain/CyberOntology</cco2:ont00001760>
    </owl:Class>
    


    <!-- http://www.ontologyrepository.com/CommonCoreOntologies/RootDirectory -->

    <owl:Class rdf:about="http://www.ontologyrepository.com/CommonCoreOntologies/RootDirectory">
        <rdfs:subClassOf rdf:resource="http://www.ontologyrepository.com/CommonCoreOntologies/FileSystemDirectory"/>
        <skos:definition xml:lang="en">A File System Directory that is the first or top-most directory in a hierarchy of File System Directories.</skos:definition>
        <rdfs:label xml:lang="en">Root Directory</rdfs:label>
        <cco2:ont00001754>https://en.wikipedia.org/wiki/Root_directory</cco2:ont00001754>
        <cco2:ont00001760 rdf:datatype="http://www.w3.org/2001/XMLSchema#anyURI">http://www.ontologyrepository.com/CommonCoreOntologies/Domain/CyberOntology</cco2:ont00001760>
    </owl:Class>
    


    <!-- http://www.ontologyrepository.com/CommonCoreOntologies/Rootkit -->

    <owl:Class rdf:about="http://www.ontologyrepository.com/CommonCoreOntologies/Rootkit">
        <rdfs:subClassOf rdf:resource="http://www.ontologyrepository.com/CommonCoreOntologies/Malware"/>
        <skos:definition xml:lang="en">Malware that is designed to enable an unauthorized user to gain administrator access to a Computer.</skos:definition>
        <rdfs:label xml:lang="en">Rootkit</rdfs:label>
        <cco2:ont00001754>https://en.wikipedia.org/wiki/Rootkit</cco2:ont00001754>
        <cco2:ont00001760 rdf:datatype="http://www.w3.org/2001/XMLSchema#anyURI">http://www.ontologyrepository.com/CommonCoreOntologies/Domain/CyberOntology</cco2:ont00001760>
    </owl:Class>
    


    <!-- http://www.ontologyrepository.com/CommonCoreOntologies/STIXComponentCategory -->

    <owl:Class rdf:about="http://www.ontologyrepository.com/CommonCoreOntologies/STIXComponentCategory">
        <rdfs:subClassOf rdf:resource="https://www.commoncoreontologies.org/ont00000293"/>
        <rdfs:label xml:lang="en">STIX Component Category</rdfs:label>
        <cco2:ont00001760 rdf:datatype="http://www.w3.org/2001/XMLSchema#anyURI">http://www.ontologyrepository.com/CommonCoreOntologies/Domain/CyberOntology</cco2:ont00001760>
    </owl:Class>
    


    <!-- http://www.ontologyrepository.com/CommonCoreOntologies/SYNFlood -->

    <owl:Class rdf:about="http://www.ontologyrepository.com/CommonCoreOntologies/SYNFlood">
        <rdfs:subClassOf rdf:resource="http://www.ontologyrepository.com/CommonCoreOntologies/DenialOfService"/>
        <skos:definition xml:lang="en">A Denial of Service in which an Agent sends a succession of SYN requests to a target&apos;s system in an attempt to consume enough server resources to make the system unresponsive to legitimate traffic.</skos:definition>
        <rdfs:label xml:lang="en">SYN Flood</rdfs:label>
        <cco2:ont00001754>https://en.wikipedia.org/wiki/SYN_flood</cco2:ont00001754>
        <cco2:ont00001760 rdf:datatype="http://www.w3.org/2001/XMLSchema#anyURI">http://www.ontologyrepository.com/CommonCoreOntologies/Domain/CyberOntology</cco2:ont00001760>
    </owl:Class>
    


    <!-- http://www.ontologyrepository.com/CommonCoreOntologies/ScientificSimulator -->

    <owl:Class rdf:about="http://www.ontologyrepository.com/CommonCoreOntologies/ScientificSimulator">
        <rdfs:subClassOf rdf:resource="http://www.ontologyrepository.com/CommonCoreOntologies/SimulationSoftware"/>
        <skos:definition xml:lang="en">Simulation Software that is designed to enable a user to model some scientific phenomenon.</skos:definition>
        <rdfs:label xml:lang="en">Scientific Simulator</rdfs:label>
        <cco2:ont00001760 rdf:datatype="http://www.w3.org/2001/XMLSchema#anyURI">http://www.ontologyrepository.com/CommonCoreOntologies/Domain/CyberOntology</cco2:ont00001760>
    </owl:Class>
    


    <!-- http://www.ontologyrepository.com/CommonCoreOntologies/Screensaver -->

    <owl:Class rdf:about="http://www.ontologyrepository.com/CommonCoreOntologies/Screensaver">
        <rdfs:subClassOf rdf:resource="http://www.ontologyrepository.com/CommonCoreOntologies/UtilityProgram"/>
        <skos:definition xml:lang="en">A Utility Program that is designed to blank the Screen or to fill it with Images when the Computer is not in use.</skos:definition>
        <rdfs:label xml:lang="en">Screensaver</rdfs:label>
        <cco2:ont00001754>https://en.wikipedia.org/wiki/Screensaver</cco2:ont00001754>
        <cco2:ont00001760 rdf:datatype="http://www.w3.org/2001/XMLSchema#anyURI">http://www.ontologyrepository.com/CommonCoreOntologies/Domain/CyberOntology</cco2:ont00001760>
    </owl:Class>
    


    <!-- http://www.ontologyrepository.com/CommonCoreOntologies/ServiceAccount -->

    <owl:Class rdf:about="http://www.ontologyrepository.com/CommonCoreOntologies/ServiceAccount">
        <rdfs:subClassOf rdf:resource="http://www.ontologyrepository.com/CommonCoreOntologies/UserAccount"/>
        <skos:definition xml:lang="en">A User Account that is used  to run applications and other processes.</skos:definition>
        <rdfs:label xml:lang="en">Service Account</rdfs:label>
        <cco2:ont00001754 rdf:datatype="http://www.w3.org/2001/XMLSchema#anyURI">https://www.ssh.com/iam/user/service-account</cco2:ont00001754>
        <cco2:ont00001760 rdf:datatype="http://www.w3.org/2001/XMLSchema#anyURI">http://www.ontologyrepository.com/CommonCoreOntologies/Domain/CyberOntology</cco2:ont00001760>
    </owl:Class>
    


    <!-- http://www.ontologyrepository.com/CommonCoreOntologies/SignalBandwidthMeasurement -->

    <owl:Class rdf:about="http://www.ontologyrepository.com/CommonCoreOntologies/SignalBandwidthMeasurement">
        <rdfs:subClassOf rdf:resource="https://www.commoncoreontologies.org/ont00001022"/>
        <skos:definition xml:lang="en">A Ratio Measurement Information Content Entity that is a measurement of the range of some continuous band of Frequencies in the transmission of a signal.</skos:definition>
        <rdfs:label xml:lang="en">Signal Bandwidth Measurement</rdfs:label>
        <cco2:ont00001760 rdf:datatype="http://www.w3.org/2001/XMLSchema#anyURI">http://www.ontologyrepository.com/CommonCoreOntologies/Domain/CyberOntology</cco2:ont00001760>
    </owl:Class>
    


    <!-- http://www.ontologyrepository.com/CommonCoreOntologies/SimulationSoftware -->

    <owl:Class rdf:about="http://www.ontologyrepository.com/CommonCoreOntologies/SimulationSoftware">
        <rdfs:subClassOf rdf:resource="http://www.ontologyrepository.com/CommonCoreOntologies/ApplicationSoftware"/>
        <skos:definition xml:lang="en">Application Software that is designed to enable a user to model a process with a set of mathematical formulas.</skos:definition>
        <rdfs:label xml:lang="en">Simulation Software</rdfs:label>
        <cco2:ont00001754>https://en.wikipedia.org/wiki/Simulation_software</cco2:ont00001754>
        <cco2:ont00001760 rdf:datatype="http://www.w3.org/2001/XMLSchema#anyURI">http://www.ontologyrepository.com/CommonCoreOntologies/Domain/CyberOntology</cco2:ont00001760>
    </owl:Class>
    


    <!-- http://www.ontologyrepository.com/CommonCoreOntologies/SiteControlAndDataAcquisitionSystem -->

    <owl:Class rdf:about="http://www.ontologyrepository.com/CommonCoreOntologies/SiteControlAndDataAcquisitionSystem">
        <rdfs:subClassOf rdf:resource="https://www.commoncoreontologies.org/ont00000781"/>
        <skos:altLabel xml:lang="en">SCADA System</skos:altLabel>
        <skos:definition xml:lang="en">A Control System that is designed to allow high-level process supervisory management of resources by means of computers, networked data communications, and graphical user interfaces.</skos:definition>
        <rdfs:label xml:lang="en">Site Control And Data Acquisition System</rdfs:label>
        <cco2:ont00001754>https://en.wikipedia.org/wiki/SCADA</cco2:ont00001754>
        <cco2:ont00001760 rdf:datatype="http://www.w3.org/2001/XMLSchema#anyURI">http://www.ontologyrepository.com/CommonCoreOntologies/Domain/CyberOntology</cco2:ont00001760>
    </owl:Class>
    


    <!-- http://www.ontologyrepository.com/CommonCoreOntologies/SocialNetworkingSite -->

    <owl:Class rdf:about="http://www.ontologyrepository.com/CommonCoreOntologies/SocialNetworkingSite">
        <rdfs:subClassOf rdf:resource="http://www.ontologyrepository.com/CommonCoreOntologies/Website"/>
        <skos:definition xml:lang="en">A Website that is used by people to build social networks or social relations with other people who share similar personal or career interests, activities, backgrounds, or real-life connections.</skos:definition>
        <rdfs:label xml:lang="en">Social Networking Site</rdfs:label>
        <cco2:ont00001754>https://en.wikipedia.org/wiki/Social_networking_service</cco2:ont00001754>
        <cco2:ont00001760 rdf:datatype="http://www.w3.org/2001/XMLSchema#anyURI">http://www.ontologyrepository.com/CommonCoreOntologies/Domain/CyberOntology</cco2:ont00001760>
    </owl:Class>
    


    <!-- http://www.ontologyrepository.com/CommonCoreOntologies/SocialSimulator -->

    <owl:Class rdf:about="http://www.ontologyrepository.com/CommonCoreOntologies/SocialSimulator">
        <rdfs:subClassOf rdf:resource="http://www.ontologyrepository.com/CommonCoreOntologies/SimulationSoftware"/>
        <skos:definition xml:lang="en">Simulation Software that is designed to enable a user to model some social phenomenon.</skos:definition>
        <rdfs:label xml:lang="en">Social Simulator</rdfs:label>
        <cco2:ont00001760 rdf:datatype="http://www.w3.org/2001/XMLSchema#anyURI">http://www.ontologyrepository.com/CommonCoreOntologies/Domain/CyberOntology</cco2:ont00001760>
    </owl:Class>
    


    <!-- http://www.ontologyrepository.com/CommonCoreOntologies/SoftwareArchitecture -->

    <owl:Class rdf:about="http://www.ontologyrepository.com/CommonCoreOntologies/SoftwareArchitecture">
        <rdfs:subClassOf rdf:resource="https://www.commoncoreontologies.org/ont00000974"/>
        <skos:definition xml:lang="en">A Plan Specification that prescribes the fundamental structures of a software system and how to create such systems.</skos:definition>
        <rdfs:label xml:lang="en">Software Architecture</rdfs:label>
        <cco2:ont00001754 rdf:datatype="http://www.w3.org/2001/XMLSchema#anyURI">https://en.wikipedia.org/wiki/Software_architecture</cco2:ont00001754>
        <cco2:ont00001760 rdf:datatype="http://www.w3.org/2001/XMLSchema#anyURI">http://www.ontologyrepository.com/CommonCoreOntologies/Domain/CyberOntology</cco2:ont00001760>
    </owl:Class>
    


    <!-- http://www.ontologyrepository.com/CommonCoreOntologies/SoftwareEngineeringSoftware -->

    <owl:Class rdf:about="http://www.ontologyrepository.com/CommonCoreOntologies/SoftwareEngineeringSoftware">
        <rdfs:subClassOf rdf:resource="http://www.ontologyrepository.com/CommonCoreOntologies/ApplicationSoftware"/>
        <skos:definition xml:lang="en">Application Software that is designed to enable a user to create and manage a software product.</skos:definition>
        <rdfs:label xml:lang="en">Software Engineering Software</rdfs:label>
        <cco2:ont00001760 rdf:datatype="http://www.w3.org/2001/XMLSchema#anyURI">http://www.ontologyrepository.com/CommonCoreOntologies/Domain/CyberOntology</cco2:ont00001760>
    </owl:Class>
    


    <!-- http://www.ontologyrepository.com/CommonCoreOntologies/SoftwareFramework -->

    <owl:Class rdf:about="http://www.ontologyrepository.com/CommonCoreOntologies/SoftwareFramework">
        <rdfs:subClassOf rdf:resource="http://www.ontologyrepository.com/CommonCoreOntologies/SoftwareEngineeringSoftware"/>
        <skos:definition xml:lang="en">A Software Engineering Software that provides generic functionality and can be selectively changed by additional user-written code to provide application-specific functionality.</skos:definition>
        <rdfs:label xml:lang="en">Software Framework</rdfs:label>
        <cco2:ont00001754 rdf:datatype="http://www.w3.org/2001/XMLSchema#anyURI">https://en.wikipedia.org/wiki/Software_framework</cco2:ont00001754>
        <cco2:ont00001760 rdf:datatype="http://www.w3.org/2001/XMLSchema#anyURI">http://www.ontologyrepository.com/CommonCoreOntologies/Domain/CyberOntology</cco2:ont00001760>
    </owl:Class>
    


    <!-- http://www.ontologyrepository.com/CommonCoreOntologies/SoftwareLibrary -->

    <owl:Class rdf:about="http://www.ontologyrepository.com/CommonCoreOntologies/SoftwareLibrary">
        <rdfs:subClassOf rdf:resource="https://www.commoncoreontologies.org/ont00000798"/>
        <skos:definition xml:lang="en">An Information Bearing Artifact that is an aggregate of Digital Files and that is designed to support the development or execution of Computer Programs.</skos:definition>
        <skos:example>A collection of digital files consisting of: configuration data and documentation for a program, and pre-written methods and classes which can be called by other programs.</skos:example>
        <rdfs:label xml:lang="en">Software Library</rdfs:label>
        <cco2:ont00001760 rdf:datatype="http://www.w3.org/2001/XMLSchema#anyURI">http://www.ontologyrepository.com/CommonCoreOntologies/Domain/CyberOntology</cco2:ont00001760>
    </owl:Class>
    


    <!-- http://www.ontologyrepository.com/CommonCoreOntologies/SoftwareStack -->

    <owl:Class rdf:about="http://www.ontologyrepository.com/CommonCoreOntologies/SoftwareStack">
        <rdfs:subClassOf rdf:resource="https://www.commoncoreontologies.org/ont00000117"/>
        <skos:definition xml:lang="en">An Information Processing Artifact composed of software, software subsystems, or components needed to create a complete platform such that no additional software is needed to support applications.</skos:definition>
        <rdfs:label xml:lang="en">Software Stack</rdfs:label>
        <cco2:ont00001754>https://en.wikipedia.org/wiki/Solution_stack</cco2:ont00001754>
        <cco2:ont00001760 rdf:datatype="http://www.w3.org/2001/XMLSchema#anyURI">http://www.ontologyrepository.com/CommonCoreOntologies/Domain/CyberOntology</cco2:ont00001760>
    </owl:Class>
    


    <!-- http://www.ontologyrepository.com/CommonCoreOntologies/SpreadsheetSoftwareApplication -->

    <owl:Class rdf:about="http://www.ontologyrepository.com/CommonCoreOntologies/SpreadsheetSoftwareApplication">
        <rdfs:subClassOf rdf:resource="http://www.ontologyrepository.com/CommonCoreOntologies/InformationWorkerSoftware"/>
        <skos:definition xml:lang="en">An Information Worker Software Application that is designed to enable a user to organize, analyze, and chart/graph data in Data Rows and Data Columns.</skos:definition>
        <rdfs:label xml:lang="en">Spreadsheet Software Application</rdfs:label>
        <cco2:ont00001760 rdf:datatype="http://www.w3.org/2001/XMLSchema#anyURI">http://www.ontologyrepository.com/CommonCoreOntologies/Domain/CyberOntology</cco2:ont00001760>
    </owl:Class>
    


    <!-- http://www.ontologyrepository.com/CommonCoreOntologies/Spyware -->

    <owl:Class rdf:about="http://www.ontologyrepository.com/CommonCoreOntologies/Spyware">
        <rdfs:subClassOf rdf:resource="http://www.ontologyrepository.com/CommonCoreOntologies/ComputerProgram"/>
        <skos:definition xml:lang="en">A Computer Program that is designed to gather information about a person or organization without their knowledge, that may send such information to another entity without the consumer&apos;s consent, or that asserts control over a device without the consumer&apos;s knowledge.</skos:definition>
        <rdfs:label xml:lang="en">Spyware</rdfs:label>
        <cco2:ont00001754>https://en.wikipedia.org/wiki/Spyware</cco2:ont00001754>
        <cco2:ont00001760 rdf:datatype="http://www.w3.org/2001/XMLSchema#anyURI">http://www.ontologyrepository.com/CommonCoreOntologies/Domain/CyberOntology</cco2:ont00001760>
    </owl:Class>
    


    <!-- http://www.ontologyrepository.com/CommonCoreOntologies/StandardUserAccount -->

    <owl:Class rdf:about="http://www.ontologyrepository.com/CommonCoreOntologies/StandardUserAccount">
        <rdfs:subClassOf rdf:resource="http://www.ontologyrepository.com/CommonCoreOntologies/UserAccount"/>
        <skos:definition xml:lang="en">A User Account that is not permitted to create, edit, view, or delete system files.</skos:definition>
        <rdfs:label xml:lang="en">Standard User Account</rdfs:label>
        <cco2:ont00001754 rdf:datatype="http://www.w3.org/2001/XMLSchema#anyURI">https://www.guidingtech.com/difference-between-standard-user-administrator/</cco2:ont00001754>
        <cco2:ont00001760 rdf:datatype="http://www.w3.org/2001/XMLSchema#anyURI">http://www.ontologyrepository.com/CommonCoreOntologies/Domain/CyberOntology</cco2:ont00001760>
    </owl:Class>
    


    <!-- http://www.ontologyrepository.com/CommonCoreOntologies/StasisOfDigitalStorage -->

    <owl:Class rdf:about="http://www.ontologyrepository.com/CommonCoreOntologies/StasisOfDigitalStorage">
        <rdfs:subClassOf rdf:resource="http://www.ontologyrepository.com/CommonCoreOntologies/StasisOfInformationConcretization"/>
        <skos:definition xml:lang="en">A Stasis of Information Bearing that has as participants some Digital Storage Device and some Information Quality Entity.</skos:definition>
        <rdfs:comment xml:lang="en">The purpose of this Stasis is to represent that some Digital Storage Device (e.g., a hard drive or RAM) stores (at a given time) a Computer Program. We cannot say that a Computer Program (an IBA) is part_of some hard drive or RAM, because although the hard drive or RAM might take on qualities in order to encode the Program, the Program itself is not identical to any of those qualities.</rdfs:comment>
        <rdfs:label xml:lang="en">Stasis of Digital Storage</rdfs:label>
        <cco2:ont00001760 rdf:datatype="http://www.w3.org/2001/XMLSchema#anyURI">http://www.ontologyrepository.com/CommonCoreOntologies/Domain/CyberOntology</cco2:ont00001760>
    </owl:Class>
    


    <!-- http://www.ontologyrepository.com/CommonCoreOntologies/StasisOfInformationConcretization -->

    <owl:Class rdf:about="http://www.ontologyrepository.com/CommonCoreOntologies/StasisOfInformationConcretization">
        <rdfs:subClassOf rdf:resource="https://www.commoncoreontologies.org/ont00000335"/>
        <skos:definition xml:lang="en">A Stasis of Generically Dependent Continuant that has as participants some Information Bearing Entity and some Information Content Entity.</skos:definition>
        <rdfs:label xml:lang="en">Stasis of Information Bearing</rdfs:label>
        <cco2:ont00001760 rdf:datatype="http://www.w3.org/2001/XMLSchema#anyURI">http://www.ontologyrepository.com/CommonCoreOntologies/Domain/CyberOntology</cco2:ont00001760>
    </owl:Class>
    


    <!-- http://www.ontologyrepository.com/CommonCoreOntologies/StatefulInspectionFirewall -->

    <owl:Class rdf:about="http://www.ontologyrepository.com/CommonCoreOntologies/StatefulInspectionFirewall">
        <rdfs:subClassOf rdf:resource="http://www.ontologyrepository.com/CommonCoreOntologies/Firewall"/>
        <skos:definition xml:lang="en">A Firewall that allows or blocks traffic based on state, port, and protocol.</skos:definition>
        <rdfs:label xml:lang="en">Stateful Inspection Firewall</rdfs:label>
        <cco2:ont00001754>http://www.cisco.com/c/en/us/products/security/firewalls/what-is-a-firewall.html</cco2:ont00001754>
        <cco2:ont00001760 rdf:datatype="http://www.w3.org/2001/XMLSchema#anyURI">http://www.ontologyrepository.com/CommonCoreOntologies/Domain/CyberOntology</cco2:ont00001760>
    </owl:Class>
    


    <!-- http://www.ontologyrepository.com/CommonCoreOntologies/StorageAreaNetwork -->

    <owl:Class rdf:about="http://www.ontologyrepository.com/CommonCoreOntologies/StorageAreaNetwork">
        <rdfs:subClassOf rdf:resource="https://www.commoncoreontologies.org/ont00000700"/>
        <skos:altLabel xml:lang="en">SAN</skos:altLabel>
        <skos:definition xml:lang="en">A Computer Network that is designed to provide access to consolidated, block level data storage.</skos:definition>
        <rdfs:label xml:lang="en">Storage Area Network</rdfs:label>
        <cco2:ont00001754>https://en.wikipedia.org/wiki/Storage_area_network</cco2:ont00001754>
        <cco2:ont00001760 rdf:datatype="http://www.w3.org/2001/XMLSchema#anyURI">http://www.ontologyrepository.com/CommonCoreOntologies/Domain/CyberOntology</cco2:ont00001760>
    </owl:Class>
    


    <!-- http://www.ontologyrepository.com/CommonCoreOntologies/Subroutine -->

    <owl:Class rdf:about="http://www.ontologyrepository.com/CommonCoreOntologies/Subroutine">
        <rdfs:subClassOf rdf:resource="https://www.commoncoreontologies.org/ont00000117"/>
        <skos:altLabel xml:lang="en">Callable Unit</skos:altLabel>
        <skos:altLabel xml:lang="en">Function</skos:altLabel>
        <skos:altLabel xml:lang="en">Method</skos:altLabel>
        <skos:altLabel xml:lang="en">Procedure</skos:altLabel>
        <skos:altLabel xml:lang="en">Routine</skos:altLabel>
        <skos:altLabel xml:lang="en">Subprogram</skos:altLabel>
        <skos:definition xml:lang="en">An Information Processing Artifact that bears some Algorithm which is designed to be executed within the context of some Computer Program.</skos:definition>
        <rdfs:label xml:lang="en">Subroutine</rdfs:label>
        <cco2:ont00001760 rdf:datatype="http://www.w3.org/2001/XMLSchema#anyURI">http://www.ontologyrepository.com/CommonCoreOntologies/Domain/CyberOntology</cco2:ont00001760>
    </owl:Class>
    


    <!-- http://www.ontologyrepository.com/CommonCoreOntologies/SuperuserAccount -->

    <owl:Class rdf:about="http://www.ontologyrepository.com/CommonCoreOntologies/SuperuserAccount">
        <rdfs:subClassOf rdf:resource="http://www.ontologyrepository.com/CommonCoreOntologies/UserAccount"/>
        <skos:definition xml:lang="en">A User Account used for system adiministration that  has all permissions to all files and programs.</skos:definition>
        <rdfs:label xml:lang="en">Superuser Account</rdfs:label>
        <cco2:ont00001754 rdf:datatype="http://www.w3.org/2001/XMLSchema#anyURI">https://en.wikipedia.org/wiki/Superuser</cco2:ont00001754>
        <cco2:ont00001760 rdf:datatype="http://www.w3.org/2001/XMLSchema#anyURI">http://www.ontologyrepository.com/CommonCoreOntologies/Domain/CyberOntology</cco2:ont00001760>
    </owl:Class>
    


    <!-- http://www.ontologyrepository.com/CommonCoreOntologies/SystemAccount -->

    <owl:Class rdf:about="http://www.ontologyrepository.com/CommonCoreOntologies/SystemAccount">
        <rdfs:subClassOf rdf:resource="http://www.ontologyrepository.com/CommonCoreOntologies/UserAccount"/>
        <skos:definition xml:lang="en">A User Account  that is created by an operating system during installation and that is used for operating system defined purposes.</skos:definition>
        <rdfs:label xml:lang="en">System Account</rdfs:label>
        <cco2:ont00001754 rdf:datatype="http://www.w3.org/2001/XMLSchema#anyURI">https://www.ssh.com/iam/user/system-account</cco2:ont00001754>
        <cco2:ont00001760 rdf:datatype="http://www.w3.org/2001/XMLSchema#anyURI">http://www.ontologyrepository.com/CommonCoreOntologies/Domain/CyberOntology</cco2:ont00001760>
    </owl:Class>
    


    <!-- http://www.ontologyrepository.com/CommonCoreOntologies/SystemMonitor -->

    <owl:Class rdf:about="http://www.ontologyrepository.com/CommonCoreOntologies/SystemMonitor">
        <rdfs:subClassOf rdf:resource="http://www.ontologyrepository.com/CommonCoreOntologies/UtilityProgram"/>
        <skos:definition xml:lang="en">A Utility Program that is designed to monitor resources and performance in a Computer.</skos:definition>
        <rdfs:label xml:lang="en">System Monitor</rdfs:label>
        <cco2:ont00001754>https://en.wikipedia.org/wiki/System_monitor</cco2:ont00001754>
        <cco2:ont00001760 rdf:datatype="http://www.w3.org/2001/XMLSchema#anyURI">http://www.ontologyrepository.com/CommonCoreOntologies/Domain/CyberOntology</cco2:ont00001760>
    </owl:Class>
    


    <!-- http://www.ontologyrepository.com/CommonCoreOntologies/SystemProfiler -->

    <owl:Class rdf:about="http://www.ontologyrepository.com/CommonCoreOntologies/SystemProfiler">
        <rdfs:subClassOf rdf:resource="http://www.ontologyrepository.com/CommonCoreOntologies/UtilityProgram"/>
        <skos:definition xml:lang="en">A Utility Program that is designed to provide detailed information about the software installed and hardware attached to a Computer.</skos:definition>
        <rdfs:label xml:lang="en">System Profiler</rdfs:label>
        <cco2:ont00001754>https://en.wikipedia.org/wiki/System_profiler</cco2:ont00001754>
        <cco2:ont00001760 rdf:datatype="http://www.w3.org/2001/XMLSchema#anyURI">http://www.ontologyrepository.com/CommonCoreOntologies/Domain/CyberOntology</cco2:ont00001760>
    </owl:Class>
    


    <!-- http://www.ontologyrepository.com/CommonCoreOntologies/SystemSoftware -->

    <owl:Class rdf:about="http://www.ontologyrepository.com/CommonCoreOntologies/SystemSoftware">
        <rdfs:subClassOf rdf:resource="http://www.ontologyrepository.com/CommonCoreOntologies/ComputerProgram"/>
        <skos:definition xml:lang="en">A Computer Program that is designed to support the infrastructure of a Computer.</skos:definition>
        <rdfs:label xml:lang="en">System Software</rdfs:label>
        <cco2:ont00001760 rdf:datatype="http://www.w3.org/2001/XMLSchema#anyURI">http://www.ontologyrepository.com/CommonCoreOntologies/Domain/CyberOntology</cco2:ont00001760>
    </owl:Class>
    


    <!-- http://www.ontologyrepository.com/CommonCoreOntologies/SystemVirtualMachine -->

    <owl:Class rdf:about="http://www.ontologyrepository.com/CommonCoreOntologies/SystemVirtualMachine">
        <rdfs:subClassOf rdf:resource="http://www.ontologyrepository.com/CommonCoreOntologies/VirtualMachine"/>
        <skos:definition xml:lang="en">A Virtual Machine that provides the functionality of an entire Operating System.</skos:definition>
        <rdfs:label xml:lang="en">System Virtual Machine</rdfs:label>
        <cco2:ont00001754>https://en.wikipedia.org/wiki/Virtual_machine</cco2:ont00001754>
        <cco2:ont00001760 rdf:datatype="http://www.w3.org/2001/XMLSchema#anyURI">http://www.ontologyrepository.com/CommonCoreOntologies/Domain/CyberOntology</cco2:ont00001760>
    </owl:Class>
    


    <!-- http://www.ontologyrepository.com/CommonCoreOntologies/TCPHeader -->

    <owl:Class rdf:about="http://www.ontologyrepository.com/CommonCoreOntologies/TCPHeader">
        <rdfs:subClassOf rdf:resource="http://www.ontologyrepository.com/CommonCoreOntologies/PacketHeader"/>
        <skos:definition xml:lang="en">A Packet Header that is prescribed by the Transmission Control Protocol.</skos:definition>
        <rdfs:label xml:lang="en">TCP Header</rdfs:label>
        <cco2:ont00001760 rdf:datatype="http://www.w3.org/2001/XMLSchema#anyURI">http://www.ontologyrepository.com/CommonCoreOntologies/Domain/CyberOntology</cco2:ont00001760>
    </owl:Class>
    


    <!-- http://www.ontologyrepository.com/CommonCoreOntologies/TCPThreeWayHandshake -->

    <owl:Class rdf:about="http://www.ontologyrepository.com/CommonCoreOntologies/TCPThreeWayHandshake">
        <rdfs:subClassOf rdf:resource="http://www.ontologyrepository.com/CommonCoreOntologies/NetworkConnectionInitiated"/>
        <skos:definition xml:lang="en">A Network Connection Initiation in which two hosts establish a network connection by means of Transmission Control Protocol flags (in order): SYN, SYN-ACK, and ACK.</skos:definition>
        <rdfs:label xml:lang="en">TCP Three-Way Handshake</rdfs:label>
        <cco2:ont00001754>https://en.wikipedia.org/wiki/Transmission_Control_Protocol#Connection_establishment</cco2:ont00001754>
        <cco2:ont00001760 rdf:datatype="http://www.w3.org/2001/XMLSchema#anyURI">http://www.ontologyrepository.com/CommonCoreOntologies/Domain/CyberOntology</cco2:ont00001760>
    </owl:Class>
    


    <!-- http://www.ontologyrepository.com/CommonCoreOntologies/TextEditorSoftwareApplication -->

    <owl:Class rdf:about="http://www.ontologyrepository.com/CommonCoreOntologies/TextEditorSoftwareApplication">
        <rdfs:subClassOf rdf:resource="http://www.ontologyrepository.com/CommonCoreOntologies/InformationWorkerSoftware"/>
        <skos:definition xml:lang="en">An Information Worker Software Application that is designed to enable a user to create and edit a Text File.</skos:definition>
        <rdfs:label xml:lang="en">Text Editor Software Application</rdfs:label>
        <cco2:ont00001760 rdf:datatype="http://www.w3.org/2001/XMLSchema#anyURI">http://www.ontologyrepository.com/CommonCoreOntologies/Domain/CyberOntology</cco2:ont00001760>
    </owl:Class>
    


    <!-- http://www.ontologyrepository.com/CommonCoreOntologies/TextFile -->

    <owl:Class rdf:about="http://www.ontologyrepository.com/CommonCoreOntologies/TextFile">
        <rdfs:subClassOf rdf:resource="http://www.ontologyrepository.com/CommonCoreOntologies/DigitalFile"/>
        <skos:definition xml:lang="en">A Digital File that bears information in such a way that it can be displayed as a sequence of human-readable symbols.</skos:definition>
        <rdfs:label xml:lang="en">Text File</rdfs:label>
        <cco2:ont00001760 rdf:datatype="http://www.w3.org/2001/XMLSchema#anyURI">http://www.ontologyrepository.com/CommonCoreOntologies/Domain/CyberOntology</cco2:ont00001760>
    </owl:Class>
    


    <!-- http://www.ontologyrepository.com/CommonCoreOntologies/TorNetwork -->

    <owl:Class rdf:about="http://www.ontologyrepository.com/CommonCoreOntologies/TorNetwork">
        <rdfs:subClassOf rdf:resource="http://www.ontologyrepository.com/CommonCoreOntologies/AnonymityNetwork"/>
        <skos:definition xml:lang="en">An Anonymity Network that uses TOR software.</skos:definition>
        <rdfs:label xml:lang="en">Tor Network</rdfs:label>
        <cco2:ont00001754>https://en.wikipedia.org/wiki/Tor_(anonymity_network)</cco2:ont00001754>
        <cco2:ont00001760 rdf:datatype="http://www.w3.org/2001/XMLSchema#anyURI">http://www.ontologyrepository.com/CommonCoreOntologies/Domain/CyberOntology</cco2:ont00001760>
    </owl:Class>
    


    <!-- http://www.ontologyrepository.com/CommonCoreOntologies/TrojanHorseProgram -->

    <owl:Class rdf:about="http://www.ontologyrepository.com/CommonCoreOntologies/TrojanHorseProgram">
        <rdfs:subClassOf rdf:resource="http://www.ontologyrepository.com/CommonCoreOntologies/Malware"/>
        <skos:definition xml:lang="en">Malware that is designed to deceive a user into executing it.</skos:definition>
        <rdfs:label xml:lang="en">Trojan Horse Program</rdfs:label>
        <cco2:ont00001754>https://en.wikipedia.org/wiki/Trojan_horse_(computing)</cco2:ont00001754>
        <cco2:ont00001760 rdf:datatype="http://www.w3.org/2001/XMLSchema#anyURI">http://www.ontologyrepository.com/CommonCoreOntologies/Domain/CyberOntology</cco2:ont00001760>
    </owl:Class>
    


    <!-- http://www.ontologyrepository.com/CommonCoreOntologies/Tuple -->

    <owl:Class rdf:about="http://www.ontologyrepository.com/CommonCoreOntologies/Tuple">
        <rdfs:subClassOf rdf:resource="http://www.ontologyrepository.com/CommonCoreOntologies/Array"/>
        <skos:definition xml:lang="en">An Array which orders its elements along one dimension only.</skos:definition>
        <rdfs:label xml:lang="en">Tuple</rdfs:label>
        <cco2:ont00001760 rdf:datatype="http://www.w3.org/2001/XMLSchema#anyURI">http://www.ontologyrepository.com/CommonCoreOntologies/Domain/CyberOntology</cco2:ont00001760>
    </owl:Class>
    


    <!-- http://www.ontologyrepository.com/CommonCoreOntologies/UnifiedThreatManagementFirewall -->

    <owl:Class rdf:about="http://www.ontologyrepository.com/CommonCoreOntologies/UnifiedThreatManagementFirewall">
        <rdfs:subClassOf rdf:resource="http://www.ontologyrepository.com/CommonCoreOntologies/Firewall"/>
        <skos:altLabel xml:lang="en">UTM Firewall</skos:altLabel>
        <skos:definition xml:lang="en">A Firewall that combines the functions of a Stateful Inspection Firewall and intrusion prevention and antivirus.</skos:definition>
        <rdfs:label xml:lang="en">Unified Threat Management Firewall</rdfs:label>
        <cco2:ont00001754>http://www.cisco.com/c/en/us/products/security/firewalls/what-is-a-firewall.html</cco2:ont00001754>
        <cco2:ont00001760 rdf:datatype="http://www.w3.org/2001/XMLSchema#anyURI">http://www.ontologyrepository.com/CommonCoreOntologies/Domain/CyberOntology</cco2:ont00001760>
    </owl:Class>
    


    <!-- http://www.ontologyrepository.com/CommonCoreOntologies/UniformResourceIdentifier -->

    <owl:Class rdf:about="http://www.ontologyrepository.com/CommonCoreOntologies/UniformResourceIdentifier">
        <rdfs:subClassOf rdf:resource="https://www.commoncoreontologies.org/ont00000077"/>
        <skos:definition xml:lang="en">A Code Identifier that designates a resource on a Computer Network.</skos:definition>
        <rdfs:label xml:lang="en">Uniform Resource Identifier</rdfs:label>
        <cco2:ont00001753>URI</cco2:ont00001753>
        <cco2:ont00001754>https://en.wikipedia.org/wiki/Uniform_Resource_Identifier</cco2:ont00001754>
        <cco2:ont00001760 rdf:datatype="http://www.w3.org/2001/XMLSchema#anyURI">http://www.ontologyrepository.com/CommonCoreOntologies/Domain/CyberOntology</cco2:ont00001760>
    </owl:Class>
    


    <!-- http://www.ontologyrepository.com/CommonCoreOntologies/UniformResourceLocator -->

    <owl:Class rdf:about="http://www.ontologyrepository.com/CommonCoreOntologies/UniformResourceLocator">
        <rdfs:subClassOf rdf:resource="http://www.ontologyrepository.com/CommonCoreOntologies/UniformResourceIdentifier"/>
        <skos:altLabel xml:lang="en">Web Address</skos:altLabel>
        <skos:definition xml:lang="en">A Uniform Resource Identifier that specifies both the primary access mechanism and network location of the designated resource.</skos:definition>
        <rdfs:label xml:lang="en">Uniform Resource Locator</rdfs:label>
        <cco2:ont00001753>URL</cco2:ont00001753>
        <cco2:ont00001754>https://en.wikipedia.org/wiki/Uniform_Resource_Identifier</cco2:ont00001754>
        <cco2:ont00001760 rdf:datatype="http://www.w3.org/2001/XMLSchema#anyURI">http://www.ontologyrepository.com/CommonCoreOntologies/Domain/CyberOntology</cco2:ont00001760>
    </owl:Class>
    


    <!-- http://www.ontologyrepository.com/CommonCoreOntologies/UnixOperatingSystemModel -->

    <owl:Class rdf:about="http://www.ontologyrepository.com/CommonCoreOntologies/UnixOperatingSystemModel">
        <rdfs:subClassOf rdf:resource="http://www.ontologyrepository.com/CommonCoreOntologies/OperatingSystemSoftwareModel"/>
        <skos:definition xml:lang="en">A Operating System Software Model that has evolved from the original AT&amp;T Unix Model</skos:definition>
        <rdfs:label xml:lang="en">Unix Operating System Model</rdfs:label>
        <cco2:ont00001754 xml:lang="en">https://en.wikipedia.org/wiki/Unix</cco2:ont00001754>
        <cco2:ont00001760 rdf:datatype="http://www.w3.org/2001/XMLSchema#anyURI">http://www.ontologyrepository.com/CommonCoreOntologies/Domain/CyberOntology</cco2:ont00001760>
    </owl:Class>
    


    <!-- http://www.ontologyrepository.com/CommonCoreOntologies/UploadingProcess -->

    <owl:Class rdf:about="http://www.ontologyrepository.com/CommonCoreOntologies/UploadingProcess">
        <rdfs:subClassOf rdf:resource="http://www.ontologyrepository.com/CommonCoreOntologies/FileTransfer"/>
        <skos:definition xml:lang="en">A File Transfer in which a Computer File stored on some user&apos;s local Computer is transferred to and stored on some remote Computer.</skos:definition>
        <rdfs:label xml:lang="en">Uploading Process</rdfs:label>
        <cco2:ont00001760 rdf:datatype="http://www.w3.org/2001/XMLSchema#anyURI">http://www.ontologyrepository.com/CommonCoreOntologies/Domain/CyberOntology</cco2:ont00001760>
    </owl:Class>
    


    <!-- http://www.ontologyrepository.com/CommonCoreOntologies/UrgentNominalMeasurement -->

    <owl:Class rdf:about="http://www.ontologyrepository.com/CommonCoreOntologies/UrgentNominalMeasurement">
        <rdfs:subClassOf rdf:resource="https://www.commoncoreontologies.org/ont00000293"/>
        <skos:definition xml:lang="en">A Nominal Measurement Information Content Entity that measures some entity as needing urgent attention.</skos:definition>
        <rdfs:label xml:lang="en">Urgent Nominal Measurement</rdfs:label>
        <cco2:ont00001760 rdf:datatype="http://www.w3.org/2001/XMLSchema#anyURI">http://www.ontologyrepository.com/CommonCoreOntologies/Domain/CyberOntology</cco2:ont00001760>
    </owl:Class>
    


    <!-- http://www.ontologyrepository.com/CommonCoreOntologies/UserAccount -->

    <owl:Class rdf:about="http://www.ontologyrepository.com/CommonCoreOntologies/UserAccount">
        <rdfs:subClassOf rdf:resource="http://www.ontologyrepository.com/CommonCoreOntologies/DigitalFile"/>
        <skos:definition xml:lang="en">A Digital File that stores information about an individual&apos;s username, password, and permission to access a computer system.</skos:definition>
        <rdfs:label xml:lang="en">User Account</rdfs:label>
        <cco2:ont00001760 rdf:datatype="http://www.w3.org/2001/XMLSchema#anyURI">http://www.ontologyrepository.com/CommonCoreOntologies/Domain/CyberOntology</cco2:ont00001760>
    </owl:Class>
    


    <!-- http://www.ontologyrepository.com/CommonCoreOntologies/UserGroupIdentifier -->

    <owl:Class rdf:about="http://www.ontologyrepository.com/CommonCoreOntologies/UserGroupIdentifier">
        <rdfs:subClassOf rdf:resource="https://www.commoncoreontologies.org/ont00000077"/>
        <skos:altLabel xml:lang="en">GID</skos:altLabel>
        <skos:definition xml:lang="en">A Code Identifier that identifies a group of registered users of a computer system for the purposes of managing access to that system.</skos:definition>
        <rdfs:label xml:lang="en">User Group Identifier</rdfs:label>
        <cco2:ont00001760 rdf:datatype="http://www.w3.org/2001/XMLSchema#anyURI">http://www.ontologyrepository.com/CommonCoreOntologies/Domain/CyberOntology</cco2:ont00001760>
    </owl:Class>
    


    <!-- http://www.ontologyrepository.com/CommonCoreOntologies/UserIdentifier -->

    <owl:Class rdf:about="http://www.ontologyrepository.com/CommonCoreOntologies/UserIdentifier">
        <rdfs:subClassOf rdf:resource="https://www.commoncoreontologies.org/ont00000077"/>
        <skos:altLabel xml:lang="en">UID</skos:altLabel>
        <skos:definition xml:lang="en">A Code Identifier that identifies the account of a registered user of a computer system.</skos:definition>
        <rdfs:label xml:lang="en">User Identifier</rdfs:label>
        <cco2:ont00001760 rdf:datatype="http://www.w3.org/2001/XMLSchema#anyURI">http://www.ontologyrepository.com/CommonCoreOntologies/Domain/CyberOntology</cco2:ont00001760>
    </owl:Class>
    


    <!-- http://www.ontologyrepository.com/CommonCoreOntologies/UtilityProgram -->

    <owl:Class rdf:about="http://www.ontologyrepository.com/CommonCoreOntologies/UtilityProgram">
        <rdfs:subClassOf rdf:resource="http://www.ontologyrepository.com/CommonCoreOntologies/SystemSoftware"/>
        <skos:definition xml:lang="en">System Software that is designed to analyze, configure, optimize, or maintain a Computer.</skos:definition>
        <rdfs:label xml:lang="en">Utility Program</rdfs:label>
        <cco2:ont00001760 rdf:datatype="http://www.w3.org/2001/XMLSchema#anyURI">http://www.ontologyrepository.com/CommonCoreOntologies/Domain/CyberOntology</cco2:ont00001760>
    </owl:Class>
    


    <!-- http://www.ontologyrepository.com/CommonCoreOntologies/Variable -->

    <owl:Class rdf:about="http://www.ontologyrepository.com/CommonCoreOntologies/Variable">
        <rdfs:subClassOf rdf:resource="https://www.commoncoreontologies.org/ont00000798"/>
        <skos:definition xml:lang="en">An Information Bearing Artifact that is designed to bear different Information Content Entities within the context of an Algorithm.</skos:definition>
        <rdfs:label xml:lang="en">Variable</rdfs:label>
        <cco2:ont00001760 rdf:datatype="http://www.w3.org/2001/XMLSchema#anyURI">http://www.ontologyrepository.com/CommonCoreOntologies/Domain/CyberOntology</cco2:ont00001760>
    </owl:Class>
    


    <!-- http://www.ontologyrepository.com/CommonCoreOntologies/VariableField -->

    <owl:Class rdf:about="http://www.ontologyrepository.com/CommonCoreOntologies/VariableField">
        <rdfs:subClassOf rdf:resource="http://www.ontologyrepository.com/CommonCoreOntologies/Variable"/>
        <skos:altLabel xml:lang="en">Member Variable</skos:altLabel>
        <skos:definition xml:lang="en">A Variable that is associated with a Computer Object and accessible for all its Programming Methods.</skos:definition>
        <rdfs:label xml:lang="en">Variable Field</rdfs:label>
        <cco2:ont00001760 rdf:datatype="http://www.w3.org/2001/XMLSchema#anyURI">http://www.ontologyrepository.com/CommonCoreOntologies/Domain/CyberOntology</cco2:ont00001760>
    </owl:Class>
    


    <!-- http://www.ontologyrepository.com/CommonCoreOntologies/VehicleSimulator -->

    <owl:Class rdf:about="http://www.ontologyrepository.com/CommonCoreOntologies/VehicleSimulator">
        <rdfs:subClassOf rdf:resource="http://www.ontologyrepository.com/CommonCoreOntologies/SimulationSoftware"/>
        <skos:definition xml:lang="en">Simulation Software that is designed to enable a user to model the process of operating a Vehicle.</skos:definition>
        <rdfs:label xml:lang="en">Vehicle Simulator</rdfs:label>
        <cco2:ont00001760 rdf:datatype="http://www.w3.org/2001/XMLSchema#anyURI">http://www.ontologyrepository.com/CommonCoreOntologies/Domain/CyberOntology</cco2:ont00001760>
    </owl:Class>
    


    <!-- http://www.ontologyrepository.com/CommonCoreOntologies/VersionControlUtility -->

    <owl:Class rdf:about="http://www.ontologyrepository.com/CommonCoreOntologies/VersionControlUtility">
        <rdfs:subClassOf rdf:resource="http://www.ontologyrepository.com/CommonCoreOntologies/DataSynchronizationUtility"/>
        <skos:definition xml:lang="en">A Data Synchronization Utility that is designed to manage changes to a collection of information over time.</skos:definition>
        <rdfs:label xml:lang="en">Version Control Utility</rdfs:label>
        <cco2:ont00001754>https://en.wikipedia.org/wiki/Version_control</cco2:ont00001754>
        <cco2:ont00001760 rdf:datatype="http://www.w3.org/2001/XMLSchema#anyURI">http://www.ontologyrepository.com/CommonCoreOntologies/Domain/CyberOntology</cco2:ont00001760>
    </owl:Class>
    


    <!-- http://www.ontologyrepository.com/CommonCoreOntologies/VideoEditingSoftwareApplication -->

    <owl:Class rdf:about="http://www.ontologyrepository.com/CommonCoreOntologies/VideoEditingSoftwareApplication">
        <rdfs:subClassOf rdf:resource="http://www.ontologyrepository.com/CommonCoreOntologies/MultimediaSoftwareApplication"/>
        <skos:definition xml:lang="en">A Multimedia Software Application that is designed to enable a user to create and edit video files.</skos:definition>
        <rdfs:label xml:lang="en">Video Editing Software Application</rdfs:label>
        <cco2:ont00001760 rdf:datatype="http://www.w3.org/2001/XMLSchema#anyURI">http://www.ontologyrepository.com/CommonCoreOntologies/Domain/CyberOntology</cco2:ont00001760>
    </owl:Class>
    


    <!-- http://www.ontologyrepository.com/CommonCoreOntologies/VirtualMachine -->

    <owl:Class rdf:about="http://www.ontologyrepository.com/CommonCoreOntologies/VirtualMachine">
        <rdfs:subClassOf rdf:resource="http://www.ontologyrepository.com/CommonCoreOntologies/Emulator"/>
        <skos:definition xml:lang="en">An Emulator that simulates the functionality of a physical Computer.</skos:definition>
        <rdfs:label xml:lang="en">Virtual Machine</rdfs:label>
        <cco2:ont00001754>https://en.wikipedia.org/wiki/Virtual_machine</cco2:ont00001754>
        <cco2:ont00001760 rdf:datatype="http://www.w3.org/2001/XMLSchema#anyURI">http://www.ontologyrepository.com/CommonCoreOntologies/Domain/CyberOntology</cco2:ont00001760>
    </owl:Class>
    


    <!-- http://www.ontologyrepository.com/CommonCoreOntologies/VirtualPrivateNetwork -->

    <owl:Class rdf:about="http://www.ontologyrepository.com/CommonCoreOntologies/VirtualPrivateNetwork">
        <rdfs:subClassOf rdf:resource="http://www.ontologyrepository.com/CommonCoreOntologies/PrivateComputerNetwork"/>
        <skos:altLabel xml:lang="en">VPN</skos:altLabel>
        <skos:definition xml:lang="en">A Private Computer Network that can be accessed via a non-Private Network.</skos:definition>
        <rdfs:label xml:lang="en">Virtual Private Network</rdfs:label>
        <cco2:ont00001760 rdf:datatype="http://www.w3.org/2001/XMLSchema#anyURI">http://www.ontologyrepository.com/CommonCoreOntologies/Domain/CyberOntology</cco2:ont00001760>
    </owl:Class>
    


    <!-- http://www.ontologyrepository.com/CommonCoreOntologies/Vlog -->

    <owl:Class rdf:about="http://www.ontologyrepository.com/CommonCoreOntologies/Vlog">
        <rdfs:subClassOf rdf:resource="http://www.ontologyrepository.com/CommonCoreOntologies/Blog"/>
        <skos:definition xml:lang="en">A Blog whose posts are Videos.</skos:definition>
        <rdfs:label xml:lang="en">Vlog</rdfs:label>
        <cco2:ont00001760 rdf:datatype="http://www.w3.org/2001/XMLSchema#anyURI">http://www.ontologyrepository.com/CommonCoreOntologies/Domain/CyberOntology</cco2:ont00001760>
    </owl:Class>
    


    <!-- http://www.ontologyrepository.com/CommonCoreOntologies/VulnerabilityScannerSoftware -->

    <owl:Class rdf:about="http://www.ontologyrepository.com/CommonCoreOntologies/VulnerabilityScannerSoftware">
        <rdfs:subClassOf rdf:resource="http://www.ontologyrepository.com/CommonCoreOntologies/ApplicationSoftware"/>
        <skos:definition xml:lang="en">An Application Software designed to assess computers, networks or applications for known weaknesses.</skos:definition>
        <rdfs:label xml:lang="en">Vulnerability Scanner Software</rdfs:label>
        <cco2:ont00001754 rdf:datatype="http://www.w3.org/2001/XMLSchema#anyURI">https://en.wikipedia.org/wiki/Vulnerability_scanner</cco2:ont00001754>
        <cco2:ont00001760 rdf:datatype="http://www.w3.org/2001/XMLSchema#anyURI">http://www.ontologyrepository.com/CommonCoreOntologies/Domain/CyberOntology</cco2:ont00001760>
    </owl:Class>
    


    <!-- http://www.ontologyrepository.com/CommonCoreOntologies/Watchlist -->

    <owl:Class rdf:about="http://www.ontologyrepository.com/CommonCoreOntologies/Watchlist">
        <rdfs:subClassOf rdf:resource="https://www.commoncoreontologies.org/ont00000965"/>
        <skos:definition xml:lang="en">A Directive Information Content Entity which prescribes which individuals, groups, or items require close surveillance.</skos:definition>
        <rdfs:label xml:lang="en">Watchlist</rdfs:label>
        <cco2:ont00001760 rdf:datatype="http://www.w3.org/2001/XMLSchema#anyURI">http://www.ontologyrepository.com/CommonCoreOntologies/Domain/CyberOntology</cco2:ont00001760>
    </owl:Class>
    


    <!-- http://www.ontologyrepository.com/CommonCoreOntologies/WebBrowser -->

    <owl:Class rdf:about="http://www.ontologyrepository.com/CommonCoreOntologies/WebBrowser">
        <rdfs:subClassOf rdf:resource="http://www.ontologyrepository.com/CommonCoreOntologies/ContentAccessSoftware"/>
        <skos:definition xml:lang="en">A Content Access Software Application that is used to retrieve, present, and traverse information resources on the Internet.</skos:definition>
        <skos:example>Google Chrome</skos:example>
        <rdfs:label xml:lang="en">Web Browser</rdfs:label>
        <cco2:ont00001760 rdf:datatype="http://www.w3.org/2001/XMLSchema#anyURI">http://www.ontologyrepository.com/CommonCoreOntologies/Domain/CyberOntology</cco2:ont00001760>
    </owl:Class>
    


    <!-- http://www.ontologyrepository.com/CommonCoreOntologies/WebPage -->

    <owl:Class rdf:about="http://www.ontologyrepository.com/CommonCoreOntologies/WebPage">
        <rdfs:subClassOf rdf:resource="http://www.ontologyrepository.com/CommonCoreOntologies/DigitalFile"/>
        <skos:definition xml:lang="en">A Digital File that is accessed over the Internet using a Web Browser.</skos:definition>
        <rdfs:comment xml:lang="en">Web Pages often have Web Applications as parts.</rdfs:comment>
        <rdfs:label xml:lang="en">Web Page</rdfs:label>
        <cco2:ont00001760 rdf:datatype="http://www.w3.org/2001/XMLSchema#anyURI">http://www.ontologyrepository.com/CommonCoreOntologies/Domain/CyberOntology</cco2:ont00001760>
    </owl:Class>
    


    <!-- http://www.ontologyrepository.com/CommonCoreOntologies/WebPortal -->

    <owl:Class rdf:about="http://www.ontologyrepository.com/CommonCoreOntologies/WebPortal">
        <rdfs:subClassOf rdf:resource="http://www.ontologyrepository.com/CommonCoreOntologies/WebPage"/>
        <skos:definition xml:lang="en">A Web Page that is an organized gateway that helps to configure the access to information found on the Internet.</skos:definition>
        <rdfs:label xml:lang="en">Web Portal</rdfs:label>
        <cco2:ont00001754>https://en.wikipedia.org/wiki/Web_portal</cco2:ont00001754>
        <cco2:ont00001760 rdf:datatype="http://www.w3.org/2001/XMLSchema#anyURI">http://www.ontologyrepository.com/CommonCoreOntologies/Domain/CyberOntology</cco2:ont00001760>
    </owl:Class>
    


    <!-- http://www.ontologyrepository.com/CommonCoreOntologies/WebServer -->

    <owl:Class rdf:about="http://www.ontologyrepository.com/CommonCoreOntologies/WebServer">
        <rdfs:subClassOf rdf:resource="http://www.ontologyrepository.com/CommonCoreOntologies/NetworkServer"/>
        <skos:definition xml:lang="en">A Network Server that enables a client to access a Computer Service Function over the World Wide Web..</skos:definition>
        <rdfs:label xml:lang="en">Web Server</rdfs:label>
        <cco2:ont00001754 rdf:datatype="http://www.w3.org/2001/XMLSchema#anyURI">https://en.wikipedia.org/wiki/Web_server</cco2:ont00001754>
        <cco2:ont00001760 rdf:datatype="http://www.w3.org/2001/XMLSchema#anyURI">http://www.ontologyrepository.com/CommonCoreOntologies/Domain/CyberOntology</cco2:ont00001760>
    </owl:Class>
    


    <!-- http://www.ontologyrepository.com/CommonCoreOntologies/WebServiceFunction -->

    <owl:Class rdf:about="http://www.ontologyrepository.com/CommonCoreOntologies/WebServiceFunction">
        <rdfs:subClassOf rdf:resource="http://www.ontologyrepository.com/CommonCoreOntologies/NetworkServiceFunction"/>
        <skos:altLabel xml:lang="en">Web Service</skos:altLabel>
        <skos:definition xml:lang="en">A Computer Service Function that when realized is in a process of a client accessing a service over the World Wide Web.</skos:definition>
        <rdfs:label xml:lang="en">Web Service Function</rdfs:label>
        <cco2:ont00001754 rdf:datatype="http://www.w3.org/2001/XMLSchema#anyURI">https://en.wikipedia.org/wiki/Web_service</cco2:ont00001754>
        <cco2:ont00001760 rdf:datatype="http://www.w3.org/2001/XMLSchema#anyURI">http://www.ontologyrepository.com/CommonCoreOntologies/Domain/CyberOntology</cco2:ont00001760>
    </owl:Class>
    


    <!-- http://www.ontologyrepository.com/CommonCoreOntologies/WebServiceStack -->

    <owl:Class rdf:about="http://www.ontologyrepository.com/CommonCoreOntologies/WebServiceStack">
        <rdfs:subClassOf rdf:resource="http://www.ontologyrepository.com/CommonCoreOntologies/SoftwareStack"/>
        <skos:definition xml:lang="en">A Software Stack that is designed for enabling the use of Web Servers and their hosted services.</skos:definition>
        <rdfs:label xml:lang="en">Web Service Stack</rdfs:label>
        <cco2:ont00001760 rdf:datatype="http://www.w3.org/2001/XMLSchema#anyURI">http://www.ontologyrepository.com/CommonCoreOntologies/Domain/CyberOntology</cco2:ont00001760>
    </owl:Class>
    


    <!-- http://www.ontologyrepository.com/CommonCoreOntologies/Website -->

    <owl:Class rdf:about="http://www.ontologyrepository.com/CommonCoreOntologies/Website">
        <rdfs:subClassOf rdf:resource="https://www.commoncoreontologies.org/ont00000798"/>
        <rdfs:subClassOf>
            <owl:Restriction>
                <owl:onProperty rdf:resource="http://purl.obolibrary.org/obo/BFO_0000178"/>
                <owl:someValuesFrom rdf:resource="http://www.ontologyrepository.com/CommonCoreOntologies/WebPage"/>
            </owl:Restriction>
        </rdfs:subClassOf>
        <skos:definition xml:lang="en">An Information Bearing Artifact that is an aggregate of Web Pages.</skos:definition>
        <rdfs:label xml:lang="en">Website</rdfs:label>
        <cco2:ont00001760 rdf:datatype="http://www.w3.org/2001/XMLSchema#anyURI">http://www.ontologyrepository.com/CommonCoreOntologies/Domain/CyberOntology</cco2:ont00001760>
    </owl:Class>
    


    <!-- http://www.ontologyrepository.com/CommonCoreOntologies/WideAreaNetwork -->

    <owl:Class rdf:about="http://www.ontologyrepository.com/CommonCoreOntologies/WideAreaNetwork">
        <rdfs:subClassOf rdf:resource="https://www.commoncoreontologies.org/ont00000700"/>
        <skos:altLabel xml:lang="en">WAN</skos:altLabel>
        <skos:definition xml:lang="en">A Computer Network that is designed to connect several resources and is not restricted to a geographical location.</skos:definition>
        <rdfs:label xml:lang="en">Wide Area Network</rdfs:label>
        <cco2:ont00001754>https://kb.iu.edu/d/agki</cco2:ont00001754>
        <cco2:ont00001760 rdf:datatype="http://www.w3.org/2001/XMLSchema#anyURI">http://www.ontologyrepository.com/CommonCoreOntologies/Domain/CyberOntology</cco2:ont00001760>
    </owl:Class>
    


    <!-- http://www.ontologyrepository.com/CommonCoreOntologies/WidowsServerOperatingSystemModel -->

    <owl:Class rdf:about="http://www.ontologyrepository.com/CommonCoreOntologies/WidowsServerOperatingSystemModel">
        <rdfs:subClassOf rdf:resource="http://www.ontologyrepository.com/CommonCoreOntologies/WindowsOperatingSystemModel"/>
        <skos:definition xml:lang="en">A Windows Operating System Model that prescribes a Microsoft Server Operating System.</skos:definition>
        <rdfs:label xml:lang="en">Windows Server Operating System Model</rdfs:label>
        <cco2:ont00001754 rdf:datatype="http://www.w3.org/2001/XMLSchema#anyURI">https://en.wikipedia.org/wiki/Windows_Server</cco2:ont00001754>
        <cco2:ont00001760 rdf:datatype="http://www.w3.org/2001/XMLSchema#anyURI">http://www.ontologyrepository.com/CommonCoreOntologies/Domain/CyberOntology</cco2:ont00001760>
    </owl:Class>
    


    <!-- http://www.ontologyrepository.com/CommonCoreOntologies/WindowSizeDirective -->

    <owl:Class rdf:about="http://www.ontologyrepository.com/CommonCoreOntologies/WindowSizeDirective">
        <rdfs:subClassOf rdf:resource="http://www.ontologyrepository.com/CommonCoreOntologies/FlowControlDirective"/>
        <skos:definition xml:lang="en">A Flow Control Directive that prescribes the rate of data transmission in an Information Transfer Process.</skos:definition>
        <rdfs:label xml:lang="en">Window Size Directive</rdfs:label>
        <cco2:ont00001760 rdf:datatype="http://www.w3.org/2001/XMLSchema#anyURI">http://www.ontologyrepository.com/CommonCoreOntologies/Domain/CyberOntology</cco2:ont00001760>
    </owl:Class>
    


    <!-- http://www.ontologyrepository.com/CommonCoreOntologies/WindowsOperatingSystemModel -->

    <owl:Class rdf:about="http://www.ontologyrepository.com/CommonCoreOntologies/WindowsOperatingSystemModel">
        <rdfs:subClassOf rdf:resource="http://www.ontologyrepository.com/CommonCoreOntologies/OperatingSystemSoftwareModel"/>
        <skos:definition xml:lang="en">A Operating System Software Model that is developed and marketed by Microsoft.</skos:definition>
        <rdfs:label xml:lang="en">Windows Operating System Model</rdfs:label>
        <cco2:ont00001754 xml:lang="en">https://en.wikipedia.org/wiki/Microsoft_Windows</cco2:ont00001754>
        <cco2:ont00001760 rdf:datatype="http://www.w3.org/2001/XMLSchema#anyURI">http://www.ontologyrepository.com/CommonCoreOntologies/Domain/CyberOntology</cco2:ont00001760>
    </owl:Class>
    


    <!-- http://www.ontologyrepository.com/CommonCoreOntologies/WirelessLocalAreaNetwork -->

    <owl:Class rdf:about="http://www.ontologyrepository.com/CommonCoreOntologies/WirelessLocalAreaNetwork">
        <rdfs:subClassOf rdf:resource="http://www.ontologyrepository.com/CommonCoreOntologies/LocalAreaNetwork"/>
        <skos:altLabel xml:lang="en">WLAN</skos:altLabel>
        <skos:definition xml:lang="en">A Local Area Network that connects resources wirelessly.</skos:definition>
        <rdfs:label xml:lang="en">Wireless Local Area Network</rdfs:label>
        <cco2:ont00001760 rdf:datatype="http://www.w3.org/2001/XMLSchema#anyURI">http://www.ontologyrepository.com/CommonCoreOntologies/Domain/CyberOntology</cco2:ont00001760>
    </owl:Class>
    


    <!-- http://www.ontologyrepository.com/CommonCoreOntologies/WordProcessingSoftwareApplication -->

    <owl:Class rdf:about="http://www.ontologyrepository.com/CommonCoreOntologies/WordProcessingSoftwareApplication">
        <rdfs:subClassOf rdf:resource="http://www.ontologyrepository.com/CommonCoreOntologies/InformationWorkerSoftware"/>
        <skos:definition xml:lang="en">An Information Worker Software Application that is designed to enable a user to create, edit, and format Documents.</skos:definition>
        <rdfs:label xml:lang="en">Word Processing Software Application</rdfs:label>
        <cco2:ont00001760 rdf:datatype="http://www.w3.org/2001/XMLSchema#anyURI">http://www.ontologyrepository.com/CommonCoreOntologies/Domain/CyberOntology</cco2:ont00001760>
    </owl:Class>
    


    <!-- http://www.ontologyrepository.com/CommonCoreOntologies/WriteFilePermission -->

    <owl:Class rdf:about="http://www.ontologyrepository.com/CommonCoreOntologies/WriteFilePermission">
        <rdfs:subClassOf rdf:resource="http://www.ontologyrepository.com/CommonCoreOntologies/FilePermission"/>
        <skos:definition xml:lang="en">A File Permission that prescribes the editing of a file by a user account.</skos:definition>
        <rdfs:label xml:lang="en">Write File Permission</rdfs:label>
        <cco2:ont00001754 rdf:datatype="http://www.w3.org/2001/XMLSchema#anyURI">https://en.wikipedia.org/wiki/File_system_permissions</cco2:ont00001754>
        <cco2:ont00001760 rdf:datatype="http://www.w3.org/2001/XMLSchema#anyURI">http://www.ontologyrepository.com/CommonCoreOntologies/Domain/CyberOntology</cco2:ont00001760>
    </owl:Class>
    


    <!-- http://www.ontologyrepository.com/CommonCoreOntologies/WrittenSymbol -->

    <owl:Class rdf:about="http://www.ontologyrepository.com/CommonCoreOntologies/WrittenSymbol">
        <rdfs:subClassOf rdf:resource="https://www.commoncoreontologies.org/ont00000798"/>
        <skos:definition xml:lang="en">An Information Bearing Artifact that is designed to facilitate written communication.</skos:definition>
        <rdfs:label xml:lang="en">Written Symbol</rdfs:label>
        <cco2:ont00001760 rdf:datatype="http://www.w3.org/2001/XMLSchema#anyURI">http://www.ontologyrepository.com/CommonCoreOntologies/Domain/CyberOntology</cco2:ont00001760>
    </owl:Class>
    


    <!-- http://www.ontologyrepository.com/CommonCoreOntologies/WrittenWord -->

    <owl:Class rdf:about="http://www.ontologyrepository.com/CommonCoreOntologies/WrittenWord">
        <rdfs:subClassOf rdf:resource="http://www.ontologyrepository.com/CommonCoreOntologies/WrittenSymbol"/>
        <rdfs:subClassOf>
            <owl:Restriction>
                <owl:onProperty rdf:resource="http://purl.obolibrary.org/obo/BFO_0000178"/>
                <owl:someValuesFrom rdf:resource="http://www.ontologyrepository.com/CommonCoreOntologies/Morpheme"/>
            </owl:Restriction>
        </rdfs:subClassOf>
        <skos:definition xml:lang="en">A Written Symbol that is the smallest meaningful unit of a writing system which has freestanding semantic or pragmatic content and that consists of 1 or more Morphemes.</skos:definition>
        <rdfs:label xml:lang="en">Written Word</rdfs:label>
        <cco2:ont00001754>https://en.wikipedia.org/wiki/Word</cco2:ont00001754>
        <cco2:ont00001760 rdf:datatype="http://www.w3.org/2001/XMLSchema#anyURI">http://www.ontologyrepository.com/CommonCoreOntologies/Domain/CyberOntology</cco2:ont00001760>
    </owl:Class>
    


    <!-- http://www.ontologyrepository.com/CommonCoreOntologies/XMLDatabaseSoftwareApplicationModel -->

    <owl:Class rdf:about="http://www.ontologyrepository.com/CommonCoreOntologies/XMLDatabaseSoftwareApplicationModel">
        <rdfs:subClassOf rdf:resource="http://www.ontologyrepository.com/CommonCoreOntologies/DocumentStoreDatabaseSoftwareApplicationModel"/>
        <skos:definition xml:lang="en">A Document Store Database Software Application Model that prescribes a data persistence software system that allows data to be specified, and sometimes stored, in XML format.</skos:definition>
        <rdfs:label xml:lang="en">XML Database Software Application Model</rdfs:label>
        <cco2:ont00001754 rdf:datatype="http://www.w3.org/2001/XMLSchema#anyURI">https://en.wikipedia.org/wiki/XML_database</cco2:ont00001754>
        <cco2:ont00001760 rdf:datatype="http://www.w3.org/2001/XMLSchema#anyURI">http://www.ontologyrepository.com/CommonCoreOntologies/Domain/CyberOntology</cco2:ont00001760>
    </owl:Class>
    


    <!-- http://www.ontologyrepository.com/CommonCoreOntologies/ZombieComputerProgramExecution -->

    <owl:Class rdf:about="http://www.ontologyrepository.com/CommonCoreOntologies/ZombieComputerProgramExecution">
        <rdfs:subClassOf rdf:resource="http://www.ontologyrepository.com/CommonCoreOntologies/ChildComputerProgramExecution"/>
        <skos:altLabel xml:lang="en">Zombie Computer Process</skos:altLabel>
        <skos:definition xml:lang="en">A Child Computer Program Execution that has terminated but is still identified by an entry in a process table.</skos:definition>
        <rdfs:comment xml:lang="en">Shall be axiomatized as an equivalency, eg. Child Program Execution and  participates in some Terminated Stasis and designated by some (Identifier and part of some Process Table).</rdfs:comment>
        <rdfs:label xml:lang="en">Zombie Computer Program Execution</rdfs:label>
        <cco2:ont00001754 rdf:datatype="http://www.w3.org/2001/XMLSchema#anyURI">https://en.wikipedia.org/wiki/Zombie_process</cco2:ont00001754>
        <cco2:ont00001760 rdf:datatype="http://www.w3.org/2001/XMLSchema#anyURI">http://www.ontologyrepository.com/CommonCoreOntologies/Domain/CyberOntology</cco2:ont00001760>
    </owl:Class>
    


    <!-- http://www.ontologyrepository.com/CommonCoreOntologies/netshUtility -->

    <owl:Class rdf:about="http://www.ontologyrepository.com/CommonCoreOntologies/netshUtility">
        <rdfs:subClassOf rdf:resource="http://www.ontologyrepository.com/CommonCoreOntologies/NetworkUtility"/>
        <skos:altLabel xml:lang="en">netsh</skos:altLabel>
        <skos:definition xml:lang="en">A Network Utility that is designed to allow local or remote configuration of network devices.</skos:definition>
        <rdfs:label xml:lang="en">netsh Utility</rdfs:label>
        <cco2:ont00001754>https://en.wikipedia.org/wiki/Netsh</cco2:ont00001754>
        <cco2:ont00001760 rdf:datatype="http://www.w3.org/2001/XMLSchema#anyURI">http://www.ontologyrepository.com/CommonCoreOntologies/Domain/CyberOntology</cco2:ont00001760>
    </owl:Class>
    


    <!-- http://www.ontologyrepository.com/CommonCoreOntologies/netstatUtility -->

    <owl:Class rdf:about="http://www.ontologyrepository.com/CommonCoreOntologies/netstatUtility">
        <rdfs:subClassOf rdf:resource="http://www.ontologyrepository.com/CommonCoreOntologies/NetworkUtility"/>
        <skos:altLabel xml:lang="en">netstat</skos:altLabel>
        <skos:definition xml:lang="en">A Network Utility that is designed to display incoming and outgoing network connections for the Transmission Control Protocol, routing tables, network interfaces, and network protocol statistics.</skos:definition>
        <rdfs:label xml:lang="en">netstat Utility</rdfs:label>
        <cco2:ont00001754>https://en.wikipedia.org/wiki/Netstat</cco2:ont00001754>
        <cco2:ont00001760 rdf:datatype="http://www.w3.org/2001/XMLSchema#anyURI">http://www.ontologyrepository.com/CommonCoreOntologies/Domain/CyberOntology</cco2:ont00001760>
    </owl:Class>
    


    <!-- http://www.ontologyrepository.com/CommonCoreOntologies/nslookupUtility -->

    <owl:Class rdf:about="http://www.ontologyrepository.com/CommonCoreOntologies/nslookupUtility">
        <rdfs:subClassOf rdf:resource="http://www.ontologyrepository.com/CommonCoreOntologies/NetworkUtility"/>
        <skos:altLabel xml:lang="en">Name Server Lookup</skos:altLabel>
        <skos:altLabel xml:lang="en">nslookup</skos:altLabel>
        <skos:definition xml:lang="en">A Network Utility that is designed to query the Domain Name System (DNS) to obtain Domain Name or Internet Protocol Address mapping or for any other specific DNS record.</skos:definition>
        <rdfs:label xml:lang="en">nslookup Utility</rdfs:label>
        <cco2:ont00001754>https://en.wikipedia.org/wiki/Nslookup</cco2:ont00001754>
        <cco2:ont00001760 rdf:datatype="http://www.w3.org/2001/XMLSchema#anyURI">http://www.ontologyrepository.com/CommonCoreOntologies/Domain/CyberOntology</cco2:ont00001760>
    </owl:Class>
    


    <!-- http://www.ontologyrepository.com/CommonCoreOntologies/pingUtility -->

    <owl:Class rdf:about="http://www.ontologyrepository.com/CommonCoreOntologies/pingUtility">
        <rdfs:subClassOf rdf:resource="http://www.ontologyrepository.com/CommonCoreOntologies/NetworkUtility"/>
        <skos:altLabel xml:lang="en">ping</skos:altLabel>
        <skos:definition xml:lang="en">A Network Utility that is designed to test the reachability of a host on an Internet Protocol network.</skos:definition>
        <rdfs:label xml:lang="en">ping Utility</rdfs:label>
        <cco2:ont00001754>https://en.wikipedia.org/wiki/Ping_(networking_utility)</cco2:ont00001754>
        <cco2:ont00001760 rdf:datatype="http://www.w3.org/2001/XMLSchema#anyURI">http://www.ontologyrepository.com/CommonCoreOntologies/Domain/CyberOntology</cco2:ont00001760>
    </owl:Class>
    


    <!-- http://www.ontologyrepository.com/CommonCoreOntologies/tracerouteUtility -->

    <owl:Class rdf:about="http://www.ontologyrepository.com/CommonCoreOntologies/tracerouteUtility">
        <rdfs:subClassOf rdf:resource="http://www.ontologyrepository.com/CommonCoreOntologies/NetworkUtility"/>
        <skos:altLabel xml:lang="en">traceroute</skos:altLabel>
        <skos:definition xml:lang="en">A Network Utility that is designed to displaying the route (path) and measuring transit delays of Network Packets across an Internet Protocol network</skos:definition>
        <rdfs:label xml:lang="en">traceroute Utility</rdfs:label>
        <cco2:ont00001754>https://en.wikipedia.org/wiki/Traceroute</cco2:ont00001754>
        <cco2:ont00001760 rdf:datatype="http://www.w3.org/2001/XMLSchema#anyURI">http://www.ontologyrepository.com/CommonCoreOntologies/Domain/CyberOntology</cco2:ont00001760>
    </owl:Class>
    


    <!-- http://www.ontologyrepository.com/CommonCoreOntologies/vnStatUtility -->

    <owl:Class rdf:about="http://www.ontologyrepository.com/CommonCoreOntologies/vnStatUtility">
        <rdfs:subClassOf rdf:resource="http://www.ontologyrepository.com/CommonCoreOntologies/NetworkUtility"/>
        <skos:altLabel xml:lang="en">vnStat</skos:altLabel>
        <skos:definition xml:lang="en">A Network Utility that is designed to keeps a log of hourly, daily and monthly network traffic.</skos:definition>
        <rdfs:label xml:lang="en">vnStat Utility</rdfs:label>
        <cco2:ont00001754>https://en.wikipedia.org/wiki/Vnstat</cco2:ont00001754>
        <cco2:ont00001760 rdf:datatype="http://www.w3.org/2001/XMLSchema#anyURI">http://www.ontologyrepository.com/CommonCoreOntologies/Domain/CyberOntology</cco2:ont00001760>
    </owl:Class>
    


    <!-- https://www.commoncoreontologies.org/ont00000005 -->

    <owl:Class rdf:about="https://www.commoncoreontologies.org/ont00000005"/>
    


    <!-- https://www.commoncoreontologies.org/ont00000077 -->

    <owl:Class rdf:about="https://www.commoncoreontologies.org/ont00000077"/>
    


    <!-- https://www.commoncoreontologies.org/ont00000110 -->

    <owl:Class rdf:about="https://www.commoncoreontologies.org/ont00000110"/>
    


    <!-- https://www.commoncoreontologies.org/ont00000117 -->

    <owl:Class rdf:about="https://www.commoncoreontologies.org/ont00000117"/>
    


    <!-- https://www.commoncoreontologies.org/ont00000146 -->

    <owl:Class rdf:about="https://www.commoncoreontologies.org/ont00000146"/>
    


    <!-- https://www.commoncoreontologies.org/ont00000228 -->

    <owl:Class rdf:about="https://www.commoncoreontologies.org/ont00000228"/>
    


    <!-- https://www.commoncoreontologies.org/ont00000293 -->

    <owl:Class rdf:about="https://www.commoncoreontologies.org/ont00000293"/>
    


    <!-- https://www.commoncoreontologies.org/ont00000315 -->

    <owl:Class rdf:about="https://www.commoncoreontologies.org/ont00000315"/>
    


    <!-- https://www.commoncoreontologies.org/ont00000319 -->

    <owl:Class rdf:about="https://www.commoncoreontologies.org/ont00000319"/>
    


    <!-- https://www.commoncoreontologies.org/ont00000335 -->

    <owl:Class rdf:about="https://www.commoncoreontologies.org/ont00000335"/>
    


    <!-- https://www.commoncoreontologies.org/ont00000420 -->

    <owl:Class rdf:about="https://www.commoncoreontologies.org/ont00000420"/>
    


    <!-- https://www.commoncoreontologies.org/ont00000476 -->

    <owl:Class rdf:about="https://www.commoncoreontologies.org/ont00000476"/>
    


    <!-- https://www.commoncoreontologies.org/ont00000509 -->

    <owl:Class rdf:about="https://www.commoncoreontologies.org/ont00000509"/>
    


    <!-- https://www.commoncoreontologies.org/ont00000531 -->

    <owl:Class rdf:about="https://www.commoncoreontologies.org/ont00000531"/>
    


    <!-- https://www.commoncoreontologies.org/ont00000543 -->

    <owl:Class rdf:about="https://www.commoncoreontologies.org/ont00000543"/>
    


    <!-- https://www.commoncoreontologies.org/ont00000548 -->

    <owl:Class rdf:about="https://www.commoncoreontologies.org/ont00000548"/>
    


    <!-- https://www.commoncoreontologies.org/ont00000609 -->

    <owl:Class rdf:about="https://www.commoncoreontologies.org/ont00000609"/>
    


    <!-- https://www.commoncoreontologies.org/ont00000653 -->

    <owl:Class rdf:about="https://www.commoncoreontologies.org/ont00000653"/>
    


    <!-- https://www.commoncoreontologies.org/ont00000690 -->

    <owl:Class rdf:about="https://www.commoncoreontologies.org/ont00000690"/>
    


    <!-- https://www.commoncoreontologies.org/ont00000700 -->

    <owl:Class rdf:about="https://www.commoncoreontologies.org/ont00000700"/>
    


    <!-- https://www.commoncoreontologies.org/ont00000727 -->

    <owl:Class rdf:about="https://www.commoncoreontologies.org/ont00000727"/>
    


    <!-- https://www.commoncoreontologies.org/ont00000751 -->

    <owl:Class rdf:about="https://www.commoncoreontologies.org/ont00000751"/>
    


    <!-- https://www.commoncoreontologies.org/ont00000771 -->

    <owl:Class rdf:about="https://www.commoncoreontologies.org/ont00000771"/>
    


    <!-- https://www.commoncoreontologies.org/ont00000781 -->

    <owl:Class rdf:about="https://www.commoncoreontologies.org/ont00000781"/>
    


    <!-- https://www.commoncoreontologies.org/ont00000798 -->

    <owl:Class rdf:about="https://www.commoncoreontologies.org/ont00000798"/>
    


    <!-- https://www.commoncoreontologies.org/ont00000812 -->

    <owl:Class rdf:about="https://www.commoncoreontologies.org/ont00000812"/>
    


    <!-- https://www.commoncoreontologies.org/ont00000825 -->

    <owl:Class rdf:about="https://www.commoncoreontologies.org/ont00000825"/>
    


    <!-- https://www.commoncoreontologies.org/ont00000847 -->

    <owl:Class rdf:about="https://www.commoncoreontologies.org/ont00000847"/>
    


    <!-- https://www.commoncoreontologies.org/ont00000908 -->

    <owl:Class rdf:about="https://www.commoncoreontologies.org/ont00000908"/>
    


    <!-- https://www.commoncoreontologies.org/ont00000936 -->

    <owl:Class rdf:about="https://www.commoncoreontologies.org/ont00000936"/>
    


    <!-- https://www.commoncoreontologies.org/ont00000965 -->

    <owl:Class rdf:about="https://www.commoncoreontologies.org/ont00000965"/>
    


    <!-- https://www.commoncoreontologies.org/ont00000974 -->

    <owl:Class rdf:about="https://www.commoncoreontologies.org/ont00000974"/>
    


    <!-- https://www.commoncoreontologies.org/ont00000995 -->

    <owl:Class rdf:about="https://www.commoncoreontologies.org/ont00000995"/>
    


    <!-- https://www.commoncoreontologies.org/ont00000998 -->

    <owl:Class rdf:about="https://www.commoncoreontologies.org/ont00000998"/>
    


    <!-- https://www.commoncoreontologies.org/ont00001017 -->

    <owl:Class rdf:about="https://www.commoncoreontologies.org/ont00001017"/>
    


    <!-- https://www.commoncoreontologies.org/ont00001022 -->

    <owl:Class rdf:about="https://www.commoncoreontologies.org/ont00001022"/>
    


    <!-- https://www.commoncoreontologies.org/ont00001045 -->

    <owl:Class rdf:about="https://www.commoncoreontologies.org/ont00001045"/>
    


    <!-- https://www.commoncoreontologies.org/ont00001066 -->

    <owl:Class rdf:about="https://www.commoncoreontologies.org/ont00001066"/>
    


    <!-- https://www.commoncoreontologies.org/ont00001179 -->

    <owl:Class rdf:about="https://www.commoncoreontologies.org/ont00001179"/>
    


    <!-- https://www.commoncoreontologies.org/ont00001180 -->

    <owl:Class rdf:about="https://www.commoncoreontologies.org/ont00001180"/>
    


    <!-- https://www.commoncoreontologies.org/ont00001213 -->

    <owl:Class rdf:about="https://www.commoncoreontologies.org/ont00001213"/>
    


    <!-- https://www.commoncoreontologies.org/ont00001247 -->

    <owl:Class rdf:about="https://www.commoncoreontologies.org/ont00001247"/>
    


    <!-- https://www.commoncoreontologies.org/ont00001251 -->

    <owl:Class rdf:about="https://www.commoncoreontologies.org/ont00001251"/>
    


    <!-- https://www.commoncoreontologies.org/ont00001289 -->

    <owl:Class rdf:about="https://www.commoncoreontologies.org/ont00001289"/>
    


    <!-- https://www.commoncoreontologies.org/ont00001356 -->

    <owl:Class rdf:about="https://www.commoncoreontologies.org/ont00001356"/>
</rdf:RDF>



<!-- Generated by the OWL API (version 4.5.29) https://github.com/owlcs/owlapi -->

