<?xml version="1.0"?>
<rdf:RDF xmlns="https://hack.cybersystems.engineer/memex/ontologies/SeamlessDigitalEngineering#"
     xml:base="https://hack.cybersystems.engineer/memex/ontologies/SeamlessDigitalEngineering"
     xmlns:dc="http://purl.org/dc/elements/1.1/"
     xmlns:obo="http://purl.obolibrary.org/obo/"
     xmlns:owl="http://www.w3.org/2002/07/owl#"
     xmlns:rdf="http://www.w3.org/1999/02/22-rdf-syntax-ns#"
     xmlns:xml="http://www.w3.org/XML/1998/namespace"
     xmlns:xsd="http://www.w3.org/2001/XMLSchema#"
     xmlns:cco2="https://www.commoncoreontologies.org/"
     xmlns:rdfs="http://www.w3.org/2000/01/rdf-schema#"
     xmlns:skos="http://www.w3.org/2004/02/skos/core#"
     xmlns:Ecore="http://www.eclipse.org/emf/2002/Ecore#"
     xmlns:terms="http://purl.org/dc/terms/">
    <owl:Ontology rdf:about="https://hack.cybersystems.engineer/memex/ontologies/SeamlessDigitalEngineering">
        <owl:versionIRI rdf:resource="https://hack.cybersystems.engineer/memex/ontologies/SeamlessDigitalEngineering/v0.1"/>
        <owl:imports rdf:resource="http://www.ontologyrepository.com/CommonCoreOntologies/Domain/CyberOntology"/>
        <dc:contributor xml:lang="en">Members of INCOSE Digital Engineering Information eXchange (DEIX) Ontology Working Group</dc:contributor>
        <dc:creator xml:lang="en">James S. Wheaton</dc:creator>
        <dc:description xml:lang="en">Ontology for Seamless Digital Engineering based on Common Core Ontologies (CCO) and Basic Formal Ontology (BFO) (ISO/IEC/IEEE 21838-2:2021)</dc:description>
        <dc:license>MPL-2.0</dc:license>
        <terms:title xml:lang="en">Seamless Digital Engineering Ontology</terms:title>
        <owl:versionInfo rdf:datatype="http://www.w3.org/2001/XMLSchema#dateTime">2024-12-12T14:00:00-07:00</owl:versionInfo>
    </owl:Ontology>
    


    <!-- 
    ///////////////////////////////////////////////////////////////////////////////////////
    //
    // Annotation properties
    //
    ///////////////////////////////////////////////////////////////////////////////////////
     -->

    


    <!-- http://purl.org/dc/elements/1.1/contributor -->

    <owl:AnnotationProperty rdf:about="http://purl.org/dc/elements/1.1/contributor"/>
    


    <!-- http://purl.org/dc/elements/1.1/creator -->

    <owl:AnnotationProperty rdf:about="http://purl.org/dc/elements/1.1/creator"/>
    


    <!-- http://purl.org/dc/elements/1.1/date -->

    <owl:AnnotationProperty rdf:about="http://purl.org/dc/elements/1.1/date"/>
    


    <!-- http://purl.org/dc/elements/1.1/description -->

    <owl:AnnotationProperty rdf:about="http://purl.org/dc/elements/1.1/description"/>
    


    <!-- http://purl.org/dc/elements/1.1/license -->

    <owl:AnnotationProperty rdf:about="http://purl.org/dc/elements/1.1/license"/>
    


    <!-- http://purl.org/dc/elements/1.1/source -->

    <owl:AnnotationProperty rdf:about="http://purl.org/dc/elements/1.1/source"/>
    


    <!-- http://purl.org/dc/terms/title -->

    <owl:AnnotationProperty rdf:about="http://purl.org/dc/terms/title"/>
    


    <!-- http://www.w3.org/2002/07/owl#minQualifiedCardinality -->

    <owl:AnnotationProperty rdf:about="http://www.w3.org/2002/07/owl#minQualifiedCardinality"/>
    


    <!-- http://www.w3.org/2002/07/owl#qualifiedCardinality -->

    <owl:AnnotationProperty rdf:about="http://www.w3.org/2002/07/owl#qualifiedCardinality"/>
    


    <!-- http://www.w3.org/2004/02/skos/core#altLabel -->

    <owl:AnnotationProperty rdf:about="http://www.w3.org/2004/02/skos/core#altLabel"/>
    


    <!-- http://www.w3.org/2004/02/skos/core#definition -->

    <owl:AnnotationProperty rdf:about="http://www.w3.org/2004/02/skos/core#definition"/>
    


    <!-- http://www.w3.org/2004/02/skos/core#example -->

    <owl:AnnotationProperty rdf:about="http://www.w3.org/2004/02/skos/core#example"/>
    


    <!-- https://www.commoncoreontologies.org/ont00001753 -->

    <owl:AnnotationProperty rdf:about="https://www.commoncoreontologies.org/ont00001753"/>
    


    <!-- https://www.commoncoreontologies.org/ont00001754 -->

    <owl:AnnotationProperty rdf:about="https://www.commoncoreontologies.org/ont00001754"/>
    


    <!-- 
    ///////////////////////////////////////////////////////////////////////////////////////
    //
    // Datatypes
    //
    ///////////////////////////////////////////////////////////////////////////////////////
     -->

    


    <!-- http://www.w3.org/2001/XMLSchema#date -->

    <rdfs:Datatype rdf:about="http://www.w3.org/2001/XMLSchema#date"/>
    


    <!-- 
    ///////////////////////////////////////////////////////////////////////////////////////
    //
    // Object Properties
    //
    ///////////////////////////////////////////////////////////////////////////////////////
     -->

    


    <!-- http://purl.obolibrary.org/obo/BFO_0000055 -->

    <owl:ObjectProperty rdf:about="http://purl.obolibrary.org/obo/BFO_0000055"/>
    


    <!-- http://purl.obolibrary.org/obo/BFO_0000058 -->

    <owl:ObjectProperty rdf:about="http://purl.obolibrary.org/obo/BFO_0000058"/>
    


    <!-- http://purl.obolibrary.org/obo/BFO_0000059 -->

    <owl:ObjectProperty rdf:about="http://purl.obolibrary.org/obo/BFO_0000059"/>
    


    <!-- http://purl.obolibrary.org/obo/BFO_0000066 -->

    <owl:ObjectProperty rdf:about="http://purl.obolibrary.org/obo/BFO_0000066"/>
    


    <!-- http://purl.obolibrary.org/obo/BFO_0000084 -->

    <owl:ObjectProperty rdf:about="http://purl.obolibrary.org/obo/BFO_0000084"/>
    


    <!-- http://purl.obolibrary.org/obo/BFO_0000101 -->

    <owl:ObjectProperty rdf:about="http://purl.obolibrary.org/obo/BFO_0000101"/>
    


    <!-- http://purl.obolibrary.org/obo/BFO_0000115 -->

    <owl:ObjectProperty rdf:about="http://purl.obolibrary.org/obo/BFO_0000115"/>
    


    <!-- http://purl.obolibrary.org/obo/BFO_0000129 -->

    <owl:ObjectProperty rdf:about="http://purl.obolibrary.org/obo/BFO_0000129"/>
    


    <!-- http://purl.obolibrary.org/obo/BFO_0000176 -->

    <owl:ObjectProperty rdf:about="http://purl.obolibrary.org/obo/BFO_0000176"/>
    


    <!-- http://purl.obolibrary.org/obo/BFO_0000178 -->

    <owl:ObjectProperty rdf:about="http://purl.obolibrary.org/obo/BFO_0000178"/>
    


    <!-- http://purl.obolibrary.org/obo/BFO_0000183 -->

    <owl:ObjectProperty rdf:about="http://purl.obolibrary.org/obo/BFO_0000183"/>
    


    <!-- http://purl.obolibrary.org/obo/BFO_0000184 -->

    <owl:ObjectProperty rdf:about="http://purl.obolibrary.org/obo/BFO_0000184"/>
    


    <!-- http://purl.obolibrary.org/obo/BFO_0000185 -->

    <owl:ObjectProperty rdf:about="http://purl.obolibrary.org/obo/BFO_0000185"/>
    


    <!-- http://purl.obolibrary.org/obo/BFO_0000196 -->

    <owl:ObjectProperty rdf:about="http://purl.obolibrary.org/obo/BFO_0000196"/>
    


    <!-- https://hack.cybersystems.engineer/memex/ontologies/SeamlessDigitalEngineering#correctly_implements_language -->

    <owl:ObjectProperty rdf:about="https://hack.cybersystems.engineer/memex/ontologies/SeamlessDigitalEngineering#correctly_implements_language"/>
    


    <!-- https://www.commoncoreontologies.org/ont00001777 -->

    <owl:ObjectProperty rdf:about="https://www.commoncoreontologies.org/ont00001777"/>
    


    <!-- https://www.commoncoreontologies.org/ont00001787 -->

    <owl:ObjectProperty rdf:about="https://www.commoncoreontologies.org/ont00001787"/>
    


    <!-- https://www.commoncoreontologies.org/ont00001801 -->

    <owl:ObjectProperty rdf:about="https://www.commoncoreontologies.org/ont00001801"/>
    


    <!-- https://www.commoncoreontologies.org/ont00001803 -->

    <owl:ObjectProperty rdf:about="https://www.commoncoreontologies.org/ont00001803"/>
    


    <!-- https://www.commoncoreontologies.org/ont00001808 -->

    <owl:ObjectProperty rdf:about="https://www.commoncoreontologies.org/ont00001808"/>
    


    <!-- https://www.commoncoreontologies.org/ont00001809 -->

    <owl:ObjectProperty rdf:about="https://www.commoncoreontologies.org/ont00001809"/>
    


    <!-- https://www.commoncoreontologies.org/ont00001811 -->

    <owl:ObjectProperty rdf:about="https://www.commoncoreontologies.org/ont00001811"/>
    


    <!-- https://www.commoncoreontologies.org/ont00001816 -->

    <owl:ObjectProperty rdf:about="https://www.commoncoreontologies.org/ont00001816"/>
    


    <!-- https://www.commoncoreontologies.org/ont00001819 -->

    <owl:ObjectProperty rdf:about="https://www.commoncoreontologies.org/ont00001819"/>
    


    <!-- https://www.commoncoreontologies.org/ont00001833 -->

    <owl:ObjectProperty rdf:about="https://www.commoncoreontologies.org/ont00001833"/>
    


    <!-- https://www.commoncoreontologies.org/ont00001834 -->

    <owl:ObjectProperty rdf:about="https://www.commoncoreontologies.org/ont00001834"/>
    


    <!-- https://www.commoncoreontologies.org/ont00001836 -->

    <owl:ObjectProperty rdf:about="https://www.commoncoreontologies.org/ont00001836"/>
    


    <!-- https://www.commoncoreontologies.org/ont00001852 -->

    <owl:ObjectProperty rdf:about="https://www.commoncoreontologies.org/ont00001852"/>
    


    <!-- https://www.commoncoreontologies.org/ont00001857 -->

    <owl:ObjectProperty rdf:about="https://www.commoncoreontologies.org/ont00001857"/>
    


    <!-- https://www.commoncoreontologies.org/ont00001866 -->

    <owl:ObjectProperty rdf:about="https://www.commoncoreontologies.org/ont00001866"/>
    


    <!-- https://www.commoncoreontologies.org/ont00001888 -->

    <owl:ObjectProperty rdf:about="https://www.commoncoreontologies.org/ont00001888"/>
    


    <!-- https://www.commoncoreontologies.org/ont00001889 -->

    <owl:ObjectProperty rdf:about="https://www.commoncoreontologies.org/ont00001889"/>
    


    <!-- https://www.commoncoreontologies.org/ont00001898 -->

    <owl:ObjectProperty rdf:about="https://www.commoncoreontologies.org/ont00001898"/>
    


    <!-- https://www.commoncoreontologies.org/ont00001901 -->

    <owl:ObjectProperty rdf:about="https://www.commoncoreontologies.org/ont00001901"/>
    


    <!-- https://www.commoncoreontologies.org/ont00001904 -->

    <owl:ObjectProperty rdf:about="https://www.commoncoreontologies.org/ont00001904"/>
    


    <!-- https://www.commoncoreontologies.org/ont00001917 -->

    <owl:ObjectProperty rdf:about="https://www.commoncoreontologies.org/ont00001917"/>
    


    <!-- https://www.commoncoreontologies.org/ont00001920 -->

    <owl:ObjectProperty rdf:about="https://www.commoncoreontologies.org/ont00001920"/>
    


    <!-- https://www.commoncoreontologies.org/ont00001921 -->

    <owl:ObjectProperty rdf:about="https://www.commoncoreontologies.org/ont00001921"/>
    


    <!-- https://www.commoncoreontologies.org/ont00001925 -->

    <owl:ObjectProperty rdf:about="https://www.commoncoreontologies.org/ont00001925"/>
    


    <!-- https://www.commoncoreontologies.org/ont00001936 -->

    <owl:ObjectProperty rdf:about="https://www.commoncoreontologies.org/ont00001936"/>
    


    <!-- https://www.commoncoreontologies.org/ont00001938 -->

    <owl:ObjectProperty rdf:about="https://www.commoncoreontologies.org/ont00001938"/>
    


    <!-- https://www.commoncoreontologies.org/ont00001942 -->

    <owl:ObjectProperty rdf:about="https://www.commoncoreontologies.org/ont00001942"/>
    


    <!-- https://www.commoncoreontologies.org/ont00001947 -->

    <owl:ObjectProperty rdf:about="https://www.commoncoreontologies.org/ont00001947"/>
    


    <!-- https://www.commoncoreontologies.org/ont00001949 -->

    <owl:ObjectProperty rdf:about="https://www.commoncoreontologies.org/ont00001949"/>
    


    <!-- https://www.commoncoreontologies.org/ont00001954 -->

    <owl:ObjectProperty rdf:about="https://www.commoncoreontologies.org/ont00001954"/>
    


    <!-- https://www.commoncoreontologies.org/ont00001966 -->

    <owl:ObjectProperty rdf:about="https://www.commoncoreontologies.org/ont00001966"/>
    


    <!-- https://www.commoncoreontologies.org/ont00001976 -->

    <owl:ObjectProperty rdf:about="https://www.commoncoreontologies.org/ont00001976"/>
    


    <!-- https://www.commoncoreontologies.org/ont00001982 -->

    <owl:ObjectProperty rdf:about="https://www.commoncoreontologies.org/ont00001982"/>
    


    <!-- https://www.commoncoreontologies.org/ont00001984 -->

    <owl:ObjectProperty rdf:about="https://www.commoncoreontologies.org/ont00001984"/>
    


    <!-- https://www.commoncoreontologies.org/ont00001986 -->

    <owl:ObjectProperty rdf:about="https://www.commoncoreontologies.org/ont00001986"/>
    


    <!-- 
    ///////////////////////////////////////////////////////////////////////////////////////
    //
    // Classes
    //
    ///////////////////////////////////////////////////////////////////////////////////////
     -->

    


    <!-- http://purl.obolibrary.org/obo/BFO_0000015 -->

    <owl:Class rdf:about="http://purl.obolibrary.org/obo/BFO_0000015">
        <skos:definition xml:lang="en">set of interrelated or interacting Activities that transform inputs into outputs</skos:definition>
        <cco2:ont00001754>ISO/IEC/IEEE 15288:2023</cco2:ont00001754>
    </owl:Class>
    


    <!-- http://purl.obolibrary.org/obo/BFO_0000016 -->

    <owl:Class rdf:about="http://purl.obolibrary.org/obo/BFO_0000016"/>
    


    <!-- http://purl.obolibrary.org/obo/BFO_0000017 -->

    <owl:Class rdf:about="http://purl.obolibrary.org/obo/BFO_0000017"/>
    


    <!-- http://purl.obolibrary.org/obo/BFO_0000019 -->

    <owl:Class rdf:about="http://purl.obolibrary.org/obo/BFO_0000019"/>
    


    <!-- http://purl.obolibrary.org/obo/BFO_0000027 -->

    <owl:Class rdf:about="http://purl.obolibrary.org/obo/BFO_0000027"/>
    


    <!-- http://purl.obolibrary.org/obo/BFO_0000031 -->

    <owl:Class rdf:about="http://purl.obolibrary.org/obo/BFO_0000031"/>
    


    <!-- http://purl.obolibrary.org/obo/BFO_0000040 -->

    <owl:Class rdf:about="http://purl.obolibrary.org/obo/BFO_0000040"/>
    


    <!-- http://purl.obolibrary.org/obo/BFO_0000144 -->

    <owl:Class rdf:about="http://purl.obolibrary.org/obo/BFO_0000144"/>
    


    <!-- http://www.ontologyrepository.com/CommonCoreOntologies/ComputerSystem -->

    <rdf:Description rdf:about="http://www.ontologyrepository.com/CommonCoreOntologies/ComputerSystem">
        <owl:equivalentClass>
            <owl:Restriction>
                <owl:onProperty rdf:resource="http://purl.obolibrary.org/obo/BFO_0000115"/>
                <owl:someValuesFrom>
                    <owl:Class>
                        <owl:intersectionOf rdf:parseType="Collection">
                            <rdf:Description rdf:about="http://www.ontologyrepository.com/CommonCoreOntologies/ComputerComponent"/>
                            <rdf:Description rdf:about="http://www.ontologyrepository.com/CommonCoreOntologies/ComputerProgram"/>
                            <rdf:Description rdf:about="https://www.commoncoreontologies.org/ont00000420"/>
                        </owl:intersectionOf>
                    </owl:Class>
                </owl:someValuesFrom>
            </owl:Restriction>
        </owl:equivalentClass>
    </rdf:Description>
    


    <!-- http://www.ontologyrepository.com/CommonCoreOntologies/Constraint -->

    <owl:Class rdf:about="http://www.ontologyrepository.com/CommonCoreOntologies/Constraint">
        <rdfs:comment xml:lang="en">A constraint is a factor that is imposed on the solution by force or compulsion and may limit or modify the design.</rdfs:comment>
        <skos:definition xml:lang="en">externally-imposed limitation on the System, its design, or implementation or on the process used to develop or modify a System</skos:definition>
        <cco2:ont00001754 xml:lang="en">ISO/IEC/IEEE 15026-1:2019</cco2:ont00001754>
    </owl:Class>
    


    <!-- http://www.ontologyrepository.com/CommonCoreOntologies/DataTransfer -->

    <owl:Class rdf:about="http://www.ontologyrepository.com/CommonCoreOntologies/DataTransfer"/>
    


    <!-- http://www.ontologyrepository.com/CommonCoreOntologies/DigitalObject -->

    <rdf:Description rdf:about="http://www.ontologyrepository.com/CommonCoreOntologies/DigitalObject">
        <owl:equivalentClass>
            <owl:Class>
                <owl:intersectionOf rdf:parseType="Collection">
                    <rdf:Description rdf:about="https://www.commoncoreontologies.org/ont00000798"/>
                    <owl:Restriction>
                        <owl:onProperty rdf:resource="http://purl.obolibrary.org/obo/BFO_0000115"/>
                        <owl:someValuesFrom rdf:resource="https://hack.cybersystems.engineer/memex/ontologies/SeamlessDigitalEngineering#Data"/>
                    </owl:Restriction>
                </owl:intersectionOf>
            </owl:Class>
        </owl:equivalentClass>
        <rdfs:subClassOf>
            <owl:Restriction>
                <owl:onProperty rdf:resource="https://www.commoncoreontologies.org/ont00001879"/>
                <owl:someValuesFrom rdf:resource="https://hack.cybersystems.engineer/memex/ontologies/SeamlessDigitalEngineering#Object_Reference"/>
            </owl:Restriction>
        </rdfs:subClassOf>
        <rdfs:subClassOf>
            <owl:Restriction>
                <owl:onProperty rdf:resource="https://www.commoncoreontologies.org/ont00001936"/>
                <owl:someValuesFrom rdf:resource="https://hack.cybersystems.engineer/memex/ontologies/SeamlessDigitalEngineering#Act_of_Digital_Tool_Use"/>
            </owl:Restriction>
        </rdfs:subClassOf>
    </rdf:Description>
    


    <!-- http://www.ontologyrepository.com/CommonCoreOntologies/Ontology -->

    <owl:Class rdf:about="http://www.ontologyrepository.com/CommonCoreOntologies/Ontology"/>
    


    <!-- https://hack.cybersystems.engineer/memex/ontologies/SeamlessDigitalEngineering#Acceptability -->

    <owl:Class rdf:about="https://hack.cybersystems.engineer/memex/ontologies/SeamlessDigitalEngineering#Acceptability">
        <rdfs:subClassOf rdf:resource="https://hack.cybersystems.engineer/memex/ontologies/SeamlessDigitalEngineering#Product_Quality-in-Use"/>
        <rdfs:label xml:lang="en">Acceptability</rdfs:label>
        <skos:definition xml:lang="en">extent to which a human response is favourable when accepting or installing a Product, System or Service software tool designed to perform some frequently used function</skos:definition>
        <cco2:ont00001754 xml:lang="en">ISO/IEC 25019:2023(en)
Systems and software engineering — Systems and software Quality Requirements and Evaluation (SQuaRE) — Quality-in-use model</cco2:ont00001754>
    </owl:Class>
    


    <!-- https://hack.cybersystems.engineer/memex/ontologies/SeamlessDigitalEngineering#Acceptance_Report -->

    <owl:Class rdf:about="https://hack.cybersystems.engineer/memex/ontologies/SeamlessDigitalEngineering#Acceptance_Report">
        <rdfs:subClassOf rdf:resource="https://www.commoncoreontologies.org/ont00000624"/>
        <rdfs:label xml:lang="en">Acceptance Report</rdfs:label>
    </owl:Class>
    


    <!-- https://hack.cybersystems.engineer/memex/ontologies/SeamlessDigitalEngineering#Accessibility -->

    <owl:Class rdf:about="https://hack.cybersystems.engineer/memex/ontologies/SeamlessDigitalEngineering#Accessibility">
        <rdfs:subClassOf rdf:resource="https://hack.cybersystems.engineer/memex/ontologies/SeamlessDigitalEngineering#Beneficialness"/>
        <rdfs:label xml:lang="en">Accessibility</rdfs:label>
        <skos:definition xml:lang="en">extent to which Products, Systems, Services, environments and facilities can be used by people from a population with the widest range of User needs, characteristics and Capabilities to achieve identified Goals in identified Contexts of Use</skos:definition>
        <cco2:ont00001754 xml:lang="en">ISO/IEC 25019:2023(en)
Systems and software engineering — Systems and software Quality Requirements and Evaluation (SQuaRE) — Quality-in-use model</cco2:ont00001754>
    </owl:Class>
    


    <!-- https://hack.cybersystems.engineer/memex/ontologies/SeamlessDigitalEngineering#Acknowledged_SoS -->

    <owl:Class rdf:about="https://hack.cybersystems.engineer/memex/ontologies/SeamlessDigitalEngineering#Acknowledged_SoS">
        <rdfs:subClassOf rdf:resource="https://hack.cybersystems.engineer/memex/ontologies/SeamlessDigitalEngineering#System-of-Systems"/>
        <rdfs:label xml:lang="en">Acknowledged System-of-Systems</rdfs:label>
        <skos:definition xml:lang="en">The SoS has recognized objectives, a designated manager, and resources for the SoS; however, the constituent systems retain their independent ownership, objectives, funding, and development and sustainment approaches. Changes in the systems are based on cooperative agreements between the SoS and the constituent systems.</skos:definition>
        <cco2:ont00001754 xml:lang="en">ISO/IEC/IEEE 21841 - Systems and software engineering - Taxonomy of systems of systems</cco2:ont00001754>
    </owl:Class>
    


    <!-- https://hack.cybersystems.engineer/memex/ontologies/SeamlessDigitalEngineering#Acquirer -->

    <owl:Class rdf:about="https://hack.cybersystems.engineer/memex/ontologies/SeamlessDigitalEngineering#Acquirer">
        <owl:equivalentClass>
            <owl:Class>
                <owl:intersectionOf rdf:parseType="Collection">
                    <rdf:Description rdf:about="https://hack.cybersystems.engineer/memex/ontologies/SeamlessDigitalEngineering#Stakeholder"/>
                    <owl:Restriction>
                        <owl:onProperty rdf:resource="http://purl.obolibrary.org/obo/BFO_0000196"/>
                        <owl:someValuesFrom rdf:resource="https://www.commoncoreontologies.org/ont00000175"/>
                    </owl:Restriction>
                    <owl:Restriction>
                        <owl:onProperty rdf:resource="https://www.commoncoreontologies.org/ont00001787"/>
                        <owl:someValuesFrom rdf:resource="https://hack.cybersystems.engineer/memex/ontologies/SeamlessDigitalEngineering#Act_of_Acquisition"/>
                    </owl:Restriction>
                </owl:intersectionOf>
            </owl:Class>
        </owl:equivalentClass>
        <rdfs:subClassOf rdf:resource="https://hack.cybersystems.engineer/memex/ontologies/SeamlessDigitalEngineering#Stakeholder"/>
        <rdfs:comment xml:lang="en">Other terms commonly used for an acquirer are buyer, customer, owner, purchaser, or internal/organizational sponsor.</rdfs:comment>
        <rdfs:label xml:lang="en">Acquirer</rdfs:label>
        <skos:altLabel xml:lang="en">Buyer</skos:altLabel>
        <skos:altLabel xml:lang="en">Purchaser</skos:altLabel>
        <skos:definition xml:lang="en">Stakeholder that acquires or procures a System, Product or Service from a Supplier</skos:definition>
        <cco2:ont00001754>ISO/IEC/IEEE 15288:2023</cco2:ont00001754>
    </owl:Class>
    


    <!-- https://hack.cybersystems.engineer/memex/ontologies/SeamlessDigitalEngineering#Acquisition_Process -->

    <owl:Class rdf:about="https://hack.cybersystems.engineer/memex/ontologies/SeamlessDigitalEngineering#Acquisition_Process">
        <rdfs:subClassOf rdf:resource="https://hack.cybersystems.engineer/memex/ontologies/SeamlessDigitalEngineering#Agreement_Process"/>
        <rdfs:label xml:lang="en">Acquisition Process</rdfs:label>
        <skos:definition xml:lang="en">The purpose of the Acquisition Process is to obtain a Product or Service in accordance with the Acquirer&apos;s Requirements.</skos:definition>
        <cco2:ont00001754>ISO/IEC/IEEE 15288:2023</cco2:ont00001754>
    </owl:Class>
    


    <!-- https://hack.cybersystems.engineer/memex/ontologies/SeamlessDigitalEngineering#ActOfGovernance -->

    <owl:Class rdf:about="https://hack.cybersystems.engineer/memex/ontologies/SeamlessDigitalEngineering#ActOfGovernance">
        <owl:equivalentClass>
            <owl:Class>
                <owl:intersectionOf rdf:parseType="Collection">
                    <rdf:Description rdf:about="https://www.commoncoreontologies.org/ont00000133"/>
                    <owl:Restriction>
                        <owl:onProperty rdf:resource="https://www.commoncoreontologies.org/ont00001833"/>
                        <owl:someValuesFrom rdf:resource="https://hack.cybersystems.engineer/memex/ontologies/SeamlessDigitalEngineering#Stakeholder"/>
                    </owl:Restriction>
                    <owl:Restriction>
                        <owl:onProperty rdf:resource="https://www.commoncoreontologies.org/ont00001857"/>
                        <owl:someValuesFrom>
                            <owl:Class>
                                <owl:unionOf rdf:parseType="Collection">
                                    <rdf:Description rdf:about="https://hack.cybersystems.engineer/memex/ontologies/SeamlessDigitalEngineering#Lifecycle"/>
                                    <rdf:Description rdf:about="https://hack.cybersystems.engineer/memex/ontologies/SeamlessDigitalEngineering#Project"/>
                                </owl:unionOf>
                            </owl:Class>
                        </owl:someValuesFrom>
                    </owl:Restriction>
                </owl:intersectionOf>
            </owl:Class>
        </owl:equivalentClass>
        <rdfs:subClassOf rdf:resource="https://www.commoncoreontologies.org/ont00000133"/>
        <rdfs:label xml:lang="en">Act of Governance</rdfs:label>
        <skos:definition xml:lang="en">Act of Directive Communication by a human-based System comprising directing, overseeing and accountability</skos:definition>
        <cco2:ont00001754 xml:lang="en">derived from ISO/IEC 38500:2024</cco2:ont00001754>
        <cco2:ont00001760 rdf:datatype="http://www.w3.org/2001/XMLSchema#anyURI">https://semantic.incose.org/DEIX_Ontology</cco2:ont00001760>
    </owl:Class>
    


    <!-- https://hack.cybersystems.engineer/memex/ontologies/SeamlessDigitalEngineering#Act_of_Acquisition -->

    <owl:Class rdf:about="https://hack.cybersystems.engineer/memex/ontologies/SeamlessDigitalEngineering#Act_of_Acquisition">
        <owl:equivalentClass>
            <owl:Class>
                <owl:intersectionOf rdf:parseType="Collection">
                    <rdf:Description rdf:about="https://www.commoncoreontologies.org/ont00001334"/>
                    <owl:Restriction>
                        <owl:onProperty rdf:resource="https://www.commoncoreontologies.org/ont00001920"/>
                        <owl:someValuesFrom rdf:resource="https://www.commoncoreontologies.org/ont00000965"/>
                    </owl:Restriction>
                </owl:intersectionOf>
            </owl:Class>
        </owl:equivalentClass>
        <rdfs:subClassOf rdf:resource="https://www.commoncoreontologies.org/ont00001334"/>
        <rdfs:label xml:lang="en">Act of Acquisition</rdfs:label>
        <skos:definition xml:lang="en">process of obtaining a system, product, or service</skos:definition>
        <cco2:ont00001754 xml:lang="en">ISO/IEC/IEEE 15288:2023</cco2:ont00001754>
    </owl:Class>
    


    <!-- https://hack.cybersystems.engineer/memex/ontologies/SeamlessDigitalEngineering#Act_of_Agreement -->

    <owl:Class rdf:about="https://hack.cybersystems.engineer/memex/ontologies/SeamlessDigitalEngineering#Act_of_Agreement">
        <rdfs:subClassOf rdf:resource="https://www.commoncoreontologies.org/ont00000379"/>
        <rdfs:label xml:lang="en">Act of Agreement</rdfs:label>
    </owl:Class>
    


    <!-- https://hack.cybersystems.engineer/memex/ontologies/SeamlessDigitalEngineering#Act_of_Assertion -->

    <owl:Class rdf:about="https://hack.cybersystems.engineer/memex/ontologies/SeamlessDigitalEngineering#Act_of_Assertion">
        <rdfs:subClassOf rdf:resource="https://www.commoncoreontologies.org/ont00001374"/>
        <rdfs:label xml:lang="en">Act of Assertion</rdfs:label>
        <skos:definition xml:lang="en">statement made by an entity without accompanying Evidence of its validity</skos:definition>
        <cco2:ont00001754 xml:lang="en">ISO/IEC 29115:2013</cco2:ont00001754>
    </owl:Class>
    


    <!-- https://hack.cybersystems.engineer/memex/ontologies/SeamlessDigitalEngineering#Act_of_Assurance_Evaluation -->

    <owl:Class rdf:about="https://hack.cybersystems.engineer/memex/ontologies/SeamlessDigitalEngineering#Act_of_Assurance_Evaluation">
        <owl:equivalentClass>
            <owl:Class>
                <owl:intersectionOf rdf:parseType="Collection">
                    <rdf:Description rdf:about="https://hack.cybersystems.engineer/memex/ontologies/SeamlessDigitalEngineering#Act_of_Evaluation"/>
                    <owl:Restriction>
                        <owl:onProperty rdf:resource="https://www.commoncoreontologies.org/ont00001986"/>
                        <owl:someValuesFrom rdf:resource="https://hack.cybersystems.engineer/memex/ontologies/SeamlessDigitalEngineering#Assurance_Case_Report"/>
                    </owl:Restriction>
                </owl:intersectionOf>
            </owl:Class>
        </owl:equivalentClass>
        <rdfs:subClassOf rdf:resource="https://hack.cybersystems.engineer/memex/ontologies/SeamlessDigitalEngineering#Act_of_Evaluation"/>
        <rdfs:label xml:lang="en">Act of Assurance Evaluation</rdfs:label>
        <skos:definition xml:lang="en">assessment of a PP-Configuration, Protection Profile, a Security Target, or a Target of Evaluation, against defined criteria</skos:definition>
        <cco2:ont00001754 xml:lang="en">ISO/IEC 15408-1:2022</cco2:ont00001754>
    </owl:Class>
    


    <!-- https://hack.cybersystems.engineer/memex/ontologies/SeamlessDigitalEngineering#Act_of_Auditing -->

    <owl:Class rdf:about="https://hack.cybersystems.engineer/memex/ontologies/SeamlessDigitalEngineering#Act_of_Auditing">
        <owl:equivalentClass>
            <owl:Class>
                <owl:intersectionOf rdf:parseType="Collection">
                    <rdf:Description rdf:about="https://hack.cybersystems.engineer/memex/ontologies/SeamlessDigitalEngineering#Act_of_Evaluation"/>
                    <owl:Restriction>
                        <owl:onProperty rdf:resource="https://www.commoncoreontologies.org/ont00001833"/>
                        <owl:someValuesFrom rdf:resource="https://hack.cybersystems.engineer/memex/ontologies/SeamlessDigitalEngineering#Auditor"/>
                    </owl:Restriction>
                    <owl:Restriction>
                        <owl:onProperty rdf:resource="https://www.commoncoreontologies.org/ont00001986"/>
                        <owl:someValuesFrom rdf:resource="https://hack.cybersystems.engineer/memex/ontologies/SeamlessDigitalEngineering#Audit_Report"/>
                    </owl:Restriction>
                </owl:intersectionOf>
            </owl:Class>
        </owl:equivalentClass>
        <rdfs:subClassOf rdf:resource="https://hack.cybersystems.engineer/memex/ontologies/SeamlessDigitalEngineering#Act_of_Evaluation"/>
        <rdfs:label xml:lang="en">Act of Auditing</rdfs:label>
        <skos:altLabel xml:lang="en">Audit</skos:altLabel>
        <skos:definition xml:lang="en">independent examination of a work Product or set of work Products to assess compliance with specifications, standards, contractual Agreements, or other criteria</skos:definition>
        <cco2:ont00001754 xml:lang="en">ISO/IEC/IEEE 15288:2023</cco2:ont00001754>
    </owl:Class>
    


    <!-- https://hack.cybersystems.engineer/memex/ontologies/SeamlessDigitalEngineering#Act_of_Chemical_Engineering -->

    <owl:Class rdf:about="https://hack.cybersystems.engineer/memex/ontologies/SeamlessDigitalEngineering#Act_of_Chemical_Engineering">
        <rdfs:subClassOf rdf:resource="https://hack.cybersystems.engineer/memex/ontologies/SeamlessDigitalEngineering#Act_of_Domain-Specific_Engineering"/>
        <rdfs:label xml:lang="en">Act of Chemical Engineering</rdfs:label>
    </owl:Class>
    


    <!-- https://hack.cybersystems.engineer/memex/ontologies/SeamlessDigitalEngineering#Act_of_Computer-Assisted_Theorem_Proving -->

    <owl:Class rdf:about="https://hack.cybersystems.engineer/memex/ontologies/SeamlessDigitalEngineering#Act_of_Computer-Assisted_Theorem_Proving">
        <owl:equivalentClass>
            <owl:Class>
                <owl:intersectionOf rdf:parseType="Collection">
                    <rdf:Description rdf:about="https://hack.cybersystems.engineer/memex/ontologies/SeamlessDigitalEngineering#Act_of_Digital_Tool_Use"/>
                    <owl:Restriction>
                        <owl:onProperty rdf:resource="https://www.commoncoreontologies.org/ont00001778"/>
                        <owl:someValuesFrom rdf:resource="https://hack.cybersystems.engineer/memex/ontologies/SeamlessDigitalEngineering#Theorem"/>
                    </owl:Restriction>
                    <owl:Restriction>
                        <owl:onProperty rdf:resource="https://www.commoncoreontologies.org/ont00001986"/>
                        <owl:someValuesFrom rdf:resource="https://hack.cybersystems.engineer/memex/ontologies/SeamlessDigitalEngineering#Proof"/>
                    </owl:Restriction>
                </owl:intersectionOf>
            </owl:Class>
        </owl:equivalentClass>
        <rdfs:subClassOf rdf:resource="https://hack.cybersystems.engineer/memex/ontologies/SeamlessDigitalEngineering#Act_of_Digital_Tool_Use"/>
        <rdfs:label xml:lang="en">Act of Computer-Assisted Theorem Proving</rdfs:label>
    </owl:Class>
    


    <!-- https://hack.cybersystems.engineer/memex/ontologies/SeamlessDigitalEngineering#Act_of_Data_Transfer -->

    <owl:Class rdf:about="https://hack.cybersystems.engineer/memex/ontologies/SeamlessDigitalEngineering#Act_of_Data_Transfer">
        <owl:equivalentClass>
            <owl:Class>
                <owl:intersectionOf rdf:parseType="Collection">
                    <rdf:Description rdf:about="https://www.commoncoreontologies.org/ont00000402"/>
                    <owl:Restriction>
                        <owl:onProperty rdf:resource="http://purl.obolibrary.org/obo/BFO_0000055"/>
                        <owl:someValuesFrom rdf:resource="https://hack.cybersystems.engineer/memex/ontologies/SeamlessDigitalEngineering#Data_Transfer_Function"/>
                    </owl:Restriction>
                    <owl:Restriction>
                        <owl:onProperty rdf:resource="https://www.commoncoreontologies.org/ont00001921"/>
                        <owl:someValuesFrom rdf:resource="https://www.commoncoreontologies.org/ont00000958"/>
                    </owl:Restriction>
                    <owl:Restriction>
                        <owl:onProperty rdf:resource="https://www.commoncoreontologies.org/ont00001986"/>
                        <owl:someValuesFrom rdf:resource="https://www.commoncoreontologies.org/ont00000958"/>
                    </owl:Restriction>
                </owl:intersectionOf>
            </owl:Class>
        </owl:equivalentClass>
        <rdfs:subClassOf rdf:resource="https://www.commoncoreontologies.org/ont00000402"/>
        <rdfs:label xml:lang="en">Act of Data Transfer</rdfs:label>
        <cco2:ont00001760 rdf:datatype="http://www.w3.org/2001/XMLSchema#anyURI">https://semantic.incose.org/DEIX_Ontology</cco2:ont00001760>
    </owl:Class>
    


    <!-- https://hack.cybersystems.engineer/memex/ontologies/SeamlessDigitalEngineering#Act_of_Deciding -->

    <owl:Class rdf:about="https://hack.cybersystems.engineer/memex/ontologies/SeamlessDigitalEngineering#Act_of_Deciding">
        <rdfs:subClassOf rdf:resource="https://www.commoncoreontologies.org/ont00000511"/>
        <rdfs:label xml:lang="en">Act of Deciding</rdfs:label>
        <skos:definition xml:lang="en">An Act of Planning that often precedes an Act of Commissive Communication</skos:definition>
    </owl:Class>
    


    <!-- https://hack.cybersystems.engineer/memex/ontologies/SeamlessDigitalEngineering#Act_of_Digital_Engineering -->

    <owl:Class rdf:about="https://hack.cybersystems.engineer/memex/ontologies/SeamlessDigitalEngineering#Act_of_Digital_Engineering">
        <owl:equivalentClass>
            <owl:Class>
                <owl:intersectionOf rdf:parseType="Collection">
                    <rdf:Description rdf:about="https://hack.cybersystems.engineer/memex/ontologies/SeamlessDigitalEngineering#Act_of_Engineering"/>
                    <owl:Restriction>
                        <owl:onProperty rdf:resource="http://purl.obolibrary.org/obo/BFO_0000057"/>
                        <owl:someValuesFrom rdf:resource="https://hack.cybersystems.engineer/memex/ontologies/SeamlessDigitalEngineering#Digital_Artifact"/>
                    </owl:Restriction>
                    <owl:Restriction>
                        <owl:onProperty rdf:resource="https://www.commoncoreontologies.org/ont00001778"/>
                        <owl:someValuesFrom rdf:resource="https://hack.cybersystems.engineer/memex/ontologies/SeamlessDigitalEngineering#Digital_Authoritative_Source_of_Truth"/>
                    </owl:Restriction>
                </owl:intersectionOf>
            </owl:Class>
        </owl:equivalentClass>
        <rdfs:subClassOf rdf:resource="https://hack.cybersystems.engineer/memex/ontologies/SeamlessDigitalEngineering#Act_of_Engineering"/>
        <rdfs:label xml:lang="en">Act of Digital Engineering</rdfs:label>
        <cco2:ont00001760 rdf:datatype="http://www.w3.org/2001/XMLSchema#anyURI">https://semantic.incose.org/DEIX_Ontology</cco2:ont00001760>
    </owl:Class>
    


    <!-- https://hack.cybersystems.engineer/memex/ontologies/SeamlessDigitalEngineering#Act_of_Digital_Engineering_Transformation -->

    <owl:Class rdf:about="https://hack.cybersystems.engineer/memex/ontologies/SeamlessDigitalEngineering#Act_of_Digital_Engineering_Transformation">
        <owl:equivalentClass>
            <owl:Class>
                <owl:intersectionOf rdf:parseType="Collection">
                    <rdf:Description rdf:about="https://hack.cybersystems.engineer/memex/ontologies/SeamlessDigitalEngineering#Act_of_Digital_Transformation"/>
                    <owl:Restriction>
                        <owl:onProperty rdf:resource="https://www.commoncoreontologies.org/ont00001801"/>
                        <owl:someValuesFrom rdf:resource="https://hack.cybersystems.engineer/memex/ontologies/SeamlessDigitalEngineering#Digital_Engineering_Approach"/>
                    </owl:Restriction>
                    <owl:Restriction>
                        <owl:onProperty rdf:resource="https://www.commoncoreontologies.org/ont00001986"/>
                        <owl:someValuesFrom rdf:resource="https://hack.cybersystems.engineer/memex/ontologies/SeamlessDigitalEngineering#Digital_Engineering_Environment"/>
                    </owl:Restriction>
                </owl:intersectionOf>
            </owl:Class>
        </owl:equivalentClass>
        <rdfs:subClassOf rdf:resource="https://hack.cybersystems.engineer/memex/ontologies/SeamlessDigitalEngineering#Act_of_Digital_Transformation"/>
        <rdfs:label xml:lang="en">Act of Digital Engineering Transformation</rdfs:label>
    </owl:Class>
    


    <!-- https://hack.cybersystems.engineer/memex/ontologies/SeamlessDigitalEngineering#Act_of_Digital_Simulation -->

    <owl:Class rdf:about="https://hack.cybersystems.engineer/memex/ontologies/SeamlessDigitalEngineering#Act_of_Digital_Simulation">
        <owl:equivalentClass>
            <owl:Class>
                <owl:intersectionOf rdf:parseType="Collection">
                    <rdf:Description rdf:about="https://hack.cybersystems.engineer/memex/ontologies/SeamlessDigitalEngineering#Act_of_Digital_Tool_Use"/>
                    <rdf:Description rdf:about="https://hack.cybersystems.engineer/memex/ontologies/SeamlessDigitalEngineering#Act_of_Simulation"/>
                    <owl:Restriction>
                        <owl:onProperty rdf:resource="https://www.commoncoreontologies.org/ont00001921"/>
                        <owl:someValuesFrom rdf:resource="https://hack.cybersystems.engineer/memex/ontologies/SeamlessDigitalEngineering#Digital_Authoritative_Source_of_Truth"/>
                    </owl:Restriction>
                    <owl:Restriction>
                        <owl:onProperty rdf:resource="https://www.commoncoreontologies.org/ont00001986"/>
                        <owl:someValuesFrom rdf:resource="https://hack.cybersystems.engineer/memex/ontologies/SeamlessDigitalEngineering#Digital_Artifact"/>
                    </owl:Restriction>
                </owl:intersectionOf>
            </owl:Class>
        </owl:equivalentClass>
        <rdfs:subClassOf rdf:resource="https://hack.cybersystems.engineer/memex/ontologies/SeamlessDigitalEngineering#Act_of_Simulation"/>
        <rdfs:label xml:lang="en">Act of Digital Simulation</rdfs:label>
        <cco2:ont00001760 rdf:datatype="http://www.w3.org/2001/XMLSchema#anyURI">https://semantic.incose.org/DEIX_Ontology</cco2:ont00001760>
    </owl:Class>
    


    <!-- https://hack.cybersystems.engineer/memex/ontologies/SeamlessDigitalEngineering#Act_of_Digital_Tool_Use -->

    <owl:Class rdf:about="https://hack.cybersystems.engineer/memex/ontologies/SeamlessDigitalEngineering#Act_of_Digital_Tool_Use">
        <owl:equivalentClass>
            <owl:Class>
                <owl:intersectionOf rdf:parseType="Collection">
                    <rdf:Description rdf:about="https://www.commoncoreontologies.org/ont00000513"/>
                    <owl:Restriction>
                        <owl:onProperty rdf:resource="https://www.commoncoreontologies.org/ont00001949"/>
                        <owl:someValuesFrom rdf:resource="https://hack.cybersystems.engineer/memex/ontologies/SeamlessDigitalEngineering#Digital_Tool"/>
                    </owl:Restriction>
                </owl:intersectionOf>
            </owl:Class>
        </owl:equivalentClass>
        <rdfs:subClassOf rdf:resource="https://www.commoncoreontologies.org/ont00000513"/>
        <rdfs:label xml:lang="en">Act of Digital Tool Use</rdfs:label>
        <skos:definition xml:lang="en">An Act of Artifact Employment in which some Agent uses some Digital Tool.</skos:definition>
        <cco2:ont00001760 rdf:datatype="http://www.w3.org/2001/XMLSchema#anyURI">https://semantic.incose.org/DEIX_Ontology</cco2:ont00001760>
    </owl:Class>
    


    <!-- https://hack.cybersystems.engineer/memex/ontologies/SeamlessDigitalEngineering#Act_of_Digital_Transformation -->

    <owl:Class rdf:about="https://hack.cybersystems.engineer/memex/ontologies/SeamlessDigitalEngineering#Act_of_Digital_Transformation">
        <owl:equivalentClass>
            <owl:Class>
                <owl:intersectionOf rdf:parseType="Collection">
                    <rdf:Description rdf:about="https://hack.cybersystems.engineer/memex/ontologies/SeamlessDigitalEngineering#Program"/>
                    <owl:Restriction>
                        <owl:onProperty rdf:resource="http://purl.obolibrary.org/obo/BFO_0000066"/>
                        <owl:someValuesFrom rdf:resource="https://www.commoncoreontologies.org/ont00001180"/>
                    </owl:Restriction>
                    <owl:Restriction>
                        <owl:onProperty rdf:resource="https://www.commoncoreontologies.org/ont00001866"/>
                        <owl:someValuesFrom rdf:resource="https://hack.cybersystems.engineer/memex/ontologies/SeamlessDigitalEngineering#Stakeholder"/>
                    </owl:Restriction>
                    <owl:Restriction>
                        <owl:onProperty rdf:resource="https://www.commoncoreontologies.org/ont00001986"/>
                        <owl:someValuesFrom rdf:resource="https://hack.cybersystems.engineer/memex/ontologies/SeamlessDigitalEngineering#Digital_Environment"/>
                    </owl:Restriction>
                </owl:intersectionOf>
            </owl:Class>
        </owl:equivalentClass>
        <rdfs:subClassOf rdf:resource="https://hack.cybersystems.engineer/memex/ontologies/SeamlessDigitalEngineering#Program"/>
        <rdfs:comment xml:lang="en">The process of adoption and implementation of digital technology by an Organization in order to create new or modify existing Products, Services and operations by the means of translating business processes into a digital format.

Source: https://en.wikipedia.org/wiki/Digital_transformation</rdfs:comment>
        <rdfs:label xml:lang="en">Act of Digital Transformation</rdfs:label>
        <skos:definition xml:lang="en">A Planned Act of profound and radical change through Digital technologies that orients an Organization in a new direction and takes it to an entirely different level of effectiveness, which is based on analytics of Data</skos:definition>
        <cco2:ont00001753 xml:lang="en">DT</cco2:ont00001753>
        <cco2:ont00001754 xml:lang="en">ISO/IEC TS 30105-9:2023 - Information technology — IT Enabled Services-Business Process Outsourcing (ITES-BPO) lifecycle processes — Part 9: Guidelines on extending process capability assessment for digital transformation</cco2:ont00001754>
        <cco2:ont00001760 rdf:datatype="http://www.w3.org/2001/XMLSchema#anyURI">https://semantic.incose.org/DEIX_Ontology</cco2:ont00001760>
    </owl:Class>
    


    <!-- https://hack.cybersystems.engineer/memex/ontologies/SeamlessDigitalEngineering#Act_of_Domain-Specific_Engineering -->

    <owl:Class rdf:about="https://hack.cybersystems.engineer/memex/ontologies/SeamlessDigitalEngineering#Act_of_Domain-Specific_Engineering">
        <owl:equivalentClass>
            <owl:Class>
                <owl:intersectionOf rdf:parseType="Collection">
                    <rdf:Description rdf:about="https://hack.cybersystems.engineer/memex/ontologies/SeamlessDigitalEngineering#Act_of_Engineering"/>
                    <owl:Restriction>
                        <owl:onProperty rdf:resource="https://www.commoncoreontologies.org/ont00001921"/>
                        <owl:someValuesFrom rdf:resource="https://hack.cybersystems.engineer/memex/ontologies/SeamlessDigitalEngineering#Problem_Definition"/>
                    </owl:Restriction>
                    <owl:Restriction>
                        <owl:onProperty rdf:resource="https://www.commoncoreontologies.org/ont00001986"/>
                        <owl:someValuesFrom rdf:resource="https://www.commoncoreontologies.org/ont00000319"/>
                    </owl:Restriction>
                </owl:intersectionOf>
            </owl:Class>
        </owl:equivalentClass>
        <rdfs:subClassOf rdf:resource="https://hack.cybersystems.engineer/memex/ontologies/SeamlessDigitalEngineering#Act_of_Engineering"/>
        <rdfs:label xml:lang="en">Act of Domain-Specific Engineering</rdfs:label>
    </owl:Class>
    


    <!-- https://hack.cybersystems.engineer/memex/ontologies/SeamlessDigitalEngineering#Act_of_Electrical_Engineering -->

    <owl:Class rdf:about="https://hack.cybersystems.engineer/memex/ontologies/SeamlessDigitalEngineering#Act_of_Electrical_Engineering">
        <rdfs:subClassOf rdf:resource="https://hack.cybersystems.engineer/memex/ontologies/SeamlessDigitalEngineering#Act_of_Domain-Specific_Engineering"/>
        <rdfs:label xml:lang="en">Act of Electrical Engineering</rdfs:label>
    </owl:Class>
    


    <!-- https://hack.cybersystems.engineer/memex/ontologies/SeamlessDigitalEngineering#Act_of_Engineering -->

    <owl:Class rdf:about="https://hack.cybersystems.engineer/memex/ontologies/SeamlessDigitalEngineering#Act_of_Engineering">
        <owl:equivalentClass>
            <owl:Class>
                <owl:intersectionOf rdf:parseType="Collection">
                    <rdf:Description rdf:about="https://www.commoncoreontologies.org/ont00000228"/>
                    <owl:Restriction>
                        <owl:onProperty rdf:resource="http://purl.obolibrary.org/obo/BFO_0000059"/>
                        <owl:someValuesFrom rdf:resource="https://hack.cybersystems.engineer/memex/ontologies/SeamlessDigitalEngineering#Engineering_Approach"/>
                    </owl:Restriction>
                    <owl:Restriction>
                        <owl:onProperty rdf:resource="https://www.commoncoreontologies.org/ont00001857"/>
                        <owl:someValuesFrom rdf:resource="https://hack.cybersystems.engineer/memex/ontologies/SeamlessDigitalEngineering#Lifecycle"/>
                    </owl:Restriction>
                </owl:intersectionOf>
            </owl:Class>
        </owl:equivalentClass>
        <rdfs:subClassOf rdf:resource="https://www.commoncoreontologies.org/ont00000228"/>
        <rdfs:label xml:lang="en">Act of Engineering</rdfs:label>
        <cco2:ont00001760 rdf:datatype="http://www.w3.org/2001/XMLSchema#anyURI">https://semantic.incose.org/DEIX_Ontology</cco2:ont00001760>
    </owl:Class>
    


    <!-- https://hack.cybersystems.engineer/memex/ontologies/SeamlessDigitalEngineering#Act_of_Establishing_Traceability -->

    <owl:Class rdf:about="https://hack.cybersystems.engineer/memex/ontologies/SeamlessDigitalEngineering#Act_of_Establishing_Traceability">
        <owl:equivalentClass>
            <owl:Class>
                <owl:intersectionOf rdf:parseType="Collection">
                    <rdf:Description rdf:about="https://www.commoncoreontologies.org/ont00000366"/>
                    <owl:Restriction>
                        <owl:onProperty rdf:resource="https://www.commoncoreontologies.org/ont00001778"/>
                        <owl:someValuesFrom rdf:resource="https://hack.cybersystems.engineer/memex/ontologies/SeamlessDigitalEngineering#Traceability_Relationship"/>
                    </owl:Restriction>
                </owl:intersectionOf>
            </owl:Class>
        </owl:equivalentClass>
        <rdfs:subClassOf rdf:resource="https://www.commoncoreontologies.org/ont00000366"/>
        <rdfs:label xml:lang="en">Act of Establishing Traceability</rdfs:label>
        <skos:definition xml:lang="en">An Act of Information Processing that involves discerning a Traceability Relationship among two or more logical entities</skos:definition>
        <cco2:ont00001754 xml:lang="en">derived from ISO/IEC/IEEE 15288:2023, 3.52</cco2:ont00001754>
        <cco2:ont00001760 rdf:datatype="http://www.w3.org/2001/XMLSchema#anyURI">https://semantic.incose.org/DEIX_Ontology</cco2:ont00001760>
    </owl:Class>
    


    <!-- https://hack.cybersystems.engineer/memex/ontologies/SeamlessDigitalEngineering#Act_of_Evaluation -->

    <owl:Class rdf:about="https://hack.cybersystems.engineer/memex/ontologies/SeamlessDigitalEngineering#Act_of_Evaluation">
        <owl:equivalentClass>
            <owl:Class>
                <owl:intersectionOf rdf:parseType="Collection">
                    <rdf:Description rdf:about="https://www.commoncoreontologies.org/ont00000636"/>
                    <owl:Restriction>
                        <owl:onProperty rdf:resource="https://www.commoncoreontologies.org/ont00001778"/>
                        <owl:someValuesFrom rdf:resource="https://hack.cybersystems.engineer/memex/ontologies/SeamlessDigitalEngineering#Target_of_Evaluation"/>
                    </owl:Restriction>
                    <owl:Restriction>
                        <owl:onProperty rdf:resource="https://www.commoncoreontologies.org/ont00001833"/>
                        <owl:someValuesFrom rdf:resource="https://hack.cybersystems.engineer/memex/ontologies/SeamlessDigitalEngineering#Evaluator"/>
                    </owl:Restriction>
                    <owl:Restriction>
                        <owl:onProperty rdf:resource="https://www.commoncoreontologies.org/ont00001986"/>
                        <owl:someValuesFrom rdf:resource="https://hack.cybersystems.engineer/memex/ontologies/SeamlessDigitalEngineering#Evaluation_Report"/>
                    </owl:Restriction>
                </owl:intersectionOf>
            </owl:Class>
        </owl:equivalentClass>
        <rdfs:subClassOf rdf:resource="https://www.commoncoreontologies.org/ont00000636"/>
        <rdfs:label xml:lang="en">Act of Evaluation</rdfs:label>
        <skos:definition xml:lang="en">systematic determination of the extent to which an entity meets its specified criteria</skos:definition>
        <cco2:ont00001754 xml:lang="en">ISO/IEC 25001:2014</cco2:ont00001754>
    </owl:Class>
    


    <!-- https://hack.cybersystems.engineer/memex/ontologies/SeamlessDigitalEngineering#Act_of_Formal_Transformation -->

    <owl:Class rdf:about="https://hack.cybersystems.engineer/memex/ontologies/SeamlessDigitalEngineering#Act_of_Formal_Transformation">
        <owl:equivalentClass>
            <owl:Class>
                <owl:intersectionOf rdf:parseType="Collection">
                    <rdf:Description rdf:about="https://www.commoncoreontologies.org/ont00000970"/>
                    <owl:Restriction>
                        <owl:onProperty rdf:resource="http://purl.obolibrary.org/obo/BFO_0000059"/>
                        <owl:someValuesFrom rdf:resource="https://hack.cybersystems.engineer/memex/ontologies/SeamlessDigitalEngineering#Analytical_Method"/>
                    </owl:Restriction>
                </owl:intersectionOf>
            </owl:Class>
        </owl:equivalentClass>
        <rdfs:subClassOf rdf:resource="https://www.commoncoreontologies.org/ont00000970"/>
        <rdfs:comment xml:lang="en">As with defining needs, defining requirements is an activity which, through formal requirements analysis, determines specifically what the entity must do to meet the needs they are being transformed from using a formal transformation process involving decomposition, derivation, diagrams, and architectural and analytical/behavioral models. A deeper exploration and elaboration of the lifecycle concepts, including a thorough examination of interactions between the entity and other entities, are part of the transformation from needs into requirements. As a result of the requirements analysis, there may be more than one requirement defined for each need.

Source: INCOSE Needs and Requirements Manual R1.1 (2022)</rdfs:comment>
        <rdfs:label xml:lang="en">Act of Formal Transformation</rdfs:label>
    </owl:Class>
    


    <!-- https://hack.cybersystems.engineer/memex/ontologies/SeamlessDigitalEngineering#Act_of_Formal_Verification -->

    <owl:Class rdf:about="https://hack.cybersystems.engineer/memex/ontologies/SeamlessDigitalEngineering#Act_of_Formal_Verification">
        <owl:equivalentClass>
            <owl:Class>
                <owl:intersectionOf rdf:parseType="Collection">
                    <rdf:Description rdf:about="https://hack.cybersystems.engineer/memex/ontologies/SeamlessDigitalEngineering#Act_of_Computer-Assisted_Theorem_Proving"/>
                    <owl:Restriction>
                        <owl:onProperty rdf:resource="https://www.commoncoreontologies.org/ont00001778"/>
                        <owl:someValuesFrom rdf:resource="http://www.ontologyrepository.com/CommonCoreOntologies/ComputerProgram"/>
                    </owl:Restriction>
                </owl:intersectionOf>
            </owl:Class>
        </owl:equivalentClass>
        <rdfs:subClassOf rdf:resource="https://hack.cybersystems.engineer/memex/ontologies/SeamlessDigitalEngineering#Act_of_Computer-Assisted_Theorem_Proving"/>
        <rdfs:label xml:lang="en">Act of Formal Verification</rdfs:label>
        <skos:definition xml:lang="en">the act of proving or disproving the correctness of a System with respect to a certain Formal Specification or property, using formal methods of mathematics.</skos:definition>
        <cco2:ont00001754 rdf:datatype="http://www.w3.org/2001/XMLSchema#anyURI">https://en.wikipedia.org/wiki/Formal_verification</cco2:ont00001754>
    </owl:Class>
    


    <!-- https://hack.cybersystems.engineer/memex/ontologies/SeamlessDigitalEngineering#Act_of_Inspection -->

    <owl:Class rdf:about="https://hack.cybersystems.engineer/memex/ontologies/SeamlessDigitalEngineering#Act_of_Inspection">
        <owl:equivalentClass>
            <owl:Class>
                <owl:intersectionOf rdf:parseType="Collection">
                    <rdf:Description rdf:about="https://hack.cybersystems.engineer/memex/ontologies/SeamlessDigitalEngineering#Act_of_Evaluation"/>
                    <owl:Restriction>
                        <owl:onProperty rdf:resource="https://www.commoncoreontologies.org/ont00001986"/>
                        <owl:someValuesFrom rdf:resource="https://hack.cybersystems.engineer/memex/ontologies/SeamlessDigitalEngineering#Inspection_Report"/>
                    </owl:Restriction>
                </owl:intersectionOf>
            </owl:Class>
        </owl:equivalentClass>
        <rdfs:subClassOf rdf:resource="https://hack.cybersystems.engineer/memex/ontologies/SeamlessDigitalEngineering#Act_of_Evaluation"/>
        <rdfs:label xml:lang="en">Act of Inspection</rdfs:label>
        <skos:definition xml:lang="en">determination of Conformity to specified Requirements</skos:definition>
    </owl:Class>
    


    <!-- https://hack.cybersystems.engineer/memex/ontologies/SeamlessDigitalEngineering#Act_of_Logical_Inference -->

    <owl:Class rdf:about="https://hack.cybersystems.engineer/memex/ontologies/SeamlessDigitalEngineering#Act_of_Logical_Inference">
        <owl:equivalentClass>
            <owl:Class>
                <owl:intersectionOf rdf:parseType="Collection">
                    <owl:Restriction>
                        <owl:onProperty rdf:resource="https://www.commoncoreontologies.org/ont00001921"/>
                        <owl:someValuesFrom rdf:resource="https://hack.cybersystems.engineer/memex/ontologies/SeamlessDigitalEngineering#Claim"/>
                    </owl:Restriction>
                    <owl:Restriction>
                        <owl:onProperty rdf:resource="https://www.commoncoreontologies.org/ont00001986"/>
                        <owl:someValuesFrom rdf:resource="https://hack.cybersystems.engineer/memex/ontologies/SeamlessDigitalEngineering#Claim"/>
                    </owl:Restriction>
                </owl:intersectionOf>
            </owl:Class>
        </owl:equivalentClass>
        <rdfs:subClassOf rdf:resource="https://www.commoncoreontologies.org/ont00000366"/>
        <rdfs:label xml:lang="en">Act of Logical Inference</rdfs:label>
        <skos:definition xml:lang="en">reasoning step that derives a Claim from a list of Claims (premises) under a specified Context</skos:definition>
        <cco2:ont00001754 xml:lang="en">ISO/IEC/IEEE 15026-2:2022</cco2:ont00001754>
    </owl:Class>
    


    <!-- https://hack.cybersystems.engineer/memex/ontologies/SeamlessDigitalEngineering#Act_of_Material_Science_Engineering -->

    <owl:Class rdf:about="https://hack.cybersystems.engineer/memex/ontologies/SeamlessDigitalEngineering#Act_of_Material_Science_Engineering">
        <rdfs:subClassOf rdf:resource="https://hack.cybersystems.engineer/memex/ontologies/SeamlessDigitalEngineering#Act_of_Domain-Specific_Engineering"/>
        <rdfs:label xml:lang="en">Act of Material Science Engineering</rdfs:label>
    </owl:Class>
    


    <!-- https://hack.cybersystems.engineer/memex/ontologies/SeamlessDigitalEngineering#Act_of_Mathematics -->

    <owl:Class rdf:about="https://hack.cybersystems.engineer/memex/ontologies/SeamlessDigitalEngineering#Act_of_Mathematics">
        <rdfs:subClassOf rdf:resource="https://www.commoncoreontologies.org/ont00000228"/>
        <rdfs:label xml:lang="en">Act of Mathematics</rdfs:label>
    </owl:Class>
    


    <!-- https://hack.cybersystems.engineer/memex/ontologies/SeamlessDigitalEngineering#Act_of_Mechanical_Engineering -->

    <owl:Class rdf:about="https://hack.cybersystems.engineer/memex/ontologies/SeamlessDigitalEngineering#Act_of_Mechanical_Engineering">
        <rdfs:subClassOf rdf:resource="https://hack.cybersystems.engineer/memex/ontologies/SeamlessDigitalEngineering#Act_of_Domain-Specific_Engineering"/>
        <rdfs:label xml:lang="en">Act of Mechanical Engineering</rdfs:label>
    </owl:Class>
    


    <!-- https://hack.cybersystems.engineer/memex/ontologies/SeamlessDigitalEngineering#Act_of_Model_Curation -->

    <owl:Class rdf:about="https://hack.cybersystems.engineer/memex/ontologies/SeamlessDigitalEngineering#Act_of_Model_Curation">
        <owl:equivalentClass>
            <owl:Class>
                <owl:intersectionOf rdf:parseType="Collection">
                    <rdf:Description rdf:about="https://www.commoncoreontologies.org/ont00000908"/>
                    <owl:Restriction>
                        <owl:onProperty rdf:resource="https://www.commoncoreontologies.org/ont00001778"/>
                        <owl:someValuesFrom rdf:resource="https://hack.cybersystems.engineer/memex/ontologies/SeamlessDigitalEngineering#Digital_Asset"/>
                    </owl:Restriction>
                    <owl:Restriction>
                        <owl:onProperty rdf:resource="https://www.commoncoreontologies.org/ont00001857"/>
                        <owl:someValuesFrom rdf:resource="https://hack.cybersystems.engineer/memex/ontologies/SeamlessDigitalEngineering#Lifecycle"/>
                    </owl:Restriction>
                </owl:intersectionOf>
            </owl:Class>
        </owl:equivalentClass>
        <rdfs:subClassOf rdf:resource="https://www.commoncoreontologies.org/ont00000908"/>
        <rdfs:label xml:lang="en">Act of Model Curation</rdfs:label>
        <skos:definition xml:lang="en">An Act of Artifact Processing that is part of some System Lifecycle and whose intent is the curation of a Digital Asset</skos:definition>
        <cco2:ont00001760 rdf:datatype="http://www.w3.org/2001/XMLSchema#anyURI">https://semantic.incose.org/DEIX_Ontology</cco2:ont00001760>
    </owl:Class>
    


    <!-- https://hack.cybersystems.engineer/memex/ontologies/SeamlessDigitalEngineering#Act_of_Quality_Engineering -->

    <owl:Class rdf:about="https://hack.cybersystems.engineer/memex/ontologies/SeamlessDigitalEngineering#Act_of_Quality_Engineering">
        <rdfs:subClassOf rdf:resource="https://hack.cybersystems.engineer/memex/ontologies/SeamlessDigitalEngineering#Act_of_Domain-Specific_Engineering"/>
        <rdfs:label xml:lang="en">Act of Quality Engineering</rdfs:label>
    </owl:Class>
    


    <!-- https://hack.cybersystems.engineer/memex/ontologies/SeamlessDigitalEngineering#Act_of_Requirements_Analysis -->

    <owl:Class rdf:about="https://hack.cybersystems.engineer/memex/ontologies/SeamlessDigitalEngineering#Act_of_Requirements_Analysis">
        <rdfs:subClassOf rdf:resource="https://hack.cybersystems.engineer/memex/ontologies/SeamlessDigitalEngineering#Act_of_Requirements_Development"/>
    </owl:Class>
    


    <!-- https://hack.cybersystems.engineer/memex/ontologies/SeamlessDigitalEngineering#Act_of_Requirements_Change_Control -->

    <owl:Class rdf:about="https://hack.cybersystems.engineer/memex/ontologies/SeamlessDigitalEngineering#Act_of_Requirements_Change_Control">
        <rdfs:subClassOf rdf:resource="https://hack.cybersystems.engineer/memex/ontologies/SeamlessDigitalEngineering#Act_of_Requirements_Management"/>
    </owl:Class>
    


    <!-- https://hack.cybersystems.engineer/memex/ontologies/SeamlessDigitalEngineering#Act_of_Requirements_Development -->

    <owl:Class rdf:about="https://hack.cybersystems.engineer/memex/ontologies/SeamlessDigitalEngineering#Act_of_Requirements_Development">
        <rdfs:subClassOf rdf:resource="https://hack.cybersystems.engineer/memex/ontologies/SeamlessDigitalEngineering#Act_of_Requirements_Engineering"/>
        <rdfs:label xml:lang="en">Act of Requirements Development</rdfs:label>
    </owl:Class>
    


    <!-- https://hack.cybersystems.engineer/memex/ontologies/SeamlessDigitalEngineering#Act_of_Requirements_Elicitation -->

    <owl:Class rdf:about="https://hack.cybersystems.engineer/memex/ontologies/SeamlessDigitalEngineering#Act_of_Requirements_Elicitation">
        <rdfs:subClassOf rdf:resource="https://hack.cybersystems.engineer/memex/ontologies/SeamlessDigitalEngineering#Act_of_Requirements_Development"/>
    </owl:Class>
    


    <!-- https://hack.cybersystems.engineer/memex/ontologies/SeamlessDigitalEngineering#Act_of_Requirements_Engineering -->

    <owl:Class rdf:about="https://hack.cybersystems.engineer/memex/ontologies/SeamlessDigitalEngineering#Act_of_Requirements_Engineering">
        <rdfs:subClassOf rdf:resource="https://hack.cybersystems.engineer/memex/ontologies/SeamlessDigitalEngineering#Act_of_Systems_Engineering"/>
        <rdfs:label xml:lang="en">Act of Requirements Engineering</rdfs:label>
    </owl:Class>
    


    <!-- https://hack.cybersystems.engineer/memex/ontologies/SeamlessDigitalEngineering#Act_of_Requirements_Impact_Analysis -->

    <owl:Class rdf:about="https://hack.cybersystems.engineer/memex/ontologies/SeamlessDigitalEngineering#Act_of_Requirements_Impact_Analysis">
        <rdfs:subClassOf rdf:resource="https://hack.cybersystems.engineer/memex/ontologies/SeamlessDigitalEngineering#Act_of_Requirements_Management"/>
    </owl:Class>
    


    <!-- https://hack.cybersystems.engineer/memex/ontologies/SeamlessDigitalEngineering#Act_of_Requirements_Management -->

    <owl:Class rdf:about="https://hack.cybersystems.engineer/memex/ontologies/SeamlessDigitalEngineering#Act_of_Requirements_Management">
        <rdfs:subClassOf rdf:resource="https://hack.cybersystems.engineer/memex/ontologies/SeamlessDigitalEngineering#Act_of_Requirements_Engineering"/>
        <rdfs:label xml:lang="en">Act of Requirements Management</rdfs:label>
    </owl:Class>
    


    <!-- https://hack.cybersystems.engineer/memex/ontologies/SeamlessDigitalEngineering#Act_of_Requirements_Status_Tracking -->

    <owl:Class rdf:about="https://hack.cybersystems.engineer/memex/ontologies/SeamlessDigitalEngineering#Act_of_Requirements_Status_Tracking">
        <rdfs:subClassOf rdf:resource="https://hack.cybersystems.engineer/memex/ontologies/SeamlessDigitalEngineering#Act_of_Requirements_Management"/>
    </owl:Class>
    


    <!-- https://hack.cybersystems.engineer/memex/ontologies/SeamlessDigitalEngineering#Act_of_Requirements_Version_Control -->

    <owl:Class rdf:about="https://hack.cybersystems.engineer/memex/ontologies/SeamlessDigitalEngineering#Act_of_Requirements_Version_Control">
        <rdfs:subClassOf rdf:resource="https://hack.cybersystems.engineer/memex/ontologies/SeamlessDigitalEngineering#Act_of_Requirements_Management"/>
    </owl:Class>
    


    <!-- https://hack.cybersystems.engineer/memex/ontologies/SeamlessDigitalEngineering#Act_of_Risk_Treatment -->

    <owl:Class rdf:about="https://hack.cybersystems.engineer/memex/ontologies/SeamlessDigitalEngineering#Act_of_Risk_Treatment">
        <owl:equivalentClass>
            <owl:Class>
                <owl:intersectionOf rdf:parseType="Collection">
                    <rdf:Description rdf:about="http://www.ontologyrepository.com/CommonCoreOntologies/ActOfInhibiting"/>
                    <owl:Restriction>
                        <owl:onProperty rdf:resource="https://www.commoncoreontologies.org/ont00001959"/>
                        <owl:someValuesFrom rdf:resource="https://hack.cybersystems.engineer/memex/ontologies/SeamlessDigitalEngineering#Risk"/>
                    </owl:Restriction>
                </owl:intersectionOf>
            </owl:Class>
        </owl:equivalentClass>
        <rdfs:subClassOf rdf:resource="http://www.ontologyrepository.com/CommonCoreOntologies/ActOfInhibiting"/>
        <rdfs:comment xml:lang="en">Risk treatment can involve:

— avoiding the risk by deciding not to start or continue with the activity that gives rise to the risk;
— taking or increasing risk source risk in order to pursue an opportunity;
— removing thelikelihood (3.1.6);
— changing the consequences (3.1.13);
— changing the (3.1.14);
— sharing the risk with another party or parties (including contracts and risk financing); and
— retaining the risk by informed decision.</rdfs:comment>
        <rdfs:label xml:lang="en">Act of Risk Treatment</rdfs:label>
        <skos:definition xml:lang="en">Planned Act to modify Risk</skos:definition>
        <skos:example xml:lang="en">Risk treatments that deal with negative consequences are sometimes referred to as “risk mitigation”, “risk elimination”, “risk prevention” and “risk reduction”.</skos:example>
        <cco2:ont00001754 xml:lang="en">ISO/IEC 27005:2022</cco2:ont00001754>
    </owl:Class>
    


    <!-- https://hack.cybersystems.engineer/memex/ontologies/SeamlessDigitalEngineering#Act_of_Role_Assignment -->

    <owl:Class rdf:about="https://hack.cybersystems.engineer/memex/ontologies/SeamlessDigitalEngineering#Act_of_Role_Assignment">
        <owl:equivalentClass>
            <owl:Class>
                <owl:intersectionOf rdf:parseType="Collection">
                    <rdf:Description rdf:about="https://www.commoncoreontologies.org/ont00001032"/>
                    <owl:Restriction>
                        <owl:onProperty rdf:resource="https://www.commoncoreontologies.org/ont00001778"/>
                        <owl:someValuesFrom rdf:resource="http://purl.obolibrary.org/obo/BFO_0000023"/>
                    </owl:Restriction>
                    <owl:Restriction>
                        <owl:onProperty rdf:resource="https://www.commoncoreontologies.org/ont00001857"/>
                        <owl:someValuesFrom rdf:resource="https://hack.cybersystems.engineer/memex/ontologies/SeamlessDigitalEngineering#ActOfGovernance"/>
                    </owl:Restriction>
                </owl:intersectionOf>
            </owl:Class>
        </owl:equivalentClass>
        <rdfs:subClassOf rdf:resource="https://www.commoncoreontologies.org/ont00001032"/>
        <rdfs:label xml:lang="en">Act of Role Assignment</rdfs:label>
        <skos:definition xml:lang="en">Needed for Authoritative Source of Truth, because an Authority is one who assigns the Authoritative Source of Truth Role to a Digital Asset thru an Act of Role Assignment</skos:definition>
        <cco2:ont00001760 rdf:datatype="http://www.w3.org/2001/XMLSchema#anyURI">https://semantic.incose.org/DEIX_Ontology</cco2:ont00001760>
    </owl:Class>
    


    <!-- https://hack.cybersystems.engineer/memex/ontologies/SeamlessDigitalEngineering#Act_of_Science -->

    <owl:Class rdf:about="https://hack.cybersystems.engineer/memex/ontologies/SeamlessDigitalEngineering#Act_of_Science">
        <owl:equivalentClass>
            <owl:Class>
                <owl:intersectionOf rdf:parseType="Collection">
                    <rdf:Description rdf:about="https://www.commoncoreontologies.org/ont00000228"/>
                    <owl:Restriction>
                        <owl:onProperty rdf:resource="http://purl.obolibrary.org/obo/BFO_0000059"/>
                        <owl:someValuesFrom rdf:resource="https://hack.cybersystems.engineer/memex/ontologies/SeamlessDigitalEngineering#Scientific_Method"/>
                    </owl:Restriction>
                    <owl:Restriction>
                        <owl:onProperty rdf:resource="https://www.commoncoreontologies.org/ont00001777"/>
                        <owl:someValuesFrom>
                            <owl:Class>
                                <owl:intersectionOf rdf:parseType="Collection">
                                    <rdf:Description rdf:about="http://www.ontologyrepository.com/CommonCoreOntologies/ActOfExperimentation"/>
                                    <rdf:Description rdf:about="https://www.commoncoreontologies.org/ont00000037"/>
                                    <rdf:Description rdf:about="https://www.commoncoreontologies.org/ont00000366"/>
                                </owl:intersectionOf>
                            </owl:Class>
                        </owl:someValuesFrom>
                    </owl:Restriction>
                </owl:intersectionOf>
            </owl:Class>
        </owl:equivalentClass>
        <rdfs:subClassOf rdf:resource="https://www.commoncoreontologies.org/ont00000228"/>
        <rdfs:label xml:lang="en">Act of Science</rdfs:label>
    </owl:Class>
    


    <!-- https://hack.cybersystems.engineer/memex/ontologies/SeamlessDigitalEngineering#Act_of_Simulation -->

    <owl:Class rdf:about="https://hack.cybersystems.engineer/memex/ontologies/SeamlessDigitalEngineering#Act_of_Simulation">
        <owl:equivalentClass>
            <owl:Class>
                <owl:intersectionOf rdf:parseType="Collection">
                    <rdf:Description rdf:about="https://www.commoncoreontologies.org/ont00000513"/>
                    <owl:Restriction>
                        <owl:onProperty rdf:resource="https://www.commoncoreontologies.org/ont00001921"/>
                        <owl:someValuesFrom>
                            <owl:Class>
                                <owl:intersectionOf rdf:parseType="Collection">
                                    <rdf:Description rdf:about="https://www.commoncoreontologies.org/ont00000958"/>
                                    <rdf:Description rdf:about="https://www.commoncoreontologies.org/ont00001045"/>
                                </owl:intersectionOf>
                            </owl:Class>
                        </owl:someValuesFrom>
                    </owl:Restriction>
                    <owl:Restriction>
                        <owl:onProperty rdf:resource="https://www.commoncoreontologies.org/ont00001986"/>
                        <owl:someValuesFrom>
                            <owl:Class>
                                <owl:intersectionOf rdf:parseType="Collection">
                                    <rdf:Description rdf:about="https://hack.cybersystems.engineer/memex/ontologies/SeamlessDigitalEngineering#System_View"/>
                                    <rdf:Description rdf:about="https://www.commoncoreontologies.org/ont00000958"/>
                                </owl:intersectionOf>
                            </owl:Class>
                        </owl:someValuesFrom>
                    </owl:Restriction>
                </owl:intersectionOf>
            </owl:Class>
        </owl:equivalentClass>
        <rdfs:subClassOf rdf:resource="https://www.commoncoreontologies.org/ont00000513"/>
        <rdfs:label xml:lang="en">Act of Simulation</rdfs:label>
        <skos:definition xml:lang="en">The process of using a Model that behaves or operates like a given System when provided a set of controlled inputs.</skos:definition>
        <cco2:ont00001754>ISO/IEC/IEEE 24765:2010</cco2:ont00001754>
        <cco2:ont00001760 rdf:datatype="http://www.w3.org/2001/XMLSchema#anyURI">https://semantic.incose.org/DEIX_Ontology</cco2:ont00001760>
    </owl:Class>
    


    <!-- https://hack.cybersystems.engineer/memex/ontologies/SeamlessDigitalEngineering#Act_of_Software_Engineering -->

    <owl:Class rdf:about="https://hack.cybersystems.engineer/memex/ontologies/SeamlessDigitalEngineering#Act_of_Software_Engineering">
        <owl:equivalentClass>
            <owl:Class>
                <owl:intersectionOf rdf:parseType="Collection">
                    <rdf:Description rdf:about="https://hack.cybersystems.engineer/memex/ontologies/SeamlessDigitalEngineering#Act_of_Domain-Specific_Engineering"/>
                    <owl:Restriction>
                        <owl:onProperty rdf:resource="https://www.commoncoreontologies.org/ont00001778"/>
                        <owl:someValuesFrom rdf:resource="https://hack.cybersystems.engineer/memex/ontologies/SeamlessDigitalEngineering#Software_Product"/>
                    </owl:Restriction>
                </owl:intersectionOf>
            </owl:Class>
        </owl:equivalentClass>
        <rdfs:subClassOf rdf:resource="https://hack.cybersystems.engineer/memex/ontologies/SeamlessDigitalEngineering#Act_of_Domain-Specific_Engineering"/>
        <rdfs:label xml:lang="en">Act of Software Engineering</rdfs:label>
    </owl:Class>
    


    <!-- https://hack.cybersystems.engineer/memex/ontologies/SeamlessDigitalEngineering#Act_of_Stakeholder_Agreement -->

    <owl:Class rdf:about="https://hack.cybersystems.engineer/memex/ontologies/SeamlessDigitalEngineering#Act_of_Stakeholder_Agreement">
        <owl:equivalentClass>
            <owl:Class>
                <owl:intersectionOf rdf:parseType="Collection">
                    <rdf:Description rdf:about="https://hack.cybersystems.engineer/memex/ontologies/SeamlessDigitalEngineering#Act_of_Agreement"/>
                    <owl:Restriction>
                        <owl:onProperty rdf:resource="https://www.commoncoreontologies.org/ont00001833"/>
                        <owl:someValuesFrom rdf:resource="https://hack.cybersystems.engineer/memex/ontologies/SeamlessDigitalEngineering#Stakeholder"/>
                    </owl:Restriction>
                </owl:intersectionOf>
            </owl:Class>
        </owl:equivalentClass>
        <rdfs:subClassOf rdf:resource="https://hack.cybersystems.engineer/memex/ontologies/SeamlessDigitalEngineering#Act_of_Agreement"/>
        <rdfs:label xml:lang="en">Act of Stakeholder Agreement</rdfs:label>
    </owl:Class>
    


    <!-- https://hack.cybersystems.engineer/memex/ontologies/SeamlessDigitalEngineering#Act_of_Systems_Engineering -->

    <owl:Class rdf:about="https://hack.cybersystems.engineer/memex/ontologies/SeamlessDigitalEngineering#Act_of_Systems_Engineering">
        <owl:equivalentClass>
            <owl:Class>
                <owl:intersectionOf rdf:parseType="Collection">
                    <rdf:Description rdf:about="https://hack.cybersystems.engineer/memex/ontologies/SeamlessDigitalEngineering#Act_of_Engineering"/>
                    <owl:Restriction>
                        <owl:onProperty rdf:resource="http://purl.obolibrary.org/obo/BFO_0000059"/>
                        <owl:someValuesFrom rdf:resource="https://hack.cybersystems.engineer/memex/ontologies/SeamlessDigitalEngineering#Systems_Approach"/>
                    </owl:Restriction>
                </owl:intersectionOf>
            </owl:Class>
        </owl:equivalentClass>
        <rdfs:subClassOf rdf:resource="https://hack.cybersystems.engineer/memex/ontologies/SeamlessDigitalEngineering#Act_of_Engineering"/>
        <rdfs:label xml:lang="en">Act of Systems Engineering</rdfs:label>
        <skos:definition xml:lang="en">transdisciplinary and integrative approach to enable the successful realization, use, and retirement of Engineered Systems using systems principles and concepts and scientific, technological and management methods</skos:definition>
        <cco2:ont00001754>ISO/IEC/IEEE 15288:2023</cco2:ont00001754>
    </owl:Class>
    


    <!-- https://hack.cybersystems.engineer/memex/ontologies/SeamlessDigitalEngineering#Act_of_Technology_Maturity_Assessment -->

    <owl:Class rdf:about="https://hack.cybersystems.engineer/memex/ontologies/SeamlessDigitalEngineering#Act_of_Technology_Maturity_Assessment">
        <owl:equivalentClass>
            <owl:Class>
                <owl:intersectionOf rdf:parseType="Collection">
                    <rdf:Description rdf:about="https://hack.cybersystems.engineer/memex/ontologies/SeamlessDigitalEngineering#Act_of_Evaluation"/>
                    <owl:Restriction>
                        <owl:onProperty rdf:resource="https://www.commoncoreontologies.org/ont00001986"/>
                        <owl:someValuesFrom rdf:resource="https://hack.cybersystems.engineer/memex/ontologies/SeamlessDigitalEngineering#Technology_Readiness_Assessment_Report"/>
                    </owl:Restriction>
                </owl:intersectionOf>
            </owl:Class>
        </owl:equivalentClass>
        <rdfs:subClassOf rdf:resource="https://hack.cybersystems.engineer/memex/ontologies/SeamlessDigitalEngineering#Act_of_Evaluation"/>
        <rdfs:label xml:lang="en">Act of Technology Maturity Assessment</rdfs:label>
        <rdfs:seeAlso rdf:resource="https://hack.cybersystems.engineer/memex/ontologies/SeamlessDigitalEngineering#Technology_Readiness_Level"/>
        <skos:definition xml:lang="en">A process to determine a system&apos;s technological maturity based on Technology Readiness Levels (TRLs).</skos:definition>
        <cco2:ont00001754 xml:lang="en">NASA Systems Engineering Handbook (2016)</cco2:ont00001754>
    </owl:Class>
    


    <!-- https://hack.cybersystems.engineer/memex/ontologies/SeamlessDigitalEngineering#Action -->

    <owl:Class rdf:about="https://hack.cybersystems.engineer/memex/ontologies/SeamlessDigitalEngineering#Action">
        <owl:equivalentClass>
            <owl:Class>
                <owl:intersectionOf rdf:parseType="Collection">
                    <rdf:Description rdf:about="https://hack.cybersystems.engineer/memex/ontologies/SeamlessDigitalEngineering#Activity"/>
                    <owl:Restriction>
                        <owl:onProperty rdf:resource="https://www.commoncoreontologies.org/ont00001833"/>
                        <owl:someValuesFrom rdf:resource="https://hack.cybersystems.engineer/memex/ontologies/SeamlessDigitalEngineering#Stakeholder"/>
                    </owl:Restriction>
                    <owl:Restriction>
                        <owl:onProperty rdf:resource="https://www.commoncoreontologies.org/ont00001986"/>
                        <owl:someValuesFrom rdf:resource="https://www.commoncoreontologies.org/ont00000624"/>
                    </owl:Restriction>
                </owl:intersectionOf>
            </owl:Class>
        </owl:equivalentClass>
        <rdfs:subClassOf rdf:resource="https://hack.cybersystems.engineer/memex/ontologies/SeamlessDigitalEngineering#Activity"/>
        <rdfs:label xml:lang="en">Action</rdfs:label>
        <skos:definition xml:lang="en">documented Activity of a Stakeholder</skos:definition>
        <cco2:ont00001754 xml:lang="en">derived from ISO/IEC 15408-1:2022, 3.1</cco2:ont00001754>
    </owl:Class>
    


    <!-- https://hack.cybersystems.engineer/memex/ontologies/SeamlessDigitalEngineering#Activity -->

    <owl:Class rdf:about="https://hack.cybersystems.engineer/memex/ontologies/SeamlessDigitalEngineering#Activity">
        <owl:equivalentClass>
            <owl:Restriction>
                <owl:onProperty rdf:resource="https://www.commoncoreontologies.org/ont00001777"/>
                <owl:someValuesFrom rdf:resource="https://hack.cybersystems.engineer/memex/ontologies/SeamlessDigitalEngineering#Task"/>
            </owl:Restriction>
        </owl:equivalentClass>
        <rdfs:subClassOf rdf:resource="https://www.commoncoreontologies.org/ont00000228"/>
        <skos:definition xml:lang="en">set of cohesive Tasks of a Process</skos:definition>
        <cco2:ont00001754>ISO/IEC/IEEE 15288:2023</cco2:ont00001754>
        <cco2:ont00001760 rdf:datatype="http://www.w3.org/2001/XMLSchema#anyURI">https://semantic.incose.org/DEIX_Ontology</cco2:ont00001760>
    </owl:Class>
    


    <!-- https://hack.cybersystems.engineer/memex/ontologies/SeamlessDigitalEngineering#Adverse_Consequence -->

    <owl:Class rdf:about="https://hack.cybersystems.engineer/memex/ontologies/SeamlessDigitalEngineering#Adverse_Consequence">
        <owl:equivalentClass>
            <owl:Class>
                <owl:intersectionOf rdf:parseType="Collection">
                    <rdf:Description rdf:about="https://hack.cybersystems.engineer/memex/ontologies/SeamlessDigitalEngineering#Consequence"/>
                    <owl:Restriction>
                        <owl:onProperty rdf:resource="https://www.commoncoreontologies.org/ont00001803"/>
                        <owl:someValuesFrom rdf:resource="https://www.commoncoreontologies.org/ont00000876"/>
                    </owl:Restriction>
                </owl:intersectionOf>
            </owl:Class>
        </owl:equivalentClass>
        <rdfs:subClassOf rdf:resource="https://hack.cybersystems.engineer/memex/ontologies/SeamlessDigitalEngineering#Consequence"/>
        <rdfs:comment xml:lang="en">An Adverse Consequence results from the System-of-Interest being in a Dangerous Condition combined with the System Environment being in its worst case state.</rdfs:comment>
        <rdfs:comment xml:lang="en">Harm in ISO Guide 51 is an instance of Adverse Consequence. The concept of Adverse Consequences is introduced in order to cover not only harms in the safety context but also loss of assets in the security context and any other losses.</rdfs:comment>
        <rdfs:label xml:lang="en">Adverse Consequence</rdfs:label>
        <skos:definition xml:lang="en">Consequence that results in a specified level of Loss</skos:definition>
        <cco2:ont00001754 xml:lang="en">ISO/IEC/IEEE 15026-1:2019</cco2:ont00001754>
    </owl:Class>
    


    <!-- https://hack.cybersystems.engineer/memex/ontologies/SeamlessDigitalEngineering#Agreement_Process -->

    <owl:Class rdf:about="https://hack.cybersystems.engineer/memex/ontologies/SeamlessDigitalEngineering#Agreement_Process">
        <rdfs:subClassOf rdf:resource="https://hack.cybersystems.engineer/memex/ontologies/SeamlessDigitalEngineering#System_Lifecycle_Process"/>
        <rdfs:label xml:lang="en">Agreement Process</rdfs:label>
        <skos:definition xml:lang="en">These processes define the activities necessary to establish an agreement between two organizations. If the acquisition process is invoked, it provides the means for interacting with a supplier. This may include products that are supplied for use as an operational system, services in support of operational activities, or elements of a system being provided by a supplier. If the supply process is invoked, it provides the means for an agreement for a product or service that is provided to the acquirer.</skos:definition>
        <cco2:ont00001754>ISO/IEC/IEEE 15288:2023</cco2:ont00001754>
    </owl:Class>
    


    <!-- https://hack.cybersystems.engineer/memex/ontologies/SeamlessDigitalEngineering#Analytical_Method -->

    <owl:Class rdf:about="https://hack.cybersystems.engineer/memex/ontologies/SeamlessDigitalEngineering#Analytical_Method">
        <owl:equivalentClass>
            <owl:Class>
                <owl:intersectionOf rdf:parseType="Collection">
                    <rdf:Description rdf:about="https://hack.cybersystems.engineer/memex/ontologies/SeamlessDigitalEngineering#Method"/>
                    <owl:Restriction>
                        <owl:onProperty rdf:resource="https://www.commoncoreontologies.org/ont00001942"/>
                        <owl:someValuesFrom rdf:resource="https://www.commoncoreontologies.org/ont00000366"/>
                    </owl:Restriction>
                </owl:intersectionOf>
            </owl:Class>
        </owl:equivalentClass>
        <rdfs:subClassOf rdf:resource="https://hack.cybersystems.engineer/memex/ontologies/SeamlessDigitalEngineering#Method"/>
        <rdfs:label xml:lang="en">Analytical Method</rdfs:label>
    </owl:Class>
    


    <!-- https://hack.cybersystems.engineer/memex/ontologies/SeamlessDigitalEngineering#Appliance -->

    <owl:Class rdf:about="https://hack.cybersystems.engineer/memex/ontologies/SeamlessDigitalEngineering#Appliance">
        <owl:equivalentClass>
            <owl:Class>
                <owl:intersectionOf rdf:parseType="Collection">
                    <rdf:Description rdf:about="https://hack.cybersystems.engineer/memex/ontologies/SeamlessDigitalEngineering#Product"/>
                    <owl:Restriction>
                        <owl:onProperty rdf:resource="https://www.commoncoreontologies.org/ont00001925"/>
                        <owl:someValuesFrom rdf:resource="https://hack.cybersystems.engineer/memex/ontologies/SeamlessDigitalEngineering#Customer"/>
                    </owl:Restriction>
                </owl:intersectionOf>
            </owl:Class>
        </owl:equivalentClass>
        <rdfs:subClassOf rdf:resource="https://hack.cybersystems.engineer/memex/ontologies/SeamlessDigitalEngineering#Product"/>
        <rdfs:label xml:lang="en">Appliance</rdfs:label>
        <skos:definition xml:lang="en">Product as seen by the Customer</skos:definition>
        <cco2:ont00001754 xml:lang="en">ISO/IEC 23004-5:2008</cco2:ont00001754>
    </owl:Class>
    


    <!-- https://hack.cybersystems.engineer/memex/ontologies/SeamlessDigitalEngineering#Approach -->

    <owl:Class rdf:about="https://hack.cybersystems.engineer/memex/ontologies/SeamlessDigitalEngineering#Approach">
        <owl:equivalentClass>
            <owl:Class>
                <owl:intersectionOf rdf:parseType="Collection">
                    <rdf:Description rdf:about="https://www.commoncoreontologies.org/ont00000965"/>
                    <owl:Restriction>
                        <owl:onProperty rdf:resource="https://www.commoncoreontologies.org/ont00001942"/>
                        <owl:someValuesFrom rdf:resource="https://www.commoncoreontologies.org/ont00000228"/>
                    </owl:Restriction>
                </owl:intersectionOf>
            </owl:Class>
        </owl:equivalentClass>
        <rdfs:subClassOf rdf:resource="https://www.commoncoreontologies.org/ont00000965"/>
        <rdfs:label xml:lang="en">Approach</rdfs:label>
        <skos:definition xml:lang="en">The prescribed method used in dealing with or accomplishing.</skos:definition>
        <cco2:ont00001754 xml:lang="en">derived from The American Heritage® Dictionary of the English Language, 5th Edition</cco2:ont00001754>
        <cco2:ont00001760 rdf:datatype="http://www.w3.org/2001/XMLSchema#anyURI">https://semantic.incose.org/DEIX_Ontology</cco2:ont00001760>
    </owl:Class>
    


    <!-- https://hack.cybersystems.engineer/memex/ontologies/SeamlessDigitalEngineering#Approval_Authority_Role -->

    <owl:Class rdf:about="https://hack.cybersystems.engineer/memex/ontologies/SeamlessDigitalEngineering#Approval_Authority_Role">
        <rdfs:subClassOf rdf:resource="https://www.commoncoreontologies.org/ont00000187"/>
        <rdfs:label xml:lang="en">Approval Authority Role</rdfs:label>
        <skos:definition xml:lang="en">Authority Role that inheres in a Person (or Group of Persons) and/or Organization (or Organizations) responsible for approving Activities, Material Artifacts and other aspects of the System during its Lifecycle</skos:definition>
        <cco2:ont00001754 xml:lang="en">ISO/IEC/IEEE 15026-1:2019</cco2:ont00001754>
    </owl:Class>
    


    <!-- https://hack.cybersystems.engineer/memex/ontologies/SeamlessDigitalEngineering#Architecture -->

    <owl:Class rdf:about="https://hack.cybersystems.engineer/memex/ontologies/SeamlessDigitalEngineering#Architecture">
        <owl:equivalentClass>
            <owl:Class>
                <owl:intersectionOf rdf:parseType="Collection">
                    <rdf:Description rdf:about="https://www.commoncoreontologies.org/ont00000319"/>
                    <owl:Restriction>
                        <owl:onProperty rdf:resource="https://www.commoncoreontologies.org/ont00001942"/>
                        <owl:someValuesFrom rdf:resource="https://hack.cybersystems.engineer/memex/ontologies/SeamlessDigitalEngineering#Lifecycle"/>
                    </owl:Restriction>
                </owl:intersectionOf>
            </owl:Class>
        </owl:equivalentClass>
        <rdfs:subClassOf rdf:resource="https://www.commoncoreontologies.org/ont00000319"/>
        <rdfs:label xml:lang="en">Architecture</rdfs:label>
        <skos:definition xml:lang="en">The fundamental concepts or properties of an entity in its environment and governing principles for the realization and evolution of this entity and its related life cycle processes</skos:definition>
        <cco2:ont00001754 xml:lang="en">ISO/IEC/IEEE 42010:2022</cco2:ont00001754>
    </owl:Class>
    


    <!-- https://hack.cybersystems.engineer/memex/ontologies/SeamlessDigitalEngineering#Architecture_Description -->

    <owl:Class rdf:about="https://hack.cybersystems.engineer/memex/ontologies/SeamlessDigitalEngineering#Architecture_Description">
        <owl:equivalentClass>
            <owl:Class>
                <owl:intersectionOf rdf:parseType="Collection">
                    <rdf:Description rdf:about="https://www.commoncoreontologies.org/ont00000798"/>
                    <owl:Restriction>
                        <owl:onProperty rdf:resource="http://purl.obolibrary.org/obo/BFO_0000101"/>
                        <owl:someValuesFrom rdf:resource="https://hack.cybersystems.engineer/memex/ontologies/SeamlessDigitalEngineering#Architecture_View"/>
                    </owl:Restriction>
                </owl:intersectionOf>
            </owl:Class>
        </owl:equivalentClass>
        <rdfs:subClassOf rdf:resource="https://www.commoncoreontologies.org/ont00000798"/>
        <rdfs:comment xml:lang="en">An AD is a tangible representation of Information provided to the Stakeholders.</rdfs:comment>
        <rdfs:comment xml:lang="en">An AD is considered an Information Part.</rdfs:comment>
        <rdfs:label xml:lang="en">Architecture Description</rdfs:label>
        <skos:altLabel xml:lang="en">AD</skos:altLabel>
        <skos:definition xml:lang="en">work product used to express an Architecture</skos:definition>
        <cco2:ont00001754 xml:lang="en">ISO/IEC/IEEE 42010:2022</cco2:ont00001754>
    </owl:Class>
    


    <!-- https://hack.cybersystems.engineer/memex/ontologies/SeamlessDigitalEngineering#Architecture_Description_Element -->

    <owl:Class rdf:about="https://hack.cybersystems.engineer/memex/ontologies/SeamlessDigitalEngineering#Architecture_Description_Element">
        <owl:equivalentClass>
            <owl:Restriction>
                <owl:onProperty rdf:resource="http://purl.obolibrary.org/obo/BFO_0000129"/>
                <owl:someValuesFrom rdf:resource="https://hack.cybersystems.engineer/memex/ontologies/SeamlessDigitalEngineering#Architecture_Description"/>
            </owl:Restriction>
        </owl:equivalentClass>
        <rdfs:subClassOf rdf:resource="https://hack.cybersystems.engineer/memex/ontologies/SeamlessDigitalEngineering#Architecture_Description"/>
        <rdfs:label xml:lang="en">Architecture Description Element</rdfs:label>
        <skos:definition xml:lang="en">identified or named part of an Architecture Description</skos:definition>
        <skos:example xml:lang="en">AD elements include Stakeholders, Concerns, stakeholder perspectives and aspects identified in an AD, architecture description language, architecture description framework and correspondences and correspondence methods used in an AD, and Architecture Views, View Components, Architecture Viewpoints, and Models included in an AD.</skos:example>
        <cco2:ont00001754 xml:lang="en">ISO/IEC/IEEE 42010:2022</cco2:ont00001754>
    </owl:Class>
    


    <!-- https://hack.cybersystems.engineer/memex/ontologies/SeamlessDigitalEngineering#Architecture_Description_Framework -->

    <owl:Class rdf:about="https://hack.cybersystems.engineer/memex/ontologies/SeamlessDigitalEngineering#Architecture_Description_Framework">
        <owl:equivalentClass>
            <owl:Class>
                <owl:intersectionOf rdf:parseType="Collection">
                    <owl:Restriction>
                        <owl:onProperty rdf:resource="http://purl.obolibrary.org/obo/BFO_0000178"/>
                        <owl:someValuesFrom>
                            <owl:Class>
                                <owl:intersectionOf rdf:parseType="Collection">
                                    <rdf:Description rdf:about="https://hack.cybersystems.engineer/memex/ontologies/SeamlessDigitalEngineering#Method"/>
                                    <rdf:Description rdf:about="https://hack.cybersystems.engineer/memex/ontologies/SeamlessDigitalEngineering#Principle"/>
                                </owl:intersectionOf>
                            </owl:Class>
                        </owl:someValuesFrom>
                    </owl:Restriction>
                    <owl:Restriction>
                        <owl:onProperty rdf:resource="https://www.commoncoreontologies.org/ont00001942"/>
                        <owl:someValuesFrom rdf:resource="https://hack.cybersystems.engineer/memex/ontologies/SeamlessDigitalEngineering#Architecture_Description"/>
                    </owl:Restriction>
                </owl:intersectionOf>
            </owl:Class>
        </owl:equivalentClass>
        <rdfs:subClassOf rdf:resource="https://www.commoncoreontologies.org/ont00000965"/>
        <rdfs:comment xml:lang="en">Architecture description frameworks promote structured organization, consistency of description, greater potential for reuse, and completeness of Architecture Views and Models.</rdfs:comment>
        <rdfs:label xml:lang="en">Architecture Description Framework</rdfs:label>
        <skos:definition xml:lang="en">conventions, principles and practices for the description of Architectures established within a specific domain of application or community of Stakeholders</skos:definition>
        <skos:example xml:lang="en">Generalized Enterprise-Referencing Architectures Modelling Framework (GERAM) (ISO 15704:2019, Annex B), Reference Model of Open Distributed Processing (RM-ODP), Unified Architecture Framework (UAF), and NATO Architecture Framework (NAF).</skos:example>
        <cco2:ont00001754 xml:lang="en">ISO/IEC/IEEE 42010:2022</cco2:ont00001754>
    </owl:Class>
    


    <!-- https://hack.cybersystems.engineer/memex/ontologies/SeamlessDigitalEngineering#Architecture_Description_Language -->

    <owl:Class rdf:about="https://hack.cybersystems.engineer/memex/ontologies/SeamlessDigitalEngineering#Architecture_Description_Language">
        <owl:equivalentClass>
            <owl:Class>
                <owl:intersectionOf rdf:parseType="Collection">
                    <rdf:Description rdf:about="http://www.ontologyrepository.com/CommonCoreOntologies/ComputerLanguage"/>
                    <owl:Restriction>
                        <owl:onProperty rdf:resource="https://www.commoncoreontologies.org/ont00001899"/>
                        <owl:someValuesFrom rdf:resource="https://hack.cybersystems.engineer/memex/ontologies/SeamlessDigitalEngineering#Architecture_Description_Element"/>
                    </owl:Restriction>
                </owl:intersectionOf>
            </owl:Class>
        </owl:equivalentClass>
        <rdfs:subClassOf rdf:resource="http://www.ontologyrepository.com/CommonCoreOntologies/ComputerLanguage"/>
        <rdfs:label xml:lang="en">Architecture Description Language</rdfs:label>
        <skos:definition xml:lang="en">means of expression, with syntax and semantics, consisting of a set of representations, conventions, and associated rules intended to be used to describe an architecture</skos:definition>
        <skos:example xml:lang="en">Architecture Analysis and Design Language (AADL), ArchiMate, UML, SysML, UAF Profile</skos:example>
        <cco2:ont00001754 xml:lang="en">ISO/IEC/IEEE 42010:2022</cco2:ont00001754>
    </owl:Class>
    


    <!-- https://hack.cybersystems.engineer/memex/ontologies/SeamlessDigitalEngineering#Architecture_View -->

    <owl:Class rdf:about="https://hack.cybersystems.engineer/memex/ontologies/SeamlessDigitalEngineering#Architecture_View">
        <owl:equivalentClass>
            <owl:Class>
                <owl:intersectionOf rdf:parseType="Collection">
                    <rdf:Description rdf:about="https://hack.cybersystems.engineer/memex/ontologies/SeamlessDigitalEngineering#View"/>
                    <owl:Restriction>
                        <owl:onProperty rdf:resource="https://www.commoncoreontologies.org/ont00001938"/>
                        <owl:someValuesFrom rdf:resource="https://hack.cybersystems.engineer/memex/ontologies/SeamlessDigitalEngineering#Architecture"/>
                    </owl:Restriction>
                </owl:intersectionOf>
            </owl:Class>
        </owl:equivalentClass>
        <rdfs:subClassOf rdf:resource="https://hack.cybersystems.engineer/memex/ontologies/SeamlessDigitalEngineering#View"/>
        <rdfs:comment xml:lang="en">An Information or Data View addresses information-relevant concerns framed by an Information viewpoint. It contains as view components, a conceptual data model, a data management model and a data access model and correspondences linking those components together.</rdfs:comment>
        <rdfs:label xml:lang="en">Architecture View</rdfs:label>
        <skos:definition xml:lang="en">information part (Representational ICE) comprising portion of an Architecture Description</skos:definition>
        <cco2:ont00001754 xml:lang="en">ISO/IEC/IEEE 42010:2022</cco2:ont00001754>
    </owl:Class>
    


    <!-- https://hack.cybersystems.engineer/memex/ontologies/SeamlessDigitalEngineering#Architecture_Viewpoint -->

    <owl:Class rdf:about="https://hack.cybersystems.engineer/memex/ontologies/SeamlessDigitalEngineering#Architecture_Viewpoint">
        <owl:equivalentClass>
            <owl:Class>
                <owl:intersectionOf rdf:parseType="Collection">
                    <rdf:Description rdf:about="https://hack.cybersystems.engineer/memex/ontologies/SeamlessDigitalEngineering#Viewpoint"/>
                    <owl:Restriction>
                        <owl:onProperty rdf:resource="https://www.commoncoreontologies.org/ont00001942"/>
                        <owl:someValuesFrom rdf:resource="https://hack.cybersystems.engineer/memex/ontologies/SeamlessDigitalEngineering#Architecture_View"/>
                    </owl:Restriction>
                </owl:intersectionOf>
            </owl:Class>
        </owl:equivalentClass>
        <rdfs:subClassOf rdf:resource="https://hack.cybersystems.engineer/memex/ontologies/SeamlessDigitalEngineering#Viewpoint"/>
        <rdfs:comment xml:lang="en">A viewpoint is a frame of reference for the Concerns determined by the architect as relevant to the purpose of the Architecture Description.</rdfs:comment>
        <rdfs:comment xml:lang="en">The conventions of an Architecture Viewpoint are documented in a specification of that viewpoint.</rdfs:comment>
        <rdfs:label xml:lang="en">Architecture Viewpoint</rdfs:label>
        <skos:definition xml:lang="en">A set of conventions for the creation, interpretation and use of an Architecture View to frame one or more Concerns</skos:definition>
        <cco2:ont00001754 xml:lang="en">ISO/IEC/IEEE 42010:2022</cco2:ont00001754>
    </owl:Class>
    


    <!-- https://hack.cybersystems.engineer/memex/ontologies/SeamlessDigitalEngineering#Argument -->

    <owl:Class rdf:about="https://hack.cybersystems.engineer/memex/ontologies/SeamlessDigitalEngineering#Argument">
        <rdfs:subClassOf rdf:resource="https://www.commoncoreontologies.org/ont00000965"/>
        <rdfs:comment xml:lang="en">An Argument corresponds to a Participant of an Eventuality described by the Predicate Argument Structure.</rdfs:comment>
        <rdfs:comment xml:lang="en">Arguments typically satisfy certain argument positions and can be described as being syntactico-semantic notions, whereas Participants are semantico-conceptual. The standard view is that subsets of the Participants associated with an Eventuality are selected as arguments by the verb (or nominal or adjective) expressing the Eventuality. Other Participants are either incorporated or realized as Eventuality Modifiers.</rdfs:comment>
        <rdfs:comment xml:lang="en">Natural language predicates typically have one, two, or three arguments, although they can have more.</rdfs:comment>
        <rdfs:label xml:lang="en">Argument</rdfs:label>
        <skos:definition xml:lang="en">formal semantic unit that is an essential element of a Predicate Argument Structure and can have variable instantiations depending on the utterance</skos:definition>
        <cco2:ont00001754 xml:lang="en">ISO 24617-4:2014, 2.1.1
Language resource management - Semantic annotation framework (SemAF) - Part 4: Semantic roles (SemAF-SR)</cco2:ont00001754>
    </owl:Class>
    


    <!-- https://hack.cybersystems.engineer/memex/ontologies/SeamlessDigitalEngineering#Asset -->

    <owl:Class rdf:about="https://hack.cybersystems.engineer/memex/ontologies/SeamlessDigitalEngineering#Asset">
        <owl:equivalentClass>
            <owl:Class>
                <owl:intersectionOf rdf:parseType="Collection">
                    <rdf:Description rdf:about="https://www.commoncoreontologies.org/ont00000740"/>
                    <owl:Restriction>
                        <owl:onProperty rdf:resource="https://www.commoncoreontologies.org/ont00001936"/>
                        <owl:someValuesFrom rdf:resource="https://www.commoncoreontologies.org/ont00000636"/>
                    </owl:Restriction>
                </owl:intersectionOf>
            </owl:Class>
        </owl:equivalentClass>
        <rdfs:subClassOf rdf:resource="https://www.commoncoreontologies.org/ont00000740"/>
        <rdfs:label xml:lang="en">Asset</rdfs:label>
        <skos:definition xml:lang="en">entity that the owner of the Target of Evaluation presumably places value on</skos:definition>
        <cco2:ont00001754 xml:lang="en">ISO/IEC 15408-1:2022
Information security, cybersecurity and privacy protection
Evaluation critera for IT security
Part 1: Introduction and general model</cco2:ont00001754>
        <cco2:ont00001760 rdf:datatype="http://www.w3.org/2001/XMLSchema#anyURI">https://semantic.incose.org/DEIX_Ontology</cco2:ont00001760>
    </owl:Class>
    


    <!-- https://hack.cybersystems.engineer/memex/ontologies/SeamlessDigitalEngineering#Assumption -->

    <owl:Class rdf:about="https://hack.cybersystems.engineer/memex/ontologies/SeamlessDigitalEngineering#Assumption">
        <owl:equivalentClass>
            <owl:Class>
                <owl:intersectionOf rdf:parseType="Collection">
                    <rdf:Description rdf:about="https://hack.cybersystems.engineer/memex/ontologies/SeamlessDigitalEngineering#Confidence"/>
                    <owl:Restriction>
                        <owl:onProperty rdf:resource="http://www.ontologyrepository.com/CommonCoreOntologies/is_causal_factor_in"/>
                        <owl:someValuesFrom rdf:resource="https://www.commoncoreontologies.org/ont00000511"/>
                    </owl:Restriction>
                </owl:intersectionOf>
            </owl:Class>
        </owl:equivalentClass>
        <rdfs:subClassOf rdf:resource="https://hack.cybersystems.engineer/memex/ontologies/SeamlessDigitalEngineering#Confidence"/>
        <rdfs:label xml:lang="en">Assumption</rdfs:label>
        <skos:definition xml:lang="en">a factor in the planning process that is considered to be true, real, or certain, without proof or demonstration</skos:definition>
        <cco2:ont00001754 xml:lang="en">ISO/IEC/IEEE 24765:2017, 3.276</cco2:ont00001754>
    </owl:Class>
    


    <!-- https://hack.cybersystems.engineer/memex/ontologies/SeamlessDigitalEngineering#Assumption_Field -->

    <owl:Class rdf:about="https://hack.cybersystems.engineer/memex/ontologies/SeamlessDigitalEngineering#Assumption_Field">
        <owl:equivalentClass>
            <owl:Class>
                <owl:intersectionOf rdf:parseType="Collection">
                    <rdf:Description rdf:about="https://www.commoncoreontologies.org/ont00001243"/>
                    <owl:Restriction>
                        <owl:onProperty rdf:resource="http://purl.obolibrary.org/obo/BFO_0000101"/>
                        <owl:someValuesFrom rdf:resource="https://hack.cybersystems.engineer/memex/ontologies/SeamlessDigitalEngineering#Basic_Assumption"/>
                    </owl:Restriction>
                </owl:intersectionOf>
            </owl:Class>
        </owl:equivalentClass>
        <rdfs:subClassOf rdf:resource="https://www.commoncoreontologies.org/ont00001243"/>
        <rdfs:label xml:lang="en">Assumption Field</rdfs:label>
    </owl:Class>
    


    <!-- https://hack.cybersystems.engineer/memex/ontologies/SeamlessDigitalEngineering#Assurance -->

    <owl:Class rdf:about="https://hack.cybersystems.engineer/memex/ontologies/SeamlessDigitalEngineering#Assurance">
        <owl:equivalentClass>
            <owl:Class>
                <owl:intersectionOf rdf:parseType="Collection">
                    <owl:Restriction>
                        <owl:onProperty rdf:resource="http://purl.obolibrary.org/obo/BFO_0000195"/>
                        <owl:someValuesFrom rdf:resource="https://hack.cybersystems.engineer/memex/ontologies/SeamlessDigitalEngineering#Confidence"/>
                    </owl:Restriction>
                    <owl:Restriction>
                        <owl:onProperty rdf:resource="http://purl.obolibrary.org/obo/BFO_0000195"/>
                        <owl:someValuesFrom rdf:resource="https://hack.cybersystems.engineer/memex/ontologies/SeamlessDigitalEngineering#Target_of_Evaluation"/>
                    </owl:Restriction>
                    <owl:Restriction>
                        <owl:onProperty rdf:resource="https://www.commoncoreontologies.org/ont00001801"/>
                        <owl:someValuesFrom rdf:resource="https://hack.cybersystems.engineer/memex/ontologies/SeamlessDigitalEngineering#Claim"/>
                    </owl:Restriction>
                </owl:intersectionOf>
            </owl:Class>
        </owl:equivalentClass>
        <rdfs:subClassOf rdf:resource="https://www.commoncoreontologies.org/ont00000314"/>
        <rdfs:label xml:lang="en">Assurance</rdfs:label>
        <skos:definition xml:lang="en">grounds for justified Confidence that a Claim has been or will be achieved</skos:definition>
        <cco2:ont00001754 xml:lang="en">ISO/IEC/IEEE 15026-1:2019</cco2:ont00001754>
    </owl:Class>
    


    <!-- https://hack.cybersystems.engineer/memex/ontologies/SeamlessDigitalEngineering#Assurance_Argument -->

    <owl:Class rdf:about="https://hack.cybersystems.engineer/memex/ontologies/SeamlessDigitalEngineering#Assurance_Argument">
        <owl:equivalentClass>
            <owl:Class>
                <owl:intersectionOf rdf:parseType="Collection">
                    <rdf:Description rdf:about="https://hack.cybersystems.engineer/memex/ontologies/SeamlessDigitalEngineering#Argument"/>
                    <owl:Restriction>
                        <owl:onProperty rdf:resource="https://www.commoncoreontologies.org/ont00001808"/>
                        <owl:someValuesFrom rdf:resource="https://hack.cybersystems.engineer/memex/ontologies/SeamlessDigitalEngineering#Assurance_Claim"/>
                    </owl:Restriction>
                </owl:intersectionOf>
            </owl:Class>
        </owl:equivalentClass>
        <rdfs:subClassOf rdf:resource="https://hack.cybersystems.engineer/memex/ontologies/SeamlessDigitalEngineering#Argument"/>
        <rdfs:label xml:lang="en">Assurance Argument</rdfs:label>
        <skos:definition xml:lang="en">An Argument specifically about some Assurance Claim</skos:definition>
        <cco2:ont00001754 xml:lang="en">derived from ISO/IEC/IEEE 15026-1:2019</cco2:ont00001754>
    </owl:Class>
    


    <!-- https://hack.cybersystems.engineer/memex/ontologies/SeamlessDigitalEngineering#Assurance_Argument_Record -->

    <owl:Class rdf:about="https://hack.cybersystems.engineer/memex/ontologies/SeamlessDigitalEngineering#Assurance_Argument_Record">
        <owl:equivalentClass>
            <owl:Class>
                <owl:intersectionOf rdf:parseType="Collection">
                    <rdf:Description rdf:about="https://hack.cybersystems.engineer/memex/ontologies/SeamlessDigitalEngineering#Record"/>
                    <owl:Restriction>
                        <owl:onProperty rdf:resource="http://purl.obolibrary.org/obo/BFO_0000101"/>
                        <owl:someValuesFrom rdf:resource="https://hack.cybersystems.engineer/memex/ontologies/SeamlessDigitalEngineering#Argument"/>
                    </owl:Restriction>
                </owl:intersectionOf>
            </owl:Class>
        </owl:equivalentClass>
        <rdfs:subClassOf rdf:resource="https://hack.cybersystems.engineer/memex/ontologies/SeamlessDigitalEngineering#Record"/>
        <rdfs:comment xml:lang="en">To be convincing, the Assurance Argument needs to address the Uncertainties in a balanced manner and assert that the Arguments establish the Claims only to the specified levels of validity and Confidence.</rdfs:comment>
        <rdfs:label xml:lang="en">Assurance Argument Record</rdfs:label>
        <skos:definition xml:lang="en">Report that links tangible Evidence and Assumptions to provide a convincing and valid Argument of a Claim under a given Assurance Context</skos:definition>
        <cco2:ont00001754 xml:lang="en">ISO/IEC/IEEE 15026-4:2021</cco2:ont00001754>
    </owl:Class>
    


    <!-- https://hack.cybersystems.engineer/memex/ontologies/SeamlessDigitalEngineering#Assurance_Case_Report -->

    <owl:Class rdf:about="https://hack.cybersystems.engineer/memex/ontologies/SeamlessDigitalEngineering#Assurance_Case_Report">
        <owl:equivalentClass>
            <owl:Class>
                <owl:intersectionOf rdf:parseType="Collection">
                    <rdf:Description rdf:about="https://www.commoncoreontologies.org/ont00000624"/>
                    <owl:Restriction>
                        <owl:onProperty rdf:resource="http://purl.obolibrary.org/obo/BFO_0000115"/>
                        <owl:someValuesFrom rdf:resource="https://hack.cybersystems.engineer/memex/ontologies/SeamlessDigitalEngineering#Assurance_Claim_Record"/>
                    </owl:Restriction>
                    <owl:Restriction>
                        <owl:onProperty rdf:resource="http://purl.obolibrary.org/obo/BFO_0000115"/>
                        <owl:someValuesFrom rdf:resource="https://hack.cybersystems.engineer/memex/ontologies/SeamlessDigitalEngineering#Evidence_Report"/>
                    </owl:Restriction>
                    <owl:Restriction>
                        <owl:onProperty rdf:resource="http://purl.obolibrary.org/obo/BFO_0000115"/>
                        <owl:someValuesFrom rdf:resource="https://hack.cybersystems.engineer/memex/ontologies/SeamlessDigitalEngineering#Narrative_Introduction_Report"/>
                    </owl:Restriction>
                </owl:intersectionOf>
            </owl:Class>
        </owl:equivalentClass>
        <rdfs:subClassOf rdf:resource="https://www.commoncoreontologies.org/ont00000624"/>
        <rdfs:comment xml:lang="en">An Assurance Case Report compiles the following Information Bearing Artifacts:

1) Assurance Claim Record
2) Evidence Report
c) Narrative Introduction Report whose Assurance Goal Field corresponds to the top-level Claim.</rdfs:comment>
        <rdfs:comment xml:lang="en">An Assurance Case is incomplete if its Main Field contains an Undeveloped Argument.</rdfs:comment>
        <rdfs:label xml:lang="en">Assurance Case Report</rdfs:label>
        <skos:definition xml:lang="en">reasoned, auditable Information Bearing Artifact created that supports the contention that its top-level Claim (or set of Claims) is satisfied, including systematic argumentation (Arguments) and its underlying Evidence and explicit Assumptions that support the Claim(s)</skos:definition>
        <skos:editorialNote xml:lang="en">A valid Assurance Case Report has *exactly 1* of each member part:

```
Report
 and (&apos;has member part&apos; exactly 1 &apos;Assurance Claim Record&apos;)
 and (&apos;has member part&apos; exactly 1 &apos;Evidence Report&apos;)
 and (&apos;has member part&apos; exactly 1 &apos;Narrative Introduction Report&apos;)
```</skos:editorialNote>
        <cco2:ont00001754 xml:lang="en">ISO/IEC/IEEE 15026-1:2019</cco2:ont00001754>
    </owl:Class>
    


    <!-- https://hack.cybersystems.engineer/memex/ontologies/SeamlessDigitalEngineering#Assurance_Claim -->

    <owl:Class rdf:about="https://hack.cybersystems.engineer/memex/ontologies/SeamlessDigitalEngineering#Assurance_Claim">
        <owl:equivalentClass>
            <owl:Class>
                <owl:intersectionOf rdf:parseType="Collection">
                    <rdf:Description rdf:about="https://hack.cybersystems.engineer/memex/ontologies/SeamlessDigitalEngineering#Claim"/>
                    <owl:Restriction>
                        <owl:onProperty rdf:resource="https://www.commoncoreontologies.org/ont00001942"/>
                        <owl:someValuesFrom rdf:resource="https://hack.cybersystems.engineer/memex/ontologies/SeamlessDigitalEngineering#Assurance"/>
                    </owl:Restriction>
                </owl:intersectionOf>
            </owl:Class>
        </owl:equivalentClass>
        <rdfs:subClassOf rdf:resource="https://hack.cybersystems.engineer/memex/ontologies/SeamlessDigitalEngineering#Claim"/>
        <rdfs:label xml:lang="en">Assurance Claim</rdfs:label>
        <skos:definition xml:lang="en">A structured Claim about some Assurance Information Quality Entity</skos:definition>
        <cco2:ont00001754 xml:lang="en">derived from ISO/IEC/IEEE 15026-1:2019</cco2:ont00001754>
    </owl:Class>
    


    <!-- https://hack.cybersystems.engineer/memex/ontologies/SeamlessDigitalEngineering#Assurance_Claim_Record -->

    <owl:Class rdf:about="https://hack.cybersystems.engineer/memex/ontologies/SeamlessDigitalEngineering#Assurance_Claim_Record">
        <owl:equivalentClass>
            <owl:Class>
                <owl:intersectionOf rdf:parseType="Collection">
                    <rdf:Description rdf:about="https://hack.cybersystems.engineer/memex/ontologies/SeamlessDigitalEngineering#Record"/>
                    <owl:Restriction>
                        <owl:onProperty rdf:resource="http://purl.obolibrary.org/obo/BFO_0000101"/>
                        <owl:someValuesFrom rdf:resource="https://hack.cybersystems.engineer/memex/ontologies/SeamlessDigitalEngineering#Assurance_Claim"/>
                    </owl:Restriction>
                    <owl:Restriction>
                        <owl:onProperty rdf:resource="http://purl.obolibrary.org/obo/BFO_0000115"/>
                        <owl:someValuesFrom rdf:resource="https://hack.cybersystems.engineer/memex/ontologies/SeamlessDigitalEngineering#Assurance_Argument_Record"/>
                    </owl:Restriction>
                    <owl:Restriction>
                        <owl:onProperty rdf:resource="http://purl.obolibrary.org/obo/BFO_0000115"/>
                        <owl:someValuesFrom rdf:resource="https://hack.cybersystems.engineer/memex/ontologies/SeamlessDigitalEngineering#Assurance_Context_List"/>
                    </owl:Restriction>
                </owl:intersectionOf>
            </owl:Class>
        </owl:equivalentClass>
        <rdfs:subClassOf rdf:resource="https://hack.cybersystems.engineer/memex/ontologies/SeamlessDigitalEngineering#Record"/>
        <rdfs:label xml:lang="en">Assurance Claim Record</rdfs:label>
        <skos:definition xml:lang="en">A Record about a Claim consisting of 3 Fields:

a) a Claim, C,
b) an Argument, A, that supports C, and
c) a possibly empty list of Assurance Contexts</skos:definition>
        <cco2:ont00001754 xml:lang="en">ISO/IEC/15026-2:2022</cco2:ont00001754>
    </owl:Class>
    


    <!-- https://hack.cybersystems.engineer/memex/ontologies/SeamlessDigitalEngineering#Assurance_Context_List -->

    <owl:Class rdf:about="https://hack.cybersystems.engineer/memex/ontologies/SeamlessDigitalEngineering#Assurance_Context_List">
        <owl:equivalentClass>
            <owl:Class>
                <owl:intersectionOf rdf:parseType="Collection">
                    <rdf:Description rdf:about="https://www.commoncoreontologies.org/ont00000799"/>
                    <owl:Restriction>
                        <owl:onProperty rdf:resource="http://purl.obolibrary.org/obo/BFO_0000115"/>
                        <owl:someValuesFrom rdf:resource="https://hack.cybersystems.engineer/memex/ontologies/SeamlessDigitalEngineering#Assumption_Field"/>
                    </owl:Restriction>
                    <owl:Restriction>
                        <owl:onProperty rdf:resource="http://purl.obolibrary.org/obo/BFO_0000115"/>
                        <owl:someValuesFrom rdf:resource="https://www.commoncoreontologies.org/ont00001298"/>
                    </owl:Restriction>
                    <owl:Restriction>
                        <owl:onProperty rdf:resource="http://purl.obolibrary.org/obo/BFO_0000115"/>
                        <owl:someValuesFrom>
                            <owl:Class>
                                <owl:unionOf rdf:parseType="Collection">
                                    <rdf:Description rdf:about="https://hack.cybersystems.engineer/memex/ontologies/SeamlessDigitalEngineering#Ontology_Class"/>
                                    <rdf:Description rdf:about="https://hack.cybersystems.engineer/memex/ontologies/SeamlessDigitalEngineering#Ontology_Individual"/>
                                </owl:unionOf>
                            </owl:Class>
                        </owl:someValuesFrom>
                    </owl:Restriction>
                </owl:intersectionOf>
            </owl:Class>
        </owl:equivalentClass>
        <rdfs:subClassOf rdf:resource="https://www.commoncoreontologies.org/ont00000799"/>
        <rdfs:comment xml:lang="en">Element a) should be defined in an Ontology.</rdfs:comment>
        <rdfs:label xml:lang="en">Assurance Context List</rdfs:label>
        <skos:definition xml:lang="en">A List whose elements are:

a) the definition of a term or identifier;
b) a Basic Assumption on the terms defined in the Assurance Case; or
c) a reference to a Document concerning the System-of-Interest</skos:definition>
        <cco2:ont00001754 xml:lang="en">ISO/IEC/IEEE 15026-2:2022</cco2:ont00001754>
    </owl:Class>
    


    <!-- https://hack.cybersystems.engineer/memex/ontologies/SeamlessDigitalEngineering#Assurance_Goal -->

    <owl:Class rdf:about="https://hack.cybersystems.engineer/memex/ontologies/SeamlessDigitalEngineering#Assurance_Goal">
        <owl:equivalentClass>
            <owl:Class>
                <owl:intersectionOf rdf:parseType="Collection">
                    <rdf:Description rdf:about="https://hack.cybersystems.engineer/memex/ontologies/SeamlessDigitalEngineering#Goal"/>
                    <owl:Restriction>
                        <owl:onProperty rdf:resource="https://www.commoncoreontologies.org/ont00001942"/>
                        <owl:someValuesFrom rdf:resource="https://hack.cybersystems.engineer/memex/ontologies/SeamlessDigitalEngineering#Assurance"/>
                    </owl:Restriction>
                </owl:intersectionOf>
            </owl:Class>
        </owl:equivalentClass>
        <rdfs:subClassOf rdf:resource="https://hack.cybersystems.engineer/memex/ontologies/SeamlessDigitalEngineering#Goal"/>
        <rdfs:label xml:lang="en">Assurance Goal</rdfs:label>
        <skos:definition xml:lang="en">A Goal that prescribes some Assurance Information Quality Entity</skos:definition>
        <cco2:ont00001754 xml:lang="en">derived from ISO/IEC/IEEE 15026-1:2019</cco2:ont00001754>
    </owl:Class>
    


    <!-- https://hack.cybersystems.engineer/memex/ontologies/SeamlessDigitalEngineering#Assurance_Goal_Field -->

    <owl:Class rdf:about="https://hack.cybersystems.engineer/memex/ontologies/SeamlessDigitalEngineering#Assurance_Goal_Field">
        <owl:equivalentClass>
            <owl:Class>
                <owl:intersectionOf rdf:parseType="Collection">
                    <rdf:Description rdf:about="https://www.commoncoreontologies.org/ont00001243"/>
                    <owl:Restriction>
                        <owl:onProperty rdf:resource="http://purl.obolibrary.org/obo/BFO_0000101"/>
                        <owl:someValuesFrom rdf:resource="https://hack.cybersystems.engineer/memex/ontologies/SeamlessDigitalEngineering#Assurance_Goal"/>
                    </owl:Restriction>
                </owl:intersectionOf>
            </owl:Class>
        </owl:equivalentClass>
        <rdfs:subClassOf rdf:resource="https://www.commoncoreontologies.org/ont00001243"/>
        <rdfs:label xml:lang="en">Assurance Goal Field</rdfs:label>
    </owl:Class>
    


    <!-- https://hack.cybersystems.engineer/memex/ontologies/SeamlessDigitalEngineering#Assurance_Package -->

    <owl:Class rdf:about="https://hack.cybersystems.engineer/memex/ontologies/SeamlessDigitalEngineering#Assurance_Package">
        <owl:equivalentClass>
            <owl:Class>
                <owl:intersectionOf rdf:parseType="Collection">
                    <rdf:Description rdf:about="https://hack.cybersystems.engineer/memex/ontologies/SeamlessDigitalEngineering#Requirement_Set"/>
                    <owl:Restriction>
                        <owl:onProperty rdf:resource="http://purl.obolibrary.org/obo/BFO_0000178"/>
                        <owl:someValuesFrom rdf:resource="https://hack.cybersystems.engineer/memex/ontologies/SeamlessDigitalEngineering#Security_Assurance_Requirement"/>
                    </owl:Restriction>
                </owl:intersectionOf>
            </owl:Class>
        </owl:equivalentClass>
        <rdfs:subClassOf rdf:resource="https://hack.cybersystems.engineer/memex/ontologies/SeamlessDigitalEngineering#Requirement_Set"/>
        <rdfs:label xml:lang="en">Assurance Package</rdfs:label>
        <skos:definition xml:lang="en">named set of Security Assurance Requirements</skos:definition>
        <cco2:ont00001754 xml:lang="en">ISO/IEC 15408-1:2022</cco2:ont00001754>
    </owl:Class>
    


    <!-- https://hack.cybersystems.engineer/memex/ontologies/SeamlessDigitalEngineering#Assurance_Requirement -->

    <owl:Class rdf:about="https://hack.cybersystems.engineer/memex/ontologies/SeamlessDigitalEngineering#Assurance_Requirement">
        <owl:equivalentClass>
            <owl:Class>
                <owl:intersectionOf rdf:parseType="Collection">
                    <rdf:Description rdf:about="https://hack.cybersystems.engineer/memex/ontologies/SeamlessDigitalEngineering#Requirement"/>
                    <owl:Restriction>
                        <owl:onProperty rdf:resource="https://www.commoncoreontologies.org/ont00001942"/>
                        <owl:someValuesFrom rdf:resource="https://hack.cybersystems.engineer/memex/ontologies/SeamlessDigitalEngineering#Assurance"/>
                    </owl:Restriction>
                    <owl:Restriction>
                        <owl:onProperty rdf:resource="https://www.commoncoreontologies.org/ont00001942"/>
                        <owl:someValuesFrom rdf:resource="https://hack.cybersystems.engineer/memex/ontologies/SeamlessDigitalEngineering#Condition"/>
                    </owl:Restriction>
                    <owl:Restriction>
                        <owl:onProperty rdf:resource="https://www.commoncoreontologies.org/ont00001942"/>
                        <owl:someValuesFrom rdf:resource="https://hack.cybersystems.engineer/memex/ontologies/SeamlessDigitalEngineering#Supply_Process"/>
                    </owl:Restriction>
                    <owl:Restriction>
                        <owl:onProperty rdf:resource="https://www.commoncoreontologies.org/ont00001942"/>
                        <owl:someValuesFrom rdf:resource="https://hack.cybersystems.engineer/memex/ontologies/SeamlessDigitalEngineering#Target_of_Evaluation"/>
                    </owl:Restriction>
                    <owl:Restriction>
                        <owl:onProperty rdf:resource="https://www.commoncoreontologies.org/ont00001942"/>
                        <owl:someValuesFrom rdf:resource="https://hack.cybersystems.engineer/memex/ontologies/SeamlessDigitalEngineering#Technical_Process"/>
                    </owl:Restriction>
                </owl:intersectionOf>
            </owl:Class>
        </owl:equivalentClass>
        <rdfs:subClassOf rdf:resource="https://hack.cybersystems.engineer/memex/ontologies/SeamlessDigitalEngineering#Requirement"/>
        <rdfs:label xml:lang="en">Assurance Requirement</rdfs:label>
        <cco2:ont00001754 xml:lang="en">Requirement that prescribes the Conditions, Supply Process, and Technical Processes of the Target of Evaluation, and the Actions required of Evaluators with respect to Evidence produced from these Conditions and System Lifecycle Processes</cco2:ont00001754>
        <cco2:ont00001754 xml:lang="en">derived from ISO/IEC 15408-1:2022</cco2:ont00001754>
    </owl:Class>
    


    <!-- https://hack.cybersystems.engineer/memex/ontologies/SeamlessDigitalEngineering#Attack_Potential -->

    <owl:Class rdf:about="https://hack.cybersystems.engineer/memex/ontologies/SeamlessDigitalEngineering#Attack_Potential">
        <owl:equivalentClass>
            <owl:Class>
                <owl:intersectionOf rdf:parseType="Collection">
                    <rdf:Description rdf:about="https://www.commoncoreontologies.org/ont00001176"/>
                    <owl:Restriction>
                        <owl:onProperty rdf:resource="https://www.commoncoreontologies.org/ont00001966"/>
                        <owl:someValuesFrom rdf:resource="https://hack.cybersystems.engineer/memex/ontologies/SeamlessDigitalEngineering#Attack_Surface"/>
                    </owl:Restriction>
                </owl:intersectionOf>
            </owl:Class>
        </owl:equivalentClass>
        <rdfs:subClassOf rdf:resource="https://www.commoncoreontologies.org/ont00001176"/>
        <rdfs:label xml:lang="en">Attack Potential</rdfs:label>
        <skos:definition xml:lang="en">measure of the effort needed to exploit a Vulnerability in a Target of Evaluation</skos:definition>
        <skos:example xml:lang="en">The effort is expressed as a function of properties related to the attacker (e.g. expertise, resources, and motivation) and properties related to the vulnerability itself (e.g. window of opportunity, time to exposure).</skos:example>
        <cco2:ont00001754 xml:lang="en">ISO/IEC 15408-1:2022</cco2:ont00001754>
    </owl:Class>
    


    <!-- https://hack.cybersystems.engineer/memex/ontologies/SeamlessDigitalEngineering#Attack_Surface -->

    <owl:Class rdf:about="https://hack.cybersystems.engineer/memex/ontologies/SeamlessDigitalEngineering#Attack_Surface">
        <owl:equivalentClass>
            <owl:Class>
                <owl:intersectionOf rdf:parseType="Collection">
                    <owl:Restriction>
                        <owl:onProperty rdf:resource="http://purl.obolibrary.org/obo/BFO_0000115"/>
                        <owl:someValuesFrom rdf:resource="https://hack.cybersystems.engineer/memex/ontologies/SeamlessDigitalEngineering#Interface"/>
                    </owl:Restriction>
                    <owl:Restriction>
                        <owl:onProperty rdf:resource="http://purl.obolibrary.org/obo/BFO_0000129"/>
                        <owl:someValuesFrom rdf:resource="https://www.commoncoreontologies.org/ont00000544"/>
                    </owl:Restriction>
                    <owl:Restriction>
                        <owl:onProperty rdf:resource="https://www.commoncoreontologies.org/ont00001956"/>
                        <owl:someValuesFrom rdf:resource="https://www.commoncoreontologies.org/ont00000548"/>
                    </owl:Restriction>
                </owl:intersectionOf>
            </owl:Class>
        </owl:equivalentClass>
        <rdfs:subClassOf rdf:resource="http://purl.obolibrary.org/obo/BFO_0000027"/>
        <rdfs:label xml:lang="en">Attack Surface</rdfs:label>
        <skos:definition xml:lang="en">set of logical or physical Interfaces to a Target, consisting of points through which access to the Target and its functions may be attempted</skos:definition>
        <cco2:ont00001754 xml:lang="en">ISO/IEC 15408-1:2022</cco2:ont00001754>
    </owl:Class>
    


    <!-- https://hack.cybersystems.engineer/memex/ontologies/SeamlessDigitalEngineering#Attribute -->

    <owl:Class rdf:about="https://hack.cybersystems.engineer/memex/ontologies/SeamlessDigitalEngineering#Attribute">
        <owl:equivalentClass>
            <owl:Class>
                <owl:intersectionOf rdf:parseType="Collection">
                    <rdf:Description rdf:about="https://www.commoncoreontologies.org/ont00000314"/>
                    <owl:Restriction>
                        <owl:onProperty rdf:resource="http://purl.obolibrary.org/obo/BFO_0000059"/>
                        <owl:someValuesFrom rdf:resource="https://www.commoncoreontologies.org/ont00000958"/>
                    </owl:Restriction>
                </owl:intersectionOf>
            </owl:Class>
        </owl:equivalentClass>
        <rdfs:subClassOf rdf:resource="https://www.commoncoreontologies.org/ont00000314"/>
        <skos:altLabel xml:lang="en">Property</skos:altLabel>
        <skos:definition xml:lang="en">inherent property or characteristic of an entity that can be distinguished quantitatively or qualitatively by human or automated means</skos:definition>
        <cco2:ont00001754 xml:lang="en">ISO/IEC 25002:2024 Systems and software engineering - Systems and software Quality Requirements and Evaluation (SQuaRE) - Quality model overview and usage</cco2:ont00001754>
    </owl:Class>
    


    <!-- https://hack.cybersystems.engineer/memex/ontologies/SeamlessDigitalEngineering#Audit_Report -->

    <owl:Class rdf:about="https://hack.cybersystems.engineer/memex/ontologies/SeamlessDigitalEngineering#Audit_Report">
        <rdfs:subClassOf rdf:resource="https://hack.cybersystems.engineer/memex/ontologies/SeamlessDigitalEngineering#Evaluation_Report"/>
        <rdfs:label xml:lang="en">Audit Report</rdfs:label>
    </owl:Class>
    


    <!-- https://hack.cybersystems.engineer/memex/ontologies/SeamlessDigitalEngineering#Auditor -->

    <owl:Class rdf:about="https://hack.cybersystems.engineer/memex/ontologies/SeamlessDigitalEngineering#Auditor">
        <owl:equivalentClass>
            <owl:Class>
                <owl:intersectionOf rdf:parseType="Collection">
                    <rdf:Description rdf:about="https://hack.cybersystems.engineer/memex/ontologies/SeamlessDigitalEngineering#Stakeholder"/>
                    <owl:Restriction>
                        <owl:onProperty rdf:resource="https://www.commoncoreontologies.org/ont00001787"/>
                        <owl:someValuesFrom rdf:resource="https://hack.cybersystems.engineer/memex/ontologies/SeamlessDigitalEngineering#Act_of_Auditing"/>
                    </owl:Restriction>
                </owl:intersectionOf>
            </owl:Class>
        </owl:equivalentClass>
        <rdfs:subClassOf rdf:resource="https://hack.cybersystems.engineer/memex/ontologies/SeamlessDigitalEngineering#Evaluator"/>
        <rdfs:label xml:lang="en">Auditor</rdfs:label>
        <skos:definition xml:lang="en">Person who conducts an Act of Audit</skos:definition>
        <cco2:ont00001754 xml:lang="en">ISO/IEC 29110-1-2:2024
Systems and software engineering
Lifecycle profiles for Very Small Entities (VSEs)
Part 1-2: Vocabulary</cco2:ont00001754>
    </owl:Class>
    


    <!-- https://hack.cybersystems.engineer/memex/ontologies/SeamlessDigitalEngineering#Authoritative_Knowledge -->

    <owl:Class rdf:about="https://hack.cybersystems.engineer/memex/ontologies/SeamlessDigitalEngineering#Authoritative_Knowledge">
        <owl:equivalentClass>
            <owl:Class>
                <owl:intersectionOf rdf:parseType="Collection">
                    <rdf:Description rdf:about="https://hack.cybersystems.engineer/memex/ontologies/SeamlessDigitalEngineering#Knowledge"/>
                    <owl:Restriction>
                        <owl:onProperty rdf:resource="http://purl.obolibrary.org/obo/BFO_0000178"/>
                        <owl:someValuesFrom rdf:resource="https://www.commoncoreontologies.org/ont00000592"/>
                    </owl:Restriction>
                </owl:intersectionOf>
            </owl:Class>
        </owl:equivalentClass>
        <rdfs:subClassOf rdf:resource="https://hack.cybersystems.engineer/memex/ontologies/SeamlessDigitalEngineering#Knowledge"/>
        <rdfs:comment xml:lang="en">CONJECTURE Ω(Α) = &lt;φ|θ|α(Α)&gt;
            - Ω : Authoritative Knowledge
            - A : &apos;as-is&apos; subject, in context of an application
            - φ : Utility of Representation (i.e., Model Elegance)
            - θ : Parameters of Curation
            - α-hat : Representation &apos;is output of&apos; Act of Model Curation
            - α-hat(A) : Representation (α-hat) in an ASoT of an &apos;as-is&apos; subject (A)

Source: Clarence &quot;Moe&quot; Moreland, (2024) &quot;ASOT Definition/Certification Process&quot;, Presentation, INCOSE Digital Engineering Information eXchange (DEIX) Ontology Working Group.</rdfs:comment>
        <rdfs:label xml:lang="en">Authoritative Knowledge</rdfs:label>
        <cco2:ont00001760 rdf:datatype="http://www.w3.org/2001/XMLSchema#anyURI">https://semantic.incose.org/DEIX_Ontology</cco2:ont00001760>
    </owl:Class>
    


    <!-- https://hack.cybersystems.engineer/memex/ontologies/SeamlessDigitalEngineering#Authoritative_Source_of_Truth_Role -->

    <owl:Class rdf:about="https://hack.cybersystems.engineer/memex/ontologies/SeamlessDigitalEngineering#Authoritative_Source_of_Truth_Role">
        <owl:equivalentClass>
            <owl:Class>
                <owl:intersectionOf rdf:parseType="Collection">
                    <rdf:Description rdf:about="https://hack.cybersystems.engineer/memex/ontologies/SeamlessDigitalEngineering#Source_of_Truth_Role"/>
                    <owl:Restriction>
                        <owl:onProperty rdf:resource="http://purl.obolibrary.org/obo/BFO_0000054"/>
                        <owl:someValuesFrom rdf:resource="https://hack.cybersystems.engineer/memex/ontologies/SeamlessDigitalEngineering#Act_of_Role_Assignment"/>
                    </owl:Restriction>
                </owl:intersectionOf>
            </owl:Class>
        </owl:equivalentClass>
        <rdfs:subClassOf rdf:resource="https://hack.cybersystems.engineer/memex/ontologies/SeamlessDigitalEngineering#Source_of_Truth_Role"/>
        <rdfs:label xml:lang="en">Authoritative Source of Truth Role</rdfs:label>
        <skos:altLabel xml:lang="en">ASoT Role</skos:altLabel>
        <skos:definition xml:lang="en">A Source of Truth Role that has been assigned thru an Act of Role Assignment by a relevant Authority</skos:definition>
        <cco2:ont00001760 rdf:datatype="http://www.w3.org/2001/XMLSchema#anyURI">https://semantic.incose.org/DEIX_Ontology</cco2:ont00001760>
    </owl:Class>
    


    <!-- https://hack.cybersystems.engineer/memex/ontologies/SeamlessDigitalEngineering#Authority -->

    <owl:Class rdf:about="https://hack.cybersystems.engineer/memex/ontologies/SeamlessDigitalEngineering#Authority">
        <owl:equivalentClass>
            <owl:Class>
                <owl:intersectionOf rdf:parseType="Collection">
                    <rdf:Description rdf:about="https://hack.cybersystems.engineer/memex/ontologies/SeamlessDigitalEngineering#Stakeholder"/>
                    <owl:Restriction>
                        <owl:onProperty rdf:resource="http://purl.obolibrary.org/obo/BFO_0000196"/>
                        <owl:someValuesFrom rdf:resource="https://www.commoncoreontologies.org/ont00000187"/>
                    </owl:Restriction>
                    <owl:Restriction>
                        <owl:onProperty rdf:resource="https://www.commoncoreontologies.org/ont00001787"/>
                        <owl:someValuesFrom>
                            <owl:Class>
                                <owl:unionOf rdf:parseType="Collection">
                                    <rdf:Description rdf:about="https://www.commoncoreontologies.org/ont00000133"/>
                                    <rdf:Description rdf:about="https://www.commoncoreontologies.org/ont00001374"/>
                                </owl:unionOf>
                            </owl:Class>
                        </owl:someValuesFrom>
                    </owl:Restriction>
                </owl:intersectionOf>
            </owl:Class>
        </owl:equivalentClass>
        <rdfs:subClassOf rdf:resource="https://hack.cybersystems.engineer/memex/ontologies/SeamlessDigitalEngineering#Stakeholder"/>
        <rdfs:comment xml:lang="en">An Agent such as a Person, governing body, or System that applies expert judgment and rules to proclaim a Digital Artifact is valid and originates from a sanctioned source.

Derived from source: https://www.dau.edu/glossary/asot</rdfs:comment>
        <rdfs:label xml:lang="en">Authority</rdfs:label>
        <skos:definition xml:lang="en">A Stakeholder who has the right to apply project resources, expend funds, make decisions, or give approvals</skos:definition>
        <cco2:ont00001754>ISO/IEC/IEEE 24765:2017, 3.305</cco2:ont00001754>
        <cco2:ont00001760 rdf:datatype="http://www.w3.org/2001/XMLSchema#anyURI">https://semantic.incose.org/DEIX_Ontology</cco2:ont00001760>
    </owl:Class>
    


    <!-- https://hack.cybersystems.engineer/memex/ontologies/SeamlessDigitalEngineering#Automated_Theorem_Prover -->

    <owl:Class rdf:about="https://hack.cybersystems.engineer/memex/ontologies/SeamlessDigitalEngineering#Automated_Theorem_Prover">
        <rdfs:subClassOf rdf:resource="https://hack.cybersystems.engineer/memex/ontologies/SeamlessDigitalEngineering#Theorem_Prover"/>
        <rdfs:label xml:lang="en">Automated Theorem Prover</rdfs:label>
    </owl:Class>
    


    <!-- https://hack.cybersystems.engineer/memex/ontologies/SeamlessDigitalEngineering#Basic_Assumption -->

    <owl:Class rdf:about="https://hack.cybersystems.engineer/memex/ontologies/SeamlessDigitalEngineering#Basic_Assumption">
        <owl:equivalentClass>
            <owl:Restriction>
                <owl:onProperty rdf:resource="https://www.commoncoreontologies.org/ont00001808"/>
                <owl:someValuesFrom rdf:resource="https://hack.cybersystems.engineer/memex/ontologies/SeamlessDigitalEngineering#Assumption"/>
            </owl:Restriction>
        </owl:equivalentClass>
        <rdfs:subClassOf rdf:resource="https://www.commoncoreontologies.org/ont00000965"/>
        <rdfs:comment xml:lang="en">Such a collection corresponds to a set of axioms in formal system in logic.</rdfs:comment>
        <rdfs:label xml:lang="en">Basic Assumption</rdfs:label>
        <skos:definition xml:lang="en">Assumption in a collection of Claims shared by Assurance Cases in a specific field</skos:definition>
        <cco2:ont00001754 xml:lang="en">ISO/IEC/IEEE 15026-2:2022</cco2:ont00001754>
    </owl:Class>
    


    <!-- https://hack.cybersystems.engineer/memex/ontologies/SeamlessDigitalEngineering#Beneficialness -->

    <owl:Class rdf:about="https://hack.cybersystems.engineer/memex/ontologies/SeamlessDigitalEngineering#Beneficialness">
        <rdfs:subClassOf rdf:resource="https://hack.cybersystems.engineer/memex/ontologies/SeamlessDigitalEngineering#Product_Quality-in-Use"/>
        <rdfs:label xml:lang="en">Beneficialness</rdfs:label>
        <skos:definition xml:lang="en">extent of benefit resulting from the use of a Product, System or Service</skos:definition>
        <cco2:ont00001754 xml:lang="en">ISO/IEC 25019:2023(en)
Systems and software engineering — Systems and software Quality Requirements and Evaluation (SQuaRE) — Quality-in-use model</cco2:ont00001754>
    </owl:Class>
    


    <!-- https://hack.cybersystems.engineer/memex/ontologies/SeamlessDigitalEngineering#Bootstrappability -->

    <owl:Class rdf:about="https://hack.cybersystems.engineer/memex/ontologies/SeamlessDigitalEngineering#Bootstrappability">
        <owl:equivalentClass>
            <owl:Class>
                <owl:intersectionOf rdf:parseType="Collection">
                    <rdf:Description rdf:about="https://hack.cybersystems.engineer/memex/ontologies/SeamlessDigitalEngineering#Product_Capability"/>
                    <owl:Restriction>
                        <owl:onProperty rdf:resource="http://purl.obolibrary.org/obo/BFO_0000178"/>
                        <owl:someValuesFrom>
                            <owl:Class>
                                <owl:intersectionOf rdf:parseType="Collection">
                                    <rdf:Description rdf:about="https://hack.cybersystems.engineer/memex/ontologies/SeamlessDigitalEngineering#Product_Authenticity"/>
                                    <rdf:Description rdf:about="https://hack.cybersystems.engineer/memex/ontologies/SeamlessDigitalEngineering#Product_Integrity"/>
                                </owl:intersectionOf>
                            </owl:Class>
                        </owl:someValuesFrom>
                    </owl:Restriction>
                </owl:intersectionOf>
            </owl:Class>
        </owl:equivalentClass>
        <rdfs:subClassOf rdf:resource="https://hack.cybersystems.engineer/memex/ontologies/SeamlessDigitalEngineering#Product_Capability"/>
        <rdfs:label xml:lang="en">Bootstrappability</rdfs:label>
    </owl:Class>
    


    <!-- https://hack.cybersystems.engineer/memex/ontologies/SeamlessDigitalEngineering#Business_or_Mission_Analysis_Process -->

    <owl:Class rdf:about="https://hack.cybersystems.engineer/memex/ontologies/SeamlessDigitalEngineering#Business_or_Mission_Analysis_Process">
        <rdfs:subClassOf rdf:resource="https://hack.cybersystems.engineer/memex/ontologies/SeamlessDigitalEngineering#Technical_Process"/>
        <rdfs:label xml:lang="en">Business or Mission Analysis Process</rdfs:label>
        <skos:definition xml:lang="en">The purpose of the business or mission analysis process is to define the overall strategic problem or opportunity, characterize the solution space, and determine potential solution class(es) that can address a problem or take advantage of an opportunity.</skos:definition>
        <cco2:ont00001754>ISO/IEC/IEEE 15288:2023</cco2:ont00001754>
    </owl:Class>
    


    <!-- https://hack.cybersystems.engineer/memex/ontologies/SeamlessDigitalEngineering#Capability -->

    <owl:Class rdf:about="https://hack.cybersystems.engineer/memex/ontologies/SeamlessDigitalEngineering#Capability">
        <owl:equivalentClass>
            <owl:Restriction>
                <owl:onProperty rdf:resource="https://www.commoncoreontologies.org/ont00001889"/>
                <owl:someValuesFrom rdf:resource="https://hack.cybersystems.engineer/memex/ontologies/SeamlessDigitalEngineering#System"/>
            </owl:Restriction>
        </owl:equivalentClass>
        <rdfs:subClassOf rdf:resource="http://purl.obolibrary.org/obo/BFO_0000017"/>
        <rdfs:comment xml:lang="en">Generally, different kinds of capabilities exist: organizational capability, system (3.1.35) capability, and operational capability. Organizational capabilities relate through the work practices that are adopted by the organizations. New systems (with new or enhanced system capabilities) are developed to enhance enterprise operational capability in response to stakeholders&apos; (3.1.32) concerns (3.1.5) about a problem situation. Operational capabilities provide operational services that are enabled by system capabilities. These system capabilities are inherent in the system that is conceived, developed, created, and/or operated by an enterprise. Enterprise SE concentrates its efforts on maximizing operational value for various stakeholders, some of whom can be interested in the improvement of some problem situation.</rdfs:comment>
        <rdfs:label xml:lang="en">Capability</rdfs:label>
        <skos:definition xml:lang="en">A Realizable Entity that inheres in a System to the extent of that System&apos;s capacity to realize it in Intentional Acts of a certain type.</skos:definition>
        <skos:definition xml:lang="en">ability to do something useful under a particular set of conditions</skos:definition>
        <cco2:ont00001754 xml:lang="en">ISO/IEC/IEEE 24641:2023 — Systems and Software engineering — Methods and tools for model-based systems and software engineering</cco2:ont00001754>
    </owl:Class>
    


    <!-- https://hack.cybersystems.engineer/memex/ontologies/SeamlessDigitalEngineering#Certainty -->

    <owl:Class rdf:about="https://hack.cybersystems.engineer/memex/ontologies/SeamlessDigitalEngineering#Certainty">
        <rdfs:subClassOf rdf:resource="https://www.commoncoreontologies.org/ont00000555"/>
        <owl:disjointWith rdf:resource="https://hack.cybersystems.engineer/memex/ontologies/SeamlessDigitalEngineering#Uncertainty"/>
        <rdfs:label xml:lang="en">Certainty</rdfs:label>
        <skos:definition xml:lang="en">the state, even partial, of adequacy of information related to understanding or knowledge of an event, its consequence, or likelihood.</skos:definition>
        <cco2:ont00001754 xml:lang="en">derived from definition for uncertainty in ISO/IEC/IEEE 15288:2023</cco2:ont00001754>
    </owl:Class>
    


    <!-- https://hack.cybersystems.engineer/memex/ontologies/SeamlessDigitalEngineering#Claim -->

    <owl:Class rdf:about="https://hack.cybersystems.engineer/memex/ontologies/SeamlessDigitalEngineering#Claim">
        <owl:equivalentClass>
            <owl:Class>
                <owl:intersectionOf rdf:parseType="Collection">
                    <owl:Restriction>
                        <owl:onProperty rdf:resource="https://www.commoncoreontologies.org/ont00001942"/>
                        <owl:someValuesFrom rdf:resource="https://hack.cybersystems.engineer/memex/ontologies/SeamlessDigitalEngineering#Attribute"/>
                    </owl:Restriction>
                    <owl:Restriction>
                        <owl:onProperty rdf:resource="https://www.commoncoreontologies.org/ont00001942"/>
                        <owl:someValuesFrom rdf:resource="https://hack.cybersystems.engineer/memex/ontologies/SeamlessDigitalEngineering#Condition"/>
                    </owl:Restriction>
                    <owl:Restriction>
                        <owl:onProperty rdf:resource="https://www.commoncoreontologies.org/ont00001942"/>
                        <owl:someValuesFrom rdf:resource="https://hack.cybersystems.engineer/memex/ontologies/SeamlessDigitalEngineering#Uncertainty"/>
                    </owl:Restriction>
                </owl:intersectionOf>
            </owl:Class>
        </owl:equivalentClass>
        <rdfs:subClassOf rdf:resource="http://www.ontologyrepository.com/CommonCoreOntologies/Constraint"/>
        <rdfs:comment xml:lang="en">A claim potentially contains the following:

- Property of the System-of-Interest;
- limitations on the value of the Property associated with the Claim (e.g., on its range);
- limitations on the Uncertainty of the Property value meeting its limitations;
- limitations on duration of Claim&apos;s applicability;
- duration-related Uncertainty;
- limitations on Conditions associated with the Claim; and
- condition-related Uncertainty.</rdfs:comment>
        <rdfs:comment xml:lang="en">The term &quot;limitations&quot; is used to fit the many situations that can exist. Values can be a single value or multiple single values, a range of values or multiple ranges of values, and can be multi-dimensional. The boundaries of these limitations are sometimes not sharp, e.g., they can involve probability distributions and can be incremental.</rdfs:comment>
        <rdfs:comment xml:lang="en">Uncertainties may also be associated with the duration of applicability and the stated Conditions.</rdfs:comment>
        <rdfs:label xml:lang="en">Claim</rdfs:label>
        <skos:definition xml:lang="en">true-false statement about the limitations on the values of an unambiguously defined Property - called the Claim&apos;s Property - and limitations on the Uncertainty of the Property&apos;s values falling within these limitations during the Claim&apos;s duration of applicability under stated Conditions</skos:definition>
        <cco2:ont00001754 xml:lang="en">ISO/IEC/IEEE 15026-1:2019</cco2:ont00001754>
    </owl:Class>
    


    <!-- https://hack.cybersystems.engineer/memex/ontologies/SeamlessDigitalEngineering#Claim_Derived_by_Inference -->

    <owl:Class rdf:about="https://hack.cybersystems.engineer/memex/ontologies/SeamlessDigitalEngineering#Claim_Derived_by_Inference">
        <owl:equivalentClass>
            <owl:Class>
                <owl:intersectionOf rdf:parseType="Collection">
                    <rdf:Description rdf:about="https://hack.cybersystems.engineer/memex/ontologies/SeamlessDigitalEngineering#Claim"/>
                    <owl:Restriction>
                        <owl:onProperty rdf:resource="https://www.commoncoreontologies.org/ont00001816"/>
                        <owl:someValuesFrom rdf:resource="https://hack.cybersystems.engineer/memex/ontologies/SeamlessDigitalEngineering#Act_of_Logical_Inference"/>
                    </owl:Restriction>
                    <owl:Restriction>
                        <owl:onProperty rdf:resource="https://www.commoncoreontologies.org/ont00001920"/>
                        <owl:someValuesFrom rdf:resource="https://hack.cybersystems.engineer/memex/ontologies/SeamlessDigitalEngineering#Inference_Argument"/>
                    </owl:Restriction>
                </owl:intersectionOf>
            </owl:Class>
        </owl:equivalentClass>
        <rdfs:subClassOf rdf:resource="https://hack.cybersystems.engineer/memex/ontologies/SeamlessDigitalEngineering#Claim"/>
        <rdfs:label xml:lang="en">Claim Derived by Inference</rdfs:label>
        <cco2:ont00001754 xml:lang="en">derived from ISO/IEC/IEEE 15026-1:2019</cco2:ont00001754>
    </owl:Class>
    


    <!-- https://hack.cybersystems.engineer/memex/ontologies/SeamlessDigitalEngineering#Clean-Slate_Design_Approach -->

    <owl:Class rdf:about="https://hack.cybersystems.engineer/memex/ontologies/SeamlessDigitalEngineering#Clean-Slate_Design_Approach">
        <rdfs:subClassOf rdf:resource="https://hack.cybersystems.engineer/memex/ontologies/SeamlessDigitalEngineering#Design_Approach"/>
        <rdfs:label xml:lang="en">Clean-Slate Design Approach</rdfs:label>
        <skos:definition xml:lang="en">Approach where a System and Network are designed from scratch, based on a long-term, revolutionary Approach</skos:definition>
        <cco2:ont00001754 xml:lang="en">ISO/IEC TR 29181-1:2012
Information technology
Future Network
Problem statement and requirements
Part 1: Overall aspects</cco2:ont00001754>
    </owl:Class>
    


    <!-- https://hack.cybersystems.engineer/memex/ontologies/SeamlessDigitalEngineering#Client -->

    <owl:Class rdf:about="https://hack.cybersystems.engineer/memex/ontologies/SeamlessDigitalEngineering#Client">
        <rdfs:subClassOf rdf:resource="https://hack.cybersystems.engineer/memex/ontologies/SeamlessDigitalEngineering#Customer"/>
    </owl:Class>
    


    <!-- https://hack.cybersystems.engineer/memex/ontologies/SeamlessDigitalEngineering#Collaborative_SoS -->

    <owl:Class rdf:about="https://hack.cybersystems.engineer/memex/ontologies/SeamlessDigitalEngineering#Collaborative_SoS">
        <rdfs:subClassOf rdf:resource="https://hack.cybersystems.engineer/memex/ontologies/SeamlessDigitalEngineering#System-of-Systems"/>
        <rdfs:label xml:lang="en">Collaborative System-of-Systems</rdfs:label>
        <skos:definition xml:lang="en">The constituent systems interact more or less voluntarily to fulfill agreed upon central purposes. The central players collectively decide how to provide or deny service, thereby providing some means of enforcing and maintaining standards.</skos:definition>
        <cco2:ont00001754 xml:lang="en">ISO/IEC/IEEE 21841 - Systems and software engineering - Taxonomy of systems of systems</cco2:ont00001754>
    </owl:Class>
    


    <!-- https://hack.cybersystems.engineer/memex/ontologies/SeamlessDigitalEngineering#Complete_Assurance_Case_Report -->

    <owl:Class rdf:about="https://hack.cybersystems.engineer/memex/ontologies/SeamlessDigitalEngineering#Complete_Assurance_Case_Report">
        <owl:equivalentClass>
            <owl:Class>
                <owl:intersectionOf rdf:parseType="Collection">
                    <rdf:Description rdf:about="https://hack.cybersystems.engineer/memex/ontologies/SeamlessDigitalEngineering#Assurance_Case_Report"/>
                    <owl:Restriction>
                        <owl:onProperty rdf:resource="http://purl.obolibrary.org/obo/BFO_0000115"/>
                        <owl:someValuesFrom rdf:resource="https://hack.cybersystems.engineer/memex/ontologies/SeamlessDigitalEngineering#Supported_Assurance_Claim_Record"/>
                    </owl:Restriction>
                </owl:intersectionOf>
            </owl:Class>
        </owl:equivalentClass>
        <rdfs:subClassOf rdf:resource="https://hack.cybersystems.engineer/memex/ontologies/SeamlessDigitalEngineering#Assurance_Case_Report"/>
        <owl:disjointWith rdf:resource="https://hack.cybersystems.engineer/memex/ontologies/SeamlessDigitalEngineering#Incomplete_Assurance_Case_Report"/>
        <rdfs:label xml:lang="en">Complete Assurance Case Report</rdfs:label>
    </owl:Class>
    


    <!-- https://hack.cybersystems.engineer/memex/ontologies/SeamlessDigitalEngineering#Complex_Adaptive_System -->

    <owl:Class rdf:about="https://hack.cybersystems.engineer/memex/ontologies/SeamlessDigitalEngineering#Complex_Adaptive_System">
        <rdfs:subClassOf rdf:resource="https://hack.cybersystems.engineer/memex/ontologies/SeamlessDigitalEngineering#System"/>
        <rdfs:comment xml:lang="en">A complex adaptive system is a system that is complex in that it is a dynamic network of interactions, but the behavior of the ensemble may not be predictable according to the behavior of the components. It is adaptive in that the individual and collective behavior mutate and self-organize corresponding to the change-initiating micro-event or collection of events.

Source: https://en.wikipedia.org/wiki/Complex_adaptive_system</rdfs:comment>
        <rdfs:label xml:lang="en">Complex Adaptive System</rdfs:label>
        <cco2:ont00001760 rdf:datatype="http://www.w3.org/2001/XMLSchema#anyURI">https://semantic.incose.org/DEIX_Ontology</cco2:ont00001760>
    </owl:Class>
    


    <!-- https://hack.cybersystems.engineer/memex/ontologies/SeamlessDigitalEngineering#Compliance -->

    <owl:Class rdf:about="https://hack.cybersystems.engineer/memex/ontologies/SeamlessDigitalEngineering#Compliance">
        <rdfs:subClassOf rdf:resource="https://hack.cybersystems.engineer/memex/ontologies/SeamlessDigitalEngineering#Acceptability"/>
        <rdfs:label xml:lang="en">Compliance</rdfs:label>
        <skos:definition xml:lang="en">extent to which a User or other Stakeholder has confidence that a Product, System, Software, or Service in use meets Requirements, as required by rules or laws</skos:definition>
        <cco2:ont00001754 xml:lang="en">ISO/IEC 25019:2023(en)
Systems and software engineering — Systems and software Quality Requirements and Evaluation (SQuaRE) — Quality-in-use model</cco2:ont00001754>
    </owl:Class>
    


    <!-- https://hack.cybersystems.engineer/memex/ontologies/SeamlessDigitalEngineering#Computability_Theory_Discipline -->

    <owl:Class rdf:about="https://hack.cybersystems.engineer/memex/ontologies/SeamlessDigitalEngineering#Computability_Theory_Discipline">
        <rdfs:subClassOf rdf:resource="https://hack.cybersystems.engineer/memex/ontologies/SeamlessDigitalEngineering#Mathematical_Logic_Discipline"/>
        <rdfs:label xml:lang="en">Computability Theory Discipline</rdfs:label>
    </owl:Class>
    


    <!-- https://hack.cybersystems.engineer/memex/ontologies/SeamlessDigitalEngineering#Computer_Architecture -->

    <owl:Class rdf:about="https://hack.cybersystems.engineer/memex/ontologies/SeamlessDigitalEngineering#Computer_Architecture">
        <owl:equivalentClass>
            <owl:Class>
                <owl:intersectionOf rdf:parseType="Collection">
                    <rdf:Description rdf:about="https://hack.cybersystems.engineer/memex/ontologies/SeamlessDigitalEngineering#System_Architecture_Model"/>
                    <owl:Restriction>
                        <owl:onProperty rdf:resource="https://www.commoncoreontologies.org/ont00001942"/>
                        <owl:someValuesFrom rdf:resource="http://www.ontologyrepository.com/CommonCoreOntologies/ComputerSystem"/>
                    </owl:Restriction>
                </owl:intersectionOf>
            </owl:Class>
        </owl:equivalentClass>
        <rdfs:subClassOf rdf:resource="https://hack.cybersystems.engineer/memex/ontologies/SeamlessDigitalEngineering#System_Architecture_Model"/>
        <rdfs:label xml:lang="en">Computer Architecture</rdfs:label>
        <skos:altLabel xml:lang="en">Digital Architecture</skos:altLabel>
        <skos:definition xml:lang="en">a System Architecture that prescribes a Computer System and Computer Components, which may include System Software</skos:definition>
    </owl:Class>
    


    <!-- https://hack.cybersystems.engineer/memex/ontologies/SeamlessDigitalEngineering#Computing_Process -->

    <owl:Class rdf:about="https://hack.cybersystems.engineer/memex/ontologies/SeamlessDigitalEngineering#Computing_Process">
        <owl:equivalentClass>
            <owl:Class>
                <owl:intersectionOf rdf:parseType="Collection">
                    <rdf:Description rdf:about="http://www.ontologyrepository.com/CommonCoreOntologies/ComputerProgramExecution"/>
                    <owl:Restriction>
                        <owl:onProperty rdf:resource="http://purl.obolibrary.org/obo/BFO_0000055"/>
                        <owl:someValuesFrom rdf:resource="https://www.commoncoreontologies.org/ont00000932"/>
                    </owl:Restriction>
                    <owl:Restriction>
                        <owl:onProperty rdf:resource="http://purl.obolibrary.org/obo/BFO_0000057"/>
                        <owl:someValuesFrom rdf:resource="http://www.ontologyrepository.com/CommonCoreOntologies/DigitalObject"/>
                    </owl:Restriction>
                </owl:intersectionOf>
            </owl:Class>
        </owl:equivalentClass>
        <rdfs:subClassOf rdf:resource="http://www.ontologyrepository.com/CommonCoreOntologies/ComputerProgramExecution"/>
        <rdfs:label xml:lang="en">Computing Process</rdfs:label>
        <skos:editorialNote xml:lang="en">FIXME: This class is more specific than Computer Program Execution. Should the axiom be applied to that class instead? Is this class useful?</skos:editorialNote>
    </owl:Class>
    


    <!-- https://hack.cybersystems.engineer/memex/ontologies/SeamlessDigitalEngineering#Concept_Stage -->

    <owl:Class rdf:about="https://hack.cybersystems.engineer/memex/ontologies/SeamlessDigitalEngineering#Concept_Stage">
        <owl:equivalentClass>
            <owl:Class>
                <owl:intersectionOf rdf:parseType="Collection">
                    <rdf:Description rdf:about="https://hack.cybersystems.engineer/memex/ontologies/SeamlessDigitalEngineering#Lifecycle_Stage"/>
                    <owl:Restriction>
                        <owl:onProperty rdf:resource="https://www.commoncoreontologies.org/ont00001819"/>
                        <owl:someValuesFrom>
                            <owl:Class>
                                <owl:unionOf rdf:parseType="Collection">
                                    <rdf:Description rdf:about="https://hack.cybersystems.engineer/memex/ontologies/SeamlessDigitalEngineering#Opportunity"/>
                                    <rdf:Description rdf:about="https://hack.cybersystems.engineer/memex/ontologies/SeamlessDigitalEngineering#Problem"/>
                                    <rdf:Description rdf:about="https://hack.cybersystems.engineer/memex/ontologies/SeamlessDigitalEngineering#Threat"/>
                                </owl:unionOf>
                            </owl:Class>
                        </owl:someValuesFrom>
                    </owl:Restriction>
                    <owl:Restriction>
                        <owl:onProperty rdf:resource="https://www.commoncoreontologies.org/ont00001986"/>
                        <owl:someValuesFrom>
                            <owl:Class>
                                <owl:intersectionOf rdf:parseType="Collection">
                                    <rdf:Description rdf:about="https://hack.cybersystems.engineer/memex/ontologies/SeamlessDigitalEngineering#Need_Set"/>
                                    <rdf:Description rdf:about="https://hack.cybersystems.engineer/memex/ontologies/SeamlessDigitalEngineering#Requirement_Set"/>
                                </owl:intersectionOf>
                            </owl:Class>
                        </owl:someValuesFrom>
                    </owl:Restriction>
                </owl:intersectionOf>
            </owl:Class>
        </owl:equivalentClass>
        <rdfs:subClassOf rdf:resource="https://hack.cybersystems.engineer/memex/ontologies/SeamlessDigitalEngineering#Lifecycle_Stage"/>
        <rdfs:comment xml:lang="en">Purpose: The concept stage is executed to assess new business opportunities or mission assignments for feasibility and to discern stakeholder needs and requirements. The concept stage can be extended into evaluation of conceptual architecture and design solution.</rdfs:comment>
        <rdfs:label xml:lang="en">Concept Stage</rdfs:label>
        <cco2:ont00001754>ISO/IEC/IEEE 24748-1:2024</cco2:ont00001754>
    </owl:Class>
    


    <!-- https://hack.cybersystems.engineer/memex/ontologies/SeamlessDigitalEngineering#Concept_of_Operations -->

    <owl:Class rdf:about="https://hack.cybersystems.engineer/memex/ontologies/SeamlessDigitalEngineering#Concept_of_Operations">
        <owl:equivalentClass>
            <owl:Class>
                <owl:intersectionOf rdf:parseType="Collection">
                    <owl:Restriction>
                        <owl:onProperty rdf:resource="https://www.commoncoreontologies.org/ont00001942"/>
                        <owl:someValuesFrom rdf:resource="https://hack.cybersystems.engineer/memex/ontologies/SeamlessDigitalEngineering#Context_of_Use"/>
                    </owl:Restriction>
                    <owl:Restriction>
                        <owl:onProperty rdf:resource="https://www.commoncoreontologies.org/ont00001942"/>
                        <owl:someValuesFrom rdf:resource="https://www.commoncoreontologies.org/ont00001180"/>
                    </owl:Restriction>
                </owl:intersectionOf>
            </owl:Class>
        </owl:equivalentClass>
        <rdfs:subClassOf rdf:resource="https://hack.cybersystems.engineer/memex/ontologies/SeamlessDigitalEngineering#Lifecycle_Concept"/>
        <owl:disjointWith rdf:resource="https://hack.cybersystems.engineer/memex/ontologies/SeamlessDigitalEngineering#Operational_Concept"/>
        <rdfs:label xml:lang="en">Concept of Operations</rdfs:label>
        <skos:altLabel>ConOps</skos:altLabel>
        <skos:definition xml:lang="en">A verbal and graphic statement, in broad outline, of an Organization’s assumptions or intent in regard to an operation or series of operations of new, modified, or existing organizational Systems</skos:definition>
        <cco2:ont00001754>ISO/IEC/IEEE 15288:2023</cco2:ont00001754>
    </owl:Class>
    


    <!-- https://hack.cybersystems.engineer/memex/ontologies/SeamlessDigitalEngineering#Concern_Disposition -->

    <owl:Class rdf:about="https://hack.cybersystems.engineer/memex/ontologies/SeamlessDigitalEngineering#Concern_Disposition">
        <owl:equivalentClass>
            <owl:Class>
                <owl:intersectionOf rdf:parseType="Collection">
                    <rdf:Description rdf:about="http://purl.obolibrary.org/obo/BFO_0000016"/>
                    <owl:Restriction>
                        <owl:onProperty rdf:resource="http://purl.obolibrary.org/obo/BFO_0000197"/>
                        <owl:someValuesFrom rdf:resource="https://hack.cybersystems.engineer/memex/ontologies/SeamlessDigitalEngineering#Stakeholder"/>
                    </owl:Restriction>
                </owl:intersectionOf>
            </owl:Class>
        </owl:equivalentClass>
        <rdfs:subClassOf rdf:resource="http://purl.obolibrary.org/obo/BFO_0000016"/>
        <rdfs:comment xml:lang="en">matter of interest or importance to a Stakeholder

Source: ISO/IEC/IEEE 15288:2023</rdfs:comment>
        <rdfs:label xml:lang="en">Concern Disposition</rdfs:label>
        <skos:definition xml:lang="en">A Disposition that is realized when a Stakeholder bearer identifies a matter of interest or importance</skos:definition>
        <skos:scopeNote xml:lang="en">TBR: move concept to Systems Engineering domain ontology</skos:scopeNote>
        <cco2:ont00001754 xml:lang="en">derived from ISO/IEC/IEEE 15288:2023</cco2:ont00001754>
        <cco2:ont00001760 rdf:datatype="http://www.w3.org/2001/XMLSchema#anyURI">https://semantic.incose.org/DEIX_Ontology</cco2:ont00001760>
    </owl:Class>
    


    <!-- https://hack.cybersystems.engineer/memex/ontologies/SeamlessDigitalEngineering#Concern_Expression -->

    <owl:Class rdf:about="https://hack.cybersystems.engineer/memex/ontologies/SeamlessDigitalEngineering#Concern_Expression">
        <owl:equivalentClass>
            <owl:Class>
                <owl:intersectionOf rdf:parseType="Collection">
                    <rdf:Description rdf:about="https://www.commoncoreontologies.org/ont00000853"/>
                    <owl:Restriction>
                        <owl:onProperty rdf:resource="https://www.commoncoreontologies.org/ont00001982"/>
                        <owl:someValuesFrom rdf:resource="https://hack.cybersystems.engineer/memex/ontologies/SeamlessDigitalEngineering#Concern_Disposition"/>
                    </owl:Restriction>
                </owl:intersectionOf>
            </owl:Class>
        </owl:equivalentClass>
        <rdfs:subClassOf rdf:resource="https://www.commoncoreontologies.org/ont00000853"/>
        <rdfs:comment xml:lang="en">In the systems engineering domain, Concern Expressions have an associated Stakeholder that is the bearer of a particular role, e.g. Engineer Role. That is, this engineer stakeholder has expressed a concern about the system-of-interest which is then recorded in an Information Bearing Artifact and subject to change control.</rdfs:comment>
        <rdfs:label xml:lang="en">Concern Expression</rdfs:label>
        <skos:definition xml:lang="en">A Descriptive Information Content Entity that describes a Concern Disposition that a particular Stakeholder bears</skos:definition>
        <skos:scopeNote xml:lang="en">TBR: move concept to Systems Engineering domain ontology</skos:scopeNote>
        <cco2:ont00001760 rdf:datatype="http://www.w3.org/2001/XMLSchema#anyURI">https://semantic.incose.org/DEIX_Ontology</cco2:ont00001760>
    </owl:Class>
    


    <!-- https://hack.cybersystems.engineer/memex/ontologies/SeamlessDigitalEngineering#Condition -->

    <owl:Class rdf:about="https://hack.cybersystems.engineer/memex/ontologies/SeamlessDigitalEngineering#Condition">
        <owl:equivalentClass>
            <owl:Class>
                <owl:intersectionOf rdf:parseType="Collection">
                    <rdf:Description rdf:about="https://hack.cybersystems.engineer/memex/ontologies/SeamlessDigitalEngineering#Attribute"/>
                    <owl:Restriction>
                        <owl:onProperty rdf:resource="https://www.commoncoreontologies.org/ont00001920"/>
                        <owl:someValuesFrom rdf:resource="https://hack.cybersystems.engineer/memex/ontologies/SeamlessDigitalEngineering#Requirement"/>
                    </owl:Restriction>
                </owl:intersectionOf>
            </owl:Class>
        </owl:equivalentClass>
        <rdfs:subClassOf rdf:resource="https://hack.cybersystems.engineer/memex/ontologies/SeamlessDigitalEngineering#Attribute"/>
        <rdfs:label xml:lang="en">Condition</rdfs:label>
        <skos:definition xml:lang="en">measurable qualitative or quantitative Attribute that is stipulated for a Requirement and that indicates a circumstance or event under which a Requirement applies</skos:definition>
        <cco2:ont00001754 xml:lang="en">ISO/IEC/IEEE 15026-1:2019</cco2:ont00001754>
    </owl:Class>
    


    <!-- https://hack.cybersystems.engineer/memex/ontologies/SeamlessDigitalEngineering#Confidence -->

    <owl:Class rdf:about="https://hack.cybersystems.engineer/memex/ontologies/SeamlessDigitalEngineering#Confidence">
        <rdfs:subClassOf rdf:resource="http://purl.obolibrary.org/obo/BFO_0000016"/>
        <rdfs:subClassOf>
            <owl:Class>
                <owl:unionOf rdf:parseType="Collection">
                    <owl:Restriction>
                        <owl:onProperty rdf:resource="http://purl.obolibrary.org/obo/BFO_0000197"/>
                        <owl:someValuesFrom rdf:resource="https://www.commoncoreontologies.org/ont00001017"/>
                    </owl:Restriction>
                    <owl:Restriction>
                        <owl:onProperty rdf:resource="https://www.commoncoreontologies.org/ont00001829"/>
                        <owl:someValuesFrom rdf:resource="https://www.commoncoreontologies.org/ont00000300"/>
                    </owl:Restriction>
                </owl:unionOf>
            </owl:Class>
        </rdfs:subClassOf>
        <rdfs:subClassOf>
            <owl:Restriction>
                <owl:onProperty rdf:resource="http://purl.obolibrary.org/obo/BFO_0000054"/>
                <owl:someValuesFrom rdf:resource="https://hack.cybersystems.engineer/memex/ontologies/SeamlessDigitalEngineering#Certainty"/>
            </owl:Restriction>
        </rdfs:subClassOf>
        <rdfs:label xml:lang="en">Confidence</rdfs:label>
        <skos:definition xml:lang="en">belief in the Certainty of something</skos:definition>
        <cco2:ont00001754 xml:lang="en">The American Heritage Dictionary of the English Language, 5th Edition.</cco2:ont00001754>
    </owl:Class>
    


    <!-- https://hack.cybersystems.engineer/memex/ontologies/SeamlessDigitalEngineering#Configuration_Management_Process -->

    <owl:Class rdf:about="https://hack.cybersystems.engineer/memex/ontologies/SeamlessDigitalEngineering#Configuration_Management_Process">
        <rdfs:subClassOf rdf:resource="https://hack.cybersystems.engineer/memex/ontologies/SeamlessDigitalEngineering#Technical_Management_Process"/>
        <rdfs:label xml:lang="en">Configuration Management Process</rdfs:label>
        <skos:definition xml:lang="en">The purpose of the configuration management process is to manage system and system element configurations over their life cycle.</skos:definition>
        <cco2:ont00001754>ISO/IEC/IEEE 15288:2023</cco2:ont00001754>
    </owl:Class>
    


    <!-- https://hack.cybersystems.engineer/memex/ontologies/SeamlessDigitalEngineering#Configuration_Status_Report -->

    <owl:Class rdf:about="https://hack.cybersystems.engineer/memex/ontologies/SeamlessDigitalEngineering#Configuration_Status_Report">
        <rdfs:subClassOf rdf:resource="https://www.commoncoreontologies.org/ont00000624"/>
    </owl:Class>
    


    <!-- https://hack.cybersystems.engineer/memex/ontologies/SeamlessDigitalEngineering#Conformity -->

    <owl:Class rdf:about="https://hack.cybersystems.engineer/memex/ontologies/SeamlessDigitalEngineering#Conformity">
        <owl:equivalentClass>
            <owl:Class>
                <owl:intersectionOf rdf:parseType="Collection">
                    <owl:Restriction>
                        <owl:onProperty rdf:resource="http://purl.obolibrary.org/obo/BFO_0000197"/>
                        <owl:someValuesFrom rdf:resource="https://hack.cybersystems.engineer/memex/ontologies/SeamlessDigitalEngineering#System"/>
                    </owl:Restriction>
                    <owl:Restriction>
                        <owl:onProperty rdf:resource="https://www.commoncoreontologies.org/ont00001920"/>
                        <owl:someValuesFrom rdf:resource="https://hack.cybersystems.engineer/memex/ontologies/SeamlessDigitalEngineering#Requirement"/>
                    </owl:Restriction>
                </owl:intersectionOf>
            </owl:Class>
        </owl:equivalentClass>
        <rdfs:subClassOf rdf:resource="http://purl.obolibrary.org/obo/BFO_0000016"/>
        <rdfs:label xml:lang="en">Conformity</rdfs:label>
        <skos:definition xml:lang="en">fulfilment of a Requirement</skos:definition>
        <cco2:ont00001754 xml:lang="en">ISO 9000:2015, 3.6.11</cco2:ont00001754>
    </owl:Class>
    


    <!-- https://hack.cybersystems.engineer/memex/ontologies/SeamlessDigitalEngineering#Conformity_Measure -->

    <owl:Class rdf:about="https://hack.cybersystems.engineer/memex/ontologies/SeamlessDigitalEngineering#Conformity_Measure">
        <owl:equivalentClass>
            <owl:Class>
                <owl:intersectionOf rdf:parseType="Collection">
                    <rdf:Description rdf:about="https://www.commoncoreontologies.org/ont00000731"/>
                    <owl:Restriction>
                        <owl:onProperty rdf:resource="https://www.commoncoreontologies.org/ont00001966"/>
                        <owl:someValuesFrom rdf:resource="https://hack.cybersystems.engineer/memex/ontologies/SeamlessDigitalEngineering#Conformity"/>
                    </owl:Restriction>
                </owl:intersectionOf>
            </owl:Class>
        </owl:equivalentClass>
        <rdfs:subClassOf rdf:resource="https://www.commoncoreontologies.org/ont00000731"/>
        <rdfs:label xml:lang="en">Conformity Measure</rdfs:label>
        <skos:definition xml:lang="en">measure of fulfilment of a Requirement</skos:definition>
        <cco2:ont00001754 xml:lang="en">derived from ISO 9000:2015, 3.6.11</cco2:ont00001754>
    </owl:Class>
    


    <!-- https://hack.cybersystems.engineer/memex/ontologies/SeamlessDigitalEngineering#Consequence -->

    <owl:Class rdf:about="https://hack.cybersystems.engineer/memex/ontologies/SeamlessDigitalEngineering#Consequence">
        <owl:equivalentClass>
            <owl:Class>
                <owl:intersectionOf rdf:parseType="Collection">
                    <rdf:Description rdf:about="https://www.commoncoreontologies.org/ont00000660"/>
                    <owl:Restriction>
                        <owl:onProperty rdf:resource="https://www.commoncoreontologies.org/ont00001834"/>
                        <owl:someValuesFrom rdf:resource="https://www.commoncoreontologies.org/ont00000476"/>
                    </owl:Restriction>
                </owl:intersectionOf>
            </owl:Class>
        </owl:equivalentClass>
        <rdfs:subClassOf rdf:resource="https://www.commoncoreontologies.org/ont00000660"/>
        <rdfs:label xml:lang="en">Consequence</rdfs:label>
        <skos:definition xml:lang="en">outcome of an event affecting Objectives</skos:definition>
        <cco2:ont00001754 xml:lang="en">ISO/IEC/IEEE 15026-1:2019</cco2:ont00001754>
    </owl:Class>
    


    <!-- https://hack.cybersystems.engineer/memex/ontologies/SeamlessDigitalEngineering#Constraint_Logic_Programming_Language -->

    <owl:Class rdf:about="https://hack.cybersystems.engineer/memex/ontologies/SeamlessDigitalEngineering#Constraint_Logic_Programming_Language">
        <rdfs:subClassOf rdf:resource="https://hack.cybersystems.engineer/memex/ontologies/SeamlessDigitalEngineering#Logic_Programming_Language"/>
        <rdfs:label xml:lang="en">Constraint Logic Programming Language</rdfs:label>
    </owl:Class>
    


    <!-- https://hack.cybersystems.engineer/memex/ontologies/SeamlessDigitalEngineering#Constraint_Solver -->

    <owl:Class rdf:about="https://hack.cybersystems.engineer/memex/ontologies/SeamlessDigitalEngineering#Constraint_Solver">
        <rdfs:subClassOf rdf:resource="http://www.ontologyrepository.com/CommonCoreOntologies/SoftwareEngineeringSoftware"/>
        <rdfs:label xml:lang="en">Constraint Solver</rdfs:label>
    </owl:Class>
    


    <!-- https://hack.cybersystems.engineer/memex/ontologies/SeamlessDigitalEngineering#Context_of_Use -->

    <owl:Class rdf:about="https://hack.cybersystems.engineer/memex/ontologies/SeamlessDigitalEngineering#Context_of_Use">
        <owl:equivalentClass>
            <owl:Class>
                <owl:intersectionOf rdf:parseType="Collection">
                    <owl:Restriction>
                        <owl:onProperty rdf:resource="http://purl.obolibrary.org/obo/BFO_0000115"/>
                        <owl:someValuesFrom rdf:resource="https://hack.cybersystems.engineer/memex/ontologies/SeamlessDigitalEngineering#System_Environment"/>
                    </owl:Restriction>
                    <owl:Restriction>
                        <owl:onProperty rdf:resource="http://purl.obolibrary.org/obo/BFO_0000115"/>
                        <owl:someValuesFrom>
                            <owl:Class>
                                <owl:intersectionOf rdf:parseType="Collection">
                                    <rdf:Description rdf:about="https://hack.cybersystems.engineer/memex/ontologies/SeamlessDigitalEngineering#System"/>
                                    <rdf:Description rdf:about="https://www.commoncoreontologies.org/ont00001017"/>
                                </owl:intersectionOf>
                            </owl:Class>
                        </owl:someValuesFrom>
                    </owl:Restriction>
                    <owl:Restriction>
                        <owl:onProperty rdf:resource="http://purl.obolibrary.org/obo/BFO_0000183"/>
                        <owl:someValuesFrom>
                            <owl:Class>
                                <owl:intersectionOf rdf:parseType="Collection">
                                    <rdf:Description rdf:about="https://hack.cybersystems.engineer/memex/ontologies/SeamlessDigitalEngineering#Activity"/>
                                    <rdf:Description rdf:about="https://www.commoncoreontologies.org/ont00000566"/>
                                </owl:intersectionOf>
                            </owl:Class>
                        </owl:someValuesFrom>
                    </owl:Restriction>
                </owl:intersectionOf>
            </owl:Class>
        </owl:equivalentClass>
        <rdfs:subClassOf rdf:resource="http://purl.obolibrary.org/obo/BFO_0000027"/>
        <rdfs:label xml:lang="en">Context of Use</rdfs:label>
        <skos:definition xml:lang="en">Users, Tasks, equipment (hardware, software, and materials) (Systems), and the physical and social environments (System Environments) in which a Product is used</skos:definition>
        <cco2:ont00001754 xml:lang="en">ISO/IEC 25002:2024</cco2:ont00001754>
        <cco2:ont00001760 rdf:datatype="http://www.w3.org/2001/XMLSchema#anyURI">https://semantic.incose.org/DEIX_Ontology</cco2:ont00001760>
    </owl:Class>
    


    <!-- https://hack.cybersystems.engineer/memex/ontologies/SeamlessDigitalEngineering#Contractor -->

    <owl:Class rdf:about="https://hack.cybersystems.engineer/memex/ontologies/SeamlessDigitalEngineering#Contractor">
        <rdfs:subClassOf rdf:resource="https://hack.cybersystems.engineer/memex/ontologies/SeamlessDigitalEngineering#Supplier"/>
        <rdfs:label xml:lang="en">Contractor</rdfs:label>
        <cco2:ont00001754 xml:lang="en">ISO/IEC/IEEE 24765:2017</cco2:ont00001754>
    </owl:Class>
    


    <!-- https://hack.cybersystems.engineer/memex/ontologies/SeamlessDigitalEngineering#Correct-by-Construction -->

    <owl:Class rdf:about="https://hack.cybersystems.engineer/memex/ontologies/SeamlessDigitalEngineering#Correct-by-Construction">
        <owl:equivalentClass>
            <owl:Class>
                <owl:intersectionOf rdf:parseType="Collection">
                    <rdf:Description rdf:about="https://hack.cybersystems.engineer/memex/ontologies/SeamlessDigitalEngineering#Assurance_Goal"/>
                    <owl:Restriction>
                        <owl:onProperty rdf:resource="http://purl.obolibrary.org/obo/BFO_0000058"/>
                        <owl:someValuesFrom rdf:resource="https://hack.cybersystems.engineer/memex/ontologies/SeamlessDigitalEngineering#Integration_Process"/>
                    </owl:Restriction>
                    <owl:Restriction>
                        <owl:onProperty rdf:resource="http://purl.obolibrary.org/obo/BFO_0000058"/>
                        <owl:someValuesFrom rdf:resource="https://hack.cybersystems.engineer/memex/ontologies/SeamlessDigitalEngineering#Loss_of_Error"/>
                    </owl:Restriction>
                    <owl:Restriction>
                        <owl:onProperty rdf:resource="https://www.commoncoreontologies.org/ont00001942"/>
                        <owl:someValuesFrom rdf:resource="https://hack.cybersystems.engineer/memex/ontologies/SeamlessDigitalEngineering#High-Integrity_Level"/>
                    </owl:Restriction>
                    <owl:Restriction>
                        <owl:onProperty rdf:resource="https://www.commoncoreontologies.org/ont00001942"/>
                        <owl:someValuesFrom rdf:resource="https://hack.cybersystems.engineer/memex/ontologies/SeamlessDigitalEngineering#Process_Outcome"/>
                    </owl:Restriction>
                </owl:intersectionOf>
            </owl:Class>
        </owl:equivalentClass>
        <rdfs:subClassOf rdf:resource="https://hack.cybersystems.engineer/memex/ontologies/SeamlessDigitalEngineering#Assurance_Goal"/>
        <rdfs:comment xml:lang="en">&quot;Achieving the goal of Correct-by-Construction design requires that models and analysis methods in the design phase predict with the required accuracy the behavior of the designed system.&quot; - doi:10.1007/978-3-642-54848-2_16</rdfs:comment>
        <rdfs:label xml:lang="en">Correct-by-Construction</rdfs:label>
        <skos:definition xml:lang="en">An Assurance Goal to eliminate Integration Process-time errors emerging from undesirable cross-layer interactions</skos:definition>
        <cco2:ont00001754 rdf:datatype="http://www.w3.org/2001/XMLSchema#anyURI">https://dx.doi.org/10.1109/JPROC.2011.2161529</cco2:ont00001754>
    </owl:Class>
    


    <!-- https://hack.cybersystems.engineer/memex/ontologies/SeamlessDigitalEngineering#Correctness -->

    <owl:Class rdf:about="https://hack.cybersystems.engineer/memex/ontologies/SeamlessDigitalEngineering#Correctness">
        <owl:equivalentClass>
            <owl:Class>
                <owl:intersectionOf rdf:parseType="Collection">
                    <rdf:Description rdf:about="https://hack.cybersystems.engineer/memex/ontologies/SeamlessDigitalEngineering#Conformity"/>
                    <owl:Restriction>
                        <owl:onProperty rdf:resource="http://purl.obolibrary.org/obo/BFO_0000195"/>
                        <owl:someValuesFrom rdf:resource="https://hack.cybersystems.engineer/memex/ontologies/SeamlessDigitalEngineering#Product_Faultlessness"/>
                    </owl:Restriction>
                </owl:intersectionOf>
            </owl:Class>
        </owl:equivalentClass>
        <rdfs:subClassOf rdf:resource="https://hack.cybersystems.engineer/memex/ontologies/SeamlessDigitalEngineering#Conformity"/>
        <rdfs:label xml:lang="en">Correctness</rdfs:label>
        <skos:definition xml:lang="en">degree to which a System or System Element is free from Faults in its specification, design, and implementation</skos:definition>
        <cco2:ont00001754 xml:lang="en">ISO/IEC/IEEE 24765:2017, 3.892</cco2:ont00001754>
    </owl:Class>
    


    <!-- https://hack.cybersystems.engineer/memex/ontologies/SeamlessDigitalEngineering#Correctness_Measure -->

    <owl:Class rdf:about="https://hack.cybersystems.engineer/memex/ontologies/SeamlessDigitalEngineering#Correctness_Measure">
        <owl:equivalentClass>
            <owl:Class>
                <owl:intersectionOf rdf:parseType="Collection">
                    <rdf:Description rdf:about="https://www.commoncoreontologies.org/ont00001256"/>
                    <owl:Restriction>
                        <owl:onProperty rdf:resource="https://www.commoncoreontologies.org/ont00001966"/>
                        <owl:someValuesFrom>
                            <owl:Class>
                                <owl:unionOf rdf:parseType="Collection">
                                    <rdf:Description rdf:about="https://hack.cybersystems.engineer/memex/ontologies/SeamlessDigitalEngineering#Correctness"/>
                                    <rdf:Description rdf:about="https://hack.cybersystems.engineer/memex/ontologies/SeamlessDigitalEngineering#Product_Functional_Correctness"/>
                                </owl:unionOf>
                            </owl:Class>
                        </owl:someValuesFrom>
                    </owl:Restriction>
                </owl:intersectionOf>
            </owl:Class>
        </owl:equivalentClass>
        <rdfs:subClassOf rdf:resource="https://www.commoncoreontologies.org/ont00001256"/>
        <rdfs:label xml:lang="en">Correctness Measure</rdfs:label>
        <skos:definition xml:lang="en">A Measurement Information Content Entity that is a measurement of the degree to which a System or System Element is free from Faults in its specification, design, and implementation</skos:definition>
        <cco2:ont00001754 xml:lang="en">ISO/IEC/IEEE 24765:2017, 3.892</cco2:ont00001754>
    </owl:Class>
    


    <!-- https://hack.cybersystems.engineer/memex/ontologies/SeamlessDigitalEngineering#Customer -->

    <owl:Class rdf:about="https://hack.cybersystems.engineer/memex/ontologies/SeamlessDigitalEngineering#Customer">
        <owl:equivalentClass>
            <owl:Class>
                <owl:intersectionOf rdf:parseType="Collection">
                    <rdf:Description rdf:about="https://hack.cybersystems.engineer/memex/ontologies/SeamlessDigitalEngineering#Stakeholder"/>
                    <owl:Restriction>
                        <owl:onProperty rdf:resource="http://purl.obolibrary.org/obo/BFO_0000196"/>
                        <owl:someValuesFrom>
                            <owl:Class>
                                <owl:intersectionOf rdf:parseType="Collection">
                                    <rdf:Description rdf:about="https://www.commoncoreontologies.org/ont00000038"/>
                                    <rdf:Description rdf:about="https://www.commoncoreontologies.org/ont00000485"/>
                                </owl:intersectionOf>
                            </owl:Class>
                        </owl:someValuesFrom>
                    </owl:Restriction>
                </owl:intersectionOf>
            </owl:Class>
        </owl:equivalentClass>
        <rdfs:subClassOf rdf:resource="https://hack.cybersystems.engineer/memex/ontologies/SeamlessDigitalEngineering#Stakeholder"/>
        <skos:definition xml:lang="en">Organization or person that receives a Product or Service</skos:definition>
        <skos:example>consumer; client; user; acquirer; buyer; purchaser</skos:example>
        <cco2:ont00001754>ISO/IEC/IEEE 15288:2023</cco2:ont00001754>
    </owl:Class>
    


    <!-- https://hack.cybersystems.engineer/memex/ontologies/SeamlessDigitalEngineering#Cyber_Regulation -->

    <owl:Class rdf:about="https://hack.cybersystems.engineer/memex/ontologies/SeamlessDigitalEngineering#Cyber_Regulation">
        <owl:equivalentClass>
            <owl:Class>
                <owl:intersectionOf rdf:parseType="Collection">
                    <rdf:Description rdf:about="https://www.commoncoreontologies.org/ont00001324"/>
                    <owl:Restriction>
                        <owl:onProperty rdf:resource="https://www.commoncoreontologies.org/ont00001942"/>
                        <owl:someValuesFrom rdf:resource="http://www.ontologyrepository.com/CommonCoreOntologies/CyberAct"/>
                    </owl:Restriction>
                </owl:intersectionOf>
            </owl:Class>
        </owl:equivalentClass>
        <rdfs:subClassOf rdf:resource="https://www.commoncoreontologies.org/ont00001324"/>
        <rdfs:label xml:lang="en">Cyber Regulation</rdfs:label>
    </owl:Class>
    


    <!-- https://hack.cybersystems.engineer/memex/ontologies/SeamlessDigitalEngineering#Cyber_Right -->

    <owl:Class rdf:about="https://hack.cybersystems.engineer/memex/ontologies/SeamlessDigitalEngineering#Cyber_Right">
        <owl:equivalentClass>
            <owl:Class>
                <owl:intersectionOf rdf:parseType="Collection">
                    <rdf:Description rdf:about="https://hack.cybersystems.engineer/memex/ontologies/SeamlessDigitalEngineering#Right"/>
                    <owl:Restriction>
                        <owl:onProperty rdf:resource="http://purl.obolibrary.org/obo/BFO_0000054"/>
                        <owl:someValuesFrom rdf:resource="http://www.ontologyrepository.com/CommonCoreOntologies/CyberAct"/>
                    </owl:Restriction>
                </owl:intersectionOf>
            </owl:Class>
        </owl:equivalentClass>
        <rdfs:subClassOf rdf:resource="https://hack.cybersystems.engineer/memex/ontologies/SeamlessDigitalEngineering#Right"/>
        <rdfs:label xml:lang="en">Cyber Right</rdfs:label>
        <skos:definition xml:lang="en">A Right which is realized by some Cyber Act</skos:definition>
    </owl:Class>
    


    <!-- https://hack.cybersystems.engineer/memex/ontologies/SeamlessDigitalEngineering#Cyberspace -->

    <owl:Class rdf:about="https://hack.cybersystems.engineer/memex/ontologies/SeamlessDigitalEngineering#Cyberspace">
        <owl:equivalentClass>
            <owl:Class>
                <owl:intersectionOf rdf:parseType="Collection">
                    <rdf:Description rdf:about="https://www.commoncoreontologies.org/ont00000591"/>
                    <owl:Restriction>
                        <owl:onProperty rdf:resource="http://purl.obolibrary.org/obo/BFO_0000124"/>
                        <owl:someValuesFrom rdf:resource="https://www.commoncoreontologies.org/ont00000700"/>
                    </owl:Restriction>
                    <owl:Restriction>
                        <owl:onProperty rdf:resource="http://purl.obolibrary.org/obo/BFO_0000183"/>
                        <owl:someValuesFrom rdf:resource="http://www.ontologyrepository.com/CommonCoreOntologies/CyberAct"/>
                    </owl:Restriction>
                </owl:intersectionOf>
            </owl:Class>
        </owl:equivalentClass>
        <rdfs:subClassOf rdf:resource="https://www.commoncoreontologies.org/ont00000591"/>
        <rdfs:label xml:lang="en">Cyberspace</rdfs:label>
        <skos:definition xml:lang="en">interconnected digital environment of Computer Networks, Services, Systems, People, Cyber Acts, Organizations, and that which resides on the Digital Environment or traverses through it</skos:definition>
        <cco2:ont00001754 xml:lang="en">ISO/IEC TS 27100:2020, 3.5</cco2:ont00001754>
    </owl:Class>
    


    <!-- https://hack.cybersystems.engineer/memex/ontologies/SeamlessDigitalEngineering#Danger -->

    <owl:Class rdf:about="https://hack.cybersystems.engineer/memex/ontologies/SeamlessDigitalEngineering#Danger">
        <rdfs:subClassOf rdf:resource="https://www.commoncoreontologies.org/ont00000997"/>
        <rdfs:subClassOf>
            <owl:Restriction>
                <owl:onProperty rdf:resource="http://purl.obolibrary.org/obo/BFO_0000197"/>
                <owl:someValuesFrom rdf:resource="https://hack.cybersystems.engineer/memex/ontologies/SeamlessDigitalEngineering#Context_of_Use"/>
            </owl:Restriction>
        </rdfs:subClassOf>
        <rdfs:label xml:lang="en">Danger</rdfs:label>
        <skos:definition xml:lang="en">hazardous situation, which if not avoided, can result in death or serious injury</skos:definition>
        <cco2:ont00001754 xml:lang="en">ISO/IEC/IEEE 26514:2022 — Systems and software engineering — Design and development of information for users</cco2:ont00001754>
    </owl:Class>
    


    <!-- https://hack.cybersystems.engineer/memex/ontologies/SeamlessDigitalEngineering#Data -->

    <owl:Class rdf:about="https://hack.cybersystems.engineer/memex/ontologies/SeamlessDigitalEngineering#Data">
        <owl:equivalentClass>
            <owl:Class>
                <owl:intersectionOf rdf:parseType="Collection">
                    <rdf:Description rdf:about="https://www.commoncoreontologies.org/ont00000798"/>
                    <owl:Class>
                        <owl:unionOf rdf:parseType="Collection">
                            <owl:Restriction>
                                <owl:onProperty rdf:resource="https://www.commoncoreontologies.org/ont00001816"/>
                                <owl:someValuesFrom rdf:resource="https://www.commoncoreontologies.org/ont00001158"/>
                            </owl:Restriction>
                            <owl:Restriction>
                                <owl:onProperty rdf:resource="https://www.commoncoreontologies.org/ont00001841"/>
                                <owl:someValuesFrom rdf:resource="https://www.commoncoreontologies.org/ont00001158"/>
                            </owl:Restriction>
                        </owl:unionOf>
                    </owl:Class>
                    <owl:Restriction>
                        <owl:onProperty rdf:resource="https://www.commoncoreontologies.org/ont00001956"/>
                        <owl:someValuesFrom rdf:resource="https://hack.cybersystems.engineer/memex/ontologies/SeamlessDigitalEngineering#Digital"/>
                    </owl:Restriction>
                </owl:intersectionOf>
            </owl:Class>
        </owl:equivalentClass>
        <rdfs:subClassOf rdf:resource="https://www.commoncoreontologies.org/ont00000798"/>
        <rdfs:label xml:lang="en">Data</rdfs:label>
        <skos:definition xml:lang="en">reinterpretable representation of information in a formalized manner suitable for communication, interpretation, or processing</skos:definition>
        <cco2:ont00001754 xml:lang="en">ISO/IEC 25000:2014 Systems and software engineering —Systems and software Quality Requirements and Evaluation (SQuaRE) — Guide to SQuaRE</cco2:ont00001754>
        <cco2:ont00001760 rdf:datatype="http://www.w3.org/2001/XMLSchema#anyURI">https://semantic.incose.org/DEIX_Ontology</cco2:ont00001760>
    </owl:Class>
    


    <!-- https://hack.cybersystems.engineer/memex/ontologies/SeamlessDigitalEngineering#Data_Quality -->

    <owl:Class rdf:about="https://hack.cybersystems.engineer/memex/ontologies/SeamlessDigitalEngineering#Data_Quality">
        <owl:equivalentClass>
            <owl:Class>
                <owl:intersectionOf rdf:parseType="Collection">
                    <rdf:Description rdf:about="https://hack.cybersystems.engineer/memex/ontologies/SeamlessDigitalEngineering#Quality"/>
                    <owl:Restriction>
                        <owl:onProperty rdf:resource="http://purl.obolibrary.org/obo/BFO_0000195"/>
                        <owl:someValuesFrom rdf:resource="https://hack.cybersystems.engineer/memex/ontologies/SeamlessDigitalEngineering#Data"/>
                    </owl:Restriction>
                </owl:intersectionOf>
            </owl:Class>
        </owl:equivalentClass>
        <rdfs:subClassOf rdf:resource="https://hack.cybersystems.engineer/memex/ontologies/SeamlessDigitalEngineering#Quality"/>
        <rdfs:label xml:lang="en">Data Quality</rdfs:label>
        <skos:definition xml:lang="en">capability of the characteristics of Data to satisfy stated and implied Needs when used under specified conditions</skos:definition>
        <cco2:ont00001754 xml:lang="en">ISO/IEC 25002:2024 Systems and software engineering - Systems and software Quality Requirements and Evaluation (SQuaRE) - Quality model overview and usage</cco2:ont00001754>
    </owl:Class>
    


    <!-- https://hack.cybersystems.engineer/memex/ontologies/SeamlessDigitalEngineering#Data_Transfer_Function -->

    <owl:Class rdf:about="https://hack.cybersystems.engineer/memex/ontologies/SeamlessDigitalEngineering#Data_Transfer_Function">
        <rdfs:subClassOf rdf:resource="https://www.commoncoreontologies.org/ont00000323"/>
        <rdfs:label xml:lang="en">Data Transfer Function</rdfs:label>
        <cco2:ont00001760 rdf:datatype="http://www.w3.org/2001/XMLSchema#anyURI">https://semantic.incose.org/DEIX_Ontology</cco2:ont00001760>
    </owl:Class>
    


    <!-- https://hack.cybersystems.engineer/memex/ontologies/SeamlessDigitalEngineering#Decision_Management_Process -->

    <owl:Class rdf:about="https://hack.cybersystems.engineer/memex/ontologies/SeamlessDigitalEngineering#Decision_Management_Process">
        <rdfs:subClassOf rdf:resource="https://hack.cybersystems.engineer/memex/ontologies/SeamlessDigitalEngineering#Technical_Management_Process"/>
        <rdfs:label xml:lang="en">Decision Management Process</rdfs:label>
        <skos:definition xml:lang="en">The purpose of the decision management process is to provide a structured, analytical framework for objectively identifying, characterizing, and evaluating a set of alternatives for a decision at any point in the life cycle and select the most beneficial course of action.</skos:definition>
        <cco2:ont00001754>ISO/IEC/IEEE 15288:2023</cco2:ont00001754>
    </owl:Class>
    


    <!-- https://hack.cybersystems.engineer/memex/ontologies/SeamlessDigitalEngineering#Decision_Support_Problem_Definition -->

    <owl:Class rdf:about="https://hack.cybersystems.engineer/memex/ontologies/SeamlessDigitalEngineering#Decision_Support_Problem_Definition">
        <rdfs:subClassOf rdf:resource="https://hack.cybersystems.engineer/memex/ontologies/SeamlessDigitalEngineering#Problem_Definition"/>
        <rdfs:label xml:lang="en">Decision Support Problem Definition</rdfs:label>
    </owl:Class>
    


    <!-- https://hack.cybersystems.engineer/memex/ontologies/SeamlessDigitalEngineering#Defect -->

    <owl:Class rdf:about="https://hack.cybersystems.engineer/memex/ontologies/SeamlessDigitalEngineering#Defect">
        <rdfs:subClassOf rdf:resource="https://www.commoncoreontologies.org/ont00000997"/>
        <rdfs:subClassOf>
            <owl:Restriction>
                <owl:onProperty rdf:resource="http://purl.obolibrary.org/obo/BFO_0000197"/>
                <owl:someValuesFrom rdf:resource="https://hack.cybersystems.engineer/memex/ontologies/SeamlessDigitalEngineering#System"/>
            </owl:Restriction>
        </rdfs:subClassOf>
        <rdfs:label xml:lang="en">Defect</rdfs:label>
        <skos:definition xml:lang="en">Fault or deviation from the Performance Specification of a System or Software</skos:definition>
        <cco2:ont00001754>ISO/IEC/IEEE 41062:2024 — Software engineering — Life cycle processes — Software acquisition
ISO/IEC 23643:2020, 3.4</cco2:ont00001754>
    </owl:Class>
    


    <!-- https://hack.cybersystems.engineer/memex/ontologies/SeamlessDigitalEngineering#Design_Approach -->

    <owl:Class rdf:about="https://hack.cybersystems.engineer/memex/ontologies/SeamlessDigitalEngineering#Design_Approach">
        <owl:equivalentClass>
            <owl:Class>
                <owl:intersectionOf rdf:parseType="Collection">
                    <rdf:Description rdf:about="https://hack.cybersystems.engineer/memex/ontologies/SeamlessDigitalEngineering#Approach"/>
                    <owl:Restriction>
                        <owl:onProperty rdf:resource="https://www.commoncoreontologies.org/ont00001808"/>
                        <owl:someValuesFrom rdf:resource="https://www.commoncoreontologies.org/ont00000319"/>
                    </owl:Restriction>
                    <owl:Restriction>
                        <owl:onProperty rdf:resource="https://www.commoncoreontologies.org/ont00001942"/>
                        <owl:someValuesFrom rdf:resource="http://www.ontologyrepository.com/CommonCoreOntologies/ActOfArtifactCreation"/>
                    </owl:Restriction>
                </owl:intersectionOf>
            </owl:Class>
        </owl:equivalentClass>
        <rdfs:subClassOf rdf:resource="https://hack.cybersystems.engineer/memex/ontologies/SeamlessDigitalEngineering#Approach"/>
        <rdfs:label xml:lang="en">Design Approach</rdfs:label>
    </owl:Class>
    


    <!-- https://hack.cybersystems.engineer/memex/ontologies/SeamlessDigitalEngineering#Design_Authority_Role -->

    <owl:Class rdf:about="https://hack.cybersystems.engineer/memex/ontologies/SeamlessDigitalEngineering#Design_Authority_Role">
        <rdfs:subClassOf rdf:resource="https://www.commoncoreontologies.org/ont00000187"/>
        <rdfs:label xml:lang="en">Design Authority Role</rdfs:label>
        <skos:definition xml:lang="en">Authority Role that inheres in a Person or Organization that is responsible for the Artifact Design of the Product</skos:definition>
        <cco2:ont00001754 xml:lang="en">ISO/IEC/IEEE 15026-1:2019</cco2:ont00001754>
    </owl:Class>
    


    <!-- https://hack.cybersystems.engineer/memex/ontologies/SeamlessDigitalEngineering#Design_Definition_Process -->

    <owl:Class rdf:about="https://hack.cybersystems.engineer/memex/ontologies/SeamlessDigitalEngineering#Design_Definition_Process">
        <rdfs:subClassOf rdf:resource="https://hack.cybersystems.engineer/memex/ontologies/SeamlessDigitalEngineering#Technical_Process"/>
        <rdfs:label xml:lang="en">Design Definition Process</rdfs:label>
        <skos:definition xml:lang="en">The purpose of the design definition process is to provide sufficient detailed data and information about the system and its elements to realise the solution in accordance with the system requirements and architecture.</skos:definition>
        <cco2:ont00001754>ISO/IEC/IEEE 15288:2023</cco2:ont00001754>
    </owl:Class>
    


    <!-- https://hack.cybersystems.engineer/memex/ontologies/SeamlessDigitalEngineering#Design_Output_Specification -->

    <owl:Class rdf:about="https://hack.cybersystems.engineer/memex/ontologies/SeamlessDigitalEngineering#Design_Output_Specification">
        <rdfs:subClassOf rdf:resource="https://www.commoncoreontologies.org/ont00000319"/>
        <rdfs:label xml:lang="en">Design Output Specification</rdfs:label>
        <skos:definition xml:lang="en">The set of design characteristics described in a form suitable for implementation, design descriptions, end-item specifications, or technical data package (TDP) that include equipment lists, parts lists, drawings, wiring diagrams, plumbing diagrams, labeling diagrams and requirements, logic diagrams, algorithms, Computer-aided Design (CAD) files, STL files (for 3D printing), end-item specification requirements on the system to be manufactured or coded that can be thought of as the &quot;build-to/code-to&quot; requirements, and other design output artifacts.</skos:definition>
        <cco2:ont00001754 xml:lang="en">INCOSE Needs and Requirements Manual R1.1 (2022)</cco2:ont00001754>
    </owl:Class>
    


    <!-- https://hack.cybersystems.engineer/memex/ontologies/SeamlessDigitalEngineering#Developed_Assurance_Argument_Record -->

    <owl:Class rdf:about="https://hack.cybersystems.engineer/memex/ontologies/SeamlessDigitalEngineering#Developed_Assurance_Argument_Record">
        <owl:equivalentClass>
            <owl:Class>
                <owl:intersectionOf rdf:parseType="Collection">
                    <rdf:Description rdf:about="https://hack.cybersystems.engineer/memex/ontologies/SeamlessDigitalEngineering#Assurance_Argument_Record"/>
                    <owl:Class>
                        <owl:unionOf rdf:parseType="Collection">
                            <owl:Class>
                                <owl:intersectionOf rdf:parseType="Collection">
                                    <owl:Restriction>
                                        <owl:onProperty rdf:resource="http://purl.obolibrary.org/obo/BFO_0000101"/>
                                        <owl:someValuesFrom rdf:resource="https://hack.cybersystems.engineer/memex/ontologies/SeamlessDigitalEngineering#Supported_Assurance_Claim"/>
                                    </owl:Restriction>
                                    <owl:Restriction>
                                        <owl:onProperty rdf:resource="http://purl.obolibrary.org/obo/BFO_0000115"/>
                                        <owl:someValuesFrom rdf:resource="https://hack.cybersystems.engineer/memex/ontologies/SeamlessDigitalEngineering#Inference_Argument_Record"/>
                                    </owl:Restriction>
                                </owl:intersectionOf>
                            </owl:Class>
                            <owl:Restriction>
                                <owl:onProperty rdf:resource="http://purl.obolibrary.org/obo/BFO_0000115"/>
                                <owl:someValuesFrom rdf:resource="https://hack.cybersystems.engineer/memex/ontologies/SeamlessDigitalEngineering#Evidence_Report"/>
                            </owl:Restriction>
                        </owl:unionOf>
                    </owl:Class>
                    <owl:Restriction>
                        <owl:onProperty rdf:resource="http://purl.obolibrary.org/obo/BFO_0000115"/>
                        <owl:someValuesFrom rdf:resource="https://hack.cybersystems.engineer/memex/ontologies/SeamlessDigitalEngineering#Assurance_Context_List"/>
                    </owl:Restriction>
                </owl:intersectionOf>
            </owl:Class>
        </owl:equivalentClass>
        <rdfs:subClassOf rdf:resource="https://hack.cybersystems.engineer/memex/ontologies/SeamlessDigitalEngineering#Assurance_Argument_Record"/>
        <owl:disjointWith rdf:resource="https://hack.cybersystems.engineer/memex/ontologies/SeamlessDigitalEngineering#Undeveloped_Assurance_Argument_Record"/>
        <rdfs:label xml:lang="en">Developed Assurance Argument Record</rdfs:label>
        <skos:definition xml:lang="en">An Assurance Argument A that supports a claim C, is a pair consisting of:

1) a list of Assurance Context(s), and
2) either
    i) an Inference R with a list of supported claims SC1, SC2, SC3, ... SCn, where R derives C from the set of claims of SC1, SC2, SC3, ... SCn, or
    ii) a reference to an Evidence Item that supports the truth of C.</skos:definition>
        <skos:editorialNote xml:lang="en">A valid Developed Assurance Argument Record must have *exactly 1* Inference Argument Record. (OWL reasoner limitations)</skos:editorialNote>
        <cco2:ont00001754 xml:lang="en">ISO/IEC/IEEE 15026-2:2022</cco2:ont00001754>
    </owl:Class>
    


    <!-- https://hack.cybersystems.engineer/memex/ontologies/SeamlessDigitalEngineering#Developer -->

    <owl:Class rdf:about="https://hack.cybersystems.engineer/memex/ontologies/SeamlessDigitalEngineering#Developer">
        <owl:equivalentClass>
            <owl:Class>
                <owl:intersectionOf rdf:parseType="Collection">
                    <rdf:Description rdf:about="https://hack.cybersystems.engineer/memex/ontologies/SeamlessDigitalEngineering#Supplier"/>
                    <owl:Restriction>
                        <owl:onProperty rdf:resource="https://www.commoncoreontologies.org/ont00001787"/>
                        <owl:someValuesFrom rdf:resource="https://hack.cybersystems.engineer/memex/ontologies/SeamlessDigitalEngineering#Technical_Process"/>
                    </owl:Restriction>
                </owl:intersectionOf>
            </owl:Class>
        </owl:equivalentClass>
        <rdfs:subClassOf rdf:resource="https://hack.cybersystems.engineer/memex/ontologies/SeamlessDigitalEngineering#Supplier"/>
        <rdfs:label xml:lang="en">Developer</rdfs:label>
        <skos:definition xml:lang="en">Supplier responsible for the development of the Target of Evaluation</skos:definition>
        <cco2:ont00001754 xml:lang="en">ISO/IEC 15408-1:2022, 3.33</cco2:ont00001754>
    </owl:Class>
    


    <!-- https://hack.cybersystems.engineer/memex/ontologies/SeamlessDigitalEngineering#Developer_Action -->

    <owl:Class rdf:about="https://hack.cybersystems.engineer/memex/ontologies/SeamlessDigitalEngineering#Developer_Action">
        <owl:equivalentClass>
            <owl:Class>
                <owl:intersectionOf rdf:parseType="Collection">
                    <rdf:Description rdf:about="https://hack.cybersystems.engineer/memex/ontologies/SeamlessDigitalEngineering#Action"/>
                    <owl:Restriction>
                        <owl:onProperty rdf:resource="https://www.commoncoreontologies.org/ont00001778"/>
                        <owl:someValuesFrom rdf:resource="https://hack.cybersystems.engineer/memex/ontologies/SeamlessDigitalEngineering#Target_of_Evaluation"/>
                    </owl:Restriction>
                    <owl:Restriction>
                        <owl:onProperty rdf:resource="https://www.commoncoreontologies.org/ont00001833"/>
                        <owl:someValuesFrom rdf:resource="https://hack.cybersystems.engineer/memex/ontologies/SeamlessDigitalEngineering#Developer"/>
                    </owl:Restriction>
                    <owl:Restriction>
                        <owl:onProperty rdf:resource="https://www.commoncoreontologies.org/ont00001857"/>
                        <owl:someValuesFrom rdf:resource="https://hack.cybersystems.engineer/memex/ontologies/SeamlessDigitalEngineering#Technical_Process"/>
                    </owl:Restriction>
                </owl:intersectionOf>
            </owl:Class>
        </owl:equivalentClass>
        <rdfs:subClassOf rdf:resource="https://hack.cybersystems.engineer/memex/ontologies/SeamlessDigitalEngineering#Action"/>
        <rdfs:label xml:lang="en">Developer Action</rdfs:label>
        <skos:definition xml:lang="en">Action of an Developer</skos:definition>
    </owl:Class>
    


    <!-- https://hack.cybersystems.engineer/memex/ontologies/SeamlessDigitalEngineering#Development_Stage -->

    <owl:Class rdf:about="https://hack.cybersystems.engineer/memex/ontologies/SeamlessDigitalEngineering#Development_Stage">
        <owl:equivalentClass>
            <owl:Class>
                <owl:intersectionOf rdf:parseType="Collection">
                    <rdf:Description rdf:about="https://hack.cybersystems.engineer/memex/ontologies/SeamlessDigitalEngineering#Lifecycle_Stage"/>
                    <owl:Restriction>
                        <owl:onProperty rdf:resource="https://www.commoncoreontologies.org/ont00001921"/>
                        <owl:someValuesFrom rdf:resource="https://hack.cybersystems.engineer/memex/ontologies/SeamlessDigitalEngineering#Requirement_Set"/>
                    </owl:Restriction>
                    <owl:Restriction>
                        <owl:onProperty rdf:resource="https://www.commoncoreontologies.org/ont00001986"/>
                        <owl:someValuesFrom rdf:resource="https://hack.cybersystems.engineer/memex/ontologies/SeamlessDigitalEngineering#System_Architecture_Model"/>
                    </owl:Restriction>
                </owl:intersectionOf>
            </owl:Class>
        </owl:equivalentClass>
        <rdfs:subClassOf rdf:resource="https://hack.cybersystems.engineer/memex/ontologies/SeamlessDigitalEngineering#Lifecycle_Stage"/>
        <rdfs:comment xml:lang="en">Purpose: The development stage is executed to develop a SoI that meets stakeholder requirements and can be produced, tested, evaluated, operated, supported and retired.</rdfs:comment>
        <rdfs:label xml:lang="en">Development Stage</rdfs:label>
        <cco2:ont00001754>ISO/IEC/IEEE 24748-1:2024</cco2:ont00001754>
    </owl:Class>
    


    <!-- https://hack.cybersystems.engineer/memex/ontologies/SeamlessDigitalEngineering#Digital -->

    <owl:Class rdf:about="https://hack.cybersystems.engineer/memex/ontologies/SeamlessDigitalEngineering#Digital">
        <owl:equivalentClass>
            <owl:Class>
                <owl:intersectionOf rdf:parseType="Collection">
                    <rdf:Description rdf:about="http://purl.obolibrary.org/obo/BFO_0000016"/>
                    <owl:Restriction>
                        <owl:onProperty rdf:resource="http://purl.obolibrary.org/obo/BFO_0000054"/>
                        <owl:someValuesFrom rdf:resource="https://hack.cybersystems.engineer/memex/ontologies/SeamlessDigitalEngineering#Digital_Process"/>
                    </owl:Restriction>
                    <owl:Restriction>
                        <owl:onProperty rdf:resource="http://purl.obolibrary.org/obo/BFO_0000218"/>
                        <owl:someValuesFrom rdf:resource="https://hack.cybersystems.engineer/memex/ontologies/SeamlessDigitalEngineering#Data"/>
                    </owl:Restriction>
                </owl:intersectionOf>
            </owl:Class>
        </owl:equivalentClass>
        <rdfs:subClassOf rdf:resource="http://purl.obolibrary.org/obo/BFO_0000016"/>
        <rdfs:label xml:lang="en">Digital</rdfs:label>
        <skos:definition xml:lang="en">a disposition pertaining to Data that consists of digits</skos:definition>
        <cco2:ont00001754 xml:lang="en">derived from ISO/IEC/IEEE 24765:2017, 3.1206</cco2:ont00001754>
        <cco2:ont00001760 rdf:datatype="http://www.w3.org/2001/XMLSchema#anyURI">https://semantic.incose.org/DEIX_Ontology</cco2:ont00001760>
    </owl:Class>
    


    <!-- https://hack.cybersystems.engineer/memex/ontologies/SeamlessDigitalEngineering#Digital_Architecture_Description -->

    <owl:Class rdf:about="https://hack.cybersystems.engineer/memex/ontologies/SeamlessDigitalEngineering#Digital_Architecture_Description">
        <owl:equivalentClass>
            <owl:Class>
                <owl:intersectionOf rdf:parseType="Collection">
                    <rdf:Description rdf:about="https://hack.cybersystems.engineer/memex/ontologies/SeamlessDigitalEngineering#Architecture_Description"/>
                    <rdf:Description rdf:about="https://hack.cybersystems.engineer/memex/ontologies/SeamlessDigitalEngineering#Digital_Model"/>
                </owl:intersectionOf>
            </owl:Class>
        </owl:equivalentClass>
        <rdfs:subClassOf rdf:resource="https://hack.cybersystems.engineer/memex/ontologies/SeamlessDigitalEngineering#Digital_Model"/>
        <rdfs:comment xml:lang="en">It could be a Website, or special-purpose Software, or other Digital Object, indicating that the viewed content is linked directly to the System Architecture.</rdfs:comment>
        <rdfs:label xml:lang="en">Digital Architecture Description</rdfs:label>
        <skos:definition xml:lang="en">A structured, interactive digital portal for exploring an Architecture Description</skos:definition>
    </owl:Class>
    


    <!-- https://hack.cybersystems.engineer/memex/ontologies/SeamlessDigitalEngineering#Digital_Artifact -->

    <owl:Class rdf:about="https://hack.cybersystems.engineer/memex/ontologies/SeamlessDigitalEngineering#Digital_Artifact">
        <owl:equivalentClass>
            <owl:Class>
                <owl:intersectionOf rdf:parseType="Collection">
                    <rdf:Description rdf:about="http://www.ontologyrepository.com/CommonCoreOntologies/DigitalObject"/>
                    <owl:Restriction>
                        <owl:onProperty rdf:resource="http://purl.obolibrary.org/obo/BFO_0000129"/>
                        <owl:someValuesFrom rdf:resource="https://hack.cybersystems.engineer/memex/ontologies/SeamlessDigitalEngineering#Digital_Engineering_Environment"/>
                    </owl:Restriction>
                    <owl:Restriction>
                        <owl:onProperty rdf:resource="https://www.commoncoreontologies.org/ont00001816"/>
                        <owl:someValuesFrom rdf:resource="https://hack.cybersystems.engineer/memex/ontologies/SeamlessDigitalEngineering#Act_of_Digital_Engineering"/>
                    </owl:Restriction>
                </owl:intersectionOf>
            </owl:Class>
        </owl:equivalentClass>
        <rdfs:subClassOf rdf:resource="http://www.ontologyrepository.com/CommonCoreOntologies/DigitalObject"/>
        <rdfs:comment xml:lang="en">Digital Artifacts provide Data for alternative Views to visualize, communicate, and deliver Data, Information, and Knowledge to Stakeholders.

Soruce: https://www.dau.edu/glossary/digital-artifact</rdfs:comment>
        <rdfs:label xml:lang="en">Digital Artifact</rdfs:label>
        <skos:definition xml:lang="en">A Product or output, in Computer (i.e., digital) format, created within or generated from the Digital Engineering Environment.</skos:definition>
        <cco2:ont00001754 rdf:datatype="http://www.w3.org/2001/XMLSchema#anyURI">https://www.dau.edu/glossary/digital-artifact</cco2:ont00001754>
        <cco2:ont00001760 rdf:datatype="http://www.w3.org/2001/XMLSchema#anyURI">https://semantic.incose.org/DEIX_Ontology</cco2:ont00001760>
    </owl:Class>
    


    <!-- https://hack.cybersystems.engineer/memex/ontologies/SeamlessDigitalEngineering#Digital_Asset -->

    <owl:Class rdf:about="https://hack.cybersystems.engineer/memex/ontologies/SeamlessDigitalEngineering#Digital_Asset">
        <owl:equivalentClass>
            <owl:Class>
                <owl:intersectionOf rdf:parseType="Collection">
                    <rdf:Description rdf:about="https://hack.cybersystems.engineer/memex/ontologies/SeamlessDigitalEngineering#Asset"/>
                    <rdf:Description rdf:about="https://hack.cybersystems.engineer/memex/ontologies/SeamlessDigitalEngineering#Digital_Artifact"/>
                    <owl:Restriction>
                        <owl:onProperty rdf:resource="http://purl.obolibrary.org/obo/BFO_0000196"/>
                        <owl:someValuesFrom rdf:resource="https://hack.cybersystems.engineer/memex/ontologies/SeamlessDigitalEngineering#Source_of_Truth_Role"/>
                    </owl:Restriction>
                    <owl:Restriction>
                        <owl:onProperty rdf:resource="https://www.commoncoreontologies.org/ont00001816"/>
                        <owl:someValuesFrom rdf:resource="https://hack.cybersystems.engineer/memex/ontologies/SeamlessDigitalEngineering#Act_of_Model_Curation"/>
                    </owl:Restriction>
                    <owl:Restriction>
                        <owl:onProperty rdf:resource="https://www.commoncoreontologies.org/ont00001879"/>
                        <owl:someValuesFrom rdf:resource="https://www.commoncoreontologies.org/ont00000292"/>
                    </owl:Restriction>
                    <owl:Restriction>
                        <owl:onProperty rdf:resource="https://www.commoncoreontologies.org/ont00001904"/>
                        <owl:someValuesFrom rdf:resource="https://www.commoncoreontologies.org/ont00000592"/>
                    </owl:Restriction>
                    <owl:Restriction>
                        <owl:onProperty rdf:resource="https://www.commoncoreontologies.org/ont00001963"/>
                        <owl:someValuesFrom rdf:resource="https://www.commoncoreontologies.org/ont00000186"/>
                    </owl:Restriction>
                </owl:intersectionOf>
            </owl:Class>
        </owl:equivalentClass>
        <rdfs:subClassOf rdf:resource="https://hack.cybersystems.engineer/memex/ontologies/SeamlessDigitalEngineering#Digital_Artifact"/>
        <rdfs:label xml:lang="en">Digital Asset</rdfs:label>
        <skos:definition xml:lang="en">a curated, version-controlled Digital Artifact that carries accurate Information about an entity</skos:definition>
        <cco2:ont00001760 rdf:datatype="http://www.w3.org/2001/XMLSchema#anyURI">https://semantic.incose.org/DEIX_Ontology</cco2:ont00001760>
    </owl:Class>
    


    <!-- https://hack.cybersystems.engineer/memex/ontologies/SeamlessDigitalEngineering#Digital_Authoritative_Source_of_Truth -->

    <owl:Class rdf:about="https://hack.cybersystems.engineer/memex/ontologies/SeamlessDigitalEngineering#Digital_Authoritative_Source_of_Truth">
        <owl:equivalentClass>
            <owl:Class>
                <owl:intersectionOf rdf:parseType="Collection">
                    <rdf:Description rdf:about="https://hack.cybersystems.engineer/memex/ontologies/SeamlessDigitalEngineering#Digital_Asset"/>
                    <owl:Restriction>
                        <owl:onProperty rdf:resource="http://purl.obolibrary.org/obo/BFO_0000115"/>
                        <owl:someValuesFrom rdf:resource="https://hack.cybersystems.engineer/memex/ontologies/SeamlessDigitalEngineering#Digital_Model"/>
                    </owl:Restriction>
                    <owl:Restriction>
                        <owl:onProperty rdf:resource="http://purl.obolibrary.org/obo/BFO_0000196"/>
                        <owl:someValuesFrom rdf:resource="https://hack.cybersystems.engineer/memex/ontologies/SeamlessDigitalEngineering#Authoritative_Source_of_Truth_Role"/>
                    </owl:Restriction>
                </owl:intersectionOf>
            </owl:Class>
        </owl:equivalentClass>
        <rdfs:subClassOf rdf:resource="https://hack.cybersystems.engineer/memex/ontologies/SeamlessDigitalEngineering#Digital_Asset"/>
        <rdfs:comment xml:lang="en">Potential definition: A Digital Asset that provides Traceability and Authoritative Knowledge, Information, and Data, and which bears an Authoritative Source of Truth Role assigned by an Authority

Source: adapted from discussions by INCOSE DEIX Ontology WG</rdfs:comment>
        <rdfs:comment xml:lang="en">The reference point for models and data across the system life cycle. The authoritative source of truth provides traceability as the system evolves, capturing historical knowledge and connecting configuration-controlled versions of models and data.

Source: https://www.dau.edu/glossary/authoritative-source-truth</rdfs:comment>
        <rdfs:label xml:lang="en">Digital Authoritative Source of Truth</rdfs:label>
        <skos:altLabel xml:lang="en">Digital ASoT</skos:altLabel>
        <skos:definition xml:lang="en">A Digital Asset that bears an ASoT Role, where that ASoT Role has a defined ASoT context of a particular Act of Digital Engineering, and which carries at least one View that addresses particular Stakeholder Concern(s)</skos:definition>
        <cco2:ont00001754 xml:lang="en">INCOSE DEIX WG</cco2:ont00001754>
        <cco2:ont00001760 rdf:datatype="http://www.w3.org/2001/XMLSchema#anyURI">https://semantic.incose.org/DEIX_Ontology</cco2:ont00001760>
    </owl:Class>
    


    <!-- https://hack.cybersystems.engineer/memex/ontologies/SeamlessDigitalEngineering#Digital_Capability -->

    <owl:Class rdf:about="https://hack.cybersystems.engineer/memex/ontologies/SeamlessDigitalEngineering#Digital_Capability">
        <owl:equivalentClass>
            <owl:Class>
                <owl:intersectionOf rdf:parseType="Collection">
                    <rdf:Description rdf:about="https://hack.cybersystems.engineer/memex/ontologies/SeamlessDigitalEngineering#Capability"/>
                    <owl:Restriction>
                        <owl:onProperty rdf:resource="http://purl.obolibrary.org/obo/BFO_0000054"/>
                        <owl:someValuesFrom rdf:resource="https://www.commoncoreontologies.org/ont00001158"/>
                    </owl:Restriction>
                </owl:intersectionOf>
            </owl:Class>
        </owl:equivalentClass>
        <rdfs:subClassOf rdf:resource="https://hack.cybersystems.engineer/memex/ontologies/SeamlessDigitalEngineering#Capability"/>
        <rdfs:label xml:lang="en">Digital Capability</rdfs:label>
        <skos:definition xml:lang="en">A Capability that is realized by some Act of Data Transformation</skos:definition>
    </owl:Class>
    


    <!-- https://hack.cybersystems.engineer/memex/ontologies/SeamlessDigitalEngineering#Digital_Ecosystem -->

    <owl:Class rdf:about="https://hack.cybersystems.engineer/memex/ontologies/SeamlessDigitalEngineering#Digital_Ecosystem">
        <owl:equivalentClass>
            <owl:Class>
                <owl:intersectionOf rdf:parseType="Collection">
                    <owl:Restriction>
                        <owl:onProperty rdf:resource="http://purl.obolibrary.org/obo/BFO_0000178"/>
                        <owl:someValuesFrom>
                            <owl:Class>
                                <owl:intersectionOf rdf:parseType="Collection">
                                    <rdf:Description rdf:about="https://hack.cybersystems.engineer/memex/ontologies/SeamlessDigitalEngineering#Digital_Environment"/>
                                    <rdf:Description rdf:about="https://hack.cybersystems.engineer/memex/ontologies/SeamlessDigitalEngineering#Software_Product"/>
                                    <rdf:Description rdf:about="https://www.commoncoreontologies.org/ont00000509"/>
                                    <rdf:Description rdf:about="https://www.commoncoreontologies.org/ont00001180"/>
                                </owl:intersectionOf>
                            </owl:Class>
                        </owl:someValuesFrom>
                    </owl:Restriction>
                    <owl:Restriction>
                        <owl:onProperty rdf:resource="http://purl.obolibrary.org/obo/BFO_0000183"/>
                        <owl:someValuesFrom rdf:resource="https://www.commoncoreontologies.org/ont00000836"/>
                    </owl:Restriction>
                </owl:intersectionOf>
            </owl:Class>
        </owl:equivalentClass>
        <rdfs:subClassOf rdf:resource="https://hack.cybersystems.engineer/memex/ontologies/SeamlessDigitalEngineering#Ecosystem"/>
        <dc:date rdf:datatype="http://www.w3.org/2001/XMLSchema#dateTime">2024-06-21T12:50:04-0600</dc:date>
        <rdfs:comment xml:lang="en">Defined as a set of businesses functioning as a unit and interacting with a shared market for software and services, together with relationships among them. These relationships are frequently underpinned by a common technological platform and operate through the exchange of information, resources, and artifacts.

Source: https://en.wikipedia.org/wiki/Digital_ecosystem</rdfs:comment>
        <rdfs:label xml:lang="en">Digital Ecosystem</rdfs:label>
        <rdfs:seeAlso rdf:resource="https://en.wikipedia.org/wiki/Digital_ecosystem"/>
        <rdfs:seeAlso rdf:datatype="http://www.w3.org/2001/XMLSchema#anyURI">https://en.wikipedia.org/wiki/Software_ecosystem</rdfs:seeAlso>
        <skos:definition xml:lang="en">distributed, adaptive, open Socio-Technical System with properties of self-organization, scalability and sustainability inspired from natural ecosystems</skos:definition>
        <cco2:ont00001754 xml:lang="en">ISO/IEC TS 30105-9:2023, 3.3</cco2:ont00001754>
        <cco2:ont00001760 rdf:datatype="http://www.w3.org/2001/XMLSchema#anyURI">https://semantic.incose.org/DEIX_Ontology</cco2:ont00001760>
    </owl:Class>
    


    <!-- https://hack.cybersystems.engineer/memex/ontologies/SeamlessDigitalEngineering#Digital_Engineering_Approach -->

    <owl:Class rdf:about="https://hack.cybersystems.engineer/memex/ontologies/SeamlessDigitalEngineering#Digital_Engineering_Approach">
        <owl:equivalentClass>
            <owl:Class>
                <owl:intersectionOf rdf:parseType="Collection">
                    <rdf:Description rdf:about="https://hack.cybersystems.engineer/memex/ontologies/SeamlessDigitalEngineering#Engineering_Approach"/>
                    <owl:Restriction>
                        <owl:onProperty rdf:resource="https://www.commoncoreontologies.org/ont00001942"/>
                        <owl:someValuesFrom rdf:resource="https://hack.cybersystems.engineer/memex/ontologies/SeamlessDigitalEngineering#Act_of_Digital_Engineering"/>
                    </owl:Restriction>
                </owl:intersectionOf>
            </owl:Class>
        </owl:equivalentClass>
        <rdfs:subClassOf rdf:resource="https://hack.cybersystems.engineer/memex/ontologies/SeamlessDigitalEngineering#Engineering_Approach"/>
        <rdfs:label xml:lang="en">Digital Engineering Approach</rdfs:label>
        <skos:definition xml:lang="en">An integrated digital approach that uses authoritative sources of systems’ data and models as a continuum across Disciplines to support Lifecycle Activities from Concept Stage through Retirement Stage.</skos:definition>
        <cco2:ont00001754 rdf:datatype="http://www.w3.org/2001/XMLSchema#anyURI">https://www.dau.edu/glossary/digital-engineering</cco2:ont00001754>
        <cco2:ont00001760 rdf:datatype="http://www.w3.org/2001/XMLSchema#anyURI">https://semantic.incose.org/DEIX_Ontology</cco2:ont00001760>
    </owl:Class>
    


    <!-- https://hack.cybersystems.engineer/memex/ontologies/SeamlessDigitalEngineering#Digital_Engineering_Capability -->

    <owl:Class rdf:about="https://hack.cybersystems.engineer/memex/ontologies/SeamlessDigitalEngineering#Digital_Engineering_Capability">
        <owl:equivalentClass>
            <owl:Class>
                <owl:intersectionOf rdf:parseType="Collection">
                    <rdf:Description rdf:about="https://hack.cybersystems.engineer/memex/ontologies/SeamlessDigitalEngineering#Digital_Capability"/>
                    <owl:Restriction>
                        <owl:onProperty rdf:resource="http://purl.obolibrary.org/obo/BFO_0000054"/>
                        <owl:someValuesFrom rdf:resource="https://hack.cybersystems.engineer/memex/ontologies/SeamlessDigitalEngineering#Act_of_Digital_Engineering"/>
                    </owl:Restriction>
                </owl:intersectionOf>
            </owl:Class>
        </owl:equivalentClass>
        <rdfs:subClassOf rdf:resource="https://hack.cybersystems.engineer/memex/ontologies/SeamlessDigitalEngineering#Digital_Capability"/>
        <rdfs:label xml:lang="en">Digital Engineering Capability</rdfs:label>
        <skos:definition xml:lang="en">Capability to develop, validate, use, curate, and maintain technically accurate Digital Twins and Digital System Models at the appropriate level of fidelity to ensure test Activities adequately simulate the Operational Environment in which a System will be deployed.</skos:definition>
        <cco2:ont00001754 rdf:datatype="http://www.w3.org/2001/XMLSchema#anyURI">https://www.dau.edu/glossary/digital-engineering-capability</cco2:ont00001754>
    </owl:Class>
    


    <!-- https://hack.cybersystems.engineer/memex/ontologies/SeamlessDigitalEngineering#Digital_Engineering_Ecosystem -->

    <owl:Class rdf:about="https://hack.cybersystems.engineer/memex/ontologies/SeamlessDigitalEngineering#Digital_Engineering_Ecosystem">
        <owl:equivalentClass>
            <owl:Class>
                <owl:intersectionOf rdf:parseType="Collection">
                    <rdf:Description rdf:about="https://hack.cybersystems.engineer/memex/ontologies/SeamlessDigitalEngineering#Digital_Ecosystem"/>
                    <owl:Restriction>
                        <owl:onProperty rdf:resource="http://purl.obolibrary.org/obo/BFO_0000178"/>
                        <owl:someValuesFrom rdf:resource="https://hack.cybersystems.engineer/memex/ontologies/SeamlessDigitalEngineering#Digital_Engineering_Environment"/>
                    </owl:Restriction>
                </owl:intersectionOf>
            </owl:Class>
        </owl:equivalentClass>
        <rdfs:subClassOf rdf:resource="https://hack.cybersystems.engineer/memex/ontologies/SeamlessDigitalEngineering#Digital_Ecosystem"/>
        <rdfs:comment xml:lang="en">The Digital Engineering ecosystem can be vast, crossing engineering domain and organizational boundaries. The Digital Engineering ecosystem should be treated as an SoS and must be developed using SE good practices. The Digital Engineering ecosystem consists of the models, tools, processes, and people/roles that come together to develop the systems the organization cares about. The ecosystem can be broader than this, depending on the scope. For example, some organizations utilize their Digital Engineering ecosystems to support the operation of their systems. Others include cross-project libraries and methods in their Digital Engineering ecosystems, as well as interconnections with external Digital Engineering ecosystems across their supply chain.

Source: INCOSE Systems Engineering Handbook, Fifth Edition (2023)</rdfs:comment>
        <rdfs:label xml:lang="en">Digital Engineering Ecosystem</rdfs:label>
        <skos:definition xml:lang="en">A Digital Ecosystem encompassing some shared market(s) of Organizations and their Products and Services, whose Digital Environments, including Digital Engineering Environments, are networked to share Resources, Artifacts, and Information.</skos:definition>
        <cco2:ont00001760 rdf:datatype="http://www.w3.org/2001/XMLSchema#anyURI">https://semantic.incose.org/DEIX_Ontology</cco2:ont00001760>
    </owl:Class>
    


    <!-- https://hack.cybersystems.engineer/memex/ontologies/SeamlessDigitalEngineering#Digital_Engineering_Enterprise -->

    <owl:Class rdf:about="https://hack.cybersystems.engineer/memex/ontologies/SeamlessDigitalEngineering#Digital_Engineering_Enterprise">
        <owl:equivalentClass>
            <owl:Class>
                <owl:intersectionOf rdf:parseType="Collection">
                    <rdf:Description rdf:about="https://hack.cybersystems.engineer/memex/ontologies/SeamlessDigitalEngineering#Digital_Enterprise"/>
                    <owl:Restriction>
                        <owl:onProperty rdf:resource="https://www.commoncoreontologies.org/ont00001898"/>
                        <owl:someValuesFrom rdf:resource="https://hack.cybersystems.engineer/memex/ontologies/SeamlessDigitalEngineering#Digital_Engineering_Capability"/>
                    </owl:Restriction>
                </owl:intersectionOf>
            </owl:Class>
        </owl:equivalentClass>
        <rdfs:subClassOf rdf:resource="https://hack.cybersystems.engineer/memex/ontologies/SeamlessDigitalEngineering#Digital_Enterprise"/>
        <rdfs:label xml:lang="en">Digital Engineering Enterprise</rdfs:label>
    </owl:Class>
    


    <!-- https://hack.cybersystems.engineer/memex/ontologies/SeamlessDigitalEngineering#Digital_Engineering_Environment -->

    <owl:Class rdf:about="https://hack.cybersystems.engineer/memex/ontologies/SeamlessDigitalEngineering#Digital_Engineering_Environment">
        <owl:equivalentClass>
            <owl:Class>
                <owl:intersectionOf rdf:parseType="Collection">
                    <rdf:Description rdf:about="https://hack.cybersystems.engineer/memex/ontologies/SeamlessDigitalEngineering#Digital_Environment"/>
                    <owl:Restriction>
                        <owl:onProperty rdf:resource="http://purl.obolibrary.org/obo/BFO_0000115"/>
                        <owl:someValuesFrom rdf:resource="https://hack.cybersystems.engineer/memex/ontologies/SeamlessDigitalEngineering#Digital_Tool"/>
                    </owl:Restriction>
                    <owl:Restriction>
                        <owl:onProperty rdf:resource="http://purl.obolibrary.org/obo/BFO_0000183"/>
                        <owl:someValuesFrom rdf:resource="https://hack.cybersystems.engineer/memex/ontologies/SeamlessDigitalEngineering#Act_of_Digital_Engineering"/>
                    </owl:Restriction>
                </owl:intersectionOf>
            </owl:Class>
        </owl:equivalentClass>
        <rdfs:subClassOf rdf:resource="https://hack.cybersystems.engineer/memex/ontologies/SeamlessDigitalEngineering#Digital_Environment"/>
        <rdfs:label xml:lang="en">Digital Engineering Environment</rdfs:label>
        <rdfs:seeAlso rdf:resource="https://hack.cybersystems.engineer/memex/ontologies/SeamlessDigitalEngineering#Digital_Engineering_Ecosystem"/>
        <skos:definition xml:lang="en">The interconnected infrastructure and methodology (process, methods, and tools) used to store, access, analyze, and visualize evolving systems&apos; data and models to address the needs of the stakeholders.</skos:definition>
        <cco2:ont00001754 xml:lang="en">derived from https://www.dau.edu/glossary/digital-engineering-ecosystem</cco2:ont00001754>
        <cco2:ont00001760 rdf:datatype="http://www.w3.org/2001/XMLSchema#anyURI">https://semantic.incose.org/DEIX_Ontology</cco2:ont00001760>
    </owl:Class>
    


    <!-- https://hack.cybersystems.engineer/memex/ontologies/SeamlessDigitalEngineering#Digital_Engineering_Environment_Enterprise_Architecture -->

    <owl:Class rdf:about="https://hack.cybersystems.engineer/memex/ontologies/SeamlessDigitalEngineering#Digital_Engineering_Environment_Enterprise_Architecture">
        <owl:equivalentClass>
            <owl:Class>
                <owl:intersectionOf rdf:parseType="Collection">
                    <rdf:Description rdf:about="https://hack.cybersystems.engineer/memex/ontologies/SeamlessDigitalEngineering#Enterprise_Architecture"/>
                    <owl:Restriction>
                        <owl:onProperty rdf:resource="https://www.commoncoreontologies.org/ont00001942"/>
                        <owl:someValuesFrom rdf:resource="https://hack.cybersystems.engineer/memex/ontologies/SeamlessDigitalEngineering#Digital_Engineering_Environment"/>
                    </owl:Restriction>
                </owl:intersectionOf>
            </owl:Class>
        </owl:equivalentClass>
        <rdfs:subClassOf rdf:resource="https://hack.cybersystems.engineer/memex/ontologies/SeamlessDigitalEngineering#Enterprise_Architecture"/>
        <rdfs:label xml:lang="en">Digital Engineering Environment Enterprise Architecture</rdfs:label>
    </owl:Class>
    


    <!-- https://hack.cybersystems.engineer/memex/ontologies/SeamlessDigitalEngineering#Digital_Engineering_Environment_Reference_Architecture -->

    <owl:Class rdf:about="https://hack.cybersystems.engineer/memex/ontologies/SeamlessDigitalEngineering#Digital_Engineering_Environment_Reference_Architecture">
        <owl:equivalentClass>
            <owl:Restriction>
                <owl:onProperty rdf:resource="https://www.commoncoreontologies.org/ont00001942"/>
                <owl:someValuesFrom rdf:resource="https://hack.cybersystems.engineer/memex/ontologies/SeamlessDigitalEngineering#Digital_Engineering_Environment_Enterprise_Architecture"/>
            </owl:Restriction>
        </owl:equivalentClass>
        <rdfs:subClassOf rdf:resource="https://hack.cybersystems.engineer/memex/ontologies/SeamlessDigitalEngineering#Reference_Architecture"/>
        <rdfs:label xml:lang="en">Digital Engineering Environment Reference Architecture</rdfs:label>
    </owl:Class>
    


    <!-- https://hack.cybersystems.engineer/memex/ontologies/SeamlessDigitalEngineering#Digital_Enterprise -->

    <owl:Class rdf:about="https://hack.cybersystems.engineer/memex/ontologies/SeamlessDigitalEngineering#Digital_Enterprise">
        <owl:equivalentClass>
            <owl:Class>
                <owl:intersectionOf rdf:parseType="Collection">
                    <rdf:Description rdf:about="https://hack.cybersystems.engineer/memex/ontologies/SeamlessDigitalEngineering#Enterprise"/>
                    <owl:Restriction>
                        <owl:onProperty rdf:resource="http://purl.obolibrary.org/obo/BFO_0000115"/>
                        <owl:someValuesFrom rdf:resource="https://www.commoncoreontologies.org/ont00000700"/>
                    </owl:Restriction>
                    <owl:Restriction>
                        <owl:onProperty rdf:resource="https://www.commoncoreontologies.org/ont00001898"/>
                        <owl:someValuesFrom rdf:resource="https://hack.cybersystems.engineer/memex/ontologies/SeamlessDigitalEngineering#Digital_Capability"/>
                    </owl:Restriction>
                </owl:intersectionOf>
            </owl:Class>
        </owl:equivalentClass>
        <rdfs:subClassOf rdf:resource="https://hack.cybersystems.engineer/memex/ontologies/SeamlessDigitalEngineering#Enterprise"/>
        <rdfs:label xml:lang="en">Digital Enterprise</rdfs:label>
        <skos:altLabel xml:lang="en">Digital Firm</skos:altLabel>
        <skos:definition xml:lang="en">An Organization that has enabled core business relationships through Digital Networks.</skos:definition>
        <cco2:ont00001754 rdf:datatype="http://www.w3.org/2001/XMLSchema#anyURI">https://en.wikipedia.org/wiki/Digital_firm</cco2:ont00001754>
    </owl:Class>
    


    <!-- https://hack.cybersystems.engineer/memex/ontologies/SeamlessDigitalEngineering#Digital_Environment -->

    <owl:Class rdf:about="https://hack.cybersystems.engineer/memex/ontologies/SeamlessDigitalEngineering#Digital_Environment">
        <owl:equivalentClass>
            <owl:Class>
                <owl:intersectionOf rdf:parseType="Collection">
                    <owl:Restriction>
                        <owl:onProperty rdf:resource="http://purl.obolibrary.org/obo/BFO_0000115"/>
                        <owl:someValuesFrom>
                            <owl:Class>
                                <owl:intersectionOf rdf:parseType="Collection">
                                    <rdf:Description rdf:about="https://hack.cybersystems.engineer/memex/ontologies/SeamlessDigitalEngineering#Software_Product"/>
                                    <rdf:Description rdf:about="https://www.commoncoreontologies.org/ont00000420"/>
                                    <rdf:Description rdf:about="https://www.commoncoreontologies.org/ont00000700"/>
                                    <rdf:Description rdf:about="https://www.commoncoreontologies.org/ont00000756"/>
                                </owl:intersectionOf>
                            </owl:Class>
                        </owl:someValuesFrom>
                    </owl:Restriction>
                    <owl:Restriction>
                        <owl:onProperty rdf:resource="http://purl.obolibrary.org/obo/BFO_0000176"/>
                        <owl:someValuesFrom rdf:resource="https://www.commoncoreontologies.org/ont00001180"/>
                    </owl:Restriction>
                    <owl:Restriction>
                        <owl:onProperty rdf:resource="http://purl.obolibrary.org/obo/BFO_0000183"/>
                        <owl:someValuesFrom rdf:resource="https://hack.cybersystems.engineer/memex/ontologies/SeamlessDigitalEngineering#Computing_Process"/>
                    </owl:Restriction>
                    <owl:Restriction>
                        <owl:onProperty rdf:resource="https://www.commoncoreontologies.org/ont00001852"/>
                        <owl:someValuesFrom rdf:resource="https://hack.cybersystems.engineer/memex/ontologies/SeamlessDigitalEngineering#Activity"/>
                    </owl:Restriction>
                    <owl:Restriction>
                        <owl:onProperty rdf:resource="https://www.commoncoreontologies.org/ont00001925"/>
                        <owl:someValuesFrom rdf:resource="https://hack.cybersystems.engineer/memex/ontologies/SeamlessDigitalEngineering#User"/>
                    </owl:Restriction>
                </owl:intersectionOf>
            </owl:Class>
        </owl:equivalentClass>
        <rdfs:subClassOf rdf:resource="https://hack.cybersystems.engineer/memex/ontologies/SeamlessDigitalEngineering#System-of-Systems"/>
        <dc:date rdf:datatype="http://www.w3.org/2001/XMLSchema#dateTime">2024-06-21T12:50:04-0600</dc:date>
        <rdfs:comment xml:lang="en">May be a System Environment if a Software System is deployed to the Digital Environment. Otherwise, it may be the SoI itself.</rdfs:comment>
        <rdfs:comment xml:lang="en">The concept is based on digital electronics systems which are integrated and implemented for a global community.</rdfs:comment>
        <rdfs:label xml:lang="en">Digital Environment</rdfs:label>
        <skos:definition xml:lang="en">an integrated communications environment where digital devices communicate and manage the content and activities within it.</skos:definition>
        <skos:example xml:lang="en">Major components of a digital environment generally include websites, cloud servers, search engines, social media outlets, mobile apps, audio and video, and other web-based resources.</skos:example>
        <cco2:ont00001754 rdf:resource="https://en.wikipedia.org/wiki/Digital_environments"/>
        <cco2:ont00001760 rdf:datatype="http://www.w3.org/2001/XMLSchema#anyURI">https://semantic.incose.org/DEIX_Ontology</cco2:ont00001760>
    </owl:Class>
    


    <!-- https://hack.cybersystems.engineer/memex/ontologies/SeamlessDigitalEngineering#Digital_Information -->

    <owl:Class rdf:about="https://hack.cybersystems.engineer/memex/ontologies/SeamlessDigitalEngineering#Digital_Information">
        <owl:equivalentClass>
            <owl:Class>
                <owl:intersectionOf rdf:parseType="Collection">
                    <rdf:Description rdf:about="https://hack.cybersystems.engineer/memex/ontologies/SeamlessDigitalEngineering#Data"/>
                    <owl:Class>
                        <owl:unionOf rdf:parseType="Collection">
                            <owl:Restriction>
                                <owl:onProperty rdf:resource="https://www.commoncoreontologies.org/ont00001816"/>
                                <owl:someValuesFrom rdf:resource="https://www.commoncoreontologies.org/ont00000366"/>
                            </owl:Restriction>
                            <owl:Restriction>
                                <owl:onProperty rdf:resource="https://www.commoncoreontologies.org/ont00001841"/>
                                <owl:someValuesFrom rdf:resource="https://www.commoncoreontologies.org/ont00000366"/>
                            </owl:Restriction>
                        </owl:unionOf>
                    </owl:Class>
                </owl:intersectionOf>
            </owl:Class>
        </owl:equivalentClass>
        <rdfs:subClassOf rdf:resource="https://hack.cybersystems.engineer/memex/ontologies/SeamlessDigitalEngineering#Data"/>
        <rdfs:label xml:lang="en">Digital Information</rdfs:label>
        <skos:definition xml:lang="en">Data that are processed, organized and correlated to produce meaning</skos:definition>
        <cco2:ont00001754 xml:lang="en">ISO 5127:2017 — Information and documentation — Foundation and vocabulary, 3.1.1.16</cco2:ont00001754>
        <cco2:ont00001760 rdf:datatype="http://www.w3.org/2001/XMLSchema#anyURI">https://semantic.incose.org/DEIX_Ontology</cco2:ont00001760>
    </owl:Class>
    


    <!-- https://hack.cybersystems.engineer/memex/ontologies/SeamlessDigitalEngineering#Digital_Infrastructure -->

    <owl:Class rdf:about="https://hack.cybersystems.engineer/memex/ontologies/SeamlessDigitalEngineering#Digital_Infrastructure">
        <rdfs:subClassOf rdf:resource="https://www.commoncoreontologies.org/ont00000954"/>
        <rdfs:subClassOf>
            <owl:Restriction>
                <owl:onProperty rdf:resource="http://purl.obolibrary.org/obo/BFO_0000178"/>
                <owl:someValuesFrom rdf:resource="https://hack.cybersystems.engineer/memex/ontologies/SeamlessDigitalEngineering#Digital_Environment"/>
            </owl:Restriction>
        </rdfs:subClassOf>
        <rdfs:label xml:lang="en">Digital Infrastructure</rdfs:label>
        <skos:definition xml:lang="en">Digital Environment to support Computer System and Software design, development, and modification</skos:definition>
        <cco2:ont00001754 xml:lang="en">derived from ISO/IEC/IEEE 12207:2017, 3.1.25</cco2:ont00001754>
    </owl:Class>
    


    <!-- https://hack.cybersystems.engineer/memex/ontologies/SeamlessDigitalEngineering#Digital_Instance -->

    <owl:Class rdf:about="https://hack.cybersystems.engineer/memex/ontologies/SeamlessDigitalEngineering#Digital_Instance">
        <rdfs:subClassOf rdf:resource="https://hack.cybersystems.engineer/memex/ontologies/SeamlessDigitalEngineering#Digital_Twin"/>
        <owl:disjointWith rdf:resource="https://hack.cybersystems.engineer/memex/ontologies/SeamlessDigitalEngineering#Digital_Prototype"/>
        <rdfs:comment xml:lang="en">A virtual replica of the physical configuration of an existing entity. The digital instance typically exists to replicate each individual configuration of a product as-built or as-maintained.

Source: https://www.dau.edu/glossary/digital-instance</rdfs:comment>
        <rdfs:label xml:lang="en">Digital Instance</rdfs:label>
        <cco2:ont00001760 rdf:datatype="http://www.w3.org/2001/XMLSchema#anyURI">https://semantic.incose.org/DEIX_Ontology</cco2:ont00001760>
    </owl:Class>
    


    <!-- https://hack.cybersystems.engineer/memex/ontologies/SeamlessDigitalEngineering#Digital_Laboratory_Environment -->

    <owl:Class rdf:about="https://hack.cybersystems.engineer/memex/ontologies/SeamlessDigitalEngineering#Digital_Laboratory_Environment">
        <owl:equivalentClass>
            <owl:Class>
                <owl:intersectionOf rdf:parseType="Collection">
                    <rdf:Description rdf:about="https://hack.cybersystems.engineer/memex/ontologies/SeamlessDigitalEngineering#Digital_Engineering_Environment"/>
                    <owl:Restriction>
                        <owl:onProperty rdf:resource="http://purl.obolibrary.org/obo/BFO_0000183"/>
                        <owl:someValuesFrom rdf:resource="https://hack.cybersystems.engineer/memex/ontologies/SeamlessDigitalEngineering#Act_of_Science"/>
                    </owl:Restriction>
                    <owl:Restriction>
                        <owl:onProperty rdf:resource="https://www.commoncoreontologies.org/ont00001925"/>
                        <owl:someValuesFrom rdf:resource="https://hack.cybersystems.engineer/memex/ontologies/SeamlessDigitalEngineering#Scientist"/>
                    </owl:Restriction>
                </owl:intersectionOf>
            </owl:Class>
        </owl:equivalentClass>
        <rdfs:subClassOf rdf:resource="https://hack.cybersystems.engineer/memex/ontologies/SeamlessDigitalEngineering#Digital_Engineering_Environment"/>
        <rdfs:label xml:lang="en">Digital Laboratory Environment</rdfs:label>
    </owl:Class>
    


    <!-- https://hack.cybersystems.engineer/memex/ontologies/SeamlessDigitalEngineering#Digital_Model -->

    <owl:Class rdf:about="https://hack.cybersystems.engineer/memex/ontologies/SeamlessDigitalEngineering#Digital_Model">
        <owl:equivalentClass>
            <owl:Class>
                <owl:intersectionOf rdf:parseType="Collection">
                    <rdf:Description rdf:about="https://hack.cybersystems.engineer/memex/ontologies/SeamlessDigitalEngineering#Digital_Artifact"/>
                    <owl:Restriction>
                        <owl:onProperty rdf:resource="http://purl.obolibrary.org/obo/BFO_0000101"/>
                        <owl:someValuesFrom rdf:resource="https://www.commoncoreontologies.org/ont00000965"/>
                    </owl:Restriction>
                </owl:intersectionOf>
            </owl:Class>
        </owl:equivalentClass>
        <rdfs:subClassOf rdf:resource="https://hack.cybersystems.engineer/memex/ontologies/SeamlessDigitalEngineering#Digital_Artifact"/>
        <rdfs:comment xml:lang="en">The representation can include form, attributes, and functions and may be depicted visually or described via mathematical or logical expressions.</rdfs:comment>
        <rdfs:label xml:lang="en">Digital Model</rdfs:label>
        <skos:definition xml:lang="en">A Digital Artifact that carries a Directive ICE of an object, phenomenon, process, or System.</skos:definition>
        <skos:editorialNote xml:lang="en">Since Digital Representation carries a Representational ICE, it is fitting that Digital Model carries a Directive ICE, despite the definition in the literature saying that a Digital Model is a representation.</skos:editorialNote>
        <cco2:ont00001754 xml:lang="en">derived from https://www.dau.edu/glossary/digital-model</cco2:ont00001754>
        <cco2:ont00001760 rdf:datatype="http://www.w3.org/2001/XMLSchema#anyURI">https://semantic.incose.org/DEIX_Ontology</cco2:ont00001760>
    </owl:Class>
    


    <!-- https://hack.cybersystems.engineer/memex/ontologies/SeamlessDigitalEngineering#Digital_Object_Reference_Field -->

    <owl:Class rdf:about="https://hack.cybersystems.engineer/memex/ontologies/SeamlessDigitalEngineering#Digital_Object_Reference_Field">
        <owl:equivalentClass>
            <owl:Class>
                <owl:intersectionOf rdf:parseType="Collection">
                    <rdf:Description rdf:about="https://www.commoncoreontologies.org/ont00000253"/>
                    <owl:Restriction>
                        <owl:onProperty rdf:resource="http://purl.obolibrary.org/obo/BFO_0000101"/>
                        <owl:someValuesFrom rdf:resource="https://hack.cybersystems.engineer/memex/ontologies/SeamlessDigitalEngineering#Object_Reference"/>
                    </owl:Restriction>
                    <owl:Restriction>
                        <owl:onProperty rdf:resource="http://purl.obolibrary.org/obo/BFO_0000176"/>
                        <owl:someValuesFrom rdf:resource="http://www.ontologyrepository.com/CommonCoreOntologies/DigitalObject"/>
                    </owl:Restriction>
                </owl:intersectionOf>
            </owl:Class>
        </owl:equivalentClass>
        <rdfs:subClassOf rdf:resource="https://www.commoncoreontologies.org/ont00000253"/>
        <rdfs:label xml:lang="en">Digital Object Reference Field</rdfs:label>
        <skos:definition xml:lang="en">An Information Bearing Entity upon which a Digital Object Reference generically depends.</skos:definition>
    </owl:Class>
    


    <!-- https://hack.cybersystems.engineer/memex/ontologies/SeamlessDigitalEngineering#Digital_Process -->

    <owl:Class rdf:about="https://hack.cybersystems.engineer/memex/ontologies/SeamlessDigitalEngineering#Digital_Process">
        <owl:equivalentClass>
            <owl:Class>
                <owl:intersectionOf rdf:parseType="Collection">
                    <rdf:Description rdf:about="https://www.commoncoreontologies.org/ont00000110"/>
                    <owl:Restriction>
                        <owl:onProperty rdf:resource="https://www.commoncoreontologies.org/ont00001949"/>
                        <owl:someValuesFrom rdf:resource="https://hack.cybersystems.engineer/memex/ontologies/SeamlessDigitalEngineering#Data"/>
                    </owl:Restriction>
                </owl:intersectionOf>
            </owl:Class>
        </owl:equivalentClass>
        <rdfs:subClassOf rdf:resource="https://www.commoncoreontologies.org/ont00000110"/>
        <rdfs:label xml:lang="en">Digital Process</rdfs:label>
        <skos:definition xml:lang="en">a Mechanical Process that uses Data</skos:definition>
        <skos:editorialNote xml:lang="en">TBD: May substitute &apos;Computer Program Execution&apos;, or be a synonym of it, to avoid importing Common Core Cyber Ontology</skos:editorialNote>
        <cco2:ont00001754 xml:lang="en">derived from ISO/IEC/IEEE 24765:2017, 3.1206</cco2:ont00001754>
        <cco2:ont00001760 rdf:datatype="http://www.w3.org/2001/XMLSchema#anyURI">https://semantic.incose.org/DEIX_Ontology</cco2:ont00001760>
    </owl:Class>
    


    <!-- https://hack.cybersystems.engineer/memex/ontologies/SeamlessDigitalEngineering#Digital_Prototype -->

    <owl:Class rdf:about="https://hack.cybersystems.engineer/memex/ontologies/SeamlessDigitalEngineering#Digital_Prototype">
        <rdfs:subClassOf rdf:resource="https://hack.cybersystems.engineer/memex/ontologies/SeamlessDigitalEngineering#Digital_Twin"/>
        <rdfs:comment xml:lang="en">An integrated multi-physics, multiscale, probabilistic model of a system design. The digital prototype may use sensor information and input data to simulate the performance of its corresponding physical twin. The digital prototype may exist prior to realization of its physical counterpart.

Source: https://www.dau.edu/glossary/digital-prototype</rdfs:comment>
        <rdfs:label xml:lang="en">Digital Prototype</rdfs:label>
        <cco2:ont00001760 rdf:datatype="http://www.w3.org/2001/XMLSchema#anyURI">https://semantic.incose.org/DEIX_Ontology</cco2:ont00001760>
    </owl:Class>
    


    <!-- https://hack.cybersystems.engineer/memex/ontologies/SeamlessDigitalEngineering#Digital_Quality_Engineering_Approach -->

    <owl:Class rdf:about="https://hack.cybersystems.engineer/memex/ontologies/SeamlessDigitalEngineering#Digital_Quality_Engineering_Approach">
        <owl:equivalentClass>
            <owl:Class>
                <owl:intersectionOf rdf:parseType="Collection">
                    <rdf:Description rdf:about="https://hack.cybersystems.engineer/memex/ontologies/SeamlessDigitalEngineering#Digital_Engineering_Approach"/>
                    <owl:Restriction>
                        <owl:onProperty rdf:resource="http://purl.obolibrary.org/obo/BFO_0000084"/>
                        <owl:someValuesFrom rdf:resource="http://www.ontologyrepository.com/CommonCoreOntologies/Ontology"/>
                    </owl:Restriction>
                    <owl:Restriction>
                        <owl:onProperty rdf:resource="http://purl.obolibrary.org/obo/BFO_0000178"/>
                        <owl:someValuesFrom rdf:resource="https://hack.cybersystems.engineer/memex/ontologies/SeamlessDigitalEngineering#High-Integrity_Level"/>
                    </owl:Restriction>
                    <owl:Restriction>
                        <owl:onProperty rdf:resource="https://www.commoncoreontologies.org/ont00001942"/>
                        <owl:someValuesFrom rdf:resource="https://hack.cybersystems.engineer/memex/ontologies/SeamlessDigitalEngineering#Act_of_Quality_Engineering"/>
                    </owl:Restriction>
                </owl:intersectionOf>
            </owl:Class>
        </owl:equivalentClass>
        <rdfs:subClassOf rdf:resource="https://hack.cybersystems.engineer/memex/ontologies/SeamlessDigitalEngineering#Digital_Engineering_Approach"/>
        <rdfs:label xml:lang="en">Digital Quality Engineering Approach</rdfs:label>
    </owl:Class>
    


    <!-- https://hack.cybersystems.engineer/memex/ontologies/SeamlessDigitalEngineering#Digital_Realm -->

    <owl:Class rdf:about="https://hack.cybersystems.engineer/memex/ontologies/SeamlessDigitalEngineering#Digital_Realm">
        <owl:equivalentClass>
            <owl:Class>
                <owl:intersectionOf rdf:parseType="Collection">
                    <rdf:Description rdf:about="https://www.commoncoreontologies.org/ont00000591"/>
                    <owl:Restriction>
                        <owl:onProperty rdf:resource="http://purl.obolibrary.org/obo/BFO_0000124"/>
                        <owl:someValuesFrom rdf:resource="http://www.ontologyrepository.com/CommonCoreOntologies/DigitalObject"/>
                    </owl:Restriction>
                </owl:intersectionOf>
            </owl:Class>
        </owl:equivalentClass>
        <rdfs:subClassOf rdf:resource="https://www.commoncoreontologies.org/ont00000591"/>
        <rdfs:label xml:lang="en">An Artifact Location of a Digital Object(s).</rdfs:label>
        <rdfs:label xml:lang="en">Digital Realm</rdfs:label>
        <cco2:ont00001760 rdf:datatype="http://www.w3.org/2001/XMLSchema#anyURI">https://semantic.incose.org/DEIX_Ontology</cco2:ont00001760>
    </owl:Class>
    


    <!-- https://hack.cybersystems.engineer/memex/ontologies/SeamlessDigitalEngineering#Digital_Repository -->

    <owl:Class rdf:about="https://hack.cybersystems.engineer/memex/ontologies/SeamlessDigitalEngineering#Digital_Repository">
        <owl:equivalentClass>
            <owl:Class>
                <owl:intersectionOf rdf:parseType="Collection">
                    <rdf:Description rdf:about="https://www.commoncoreontologies.org/ont00000756"/>
                    <owl:Restriction>
                        <owl:onProperty rdf:resource="http://purl.obolibrary.org/obo/BFO_0000101"/>
                        <owl:someValuesFrom rdf:resource="https://www.commoncoreontologies.org/ont00000186"/>
                    </owl:Restriction>
                    <owl:Restriction>
                        <owl:onProperty rdf:resource="http://purl.obolibrary.org/obo/BFO_0000115"/>
                        <owl:someValuesFrom rdf:resource="https://hack.cybersystems.engineer/memex/ontologies/SeamlessDigitalEngineering#Digital_Artifact"/>
                    </owl:Restriction>
                </owl:intersectionOf>
            </owl:Class>
        </owl:equivalentClass>
        <rdfs:subClassOf rdf:resource="https://www.commoncoreontologies.org/ont00000756"/>
        <rdfs:label xml:lang="en">Digital Repository</rdfs:label>
        <skos:definition xml:lang="en">a change-controlled Database that contains Digital Artifacts</skos:definition>
        <cco2:ont00001760 rdf:datatype="http://www.w3.org/2001/XMLSchema#anyURI">https://semantic.incose.org/DEIX_Ontology</cco2:ont00001760>
    </owl:Class>
    


    <!-- https://hack.cybersystems.engineer/memex/ontologies/SeamlessDigitalEngineering#Digital_Representation -->

    <owl:Class rdf:about="https://hack.cybersystems.engineer/memex/ontologies/SeamlessDigitalEngineering#Digital_Representation">
        <owl:equivalentClass>
            <owl:Class>
                <owl:intersectionOf rdf:parseType="Collection">
                    <rdf:Description rdf:about="https://hack.cybersystems.engineer/memex/ontologies/SeamlessDigitalEngineering#Digital_Model"/>
                    <owl:Restriction>
                        <owl:onProperty rdf:resource="http://purl.obolibrary.org/obo/BFO_0000101"/>
                        <owl:someValuesFrom>
                            <owl:Restriction>
                                <owl:onProperty rdf:resource="https://www.commoncoreontologies.org/ont00001938"/>
                                <owl:someValuesFrom rdf:resource="https://hack.cybersystems.engineer/memex/ontologies/SeamlessDigitalEngineering#Observable_Element"/>
                            </owl:Restriction>
                        </owl:someValuesFrom>
                    </owl:Restriction>
                </owl:intersectionOf>
            </owl:Class>
        </owl:equivalentClass>
        <rdfs:subClassOf rdf:resource="https://hack.cybersystems.engineer/memex/ontologies/SeamlessDigitalEngineering#Digital_Model"/>
        <rdfs:label xml:lang="en">Digital Representation</rdfs:label>
        <skos:altLabel xml:lang="en">Virtual Representation</skos:altLabel>
        <skos:definition xml:lang="en">A Digital Model representing either a set of properties or Behaviours or both of one or more Observable Elements</skos:definition>
        <skos:editorialNote xml:lang="en">The more general definition from ISO/IEC 30173:2023 is used here, instead of the one focused on Observable Manufacturing Element from ISO 23247-1:2021.</skos:editorialNote>
        <cco2:ont00001754 xml:lang="en">ISO/IEC 30173:2023 - Digital twin — Concepts and terminology</cco2:ont00001754>
        <cco2:ont00001760 rdf:datatype="http://www.w3.org/2001/XMLSchema#anyURI">https://semantic.incose.org/DEIX_Ontology</cco2:ont00001760>
    </owl:Class>
    


    <!-- https://hack.cybersystems.engineer/memex/ontologies/SeamlessDigitalEngineering#Digital_Requirements_Engineering_Approach -->

    <owl:Class rdf:about="https://hack.cybersystems.engineer/memex/ontologies/SeamlessDigitalEngineering#Digital_Requirements_Engineering_Approach">
        <owl:equivalentClass>
            <owl:Class>
                <owl:intersectionOf rdf:parseType="Collection">
                    <rdf:Description rdf:about="https://hack.cybersystems.engineer/memex/ontologies/SeamlessDigitalEngineering#Digital_Engineering_Approach"/>
                    <owl:Restriction>
                        <owl:onProperty rdf:resource="http://purl.obolibrary.org/obo/BFO_0000084"/>
                        <owl:someValuesFrom rdf:resource="http://www.ontologyrepository.com/CommonCoreOntologies/Ontology"/>
                    </owl:Restriction>
                    <owl:Restriction>
                        <owl:onProperty rdf:resource="https://www.commoncoreontologies.org/ont00001942"/>
                        <owl:someValuesFrom rdf:resource="https://hack.cybersystems.engineer/memex/ontologies/SeamlessDigitalEngineering#Act_of_Requirements_Engineering"/>
                    </owl:Restriction>
                </owl:intersectionOf>
            </owl:Class>
        </owl:equivalentClass>
        <rdfs:subClassOf rdf:resource="https://hack.cybersystems.engineer/memex/ontologies/SeamlessDigitalEngineering#Digital_Engineering_Approach"/>
        <rdfs:label xml:lang="en">Digital Requirements Engineering Approach</rdfs:label>
    </owl:Class>
    


    <!-- https://hack.cybersystems.engineer/memex/ontologies/SeamlessDigitalEngineering#Digital_System_Environment -->

    <owl:Class rdf:about="https://hack.cybersystems.engineer/memex/ontologies/SeamlessDigitalEngineering#Digital_System_Environment">
        <owl:equivalentClass>
            <owl:Class>
                <owl:intersectionOf rdf:parseType="Collection">
                    <rdf:Description rdf:about="https://hack.cybersystems.engineer/memex/ontologies/SeamlessDigitalEngineering#System_Environment"/>
                    <owl:Restriction>
                        <owl:onProperty rdf:resource="http://purl.obolibrary.org/obo/BFO_0000183"/>
                        <owl:someValuesFrom rdf:resource="https://hack.cybersystems.engineer/memex/ontologies/SeamlessDigitalEngineering#Digital_System_Lifecycle"/>
                    </owl:Restriction>
                </owl:intersectionOf>
            </owl:Class>
        </owl:equivalentClass>
        <rdfs:subClassOf rdf:resource="https://hack.cybersystems.engineer/memex/ontologies/SeamlessDigitalEngineering#System_Environment"/>
        <rdfs:label xml:lang="en">Digital System Environment</rdfs:label>
    </owl:Class>
    


    <!-- https://hack.cybersystems.engineer/memex/ontologies/SeamlessDigitalEngineering#Digital_System_Lifecycle -->

    <owl:Class rdf:about="https://hack.cybersystems.engineer/memex/ontologies/SeamlessDigitalEngineering#Digital_System_Lifecycle">
        <owl:equivalentClass>
            <owl:Class>
                <owl:intersectionOf rdf:parseType="Collection">
                    <rdf:Description rdf:about="https://hack.cybersystems.engineer/memex/ontologies/SeamlessDigitalEngineering#Lifecycle"/>
                    <owl:Restriction>
                        <owl:onProperty rdf:resource="http://purl.obolibrary.org/obo/BFO_0000184"/>
                        <owl:someValuesFrom>
                            <owl:Class>
                                <owl:unionOf rdf:parseType="Collection">
                                    <rdf:Description rdf:about="http://www.ontologyrepository.com/CommonCoreOntologies/ComputerAggregate"/>
                                    <rdf:Description rdf:about="http://www.ontologyrepository.com/CommonCoreOntologies/ComputerSystem"/>
                                </owl:unionOf>
                            </owl:Class>
                        </owl:someValuesFrom>
                    </owl:Restriction>
                </owl:intersectionOf>
            </owl:Class>
        </owl:equivalentClass>
        <rdfs:subClassOf rdf:resource="https://hack.cybersystems.engineer/memex/ontologies/SeamlessDigitalEngineering#Lifecycle"/>
        <rdfs:label xml:lang="en">Digital System Lifecycle</rdfs:label>
    </owl:Class>
    


    <!-- https://hack.cybersystems.engineer/memex/ontologies/SeamlessDigitalEngineering#Digital_System_Model -->

    <owl:Class rdf:about="https://hack.cybersystems.engineer/memex/ontologies/SeamlessDigitalEngineering#Digital_System_Model">
        <owl:equivalentClass>
            <owl:Class>
                <owl:intersectionOf rdf:parseType="Collection">
                    <rdf:Description rdf:about="https://hack.cybersystems.engineer/memex/ontologies/SeamlessDigitalEngineering#Digital_Representation"/>
                    <owl:Restriction>
                        <owl:onProperty rdf:resource="http://purl.obolibrary.org/obo/BFO_0000101"/>
                        <owl:someValuesFrom rdf:resource="https://hack.cybersystems.engineer/memex/ontologies/SeamlessDigitalEngineering#System_Model"/>
                    </owl:Restriction>
                    <owl:Restriction>
                        <owl:onProperty rdf:resource="http://purl.obolibrary.org/obo/BFO_0000101"/>
                        <owl:someValuesFrom rdf:resource="https://www.commoncoreontologies.org/ont00000686"/>
                    </owl:Restriction>
                    <owl:Restriction>
                        <owl:onProperty rdf:resource="http://purl.obolibrary.org/obo/BFO_0000101"/>
                        <owl:someValuesFrom rdf:resource="https://www.commoncoreontologies.org/ont00000853"/>
                    </owl:Restriction>
                    <owl:Restriction>
                        <owl:onProperty rdf:resource="http://purl.obolibrary.org/obo/BFO_0000115"/>
                        <owl:someValuesFrom rdf:resource="https://hack.cybersystems.engineer/memex/ontologies/SeamlessDigitalEngineering#Digital_View"/>
                    </owl:Restriction>
                </owl:intersectionOf>
            </owl:Class>
        </owl:equivalentClass>
        <rdfs:subClassOf rdf:resource="https://hack.cybersystems.engineer/memex/ontologies/SeamlessDigitalEngineering#Digital_Representation"/>
        <rdfs:comment xml:lang="en">In MBSE and Digital Engineering, a Digital System Model is a digital representation of a system. It integrates the authoritative MBSE and other Digital Engineering technical data and associated artifacts, defining all aspects of the system throughout the system life cycle. The Digital System Model is composed of a federated set of models that serve as an authoritative source of truth (ASOT) for the system’s design. Digital Engineering leverages MBSE and the Digital System Model to enable digital threads and digital twins.

Source: INCOSE Systems Engineering Handbook, Fifth Edition</rdfs:comment>
        <rdfs:label xml:lang="en">Digital System Model</rdfs:label>
        <skos:definition xml:lang="en">A Digital Model of a System, generated by all Stakeholders that integrates the Authoritative Source(s) of Truth and associated Digital Artifacts which define all aspects of the System for the specific Activities throughout the System Lifecycle.</skos:definition>
        <cco2:ont00001754 rdf:datatype="http://www.w3.org/2001/XMLSchema#anyURI">https://www.dau.edu/glossary/digital-system-model</cco2:ont00001754>
        <cco2:ont00001760 rdf:datatype="http://www.w3.org/2001/XMLSchema#anyURI">https://semantic.incose.org/DEIX_Ontology</cco2:ont00001760>
    </owl:Class>
    


    <!-- https://hack.cybersystems.engineer/memex/ontologies/SeamlessDigitalEngineering#Digital_System_View -->

    <owl:Class rdf:about="https://hack.cybersystems.engineer/memex/ontologies/SeamlessDigitalEngineering#Digital_System_View">
        <owl:equivalentClass>
            <owl:Class>
                <owl:intersectionOf rdf:parseType="Collection">
                    <rdf:Description rdf:about="https://hack.cybersystems.engineer/memex/ontologies/SeamlessDigitalEngineering#Digital_View"/>
                    <owl:Restriction>
                        <owl:onProperty rdf:resource="http://purl.obolibrary.org/obo/BFO_0000101"/>
                        <owl:someValuesFrom rdf:resource="https://hack.cybersystems.engineer/memex/ontologies/SeamlessDigitalEngineering#System_View"/>
                    </owl:Restriction>
                </owl:intersectionOf>
            </owl:Class>
        </owl:equivalentClass>
        <rdfs:subClassOf rdf:resource="https://hack.cybersystems.engineer/memex/ontologies/SeamlessDigitalEngineering#Digital_View"/>
        <rdfs:label xml:lang="en">Digital System View</rdfs:label>
        <skos:definition xml:lang="en">A Digital View of a System</skos:definition>
        <cco2:ont00001760 rdf:datatype="http://www.w3.org/2001/XMLSchema#anyURI">https://semantic.incose.org/DEIX_Ontology</cco2:ont00001760>
    </owl:Class>
    


    <!-- https://hack.cybersystems.engineer/memex/ontologies/SeamlessDigitalEngineering#Digital_Thread -->

    <owl:Class rdf:about="https://hack.cybersystems.engineer/memex/ontologies/SeamlessDigitalEngineering#Digital_Thread">
        <owl:equivalentClass>
            <owl:Class>
                <owl:intersectionOf rdf:parseType="Collection">
                    <rdf:Description rdf:about="https://hack.cybersystems.engineer/memex/ontologies/SeamlessDigitalEngineering#Digital_Repository"/>
                    <owl:Restriction>
                        <owl:onProperty rdf:resource="http://purl.obolibrary.org/obo/BFO_0000056"/>
                        <owl:someValuesFrom rdf:resource="https://hack.cybersystems.engineer/memex/ontologies/SeamlessDigitalEngineering#Lifecycle"/>
                    </owl:Restriction>
                    <owl:Restriction>
                        <owl:onProperty rdf:resource="http://purl.obolibrary.org/obo/BFO_0000101"/>
                        <owl:someValuesFrom rdf:resource="https://hack.cybersystems.engineer/memex/ontologies/SeamlessDigitalEngineering#Traceability_Measurement_Information_Content_Entity"/>
                    </owl:Restriction>
                    <owl:Restriction>
                        <owl:onProperty rdf:resource="http://purl.obolibrary.org/obo/BFO_0000115"/>
                        <owl:someValuesFrom rdf:resource="https://hack.cybersystems.engineer/memex/ontologies/SeamlessDigitalEngineering#Digital_Artifact"/>
                    </owl:Restriction>
                </owl:intersectionOf>
            </owl:Class>
        </owl:equivalentClass>
        <rdfs:subClassOf rdf:resource="https://hack.cybersystems.engineer/memex/ontologies/SeamlessDigitalEngineering#Digital_Repository"/>
        <rdfs:comment xml:lang="en">An extensible and configurable analytical framework that seamlessly expedites the controlled interplay of technical Data, Software, Information, and Knowledge in the Digital Engineering Ecosystem, based on the established Requirements, Architectures, formats, and rules for building Digital Artifact Models.

Source: https://www.dau.edu/glossary/digital-thread</rdfs:comment>
        <rdfs:comment xml:lang="en">Digital Threads can be used to produce Digital Artifacts that are a combination of Authoritative Data, Information, Knowledge, and wisdom addressing Stakeholders’ unique perspective.

Source: INCOSE Systems Engineering Handbook, Fifth Edition (2023)</rdfs:comment>
        <rdfs:comment>It is used to inform decision makers throughout a System&apos;s Lifecycle by providing the Capability to access, integrate, and transform Data into actionable Information.

Source: https://www.dau.edu/glossary/digital-thread</rdfs:comment>
        <rdfs:label xml:lang="en">Digital Thread</rdfs:label>
        <rdfs:seeAlso rdf:resource="https://hack.cybersystems.engineer/memex/ontologies/SeamlessDigitalEngineering#Digital_Repository"/>
        <skos:definition xml:lang="en">A Digital Asset composed of a linked set of Digital Artifacts whose consistency is actively managed over the Lifecycle of a Product, process, or System.</skos:definition>
        <cco2:ont00001754 xml:lang="en">derived from &quot;Digital Thread: Definition, Value, and Reference Model&quot; (AIAA Position Paper, published June 2023)</cco2:ont00001754>
        <cco2:ont00001760 rdf:datatype="http://www.w3.org/2001/XMLSchema#anyURI">https://semantic.incose.org/DEIX_Ontology</cco2:ont00001760>
    </owl:Class>
    


    <!-- https://hack.cybersystems.engineer/memex/ontologies/SeamlessDigitalEngineering#Digital_Tool -->

    <owl:Class rdf:about="https://hack.cybersystems.engineer/memex/ontologies/SeamlessDigitalEngineering#Digital_Tool">
        <owl:equivalentClass>
            <owl:Class>
                <owl:intersectionOf rdf:parseType="Collection">
                    <rdf:Description rdf:about="https://hack.cybersystems.engineer/memex/ontologies/SeamlessDigitalEngineering#Software_Product"/>
                    <rdf:Description rdf:about="https://www.commoncoreontologies.org/ont00000581"/>
                    <owl:Restriction>
                        <owl:onProperty rdf:resource="http://purl.obolibrary.org/obo/BFO_0000178"/>
                        <owl:someValuesFrom rdf:resource="https://hack.cybersystems.engineer/memex/ontologies/SeamlessDigitalEngineering#Digital_Artifact"/>
                    </owl:Restriction>
                    <owl:Restriction>
                        <owl:onProperty rdf:resource="http://purl.obolibrary.org/obo/BFO_0000196"/>
                        <owl:someValuesFrom rdf:resource="https://www.commoncoreontologies.org/ont00000932"/>
                    </owl:Restriction>
                </owl:intersectionOf>
            </owl:Class>
        </owl:equivalentClass>
        <rdfs:subClassOf rdf:resource="https://www.commoncoreontologies.org/ont00000581"/>
        <rdfs:label xml:lang="en">Digital Tool</rdfs:label>
        <cco2:ont00001760 rdf:datatype="http://www.w3.org/2001/XMLSchema#anyURI">https://semantic.incose.org/DEIX_Ontology</cco2:ont00001760>
    </owl:Class>
    


    <!-- https://hack.cybersystems.engineer/memex/ontologies/SeamlessDigitalEngineering#Digital_Twin -->

    <owl:Class rdf:about="https://hack.cybersystems.engineer/memex/ontologies/SeamlessDigitalEngineering#Digital_Twin">
        <owl:equivalentClass>
            <owl:Class>
                <owl:intersectionOf rdf:parseType="Collection">
                    <rdf:Description rdf:about="https://hack.cybersystems.engineer/memex/ontologies/SeamlessDigitalEngineering#Digital_System_Model"/>
                    <owl:Restriction>
                        <owl:onProperty rdf:resource="http://purl.obolibrary.org/obo/BFO_0000101"/>
                        <owl:someValuesFrom rdf:resource="https://hack.cybersystems.engineer/memex/ontologies/SeamlessDigitalEngineering#Lifecycle_View"/>
                    </owl:Restriction>
                    <owl:Restriction>
                        <owl:onProperty rdf:resource="http://purl.obolibrary.org/obo/BFO_0000101"/>
                        <owl:someValuesFrom rdf:resource="https://hack.cybersystems.engineer/memex/ontologies/SeamlessDigitalEngineering#System_View"/>
                    </owl:Restriction>
                </owl:intersectionOf>
            </owl:Class>
        </owl:equivalentClass>
        <rdfs:subClassOf rdf:resource="https://hack.cybersystems.engineer/memex/ontologies/SeamlessDigitalEngineering#Digital_System_Model"/>
        <rdfs:comment xml:lang="en">A digital twin is a digital surrogate of the system, incorporating models to emulate the actual system or some of its elements. The digital twin evolves through the life cycle with the mission and definition of the system.

Source: INCOSE Systems Engineering Handbook, Fifth Edition (2023)</rdfs:comment>
        <rdfs:comment xml:lang="en">A virtual replica of a physical entity that is synchronized across time.

Source: https://www.dau.edu/glossary/digital-twin</rdfs:comment>
        <rdfs:comment xml:lang="en">Digital Twins exist to replicate configuration, performance, or history of a System.</rdfs:comment>
        <rdfs:label xml:lang="en">Digital Twin</rdfs:label>
        <skos:altLabel xml:lang="en">Virtual Twin</skos:altLabel>
        <skos:definition xml:lang="en">fit-for-purpose Digital Representation of an Observable Manufacturing Element with syncronization between the element and its Digital Representation</skos:definition>
        <skos:example xml:lang="en">Two primary sub-categories of Digital Twin are Digital Instance and Digital Prototype.</skos:example>
        <cco2:ont00001754 xml:lang="en">ISO 23247-1:2021 Automation systems and integration - Digital twin framework for manufacturing - Part 1: Overview and general principles</cco2:ont00001754>
        <cco2:ont00001760 rdf:datatype="http://www.w3.org/2001/XMLSchema#anyURI">https://semantic.incose.org/DEIX_Ontology</cco2:ont00001760>
    </owl:Class>
    


    <!-- https://hack.cybersystems.engineer/memex/ontologies/SeamlessDigitalEngineering#Digital_Twin_Role -->

    <owl:Class rdf:about="https://hack.cybersystems.engineer/memex/ontologies/SeamlessDigitalEngineering#Digital_Twin_Role">
        <rdfs:subClassOf rdf:resource="https://hack.cybersystems.engineer/memex/ontologies/SeamlessDigitalEngineering#Source_of_Truth_Role"/>
        <rdfs:subClassOf>
            <owl:Restriction>
                <owl:onProperty rdf:resource="http://purl.obolibrary.org/obo/BFO_0000195"/>
                <owl:someValuesFrom rdf:resource="https://hack.cybersystems.engineer/memex/ontologies/SeamlessDigitalEngineering#Physical_Twin_Role"/>
            </owl:Restriction>
        </rdfs:subClassOf>
        <rdfs:label xml:lang="en">Digital Twin Role</rdfs:label>
    </owl:Class>
    


    <!-- https://hack.cybersystems.engineer/memex/ontologies/SeamlessDigitalEngineering#Digital_Twin_System -->

    <owl:Class rdf:about="https://hack.cybersystems.engineer/memex/ontologies/SeamlessDigitalEngineering#Digital_Twin_System">
        <owl:equivalentClass>
            <owl:Class>
                <owl:intersectionOf rdf:parseType="Collection">
                    <rdf:Description rdf:about="https://hack.cybersystems.engineer/memex/ontologies/SeamlessDigitalEngineering#Engineered_System"/>
                    <owl:Restriction>
                        <owl:onProperty rdf:resource="http://purl.obolibrary.org/obo/BFO_0000115"/>
                        <owl:someValuesFrom rdf:resource="https://hack.cybersystems.engineer/memex/ontologies/SeamlessDigitalEngineering#Digital_Twin"/>
                    </owl:Restriction>
                    <owl:Restriction>
                        <owl:onProperty rdf:resource="http://purl.obolibrary.org/obo/BFO_0000115"/>
                        <owl:someValuesFrom rdf:resource="https://hack.cybersystems.engineer/memex/ontologies/SeamlessDigitalEngineering#System"/>
                    </owl:Restriction>
                    <owl:Restriction>
                        <owl:onProperty rdf:resource="http://purl.obolibrary.org/obo/BFO_0000183"/>
                        <owl:someValuesFrom rdf:resource="https://hack.cybersystems.engineer/memex/ontologies/SeamlessDigitalEngineering#Act_of_Digital_Simulation"/>
                    </owl:Restriction>
                    <owl:Restriction>
                        <owl:onProperty rdf:resource="http://purl.obolibrary.org/obo/BFO_0000183"/>
                        <owl:someValuesFrom rdf:resource="https://www.commoncoreontologies.org/ont00000345"/>
                    </owl:Restriction>
                </owl:intersectionOf>
            </owl:Class>
        </owl:equivalentClass>
        <rdfs:subClassOf rdf:resource="https://hack.cybersystems.engineer/memex/ontologies/SeamlessDigitalEngineering#Engineered_System"/>
        <rdfs:label xml:lang="en">Digital Twin System</rdfs:label>
        <skos:definition xml:lang="en">A System providing functionalities for the Digital Twin composed of inter-operating Target Entities, Digital Entities, data connections, and Digital Models, Data and Interfaces involved in the data connection process.</skos:definition>
        <cco2:ont00001754>ISO/IEC 30173:2023, 3.1.21</cco2:ont00001754>
        <cco2:ont00001760 rdf:datatype="http://www.w3.org/2001/XMLSchema#anyURI">https://semantic.incose.org/DEIX_Ontology</cco2:ont00001760>
    </owl:Class>
    


    <!-- https://hack.cybersystems.engineer/memex/ontologies/SeamlessDigitalEngineering#Digital_View -->

    <owl:Class rdf:about="https://hack.cybersystems.engineer/memex/ontologies/SeamlessDigitalEngineering#Digital_View">
        <owl:equivalentClass>
            <owl:Class>
                <owl:intersectionOf rdf:parseType="Collection">
                    <rdf:Description rdf:about="https://hack.cybersystems.engineer/memex/ontologies/SeamlessDigitalEngineering#Digital_Model"/>
                    <owl:Restriction>
                        <owl:onProperty rdf:resource="http://purl.obolibrary.org/obo/BFO_0000101"/>
                        <owl:someValuesFrom rdf:resource="https://hack.cybersystems.engineer/memex/ontologies/SeamlessDigitalEngineering#View"/>
                    </owl:Restriction>
                </owl:intersectionOf>
            </owl:Class>
        </owl:equivalentClass>
        <rdfs:subClassOf rdf:resource="https://hack.cybersystems.engineer/memex/ontologies/SeamlessDigitalEngineering#Digital_Model"/>
        <rdfs:label xml:lang="en">Digital View</rdfs:label>
        <skos:definition xml:lang="en">A Digital Model of an entity from the perspective of a related set of Concerns</skos:definition>
        <cco2:ont00001760 rdf:datatype="http://www.w3.org/2001/XMLSchema#anyURI">https://semantic.incose.org/DEIX_Ontology</cco2:ont00001760>
    </owl:Class>
    


    <!-- https://hack.cybersystems.engineer/memex/ontologies/SeamlessDigitalEngineering#Digital_Viewpoint -->

    <owl:Class rdf:about="https://hack.cybersystems.engineer/memex/ontologies/SeamlessDigitalEngineering#Digital_Viewpoint">
        <owl:equivalentClass>
            <owl:Class>
                <owl:intersectionOf rdf:parseType="Collection">
                    <rdf:Description rdf:about="https://hack.cybersystems.engineer/memex/ontologies/SeamlessDigitalEngineering#Digital_Artifact"/>
                    <owl:Restriction>
                        <owl:onProperty rdf:resource="http://purl.obolibrary.org/obo/BFO_0000101"/>
                        <owl:someValuesFrom rdf:resource="https://hack.cybersystems.engineer/memex/ontologies/SeamlessDigitalEngineering#Viewpoint"/>
                    </owl:Restriction>
                </owl:intersectionOf>
            </owl:Class>
        </owl:equivalentClass>
        <rdfs:subClassOf rdf:resource="https://hack.cybersystems.engineer/memex/ontologies/SeamlessDigitalEngineering#Digital_Artifact"/>
        <rdfs:label xml:lang="en">Digital Viewpoint</rdfs:label>
        <skos:definition xml:lang="en">A Digital Artifact that carries a Viewpoint specification</skos:definition>
        <cco2:ont00001760 rdf:datatype="http://www.w3.org/2001/XMLSchema#anyURI">https://semantic.incose.org/DEIX_Ontology</cco2:ont00001760>
    </owl:Class>
    


    <!-- https://hack.cybersystems.engineer/memex/ontologies/SeamlessDigitalEngineering#Directed_SoS -->

    <owl:Class rdf:about="https://hack.cybersystems.engineer/memex/ontologies/SeamlessDigitalEngineering#Directed_SoS">
        <rdfs:subClassOf rdf:resource="https://hack.cybersystems.engineer/memex/ontologies/SeamlessDigitalEngineering#System-of-Systems"/>
        <rdfs:label xml:lang="en">Directed System-of-Systems</rdfs:label>
        <skos:definition xml:lang="en">The SoS is created and managed to fulfill specific purposes and the constituent systems are subordinated to the SoS. The constituent systems maintain an ability to operate independently; however, their normal operational mode is subordinated to the central managed purpose.</skos:definition>
        <cco2:ont00001754 xml:lang="en">ISO/IEC/IEEE 21841 - Systems and software engineering - Taxonomy of systems of systems</cco2:ont00001754>
    </owl:Class>
    


    <!-- https://hack.cybersystems.engineer/memex/ontologies/SeamlessDigitalEngineering#Director -->

    <owl:Class rdf:about="https://hack.cybersystems.engineer/memex/ontologies/SeamlessDigitalEngineering#Director">
        <rdfs:subClassOf rdf:resource="https://hack.cybersystems.engineer/memex/ontologies/SeamlessDigitalEngineering#Project_Team_Member"/>
        <rdfs:label xml:lang="en">Director</rdfs:label>
    </owl:Class>
    


    <!-- https://hack.cybersystems.engineer/memex/ontologies/SeamlessDigitalEngineering#Discipline -->

    <owl:Class rdf:about="https://hack.cybersystems.engineer/memex/ontologies/SeamlessDigitalEngineering#Discipline">
        <owl:equivalentClass>
            <owl:Restriction>
                <owl:onProperty rdf:resource="http://purl.obolibrary.org/obo/BFO_0000176"/>
                <owl:someValuesFrom rdf:resource="https://hack.cybersystems.engineer/memex/ontologies/SeamlessDigitalEngineering#Knowledge"/>
            </owl:Restriction>
        </owl:equivalentClass>
        <rdfs:subClassOf rdf:resource="https://hack.cybersystems.engineer/memex/ontologies/SeamlessDigitalEngineering#Knowledge"/>
        <rdfs:label xml:lang="en">Discipline</rdfs:label>
        <skos:definition xml:lang="en">a branch of Knowledge or teaching</skos:definition>
        <cco2:ont00001754 xml:lang="en">The American Heritage Dictionary of the English Language, 5th Edition</cco2:ont00001754>
    </owl:Class>
    


    <!-- https://hack.cybersystems.engineer/memex/ontologies/SeamlessDigitalEngineering#Disposal_Process -->

    <owl:Class rdf:about="https://hack.cybersystems.engineer/memex/ontologies/SeamlessDigitalEngineering#Disposal_Process">
        <rdfs:subClassOf rdf:resource="https://hack.cybersystems.engineer/memex/ontologies/SeamlessDigitalEngineering#Technical_Process"/>
        <rdfs:label xml:lang="en">Disposal Process</rdfs:label>
        <skos:definition xml:lang="en">The purpose of the disposal process is to end the existence of a system element or system for a specified intended use, appropriately handle replaced or retired elements, appropriately handle any waste products, and to properly attend to identified critical disposal needs (e.g. per an agreement; per organizational policy; or for environmental, legal, safety, or security aspects).</skos:definition>
        <cco2:ont00001754>ISO/IEC/IEEE 15288:2023</cco2:ont00001754>
    </owl:Class>
    


    <!-- https://hack.cybersystems.engineer/memex/ontologies/SeamlessDigitalEngineering#Distributed_System -->

    <owl:Class rdf:about="https://hack.cybersystems.engineer/memex/ontologies/SeamlessDigitalEngineering#Distributed_System">
        <rdfs:subClassOf rdf:resource="https://hack.cybersystems.engineer/memex/ontologies/SeamlessDigitalEngineering#System"/>
        <rdfs:label xml:lang="en">Distributed System</rdfs:label>
        <skos:definition xml:lang="en">Defined as computer systems whose inter-communicating components are located on different networked computers.</skos:definition>
    </owl:Class>
    


    <!-- https://hack.cybersystems.engineer/memex/ontologies/SeamlessDigitalEngineering#Document-Centric_Engineering -->

    <owl:Class rdf:about="https://hack.cybersystems.engineer/memex/ontologies/SeamlessDigitalEngineering#Document-Centric_Engineering">
        <owl:equivalentClass>
            <owl:Class>
                <owl:intersectionOf rdf:parseType="Collection">
                    <rdf:Description rdf:about="https://hack.cybersystems.engineer/memex/ontologies/SeamlessDigitalEngineering#Engineering_Approach"/>
                    <owl:Restriction>
                        <owl:onProperty rdf:resource="https://www.commoncoreontologies.org/ont00001808"/>
                        <owl:someValuesFrom rdf:resource="https://www.commoncoreontologies.org/ont00001298"/>
                    </owl:Restriction>
                </owl:intersectionOf>
            </owl:Class>
        </owl:equivalentClass>
        <rdfs:subClassOf rdf:resource="https://hack.cybersystems.engineer/memex/ontologies/SeamlessDigitalEngineering#Engineering_Approach"/>
        <rdfs:label xml:lang="en">Document-Centric Engineering</rdfs:label>
    </owl:Class>
    


    <!-- https://hack.cybersystems.engineer/memex/ontologies/SeamlessDigitalEngineering#Document-Centric_Systems_Engineering -->

    <owl:Class rdf:about="https://hack.cybersystems.engineer/memex/ontologies/SeamlessDigitalEngineering#Document-Centric_Systems_Engineering">
        <owl:equivalentClass>
            <owl:Class>
                <owl:intersectionOf rdf:parseType="Collection">
                    <rdf:Description rdf:about="https://hack.cybersystems.engineer/memex/ontologies/SeamlessDigitalEngineering#Document-Centric_Engineering"/>
                    <owl:Restriction>
                        <owl:onProperty rdf:resource="http://purl.obolibrary.org/obo/BFO_0000058"/>
                        <owl:someValuesFrom rdf:resource="https://hack.cybersystems.engineer/memex/ontologies/SeamlessDigitalEngineering#Act_of_Systems_Engineering"/>
                    </owl:Restriction>
                </owl:intersectionOf>
            </owl:Class>
        </owl:equivalentClass>
        <rdfs:subClassOf rdf:resource="https://hack.cybersystems.engineer/memex/ontologies/SeamlessDigitalEngineering#Document-Centric_Engineering"/>
        <rdfs:label xml:lang="en">Document-Centric Systems Engineering</rdfs:label>
        <skos:altLabel>DCSE</skos:altLabel>
    </owl:Class>
    


    <!-- https://hack.cybersystems.engineer/memex/ontologies/SeamlessDigitalEngineering#Document_Identifier -->

    <owl:Class rdf:about="https://hack.cybersystems.engineer/memex/ontologies/SeamlessDigitalEngineering#Document_Identifier">
        <owl:equivalentClass>
            <owl:Class>
                <owl:intersectionOf rdf:parseType="Collection">
                    <rdf:Description rdf:about="https://www.commoncoreontologies.org/ont00000292"/>
                    <owl:Restriction>
                        <owl:onProperty rdf:resource="https://www.commoncoreontologies.org/ont00001916"/>
                        <owl:someValuesFrom rdf:resource="https://www.commoncoreontologies.org/ont00001298"/>
                    </owl:Restriction>
                </owl:intersectionOf>
            </owl:Class>
        </owl:equivalentClass>
        <rdfs:subClassOf rdf:resource="https://www.commoncoreontologies.org/ont00000292"/>
        <rdfs:label xml:lang="en">Document Identifier</rdfs:label>
    </owl:Class>
    


    <!-- https://hack.cybersystems.engineer/memex/ontologies/SeamlessDigitalEngineering#Documentation -->

    <owl:Class rdf:about="https://hack.cybersystems.engineer/memex/ontologies/SeamlessDigitalEngineering#Documentation">
        <owl:equivalentClass>
            <owl:Restriction>
                <owl:onProperty rdf:resource="http://purl.obolibrary.org/obo/BFO_0000115"/>
                <owl:someValuesFrom rdf:resource="https://www.commoncoreontologies.org/ont00001298"/>
            </owl:Restriction>
        </owl:equivalentClass>
        <rdfs:subClassOf rdf:resource="http://purl.obolibrary.org/obo/BFO_0000027"/>
        <rdfs:label xml:lang="en">Documentation</rdfs:label>
        <skos:definition xml:lang="en">collection of Documents related to a given subject</skos:definition>
    </owl:Class>
    


    <!-- https://hack.cybersystems.engineer/memex/ontologies/SeamlessDigitalEngineering#Documentation_Goal -->

    <owl:Class rdf:about="https://hack.cybersystems.engineer/memex/ontologies/SeamlessDigitalEngineering#Documentation_Goal">
        <rdfs:subClassOf rdf:resource="https://hack.cybersystems.engineer/memex/ontologies/SeamlessDigitalEngineering#Goal"/>
        <rdfs:label xml:lang="en">Documentation Goal</rdfs:label>
    </owl:Class>
    


    <!-- https://hack.cybersystems.engineer/memex/ontologies/SeamlessDigitalEngineering#Domain-Specific_Language -->

    <owl:Class rdf:about="https://hack.cybersystems.engineer/memex/ontologies/SeamlessDigitalEngineering#Domain-Specific_Language">
        <rdfs:subClassOf rdf:resource="http://www.ontologyrepository.com/CommonCoreOntologies/ComputerLanguage"/>
        <rdfs:label xml:lang="en">Domain-Specific Language</rdfs:label>
    </owl:Class>
    


    <!-- https://hack.cybersystems.engineer/memex/ontologies/SeamlessDigitalEngineering#Ecosystem -->

    <owl:Class rdf:about="https://hack.cybersystems.engineer/memex/ontologies/SeamlessDigitalEngineering#Ecosystem">
        <owl:equivalentClass>
            <owl:Restriction>
                <owl:onProperty rdf:resource="http://purl.obolibrary.org/obo/BFO_0000115"/>
                <owl:someValuesFrom>
                    <owl:Class>
                        <owl:intersectionOf rdf:parseType="Collection">
                            <rdf:Description rdf:about="https://hack.cybersystems.engineer/memex/ontologies/SeamlessDigitalEngineering#Stakeholder"/>
                            <rdf:Description rdf:about="https://www.commoncoreontologies.org/ont00000509"/>
                            <rdf:Description rdf:about="https://www.commoncoreontologies.org/ont00000870"/>
                            <rdf:Description rdf:about="https://www.commoncoreontologies.org/ont00001180"/>
                        </owl:intersectionOf>
                    </owl:Class>
                </owl:someValuesFrom>
            </owl:Restriction>
        </owl:equivalentClass>
        <rdfs:subClassOf rdf:resource="https://hack.cybersystems.engineer/memex/ontologies/SeamlessDigitalEngineering#Complex_Adaptive_System"/>
        <rdfs:label xml:lang="en">Ecosystem</rdfs:label>
        <skos:definition xml:lang="en">ISO/IEC TS 27400:2022, 3.8</skos:definition>
        <skos:definition xml:lang="en">Infrastructure and Services based on a network of Organizations and Stakeholders</skos:definition>
        <cco2:ont00001760 rdf:datatype="http://www.w3.org/2001/XMLSchema#anyURI">https://semantic.incose.org/DEIX_Ontology</cco2:ont00001760>
    </owl:Class>
    


    <!-- https://hack.cybersystems.engineer/memex/ontologies/SeamlessDigitalEngineering#Embedded_Domain-Specific_Language -->

    <owl:Class rdf:about="https://hack.cybersystems.engineer/memex/ontologies/SeamlessDigitalEngineering#Embedded_Domain-Specific_Language">
        <rdfs:subClassOf rdf:resource="https://hack.cybersystems.engineer/memex/ontologies/SeamlessDigitalEngineering#Domain-Specific_Language"/>
        <rdfs:label xml:lang="en">Embedded Domain-Specific Language</rdfs:label>
    </owl:Class>
    


    <!-- https://hack.cybersystems.engineer/memex/ontologies/SeamlessDigitalEngineering#Enabling_System -->

    <owl:Class rdf:about="https://hack.cybersystems.engineer/memex/ontologies/SeamlessDigitalEngineering#Enabling_System">
        <rdfs:subClassOf rdf:resource="https://hack.cybersystems.engineer/memex/ontologies/SeamlessDigitalEngineering#System"/>
        <rdfs:label xml:lang="en">Enabling System</rdfs:label>
        <skos:definition xml:lang="en">System that supports a System-of-Interest during its Lifecycle stages but does not necessarily contribute directly to its function during operation</skos:definition>
        <skos:example xml:lang="en">Production-enabling system, which is required when a system-of-interest enters the production stage.</skos:example>
        <cco2:ont00001754>ISO/IEC/IEEE 15288:2023</cco2:ont00001754>
    </owl:Class>
    


    <!-- https://hack.cybersystems.engineer/memex/ontologies/SeamlessDigitalEngineering#Engineer -->

    <owl:Class rdf:about="https://hack.cybersystems.engineer/memex/ontologies/SeamlessDigitalEngineering#Engineer">
        <rdfs:subClassOf rdf:resource="https://hack.cybersystems.engineer/memex/ontologies/SeamlessDigitalEngineering#Project_Team_Member"/>
    </owl:Class>
    


    <!-- https://hack.cybersystems.engineer/memex/ontologies/SeamlessDigitalEngineering#Engineered_System -->

    <owl:Class rdf:about="https://hack.cybersystems.engineer/memex/ontologies/SeamlessDigitalEngineering#Engineered_System">
        <rdfs:subClassOf rdf:resource="https://hack.cybersystems.engineer/memex/ontologies/SeamlessDigitalEngineering#System"/>
        <rdfs:label xml:lang="en">Engineered System</rdfs:label>
        <skos:definition xml:lang="en">A System designed or adapted to interact with an anticipated Operational Environment to achieve one or more intended Purposes while complying with applicable Constraints.</skos:definition>
        <cco2:ont00001754 xml:lang="en">https://sebokwiki.org/wiki/Engineered_System_(glossary)</cco2:ont00001754>
        <cco2:ont00001760 rdf:datatype="http://www.w3.org/2001/XMLSchema#anyURI">https://semantic.incose.org/DEIX_Ontology</cco2:ont00001760>
    </owl:Class>
    


    <!-- https://hack.cybersystems.engineer/memex/ontologies/SeamlessDigitalEngineering#Engineering_Approach -->

    <owl:Class rdf:about="https://hack.cybersystems.engineer/memex/ontologies/SeamlessDigitalEngineering#Engineering_Approach">
        <owl:equivalentClass>
            <owl:Class>
                <owl:intersectionOf rdf:parseType="Collection">
                    <rdf:Description rdf:about="https://hack.cybersystems.engineer/memex/ontologies/SeamlessDigitalEngineering#Approach"/>
                    <owl:Restriction>
                        <owl:onProperty rdf:resource="https://www.commoncoreontologies.org/ont00001942"/>
                        <owl:someValuesFrom rdf:resource="https://hack.cybersystems.engineer/memex/ontologies/SeamlessDigitalEngineering#Act_of_Engineering"/>
                    </owl:Restriction>
                </owl:intersectionOf>
            </owl:Class>
        </owl:equivalentClass>
        <rdfs:subClassOf rdf:resource="https://hack.cybersystems.engineer/memex/ontologies/SeamlessDigitalEngineering#Approach"/>
        <rdfs:label xml:lang="en">Engineering Approach</rdfs:label>
        <skos:definition xml:lang="en">An Approach which prescribes how an Act of Engineering is performed</skos:definition>
        <cco2:ont00001760 rdf:datatype="http://www.w3.org/2001/XMLSchema#anyURI">https://semantic.incose.org/DEIX_Ontology</cco2:ont00001760>
    </owl:Class>
    


    <!-- https://hack.cybersystems.engineer/memex/ontologies/SeamlessDigitalEngineering#Engineering_Discipline -->

    <owl:Class rdf:about="https://hack.cybersystems.engineer/memex/ontologies/SeamlessDigitalEngineering#Engineering_Discipline">
        <owl:equivalentClass>
            <owl:Class>
                <owl:intersectionOf rdf:parseType="Collection">
                    <rdf:Description rdf:about="https://hack.cybersystems.engineer/memex/ontologies/SeamlessDigitalEngineering#Discipline"/>
                    <owl:Restriction>
                        <owl:onProperty rdf:resource="https://www.commoncoreontologies.org/ont00001808"/>
                        <owl:someValuesFrom rdf:resource="https://hack.cybersystems.engineer/memex/ontologies/SeamlessDigitalEngineering#Act_of_Engineering"/>
                    </owl:Restriction>
                </owl:intersectionOf>
            </owl:Class>
        </owl:equivalentClass>
        <rdfs:subClassOf rdf:resource="https://hack.cybersystems.engineer/memex/ontologies/SeamlessDigitalEngineering#Discipline"/>
        <rdfs:label xml:lang="en">Engineering Discipline</rdfs:label>
    </owl:Class>
    


    <!-- https://hack.cybersystems.engineer/memex/ontologies/SeamlessDigitalEngineering#Engineering_Methodology -->

    <owl:Class rdf:about="https://hack.cybersystems.engineer/memex/ontologies/SeamlessDigitalEngineering#Engineering_Methodology">
        <owl:equivalentClass>
            <owl:Class>
                <owl:intersectionOf rdf:parseType="Collection">
                    <rdf:Description rdf:about="https://hack.cybersystems.engineer/memex/ontologies/SeamlessDigitalEngineering#Methodology"/>
                    <owl:Restriction>
                        <owl:onProperty rdf:resource="https://www.commoncoreontologies.org/ont00001942"/>
                        <owl:someValuesFrom rdf:resource="https://hack.cybersystems.engineer/memex/ontologies/SeamlessDigitalEngineering#Act_of_Engineering"/>
                    </owl:Restriction>
                </owl:intersectionOf>
            </owl:Class>
        </owl:equivalentClass>
        <rdfs:subClassOf rdf:resource="https://hack.cybersystems.engineer/memex/ontologies/SeamlessDigitalEngineering#Methodology"/>
        <rdfs:label xml:lang="en">Engineering Methodology</rdfs:label>
    </owl:Class>
    


    <!-- https://hack.cybersystems.engineer/memex/ontologies/SeamlessDigitalEngineering#Enterprise -->

    <owl:Class rdf:about="https://hack.cybersystems.engineer/memex/ontologies/SeamlessDigitalEngineering#Enterprise">
        <rdfs:subClassOf rdf:resource="https://www.commoncoreontologies.org/ont00001180"/>
        <skos:definition xml:lang="en">A purposeful combination of interdependent resources that interact with each other to achieve business and operational Goals.</skos:definition>
        <cco2:ont00001754>INCOSE (2023). Systems Engineering Handbook, Fifth Edition. No. INCOSE-TP-2003-002-05. ISBN: 9781119814306</cco2:ont00001754>
    </owl:Class>
    


    <!-- https://hack.cybersystems.engineer/memex/ontologies/SeamlessDigitalEngineering#Enterprise_Architecture -->

    <owl:Class rdf:about="https://hack.cybersystems.engineer/memex/ontologies/SeamlessDigitalEngineering#Enterprise_Architecture">
        <owl:equivalentClass>
            <owl:Restriction>
                <owl:onProperty rdf:resource="https://www.commoncoreontologies.org/ont00001942"/>
                <owl:someValuesFrom rdf:resource="https://hack.cybersystems.engineer/memex/ontologies/SeamlessDigitalEngineering#Enterprise"/>
            </owl:Restriction>
        </owl:equivalentClass>
        <rdfs:subClassOf rdf:resource="https://hack.cybersystems.engineer/memex/ontologies/SeamlessDigitalEngineering#Architecture"/>
        <rdfs:label xml:lang="en">Enterprise Architecture</rdfs:label>
        <skos:definition xml:lang="en">An enterprise architecture is either the architecture of an enterprise or the architecture of an entity from an enterprise point of view. In both cases, it has a defined overall business objective and may include one or more participating organization.

Enterprise architecture is the organizing logic for business processes and information technology infrastructure reflecting the integration and standardization requirements of the company&apos;s operating model. The operating model is the desired state of business process integration and business process standardization for delivering goods and services to customers.</skos:definition>
        <cco2:ont00001754 xml:lang="en">ISO/IEC/IEEE 42020:2019</cco2:ont00001754>
    </owl:Class>
    


    <!-- https://hack.cybersystems.engineer/memex/ontologies/SeamlessDigitalEngineering#Error -->

    <owl:Class rdf:about="https://hack.cybersystems.engineer/memex/ontologies/SeamlessDigitalEngineering#Error">
        <rdfs:subClassOf rdf:resource="https://www.commoncoreontologies.org/ont00000997"/>
        <rdfs:subClassOf>
            <owl:Restriction>
                <owl:onProperty rdf:resource="http://purl.obolibrary.org/obo/BFO_0000197"/>
                <owl:someValuesFrom rdf:resource="https://hack.cybersystems.engineer/memex/ontologies/SeamlessDigitalEngineering#System"/>
            </owl:Restriction>
        </rdfs:subClassOf>
        <rdfs:label xml:lang="en">Error</rdfs:label>
        <skos:definition xml:lang="en">discrepancy between a computed, observed or measured value or Condition, and the true, specified or theoretically correct value or Condition.</skos:definition>
        <skos:editorialNote xml:lang="en">Defined in &apos;subclass of&apos; instead of &apos;equivalent to&apos; because an Error is not a necessary condition of a System. (double-check later)</skos:editorialNote>
        <skos:example xml:lang="en">omission or misinterpretation of user requirements in a software specification, incorrect translation, or omission of a requirement in the design specification</skos:example>
        <cco2:ont00001754 xml:lang="en">ISO/IEC 15026-1:2019 Systems and software engineering — Systems and software assurance — Part 1: Concepts and vocabulary, 3.4.5</cco2:ont00001754>
    </owl:Class>
    


    <!-- https://hack.cybersystems.engineer/memex/ontologies/SeamlessDigitalEngineering#Evaluation_Assurance -->

    <owl:Class rdf:about="https://hack.cybersystems.engineer/memex/ontologies/SeamlessDigitalEngineering#Evaluation_Assurance">
        <owl:equivalentClass>
            <owl:Class>
                <owl:intersectionOf rdf:parseType="Collection">
                    <rdf:Description rdf:about="https://hack.cybersystems.engineer/memex/ontologies/SeamlessDigitalEngineering#Assurance"/>
                    <owl:Restriction>
                        <owl:onProperty rdf:resource="https://www.commoncoreontologies.org/ont00001801"/>
                        <owl:someValuesFrom rdf:resource="https://hack.cybersystems.engineer/memex/ontologies/SeamlessDigitalEngineering#Assurance_Requirement"/>
                    </owl:Restriction>
                </owl:intersectionOf>
            </owl:Class>
        </owl:equivalentClass>
        <rdfs:subClassOf rdf:resource="https://hack.cybersystems.engineer/memex/ontologies/SeamlessDigitalEngineering#Assurance"/>
        <rdfs:label xml:lang="en">Evaluation Assurance</rdfs:label>
    </owl:Class>
    


    <!-- https://hack.cybersystems.engineer/memex/ontologies/SeamlessDigitalEngineering#Evaluation_Assurance_Level -->

    <owl:Class rdf:about="https://hack.cybersystems.engineer/memex/ontologies/SeamlessDigitalEngineering#Evaluation_Assurance_Level">
        <owl:equivalentClass>
            <owl:Class>
                <owl:intersectionOf rdf:parseType="Collection">
                    <rdf:Description rdf:about="https://www.commoncoreontologies.org/ont00001010"/>
                    <owl:Restriction>
                        <owl:onProperty rdf:resource="http://purl.obolibrary.org/obo/BFO_0000178"/>
                        <owl:someValuesFrom rdf:resource="https://hack.cybersystems.engineer/memex/ontologies/SeamlessDigitalEngineering#Security_Assurance_Requirement"/>
                    </owl:Restriction>
                </owl:intersectionOf>
            </owl:Class>
        </owl:equivalentClass>
        <rdfs:subClassOf rdf:resource="https://www.commoncoreontologies.org/ont00001010"/>
        <rdfs:label xml:lang="en">Evaluation Assurance Level</rdfs:label>
        <skos:definition xml:lang="en">well-formed package of Security Assurance Requirements representing a point on the pre-defined assurance scale</skos:definition>
        <cco2:ont00001753 xml:lang="en">EAL</cco2:ont00001753>
        <cco2:ont00001754 xml:lang="en">ISO/IEC 15408-1:2022</cco2:ont00001754>
    </owl:Class>
    


    <!-- https://hack.cybersystems.engineer/memex/ontologies/SeamlessDigitalEngineering#Evaluation_Authority -->

    <owl:Class rdf:about="https://hack.cybersystems.engineer/memex/ontologies/SeamlessDigitalEngineering#Evaluation_Authority">
        <rdfs:subClassOf rdf:resource="https://hack.cybersystems.engineer/memex/ontologies/SeamlessDigitalEngineering#Authority"/>
        <rdfs:label xml:lang="en">Evaluation Authority</rdfs:label>
        <skos:definition xml:lang="en">Agent operating an Evaluation Scheme</skos:definition>
        <cco2:ont00001754 xml:lang="en">ISO/IEC 15408-1:2022</cco2:ont00001754>
    </owl:Class>
    


    <!-- https://hack.cybersystems.engineer/memex/ontologies/SeamlessDigitalEngineering#Evaluation_Authority_Role -->

    <owl:Class rdf:about="https://hack.cybersystems.engineer/memex/ontologies/SeamlessDigitalEngineering#Evaluation_Authority_Role">
        <rdfs:subClassOf rdf:resource="https://www.commoncoreontologies.org/ont00000187"/>
        <rdfs:label xml:lang="en">Evaluation Authority Role</rdfs:label>
        <skos:definition xml:lang="en">Authority Role of an Agent operating an Evaluation Scheme</skos:definition>
        <cco2:ont00001754 xml:lang="en">ISO/IEC 15408-1:2022</cco2:ont00001754>
    </owl:Class>
    


    <!-- https://hack.cybersystems.engineer/memex/ontologies/SeamlessDigitalEngineering#Evaluation_Method -->

    <owl:Class rdf:about="https://hack.cybersystems.engineer/memex/ontologies/SeamlessDigitalEngineering#Evaluation_Method">
        <owl:equivalentClass>
            <owl:Class>
                <owl:intersectionOf rdf:parseType="Collection">
                    <rdf:Description rdf:about="https://hack.cybersystems.engineer/memex/ontologies/SeamlessDigitalEngineering#Evaluation_Scheme"/>
                    <owl:Restriction>
                        <owl:onProperty rdf:resource="https://www.commoncoreontologies.org/ont00001808"/>
                        <owl:someValuesFrom rdf:resource="https://hack.cybersystems.engineer/memex/ontologies/SeamlessDigitalEngineering#Product"/>
                    </owl:Restriction>
                </owl:intersectionOf>
            </owl:Class>
        </owl:equivalentClass>
        <rdfs:subClassOf rdf:resource="https://hack.cybersystems.engineer/memex/ontologies/SeamlessDigitalEngineering#Evaluation_Scheme"/>
        <rdfs:label xml:lang="en">Evaluation Method</rdfs:label>
        <skos:definition xml:lang="en">procedure describing actions to be performed by the Evaluator in order to obtain results for the specified measurement applied to the specified product components or on the product as a whole</skos:definition>
        <cco2:ont00001754 xml:lang="en">ISO/IEC 25040:2011</cco2:ont00001754>
    </owl:Class>
    


    <!-- https://hack.cybersystems.engineer/memex/ontologies/SeamlessDigitalEngineering#Evaluation_Report -->

    <owl:Class rdf:about="https://hack.cybersystems.engineer/memex/ontologies/SeamlessDigitalEngineering#Evaluation_Report">
        <owl:equivalentClass>
            <owl:Class>
                <owl:intersectionOf rdf:parseType="Collection">
                    <rdf:Description rdf:about="https://www.commoncoreontologies.org/ont00000624"/>
                    <owl:Restriction>
                        <owl:onProperty rdf:resource="http://purl.obolibrary.org/obo/BFO_0000101"/>
                        <owl:someValuesFrom rdf:resource="https://www.commoncoreontologies.org/ont00001163"/>
                    </owl:Restriction>
                </owl:intersectionOf>
            </owl:Class>
        </owl:equivalentClass>
        <rdfs:subClassOf rdf:resource="https://www.commoncoreontologies.org/ont00000624"/>
        <rdfs:label xml:lang="en">Evaluation Report</rdfs:label>
    </owl:Class>
    


    <!-- https://hack.cybersystems.engineer/memex/ontologies/SeamlessDigitalEngineering#Evaluation_Scheme -->

    <owl:Class rdf:about="https://hack.cybersystems.engineer/memex/ontologies/SeamlessDigitalEngineering#Evaluation_Scheme">
        <owl:equivalentClass>
            <owl:Class>
                <owl:intersectionOf rdf:parseType="Collection">
                    <rdf:Description rdf:about="https://hack.cybersystems.engineer/memex/ontologies/SeamlessDigitalEngineering#Method"/>
                    <owl:Restriction>
                        <owl:onProperty rdf:resource="https://www.commoncoreontologies.org/ont00001942"/>
                        <owl:someValuesFrom rdf:resource="https://hack.cybersystems.engineer/memex/ontologies/SeamlessDigitalEngineering#Act_of_Evaluation"/>
                    </owl:Restriction>
                </owl:intersectionOf>
            </owl:Class>
        </owl:equivalentClass>
        <rdfs:subClassOf rdf:resource="https://hack.cybersystems.engineer/memex/ontologies/SeamlessDigitalEngineering#Method"/>
        <rdfs:label xml:lang="en">Evaluation Scheme</rdfs:label>
        <skos:definition xml:lang="en">rules, procedures, and management to performing some Act of Evaluation (e.g., of Product Security)</skos:definition>
        <cco2:ont00001754 xml:lang="en">ISO/IEC 15408-1:2022</cco2:ont00001754>
    </owl:Class>
    


    <!-- https://hack.cybersystems.engineer/memex/ontologies/SeamlessDigitalEngineering#Evaluator -->

    <owl:Class rdf:about="https://hack.cybersystems.engineer/memex/ontologies/SeamlessDigitalEngineering#Evaluator">
        <owl:equivalentClass>
            <owl:Class>
                <owl:intersectionOf rdf:parseType="Collection">
                    <rdf:Description rdf:about="https://hack.cybersystems.engineer/memex/ontologies/SeamlessDigitalEngineering#Stakeholder"/>
                    <owl:Restriction>
                        <owl:onProperty rdf:resource="https://www.commoncoreontologies.org/ont00001787"/>
                        <owl:someValuesFrom rdf:resource="https://hack.cybersystems.engineer/memex/ontologies/SeamlessDigitalEngineering#Act_of_Evaluation"/>
                    </owl:Restriction>
                </owl:intersectionOf>
            </owl:Class>
        </owl:equivalentClass>
        <rdfs:subClassOf rdf:resource="https://hack.cybersystems.engineer/memex/ontologies/SeamlessDigitalEngineering#Stakeholder"/>
        <skos:definition xml:lang="en">Agent (individual) or Organization that performs an evaluation</skos:definition>
        <cco2:ont00001754 xml:lang="en">ISO/IEC 25002:2024 Systems and software engineering - Systems and software Quality Requirements and Evaluation (SQuaRE) - Quality model overview and usage</cco2:ont00001754>
    </owl:Class>
    


    <!-- https://hack.cybersystems.engineer/memex/ontologies/SeamlessDigitalEngineering#Evaluator_Action -->

    <owl:Class rdf:about="https://hack.cybersystems.engineer/memex/ontologies/SeamlessDigitalEngineering#Evaluator_Action">
        <owl:equivalentClass>
            <owl:Class>
                <owl:intersectionOf rdf:parseType="Collection">
                    <rdf:Description rdf:about="https://hack.cybersystems.engineer/memex/ontologies/SeamlessDigitalEngineering#Action"/>
                    <owl:Restriction>
                        <owl:onProperty rdf:resource="https://www.commoncoreontologies.org/ont00001778"/>
                        <owl:someValuesFrom rdf:resource="https://hack.cybersystems.engineer/memex/ontologies/SeamlessDigitalEngineering#Target_of_Evaluation"/>
                    </owl:Restriction>
                    <owl:Restriction>
                        <owl:onProperty rdf:resource="https://www.commoncoreontologies.org/ont00001857"/>
                        <owl:someValuesFrom rdf:resource="https://hack.cybersystems.engineer/memex/ontologies/SeamlessDigitalEngineering#Act_of_Evaluation"/>
                    </owl:Restriction>
                </owl:intersectionOf>
            </owl:Class>
        </owl:equivalentClass>
        <rdfs:subClassOf rdf:resource="https://hack.cybersystems.engineer/memex/ontologies/SeamlessDigitalEngineering#Action"/>
        <rdfs:label xml:lang="en">Evaluator Action</rdfs:label>
        <skos:definition xml:lang="en">Action of an Evaluator</skos:definition>
    </owl:Class>
    


    <!-- https://hack.cybersystems.engineer/memex/ontologies/SeamlessDigitalEngineering#Evidence_Item -->

    <owl:Class rdf:about="https://hack.cybersystems.engineer/memex/ontologies/SeamlessDigitalEngineering#Evidence_Item">
        <rdfs:subClassOf rdf:resource="https://hack.cybersystems.engineer/memex/ontologies/SeamlessDigitalEngineering#Information_Part"/>
        <rdfs:comment xml:lang="en">An Evidence Item can exist independently of the Assurance Case before its construction, or can be newly created or collected for the purpose of constructing the Assurance Case. A description of preparation for collecting an Evidence Item, such as field Data, can be another Evidence Item. An Evidence Item is to support a Claim in the Assurance Case, as indicated in the definition of Argument type.</rdfs:comment>
        <rdfs:comment xml:lang="en">When Evidence Items are created in developing the Assurance Case, it is more convenient for them to be managed independently of the Arguments.</rdfs:comment>
        <rdfs:label xml:lang="en">Evidence Item</rdfs:label>
        <skos:definition xml:lang="en">an available body of facts or Information that support an assertion of truth of a Claim</skos:definition>
        <cco2:ont00001754 xml:lang="en">ISO/IEC/IEEE 15026-2:2022</cco2:ont00001754>
    </owl:Class>
    


    <!-- https://hack.cybersystems.engineer/memex/ontologies/SeamlessDigitalEngineering#Evidence_Report -->

    <owl:Class rdf:about="https://hack.cybersystems.engineer/memex/ontologies/SeamlessDigitalEngineering#Evidence_Report">
        <owl:equivalentClass>
            <owl:Class>
                <owl:intersectionOf rdf:parseType="Collection">
                    <rdf:Description rdf:about="https://www.commoncoreontologies.org/ont00000624"/>
                    <owl:Restriction>
                        <owl:onProperty rdf:resource="http://purl.obolibrary.org/obo/BFO_0000101"/>
                        <owl:someValuesFrom>
                            <owl:Class>
                                <owl:intersectionOf rdf:parseType="Collection">
                                    <rdf:Description rdf:about="https://hack.cybersystems.engineer/memex/ontologies/SeamlessDigitalEngineering#Basic_Assumption"/>
                                    <rdf:Description rdf:about="https://hack.cybersystems.engineer/memex/ontologies/SeamlessDigitalEngineering#Evidence_Item"/>
                                </owl:intersectionOf>
                            </owl:Class>
                        </owl:someValuesFrom>
                    </owl:Restriction>
                </owl:intersectionOf>
            </owl:Class>
        </owl:equivalentClass>
        <rdfs:subClassOf rdf:resource="https://www.commoncoreontologies.org/ont00000624"/>
        <rdfs:comment xml:lang="en">Evidence and Claims are related by Supported Claim. Additional explanation can be given in a context of that Supported Claim.</rdfs:comment>
        <rdfs:comment xml:lang="en">Evidence can be a Document that demonstrates a redundancy Requirement has been physically implemented in a System Element. It can also be operator and training manuals.</rdfs:comment>
        <rdfs:comment xml:lang="en">Multiple Assumptions in d) are taken as their conjunction.</rdfs:comment>
        <rdfs:comment xml:lang="en">The artifact can become quite large. In such cases, the artifact is organized, located, and presented to be understandable to those who review, approve, or directly use it.</rdfs:comment>
        <rdfs:label xml:lang="en">Evidence Report</rdfs:label>
        <skos:definition xml:lang="en">A Report containing the following 4 Document Fields:

a) an Information Bearing Artifact consisting of tangible data or information which includes the following:
  1) description of items produced by the Lifecycle Processes of the System-of-Interest, such as Contracts and Design Descriptions;
  2) Reports provided by the Activities of the System-of-Interest, as listed in ISO/IEC/IEEE 15289:2019, 7.6;
  3) Report provided by the Activities of the System-of-Interest, as listed in ISO/IEC/IEEE 15289:2019, 9.3;
  4) authoritative Documents such as Laws, Standards, and Scientific Documents on established Theory, History, and Observations;
b) scope of applicability of the Evidence;
c) Uncertainty, including the Credibility of its source (e.g. Authenticity, Trustworthiness, and Competence) and the Measurement Accuracy.
d) Assumptions associated with the Evidence.</skos:definition>
        <cco2:ont00001754 xml:lang="en">ISO/IEC/IEEE 15026-2:2022</cco2:ont00001754>
    </owl:Class>
    


    <!-- https://hack.cybersystems.engineer/memex/ontologies/SeamlessDigitalEngineering#Experience -->

    <owl:Class rdf:about="https://hack.cybersystems.engineer/memex/ontologies/SeamlessDigitalEngineering#Experience">
        <rdfs:subClassOf rdf:resource="https://hack.cybersystems.engineer/memex/ontologies/SeamlessDigitalEngineering#Acceptability"/>
        <rdfs:label xml:lang="en">Experience</rdfs:label>
        <skos:definition xml:lang="en">extent to which Users or Stakeholders accumulate knowledge or skill acquired over time, especially that gained in a particular profession</skos:definition>
        <cco2:ont00001754 xml:lang="en">ISO/IEC 25019:2023(en)
Systems and software engineering — Systems and software Quality Requirements and Evaluation (SQuaRE) — Quality-in-use model</cco2:ont00001754>
    </owl:Class>
    


    <!-- https://hack.cybersystems.engineer/memex/ontologies/SeamlessDigitalEngineering#Explanation_Material -->

    <owl:Class rdf:about="https://hack.cybersystems.engineer/memex/ontologies/SeamlessDigitalEngineering#Explanation_Material">
        <rdfs:subClassOf rdf:resource="https://www.commoncoreontologies.org/ont00000798"/>
        <rdfs:subClassOf>
            <owl:Restriction>
                <owl:onProperty rdf:resource="http://purl.obolibrary.org/obo/BFO_0000101"/>
                <owl:someValuesFrom rdf:resource="https://hack.cybersystems.engineer/memex/ontologies/SeamlessDigitalEngineering#Knowledge"/>
            </owl:Restriction>
        </rdfs:subClassOf>
        <rdfs:comment xml:lang="en">Explanation is understanding- (or Knowledge-)oriented.</rdfs:comment>
        <rdfs:label xml:lang="en">Explanation Material</rdfs:label>
        <skos:definition xml:lang="en">Information Bearing Artifact that is a discursive treatment of a subject, that permits reflection.</skos:definition>
        <cco2:ont00001754 rdf:datatype="http://www.w3.org/2001/XMLSchema#anyURI">https://diataxis.fr/explanation/</cco2:ont00001754>
    </owl:Class>
    


    <!-- https://hack.cybersystems.engineer/memex/ontologies/SeamlessDigitalEngineering#Failure -->

    <owl:Class rdf:about="https://hack.cybersystems.engineer/memex/ontologies/SeamlessDigitalEngineering#Failure">
        <rdfs:subClassOf rdf:resource="https://www.commoncoreontologies.org/ont00000997"/>
        <rdfs:subClassOf>
            <owl:Restriction>
                <owl:onProperty rdf:resource="http://purl.obolibrary.org/obo/BFO_0000197"/>
                <owl:someValuesFrom rdf:resource="https://hack.cybersystems.engineer/memex/ontologies/SeamlessDigitalEngineering#System"/>
            </owl:Restriction>
        </rdfs:subClassOf>
        <rdfs:label xml:lang="en">Failure</rdfs:label>
        <skos:definition xml:lang="en">termination of the Capability of a System Element to perform a required function</skos:definition>
        <cco2:ont00001754 xml:lang="en">ISO 10795:2019(en)
Space systems — Programme management and quality — Vocabulary</cco2:ont00001754>
    </owl:Class>
    


    <!-- https://hack.cybersystems.engineer/memex/ontologies/SeamlessDigitalEngineering#Fault -->

    <owl:Class rdf:about="https://hack.cybersystems.engineer/memex/ontologies/SeamlessDigitalEngineering#Fault">
        <owl:equivalentClass>
            <owl:Class>
                <owl:intersectionOf rdf:parseType="Collection">
                    <rdf:Description rdf:about="https://hack.cybersystems.engineer/memex/ontologies/SeamlessDigitalEngineering#Defect"/>
                    <owl:Restriction>
                        <owl:onProperty rdf:resource="http://purl.obolibrary.org/obo/BFO_0000054"/>
                        <owl:someValuesFrom rdf:resource="https://hack.cybersystems.engineer/memex/ontologies/SeamlessDigitalEngineering#Lifecycle"/>
                    </owl:Restriction>
                    <owl:Restriction>
                        <owl:onProperty rdf:resource="http://purl.obolibrary.org/obo/BFO_0000194"/>
                        <owl:someValuesFrom rdf:resource="https://hack.cybersystems.engineer/memex/ontologies/SeamlessDigitalEngineering#Error"/>
                    </owl:Restriction>
                </owl:intersectionOf>
            </owl:Class>
        </owl:equivalentClass>
        <rdfs:subClassOf rdf:resource="https://hack.cybersystems.engineer/memex/ontologies/SeamlessDigitalEngineering#Defect"/>
        <rdfs:comment xml:lang="en">Faults can occur in specifications when they are not correct.</rdfs:comment>
        <rdfs:label xml:lang="en">Fault</rdfs:label>
        <skos:definition xml:lang="en">Defect in a System or a representation of a System that if executed/activated can potentially result in an Error</skos:definition>
        <cco2:ont00001754 xml:lang="en">ISO/IEC/IEEE 15026-1:2019, 3.4.6</cco2:ont00001754>
    </owl:Class>
    


    <!-- https://hack.cybersystems.engineer/memex/ontologies/SeamlessDigitalEngineering#Formal_Grammar -->

    <owl:Class rdf:about="https://hack.cybersystems.engineer/memex/ontologies/SeamlessDigitalEngineering#Formal_Grammar">
        <owl:equivalentClass>
            <owl:Restriction>
                <owl:onProperty rdf:resource="https://www.commoncoreontologies.org/ont00001942"/>
                <owl:someValuesFrom rdf:resource="https://hack.cybersystems.engineer/memex/ontologies/SeamlessDigitalEngineering#Formal_Language"/>
            </owl:Restriction>
        </owl:equivalentClass>
        <rdfs:subClassOf rdf:resource="https://hack.cybersystems.engineer/memex/ontologies/SeamlessDigitalEngineering#Formal_Language"/>
        <rdfs:label xml:lang="en">Formal Grammar</rdfs:label>
        <skos:definition xml:lang="en">describes which strings from an alphabet of a Formal Language are valid according to the language&apos;s syntax</skos:definition>
        <cco2:ont00001754 rdf:datatype="http://www.w3.org/2001/XMLSchema#anyURI">https://en.wikipedia.org/wiki/Formal_grammar</cco2:ont00001754>
    </owl:Class>
    


    <!-- https://hack.cybersystems.engineer/memex/ontologies/SeamlessDigitalEngineering#Formal_Language -->

    <owl:Class rdf:about="https://hack.cybersystems.engineer/memex/ontologies/SeamlessDigitalEngineering#Formal_Language">
        <rdfs:subClassOf rdf:resource="https://www.commoncoreontologies.org/ont00000146"/>
        <rdfs:label xml:lang="en">Formal Language</rdfs:label>
        <skos:definition xml:lang="en">an Artificial Language consisting of words whose letters are taken from an alphabet and are well-formed according to a specific set of rules called a Formal Grammar</skos:definition>
        <cco2:ont00001754 rdf:datatype="http://www.w3.org/2001/XMLSchema#anyURI">https://en.wikipedia.org/wiki/Formal_language</cco2:ont00001754>
    </owl:Class>
    


    <!-- https://hack.cybersystems.engineer/memex/ontologies/SeamlessDigitalEngineering#Formal_Method -->

    <owl:Class rdf:about="https://hack.cybersystems.engineer/memex/ontologies/SeamlessDigitalEngineering#Formal_Method">
        <owl:equivalentClass>
            <owl:Class>
                <owl:intersectionOf rdf:parseType="Collection">
                    <rdf:Description rdf:about="https://hack.cybersystems.engineer/memex/ontologies/SeamlessDigitalEngineering#Method"/>
                    <owl:Restriction>
                        <owl:onProperty rdf:resource="http://purl.obolibrary.org/obo/BFO_0000178"/>
                        <owl:someValuesFrom rdf:resource="https://hack.cybersystems.engineer/memex/ontologies/SeamlessDigitalEngineering#Formal_System"/>
                    </owl:Restriction>
                </owl:intersectionOf>
            </owl:Class>
        </owl:equivalentClass>
        <rdfs:subClassOf rdf:resource="https://hack.cybersystems.engineer/memex/ontologies/SeamlessDigitalEngineering#Method"/>
        <rdfs:label xml:lang="en">Formal Method</rdfs:label>
    </owl:Class>
    


    <!-- https://hack.cybersystems.engineer/memex/ontologies/SeamlessDigitalEngineering#Formal_Specification -->

    <owl:Class rdf:about="https://hack.cybersystems.engineer/memex/ontologies/SeamlessDigitalEngineering#Formal_Specification">
        <owl:equivalentClass>
            <owl:Class>
                <owl:intersectionOf rdf:parseType="Collection">
                    <rdf:Description rdf:about="https://hack.cybersystems.engineer/memex/ontologies/SeamlessDigitalEngineering#Information_Model"/>
                    <owl:Restriction>
                        <owl:onProperty rdf:resource="http://purl.obolibrary.org/obo/BFO_0000058"/>
                        <owl:someValuesFrom rdf:resource="https://hack.cybersystems.engineer/memex/ontologies/SeamlessDigitalEngineering#Act_of_Formal_Verification"/>
                    </owl:Restriction>
                </owl:intersectionOf>
            </owl:Class>
        </owl:equivalentClass>
        <rdfs:subClassOf rdf:resource="https://hack.cybersystems.engineer/memex/ontologies/SeamlessDigitalEngineering#Information_Model"/>
        <rdfs:label xml:lang="en">Formal Specification</rdfs:label>
        <rdfs:seeAlso xml:lang="en">Proof of Correctness</rdfs:seeAlso>
        <skos:definition xml:lang="en">specification that is used to prove mathematically the validity of an implementation or to derive mathematically the implementation</skos:definition>
        <cco2:ont00001754 xml:lang="en">ISO/IEC/IEEE 24765:2017 — Systems and software engineering — Vocabulary</cco2:ont00001754>
    </owl:Class>
    


    <!-- https://hack.cybersystems.engineer/memex/ontologies/SeamlessDigitalEngineering#Formal_System -->

    <owl:Class rdf:about="https://hack.cybersystems.engineer/memex/ontologies/SeamlessDigitalEngineering#Formal_System">
        <owl:equivalentClass>
            <owl:Class>
                <owl:intersectionOf rdf:parseType="Collection">
                    <rdf:Description rdf:about="https://hack.cybersystems.engineer/memex/ontologies/SeamlessDigitalEngineering#Formal_Language"/>
                    <owl:Restriction>
                        <owl:onProperty rdf:resource="http://purl.obolibrary.org/obo/BFO_0000058"/>
                        <owl:someValuesFrom rdf:resource="https://hack.cybersystems.engineer/memex/ontologies/SeamlessDigitalEngineering#Act_of_Logical_Inference"/>
                    </owl:Restriction>
                </owl:intersectionOf>
            </owl:Class>
        </owl:equivalentClass>
        <rdfs:subClassOf rdf:resource="https://hack.cybersystems.engineer/memex/ontologies/SeamlessDigitalEngineering#Formal_Language"/>
        <rdfs:label xml:lang="en">Formal System</rdfs:label>
        <skos:definition xml:lang="en">An abstract structure and formalization of an axiomatic system used for deducing, using rules of inference, theorems from axioms by a set of inference rules.</skos:definition>
        <cco2:ont00001754 rdf:datatype="http://www.w3.org/2001/XMLSchema#anyURI">https://en.wikipedia.org/wiki/Formal_system</cco2:ont00001754>
    </owl:Class>
    


    <!-- https://hack.cybersystems.engineer/memex/ontologies/SeamlessDigitalEngineering#Formal_Verification_Proof_Goal -->

    <owl:Class rdf:about="https://hack.cybersystems.engineer/memex/ontologies/SeamlessDigitalEngineering#Formal_Verification_Proof_Goal">
        <owl:equivalentClass>
            <owl:Class>
                <owl:intersectionOf rdf:parseType="Collection">
                    <owl:Restriction>
                        <owl:onProperty rdf:resource="http://purl.obolibrary.org/obo/BFO_0000101"/>
                        <owl:someValuesFrom rdf:resource="https://hack.cybersystems.engineer/memex/ontologies/SeamlessDigitalEngineering#Formal_Specification"/>
                    </owl:Restriction>
                    <owl:Restriction>
                        <owl:onProperty rdf:resource="https://www.commoncoreontologies.org/ont00001936"/>
                        <owl:someValuesFrom rdf:resource="https://hack.cybersystems.engineer/memex/ontologies/SeamlessDigitalEngineering#Act_of_Formal_Verification"/>
                    </owl:Restriction>
                </owl:intersectionOf>
            </owl:Class>
        </owl:equivalentClass>
        <rdfs:subClassOf rdf:resource="https://www.commoncoreontologies.org/ont00000253"/>
        <rdfs:label xml:lang="en">Formal Verification Proof Goal</rdfs:label>
    </owl:Class>
    


    <!-- https://hack.cybersystems.engineer/memex/ontologies/SeamlessDigitalEngineering#Freedom_from_Economic_Risk -->

    <owl:Class rdf:about="https://hack.cybersystems.engineer/memex/ontologies/SeamlessDigitalEngineering#Freedom_from_Economic_Risk">
        <rdfs:subClassOf rdf:resource="https://hack.cybersystems.engineer/memex/ontologies/SeamlessDigitalEngineering#Freedom_from_Risk"/>
        <rdfs:label xml:lang="en">Freedom from Economic Risk</rdfs:label>
        <skos:definition xml:lang="en">extent to which a Product or System mitigates the potential Risk to financial status, efficient operation, commercial property, reputation, or other aspects in the intended Contexts of Use</skos:definition>
        <cco2:ont00001754 xml:lang="en">ISO/IEC 25019:2023(en)
Systems and software engineering — Systems and software Quality Requirements and Evaluation (SQuaRE) — Quality-in-use model</cco2:ont00001754>
    </owl:Class>
    


    <!-- https://hack.cybersystems.engineer/memex/ontologies/SeamlessDigitalEngineering#Freedom_from_Environmental_and_Societal_Risk -->

    <owl:Class rdf:about="https://hack.cybersystems.engineer/memex/ontologies/SeamlessDigitalEngineering#Freedom_from_Environmental_and_Societal_Risk">
        <rdfs:subClassOf rdf:resource="https://hack.cybersystems.engineer/memex/ontologies/SeamlessDigitalEngineering#Freedom_from_Risk"/>
        <rdfs:label xml:lang="en">Freedom from Environmental and Societal Risk</rdfs:label>
        <skos:definition xml:lang="en">extent to which a Product or System mitigates the potential Risk to the environment and society at large in the intended Contexts of Use</skos:definition>
        <cco2:ont00001754 xml:lang="en">ISO/IEC 25019:2023(en)
Systems and software engineering — Systems and software Quality Requirements and Evaluation (SQuaRE) — Quality-in-use model</cco2:ont00001754>
    </owl:Class>
    


    <!-- https://hack.cybersystems.engineer/memex/ontologies/SeamlessDigitalEngineering#Freedom_from_Health_Risk -->

    <owl:Class rdf:about="https://hack.cybersystems.engineer/memex/ontologies/SeamlessDigitalEngineering#Freedom_from_Health_Risk">
        <rdfs:subClassOf rdf:resource="https://hack.cybersystems.engineer/memex/ontologies/SeamlessDigitalEngineering#Freedom_from_Risk"/>
        <rdfs:label xml:lang="en">Freedom from Health Risk</rdfs:label>
        <skos:definition xml:lang="en">extent to which a Product or System mitigates the potential Risk to people’s health in the intended Contexts of Use</skos:definition>
        <cco2:ont00001754 xml:lang="en">ISO/IEC 25019:2023(en)
Systems and software engineering — Systems and software Quality Requirements and Evaluation (SQuaRE) — Quality-in-use model</cco2:ont00001754>
    </owl:Class>
    


    <!-- https://hack.cybersystems.engineer/memex/ontologies/SeamlessDigitalEngineering#Freedom_from_Human_Life_Risk -->

    <owl:Class rdf:about="https://hack.cybersystems.engineer/memex/ontologies/SeamlessDigitalEngineering#Freedom_from_Human_Life_Risk">
        <rdfs:subClassOf rdf:resource="https://hack.cybersystems.engineer/memex/ontologies/SeamlessDigitalEngineering#Freedom_from_Risk"/>
        <rdfs:label xml:lang="en">Freedom from Human Life Risk</rdfs:label>
        <skos:definition xml:lang="en">extent to which a Product or System mitigates the potential Risk to people’s lives in the intended Contexts of Use</skos:definition>
        <cco2:ont00001754 xml:lang="en">ISO/IEC 25019:2023(en)
Systems and software engineering — Systems and software Quality Requirements and Evaluation (SQuaRE) — Quality-in-use model</cco2:ont00001754>
    </owl:Class>
    


    <!-- https://hack.cybersystems.engineer/memex/ontologies/SeamlessDigitalEngineering#Freedom_from_Risk -->

    <owl:Class rdf:about="https://hack.cybersystems.engineer/memex/ontologies/SeamlessDigitalEngineering#Freedom_from_Risk">
        <rdfs:subClassOf rdf:resource="https://hack.cybersystems.engineer/memex/ontologies/SeamlessDigitalEngineering#Product_Quality-in-Use"/>
        <rdfs:label xml:lang="en">Freedom from Risk</rdfs:label>
        <skos:definition xml:lang="en">extent to which a Product or System mitigates the potential Risk to economic status, human life, health, society, financial values, enterprise activities, or the environment</skos:definition>
        <cco2:ont00001754 xml:lang="en">ISO/IEC 25019:2023(en)
Systems and software engineering — Systems and software Quality Requirements and Evaluation (SQuaRE) — Quality-in-use model</cco2:ont00001754>
    </owl:Class>
    


    <!-- https://hack.cybersystems.engineer/memex/ontologies/SeamlessDigitalEngineering#Functional_Architecture -->

    <owl:Class rdf:about="https://hack.cybersystems.engineer/memex/ontologies/SeamlessDigitalEngineering#Functional_Architecture">
        <rdfs:subClassOf rdf:resource="https://hack.cybersystems.engineer/memex/ontologies/SeamlessDigitalEngineering#Architecture_View"/>
        <rdfs:label xml:lang="en">Functional Architecture</rdfs:label>
        <skos:altLabel xml:lang="en">Functional (View of) Architecture</skos:altLabel>
        <skos:definition xml:lang="en">ISO/IEC/IEEE 42010 conformant architecture description document will normally contain a view capturing the functions of the system of interest (it is not a 42010 normative requirement but would almost always be included). A functional architecture can be said to be the essential or organizing functional structure, the way abstracted inputs are transformed into outputs by the system to achieve its mission.</skos:definition>
        <cco2:ont00001754 xml:lang="en">ISO/IEC/IEEE 42020:2019</cco2:ont00001754>
    </owl:Class>
    


    <!-- https://hack.cybersystems.engineer/memex/ontologies/SeamlessDigitalEngineering#Functional_Programming_Language -->

    <owl:Class rdf:about="https://hack.cybersystems.engineer/memex/ontologies/SeamlessDigitalEngineering#Functional_Programming_Language">
        <rdfs:subClassOf rdf:resource="http://www.ontologyrepository.com/CommonCoreOntologies/HighLevelProgrammingLanguage"/>
        <rdfs:label xml:lang="en">Functional Programming Language</rdfs:label>
    </owl:Class>
    


    <!-- https://hack.cybersystems.engineer/memex/ontologies/SeamlessDigitalEngineering#Functional_Requirement -->

    <owl:Class rdf:about="https://hack.cybersystems.engineer/memex/ontologies/SeamlessDigitalEngineering#Functional_Requirement">
        <owl:equivalentClass>
            <owl:Class>
                <owl:intersectionOf rdf:parseType="Collection">
                    <rdf:Description rdf:about="https://hack.cybersystems.engineer/memex/ontologies/SeamlessDigitalEngineering#Requirement"/>
                    <rdf:Description rdf:about="https://www.commoncoreontologies.org/ont00000118"/>
                    <rdf:Description rdf:about="https://www.commoncoreontologies.org/ont00000127"/>
                </owl:intersectionOf>
            </owl:Class>
        </owl:equivalentClass>
        <rdfs:subClassOf rdf:resource="https://www.commoncoreontologies.org/ont00000127"/>
        <rdfs:comment xml:lang="en">A well-formed functional requirement includes the condition(s) and constraint(s) of when the functional performance is valid.</rdfs:comment>
        <rdfs:comment xml:lang="en">See INCOSE Needs &amp; Requirements Manual, attribute A40 - Type/Category.</rdfs:comment>
        <rdfs:label xml:lang="en">Functional Requirement</rdfs:label>
        <skos:definition xml:lang="en">Requirement that specifies a Function that a System or System Element performs</skos:definition>
        <cco2:ont00001754 xml:lang="en">ISO/IEC/IEEE 41062:2024, 3.1.8
Software engineering - Life cycle processes - Software acquisition</cco2:ont00001754>
    </owl:Class>
    


    <!-- https://hack.cybersystems.engineer/memex/ontologies/SeamlessDigitalEngineering#Functional_Unit -->

    <owl:Class rdf:about="https://hack.cybersystems.engineer/memex/ontologies/SeamlessDigitalEngineering#Functional_Unit">
        <owl:equivalentClass>
            <owl:Class>
                <owl:intersectionOf rdf:parseType="Collection">
                    <rdf:Description rdf:about="https://www.commoncoreontologies.org/ont00000740"/>
                    <owl:Class>
                        <owl:unionOf rdf:parseType="Collection">
                            <rdf:Description rdf:about="http://www.ontologyrepository.com/CommonCoreOntologies/ComputerComponent"/>
                            <rdf:Description rdf:about="http://www.ontologyrepository.com/CommonCoreOntologies/ComputerProgram"/>
                            <rdf:Description rdf:about="https://www.commoncoreontologies.org/ont00000420"/>
                        </owl:unionOf>
                    </owl:Class>
                </owl:intersectionOf>
            </owl:Class>
        </owl:equivalentClass>
        <rdfs:subClassOf rdf:resource="https://www.commoncoreontologies.org/ont00000740"/>
        <rdfs:label xml:lang="en">Functional Unit</rdfs:label>
        <skos:definition xml:lang="en">An entity of Computer Hardware or Software, or both (Computer), capable of accomplishing a specified Purpose</skos:definition>
        <cco2:ont00001754>ISO/IEC/IEEE 24765:2017, 3.1713</cco2:ont00001754>
        <cco2:ont00001760 rdf:datatype="http://www.w3.org/2001/XMLSchema#anyURI">https://semantic.incose.org/DEIX_Ontology</cco2:ont00001760>
    </owl:Class>
    


    <!-- https://hack.cybersystems.engineer/memex/ontologies/SeamlessDigitalEngineering#Functional_Viewpoint -->

    <owl:Class rdf:about="https://hack.cybersystems.engineer/memex/ontologies/SeamlessDigitalEngineering#Functional_Viewpoint">
        <owl:equivalentClass>
            <owl:Class>
                <owl:intersectionOf rdf:parseType="Collection">
                    <rdf:Description rdf:about="https://hack.cybersystems.engineer/memex/ontologies/SeamlessDigitalEngineering#Architecture_Viewpoint"/>
                    <owl:Restriction>
                        <owl:onProperty rdf:resource="https://www.commoncoreontologies.org/ont00001942"/>
                        <owl:someValuesFrom rdf:resource="https://hack.cybersystems.engineer/memex/ontologies/SeamlessDigitalEngineering#Functional_Architecture"/>
                    </owl:Restriction>
                </owl:intersectionOf>
            </owl:Class>
        </owl:equivalentClass>
        <rdfs:subClassOf rdf:resource="https://hack.cybersystems.engineer/memex/ontologies/SeamlessDigitalEngineering#Architecture_Viewpoint"/>
        <rdfs:label xml:lang="en">Functional Viewpoint</rdfs:label>
    </owl:Class>
    


    <!-- https://hack.cybersystems.engineer/memex/ontologies/SeamlessDigitalEngineering#Gain_of_Value -->

    <owl:Class rdf:about="https://hack.cybersystems.engineer/memex/ontologies/SeamlessDigitalEngineering#Gain_of_Value">
        <rdfs:subClassOf rdf:resource="https://www.commoncoreontologies.org/ont00001068"/>
        <rdfs:comment xml:lang="en">The Value of an entity is generally determined in terms of the amount of other entities for which it can be exchanged.</rdfs:comment>
        <rdfs:comment xml:lang="en">Value can be created, realized, acquired, redistributed, shared, lost, or destroyed.</rdfs:comment>
        <rdfs:comment xml:lang="en">Value can be financial or non-financial.</rdfs:comment>
        <rdfs:comment xml:lang="en">Value is relative to, and determined by the perception of, the Organization and Stakeholders.</rdfs:comment>
        <rdfs:label xml:lang="en">Gain of Value</rdfs:label>
        <skos:definition xml:lang="en">gains from satisfying Need and Expectations, in relation to the Resources used</skos:definition>
        <skos:example xml:lang="en">Revenue, savings, productivity, sustainability, satisfaction, empowerment, engagement, experience, trust.</skos:example>
        <cco2:ont00001754 xml:lang="en">ISO 56000:2020 - Innovation management - Fundamentals and vocabulary</cco2:ont00001754>
    </owl:Class>
    


    <!-- https://hack.cybersystems.engineer/memex/ontologies/SeamlessDigitalEngineering#Global_Region -->

    <owl:Class rdf:about="https://hack.cybersystems.engineer/memex/ontologies/SeamlessDigitalEngineering#Global_Region">
        <rdfs:subClassOf rdf:resource="https://www.commoncoreontologies.org/ont00000472"/>
        <rdfs:label xml:lang="en">Global Region</rdfs:label>
        <skos:definition xml:lang="en">the occupied regions of planet Earth, including up thru its exosphere</skos:definition>
    </owl:Class>
    


    <!-- https://hack.cybersystems.engineer/memex/ontologies/SeamlessDigitalEngineering#Goal -->

    <owl:Class rdf:about="https://hack.cybersystems.engineer/memex/ontologies/SeamlessDigitalEngineering#Goal">
        <owl:equivalentClass>
            <owl:Class>
                <owl:intersectionOf rdf:parseType="Collection">
                    <rdf:Description rdf:about="https://hack.cybersystems.engineer/memex/ontologies/SeamlessDigitalEngineering#Need"/>
                    <owl:Restriction>
                        <owl:onProperty rdf:resource="http://purl.obolibrary.org/obo/BFO_0000178"/>
                        <owl:someValuesFrom rdf:resource="https://www.commoncoreontologies.org/ont00000476"/>
                    </owl:Restriction>
                </owl:intersectionOf>
            </owl:Class>
        </owl:equivalentClass>
        <rdfs:subClassOf rdf:resource="https://hack.cybersystems.engineer/memex/ontologies/SeamlessDigitalEngineering#Need"/>
        <rdfs:comment xml:lang="en">Goals are elaborated from the Mission statement communicating those things that need to be achieved that will result in achieving the Mission.</rdfs:comment>
        <rdfs:comment xml:lang="en">Goals describe future Outcomes that will result in the Mission to be achieved.</rdfs:comment>
        <skos:definition xml:lang="en">Goals are upper-level Needs that form the second level of the hierarchy of the Integrated Set of Needs.</skos:definition>
        <cco2:ont00001754>INCOSE Needs and Requirements Manual R1.1 (2022)</cco2:ont00001754>
    </owl:Class>
    


    <!-- https://hack.cybersystems.engineer/memex/ontologies/SeamlessDigitalEngineering#Hazard -->

    <owl:Class rdf:about="https://hack.cybersystems.engineer/memex/ontologies/SeamlessDigitalEngineering#Hazard">
        <rdfs:subClassOf rdf:resource="https://www.commoncoreontologies.org/ont00000997"/>
        <rdfs:subClassOf>
            <owl:Restriction>
                <owl:onProperty rdf:resource="http://purl.obolibrary.org/obo/BFO_0000197"/>
                <owl:someValuesFrom rdf:resource="https://hack.cybersystems.engineer/memex/ontologies/SeamlessDigitalEngineering#Context_of_Use"/>
            </owl:Restriction>
        </rdfs:subClassOf>
        <rdfs:label xml:lang="en">Hazard</rdfs:label>
        <skos:definition xml:lang="en">source or situation with a potential for harm in terms of human injury or ill health (both short and long term), damage to property, damage to the environment, or a combination of these</skos:definition>
        <cco2:ont00001754>ISO/IEC/IEEE 41062:2024 — Software engineering — Life cycle processes — Software acquisition
IEEE 7000:2021</cco2:ont00001754>
    </owl:Class>
    


    <!-- https://hack.cybersystems.engineer/memex/ontologies/SeamlessDigitalEngineering#High-Integrity_Level -->

    <owl:Class rdf:about="https://hack.cybersystems.engineer/memex/ontologies/SeamlessDigitalEngineering#High-Integrity_Level">
        <rdfs:subClassOf rdf:resource="https://hack.cybersystems.engineer/memex/ontologies/SeamlessDigitalEngineering#Integrity_Level"/>
        <rdfs:label xml:lang="en">High-Integrity Level</rdfs:label>
    </owl:Class>
    


    <!-- https://hack.cybersystems.engineer/memex/ontologies/SeamlessDigitalEngineering#High-Integrity_Level_Claim -->

    <owl:Class rdf:about="https://hack.cybersystems.engineer/memex/ontologies/SeamlessDigitalEngineering#High-Integrity_Level_Claim">
        <owl:equivalentClass>
            <owl:Class>
                <owl:intersectionOf rdf:parseType="Collection">
                    <rdf:Description rdf:about="https://hack.cybersystems.engineer/memex/ontologies/SeamlessDigitalEngineering#Integrity_Level_Claim"/>
                    <owl:Restriction>
                        <owl:onProperty rdf:resource="https://www.commoncoreontologies.org/ont00001942"/>
                        <owl:someValuesFrom rdf:resource="https://hack.cybersystems.engineer/memex/ontologies/SeamlessDigitalEngineering#High-Integrity_Level"/>
                    </owl:Restriction>
                </owl:intersectionOf>
            </owl:Class>
        </owl:equivalentClass>
        <rdfs:subClassOf rdf:resource="https://hack.cybersystems.engineer/memex/ontologies/SeamlessDigitalEngineering#Integrity_Level_Claim"/>
        <rdfs:label xml:lang="en">High-Integrity Level Claim</rdfs:label>
    </owl:Class>
    


    <!-- https://hack.cybersystems.engineer/memex/ontologies/SeamlessDigitalEngineering#How-to_Guide -->

    <owl:Class rdf:about="https://hack.cybersystems.engineer/memex/ontologies/SeamlessDigitalEngineering#How-to_Guide">
        <rdfs:subClassOf rdf:resource="https://www.commoncoreontologies.org/ont00000798"/>
        <rdfs:subClassOf>
            <owl:Class>
                <owl:intersectionOf rdf:parseType="Collection">
                    <owl:Restriction>
                        <owl:onProperty rdf:resource="http://purl.obolibrary.org/obo/BFO_0000101"/>
                        <owl:someValuesFrom rdf:resource="https://hack.cybersystems.engineer/memex/ontologies/SeamlessDigitalEngineering#Goal"/>
                    </owl:Restriction>
                    <owl:Restriction>
                        <owl:onProperty rdf:resource="http://purl.obolibrary.org/obo/BFO_0000101"/>
                        <owl:someValuesFrom rdf:resource="https://hack.cybersystems.engineer/memex/ontologies/SeamlessDigitalEngineering#Problem_Definition"/>
                    </owl:Restriction>
                </owl:intersectionOf>
            </owl:Class>
        </rdfs:subClassOf>
        <rdfs:comment xml:lang="en">A How-to Guide helps the Stakeholder get something done, correctly and safely; it guides the User’s Act(s).</rdfs:comment>
        <rdfs:comment xml:lang="en">How-to Guides are Goal-oriented.</rdfs:comment>
        <rdfs:label xml:lang="en">How-to Guide</rdfs:label>
        <skos:definition xml:lang="en">Information Bearing Artifact that guides the Stakeholder through a Problem or towards a Process Outcome.</skos:definition>
        <cco2:ont00001754 rdf:datatype="http://www.w3.org/2001/XMLSchema#anyURI">https://diataxis.fr/how-to-guides/</cco2:ont00001754>
    </owl:Class>
    


    <!-- https://hack.cybersystems.engineer/memex/ontologies/SeamlessDigitalEngineering#Human-Centric_Design_Approach -->

    <owl:Class rdf:about="https://hack.cybersystems.engineer/memex/ontologies/SeamlessDigitalEngineering#Human-Centric_Design_Approach">
        <owl:equivalentClass>
            <owl:Class>
                <owl:intersectionOf rdf:parseType="Collection">
                    <owl:Restriction>
                        <owl:onProperty rdf:resource="https://www.commoncoreontologies.org/ont00001808"/>
                        <owl:someValuesFrom rdf:resource="https://hack.cybersystems.engineer/memex/ontologies/SeamlessDigitalEngineering#Human_Factors_Discipline"/>
                    </owl:Restriction>
                    <owl:Restriction>
                        <owl:onProperty rdf:resource="https://www.commoncoreontologies.org/ont00001942"/>
                        <owl:someValuesFrom>
                            <owl:Class>
                                <owl:unionOf rdf:parseType="Collection">
                                    <rdf:Description rdf:about="https://hack.cybersystems.engineer/memex/ontologies/SeamlessDigitalEngineering#System"/>
                                    <rdf:Description rdf:about="https://www.commoncoreontologies.org/ont00001262"/>
                                </owl:unionOf>
                            </owl:Class>
                        </owl:someValuesFrom>
                    </owl:Restriction>
                </owl:intersectionOf>
            </owl:Class>
        </owl:equivalentClass>
        <rdfs:subClassOf rdf:resource="https://hack.cybersystems.engineer/memex/ontologies/SeamlessDigitalEngineering#Design_Approach"/>
        <rdfs:comment xml:lang="en">Usable systems can provide a number of benefits, including improved productivity, enhanced user well-being, avoidance of stress, increased accessibility and reduced risk of harm. (ISO 9241-210:2019)</rdfs:comment>
        <rdfs:comment xml:lang="en">human-centred design:
approach to systems design and development that aims to make interactive systems more usable by focusing on the use of the system and applying human factors/ergonomics and usability knowledge and techniques (ISO 9241-210:2019)</rdfs:comment>
        <rdfs:label xml:lang="en">Human-Centric Design Approach</rdfs:label>
        <skos:definition xml:lang="en">Approach to interactive system development, focusing specifically on making systems usable, and emphasizing the role of human Operators as control agents who maintain Authority within a working System</skos:definition>
        <cco2:ont00001754 xml:lang="en">ISO 11064-1:2000
Ergonomic design of control centres
Part 1: Principles for the design of control centres</cco2:ont00001754>
    </owl:Class>
    


    <!-- https://hack.cybersystems.engineer/memex/ontologies/SeamlessDigitalEngineering#Human_Cyber_Right -->

    <owl:Class rdf:about="https://hack.cybersystems.engineer/memex/ontologies/SeamlessDigitalEngineering#Human_Cyber_Right">
        <rdfs:subClassOf rdf:resource="https://hack.cybersystems.engineer/memex/ontologies/SeamlessDigitalEngineering#Human_Rights"/>
        <rdfs:label xml:lang="en">Human Cyber Right</rdfs:label>
    </owl:Class>
    


    <!-- https://hack.cybersystems.engineer/memex/ontologies/SeamlessDigitalEngineering#Human_Factors_Discipline -->

    <owl:Class rdf:about="https://hack.cybersystems.engineer/memex/ontologies/SeamlessDigitalEngineering#Human_Factors_Discipline">
        <owl:equivalentClass>
            <owl:Class>
                <owl:intersectionOf rdf:parseType="Collection">
                    <rdf:Description rdf:about="https://hack.cybersystems.engineer/memex/ontologies/SeamlessDigitalEngineering#Scientific_Discipline"/>
                    <owl:Restriction>
                        <owl:onProperty rdf:resource="https://www.commoncoreontologies.org/ont00001808"/>
                        <owl:someValuesFrom>
                            <owl:Class>
                                <owl:intersectionOf rdf:parseType="Collection">
                                    <rdf:Description rdf:about="https://hack.cybersystems.engineer/memex/ontologies/SeamlessDigitalEngineering#System"/>
                                    <rdf:Description rdf:about="https://www.commoncoreontologies.org/ont00001262"/>
                                </owl:intersectionOf>
                            </owl:Class>
                        </owl:someValuesFrom>
                    </owl:Restriction>
                </owl:intersectionOf>
            </owl:Class>
        </owl:equivalentClass>
        <rdfs:subClassOf rdf:resource="https://hack.cybersystems.engineer/memex/ontologies/SeamlessDigitalEngineering#Scientific_Discipline"/>
        <rdfs:label xml:lang="en">Human Factors Discipline</rdfs:label>
        <skos:altLabel xml:lang="en">Ergonomics</skos:altLabel>
        <skos:definition xml:lang="en">Scientific Discipline concerned with the understanding of interactions among human and other elements of a System, and the profession that applies theory, Principles, Data and Methods to design in order to optimize human well-being and overall System Performance</skos:definition>
        <cco2:ont00001754 xml:lang="en">ISO 9241-210:2019
Ergonomics of human-system interaction
Part 210: Human-centred design for interactive systems</cco2:ont00001754>
    </owl:Class>
    


    <!-- https://hack.cybersystems.engineer/memex/ontologies/SeamlessDigitalEngineering#Human_Resource_Management_Process -->

    <owl:Class rdf:about="https://hack.cybersystems.engineer/memex/ontologies/SeamlessDigitalEngineering#Human_Resource_Management_Process">
        <rdfs:subClassOf rdf:resource="https://hack.cybersystems.engineer/memex/ontologies/SeamlessDigitalEngineering#Organizational_Project-enabling_Process"/>
        <rdfs:label xml:lang="en">Human Resource Management Process</rdfs:label>
        <skos:definition xml:lang="en">The purpose of the human resource management process is to provide the organization with necessary human resources and to maintain their competencies, consistent with strategic needs.</skos:definition>
        <cco2:ont00001754>ISO/IEC/IEEE 15288:2023</cco2:ont00001754>
    </owl:Class>
    


    <!-- https://hack.cybersystems.engineer/memex/ontologies/SeamlessDigitalEngineering#Human_Right -->

    <owl:Class rdf:about="https://hack.cybersystems.engineer/memex/ontologies/SeamlessDigitalEngineering#Human_Right">
        <owl:equivalentClass>
            <owl:Class>
                <owl:intersectionOf rdf:parseType="Collection">
                    <rdf:Description rdf:about="https://hack.cybersystems.engineer/memex/ontologies/SeamlessDigitalEngineering#Right"/>
                    <owl:Restriction>
                        <owl:onProperty rdf:resource="http://purl.obolibrary.org/obo/BFO_0000195"/>
                        <owl:someValuesFrom rdf:resource="https://www.commoncoreontologies.org/ont00001262"/>
                    </owl:Restriction>
                </owl:intersectionOf>
            </owl:Class>
        </owl:equivalentClass>
        <rdfs:subClassOf rdf:resource="https://hack.cybersystems.engineer/memex/ontologies/SeamlessDigitalEngineering#Right"/>
        <rdfs:label xml:lang="en">Human Right</rdfs:label>
        <skos:definition xml:lang="en">Right to which every Person is entitled</skos:definition>
        <cco2:ont00001754 xml:lang="en">ISO/IEC/IEEE 24738-7000:2022 (3.1.33)
Systems and software engineering - Life cycle management - Part 7000: Standard model process for addressing ethical concerns during system design</cco2:ont00001754>
    </owl:Class>
    


    <!-- https://hack.cybersystems.engineer/memex/ontologies/SeamlessDigitalEngineering#Human_Rights -->

    <owl:Class rdf:about="https://hack.cybersystems.engineer/memex/ontologies/SeamlessDigitalEngineering#Human_Rights">
        <owl:equivalentClass>
            <owl:Class>
                <owl:intersectionOf rdf:parseType="Collection">
                    <owl:Restriction>
                        <owl:onProperty rdf:resource="http://purl.obolibrary.org/obo/BFO_0000084"/>
                        <owl:someValuesFrom rdf:resource="https://www.commoncoreontologies.org/ont00001017"/>
                    </owl:Restriction>
                    <owl:Restriction>
                        <owl:onProperty rdf:resource="https://www.commoncoreontologies.org/ont00001808"/>
                        <owl:someValuesFrom rdf:resource="https://hack.cybersystems.engineer/memex/ontologies/SeamlessDigitalEngineering#Right"/>
                    </owl:Restriction>
                </owl:intersectionOf>
            </owl:Class>
        </owl:equivalentClass>
        <rdfs:subClassOf rdf:resource="https://www.commoncoreontologies.org/ont00000696"/>
        <rdfs:label xml:lang="en">Agent Right</rdfs:label>
        <rdfs:seeAlso rdf:resource="https://hack.cybersystems.engineer/memex/ontologies/SeamlessDigitalEngineering#Right"/>
    </owl:Class>
    


    <!-- https://hack.cybersystems.engineer/memex/ontologies/SeamlessDigitalEngineering#IT_Service -->

    <owl:Class rdf:about="https://hack.cybersystems.engineer/memex/ontologies/SeamlessDigitalEngineering#IT_Service">
        <owl:equivalentClass>
            <owl:Class>
                <owl:intersectionOf rdf:parseType="Collection">
                    <rdf:Description rdf:about="https://hack.cybersystems.engineer/memex/ontologies/SeamlessDigitalEngineering#Service"/>
                    <owl:Restriction>
                        <owl:onProperty rdf:resource="http://purl.obolibrary.org/obo/BFO_0000054"/>
                        <owl:someValuesFrom rdf:resource="https://hack.cybersystems.engineer/memex/ontologies/SeamlessDigitalEngineering#Act_of_Digital_Tool_Use"/>
                    </owl:Restriction>
                </owl:intersectionOf>
            </owl:Class>
        </owl:equivalentClass>
        <rdfs:subClassOf rdf:resource="https://hack.cybersystems.engineer/memex/ontologies/SeamlessDigitalEngineering#Service"/>
        <rdfs:label xml:lang="en">IT Service</rdfs:label>
        <skos:definition xml:lang="en">Service that makes use of IT systems as Tools to provide value to an individual User or a Business by facilitating results the User or Business wants to achieve.</skos:definition>
        <cco2:ont00001754 xml:lang="en">ISO/IEC 25002:2024 Systems and software engineering - Systems and software Quality Requirements and Evaluation (SQuaRE) - Quality model overview and usage</cco2:ont00001754>
    </owl:Class>
    


    <!-- https://hack.cybersystems.engineer/memex/ontologies/SeamlessDigitalEngineering#IT_Service_Quality -->

    <owl:Class rdf:about="https://hack.cybersystems.engineer/memex/ontologies/SeamlessDigitalEngineering#IT_Service_Quality">
        <owl:equivalentClass>
            <owl:Class>
                <owl:intersectionOf rdf:parseType="Collection">
                    <rdf:Description rdf:about="https://hack.cybersystems.engineer/memex/ontologies/SeamlessDigitalEngineering#Quality"/>
                    <owl:Restriction>
                        <owl:onProperty rdf:resource="http://purl.obolibrary.org/obo/BFO_0000195"/>
                        <owl:someValuesFrom rdf:resource="https://hack.cybersystems.engineer/memex/ontologies/SeamlessDigitalEngineering#IT_Service"/>
                    </owl:Restriction>
                    <owl:Restriction>
                        <owl:onProperty rdf:resource="https://www.commoncoreontologies.org/ont00001947"/>
                        <owl:someValuesFrom rdf:resource="https://hack.cybersystems.engineer/memex/ontologies/SeamlessDigitalEngineering#Digital_Environment"/>
                    </owl:Restriction>
                </owl:intersectionOf>
            </owl:Class>
        </owl:equivalentClass>
        <rdfs:subClassOf rdf:resource="https://hack.cybersystems.engineer/memex/ontologies/SeamlessDigitalEngineering#Quality"/>
        <rdfs:label xml:lang="en">IT Service Quality</rdfs:label>
        <skos:definition xml:lang="en">capability of an IT Service to satisfy stated and implied Quality Needs when delivered under specified conditions</skos:definition>
        <cco2:ont00001754 xml:lang="en">ISO/IEC 25002:2024 Systems and software engineering - Systems and software Quality Requirements and Evaluation (SQuaRE) - Quality model overview and usage</cco2:ont00001754>
    </owl:Class>
    


    <!-- https://hack.cybersystems.engineer/memex/ontologies/SeamlessDigitalEngineering#Implementation_Process -->

    <owl:Class rdf:about="https://hack.cybersystems.engineer/memex/ontologies/SeamlessDigitalEngineering#Implementation_Process">
        <rdfs:subClassOf rdf:resource="https://hack.cybersystems.engineer/memex/ontologies/SeamlessDigitalEngineering#Technical_Process"/>
        <rdfs:label xml:lang="en">Implementation Process</rdfs:label>
        <skos:definition xml:lang="en">The purpose of the implementation process is to realise a specified system element.</skos:definition>
        <cco2:ont00001754>ISO/IEC/IEEE 15288:2023</cco2:ont00001754>
    </owl:Class>
    


    <!-- https://hack.cybersystems.engineer/memex/ontologies/SeamlessDigitalEngineering#Incident_Report -->

    <owl:Class rdf:about="https://hack.cybersystems.engineer/memex/ontologies/SeamlessDigitalEngineering#Incident_Report">
        <rdfs:subClassOf rdf:resource="https://www.commoncoreontologies.org/ont00000624"/>
    </owl:Class>
    


    <!-- https://hack.cybersystems.engineer/memex/ontologies/SeamlessDigitalEngineering#Incomplete_Assurance_Case_Report -->

    <owl:Class rdf:about="https://hack.cybersystems.engineer/memex/ontologies/SeamlessDigitalEngineering#Incomplete_Assurance_Case_Report">
        <owl:equivalentClass>
            <owl:Class>
                <owl:intersectionOf rdf:parseType="Collection">
                    <rdf:Description rdf:about="https://hack.cybersystems.engineer/memex/ontologies/SeamlessDigitalEngineering#Assurance_Case_Report"/>
                    <owl:Restriction>
                        <owl:onProperty rdf:resource="http://purl.obolibrary.org/obo/BFO_0000115"/>
                        <owl:someValuesFrom rdf:resource="https://hack.cybersystems.engineer/memex/ontologies/SeamlessDigitalEngineering#Incomplete_Assurance_Claim_Record"/>
                    </owl:Restriction>
                </owl:intersectionOf>
            </owl:Class>
        </owl:equivalentClass>
        <rdfs:subClassOf rdf:resource="https://hack.cybersystems.engineer/memex/ontologies/SeamlessDigitalEngineering#Assurance_Case_Report"/>
        <rdfs:label xml:lang="en">Incomplete Assurance Case Report</rdfs:label>
    </owl:Class>
    


    <!-- https://hack.cybersystems.engineer/memex/ontologies/SeamlessDigitalEngineering#Incomplete_Assurance_Claim_Record -->

    <owl:Class rdf:about="https://hack.cybersystems.engineer/memex/ontologies/SeamlessDigitalEngineering#Incomplete_Assurance_Claim_Record">
        <owl:equivalentClass>
            <owl:Class>
                <owl:intersectionOf rdf:parseType="Collection">
                    <rdf:Description rdf:about="https://hack.cybersystems.engineer/memex/ontologies/SeamlessDigitalEngineering#Assurance_Claim_Record"/>
                    <owl:Restriction>
                        <owl:onProperty rdf:resource="http://purl.obolibrary.org/obo/BFO_0000115"/>
                        <owl:someValuesFrom rdf:resource="https://hack.cybersystems.engineer/memex/ontologies/SeamlessDigitalEngineering#Undeveloped_Assurance_Argument_Record"/>
                    </owl:Restriction>
                </owl:intersectionOf>
            </owl:Class>
        </owl:equivalentClass>
        <rdfs:subClassOf rdf:resource="https://hack.cybersystems.engineer/memex/ontologies/SeamlessDigitalEngineering#Assurance_Claim_Record"/>
        <owl:disjointWith rdf:resource="https://hack.cybersystems.engineer/memex/ontologies/SeamlessDigitalEngineering#Supported_Assurance_Claim_Record"/>
        <rdfs:label xml:lang="en">Incomplete Assurance Claim Record</rdfs:label>
    </owl:Class>
    


    <!-- https://hack.cybersystems.engineer/memex/ontologies/SeamlessDigitalEngineering#Individual_Knowledge -->

    <owl:Class rdf:about="https://hack.cybersystems.engineer/memex/ontologies/SeamlessDigitalEngineering#Individual_Knowledge">
        <owl:equivalentClass>
            <owl:Class>
                <owl:intersectionOf rdf:parseType="Collection">
                    <rdf:Description rdf:about="https://www.commoncoreontologies.org/ont00001379"/>
                    <owl:Restriction>
                        <owl:onProperty rdf:resource="http://purl.obolibrary.org/obo/BFO_0000059"/>
                        <owl:someValuesFrom rdf:resource="https://hack.cybersystems.engineer/memex/ontologies/SeamlessDigitalEngineering#Knowledge"/>
                    </owl:Restriction>
                    <owl:Restriction>
                        <owl:onProperty rdf:resource="https://www.commoncoreontologies.org/ont00001889"/>
                        <owl:someValuesFrom rdf:resource="https://www.commoncoreontologies.org/ont00001262"/>
                    </owl:Restriction>
                </owl:intersectionOf>
            </owl:Class>
        </owl:equivalentClass>
        <rdfs:subClassOf rdf:resource="https://www.commoncoreontologies.org/ont00001379"/>
        <rdfs:label xml:lang="en">Individual Knowledge</rdfs:label>
        <skos:definition xml:lang="en">Knowledge present in, and disposable to, a given human individual</skos:definition>
        <cco2:ont00001754 xml:lang="en">ISO 5127:2017 — Information and documentation — Foundation and vocabulary</cco2:ont00001754>
    </owl:Class>
    


    <!-- https://hack.cybersystems.engineer/memex/ontologies/SeamlessDigitalEngineering#Inference_Argument -->

    <owl:Class rdf:about="https://hack.cybersystems.engineer/memex/ontologies/SeamlessDigitalEngineering#Inference_Argument">
        <owl:equivalentClass>
            <owl:Class>
                <owl:intersectionOf rdf:parseType="Collection">
                    <rdf:Description rdf:about="https://hack.cybersystems.engineer/memex/ontologies/SeamlessDigitalEngineering#Argument"/>
                    <owl:Restriction>
                        <owl:onProperty rdf:resource="http://purl.obolibrary.org/obo/BFO_0000178"/>
                        <owl:someValuesFrom rdf:resource="https://hack.cybersystems.engineer/memex/ontologies/SeamlessDigitalEngineering#Supported_Claim"/>
                    </owl:Restriction>
                </owl:intersectionOf>
            </owl:Class>
        </owl:equivalentClass>
        <rdfs:subClassOf rdf:resource="https://hack.cybersystems.engineer/memex/ontologies/SeamlessDigitalEngineering#Argument"/>
        <rdfs:label xml:lang="en">Inference Argument</rdfs:label>
        <skos:definition xml:lang="en">Argument derived from premises, Supported Claims, that produces a conclusion, Claim Derived by Inference.</skos:definition>
        <cco2:ont00001754 xml:lang="en">ISO/IEC/IEEE 15026-2:2022</cco2:ont00001754>
    </owl:Class>
    


    <!-- https://hack.cybersystems.engineer/memex/ontologies/SeamlessDigitalEngineering#Inference_Argument_Record -->

    <owl:Class rdf:about="https://hack.cybersystems.engineer/memex/ontologies/SeamlessDigitalEngineering#Inference_Argument_Record">
        <owl:equivalentClass>
            <owl:Class>
                <owl:intersectionOf rdf:parseType="Collection">
                    <rdf:Description rdf:about="https://hack.cybersystems.engineer/memex/ontologies/SeamlessDigitalEngineering#Assurance_Argument_Record"/>
                    <owl:Restriction>
                        <owl:onProperty rdf:resource="http://purl.obolibrary.org/obo/BFO_0000101"/>
                        <owl:someValuesFrom rdf:resource="https://hack.cybersystems.engineer/memex/ontologies/SeamlessDigitalEngineering#Inference_Argument"/>
                    </owl:Restriction>
                </owl:intersectionOf>
            </owl:Class>
        </owl:equivalentClass>
        <rdfs:subClassOf rdf:resource="https://hack.cybersystems.engineer/memex/ontologies/SeamlessDigitalEngineering#Assurance_Argument_Record"/>
        <rdfs:comment xml:lang="en">An Inference Argument Record lacks the Assurance Contexts needed to form a complete Assurance Argument Record.</rdfs:comment>
        <rdfs:label xml:lang="en">Inference Argument Record</rdfs:label>
        <skos:definition xml:lang="en">a Record that combines Supported Claim Records to form an Inference Argument</skos:definition>
        <cco2:ont00001754 xml:lang="en">ISO/IEC/15026-2:2022</cco2:ont00001754>
    </owl:Class>
    


    <!-- https://hack.cybersystems.engineer/memex/ontologies/SeamlessDigitalEngineering#Information_Appliance -->

    <owl:Class rdf:about="https://hack.cybersystems.engineer/memex/ontologies/SeamlessDigitalEngineering#Information_Appliance">
        <owl:equivalentClass>
            <owl:Class>
                <owl:intersectionOf rdf:parseType="Collection">
                    <rdf:Description rdf:about="https://hack.cybersystems.engineer/memex/ontologies/SeamlessDigitalEngineering#Appliance"/>
                    <owl:Restriction>
                        <owl:onProperty rdf:resource="https://www.commoncoreontologies.org/ont00001787"/>
                        <owl:someValuesFrom>
                            <owl:Class>
                                <owl:intersectionOf rdf:parseType="Collection">
                                    <rdf:Description rdf:about="http://www.ontologyrepository.com/CommonCoreOntologies/DataTransfer"/>
                                    <rdf:Description rdf:about="https://hack.cybersystems.engineer/memex/ontologies/SeamlessDigitalEngineering#Activity"/>
                                    <rdf:Description rdf:about="https://hack.cybersystems.engineer/memex/ontologies/SeamlessDigitalEngineering#Computing_Process"/>
                                </owl:intersectionOf>
                            </owl:Class>
                        </owl:someValuesFrom>
                    </owl:Restriction>
                </owl:intersectionOf>
            </owl:Class>
        </owl:equivalentClass>
        <rdfs:subClassOf rdf:resource="http://www.ontologyrepository.com/CommonCoreOntologies/ComputerSystem"/>
        <rdfs:subClassOf rdf:resource="https://hack.cybersystems.engineer/memex/ontologies/SeamlessDigitalEngineering#Appliance"/>
        <rdfs:label xml:lang="en">Information Appliance</rdfs:label>
        <skos:definition xml:lang="en">An appliance specializing in information: knowledge, facts, graphics, images, video, or sound. An information appliance is designed to perform a specific activity, such as music, photography, or writing. A distinguishing feature of information appliances is the ability to share information among themselves.</skos:definition>
        <cco2:ont00001754 xml:lang="en">Information Appliances and Beyond (Interactive Technologies), 1st edition</cco2:ont00001754>
    </owl:Class>
    


    <!-- https://hack.cybersystems.engineer/memex/ontologies/SeamlessDigitalEngineering#Information_Architecture -->

    <owl:Class rdf:about="https://hack.cybersystems.engineer/memex/ontologies/SeamlessDigitalEngineering#Information_Architecture">
        <owl:equivalentClass>
            <owl:Restriction>
                <owl:onProperty rdf:resource="https://www.commoncoreontologies.org/ont00001942"/>
                <owl:someValuesFrom rdf:resource="https://hack.cybersystems.engineer/memex/ontologies/SeamlessDigitalEngineering#Documentation"/>
            </owl:Restriction>
        </owl:equivalentClass>
        <rdfs:subClassOf rdf:resource="https://hack.cybersystems.engineer/memex/ontologies/SeamlessDigitalEngineering#Architecture"/>
        <rdfs:label xml:lang="en">Information Architecture</rdfs:label>
        <skos:definition xml:lang="en">structure of an Information space and the semantics for accessing Information on Tasks, System Functions and features, and other Information</skos:definition>
        <cco2:ont00001754 xml:lang="en">ISO/IEC/IEEE 26514:2022
Systems and software engineering
Design and development of information for users</cco2:ont00001754>
    </owl:Class>
    


    <!-- https://hack.cybersystems.engineer/memex/ontologies/SeamlessDigitalEngineering#Information_Management_Process -->

    <owl:Class rdf:about="https://hack.cybersystems.engineer/memex/ontologies/SeamlessDigitalEngineering#Information_Management_Process">
        <rdfs:subClassOf rdf:resource="https://hack.cybersystems.engineer/memex/ontologies/SeamlessDigitalEngineering#Technical_Management_Process"/>
        <rdfs:label xml:lang="en">Information Management Process</rdfs:label>
        <skos:definition xml:lang="en">The purpose of the information management process is to generate, obtain, confirm, transform, retain, retrieve, disseminate, and dispose of information for designated stakeholders.</skos:definition>
        <cco2:ont00001754>ISO/IEC/IEEE 15288:2023</cco2:ont00001754>
    </owl:Class>
    


    <!-- https://hack.cybersystems.engineer/memex/ontologies/SeamlessDigitalEngineering#Information_Model -->

    <owl:Class rdf:about="https://hack.cybersystems.engineer/memex/ontologies/SeamlessDigitalEngineering#Information_Model">
        <owl:equivalentClass>
            <owl:Class>
                <owl:intersectionOf rdf:parseType="Collection">
                    <rdf:Description rdf:about="https://www.commoncoreontologies.org/ont00000965"/>
                    <owl:Restriction>
                        <owl:onProperty rdf:resource="https://www.commoncoreontologies.org/ont00001942"/>
                        <owl:someValuesFrom rdf:resource="https://www.commoncoreontologies.org/ont00000958"/>
                    </owl:Restriction>
                </owl:intersectionOf>
            </owl:Class>
        </owl:equivalentClass>
        <rdfs:subClassOf rdf:resource="https://www.commoncoreontologies.org/ont00000965"/>
        <rdfs:label xml:lang="en">Information Model</rdfs:label>
        <skos:altLabel xml:lang="en">Formal Model</skos:altLabel>
        <skos:definition xml:lang="en">formal model of Information</skos:definition>
        <skos:example xml:lang="en">ISO 10303-242 provides an information model.</skos:example>
        <cco2:ont00001754 xml:lang="en">ISO 10303-2:2024 Industrial automation systems and integration - Product data representation and exchange - Part 2: Vocabulary, 3.1.228</cco2:ont00001754>
    </owl:Class>
    


    <!-- https://hack.cybersystems.engineer/memex/ontologies/SeamlessDigitalEngineering#Information_Need -->

    <owl:Class rdf:about="https://hack.cybersystems.engineer/memex/ontologies/SeamlessDigitalEngineering#Information_Need">
        <owl:equivalentClass>
            <owl:Class>
                <owl:intersectionOf rdf:parseType="Collection">
                    <rdf:Description rdf:about="https://hack.cybersystems.engineer/memex/ontologies/SeamlessDigitalEngineering#Insight"/>
                    <owl:Restriction>
                        <owl:onProperty rdf:resource="https://www.commoncoreontologies.org/ont00001808"/>
                        <owl:someValuesFrom rdf:resource="https://hack.cybersystems.engineer/memex/ontologies/SeamlessDigitalEngineering#System_Lifecycle_Process"/>
                    </owl:Restriction>
                    <owl:Restriction>
                        <owl:onProperty rdf:resource="https://www.commoncoreontologies.org/ont00001808"/>
                        <owl:someValuesFrom>
                            <owl:Class>
                                <owl:unionOf rdf:parseType="Collection">
                                    <rdf:Description rdf:about="https://hack.cybersystems.engineer/memex/ontologies/SeamlessDigitalEngineering#Goal"/>
                                    <rdf:Description rdf:about="https://hack.cybersystems.engineer/memex/ontologies/SeamlessDigitalEngineering#Problem"/>
                                    <rdf:Description rdf:about="https://hack.cybersystems.engineer/memex/ontologies/SeamlessDigitalEngineering#Risk"/>
                                    <rdf:Description rdf:about="https://www.commoncoreontologies.org/ont00000476"/>
                                </owl:unionOf>
                            </owl:Class>
                        </owl:someValuesFrom>
                    </owl:Restriction>
                </owl:intersectionOf>
            </owl:Class>
        </owl:equivalentClass>
        <rdfs:subClassOf rdf:resource="https://hack.cybersystems.engineer/memex/ontologies/SeamlessDigitalEngineering#Insight"/>
        <rdfs:comment xml:lang="en">Information Needs originate from the Technical and Management Processes.</rdfs:comment>
        <rdfs:comment xml:lang="en">The Information Needs can be derived from the business, organizational, regulatory (such as legal or governmental), Product or Project Objectives.</rdfs:comment>
        <rdfs:label xml:lang="en">Information Need</rdfs:label>
        <skos:definition xml:lang="en">An Insight necessary to manage Objectives, Goals, Risks and Problems</skos:definition>
        <cco2:ont00001754 xml:lang="en">ISO/IEC 25040:2024</cco2:ont00001754>
    </owl:Class>
    


    <!-- https://hack.cybersystems.engineer/memex/ontologies/SeamlessDigitalEngineering#Information_Part -->

    <owl:Class rdf:about="https://hack.cybersystems.engineer/memex/ontologies/SeamlessDigitalEngineering#Information_Part">
        <owl:equivalentClass>
            <owl:Class>
                <owl:intersectionOf rdf:parseType="Collection">
                    <rdf:Description rdf:about="https://www.commoncoreontologies.org/ont00000958"/>
                    <owl:Restriction>
                        <owl:onProperty rdf:resource="http://purl.obolibrary.org/obo/BFO_0000176"/>
                        <owl:someValuesFrom rdf:resource="https://www.commoncoreontologies.org/ont00000958"/>
                    </owl:Restriction>
                </owl:intersectionOf>
            </owl:Class>
        </owl:equivalentClass>
        <rdfs:subClassOf rdf:resource="https://www.commoncoreontologies.org/ont00000958"/>
        <rdfs:label xml:lang="en">Information Part</rdfs:label>
        <skos:altLabel xml:lang="en">Information Item</skos:altLabel>
        <skos:definition xml:lang="en">separately identifiable body of Information that is produced, stored, and delivered for human and machine use</skos:definition>
        <cco2:ont00001754 xml:lang="en">ISO/IEC/IEEE 42010:2022</cco2:ont00001754>
    </owl:Class>
    


    <!-- https://hack.cybersystems.engineer/memex/ontologies/SeamlessDigitalEngineering#Information_System -->

    <owl:Class rdf:about="https://hack.cybersystems.engineer/memex/ontologies/SeamlessDigitalEngineering#Information_System">
        <owl:equivalentClass>
            <owl:Class>
                <owl:intersectionOf rdf:parseType="Collection">
                    <owl:Restriction>
                        <owl:onProperty rdf:resource="http://purl.obolibrary.org/obo/BFO_0000101"/>
                        <owl:someValuesFrom rdf:resource="https://hack.cybersystems.engineer/memex/ontologies/SeamlessDigitalEngineering#Procedure"/>
                    </owl:Restriction>
                    <owl:Restriction>
                        <owl:onProperty rdf:resource="http://purl.obolibrary.org/obo/BFO_0000115"/>
                        <owl:someValuesFrom>
                            <owl:Class>
                                <owl:intersectionOf rdf:parseType="Collection">
                                    <rdf:Description rdf:about="https://hack.cybersystems.engineer/memex/ontologies/SeamlessDigitalEngineering#Data"/>
                                    <rdf:Description rdf:about="https://www.commoncoreontologies.org/ont00000740"/>
                                </owl:intersectionOf>
                            </owl:Class>
                        </owl:someValuesFrom>
                    </owl:Restriction>
                    <owl:Restriction>
                        <owl:onProperty rdf:resource="https://www.commoncoreontologies.org/ont00001852"/>
                        <owl:someValuesFrom rdf:resource="https://hack.cybersystems.engineer/memex/ontologies/SeamlessDigitalEngineering#Organizational_Project-enabling_Process"/>
                    </owl:Restriction>
                </owl:intersectionOf>
            </owl:Class>
        </owl:equivalentClass>
        <rdfs:subClassOf rdf:resource="https://hack.cybersystems.engineer/memex/ontologies/SeamlessDigitalEngineering#Digital_Environment"/>
        <rdfs:label xml:lang="en">Information System</rdfs:label>
        <skos:definition xml:lang="en">set of Resources, Procedures and Data required in support of Organizational Project-enabling Processes</skos:definition>
        <cco2:ont00001754 xml:lang="en">derived from ISO 10795:2019(en) - Space systems — Programme management and quality — Vocabulary</cco2:ont00001754>
    </owl:Class>
    


    <!-- https://hack.cybersystems.engineer/memex/ontologies/SeamlessDigitalEngineering#Infrastructure_Management_Process -->

    <owl:Class rdf:about="https://hack.cybersystems.engineer/memex/ontologies/SeamlessDigitalEngineering#Infrastructure_Management_Process">
        <rdfs:subClassOf rdf:resource="https://hack.cybersystems.engineer/memex/ontologies/SeamlessDigitalEngineering#Organizational_Project-enabling_Process"/>
        <rdfs:label xml:lang="en">Infrastructure Management Process</rdfs:label>
        <skos:definition xml:lang="en">The purpose of the infrastructure management process is to provide the infrastructure and services to projects to support organization and project objectives throughout the life cycle.</skos:definition>
        <cco2:ont00001754>ISO/IEC/IEEE 15288:2023</cco2:ont00001754>
    </owl:Class>
    


    <!-- https://hack.cybersystems.engineer/memex/ontologies/SeamlessDigitalEngineering#Insight -->

    <owl:Class rdf:about="https://hack.cybersystems.engineer/memex/ontologies/SeamlessDigitalEngineering#Insight">
        <rdfs:subClassOf rdf:resource="https://hack.cybersystems.engineer/memex/ontologies/SeamlessDigitalEngineering#Knowledge"/>
        <rdfs:comment xml:lang="en">Identifying Insights is generally part of the Innovation Processes.</rdfs:comment>
        <rdfs:comment xml:lang="en">In the context of Innovation Activities, Insights can reveal Opportunities for the realization of Value.</rdfs:comment>
        <rdfs:label xml:lang="en">Insight</rdfs:label>
        <skos:definition xml:lang="en">profound and unique Knowledge about an entity</skos:definition>
        <cco2:ont00001754 xml:lang="en">ISO 56000:2020 - Innovation management - Fundamentals and vocabulary</cco2:ont00001754>
    </owl:Class>
    


    <!-- https://hack.cybersystems.engineer/memex/ontologies/SeamlessDigitalEngineering#Inspection_Report -->

    <owl:Class rdf:about="https://hack.cybersystems.engineer/memex/ontologies/SeamlessDigitalEngineering#Inspection_Report">
        <owl:equivalentClass>
            <owl:Class>
                <owl:intersectionOf rdf:parseType="Collection">
                    <rdf:Description rdf:about="https://hack.cybersystems.engineer/memex/ontologies/SeamlessDigitalEngineering#Evaluation_Report"/>
                    <owl:Restriction>
                        <owl:onProperty rdf:resource="http://purl.obolibrary.org/obo/BFO_0000101"/>
                        <owl:someValuesFrom rdf:resource="https://hack.cybersystems.engineer/memex/ontologies/SeamlessDigitalEngineering#Conformity_Measure"/>
                    </owl:Restriction>
                </owl:intersectionOf>
            </owl:Class>
        </owl:equivalentClass>
        <rdfs:subClassOf rdf:resource="https://hack.cybersystems.engineer/memex/ontologies/SeamlessDigitalEngineering#Evaluation_Report"/>
        <rdfs:label xml:lang="en">Inspection Report</rdfs:label>
    </owl:Class>
    


    <!-- https://hack.cybersystems.engineer/memex/ontologies/SeamlessDigitalEngineering#Installation_Report -->

    <owl:Class rdf:about="https://hack.cybersystems.engineer/memex/ontologies/SeamlessDigitalEngineering#Installation_Report">
        <rdfs:subClassOf rdf:resource="https://www.commoncoreontologies.org/ont00000624"/>
    </owl:Class>
    


    <!-- https://hack.cybersystems.engineer/memex/ontologies/SeamlessDigitalEngineering#Integration_Process -->

    <owl:Class rdf:about="https://hack.cybersystems.engineer/memex/ontologies/SeamlessDigitalEngineering#Integration_Process">
        <rdfs:subClassOf rdf:resource="https://hack.cybersystems.engineer/memex/ontologies/SeamlessDigitalEngineering#Technical_Process"/>
        <rdfs:label xml:lang="en">Integration Process</rdfs:label>
        <skos:definition xml:lang="en">The purpose of the integration process is to synthesize a set of system elements into a realised system that satisfies the system requirements.</skos:definition>
        <cco2:ont00001754>ISO/IEC/IEEE 15288:2023</cco2:ont00001754>
    </owl:Class>
    


    <!-- https://hack.cybersystems.engineer/memex/ontologies/SeamlessDigitalEngineering#Integration_and_Test_Report -->

    <owl:Class rdf:about="https://hack.cybersystems.engineer/memex/ontologies/SeamlessDigitalEngineering#Integration_and_Test_Report">
        <rdfs:subClassOf rdf:resource="https://www.commoncoreontologies.org/ont00000624"/>
    </owl:Class>
    


    <!-- https://hack.cybersystems.engineer/memex/ontologies/SeamlessDigitalEngineering#Integrity_Level -->

    <owl:Class rdf:about="https://hack.cybersystems.engineer/memex/ontologies/SeamlessDigitalEngineering#Integrity_Level">
        <owl:equivalentClass>
            <owl:Class>
                <owl:intersectionOf rdf:parseType="Collection">
                    <owl:Restriction>
                        <owl:onProperty rdf:resource="https://www.commoncoreontologies.org/ont00001808"/>
                        <owl:someValuesFrom rdf:resource="https://hack.cybersystems.engineer/memex/ontologies/SeamlessDigitalEngineering#Assurance"/>
                    </owl:Restriction>
                    <owl:Restriction>
                        <owl:onProperty rdf:resource="https://www.commoncoreontologies.org/ont00001811"/>
                        <owl:someValuesFrom rdf:resource="https://hack.cybersystems.engineer/memex/ontologies/SeamlessDigitalEngineering#Product_Integrity"/>
                    </owl:Restriction>
                    <owl:Restriction>
                        <owl:onProperty rdf:resource="https://www.commoncoreontologies.org/ont00001920"/>
                        <owl:someValuesFrom rdf:resource="https://hack.cybersystems.engineer/memex/ontologies/SeamlessDigitalEngineering#Integrity_Level_Claim"/>
                    </owl:Restriction>
                </owl:intersectionOf>
            </owl:Class>
        </owl:equivalentClass>
        <rdfs:subClassOf rdf:resource="https://www.commoncoreontologies.org/ont00001010"/>
        <rdfs:comment xml:lang="en">An Integrity Level is different from the likelihood that the Integrity Level Claim is met but they are closely related.</rdfs:comment>
        <rdfs:comment xml:lang="en">In ISO/IEC/IEEE 15026-1, Integrity Levels are defined in terms of Risk and hence cover safety, security, economic and any other dimension of Risk that is relevant to the System-of-Interest.</rdfs:comment>
        <rdfs:comment xml:lang="en">The word &quot;Confidence&quot; implies that the definition of Integrity Levels can be a subjective concept.</rdfs:comment>
        <rdfs:label xml:lang="en">Integrity Level</rdfs:label>
        <skos:definition xml:lang="en">degree of Confidence that the System-of-Interest meets the associated Integrity Level Claim</skos:definition>
        <cco2:ont00001754 xml:lang="en">ISO/IEC/IEEE 15026-1:2019</cco2:ont00001754>
    </owl:Class>
    


    <!-- https://hack.cybersystems.engineer/memex/ontologies/SeamlessDigitalEngineering#Integrity_Level_Claim -->

    <owl:Class rdf:about="https://hack.cybersystems.engineer/memex/ontologies/SeamlessDigitalEngineering#Integrity_Level_Claim">
        <owl:equivalentClass>
            <owl:Class>
                <owl:intersectionOf rdf:parseType="Collection">
                    <rdf:Description rdf:about="https://hack.cybersystems.engineer/memex/ontologies/SeamlessDigitalEngineering#Quality_Claim"/>
                    <owl:Restriction>
                        <owl:onProperty rdf:resource="https://www.commoncoreontologies.org/ont00001942"/>
                        <owl:someValuesFrom rdf:resource="https://hack.cybersystems.engineer/memex/ontologies/SeamlessDigitalEngineering#Integrity_Level"/>
                    </owl:Restriction>
                </owl:intersectionOf>
            </owl:Class>
        </owl:equivalentClass>
        <rdfs:subClassOf rdf:resource="https://hack.cybersystems.engineer/memex/ontologies/SeamlessDigitalEngineering#Quality_Claim"/>
        <rdfs:label xml:lang="en">Integrity Level Claim</rdfs:label>
        <skos:definition xml:lang="en">proposition representing a Requirement on a Risk Reduction Measure identified in the Risk Treatment process of the System-of-Interest</skos:definition>
        <skos:editorialNote>FIXME</skos:editorialNote>
        <cco2:ont00001754 xml:lang="en">ISO/IEC/IEEE 15026-1:2019</cco2:ont00001754>
    </owl:Class>
    


    <!-- https://hack.cybersystems.engineer/memex/ontologies/SeamlessDigitalEngineering#Integrity_Level_Requirements -->

    <owl:Class rdf:about="https://hack.cybersystems.engineer/memex/ontologies/SeamlessDigitalEngineering#Integrity_Level_Requirements">
        <rdfs:subClassOf rdf:resource="https://hack.cybersystems.engineer/memex/ontologies/SeamlessDigitalEngineering#Requirement_Set"/>
        <rdfs:label xml:lang="en">Integrity Level Requirements</rdfs:label>
        <skos:definition xml:lang="en">Requirement Set that, when met, will provide a level of Confidence in the associated Integrity Level Claim commensurate with the associated Integrity Level</skos:definition>
        <cco2:ont00001754 xml:lang="en">ISO/IEC/IEEE 15026-1:2019</cco2:ont00001754>
    </owl:Class>
    


    <!-- https://hack.cybersystems.engineer/memex/ontologies/SeamlessDigitalEngineering#Interface -->

    <owl:Class rdf:about="https://hack.cybersystems.engineer/memex/ontologies/SeamlessDigitalEngineering#Interface">
        <owl:equivalentClass>
            <owl:Class>
                <owl:intersectionOf rdf:parseType="Collection">
                    <owl:Restriction>
                        <owl:onProperty rdf:resource="http://purl.obolibrary.org/obo/BFO_0000176"/>
                        <owl:someValuesFrom rdf:resource="https://hack.cybersystems.engineer/memex/ontologies/SeamlessDigitalEngineering#System"/>
                    </owl:Restriction>
                    <owl:Restriction>
                        <owl:onProperty rdf:resource="http://purl.obolibrary.org/obo/BFO_0000183"/>
                        <owl:someValuesFrom rdf:resource="https://www.commoncoreontologies.org/ont00000402"/>
                    </owl:Restriction>
                    <owl:Restriction>
                        <owl:onProperty rdf:resource="http://purl.obolibrary.org/obo/BFO_0000178"/>
                        <owl:minQualifiedCardinality rdf:datatype="http://www.w3.org/2001/XMLSchema#nonNegativeInteger">2</owl:minQualifiedCardinality>
                        <owl:onClass rdf:resource="https://hack.cybersystems.engineer/memex/ontologies/SeamlessDigitalEngineering#System_Element"/>
                    </owl:Restriction>
                </owl:intersectionOf>
            </owl:Class>
        </owl:equivalentClass>
        <rdfs:subClassOf rdf:resource="https://www.commoncoreontologies.org/ont00000798"/>
        <rdfs:label xml:lang="en">Interface</rdfs:label>
        <skos:definition xml:lang="en">point at which two or more logical, physical, or both, System Elements or Software System Elements meet and act on or communicate with each other</skos:definition>
        <cco2:ont00001754 xml:lang="en">ISO/IEC/IEEE 24748-6:2023 — Systems and software engineering — Life cycle management — Part 6: System and software integration</cco2:ont00001754>
    </owl:Class>
    


    <!-- https://hack.cybersystems.engineer/memex/ontologies/SeamlessDigitalEngineering#Key_Quality_Attribute -->

    <owl:Class rdf:about="https://hack.cybersystems.engineer/memex/ontologies/SeamlessDigitalEngineering#Key_Quality_Attribute">
        <owl:equivalentClass>
            <owl:Class>
                <owl:intersectionOf rdf:parseType="Collection">
                    <rdf:Description rdf:about="https://hack.cybersystems.engineer/memex/ontologies/SeamlessDigitalEngineering#Quality_Property"/>
                    <owl:Restriction>
                        <owl:onProperty rdf:resource="http://purl.obolibrary.org/obo/BFO_0000195"/>
                        <owl:someValuesFrom rdf:resource="https://hack.cybersystems.engineer/memex/ontologies/SeamlessDigitalEngineering#Concern_Disposition"/>
                    </owl:Restriction>
                </owl:intersectionOf>
            </owl:Class>
        </owl:equivalentClass>
        <rdfs:subClassOf rdf:resource="https://hack.cybersystems.engineer/memex/ontologies/SeamlessDigitalEngineering#Quality_Property"/>
        <rdfs:label xml:lang="en">Key Quality Attribute</rdfs:label>
        <skos:definition xml:lang="en">a Quality Attribute that is consider of prime importance by Stakeholders</skos:definition>
        <cco2:ont00001753 xml:lang="en">KQA</cco2:ont00001753>
    </owl:Class>
    


    <!-- https://hack.cybersystems.engineer/memex/ontologies/SeamlessDigitalEngineering#Knowledge -->

    <owl:Class rdf:about="https://hack.cybersystems.engineer/memex/ontologies/SeamlessDigitalEngineering#Knowledge">
        <owl:equivalentClass>
            <owl:Class>
                <owl:intersectionOf rdf:parseType="Collection">
                    <rdf:Description rdf:about="https://www.commoncoreontologies.org/ont00000958"/>
                    <owl:Restriction>
                        <owl:onProperty rdf:resource="https://www.commoncoreontologies.org/ont00001816"/>
                        <owl:someValuesFrom rdf:resource="https://www.commoncoreontologies.org/ont00000366"/>
                    </owl:Restriction>
                </owl:intersectionOf>
            </owl:Class>
        </owl:equivalentClass>
        <rdfs:subClassOf rdf:resource="https://www.commoncoreontologies.org/ont00000958"/>
        <rdfs:label xml:lang="en">Knowledge</rdfs:label>
        <skos:definition xml:lang="en">maintained, processed, and interpreted Information</skos:definition>
        <cco2:ont00001754 xml:lang="en">ISO 5127:2017 — Information and documentation — Foundation and vocabulary</cco2:ont00001754>
        <cco2:ont00001760 rdf:datatype="http://www.w3.org/2001/XMLSchema#anyURI">https://semantic.incose.org/DEIX_Ontology</cco2:ont00001760>
    </owl:Class>
    


    <!-- https://hack.cybersystems.engineer/memex/ontologies/SeamlessDigitalEngineering#Knowledge_Goal -->

    <owl:Class rdf:about="https://hack.cybersystems.engineer/memex/ontologies/SeamlessDigitalEngineering#Knowledge_Goal">
        <rdfs:subClassOf rdf:resource="https://hack.cybersystems.engineer/memex/ontologies/SeamlessDigitalEngineering#Goal"/>
        <rdfs:label xml:lang="en">Knowledge Goal</rdfs:label>
    </owl:Class>
    


    <!-- https://hack.cybersystems.engineer/memex/ontologies/SeamlessDigitalEngineering#Knowledge_Management_Process -->

    <owl:Class rdf:about="https://hack.cybersystems.engineer/memex/ontologies/SeamlessDigitalEngineering#Knowledge_Management_Process">
        <rdfs:subClassOf rdf:resource="https://hack.cybersystems.engineer/memex/ontologies/SeamlessDigitalEngineering#Organizational_Project-enabling_Process"/>
        <rdfs:label xml:lang="en">Knowledge Management Process</rdfs:label>
        <skos:definition xml:lang="en">The purpose of the knowledge management process is to create the capability and assets that enable the organization to exploit opportunities to re-apply existing knowledge.

This encompasses knowledge, skills, and knowledge assets, including system elements.</skos:definition>
        <cco2:ont00001754>ISO/IEC/IEEE 15288:2023</cco2:ont00001754>
    </owl:Class>
    


    <!-- https://hack.cybersystems.engineer/memex/ontologies/SeamlessDigitalEngineering#Lack -->

    <owl:Class rdf:about="https://hack.cybersystems.engineer/memex/ontologies/SeamlessDigitalEngineering#Lack">
        <rdfs:subClassOf rdf:resource="https://www.commoncoreontologies.org/ont00000768"/>
        <rdfs:label xml:lang="en">Lack</rdfs:label>
        <skos:definition xml:lang="en">A particular deficiency or absence.</skos:definition>
        <cco2:ont00001754 xml:lang="en">The American Heritage® Dictionary of the English Language, 5th Edition</cco2:ont00001754>
    </owl:Class>
    


    <!-- https://hack.cybersystems.engineer/memex/ontologies/SeamlessDigitalEngineering#Lifecycle -->

    <owl:Class rdf:about="https://hack.cybersystems.engineer/memex/ontologies/SeamlessDigitalEngineering#Lifecycle">
        <owl:equivalentClass>
            <owl:Restriction>
                <owl:onProperty rdf:resource="http://purl.obolibrary.org/obo/BFO_0000184"/>
                <owl:someValuesFrom rdf:resource="https://hack.cybersystems.engineer/memex/ontologies/SeamlessDigitalEngineering#System"/>
            </owl:Restriction>
        </owl:equivalentClass>
        <rdfs:subClassOf rdf:resource="https://www.commoncoreontologies.org/ont00000856"/>
        <rdfs:label xml:lang="en">Lifecycle</rdfs:label>
        <skos:altLabel xml:lang="en">Life cycle</skos:altLabel>
        <skos:definition xml:lang="en">An Artifact History of a System, Product, Service, Project or other human-made entity from conception through Retirement</skos:definition>
        <cco2:ont00001754>ISO/IEC/IEEE 15288:2023</cco2:ont00001754>
        <cco2:ont00001760 rdf:datatype="http://www.w3.org/2001/XMLSchema#anyURI">https://semantic.incose.org/DEIX_Ontology</cco2:ont00001760>
    </owl:Class>
    


    <!-- https://hack.cybersystems.engineer/memex/ontologies/SeamlessDigitalEngineering#Lifecycle_Concept -->

    <owl:Class rdf:about="https://hack.cybersystems.engineer/memex/ontologies/SeamlessDigitalEngineering#Lifecycle_Concept">
        <owl:equivalentClass>
            <owl:Class>
                <owl:intersectionOf rdf:parseType="Collection">
                    <owl:Restriction>
                        <owl:onProperty rdf:resource="http://purl.obolibrary.org/obo/BFO_0000084"/>
                        <owl:someValuesFrom rdf:resource="https://hack.cybersystems.engineer/memex/ontologies/SeamlessDigitalEngineering#Stakeholder"/>
                    </owl:Restriction>
                    <owl:Restriction>
                        <owl:onProperty rdf:resource="https://www.commoncoreontologies.org/ont00001942"/>
                        <owl:someValuesFrom rdf:resource="https://hack.cybersystems.engineer/memex/ontologies/SeamlessDigitalEngineering#Lifecycle"/>
                    </owl:Restriction>
                </owl:intersectionOf>
            </owl:Class>
        </owl:equivalentClass>
        <rdfs:subClassOf rdf:resource="https://www.commoncoreontologies.org/ont00001045"/>
        <rdfs:comment xml:lang="en">Although the provided definition uses the term &quot;representation&quot;, indicating it could be a Representational ICE, it states that it &quot;expresses how an entity can satisfy the Problem ...&quot; making it a kind of Prescriptive ICE or Artifact Model.</rdfs:comment>
        <rdfs:comment xml:lang="en">This definition, although nonstandard, was considered ontologically useful in the absence of an authoritative definition.

The ISO/IEC/IEEE 24765:2017 provides a domain-specific definition: &quot;model of the concepts relevant to some endeavor&quot;, sourced from the IEEE 1320.2-1998 (R2004) IEEE Standard for Conceptual Modeling Language Syntax and Semantics for IDEF1X97.</rdfs:comment>
        <rdfs:label xml:lang="en">Lifecycle Concept</rdfs:label>
        <skos:definition xml:lang="en">A written or graphic representation that concisely expresses how an entity can satisfy the Problem, Threat or Opportunity, Mission, Goals, Objectives, and Measures it was defined to address within specified Constraints with acceptable Risk.</skos:definition>
        <cco2:ont00001754>INCOSE Needs and Requirements Manual R1.1 (2022)</cco2:ont00001754>
    </owl:Class>
    


    <!-- https://hack.cybersystems.engineer/memex/ontologies/SeamlessDigitalEngineering#Lifecycle_Model -->

    <owl:Class rdf:about="https://hack.cybersystems.engineer/memex/ontologies/SeamlessDigitalEngineering#Lifecycle_Model">
        <owl:equivalentClass>
            <owl:Class>
                <owl:intersectionOf rdf:parseType="Collection">
                    <owl:Restriction>
                        <owl:onProperty rdf:resource="https://www.commoncoreontologies.org/ont00001942"/>
                        <owl:someValuesFrom rdf:resource="https://hack.cybersystems.engineer/memex/ontologies/SeamlessDigitalEngineering#Act_of_Engineering"/>
                    </owl:Restriction>
                    <owl:Restriction>
                        <owl:onProperty rdf:resource="https://www.commoncoreontologies.org/ont00001942"/>
                        <owl:someValuesFrom rdf:resource="https://hack.cybersystems.engineer/memex/ontologies/SeamlessDigitalEngineering#Lifecycle"/>
                    </owl:Restriction>
                </owl:intersectionOf>
            </owl:Class>
        </owl:equivalentClass>
        <rdfs:subClassOf rdf:resource="https://www.commoncoreontologies.org/ont00001324"/>
        <rdfs:label xml:lang="en">Lifecycle Model</rdfs:label>
        <skos:definition xml:lang="en">framework of processes and Activities concerned with the Lifecycle which can be organized into Stages, acting as a common reference for communication and understanding</skos:definition>
        <cco2:ont00001754>ISO/IEC/IEEE 15288:2023</cco2:ont00001754>
    </owl:Class>
    


    <!-- https://hack.cybersystems.engineer/memex/ontologies/SeamlessDigitalEngineering#Lifecycle_Model_Management_Process -->

    <owl:Class rdf:about="https://hack.cybersystems.engineer/memex/ontologies/SeamlessDigitalEngineering#Lifecycle_Model_Management_Process">
        <rdfs:subClassOf rdf:resource="https://hack.cybersystems.engineer/memex/ontologies/SeamlessDigitalEngineering#Organizational_Project-enabling_Process"/>
        <rdfs:label xml:lang="en">Lifecycle Model Management Process</rdfs:label>
        <skos:definition xml:lang="en">The purpose of the life cycle model management process is to define, maintain, and help ensure availability of policies, life cycle processes, life cycle models, and procedures for use by the organization with respect to the scope of this document.</skos:definition>
        <cco2:ont00001754>ISO/IEC/IEEE 15288:2023</cco2:ont00001754>
    </owl:Class>
    


    <!-- https://hack.cybersystems.engineer/memex/ontologies/SeamlessDigitalEngineering#Lifecycle_Stage -->

    <owl:Class rdf:about="https://hack.cybersystems.engineer/memex/ontologies/SeamlessDigitalEngineering#Lifecycle_Stage">
        <owl:equivalentClass>
            <owl:Class>
                <owl:intersectionOf rdf:parseType="Collection">
                    <owl:Restriction>
                        <owl:onProperty rdf:resource="https://www.commoncoreontologies.org/ont00001833"/>
                        <owl:someValuesFrom rdf:resource="https://hack.cybersystems.engineer/memex/ontologies/SeamlessDigitalEngineering#Stakeholder"/>
                    </owl:Restriction>
                    <owl:Restriction>
                        <owl:onProperty rdf:resource="https://www.commoncoreontologies.org/ont00001857"/>
                        <owl:someValuesFrom rdf:resource="https://hack.cybersystems.engineer/memex/ontologies/SeamlessDigitalEngineering#Lifecycle"/>
                    </owl:Restriction>
                </owl:intersectionOf>
            </owl:Class>
        </owl:equivalentClass>
        <rdfs:subClassOf rdf:resource="https://hack.cybersystems.engineer/memex/ontologies/SeamlessDigitalEngineering#Lifecycle"/>
        <rdfs:comment xml:lang="en">As used in [ISO/IEC/IEEE 15288], stages relate to major progress and achievement milestones of the entity through its life cycle.</rdfs:comment>
        <rdfs:comment xml:lang="en">Stages often overlap.</rdfs:comment>
        <rdfs:label xml:lang="en">Lifecycle Stage</rdfs:label>
        <skos:altLabel xml:lang="en">Stage</skos:altLabel>
        <skos:definition xml:lang="en">period within the Lifecycle of an entity that relates to the state of its description or realization</skos:definition>
    </owl:Class>
    


    <!-- https://hack.cybersystems.engineer/memex/ontologies/SeamlessDigitalEngineering#Lifecycle_View -->

    <owl:Class rdf:about="https://hack.cybersystems.engineer/memex/ontologies/SeamlessDigitalEngineering#Lifecycle_View">
        <owl:equivalentClass>
            <owl:Class>
                <owl:intersectionOf rdf:parseType="Collection">
                    <rdf:Description rdf:about="https://hack.cybersystems.engineer/memex/ontologies/SeamlessDigitalEngineering#View"/>
                    <owl:Restriction>
                        <owl:onProperty rdf:resource="https://www.commoncoreontologies.org/ont00001938"/>
                        <owl:someValuesFrom rdf:resource="https://hack.cybersystems.engineer/memex/ontologies/SeamlessDigitalEngineering#Lifecycle"/>
                    </owl:Restriction>
                </owl:intersectionOf>
            </owl:Class>
        </owl:equivalentClass>
        <rdfs:subClassOf rdf:resource="https://hack.cybersystems.engineer/memex/ontologies/SeamlessDigitalEngineering#View"/>
        <rdfs:label xml:lang="en">Lifecycle View</rdfs:label>
        <skos:definition xml:lang="en">A View that represents some Lifecycle</skos:definition>
        <cco2:ont00001760 rdf:datatype="http://www.w3.org/2001/XMLSchema#anyURI">https://semantic.incose.org/DEIX_Ontology</cco2:ont00001760>
    </owl:Class>
    


    <!-- https://hack.cybersystems.engineer/memex/ontologies/SeamlessDigitalEngineering#Likelihood -->

    <owl:Class rdf:about="https://hack.cybersystems.engineer/memex/ontologies/SeamlessDigitalEngineering#Likelihood">
        <owl:equivalentClass>
            <owl:Class>
                <owl:intersectionOf rdf:parseType="Collection">
                    <rdf:Description rdf:about="https://www.commoncoreontologies.org/ont00000692"/>
                    <owl:Restriction>
                        <owl:onProperty rdf:resource="https://www.commoncoreontologies.org/ont00001966"/>
                        <owl:someValuesFrom rdf:resource="http://purl.obolibrary.org/obo/BFO_0000015"/>
                    </owl:Restriction>
                </owl:intersectionOf>
            </owl:Class>
        </owl:equivalentClass>
        <rdfs:subClassOf rdf:resource="https://www.commoncoreontologies.org/ont00000692"/>
        <rdfs:label xml:lang="en">Likelihood</rdfs:label>
        <skos:definition xml:lang="en">Probability of something happening</skos:definition>
        <cco2:ont00001754 xml:lang="en">ISO/IEC/IEEE 15026-1:2019</cco2:ont00001754>
    </owl:Class>
    


    <!-- https://hack.cybersystems.engineer/memex/ontologies/SeamlessDigitalEngineering#Logic_Programming_Language -->

    <owl:Class rdf:about="https://hack.cybersystems.engineer/memex/ontologies/SeamlessDigitalEngineering#Logic_Programming_Language">
        <rdfs:subClassOf rdf:resource="http://www.ontologyrepository.com/CommonCoreOntologies/HighLevelProgrammingLanguage"/>
        <rdfs:label xml:lang="en">Logic Programming Language</rdfs:label>
    </owl:Class>
    


    <!-- https://hack.cybersystems.engineer/memex/ontologies/SeamlessDigitalEngineering#Logical_Architecture -->

    <owl:Class rdf:about="https://hack.cybersystems.engineer/memex/ontologies/SeamlessDigitalEngineering#Logical_Architecture">
        <rdfs:subClassOf rdf:resource="https://hack.cybersystems.engineer/memex/ontologies/SeamlessDigitalEngineering#Architecture_View"/>
        <rdfs:label xml:lang="en">Logical Architecture</rdfs:label>
        <skos:altLabel xml:lang="en">Logical (View of) Architecture</skos:altLabel>
        <skos:definition xml:lang="en">The logical view of an architecture in an architecture description is typically an integrated model of both the system’s functions and retained data, where the abstraction level is chosen to be directly relevant to users rather than implementation. The logical view of the architecture defines data as it makes sense in the problem domain, and defers definition of how it can be represented to other views. So, for example, the logical view would define data and functional transformations in terms of positions, currency amounts, or objects of user interest and not in terms of XML records or database fields.</skos:definition>
        <cco2:ont00001754 xml:lang="en">ISO/IEC/IEEE 42020:2019, Annex E.4.2</cco2:ont00001754>
    </owl:Class>
    


    <!-- https://hack.cybersystems.engineer/memex/ontologies/SeamlessDigitalEngineering#Logical_Viewpoint -->

    <owl:Class rdf:about="https://hack.cybersystems.engineer/memex/ontologies/SeamlessDigitalEngineering#Logical_Viewpoint">
        <owl:equivalentClass>
            <owl:Class>
                <owl:intersectionOf rdf:parseType="Collection">
                    <rdf:Description rdf:about="https://hack.cybersystems.engineer/memex/ontologies/SeamlessDigitalEngineering#Architecture_Viewpoint"/>
                    <owl:Restriction>
                        <owl:onProperty rdf:resource="https://www.commoncoreontologies.org/ont00001942"/>
                        <owl:someValuesFrom rdf:resource="https://hack.cybersystems.engineer/memex/ontologies/SeamlessDigitalEngineering#Logical_Architecture"/>
                    </owl:Restriction>
                </owl:intersectionOf>
            </owl:Class>
        </owl:equivalentClass>
        <rdfs:subClassOf rdf:resource="https://hack.cybersystems.engineer/memex/ontologies/SeamlessDigitalEngineering#Architecture_Viewpoint"/>
        <rdfs:label xml:lang="en">Logical Viewpoint</rdfs:label>
    </owl:Class>
    


    <!-- https://hack.cybersystems.engineer/memex/ontologies/SeamlessDigitalEngineering#Loss_of_Error -->

    <owl:Class rdf:about="https://hack.cybersystems.engineer/memex/ontologies/SeamlessDigitalEngineering#Loss_of_Error">
        <rdfs:subClassOf rdf:resource="https://www.commoncoreontologies.org/ont00001066"/>
        <rdfs:label xml:lang="en">Loss of Error</rdfs:label>
    </owl:Class>
    


    <!-- https://hack.cybersystems.engineer/memex/ontologies/SeamlessDigitalEngineering#Maintainer -->

    <owl:Class rdf:about="https://hack.cybersystems.engineer/memex/ontologies/SeamlessDigitalEngineering#Maintainer">
        <rdfs:subClassOf rdf:resource="https://hack.cybersystems.engineer/memex/ontologies/SeamlessDigitalEngineering#Stakeholder"/>
        <skos:definition xml:lang="en">Agent (individual) or Organization that performs maintenance activities</skos:definition>
        <cco2:ont00001754 xml:lang="en">ISO/IEC 25002:2024 Systems and software engineering - Systems and software Quality Requirements and Evaluation (SQuaRE) - Quality model overview and usage</cco2:ont00001754>
    </owl:Class>
    


    <!-- https://hack.cybersystems.engineer/memex/ontologies/SeamlessDigitalEngineering#Maintenance_Process -->

    <owl:Class rdf:about="https://hack.cybersystems.engineer/memex/ontologies/SeamlessDigitalEngineering#Maintenance_Process">
        <rdfs:subClassOf rdf:resource="https://hack.cybersystems.engineer/memex/ontologies/SeamlessDigitalEngineering#Technical_Process"/>
        <rdfs:label xml:lang="en">Maintenance Process</rdfs:label>
        <skos:definition xml:lang="en">The purpose of the maintenance process is to sustain the capability of the system to provide a product or service.</skos:definition>
        <cco2:ont00001754>ISO/IEC/IEEE 15288:2023</cco2:ont00001754>
    </owl:Class>
    


    <!-- https://hack.cybersystems.engineer/memex/ontologies/SeamlessDigitalEngineering#Mathematical_Logic_Discipline -->

    <owl:Class rdf:about="https://hack.cybersystems.engineer/memex/ontologies/SeamlessDigitalEngineering#Mathematical_Logic_Discipline">
        <rdfs:subClassOf rdf:resource="https://hack.cybersystems.engineer/memex/ontologies/SeamlessDigitalEngineering#Mathematics_Discipline"/>
        <rdfs:label xml:lang="en">Mathematical Logic Discipline</rdfs:label>
    </owl:Class>
    


    <!-- https://hack.cybersystems.engineer/memex/ontologies/SeamlessDigitalEngineering#Mathematics_Discipline -->

    <owl:Class rdf:about="https://hack.cybersystems.engineer/memex/ontologies/SeamlessDigitalEngineering#Mathematics_Discipline">
        <owl:equivalentClass>
            <owl:Class>
                <owl:intersectionOf rdf:parseType="Collection">
                    <rdf:Description rdf:about="https://hack.cybersystems.engineer/memex/ontologies/SeamlessDigitalEngineering#Discipline"/>
                    <owl:Restriction>
                        <owl:onProperty rdf:resource="https://www.commoncoreontologies.org/ont00001808"/>
                        <owl:someValuesFrom rdf:resource="https://hack.cybersystems.engineer/memex/ontologies/SeamlessDigitalEngineering#Act_of_Mathematics"/>
                    </owl:Restriction>
                </owl:intersectionOf>
            </owl:Class>
        </owl:equivalentClass>
        <rdfs:subClassOf rdf:resource="https://hack.cybersystems.engineer/memex/ontologies/SeamlessDigitalEngineering#Discipline"/>
        <rdfs:label xml:lang="en">Mathematics Discipline</rdfs:label>
    </owl:Class>
    


    <!-- https://hack.cybersystems.engineer/memex/ontologies/SeamlessDigitalEngineering#Measure -->

    <owl:Class rdf:about="https://hack.cybersystems.engineer/memex/ontologies/SeamlessDigitalEngineering#Measure">
        <owl:equivalentClass>
            <owl:Class>
                <owl:intersectionOf rdf:parseType="Collection">
                    <rdf:Description rdf:about="https://www.commoncoreontologies.org/ont00001163"/>
                    <owl:Restriction>
                        <owl:onProperty rdf:resource="http://purl.obolibrary.org/obo/BFO_0000058"/>
                        <owl:someValuesFrom rdf:resource="https://www.commoncoreontologies.org/ont00000345"/>
                    </owl:Restriction>
                </owl:intersectionOf>
            </owl:Class>
        </owl:equivalentClass>
        <rdfs:subClassOf rdf:resource="https://www.commoncoreontologies.org/ont00001163"/>
        <rdfs:label xml:lang="en">Measure</rdfs:label>
        <skos:definition xml:lang="en">variable to which a value is assigned as the result of measurement</skos:definition>
        <cco2:ont00001754 xml:lang="en">ISO/IEC 25000:2014 Systems and software Engineering — Systems and software product Quality Requirements and Evaluation (SQuaRE) — Guide to SQuaRE</cco2:ont00001754>
    </owl:Class>
    


    <!-- https://hack.cybersystems.engineer/memex/ontologies/SeamlessDigitalEngineering#Measurement_Process -->

    <owl:Class rdf:about="https://hack.cybersystems.engineer/memex/ontologies/SeamlessDigitalEngineering#Measurement_Process">
        <rdfs:subClassOf rdf:resource="https://hack.cybersystems.engineer/memex/ontologies/SeamlessDigitalEngineering#Technical_Management_Process"/>
        <rdfs:label xml:lang="en">Measurement Process</rdfs:label>
        <skos:definition xml:lang="en">The purpose of the measurement process is to collect, analyse, and report objective data and information to support effective management and address information needs about the products, services, and processes.</skos:definition>
        <cco2:ont00001754>ISO/IEC/IEEE 15288:2023</cco2:ont00001754>
    </owl:Class>
    


    <!-- https://hack.cybersystems.engineer/memex/ontologies/SeamlessDigitalEngineering#Message_Permission -->

    <owl:Class rdf:about="https://hack.cybersystems.engineer/memex/ontologies/SeamlessDigitalEngineering#Message_Permission">
        <owl:equivalentClass>
            <owl:Class>
                <owl:intersectionOf rdf:parseType="Collection">
                    <rdf:Description rdf:about="https://www.commoncoreontologies.org/ont00000751"/>
                    <owl:Restriction>
                        <owl:onProperty rdf:resource="https://www.commoncoreontologies.org/ont00001910"/>
                        <owl:someValuesFrom rdf:resource="https://www.commoncoreontologies.org/ont00000517"/>
                    </owl:Restriction>
                </owl:intersectionOf>
            </owl:Class>
        </owl:equivalentClass>
        <rdfs:subClassOf rdf:resource="https://www.commoncoreontologies.org/ont00000751"/>
        <rdfs:label xml:lang="en">Message Permission</rdfs:label>
        <skos:definition xml:lang="en">An Action Permission that prescribes the Act of Communication by Media</skos:definition>
    </owl:Class>
    


    <!-- https://hack.cybersystems.engineer/memex/ontologies/SeamlessDigitalEngineering#Method -->

    <owl:Class rdf:about="https://hack.cybersystems.engineer/memex/ontologies/SeamlessDigitalEngineering#Method">
        <owl:equivalentClass>
            <owl:Class>
                <owl:intersectionOf rdf:parseType="Collection">
                    <rdf:Description rdf:about="https://www.commoncoreontologies.org/ont00000974"/>
                    <owl:Restriction>
                        <owl:onProperty rdf:resource="https://www.commoncoreontologies.org/ont00001942"/>
                        <owl:someValuesFrom rdf:resource="https://www.commoncoreontologies.org/ont00000228"/>
                    </owl:Restriction>
                </owl:intersectionOf>
            </owl:Class>
        </owl:equivalentClass>
        <rdfs:subClassOf rdf:resource="https://www.commoncoreontologies.org/ont00000974"/>
        <rdfs:label xml:lang="en">Method</rdfs:label>
        <skos:definition xml:lang="en">prescription of an Planned Act which can be used to produce Data or derive Information as an output from specified inputs</skos:definition>
        <cco2:ont00001754 xml:lang="en">derived from ISO/IEC 27041:2015
Information technology - Security techniques - Guidance on assuring suitability and adequacy of incident investigative method</cco2:ont00001754>
    </owl:Class>
    


    <!-- https://hack.cybersystems.engineer/memex/ontologies/SeamlessDigitalEngineering#Methodology -->

    <owl:Class rdf:about="https://hack.cybersystems.engineer/memex/ontologies/SeamlessDigitalEngineering#Methodology">
        <owl:equivalentClass>
            <owl:Class>
                <owl:intersectionOf rdf:parseType="Collection">
                    <owl:Restriction>
                        <owl:onProperty rdf:resource="http://purl.obolibrary.org/obo/BFO_0000178"/>
                        <owl:someValuesFrom rdf:resource="https://hack.cybersystems.engineer/memex/ontologies/SeamlessDigitalEngineering#Method"/>
                    </owl:Restriction>
                    <owl:Restriction>
                        <owl:onProperty rdf:resource="https://www.commoncoreontologies.org/ont00001942"/>
                        <owl:someValuesFrom rdf:resource="https://www.commoncoreontologies.org/ont00000513"/>
                    </owl:Restriction>
                </owl:intersectionOf>
            </owl:Class>
        </owl:equivalentClass>
        <rdfs:subClassOf rdf:resource="https://www.commoncoreontologies.org/ont00000974"/>
        <rdfs:label xml:lang="en">Methodology</rdfs:label>
    </owl:Class>
    


    <!-- https://hack.cybersystems.engineer/memex/ontologies/SeamlessDigitalEngineering#Milestone -->

    <owl:Class rdf:about="https://hack.cybersystems.engineer/memex/ontologies/SeamlessDigitalEngineering#Milestone">
        <owl:equivalentClass>
            <owl:Class>
                <owl:intersectionOf rdf:parseType="Collection">
                    <owl:Restriction>
                        <owl:onProperty rdf:resource="https://www.commoncoreontologies.org/ont00001857"/>
                        <owl:someValuesFrom rdf:resource="https://hack.cybersystems.engineer/memex/ontologies/SeamlessDigitalEngineering#Lifecycle"/>
                    </owl:Restriction>
                    <owl:Restriction>
                        <owl:onProperty rdf:resource="https://www.commoncoreontologies.org/ont00001904"/>
                        <owl:someValuesFrom rdf:resource="https://www.commoncoreontologies.org/ont00000203"/>
                    </owl:Restriction>
                </owl:intersectionOf>
            </owl:Class>
        </owl:equivalentClass>
        <rdfs:subClassOf rdf:resource="https://www.commoncoreontologies.org/ont00000004"/>
        <rdfs:label xml:lang="en">Milestone</rdfs:label>
        <skos:definition xml:lang="en">a significant point or event in a Project</skos:definition>
        <skos:definition xml:lang="en">scheduled event used to measure progress</skos:definition>
        <skos:example xml:lang="en">Major milestones for software projects can include an acquirer or managerial sign-off, baselining of a specification, completion of system integration, and product delivery. Minor milestones can include baselining of a software module or completion of a chapter of the user manual.</skos:example>
        <cco2:ont00001754 xml:lang="en">A Guide to the Project Management Body of Knowledge (PMBOK® Guide) — Fifth Edition</cco2:ont00001754>
        <cco2:ont00001754 xml:lang="en">ISO/IEC/IEEE 24765:2017</cco2:ont00001754>
    </owl:Class>
    


    <!-- https://hack.cybersystems.engineer/memex/ontologies/SeamlessDigitalEngineering#Mission -->

    <owl:Class rdf:about="https://hack.cybersystems.engineer/memex/ontologies/SeamlessDigitalEngineering#Mission">
        <owl:equivalentClass rdf:resource="https://hack.cybersystems.engineer/memex/ontologies/SeamlessDigitalEngineering#Purpose"/>
        <owl:equivalentClass>
            <owl:Class>
                <owl:intersectionOf rdf:parseType="Collection">
                    <rdf:Description rdf:about="https://hack.cybersystems.engineer/memex/ontologies/SeamlessDigitalEngineering#Need"/>
                    <owl:Restriction>
                        <owl:onProperty rdf:resource="http://purl.obolibrary.org/obo/BFO_0000178"/>
                        <owl:someValuesFrom rdf:resource="https://hack.cybersystems.engineer/memex/ontologies/SeamlessDigitalEngineering#Goal"/>
                    </owl:Restriction>
                </owl:intersectionOf>
            </owl:Class>
        </owl:equivalentClass>
        <rdfs:subClassOf rdf:resource="https://hack.cybersystems.engineer/memex/ontologies/SeamlessDigitalEngineering#Need"/>
        <skos:definition xml:lang="en">The mission of a system is the top-level function of the system; the one that synthesizes all transformation of all inputs and solicitations into outputs and reactions.</skos:definition>
        <skos:definition xml:lang="en">The mission statement is the top tier of the needs hierarchy based on the above analysis of a problem, threat, or opportunity that the project was formed to address.</skos:definition>
        <cco2:ont00001754>INCOSE Needs and Requirements Manual R1.1 (2022)</cco2:ont00001754>
        <cco2:ont00001754 rdf:datatype="http://www.w3.org/2001/XMLSchema#anyURI">https://sebokwiki.org/wiki/Mission_(glossary)</cco2:ont00001754>
    </owl:Class>
    


    <!-- https://hack.cybersystems.engineer/memex/ontologies/SeamlessDigitalEngineering#Model-Based_Engineering_Approach -->

    <owl:Class rdf:about="https://hack.cybersystems.engineer/memex/ontologies/SeamlessDigitalEngineering#Model-Based_Engineering_Approach">
        <owl:equivalentClass>
            <owl:Class>
                <owl:intersectionOf rdf:parseType="Collection">
                    <rdf:Description rdf:about="https://hack.cybersystems.engineer/memex/ontologies/SeamlessDigitalEngineering#Engineering_Approach"/>
                    <owl:Restriction>
                        <owl:onProperty rdf:resource="https://www.commoncoreontologies.org/ont00001808"/>
                        <owl:someValuesFrom rdf:resource="https://hack.cybersystems.engineer/memex/ontologies/SeamlessDigitalEngineering#System_Model"/>
                    </owl:Restriction>
                </owl:intersectionOf>
            </owl:Class>
        </owl:equivalentClass>
        <rdfs:subClassOf rdf:resource="https://hack.cybersystems.engineer/memex/ontologies/SeamlessDigitalEngineering#Engineering_Approach"/>
        <rdfs:label xml:lang="en">Model-Based Engineering Approach</rdfs:label>
        <skos:definition xml:lang="en">An Engineering Approach that is focused on the use of System Model(s)</skos:definition>
        <cco2:ont00001760 rdf:datatype="http://www.w3.org/2001/XMLSchema#anyURI">https://semantic.incose.org/DEIX_Ontology</cco2:ont00001760>
    </owl:Class>
    


    <!-- https://hack.cybersystems.engineer/memex/ontologies/SeamlessDigitalEngineering#Model-Based_Systems_Engineering_Approach -->

    <owl:Class rdf:about="https://hack.cybersystems.engineer/memex/ontologies/SeamlessDigitalEngineering#Model-Based_Systems_Engineering_Approach">
        <owl:equivalentClass>
            <owl:Class>
                <owl:intersectionOf rdf:parseType="Collection">
                    <rdf:Description rdf:about="https://hack.cybersystems.engineer/memex/ontologies/SeamlessDigitalEngineering#Model-Based_Engineering_Approach"/>
                    <owl:Restriction>
                        <owl:onProperty rdf:resource="https://www.commoncoreontologies.org/ont00001942"/>
                        <owl:someValuesFrom rdf:resource="https://hack.cybersystems.engineer/memex/ontologies/SeamlessDigitalEngineering#Act_of_Systems_Engineering"/>
                    </owl:Restriction>
                </owl:intersectionOf>
            </owl:Class>
        </owl:equivalentClass>
        <rdfs:subClassOf rdf:resource="https://hack.cybersystems.engineer/memex/ontologies/SeamlessDigitalEngineering#Model-Based_Engineering_Approach"/>
        <rdfs:label xml:lang="en">Model-Based Systems Engineering Approach</rdfs:label>
        <skos:altLabel>MBSE</skos:altLabel>
        <skos:definition xml:lang="en">The formalized application of modeling to support system requirements, design, analysis, verification, and validation activities beginning in the conceptual design phase and continuing throughout development and later system life-cycle phases.</skos:definition>
        <cco2:ont00001754 rdf:datatype="http://www.w3.org/2001/XMLSchema#anyURI">https://www.dau.edu/glossary/model-based-systems-engineering</cco2:ont00001754>
    </owl:Class>
    


    <!-- https://hack.cybersystems.engineer/memex/ontologies/SeamlessDigitalEngineering#Model_Theory_Discipline -->

    <owl:Class rdf:about="https://hack.cybersystems.engineer/memex/ontologies/SeamlessDigitalEngineering#Model_Theory_Discipline">
        <rdfs:subClassOf rdf:resource="https://hack.cybersystems.engineer/memex/ontologies/SeamlessDigitalEngineering#Mathematical_Logic_Discipline"/>
        <rdfs:label xml:lang="en">Model Theory Discipline</rdfs:label>
    </owl:Class>
    


    <!-- https://hack.cybersystems.engineer/memex/ontologies/SeamlessDigitalEngineering#Monitoring_and_Control_Report -->

    <owl:Class rdf:about="https://hack.cybersystems.engineer/memex/ontologies/SeamlessDigitalEngineering#Monitoring_and_Control_Report">
        <rdfs:subClassOf rdf:resource="https://www.commoncoreontologies.org/ont00000624"/>
    </owl:Class>
    


    <!-- https://hack.cybersystems.engineer/memex/ontologies/SeamlessDigitalEngineering#Narrative_Introduction_Report -->

    <owl:Class rdf:about="https://hack.cybersystems.engineer/memex/ontologies/SeamlessDigitalEngineering#Narrative_Introduction_Report">
        <owl:equivalentClass>
            <owl:Class>
                <owl:intersectionOf rdf:parseType="Collection">
                    <rdf:Description rdf:about="https://www.commoncoreontologies.org/ont00000624"/>
                    <owl:Restriction>
                        <owl:onProperty rdf:resource="http://purl.obolibrary.org/obo/BFO_0000115"/>
                        <owl:someValuesFrom rdf:resource="https://www.commoncoreontologies.org/ont00000624"/>
                    </owl:Restriction>
                    <owl:Restriction>
                        <owl:onProperty rdf:resource="http://purl.obolibrary.org/obo/BFO_0000115"/>
                        <owl:qualifiedCardinality rdf:datatype="http://www.w3.org/2001/XMLSchema#nonNegativeInteger">1</owl:qualifiedCardinality>
                        <owl:onClass rdf:resource="https://hack.cybersystems.engineer/memex/ontologies/SeamlessDigitalEngineering#Assurance_Goal_Field"/>
                    </owl:Restriction>
                </owl:intersectionOf>
            </owl:Class>
        </owl:equivalentClass>
        <rdfs:subClassOf rdf:resource="https://www.commoncoreontologies.org/ont00000624"/>
        <rdfs:comment xml:lang="en">Different parts of an assurance case typically involve different technical fields with different, possibly conflicting, terminologies and notations. The mapping can be supplied with augmenting information for translation among them in order to integrate those parts into the whole structure as specified in this Document.</rdfs:comment>
        <rdfs:comment xml:lang="en">If Uncertainty is not explicitly specified in a Claim, then the mapping can augment it by stating that the Uncertainty is negligible.</rdfs:comment>
        <rdfs:comment xml:lang="en">Narrative can be used in a number of areas, such as an executive summary of findings and conclusions as well as to expand on certain points.</rdfs:comment>
        <rdfs:comment xml:lang="en">The top-level Claim represents the Goal of Assurance Activity.</rdfs:comment>
        <rdfs:label xml:lang="en">Narrative Introduction Report</rdfs:label>
        <skos:definition xml:lang="en">a Report continuant part of an Assurance Case with the following Document Fields:

a) description of the System and Service;
b) description of the environment in which the System and Service are used (Context of Use);
c) description of the System Lifecycle;
d) the top-level Claim of the Assurance Case together with a discussion of its Uncertainty;
e) description of all changes relevant to the assurance Goal that are made to the previous version of the System or are planned for the next version;
f) an unambiguous mapping between elements of the Assurance Case and the structure provided by this Document that either covers the whole structure or is accompanied by a documented justification for not covering the whole, possibly with Information augmenting the Assurance Case for the purpose of clarifying the mapping;
g) Reports documenting the fulfilment of the Requirements of this Document.</skos:definition>
        <cco2:ont00001754 xml:lang="en">ISO/IEC/IEEE 15026-2:2022</cco2:ont00001754>
    </owl:Class>
    


    <!-- https://hack.cybersystems.engineer/memex/ontologies/SeamlessDigitalEngineering#Need -->

    <owl:Class rdf:about="https://hack.cybersystems.engineer/memex/ontologies/SeamlessDigitalEngineering#Need">
        <owl:equivalentClass>
            <owl:Class>
                <owl:intersectionOf rdf:parseType="Collection">
                    <owl:Restriction>
                        <owl:onProperty rdf:resource="https://www.commoncoreontologies.org/ont00001942"/>
                        <owl:someValuesFrom rdf:resource="https://hack.cybersystems.engineer/memex/ontologies/SeamlessDigitalEngineering#Capability"/>
                    </owl:Restriction>
                    <owl:Restriction>
                        <owl:onProperty rdf:resource="https://www.commoncoreontologies.org/ont00001942"/>
                        <owl:someValuesFrom rdf:resource="https://hack.cybersystems.engineer/memex/ontologies/SeamlessDigitalEngineering#Context_of_Use"/>
                    </owl:Restriction>
                </owl:intersectionOf>
            </owl:Class>
        </owl:equivalentClass>
        <rdfs:subClassOf rdf:resource="https://www.commoncoreontologies.org/ont00000965"/>
        <rdfs:label xml:lang="en">Need</rdfs:label>
        <skos:altLabel xml:lang="en">Stakeholder Expectation</skos:altLabel>
        <skos:altLabel xml:lang="en">Stakeholder Need</skos:altLabel>
        <skos:definition xml:lang="en">prerequisite identified as necessary for a Stakeholder, or a set of Stakeholders, to achieve an intended Outcome, implied or stated within a specific Context of Use</skos:definition>
        <cco2:ont00001754 xml:lang="en">ISO/IEC TR 25060:2023, 3.3.3, modified — changed &quot;user&quot; to &quot;stakeholder&quot;.</cco2:ont00001754>
    </owl:Class>
    


    <!-- https://hack.cybersystems.engineer/memex/ontologies/SeamlessDigitalEngineering#Need_Attribute -->

    <owl:Class rdf:about="https://hack.cybersystems.engineer/memex/ontologies/SeamlessDigitalEngineering#Need_Attribute">
        <rdfs:subClassOf rdf:resource="https://hack.cybersystems.engineer/memex/ontologies/SeamlessDigitalEngineering#Need"/>
        <rdfs:label xml:lang="en">Need Attribute</rdfs:label>
    </owl:Class>
    


    <!-- https://hack.cybersystems.engineer/memex/ontologies/SeamlessDigitalEngineering#Need_Expression -->

    <owl:Class rdf:about="https://hack.cybersystems.engineer/memex/ontologies/SeamlessDigitalEngineering#Need_Expression">
        <owl:equivalentClass>
            <owl:Class>
                <owl:intersectionOf rdf:parseType="Collection">
                    <rdf:Description rdf:about="https://hack.cybersystems.engineer/memex/ontologies/SeamlessDigitalEngineering#Need"/>
                    <owl:Restriction>
                        <owl:onProperty rdf:resource="http://purl.obolibrary.org/obo/BFO_0000178"/>
                        <owl:someValuesFrom>
                            <owl:Class>
                                <owl:intersectionOf rdf:parseType="Collection">
                                    <rdf:Description rdf:about="https://hack.cybersystems.engineer/memex/ontologies/SeamlessDigitalEngineering#Need_Attribute"/>
                                    <rdf:Description rdf:about="https://hack.cybersystems.engineer/memex/ontologies/SeamlessDigitalEngineering#Need_Statement"/>
                                </owl:intersectionOf>
                            </owl:Class>
                        </owl:someValuesFrom>
                    </owl:Restriction>
                </owl:intersectionOf>
            </owl:Class>
        </owl:equivalentClass>
        <rdfs:subClassOf rdf:resource="https://hack.cybersystems.engineer/memex/ontologies/SeamlessDigitalEngineering#Need"/>
        <rdfs:label xml:lang="en">Need Expression</rdfs:label>
        <skos:definition xml:lang="en">includes a Need Statement plus a set of associated Attributes, including validation attributes.</skos:definition>
        <cco2:ont00001754 xml:lang="en">INCOSE Needs and Requirements Manual R1.1 (2022)</cco2:ont00001754>
    </owl:Class>
    


    <!-- https://hack.cybersystems.engineer/memex/ontologies/SeamlessDigitalEngineering#Need_Set -->

    <owl:Class rdf:about="https://hack.cybersystems.engineer/memex/ontologies/SeamlessDigitalEngineering#Need_Set">
        <owl:equivalentClass>
            <owl:Class>
                <owl:intersectionOf rdf:parseType="Collection">
                    <owl:Restriction>
                        <owl:onProperty rdf:resource="https://www.commoncoreontologies.org/ont00001816"/>
                        <owl:someValuesFrom rdf:resource="https://hack.cybersystems.engineer/memex/ontologies/SeamlessDigitalEngineering#Act_of_Stakeholder_Agreement"/>
                    </owl:Restriction>
                    <owl:Restriction>
                        <owl:onProperty rdf:resource="http://purl.obolibrary.org/obo/BFO_0000178"/>
                        <owl:minQualifiedCardinality rdf:datatype="http://www.w3.org/2001/XMLSchema#nonNegativeInteger">2</owl:minQualifiedCardinality>
                        <owl:onClass rdf:resource="https://hack.cybersystems.engineer/memex/ontologies/SeamlessDigitalEngineering#Need_Expression"/>
                    </owl:Restriction>
                </owl:intersectionOf>
            </owl:Class>
        </owl:equivalentClass>
        <rdfs:subClassOf rdf:resource="https://www.commoncoreontologies.org/ont00000965"/>
        <rdfs:label xml:lang="en">Need Set</rdfs:label>
        <skos:altLabel xml:lang="en">Integrated Set of Needs</skos:altLabel>
        <skos:definition xml:lang="en">a structured set of agreed-to Need Expressions for the entity (Enterprise/Business unit/System/Subsystem/System Element/process) and its external Interfaces.</skos:definition>
        <cco2:ont00001754 xml:lang="en">INCOSE Needs and Requirements Manual R1.1 (2022)</cco2:ont00001754>
    </owl:Class>
    


    <!-- https://hack.cybersystems.engineer/memex/ontologies/SeamlessDigitalEngineering#Need_Statement -->

    <owl:Class rdf:about="https://hack.cybersystems.engineer/memex/ontologies/SeamlessDigitalEngineering#Need_Statement">
        <owl:equivalentClass>
            <owl:Class>
                <owl:intersectionOf rdf:parseType="Collection">
                    <rdf:Description rdf:about="https://hack.cybersystems.engineer/memex/ontologies/SeamlessDigitalEngineering#Need"/>
                    <owl:Restriction>
                        <owl:onProperty rdf:resource="https://www.commoncoreontologies.org/ont00001816"/>
                        <owl:someValuesFrom rdf:resource="https://hack.cybersystems.engineer/memex/ontologies/SeamlessDigitalEngineering#Act_of_Formal_Transformation"/>
                    </owl:Restriction>
                    <owl:Restriction>
                        <owl:onProperty rdf:resource="https://www.commoncoreontologies.org/ont00001920"/>
                        <owl:someValuesFrom rdf:resource="https://www.commoncoreontologies.org/ont00000496"/>
                    </owl:Restriction>
                    <owl:Restriction>
                        <owl:onProperty rdf:resource="https://www.commoncoreontologies.org/ont00001942"/>
                        <owl:someValuesFrom>
                            <owl:Class>
                                <owl:unionOf rdf:parseType="Collection">
                                    <rdf:Description rdf:about="http://purl.obolibrary.org/obo/BFO_0000034"/>
                                    <rdf:Description rdf:about="https://hack.cybersystems.engineer/memex/ontologies/SeamlessDigitalEngineering#Quality"/>
                                </owl:unionOf>
                            </owl:Class>
                        </owl:someValuesFrom>
                    </owl:Restriction>
                </owl:intersectionOf>
            </owl:Class>
        </owl:equivalentClass>
        <rdfs:subClassOf rdf:resource="https://hack.cybersystems.engineer/memex/ontologies/SeamlessDigitalEngineering#Need"/>
        <rdfs:label xml:lang="en">Need Statement</rdfs:label>
        <skos:definition xml:lang="en">the result of a Act of Formal Transformation of one or more Lifecycle Concepts into an agreed-to expectation for an entity to perform some function or possess some quality within specified constraints with acceptable risk.</skos:definition>
        <cco2:ont00001754 xml:lang="en">INCOSE Needs and Requirements Manual R1.1 (2022)</cco2:ont00001754>
    </owl:Class>
    


    <!-- https://hack.cybersystems.engineer/memex/ontologies/SeamlessDigitalEngineering#Object_Capability -->

    <owl:Class rdf:about="https://hack.cybersystems.engineer/memex/ontologies/SeamlessDigitalEngineering#Object_Capability">
        <owl:equivalentClass>
            <owl:Class>
                <owl:intersectionOf rdf:parseType="Collection">
                    <rdf:Description rdf:about="https://hack.cybersystems.engineer/memex/ontologies/SeamlessDigitalEngineering#Capability"/>
                    <owl:Restriction>
                        <owl:onProperty rdf:resource="http://purl.obolibrary.org/obo/BFO_0000054"/>
                        <owl:someValuesFrom>
                            <owl:Class>
                                <owl:intersectionOf rdf:parseType="Collection">
                                    <rdf:Description rdf:about="https://www.commoncoreontologies.org/ont00000366"/>
                                    <rdf:Description rdf:about="https://www.commoncoreontologies.org/ont00001336"/>
                                </owl:intersectionOf>
                            </owl:Class>
                        </owl:someValuesFrom>
                    </owl:Restriction>
                    <owl:Restriction>
                        <owl:onProperty rdf:resource="http://purl.obolibrary.org/obo/BFO_0000195"/>
                        <owl:someValuesFrom rdf:resource="http://www.ontologyrepository.com/CommonCoreOntologies/DigitalObject"/>
                    </owl:Restriction>
                    <owl:Restriction>
                        <owl:onProperty rdf:resource="http://purl.obolibrary.org/obo/BFO_0000195"/>
                        <owl:someValuesFrom rdf:resource="https://hack.cybersystems.engineer/memex/ontologies/SeamlessDigitalEngineering#Product_Security"/>
                    </owl:Restriction>
                </owl:intersectionOf>
            </owl:Class>
        </owl:equivalentClass>
        <rdfs:subClassOf rdf:resource="https://hack.cybersystems.engineer/memex/ontologies/SeamlessDigitalEngineering#Capability"/>
        <rdfs:comment xml:lang="en">An Object Capability can be obtained by the following combination:

- An unforgeable reference (in the sense of object references or protected pointers) that can be sent in messages.
- A message that specifies the operation to be performed.</rdfs:comment>
        <rdfs:comment xml:lang="en">The security model relies on not being able to forge references.

- Objects can interact only by sending messages on references.
- A reference can be obtained by:

    1. Initial conditions: In the initial state of the computational world being described, object A may already have a reference to object B.
    2. Parenthood: If A creates B, at that moment A obtains the only reference to the newly created B.
    3. Endowment: If A creates B, B is born with that subset of A&apos;s references with which A chose to endow it.
    4. Introduction: If A has references to both B and C, A can send to B a message containing a reference to C. B can retain that reference for subsequent use.

In the object-capability model, all computation is performed following the above rules.</rdfs:comment>
        <rdfs:label xml:lang="en">Object Capability</rdfs:label>
        <rdfs:seeAlso xml:lang="en">Dennis, Jack B. and Van Horn, Earl C., (March 1966), &quot;Programming Semantics for Multiprogrammed Computations&quot;, Communications of the ACM, 9(3):142-155. DOI: https://dx.doi.org/10.1145/365230.365252</rdfs:seeAlso>
        <rdfs:seeAlso xml:lang="en">Rees, Jonathan A. and Sussman, Gerald J., (March 1996), &quot;A security kernel based on the lambda calculus&quot;, AI Memo No. AIM-1564, Massachusetts Institute of Technology. http://hdl.handle.net/1721.1/5944</rdfs:seeAlso>
        <skos:altLabel xml:lang="en">OCap</skos:altLabel>
        <skos:definition xml:lang="en">a transferable right to perform one (or more) Act of Information Processing on a given Digital Object</skos:definition>
        <cco2:ont00001754 rdf:datatype="http://www.w3.org/2001/XMLSchema#anyURI">https://en.wikipedia.org/wiki/Object-capability_model</cco2:ont00001754>
    </owl:Class>
    


    <!-- https://hack.cybersystems.engineer/memex/ontologies/SeamlessDigitalEngineering#Object_Capability_Message -->

    <owl:Class rdf:about="https://hack.cybersystems.engineer/memex/ontologies/SeamlessDigitalEngineering#Object_Capability_Message">
        <owl:equivalentClass>
            <owl:Class>
                <owl:intersectionOf rdf:parseType="Collection">
                    <rdf:Description rdf:about="http://www.ontologyrepository.com/CommonCoreOntologies/DigitalObject"/>
                    <rdf:Description rdf:about="https://www.commoncoreontologies.org/ont00001002"/>
                    <owl:Restriction>
                        <owl:onProperty rdf:resource="http://purl.obolibrary.org/obo/BFO_0000101"/>
                        <owl:someValuesFrom rdf:resource="https://www.commoncoreontologies.org/ont00000653"/>
                    </owl:Restriction>
                </owl:intersectionOf>
            </owl:Class>
        </owl:equivalentClass>
        <rdfs:subClassOf rdf:resource="https://www.commoncoreontologies.org/ont00001002"/>
        <rdfs:label xml:lang="en">Object Capability Message</rdfs:label>
        <skos:definition xml:lang="en">A Message that is the carrier of some Algorithim that specifies the Act of Information Processing to be performed.</skos:definition>
        <cco2:ont00001754 rdf:datatype="http://www.w3.org/2001/XMLSchema#anyURI">https://en.wikipedia.org/wiki/Object-capability_model</cco2:ont00001754>
    </owl:Class>
    


    <!-- https://hack.cybersystems.engineer/memex/ontologies/SeamlessDigitalEngineering#Object_Capability_Request -->

    <owl:Class rdf:about="https://hack.cybersystems.engineer/memex/ontologies/SeamlessDigitalEngineering#Object_Capability_Request">
        <owl:equivalentClass>
            <owl:Class>
                <owl:intersectionOf rdf:parseType="Collection">
                    <rdf:Description rdf:about="http://www.ontologyrepository.com/CommonCoreOntologies/DataRequest"/>
                    <owl:Restriction>
                        <owl:onProperty rdf:resource="https://www.commoncoreontologies.org/ont00001778"/>
                        <owl:someValuesFrom rdf:resource="http://www.ontologyrepository.com/CommonCoreOntologies/DigitalObject"/>
                    </owl:Restriction>
                    <owl:Restriction>
                        <owl:onProperty rdf:resource="https://www.commoncoreontologies.org/ont00001921"/>
                        <owl:someValuesFrom rdf:resource="https://hack.cybersystems.engineer/memex/ontologies/SeamlessDigitalEngineering#Object_Reference"/>
                    </owl:Restriction>
                    <owl:Restriction>
                        <owl:onProperty rdf:resource="https://www.commoncoreontologies.org/ont00001921"/>
                        <owl:someValuesFrom rdf:resource="https://www.commoncoreontologies.org/ont00001002"/>
                    </owl:Restriction>
                    <owl:Restriction>
                        <owl:onProperty rdf:resource="https://www.commoncoreontologies.org/ont00001986"/>
                        <owl:someValuesFrom rdf:resource="https://www.commoncoreontologies.org/ont00001002"/>
                    </owl:Restriction>
                </owl:intersectionOf>
            </owl:Class>
        </owl:equivalentClass>
        <rdfs:subClassOf rdf:resource="http://www.ontologyrepository.com/CommonCoreOntologies/DataRequest"/>
        <rdfs:label xml:lang="en">Object Capability Request</rdfs:label>
        <skos:definition xml:lang="en">A Data Request in which a Message is sent via a Digital Object Reference.</skos:definition>
        <cco2:ont00001754 rdf:datatype="http://www.w3.org/2001/XMLSchema#anyURI">https://en.wikipedia.org/wiki/Object-capability_model#Glossary_of_related_terms</cco2:ont00001754>
    </owl:Class>
    


    <!-- https://hack.cybersystems.engineer/memex/ontologies/SeamlessDigitalEngineering#Object_Reference -->

    <owl:Class rdf:about="https://hack.cybersystems.engineer/memex/ontologies/SeamlessDigitalEngineering#Object_Reference">
        <owl:equivalentClass>
            <owl:Class>
                <owl:intersectionOf rdf:parseType="Collection">
                    <rdf:Description rdf:about="https://www.commoncoreontologies.org/ont00000292"/>
                    <rdf:Description rdf:about="https://www.commoncoreontologies.org/ont00000649"/>
                    <owl:Restriction>
                        <owl:onProperty rdf:resource="http://purl.obolibrary.org/obo/BFO_0000178"/>
                        <owl:someValuesFrom rdf:resource="https://hack.cybersystems.engineer/memex/ontologies/SeamlessDigitalEngineering#Message_Permission"/>
                    </owl:Restriction>
                    <owl:Restriction>
                        <owl:onProperty rdf:resource="https://www.commoncoreontologies.org/ont00001916"/>
                        <owl:someValuesFrom rdf:resource="http://www.ontologyrepository.com/CommonCoreOntologies/DigitalObject"/>
                    </owl:Restriction>
                </owl:intersectionOf>
            </owl:Class>
        </owl:equivalentClass>
        <rdfs:subClassOf rdf:resource="https://www.commoncoreontologies.org/ont00000292"/>
        <rdfs:label xml:lang="en">Object Reference</rdfs:label>
        <skos:definition xml:lang="en">An unforgeable opaque address that unambiguously designates a single Digital Object, and provides Message Permission to send Messages to that Digital Object.</skos:definition>
        <cco2:ont00001754 rdf:datatype="http://www.w3.org/2001/XMLSchema#anyURI">https://en.wikipedia.org/wiki/Object-capability_model#Glossary_of_related_terms</cco2:ont00001754>
    </owl:Class>
    


    <!-- https://hack.cybersystems.engineer/memex/ontologies/SeamlessDigitalEngineering#Observable_Element -->

    <owl:Class rdf:about="https://hack.cybersystems.engineer/memex/ontologies/SeamlessDigitalEngineering#Observable_Element">
        <owl:equivalentClass>
            <owl:Class>
                <owl:intersectionOf rdf:parseType="Collection">
                    <rdf:Description rdf:about="https://www.commoncoreontologies.org/ont00000740"/>
                    <owl:Restriction>
                        <owl:onProperty rdf:resource="https://www.commoncoreontologies.org/ont00001936"/>
                        <owl:someValuesFrom rdf:resource="https://www.commoncoreontologies.org/ont00000037"/>
                    </owl:Restriction>
                </owl:intersectionOf>
            </owl:Class>
        </owl:equivalentClass>
        <rdfs:subClassOf rdf:resource="https://www.commoncoreontologies.org/ont00000740"/>
        <rdfs:label xml:lang="en">Observable Element</rdfs:label>
        <skos:definition xml:lang="en">A Resource that is the object of an Act of Observation.</skos:definition>
        <cco2:ont00001760 rdf:datatype="http://www.w3.org/2001/XMLSchema#anyURI">https://semantic.incose.org/DEIX_Ontology</cco2:ont00001760>
    </owl:Class>
    


    <!-- https://hack.cybersystems.engineer/memex/ontologies/SeamlessDigitalEngineering#Observable_Manufacturing_Element -->

    <owl:Class rdf:about="https://hack.cybersystems.engineer/memex/ontologies/SeamlessDigitalEngineering#Observable_Manufacturing_Element">
        <owl:equivalentClass>
            <owl:Class>
                <owl:intersectionOf rdf:parseType="Collection">
                    <rdf:Description rdf:about="https://hack.cybersystems.engineer/memex/ontologies/SeamlessDigitalEngineering#Observable_Element"/>
                    <owl:Restriction>
                        <owl:onProperty rdf:resource="http://purl.obolibrary.org/obo/BFO_0000056"/>
                        <owl:someValuesFrom rdf:resource="https://www.commoncoreontologies.org/ont00001359"/>
                    </owl:Restriction>
                </owl:intersectionOf>
            </owl:Class>
        </owl:equivalentClass>
        <rdfs:subClassOf rdf:resource="https://hack.cybersystems.engineer/memex/ontologies/SeamlessDigitalEngineering#Observable_Element"/>
        <rdfs:label xml:lang="en">Observable Manufacturing Element</rdfs:label>
        <skos:definition xml:lang="en">A Resource that has an observable physical presence or operation in an Act of Manufacturing</skos:definition>
        <skos:example xml:lang="en">OMEs include personnel, equipment, material, process, facility, environment, product, and supporting document.</skos:example>
        <cco2:ont00001753 xml:lang="en">OME</cco2:ont00001753>
        <cco2:ont00001754 xml:lang="en">ISO 23247-1:2021 Automation systems and integration - Digital twin framework for manufacturing - Part 1: Overview and general principles</cco2:ont00001754>
        <cco2:ont00001760 rdf:datatype="http://www.w3.org/2001/XMLSchema#anyURI">https://semantic.incose.org/DEIX_Ontology</cco2:ont00001760>
    </owl:Class>
    


    <!-- https://hack.cybersystems.engineer/memex/ontologies/SeamlessDigitalEngineering#Ontology_Annotation_Property -->

    <owl:Class rdf:about="https://hack.cybersystems.engineer/memex/ontologies/SeamlessDigitalEngineering#Ontology_Annotation_Property">
        <rdfs:subClassOf rdf:resource="https://hack.cybersystems.engineer/memex/ontologies/SeamlessDigitalEngineering#Ontology_Entity"/>
        <rdfs:label xml:lang="en">Ontology Annotation Property</rdfs:label>
    </owl:Class>
    


    <!-- https://hack.cybersystems.engineer/memex/ontologies/SeamlessDigitalEngineering#Ontology_Class -->

    <owl:Class rdf:about="https://hack.cybersystems.engineer/memex/ontologies/SeamlessDigitalEngineering#Ontology_Class">
        <rdfs:subClassOf rdf:resource="https://hack.cybersystems.engineer/memex/ontologies/SeamlessDigitalEngineering#Ontology_Entity"/>
        <rdfs:label xml:lang="en">Ontology Class</rdfs:label>
        <skos:altLabel xml:lang="en">Concept</skos:altLabel>
    </owl:Class>
    


    <!-- https://hack.cybersystems.engineer/memex/ontologies/SeamlessDigitalEngineering#Ontology_Data_Property -->

    <owl:Class rdf:about="https://hack.cybersystems.engineer/memex/ontologies/SeamlessDigitalEngineering#Ontology_Data_Property">
        <rdfs:subClassOf rdf:resource="https://hack.cybersystems.engineer/memex/ontologies/SeamlessDigitalEngineering#Ontology_Entity"/>
        <rdfs:label xml:lang="en">Ontology Data Property</rdfs:label>
    </owl:Class>
    


    <!-- https://hack.cybersystems.engineer/memex/ontologies/SeamlessDigitalEngineering#Ontology_Entity -->

    <owl:Class rdf:about="https://hack.cybersystems.engineer/memex/ontologies/SeamlessDigitalEngineering#Ontology_Entity">
        <rdfs:subClassOf rdf:resource="http://www.ontologyrepository.com/CommonCoreOntologies/Ontology"/>
        <rdfs:label xml:lang="en">Ontology Entity</rdfs:label>
    </owl:Class>
    


    <!-- https://hack.cybersystems.engineer/memex/ontologies/SeamlessDigitalEngineering#Ontology_Individual -->

    <owl:Class rdf:about="https://hack.cybersystems.engineer/memex/ontologies/SeamlessDigitalEngineering#Ontology_Individual">
        <rdfs:subClassOf rdf:resource="https://hack.cybersystems.engineer/memex/ontologies/SeamlessDigitalEngineering#Ontology_Entity"/>
        <rdfs:label xml:lang="en">Ontology Individual</rdfs:label>
    </owl:Class>
    


    <!-- https://hack.cybersystems.engineer/memex/ontologies/SeamlessDigitalEngineering#Ontology_Object_Property -->

    <owl:Class rdf:about="https://hack.cybersystems.engineer/memex/ontologies/SeamlessDigitalEngineering#Ontology_Object_Property">
        <rdfs:subClassOf rdf:resource="https://hack.cybersystems.engineer/memex/ontologies/SeamlessDigitalEngineering#Ontology_Entity"/>
        <rdfs:label xml:lang="en">Ontology Object Property</rdfs:label>
        <skos:altLabel xml:lang="en">Role</skos:altLabel>
    </owl:Class>
    


    <!-- https://hack.cybersystems.engineer/memex/ontologies/SeamlessDigitalEngineering#Operation_Process -->

    <owl:Class rdf:about="https://hack.cybersystems.engineer/memex/ontologies/SeamlessDigitalEngineering#Operation_Process">
        <rdfs:subClassOf rdf:resource="https://hack.cybersystems.engineer/memex/ontologies/SeamlessDigitalEngineering#Technical_Process"/>
        <rdfs:label xml:lang="en">Operation Process</rdfs:label>
        <skos:definition xml:lang="en">The purpose of the operation process is to use the system to provide its products or services.</skos:definition>
        <cco2:ont00001754>ISO/IEC/IEEE 15288:2023</cco2:ont00001754>
    </owl:Class>
    


    <!-- https://hack.cybersystems.engineer/memex/ontologies/SeamlessDigitalEngineering#Operational_Architecture -->

    <owl:Class rdf:about="https://hack.cybersystems.engineer/memex/ontologies/SeamlessDigitalEngineering#Operational_Architecture">
        <owl:equivalentClass>
            <owl:Restriction>
                <owl:onProperty rdf:resource="https://www.commoncoreontologies.org/ont00001920"/>
                <owl:someValuesFrom rdf:resource="https://hack.cybersystems.engineer/memex/ontologies/SeamlessDigitalEngineering#Operational_Viewpoint"/>
            </owl:Restriction>
        </owl:equivalentClass>
        <rdfs:subClassOf rdf:resource="https://hack.cybersystems.engineer/memex/ontologies/SeamlessDigitalEngineering#Architecture_View"/>
        <rdfs:label xml:lang="en">Operational Architecture</rdfs:label>
        <skos:altLabel xml:lang="en">Operational (View of) Architecture</skos:altLabel>
        <skos:definition xml:lang="en">when the associated viewpoint is dealing with operations</skos:definition>
        <cco2:ont00001754 xml:lang="en">ISO/IEC/IEEE 42020:2019</cco2:ont00001754>
    </owl:Class>
    


    <!-- https://hack.cybersystems.engineer/memex/ontologies/SeamlessDigitalEngineering#Operational_Concept -->

    <owl:Class rdf:about="https://hack.cybersystems.engineer/memex/ontologies/SeamlessDigitalEngineering#Operational_Concept">
        <owl:equivalentClass>
            <owl:Class>
                <owl:intersectionOf rdf:parseType="Collection">
                    <owl:Restriction>
                        <owl:onProperty rdf:resource="https://www.commoncoreontologies.org/ont00001942"/>
                        <owl:someValuesFrom rdf:resource="https://hack.cybersystems.engineer/memex/ontologies/SeamlessDigitalEngineering#Context_of_Use"/>
                    </owl:Restriction>
                    <owl:Restriction>
                        <owl:onProperty rdf:resource="https://www.commoncoreontologies.org/ont00001942"/>
                        <owl:someValuesFrom rdf:resource="https://hack.cybersystems.engineer/memex/ontologies/SeamlessDigitalEngineering#System"/>
                    </owl:Restriction>
                </owl:intersectionOf>
            </owl:Class>
        </owl:equivalentClass>
        <rdfs:subClassOf rdf:resource="https://hack.cybersystems.engineer/memex/ontologies/SeamlessDigitalEngineering#Lifecycle_Concept"/>
        <rdfs:comment xml:lang="en">Although the canonical definition is the same as Concept of Operations, the standard document note provided distinguishes it by perspective and thus was added to this definition.</rdfs:comment>
        <rdfs:label xml:lang="en">Operational Concept</rdfs:label>
        <skos:altLabel>OpsCon</skos:altLabel>
        <skos:definition xml:lang="en">A &quot;verbal and graphic statement of an Organization’s assumptions or intent in regard to an operation or series of operations of a specific System or a related set of specific new, existing or modified Systems&quot;, &quot;in the Organization&apos;s Operational Environment from the Users&apos; and Operators&apos; perspective&quot;</skos:definition>
        <cco2:ont00001754>ISO/IEC/IEEE 15288:2023</cco2:ont00001754>
    </owl:Class>
    


    <!-- https://hack.cybersystems.engineer/memex/ontologies/SeamlessDigitalEngineering#Operational_Environment -->

    <owl:Class rdf:about="https://hack.cybersystems.engineer/memex/ontologies/SeamlessDigitalEngineering#Operational_Environment">
        <owl:equivalentClass>
            <owl:Class>
                <owl:intersectionOf rdf:parseType="Collection">
                    <rdf:Description rdf:about="https://hack.cybersystems.engineer/memex/ontologies/SeamlessDigitalEngineering#System_Environment"/>
                    <owl:Restriction>
                        <owl:onProperty rdf:resource="http://purl.obolibrary.org/obo/BFO_0000183"/>
                        <owl:someValuesFrom rdf:resource="https://hack.cybersystems.engineer/memex/ontologies/SeamlessDigitalEngineering#Operation_Process"/>
                    </owl:Restriction>
                </owl:intersectionOf>
            </owl:Class>
        </owl:equivalentClass>
        <rdfs:subClassOf rdf:resource="https://hack.cybersystems.engineer/memex/ontologies/SeamlessDigitalEngineering#System_Environment"/>
        <rdfs:label xml:lang="en">Operational Environment</rdfs:label>
        <cco2:ont00001760 rdf:datatype="http://www.w3.org/2001/XMLSchema#anyURI">https://semantic.incose.org/DEIX_Ontology</cco2:ont00001760>
    </owl:Class>
    


    <!-- https://hack.cybersystems.engineer/memex/ontologies/SeamlessDigitalEngineering#Operational_Viewpoint -->

    <owl:Class rdf:about="https://hack.cybersystems.engineer/memex/ontologies/SeamlessDigitalEngineering#Operational_Viewpoint">
        <owl:equivalentClass>
            <owl:Class>
                <owl:intersectionOf rdf:parseType="Collection">
                    <rdf:Description rdf:about="https://hack.cybersystems.engineer/memex/ontologies/SeamlessDigitalEngineering#Architecture_Viewpoint"/>
                    <owl:Restriction>
                        <owl:onProperty rdf:resource="https://www.commoncoreontologies.org/ont00001942"/>
                        <owl:someValuesFrom rdf:resource="https://hack.cybersystems.engineer/memex/ontologies/SeamlessDigitalEngineering#Operational_Architecture"/>
                    </owl:Restriction>
                </owl:intersectionOf>
            </owl:Class>
        </owl:equivalentClass>
        <rdfs:subClassOf rdf:resource="https://hack.cybersystems.engineer/memex/ontologies/SeamlessDigitalEngineering#Architecture_Viewpoint"/>
        <rdfs:label xml:lang="en">Operational Viewpoint</rdfs:label>
        <skos:definition xml:lang="en">An architecture viewpoint focused on &quot;ongoing execution of activities that produce the same product or provide a repetitive service&quot;</skos:definition>
        <cco2:ont00001754 xml:lang="en">derived from ISO/IEC/IEEE 24765:2017 definition of &apos;operations&apos;</cco2:ont00001754>
    </owl:Class>
    


    <!-- https://hack.cybersystems.engineer/memex/ontologies/SeamlessDigitalEngineering#Operator -->

    <owl:Class rdf:about="https://hack.cybersystems.engineer/memex/ontologies/SeamlessDigitalEngineering#Operator">
        <owl:equivalentClass>
            <owl:Class>
                <owl:intersectionOf rdf:parseType="Collection">
                    <rdf:Description rdf:about="https://hack.cybersystems.engineer/memex/ontologies/SeamlessDigitalEngineering#Stakeholder"/>
                    <owl:Restriction>
                        <owl:onProperty rdf:resource="http://purl.obolibrary.org/obo/BFO_0000196"/>
                        <owl:someValuesFrom rdf:resource="https://www.commoncoreontologies.org/ont00001006"/>
                    </owl:Restriction>
                </owl:intersectionOf>
            </owl:Class>
        </owl:equivalentClass>
        <rdfs:subClassOf rdf:resource="https://hack.cybersystems.engineer/memex/ontologies/SeamlessDigitalEngineering#Stakeholder"/>
        <rdfs:label xml:lang="en">Operator</rdfs:label>
        <skos:definition xml:lang="en">individual or organization that performs the user operations of a system</skos:definition>
        <cco2:ont00001754 xml:lang="en">ISO/IEC/IEEE 15288:2023</cco2:ont00001754>
    </owl:Class>
    


    <!-- https://hack.cybersystems.engineer/memex/ontologies/SeamlessDigitalEngineering#Opportunity -->

    <owl:Class rdf:about="https://hack.cybersystems.engineer/memex/ontologies/SeamlessDigitalEngineering#Opportunity">
        <rdfs:subClassOf rdf:resource="https://www.commoncoreontologies.org/ont00000004"/>
    </owl:Class>
    


    <!-- https://hack.cybersystems.engineer/memex/ontologies/SeamlessDigitalEngineering#Organizational_Project-enabling_Process -->

    <owl:Class rdf:about="https://hack.cybersystems.engineer/memex/ontologies/SeamlessDigitalEngineering#Organizational_Project-enabling_Process">
        <rdfs:subClassOf rdf:resource="https://hack.cybersystems.engineer/memex/ontologies/SeamlessDigitalEngineering#System_Lifecycle_Process"/>
        <rdfs:label xml:lang="en">Organizational Project-enabling Process</rdfs:label>
        <skos:definition xml:lang="en">The organizational project-enabling processes are concerned with providing the resources needed to enable the project to meet the needs and expectations of the organization’s stakeholders. The organizational project-enabling processes are typically concerned at a strategic level with the management and improvement of the organization’s undertaking, with the provision and deployment of resources and assets, and with its management of risks in competitive or uncertain situations.</skos:definition>
        <cco2:ont00001754>ISO/IEC/IEEE 15288:2023</cco2:ont00001754>
    </owl:Class>
    


    <!-- https://hack.cybersystems.engineer/memex/ontologies/SeamlessDigitalEngineering#Paradigm -->

    <owl:Class rdf:about="https://hack.cybersystems.engineer/memex/ontologies/SeamlessDigitalEngineering#Paradigm">
        <owl:equivalentClass>
            <owl:Class>
                <owl:intersectionOf rdf:parseType="Collection">
                    <rdf:Description rdf:about="https://www.commoncoreontologies.org/ont00000965"/>
                    <owl:Restriction>
                        <owl:onProperty rdf:resource="http://purl.obolibrary.org/obo/BFO_0000178"/>
                        <owl:someValuesFrom>
                            <owl:Class>
                                <owl:intersectionOf rdf:parseType="Collection">
                                    <rdf:Description rdf:about="https://hack.cybersystems.engineer/memex/ontologies/SeamlessDigitalEngineering#Approach"/>
                                    <rdf:Description rdf:about="https://hack.cybersystems.engineer/memex/ontologies/SeamlessDigitalEngineering#Method"/>
                                    <rdf:Description rdf:about="https://hack.cybersystems.engineer/memex/ontologies/SeamlessDigitalEngineering#Principle"/>
                                </owl:intersectionOf>
                            </owl:Class>
                        </owl:someValuesFrom>
                    </owl:Restriction>
                </owl:intersectionOf>
            </owl:Class>
        </owl:equivalentClass>
        <rdfs:subClassOf rdf:resource="https://www.commoncoreontologies.org/ont00000965"/>
        <rdfs:label xml:lang="en">Paradigm</rdfs:label>
        <skos:definition xml:lang="en">a distinct set of concepts or thought patterns, including theories, research methods, postulates, and standards for what constitute legitimate contributions to a field</skos:definition>
        <cco2:ont00001754 rdf:datatype="http://www.w3.org/2001/XMLSchema#anyURI">https://en.wikipedia.org/wiki/Paradigm</cco2:ont00001754>
    </owl:Class>
    


    <!-- https://hack.cybersystems.engineer/memex/ontologies/SeamlessDigitalEngineering#Pattern-Based_Systems_Engineering -->

    <owl:Class rdf:about="https://hack.cybersystems.engineer/memex/ontologies/SeamlessDigitalEngineering#Pattern-Based_Systems_Engineering">
        <owl:equivalentClass>
            <owl:Class>
                <owl:intersectionOf rdf:parseType="Collection">
                    <rdf:Description rdf:about="https://hack.cybersystems.engineer/memex/ontologies/SeamlessDigitalEngineering#Model-Based_Systems_Engineering_Approach"/>
                    <owl:Restriction>
                        <owl:onProperty rdf:resource="https://www.commoncoreontologies.org/ont00001808"/>
                        <owl:someValuesFrom rdf:resource="https://hack.cybersystems.engineer/memex/ontologies/SeamlessDigitalEngineering#System_Architecture_Pattern"/>
                    </owl:Restriction>
                </owl:intersectionOf>
            </owl:Class>
        </owl:equivalentClass>
        <rdfs:subClassOf rdf:resource="https://hack.cybersystems.engineer/memex/ontologies/SeamlessDigitalEngineering#Model-Based_Systems_Engineering_Approach"/>
        <rdfs:label xml:lang="en">Pattern-Based Systems Engineering</rdfs:label>
    </owl:Class>
    


    <!-- https://hack.cybersystems.engineer/memex/ontologies/SeamlessDigitalEngineering#Physical_Architecture -->

    <owl:Class rdf:about="https://hack.cybersystems.engineer/memex/ontologies/SeamlessDigitalEngineering#Physical_Architecture">
        <rdfs:subClassOf rdf:resource="https://hack.cybersystems.engineer/memex/ontologies/SeamlessDigitalEngineering#Architecture_View"/>
        <rdfs:label xml:lang="en">Physical Architecture</rdfs:label>
        <skos:altLabel xml:lang="en">Physical (View of) Architecture</skos:altLabel>
        <skos:definition xml:lang="en">A physical view of the architecture description is an arrangement of system elements and physical interfaces that provides the design solution for a product, service or enterprise, and is intended to satisfy logical architecture elements and system requirements.</skos:definition>
        <cco2:ont00001754 xml:lang="en">ISO/IEC/IEEE 42020:2019</cco2:ont00001754>
    </owl:Class>
    


    <!-- https://hack.cybersystems.engineer/memex/ontologies/SeamlessDigitalEngineering#Physical_Twin_Role -->

    <owl:Class rdf:about="https://hack.cybersystems.engineer/memex/ontologies/SeamlessDigitalEngineering#Physical_Twin_Role">
        <rdfs:subClassOf rdf:resource="https://hack.cybersystems.engineer/memex/ontologies/SeamlessDigitalEngineering#System-of-Interest_Role"/>
        <rdfs:subClassOf>
            <owl:Restriction>
                <owl:onProperty rdf:resource="http://purl.obolibrary.org/obo/BFO_0000195"/>
                <owl:someValuesFrom rdf:resource="https://hack.cybersystems.engineer/memex/ontologies/SeamlessDigitalEngineering#Digital_Twin_Role"/>
            </owl:Restriction>
        </rdfs:subClassOf>
        <rdfs:label xml:lang="en">Physical Twin Role</rdfs:label>
    </owl:Class>
    


    <!-- https://hack.cybersystems.engineer/memex/ontologies/SeamlessDigitalEngineering#Physical_Viewpoint -->

    <owl:Class rdf:about="https://hack.cybersystems.engineer/memex/ontologies/SeamlessDigitalEngineering#Physical_Viewpoint">
        <owl:equivalentClass>
            <owl:Class>
                <owl:intersectionOf rdf:parseType="Collection">
                    <rdf:Description rdf:about="https://hack.cybersystems.engineer/memex/ontologies/SeamlessDigitalEngineering#Architecture_Viewpoint"/>
                    <owl:Restriction>
                        <owl:onProperty rdf:resource="https://www.commoncoreontologies.org/ont00001942"/>
                        <owl:someValuesFrom rdf:resource="https://hack.cybersystems.engineer/memex/ontologies/SeamlessDigitalEngineering#Physical_Architecture"/>
                    </owl:Restriction>
                </owl:intersectionOf>
            </owl:Class>
        </owl:equivalentClass>
        <rdfs:subClassOf rdf:resource="https://hack.cybersystems.engineer/memex/ontologies/SeamlessDigitalEngineering#Architecture_Viewpoint"/>
        <rdfs:label xml:lang="en">Physical Viewpoint</rdfs:label>
    </owl:Class>
    


    <!-- https://hack.cybersystems.engineer/memex/ontologies/SeamlessDigitalEngineering#Portfolio -->

    <owl:Class rdf:about="https://hack.cybersystems.engineer/memex/ontologies/SeamlessDigitalEngineering#Portfolio">
        <rdfs:subClassOf rdf:resource="https://www.commoncoreontologies.org/ont00000228"/>
        <rdfs:label xml:lang="en">Portfolio</rdfs:label>
        <skos:definition xml:lang="en">Projects, Programs, Subportfolios, and operations managed as a group to achieve strategic Objectives</skos:definition>
        <cco2:ont00001754 xml:lang="en">ISO/IEC/IEEE 24765:2017</cco2:ont00001754>
    </owl:Class>
    


    <!-- https://hack.cybersystems.engineer/memex/ontologies/SeamlessDigitalEngineering#Portfolio_Management_Process -->

    <owl:Class rdf:about="https://hack.cybersystems.engineer/memex/ontologies/SeamlessDigitalEngineering#Portfolio_Management_Process">
        <rdfs:subClassOf rdf:resource="https://hack.cybersystems.engineer/memex/ontologies/SeamlessDigitalEngineering#Organizational_Project-enabling_Process"/>
        <rdfs:label xml:lang="en">Portfolio Management Process</rdfs:label>
        <skos:definition xml:lang="en">The purpose of the portfolio management process is to initiate and sustain necessary, sufficient, and suitable projects to meet the strategic objectives of the organization.</skos:definition>
        <cco2:ont00001754>ISO/IEC/IEEE 15288:2023</cco2:ont00001754>
    </owl:Class>
    


    <!-- https://hack.cybersystems.engineer/memex/ontologies/SeamlessDigitalEngineering#Positive_Consequence -->

    <owl:Class rdf:about="https://hack.cybersystems.engineer/memex/ontologies/SeamlessDigitalEngineering#Positive_Consequence">
        <owl:equivalentClass>
            <owl:Class>
                <owl:intersectionOf rdf:parseType="Collection">
                    <rdf:Description rdf:about="https://hack.cybersystems.engineer/memex/ontologies/SeamlessDigitalEngineering#Consequence"/>
                    <owl:Restriction>
                        <owl:onProperty rdf:resource="https://www.commoncoreontologies.org/ont00001803"/>
                        <owl:someValuesFrom rdf:resource="https://www.commoncoreontologies.org/ont00000554"/>
                    </owl:Restriction>
                </owl:intersectionOf>
            </owl:Class>
        </owl:equivalentClass>
        <rdfs:subClassOf rdf:resource="https://hack.cybersystems.engineer/memex/ontologies/SeamlessDigitalEngineering#Consequence"/>
        <rdfs:label xml:lang="en">Positive Consequence</rdfs:label>
        <skos:altLabel xml:lang="en">Desirable Consequence</skos:altLabel>
        <skos:definition xml:lang="en">Consequence associated with a benefit or Gain or avoiding an Adverse Consequence</skos:definition>
        <cco2:ont00001754 xml:lang="en">ISO/IEC/IEEE 15026-1:2019</cco2:ont00001754>
    </owl:Class>
    


    <!-- https://hack.cybersystems.engineer/memex/ontologies/SeamlessDigitalEngineering#Predicate -->

    <owl:Class rdf:about="https://hack.cybersystems.engineer/memex/ontologies/SeamlessDigitalEngineering#Predicate">
        <rdfs:subClassOf rdf:resource="https://www.commoncoreontologies.org/ont00000932"/>
        <rdfs:label xml:lang="en">Predicate</rdfs:label>
        <skos:altLabel xml:lang="en">Predicate Function</skos:altLabel>
        <skos:definition xml:lang="en">a Computing Artifact Function that returns true or false</skos:definition>
    </owl:Class>
    


    <!-- https://hack.cybersystems.engineer/memex/ontologies/SeamlessDigitalEngineering#Predicate_Argument_Structure -->

    <owl:Class rdf:about="https://hack.cybersystems.engineer/memex/ontologies/SeamlessDigitalEngineering#Predicate_Argument_Structure">
        <owl:equivalentClass>
            <owl:Class>
                <owl:intersectionOf rdf:parseType="Collection">
                    <rdf:Description rdf:about="https://hack.cybersystems.engineer/memex/ontologies/SeamlessDigitalEngineering#Information_Model"/>
                    <owl:Restriction>
                        <owl:onProperty rdf:resource="https://www.commoncoreontologies.org/ont00001808"/>
                        <owl:someValuesFrom rdf:resource="https://hack.cybersystems.engineer/memex/ontologies/SeamlessDigitalEngineering#Argument"/>
                    </owl:Restriction>
                    <owl:Restriction>
                        <owl:onProperty rdf:resource="https://www.commoncoreontologies.org/ont00001808"/>
                        <owl:someValuesFrom rdf:resource="https://hack.cybersystems.engineer/memex/ontologies/SeamlessDigitalEngineering#Predicate"/>
                    </owl:Restriction>
                </owl:intersectionOf>
            </owl:Class>
        </owl:equivalentClass>
        <rdfs:subClassOf rdf:resource="https://www.commoncoreontologies.org/ont00001069"/>
        <rdfs:label xml:lang="en">Predicate Argument Structure</rdfs:label>
        <skos:altLabel xml:lang="en">Formal Argument</skos:altLabel>
        <skos:definition xml:lang="en">formal representation of the core semantic content of an utterance, consisting of a Predicate constant, and its Arguments</skos:definition>
        <cco2:ont00001754 xml:lang="en">ISO 24617-4:2014 Language resource management - Semantic annotation framework (SemAF) - Part 4: Semantic roles (SemAF-SR)</cco2:ont00001754>
    </owl:Class>
    


    <!-- https://hack.cybersystems.engineer/memex/ontologies/SeamlessDigitalEngineering#Principle -->

    <owl:Class rdf:about="https://hack.cybersystems.engineer/memex/ontologies/SeamlessDigitalEngineering#Principle">
        <owl:equivalentClass>
            <owl:Restriction>
                <owl:onProperty rdf:resource="https://www.commoncoreontologies.org/ont00001942"/>
                <owl:someValuesFrom rdf:resource="https://www.commoncoreontologies.org/ont00001347"/>
            </owl:Restriction>
        </owl:equivalentClass>
        <rdfs:subClassOf rdf:resource="https://www.commoncoreontologies.org/ont00000965"/>
        <skos:definition xml:lang="en">a fundamental truth or proposition that serves as the foundation for a system of belief or behaviour or for a chain of reasoning.</skos:definition>
        <skos:definition xml:lang="en">a rule or belief governing one’s behavior</skos:definition>
        <cco2:ont00001754 rdf:datatype="http://www.w3.org/2001/XMLSchema#anyURI">https://sebokwiki.org/wiki/Principle_(glossary)</cco2:ont00001754>
    </owl:Class>
    


    <!-- https://hack.cybersystems.engineer/memex/ontologies/SeamlessDigitalEngineering#Problem -->

    <owl:Class rdf:about="https://hack.cybersystems.engineer/memex/ontologies/SeamlessDigitalEngineering#Problem">
        <owl:equivalentClass>
            <owl:Restriction>
                <owl:onProperty rdf:resource="https://www.commoncoreontologies.org/ont00001866"/>
                <owl:someValuesFrom rdf:resource="https://hack.cybersystems.engineer/memex/ontologies/SeamlessDigitalEngineering#Stakeholder"/>
            </owl:Restriction>
        </owl:equivalentClass>
        <rdfs:subClassOf rdf:resource="https://www.commoncoreontologies.org/ont00000004"/>
        <skos:definition xml:lang="en">difficulty, uncertainty, or otherwise realised and undesirable event, set of events, condition, or situation that requires investigation and corrective action</skos:definition>
        <cco2:ont00001754>ISO/IEC/IEEE 15288:2023</cco2:ont00001754>
    </owl:Class>
    


    <!-- https://hack.cybersystems.engineer/memex/ontologies/SeamlessDigitalEngineering#Problem_Definition -->

    <owl:Class rdf:about="https://hack.cybersystems.engineer/memex/ontologies/SeamlessDigitalEngineering#Problem_Definition">
        <owl:equivalentClass>
            <owl:Class>
                <owl:intersectionOf rdf:parseType="Collection">
                    <owl:Restriction>
                        <owl:onProperty rdf:resource="https://www.commoncoreontologies.org/ont00001920"/>
                        <owl:someValuesFrom rdf:resource="https://hack.cybersystems.engineer/memex/ontologies/SeamlessDigitalEngineering#System_Architecture_Model"/>
                    </owl:Restriction>
                    <owl:Restriction>
                        <owl:onProperty rdf:resource="https://www.commoncoreontologies.org/ont00001982"/>
                        <owl:someValuesFrom rdf:resource="https://hack.cybersystems.engineer/memex/ontologies/SeamlessDigitalEngineering#Problem"/>
                    </owl:Restriction>
                </owl:intersectionOf>
            </owl:Class>
        </owl:equivalentClass>
        <rdfs:subClassOf rdf:resource="https://www.commoncoreontologies.org/ont00000853"/>
        <rdfs:label xml:lang="en">Problem Definition</rdfs:label>
        <skos:definition xml:lang="en">statement of a problem, which can include a description of the data, the method, the procedures, and algorithms used to solve it</skos:definition>
        <cco2:ont00001754 xml:lang="en">ISO/IEC/IEEE 24765:2017 — Systems and software engineering — Vocabulary</cco2:ont00001754>
    </owl:Class>
    


    <!-- https://hack.cybersystems.engineer/memex/ontologies/SeamlessDigitalEngineering#Problem_Report -->

    <owl:Class rdf:about="https://hack.cybersystems.engineer/memex/ontologies/SeamlessDigitalEngineering#Problem_Report">
        <rdfs:subClassOf rdf:resource="https://www.commoncoreontologies.org/ont00000624"/>
    </owl:Class>
    


    <!-- https://hack.cybersystems.engineer/memex/ontologies/SeamlessDigitalEngineering#Procedure -->

    <owl:Class rdf:about="https://hack.cybersystems.engineer/memex/ontologies/SeamlessDigitalEngineering#Procedure">
        <rdfs:subClassOf rdf:resource="https://hack.cybersystems.engineer/memex/ontologies/SeamlessDigitalEngineering#Method"/>
        <rdfs:comment xml:lang="en">Procedure can be documented or not.</rdfs:comment>
        <rdfs:label xml:lang="en">Procedure</rdfs:label>
        <skos:altLabel xml:lang="en">Activity Plan</skos:altLabel>
        <skos:definition xml:lang="en">specified way to carry out an Activity or Planned Act</skos:definition>
        <cco2:ont00001754 xml:lang="en">ISO/IEC 29110-1-2:2024</cco2:ont00001754>
    </owl:Class>
    


    <!-- https://hack.cybersystems.engineer/memex/ontologies/SeamlessDigitalEngineering#Process_Improvement_Report -->

    <owl:Class rdf:about="https://hack.cybersystems.engineer/memex/ontologies/SeamlessDigitalEngineering#Process_Improvement_Report">
        <rdfs:subClassOf rdf:resource="https://www.commoncoreontologies.org/ont00000624"/>
    </owl:Class>
    


    <!-- https://hack.cybersystems.engineer/memex/ontologies/SeamlessDigitalEngineering#Process_Outcome -->

    <owl:Class rdf:about="https://hack.cybersystems.engineer/memex/ontologies/SeamlessDigitalEngineering#Process_Outcome">
        <owl:equivalentClass>
            <owl:Class>
                <owl:intersectionOf rdf:parseType="Collection">
                    <rdf:Description rdf:about="https://www.commoncoreontologies.org/ont00000660"/>
                    <owl:Restriction>
                        <owl:onProperty rdf:resource="https://www.commoncoreontologies.org/ont00001920"/>
                        <owl:someValuesFrom rdf:resource="https://hack.cybersystems.engineer/memex/ontologies/SeamlessDigitalEngineering#Process_Purpose"/>
                    </owl:Restriction>
                </owl:intersectionOf>
            </owl:Class>
        </owl:equivalentClass>
        <rdfs:subClassOf rdf:resource="https://www.commoncoreontologies.org/ont00000660"/>
        <rdfs:label xml:lang="en">Process Outcome</rdfs:label>
        <skos:altLabel xml:lang="en">Outcome</skos:altLabel>
        <skos:definition xml:lang="en">observable result of the successful achievement of the Process Purpose</skos:definition>
        <cco2:ont00001754>ISO/IEC/IEEE 15288:2023</cco2:ont00001754>
        <cco2:ont00001760 rdf:datatype="http://www.w3.org/2001/XMLSchema#anyURI">https://semantic.incose.org/DEIX_Ontology</cco2:ont00001760>
    </owl:Class>
    


    <!-- https://hack.cybersystems.engineer/memex/ontologies/SeamlessDigitalEngineering#Process_Purpose -->

    <owl:Class rdf:about="https://hack.cybersystems.engineer/memex/ontologies/SeamlessDigitalEngineering#Process_Purpose">
        <owl:equivalentClass>
            <owl:Class>
                <owl:intersectionOf rdf:parseType="Collection">
                    <owl:Restriction>
                        <owl:onProperty rdf:resource="http://purl.obolibrary.org/obo/BFO_0000058"/>
                        <owl:someValuesFrom rdf:resource="https://hack.cybersystems.engineer/memex/ontologies/SeamlessDigitalEngineering#Process_Outcome"/>
                    </owl:Restriction>
                    <owl:Restriction>
                        <owl:onProperty rdf:resource="https://www.commoncoreontologies.org/ont00001808"/>
                        <owl:someValuesFrom rdf:resource="http://purl.obolibrary.org/obo/BFO_0000015"/>
                    </owl:Restriction>
                </owl:intersectionOf>
            </owl:Class>
        </owl:equivalentClass>
        <rdfs:subClassOf rdf:resource="https://hack.cybersystems.engineer/memex/ontologies/SeamlessDigitalEngineering#Purpose"/>
        <rdfs:label xml:lang="en">Process Purpose</rdfs:label>
        <skos:definition xml:lang="en">high-level objective of performing the process and the likely outcomes of effective implementation of the process</skos:definition>
        <cco2:ont00001754>ISO/IEC/IEEE 15288:2023</cco2:ont00001754>
    </owl:Class>
    


    <!-- https://hack.cybersystems.engineer/memex/ontologies/SeamlessDigitalEngineering#Product -->

    <owl:Class rdf:about="https://hack.cybersystems.engineer/memex/ontologies/SeamlessDigitalEngineering#Product">
        <owl:equivalentClass>
            <owl:Class>
                <owl:intersectionOf rdf:parseType="Collection">
                    <rdf:Description rdf:about="https://www.commoncoreontologies.org/ont00000995"/>
                    <owl:Restriction>
                        <owl:onProperty rdf:resource="http://purl.obolibrary.org/obo/BFO_0000196"/>
                        <owl:someValuesFrom rdf:resource="https://hack.cybersystems.engineer/memex/ontologies/SeamlessDigitalEngineering#Product_Capability"/>
                    </owl:Restriction>
                    <owl:Restriction>
                        <owl:onProperty rdf:resource="https://www.commoncoreontologies.org/ont00001816"/>
                        <owl:someValuesFrom>
                            <owl:Class>
                                <owl:intersectionOf rdf:parseType="Collection">
                                    <rdf:Description rdf:about="https://hack.cybersystems.engineer/memex/ontologies/SeamlessDigitalEngineering#Act_of_Engineering"/>
                                    <rdf:Description rdf:about="https://www.commoncoreontologies.org/ont00001359"/>
                                </owl:intersectionOf>
                            </owl:Class>
                        </owl:someValuesFrom>
                    </owl:Restriction>
                </owl:intersectionOf>
            </owl:Class>
        </owl:equivalentClass>
        <rdfs:subClassOf rdf:resource="https://hack.cybersystems.engineer/memex/ontologies/SeamlessDigitalEngineering#Engineered_System"/>
        <skos:altLabel xml:lang="en">Good</skos:altLabel>
        <skos:definition xml:lang="en">output of an Organization that can be produced without any transaction taking place between the Organization and the Customer</skos:definition>
        <cco2:ont00001754>ISO/IEC/IEEE 15288:2023</cco2:ont00001754>
    </owl:Class>
    


    <!-- https://hack.cybersystems.engineer/memex/ontologies/SeamlessDigitalEngineering#Product_Accountability -->

    <owl:Class rdf:about="https://hack.cybersystems.engineer/memex/ontologies/SeamlessDigitalEngineering#Product_Accountability">
        <rdfs:subClassOf rdf:resource="https://hack.cybersystems.engineer/memex/ontologies/SeamlessDigitalEngineering#Product_Security"/>
        <rdfs:label xml:lang="en">Product Accountability</rdfs:label>
        <skos:definition xml:lang="en">Capability of a Product to enable actions of an entity to be traced uniquely to the entity</skos:definition>
        <cco2:ont00001754 xml:lang="en">ISO/IEC 25010:2023</cco2:ont00001754>
    </owl:Class>
    


    <!-- https://hack.cybersystems.engineer/memex/ontologies/SeamlessDigitalEngineering#Product_Adaptability -->

    <owl:Class rdf:about="https://hack.cybersystems.engineer/memex/ontologies/SeamlessDigitalEngineering#Product_Adaptability">
        <rdfs:subClassOf rdf:resource="https://hack.cybersystems.engineer/memex/ontologies/SeamlessDigitalEngineering#Product_Flexibility"/>
        <rdfs:comment xml:lang="en">Adaptations include those carried out by specialized support staff, and those carried out by business or operational staff, or end users.</rdfs:comment>
        <rdfs:comment xml:lang="en">If the product is to be adapted by the end user, adaptability corresponds to suitability for individualization as defined in ISO 9241-110.</rdfs:comment>
        <rdfs:comment xml:lang="en">Ineffectiveness or inefficiencies for Users caused by differences or changes in their actual Contexts of Use beyond those initially specified in the Requirements can be resolved by repeating the quality improvement cycle, in which evaluation and requirements definition are iterated from the perspective of this Quality Characteristic, and problems are discovered and solved.

Also, other Quality Sub-Characteristics, typically such as Product Inclusivity and Product User Assistance, can be collaboratively applied to improve Product Adaptability and Product Flexibility.

Such differences or changes in the context of use can include, for example, the following cases:

    — when using the system initially unintended circumstances, e.g. underwater or in outer space;
    — when using the system in limited operation mode with less energy supplies or no communication network connectivity due to an accident or a disaster;
    — when initially unintended types of users are involved or influenced.</rdfs:comment>
        <rdfs:label xml:lang="en">Product Adaptability</rdfs:label>
        <skos:definition xml:lang="en">Capability of a Product to be effectively and efficiently adapted for or transferred to different hardware, software or other operational or usage environments</skos:definition>
        <cco2:ont00001754 xml:lang="en">ISO/IEC 25010:2023</cco2:ont00001754>
    </owl:Class>
    


    <!-- https://hack.cybersystems.engineer/memex/ontologies/SeamlessDigitalEngineering#Product_Analysability -->

    <owl:Class rdf:about="https://hack.cybersystems.engineer/memex/ontologies/SeamlessDigitalEngineering#Product_Analysability">
        <rdfs:subClassOf rdf:resource="https://hack.cybersystems.engineer/memex/ontologies/SeamlessDigitalEngineering#Product_Maintainability"/>
        <rdfs:comment xml:lang="en">Implementation can include providing mechanisms for the product to analyse its own faults and providing reports prior to a failure or other event.</rdfs:comment>
        <rdfs:label xml:lang="en">Product Analysability</rdfs:label>
        <skos:definition xml:lang="en">Capability of a Product to be effectively and efficiently assessed regarding the impact of an intended change to one or more of its parts, to diagnose it for deficiencies or causes of failures, or to identify parts to be modified</skos:definition>
        <cco2:ont00001754 xml:lang="en">ISO/IEC 25010:2023</cco2:ont00001754>
    </owl:Class>
    


    <!-- https://hack.cybersystems.engineer/memex/ontologies/SeamlessDigitalEngineering#Product_Appropriateness_Recognizability -->

    <owl:Class rdf:about="https://hack.cybersystems.engineer/memex/ontologies/SeamlessDigitalEngineering#Product_Appropriateness_Recognizability">
        <rdfs:subClassOf rdf:resource="https://hack.cybersystems.engineer/memex/ontologies/SeamlessDigitalEngineering#Product_Interaction_Capability"/>
        <rdfs:comment xml:lang="en">Appropriateness recognizability depends on the ability to recognize the appropriateness of the product functions from initial impressions of the product or system and/or any associated documentation.</rdfs:comment>
        <rdfs:comment xml:lang="en">The information can be provided by the product to assist users in making decisions about the adoption, acquisition, or use of products prior to the start of full-scale use, through demonstrations, tutorials, documentation or, for a website, the information on the home page.</rdfs:comment>
        <rdfs:label xml:lang="en">Product Appropriateness Recognizability</rdfs:label>
        <skos:definition xml:lang="en">Capability of a Product to be recognized by Users as appropriate for their Needs</skos:definition>
        <cco2:ont00001754 xml:lang="en">ISO/IEC 25010:2023</cco2:ont00001754>
    </owl:Class>
    


    <!-- https://hack.cybersystems.engineer/memex/ontologies/SeamlessDigitalEngineering#Product_Authenticity -->

    <owl:Class rdf:about="https://hack.cybersystems.engineer/memex/ontologies/SeamlessDigitalEngineering#Product_Authenticity">
        <rdfs:subClassOf rdf:resource="https://hack.cybersystems.engineer/memex/ontologies/SeamlessDigitalEngineering#Product_Security"/>
        <rdfs:label xml:lang="en">Product Authenticity</rdfs:label>
        <skos:definition xml:lang="en">Capability of a Product to prove that the identity of a subject or resource is the one claimed</skos:definition>
        <cco2:ont00001754 xml:lang="en">ISO/IEC 25010:2023</cco2:ont00001754>
    </owl:Class>
    


    <!-- https://hack.cybersystems.engineer/memex/ontologies/SeamlessDigitalEngineering#Product_Availability -->

    <owl:Class rdf:about="https://hack.cybersystems.engineer/memex/ontologies/SeamlessDigitalEngineering#Product_Availability">
        <rdfs:subClassOf rdf:resource="https://hack.cybersystems.engineer/memex/ontologies/SeamlessDigitalEngineering#Product_Reliability"/>
        <rdfs:comment xml:lang="en">Externally, Product Availability can be assessed by the proportion of total time during which the System, Product or Component is in an up state. Product Availability is therefore a combination of Product Faultlessness (which governs the frequency of failure), Product Fault Tolerance and Product Recoverability (which governs the length of down time following each failure).</rdfs:comment>
        <rdfs:comment xml:lang="en">Failover or duplication of systems can be applied to support Product Availability.</rdfs:comment>
        <rdfs:label xml:lang="en">Product Availability</rdfs:label>
        <skos:definition xml:lang="en">Capability of a Product to be operational and accessible when required for use</skos:definition>
        <cco2:ont00001754 xml:lang="en">ISO/IEC 25010:2023</cco2:ont00001754>
    </owl:Class>
    


    <!-- https://hack.cybersystems.engineer/memex/ontologies/SeamlessDigitalEngineering#Product_Capability -->

    <owl:Class rdf:about="https://hack.cybersystems.engineer/memex/ontologies/SeamlessDigitalEngineering#Product_Capability">
        <owl:equivalentClass>
            <owl:Class>
                <owl:intersectionOf rdf:parseType="Collection">
                    <owl:Restriction>
                        <owl:onProperty rdf:resource="http://purl.obolibrary.org/obo/BFO_0000194"/>
                        <owl:someValuesFrom rdf:resource="https://hack.cybersystems.engineer/memex/ontologies/SeamlessDigitalEngineering#Product_Quality"/>
                    </owl:Restriction>
                    <owl:Restriction>
                        <owl:onProperty rdf:resource="https://www.commoncoreontologies.org/ont00001889"/>
                        <owl:someValuesFrom rdf:resource="https://hack.cybersystems.engineer/memex/ontologies/SeamlessDigitalEngineering#Product"/>
                    </owl:Restriction>
                </owl:intersectionOf>
            </owl:Class>
        </owl:equivalentClass>
        <rdfs:subClassOf rdf:resource="https://hack.cybersystems.engineer/memex/ontologies/SeamlessDigitalEngineering#Capability"/>
        <rdfs:label xml:lang="en">Product Capability</rdfs:label>
    </owl:Class>
    


    <!-- https://hack.cybersystems.engineer/memex/ontologies/SeamlessDigitalEngineering#Product_Capacity -->

    <owl:Class rdf:about="https://hack.cybersystems.engineer/memex/ontologies/SeamlessDigitalEngineering#Product_Capacity">
        <rdfs:subClassOf rdf:resource="https://hack.cybersystems.engineer/memex/ontologies/SeamlessDigitalEngineering#Product_Performance_Efficiency"/>
        <rdfs:label xml:lang="en">Product Capacity</rdfs:label>
        <skos:definition xml:lang="en">Capability of a Product to meet Requirements for the maximum limits of a Product parameter</skos:definition>
        <cco2:ont00001754 xml:lang="en">ISO/IEC 25010:2023</cco2:ont00001754>
    </owl:Class>
    


    <!-- https://hack.cybersystems.engineer/memex/ontologies/SeamlessDigitalEngineering#Product_Co-existence -->

    <owl:Class rdf:about="https://hack.cybersystems.engineer/memex/ontologies/SeamlessDigitalEngineering#Product_Co-existence">
        <rdfs:subClassOf rdf:resource="https://hack.cybersystems.engineer/memex/ontologies/SeamlessDigitalEngineering#Product_Compatibility"/>
        <rdfs:label xml:lang="en">Product Co-existence</rdfs:label>
        <skos:definition xml:lang="en">Capability of a Product to perform its required functions efficiently while sharing a common environment and resources with other Products, without detrimental impact on any other Product</skos:definition>
        <cco2:ont00001754 xml:lang="en">ISO/IEC 25010:2023</cco2:ont00001754>
    </owl:Class>
    


    <!-- https://hack.cybersystems.engineer/memex/ontologies/SeamlessDigitalEngineering#Product_Compatibility -->

    <owl:Class rdf:about="https://hack.cybersystems.engineer/memex/ontologies/SeamlessDigitalEngineering#Product_Compatibility">
        <rdfs:subClassOf rdf:resource="https://hack.cybersystems.engineer/memex/ontologies/SeamlessDigitalEngineering#Product_Capability"/>
        <rdfs:label xml:lang="en">Product Compatibility</rdfs:label>
        <skos:definition xml:lang="en">Capability of a Product to exchange information with other Products, and/or to perform its required functions while sharing the same common environment and resources</skos:definition>
        <cco2:ont00001754 xml:lang="en">ISO/IEC 25010:2023</cco2:ont00001754>
    </owl:Class>
    


    <!-- https://hack.cybersystems.engineer/memex/ontologies/SeamlessDigitalEngineering#Product_Confidentiality -->

    <owl:Class rdf:about="https://hack.cybersystems.engineer/memex/ontologies/SeamlessDigitalEngineering#Product_Confidentiality">
        <rdfs:subClassOf rdf:resource="https://hack.cybersystems.engineer/memex/ontologies/SeamlessDigitalEngineering#Product_Security"/>
        <rdfs:label xml:lang="en">Product Confidentiality</rdfs:label>
        <skos:definition xml:lang="en">Capability of a Product to ensure that Data are accessible only to those authorized to have access</skos:definition>
        <cco2:ont00001754 xml:lang="en">ISO/IEC 25010:2023</cco2:ont00001754>
    </owl:Class>
    


    <!-- https://hack.cybersystems.engineer/memex/ontologies/SeamlessDigitalEngineering#Product_Fail_Safe -->

    <owl:Class rdf:about="https://hack.cybersystems.engineer/memex/ontologies/SeamlessDigitalEngineering#Product_Fail_Safe">
        <rdfs:subClassOf rdf:resource="https://hack.cybersystems.engineer/memex/ontologies/SeamlessDigitalEngineering#Product_Safety"/>
        <rdfs:comment xml:lang="en">The following approaches can be applied to improve the Capability of a Product for the Quality Subcharacteristic:

    — to operate in a manner that eliminates or minimizes damage caused by a failure;
    — to implement a mechanism to transfer control of a sufficient set of operations to continue safe performance when a failure occurs.</rdfs:comment>
        <rdfs:comment xml:lang="en">When the Product Fail Safe Quality Subcharacteristic is applied to a complex System or software, it is often very difficult to determine which behaviour is safer. In such a case, functional Product Safety concept can be used and then, hazard analysis and safety risk assessment can be conducted to derive safety Goals and safety Requirements to be achieved.</rdfs:comment>
        <rdfs:label xml:lang="en">Product Fail Safe</rdfs:label>
        <skos:definition xml:lang="en">Capability of a Product to automatically place itself in a safe operating mode, or to revert to a safe condition in the event of a failure</skos:definition>
        <skos:example xml:lang="en">A traffic light that reverts to blinking red in all directions when normal operation fails.</skos:example>
        <cco2:ont00001754 xml:lang="en">ISO/IEC 25010:2023</cco2:ont00001754>
    </owl:Class>
    


    <!-- https://hack.cybersystems.engineer/memex/ontologies/SeamlessDigitalEngineering#Product_Fault_Tolerance -->

    <owl:Class rdf:about="https://hack.cybersystems.engineer/memex/ontologies/SeamlessDigitalEngineering#Product_Fault_Tolerance">
        <rdfs:subClassOf rdf:resource="https://hack.cybersystems.engineer/memex/ontologies/SeamlessDigitalEngineering#Product_Reliability"/>
        <rdfs:label xml:lang="en">Product Fault Tolerance</rdfs:label>
        <skos:definition xml:lang="en">Capability of a Product to operate as intended despite the presence of hardware or software faults</skos:definition>
        <cco2:ont00001754 xml:lang="en">ISO/IEC 25010:2023</cco2:ont00001754>
    </owl:Class>
    


    <!-- https://hack.cybersystems.engineer/memex/ontologies/SeamlessDigitalEngineering#Product_Faultlessness -->

    <owl:Class rdf:about="https://hack.cybersystems.engineer/memex/ontologies/SeamlessDigitalEngineering#Product_Faultlessness">
        <rdfs:subClassOf rdf:resource="https://hack.cybersystems.engineer/memex/ontologies/SeamlessDigitalEngineering#Product_Reliability"/>
        <rdfs:comment xml:lang="en">The concept of Product Faultlessness can also be applied to other Quality Characteristics to indicate the degree to which they meet required Needs under normal operation.</rdfs:comment>
        <rdfs:label xml:lang="en">Product Faultlessness</rdfs:label>
        <skos:definition xml:lang="en">Capability of a Product to perform specified functions without Fault under normal Operation</skos:definition>
        <cco2:ont00001754 xml:lang="en">ISO/IEC 25010:2023</cco2:ont00001754>
    </owl:Class>
    


    <!-- https://hack.cybersystems.engineer/memex/ontologies/SeamlessDigitalEngineering#Product_Flexibility -->

    <owl:Class rdf:about="https://hack.cybersystems.engineer/memex/ontologies/SeamlessDigitalEngineering#Product_Flexibility">
        <rdfs:subClassOf rdf:resource="https://hack.cybersystems.engineer/memex/ontologies/SeamlessDigitalEngineering#Product_Capability"/>
        <rdfs:comment xml:lang="en">Flexibility to Context of Use should consider two distinguished aspects, i.e. technical and non-technical. The technical aspect is related with the execution environment of products, such as software, hardware and communication facility; and the non-technical aspect is related with the social environment, such as user and task, and the physical environment, such as climate and nature.</rdfs:comment>
        <rdfs:label xml:lang="en">Product Flexibility</rdfs:label>
        <skos:definition xml:lang="en">Capability of a Product to be adapted to changes in its Requirements, Contexts of Use, or System Environment</skos:definition>
        <cco2:ont00001754 xml:lang="en">ISO/IEC 25010:2023</cco2:ont00001754>
    </owl:Class>
    


    <!-- https://hack.cybersystems.engineer/memex/ontologies/SeamlessDigitalEngineering#Product_Functional_Appropriateness -->

    <owl:Class rdf:about="https://hack.cybersystems.engineer/memex/ontologies/SeamlessDigitalEngineering#Product_Functional_Appropriateness">
        <rdfs:subClassOf rdf:resource="https://hack.cybersystems.engineer/memex/ontologies/SeamlessDigitalEngineering#Product_Functional_Suitability"/>
        <rdfs:label xml:lang="en">Product Functional Appropriateness</rdfs:label>
        <skos:definition xml:lang="en">Capability of a Product to provide functions that facilitate the accomplishment of specified Tasks and Objectives</skos:definition>
        <cco2:ont00001754 xml:lang="en">ISO/IEC 25010:2023</cco2:ont00001754>
    </owl:Class>
    


    <!-- https://hack.cybersystems.engineer/memex/ontologies/SeamlessDigitalEngineering#Product_Functional_Completeness -->

    <owl:Class rdf:about="https://hack.cybersystems.engineer/memex/ontologies/SeamlessDigitalEngineering#Product_Functional_Completeness">
        <rdfs:subClassOf rdf:resource="https://hack.cybersystems.engineer/memex/ontologies/SeamlessDigitalEngineering#Product_Functional_Suitability"/>
        <rdfs:label xml:lang="en">Product Functional Completeness</rdfs:label>
        <skos:definition xml:lang="en">Capability of a Product to provide a set of functions that covers all the specified Tasks and intended Users’ Objectives</skos:definition>
        <cco2:ont00001754 xml:lang="en">ISO/IEC 25010:2023</cco2:ont00001754>
    </owl:Class>
    


    <!-- https://hack.cybersystems.engineer/memex/ontologies/SeamlessDigitalEngineering#Product_Functional_Correctness -->

    <owl:Class rdf:about="https://hack.cybersystems.engineer/memex/ontologies/SeamlessDigitalEngineering#Product_Functional_Correctness">
        <rdfs:subClassOf rdf:resource="https://hack.cybersystems.engineer/memex/ontologies/SeamlessDigitalEngineering#Product_Functional_Suitability"/>
        <rdfs:comment xml:lang="en">In case of the products requiring high precision such as scientific software, the product can provide precise results with the needed degree as well as accurate results.</rdfs:comment>
        <rdfs:comment xml:lang="en">Precision is one of the attributes of correctness.</rdfs:comment>
        <rdfs:label xml:lang="en">Product Functional Correctness</rdfs:label>
        <skos:definition xml:lang="en">Capability of a Product to provide accurate results when used by intended Users</skos:definition>
        <cco2:ont00001754 xml:lang="en">ISO/IEC 25010:2023</cco2:ont00001754>
    </owl:Class>
    


    <!-- https://hack.cybersystems.engineer/memex/ontologies/SeamlessDigitalEngineering#Product_Functional_Suitability -->

    <owl:Class rdf:about="https://hack.cybersystems.engineer/memex/ontologies/SeamlessDigitalEngineering#Product_Functional_Suitability">
        <rdfs:subClassOf rdf:resource="https://hack.cybersystems.engineer/memex/ontologies/SeamlessDigitalEngineering#Product_Capability"/>
        <rdfs:comment xml:lang="en">Functional Suitability is concerned with whether the functions meet not only stated and implied Needs, but also the Functional Specification</rdfs:comment>
        <rdfs:label xml:lang="en">Product Functional Suitability</rdfs:label>
        <skos:definition xml:lang="en">Capability of a Product to provide functions that meet stated and implied Needs of intended Users when it is used under specified conditions</skos:definition>
        <cco2:ont00001754 xml:lang="en">ISO/IEC 25010:2023</cco2:ont00001754>
    </owl:Class>
    


    <!-- https://hack.cybersystems.engineer/memex/ontologies/SeamlessDigitalEngineering#Product_Hazard_Warning -->

    <owl:Class rdf:about="https://hack.cybersystems.engineer/memex/ontologies/SeamlessDigitalEngineering#Product_Hazard_Warning">
        <rdfs:subClassOf rdf:resource="https://hack.cybersystems.engineer/memex/ontologies/SeamlessDigitalEngineering#Product_Safety"/>
        <rdfs:label xml:lang="en">Product Hazard Warning</rdfs:label>
        <skos:definition xml:lang="en">Capability of a Product to provide warnings of unacceptable Risks to operations or internal controls so that they can react in sufficient time to sustain safe operations</skos:definition>
        <skos:example xml:lang="en">A pedestrian traffic light gives a warning sign, such as showing the remaining seconds, before reverting from green to yellow or red.</skos:example>
        <cco2:ont00001754 xml:lang="en">ISO/IEC 25010:2023</cco2:ont00001754>
    </owl:Class>
    


    <!-- https://hack.cybersystems.engineer/memex/ontologies/SeamlessDigitalEngineering#Product_Inclusivity -->

    <owl:Class rdf:about="https://hack.cybersystems.engineer/memex/ontologies/SeamlessDigitalEngineering#Product_Inclusivity">
        <rdfs:subClassOf rdf:resource="https://hack.cybersystems.engineer/memex/ontologies/SeamlessDigitalEngineering#Product_Interaction_Capability"/>
        <rdfs:comment xml:lang="en">Backgrounds include (and are not limited to) people of various ages, abilities, cultures, ethnicities, languages, genders, economic situations, education, geographical locations and life situations.</rdfs:comment>
        <rdfs:label xml:lang="en">Product Inclusivity</rdfs:label>
        <skos:definition xml:lang="en">Capability of a Product to be utilised by people of various backgrounds</skos:definition>
        <cco2:ont00001754 xml:lang="en">ISO/IEC 25010:2023</cco2:ont00001754>
    </owl:Class>
    


    <!-- https://hack.cybersystems.engineer/memex/ontologies/SeamlessDigitalEngineering#Product_Information_Model -->

    <owl:Class rdf:about="https://hack.cybersystems.engineer/memex/ontologies/SeamlessDigitalEngineering#Product_Information_Model">
        <owl:equivalentClass>
            <owl:Class>
                <owl:intersectionOf rdf:parseType="Collection">
                    <rdf:Description rdf:about="https://hack.cybersystems.engineer/memex/ontologies/SeamlessDigitalEngineering#Information_Model"/>
                    <owl:Restriction>
                        <owl:onProperty rdf:resource="https://www.commoncoreontologies.org/ont00001808"/>
                        <owl:someValuesFrom rdf:resource="https://hack.cybersystems.engineer/memex/ontologies/SeamlessDigitalEngineering#Product"/>
                    </owl:Restriction>
                </owl:intersectionOf>
            </owl:Class>
        </owl:equivalentClass>
        <rdfs:subClassOf rdf:resource="https://hack.cybersystems.engineer/memex/ontologies/SeamlessDigitalEngineering#Information_Model"/>
        <rdfs:label xml:lang="en">Product Information Model</rdfs:label>
        <skos:definition xml:lang="en">ISO 10303-2:2024 Industrial automation systems and integration - Product data representation and exchange - Part 2: Vocabulary, 3.1.238</skos:definition>
        <skos:definition xml:lang="en">formal model of Product Information</skos:definition>
    </owl:Class>
    


    <!-- https://hack.cybersystems.engineer/memex/ontologies/SeamlessDigitalEngineering#Product_Installability -->

    <owl:Class rdf:about="https://hack.cybersystems.engineer/memex/ontologies/SeamlessDigitalEngineering#Product_Installability">
        <rdfs:subClassOf rdf:resource="https://hack.cybersystems.engineer/memex/ontologies/SeamlessDigitalEngineering#Product_Flexibility"/>
        <rdfs:comment xml:lang="en">If the Product is to be installed by an end User, Product Installability can affect the resulting Product Functional Appropriateness and Product Operability.</rdfs:comment>
        <rdfs:label xml:lang="en">Product Installability</rdfs:label>
        <skos:definition xml:lang="en">Capability of a Product to be effectively and efficiently installed successfully and/or uninstalled in a specified environment</skos:definition>
        <cco2:ont00001754 xml:lang="en">ISO/IEC 25010:2023</cco2:ont00001754>
    </owl:Class>
    


    <!-- https://hack.cybersystems.engineer/memex/ontologies/SeamlessDigitalEngineering#Product_Integrity -->

    <owl:Class rdf:about="https://hack.cybersystems.engineer/memex/ontologies/SeamlessDigitalEngineering#Product_Integrity">
        <rdfs:subClassOf rdf:resource="https://hack.cybersystems.engineer/memex/ontologies/SeamlessDigitalEngineering#Product_Security"/>
        <rdfs:label xml:lang="en">Product Integrity</rdfs:label>
        <skos:definition xml:lang="en">Capability of a Product to ensure that the state of its System and Data are protected from unauthorized modification or deletion either by malicious action or Computer Error</skos:definition>
        <cco2:ont00001754 xml:lang="en">ISO/IEC 25010:2023</cco2:ont00001754>
    </owl:Class>
    


    <!-- https://hack.cybersystems.engineer/memex/ontologies/SeamlessDigitalEngineering#Product_Interaction_Capability -->

    <owl:Class rdf:about="https://hack.cybersystems.engineer/memex/ontologies/SeamlessDigitalEngineering#Product_Interaction_Capability">
        <rdfs:subClassOf rdf:resource="https://hack.cybersystems.engineer/memex/ontologies/SeamlessDigitalEngineering#Product_Capability"/>
        <rdfs:comment xml:lang="en">Interaction capability in the product quality model and its subcharacteristics focus on a set of attributes that enable interaction by users (or operators) to complete specific tasks in a variety of contexts of use. On the other hand, usability as defined in the quality-in-use model (ISO/IEC 25019) comprehensively focuses on outcomes of use to determine whether tasks are achieved by users with effectiveness, efficiency and satisfaction in a specific context of use.</rdfs:comment>
        <rdfs:comment xml:lang="en">Interaction capability is a prerequisite for usability.</rdfs:comment>
        <rdfs:comment xml:lang="en">Interaction itself is defined in ISO TR 25060 as “exchange of information between a user and an interactive system via the user interface”.</rdfs:comment>
        <rdfs:label xml:lang="en">Product Interaction Capability</rdfs:label>
        <skos:definition xml:lang="en">Capability of a Product to be interacted with by specified Users to exchange information between a User and a System via the user interface to complete the intended Task</skos:definition>
        <cco2:ont00001754 xml:lang="en">ISO/IEC 25010:2023</cco2:ont00001754>
    </owl:Class>
    


    <!-- https://hack.cybersystems.engineer/memex/ontologies/SeamlessDigitalEngineering#Product_Interoperability -->

    <owl:Class rdf:about="https://hack.cybersystems.engineer/memex/ontologies/SeamlessDigitalEngineering#Product_Interoperability">
        <rdfs:subClassOf rdf:resource="https://hack.cybersystems.engineer/memex/ontologies/SeamlessDigitalEngineering#Product_Compatibility"/>
        <rdfs:comment xml:lang="en">Information is meaningful data; and information exchange includes transformation of data for exchange.</rdfs:comment>
        <rdfs:label xml:lang="en">Product Interoperability</rdfs:label>
        <skos:definition xml:lang="en">Capability of a Product to exchange information with other Products and mutually use the information that has been exchanged</skos:definition>
        <cco2:ont00001754 xml:lang="en">ISO/IEC 25010:2023</cco2:ont00001754>
    </owl:Class>
    


    <!-- https://hack.cybersystems.engineer/memex/ontologies/SeamlessDigitalEngineering#Product_Learnability -->

    <owl:Class rdf:about="https://hack.cybersystems.engineer/memex/ontologies/SeamlessDigitalEngineering#Product_Learnability">
        <rdfs:subClassOf rdf:resource="https://hack.cybersystems.engineer/memex/ontologies/SeamlessDigitalEngineering#Product_Interaction_Capability"/>
        <rdfs:label xml:lang="en">Product Learnability</rdfs:label>
        <skos:definition xml:lang="en">Capability of a Product to have specified Users learn to use specified Product functions within a specified amount of time</skos:definition>
        <cco2:ont00001754 xml:lang="en">ISO/IEC 25010:2023</cco2:ont00001754>
    </owl:Class>
    


    <!-- https://hack.cybersystems.engineer/memex/ontologies/SeamlessDigitalEngineering#Product_Maintainability -->

    <owl:Class rdf:about="https://hack.cybersystems.engineer/memex/ontologies/SeamlessDigitalEngineering#Product_Maintainability">
        <rdfs:subClassOf rdf:resource="https://hack.cybersystems.engineer/memex/ontologies/SeamlessDigitalEngineering#Product_Capability"/>
        <rdfs:comment xml:lang="en">Maintainability can be interpreted as either an inherent Capability of the Product to facilitate maintenance activities, or the Quality-in-Use experienced by the Maintainers for the Goal of maintaining the Product.</rdfs:comment>
        <rdfs:comment xml:lang="en">Maintainability includes installation of updates and upgrades.</rdfs:comment>
        <rdfs:comment xml:lang="en">Modifications can include corrections, improvements or adaptation of the product to changes in environment, and in requirements and functional specifications. Modifications include those carried out by specialized support staff, and those carried out by business or operational staff, or end users.</rdfs:comment>
        <rdfs:label xml:lang="en">Product Maintainability</rdfs:label>
        <skos:definition xml:lang="en">Capability of a Product to be modified by the intended Maintainers with effectiveness and efficiency</skos:definition>
        <cco2:ont00001754 xml:lang="en">ISO/IEC 25010:2023</cco2:ont00001754>
    </owl:Class>
    


    <!-- https://hack.cybersystems.engineer/memex/ontologies/SeamlessDigitalEngineering#Product_Modifiability -->

    <owl:Class rdf:about="https://hack.cybersystems.engineer/memex/ontologies/SeamlessDigitalEngineering#Product_Modifiability">
        <rdfs:subClassOf rdf:resource="https://hack.cybersystems.engineer/memex/ontologies/SeamlessDigitalEngineering#Product_Maintainability"/>
        <rdfs:comment xml:lang="en">Implementation includes coding, designing, documenting and verifying changes.</rdfs:comment>
        <rdfs:comment xml:lang="en">Modifiability is a combination of changeability and stability.</rdfs:comment>
        <rdfs:comment xml:lang="en">Product Modularity and Product Analysability can influence Product Modifiability.</rdfs:comment>
        <rdfs:label xml:lang="en">Product Modifiability</rdfs:label>
        <skos:definition xml:lang="en">Capability of a Product to be effectively and efficiently modified without introducing defects or degrading existing Product Quality</skos:definition>
        <cco2:ont00001754 xml:lang="en">ISO/IEC 25010:2023</cco2:ont00001754>
    </owl:Class>
    


    <!-- https://hack.cybersystems.engineer/memex/ontologies/SeamlessDigitalEngineering#Product_Modularity -->

    <owl:Class rdf:about="https://hack.cybersystems.engineer/memex/ontologies/SeamlessDigitalEngineering#Product_Modularity">
        <rdfs:subClassOf rdf:resource="https://hack.cybersystems.engineer/memex/ontologies/SeamlessDigitalEngineering#Product_Maintainability"/>
        <rdfs:comment xml:lang="en">Modularity implies that the product is composed of discrete modules or components with cohesive content and minimal coupling to other modules or components.</rdfs:comment>
        <rdfs:label xml:lang="en">Product Modularity</rdfs:label>
        <skos:definition xml:lang="en">Capability of a Product to limit changes to one component from affecting other components</skos:definition>
        <cco2:ont00001754 xml:lang="en">ISO/IEC 25010:2023</cco2:ont00001754>
    </owl:Class>
    


    <!-- https://hack.cybersystems.engineer/memex/ontologies/SeamlessDigitalEngineering#Product_Need_Assessment -->

    <owl:Class rdf:about="https://hack.cybersystems.engineer/memex/ontologies/SeamlessDigitalEngineering#Product_Need_Assessment">
        <rdfs:subClassOf rdf:resource="https://www.commoncoreontologies.org/ont00000624"/>
    </owl:Class>
    


    <!-- https://hack.cybersystems.engineer/memex/ontologies/SeamlessDigitalEngineering#Product_Non-Repudiation -->

    <owl:Class rdf:about="https://hack.cybersystems.engineer/memex/ontologies/SeamlessDigitalEngineering#Product_Non-Repudiation">
        <rdfs:subClassOf rdf:resource="https://hack.cybersystems.engineer/memex/ontologies/SeamlessDigitalEngineering#Product_Security"/>
        <rdfs:label xml:lang="en">Product Non-Repudiation</rdfs:label>
        <skos:definition xml:lang="en">Capability of a Product to prove that actions or events have taken place, so that the events or actions cannot be repudiated later</skos:definition>
        <cco2:ont00001754 xml:lang="en">ISO/IEC 25010:2023</cco2:ont00001754>
    </owl:Class>
    


    <!-- https://hack.cybersystems.engineer/memex/ontologies/SeamlessDigitalEngineering#Product_Operability -->

    <owl:Class rdf:about="https://hack.cybersystems.engineer/memex/ontologies/SeamlessDigitalEngineering#Product_Operability">
        <rdfs:subClassOf rdf:resource="https://hack.cybersystems.engineer/memex/ontologies/SeamlessDigitalEngineering#Product_Interaction_Capability"/>
        <rdfs:comment xml:lang="en">Operability is related to controllability, user error robustness and conformity with user expectations as defined in ISO 9241-110. It is also related to the effectiveness and efficiency of physical interface devices (e.g. mouse, touch pen).</rdfs:comment>
        <rdfs:label xml:lang="en">Product Operability</rdfs:label>
        <skos:definition xml:lang="en">Capability of a Product to have functions and attributes that make it easy to operate and control</skos:definition>
        <cco2:ont00001754 xml:lang="en">ISO/IEC 25010:2023</cco2:ont00001754>
    </owl:Class>
    


    <!-- https://hack.cybersystems.engineer/memex/ontologies/SeamlessDigitalEngineering#Product_Operational_Constraint -->

    <owl:Class rdf:about="https://hack.cybersystems.engineer/memex/ontologies/SeamlessDigitalEngineering#Product_Operational_Constraint">
        <rdfs:subClassOf rdf:resource="https://hack.cybersystems.engineer/memex/ontologies/SeamlessDigitalEngineering#Product_Safety"/>
        <rdfs:comment xml:lang="en">Operational hazard is a hazardous situation, a circumstance in which people, property or the environment are exposed to an unacceptable Risk during operation.</rdfs:comment>
        <rdfs:label xml:lang="en">Product Operational Constraint</rdfs:label>
        <skos:definition xml:lang="en">Capability of a Product to constrain its operation to within safe parameters or states when encountering operational hazard</skos:definition>
        <skos:example xml:lang="en">A constraint that limits the amount of radiation released by a radiology device to a safe threshold regardless of the operator input.</skos:example>
        <skos:example xml:lang="en">A constraint that prevents an airplane from entering a stall condition caused by environmental conditions or pilot error.</skos:example>
        <cco2:ont00001754 xml:lang="en">ISO/IEC 25010:2023</cco2:ont00001754>
    </owl:Class>
    


    <!-- https://hack.cybersystems.engineer/memex/ontologies/SeamlessDigitalEngineering#Product_Performance_Efficiency -->

    <owl:Class rdf:about="https://hack.cybersystems.engineer/memex/ontologies/SeamlessDigitalEngineering#Product_Performance_Efficiency">
        <rdfs:subClassOf rdf:resource="https://hack.cybersystems.engineer/memex/ontologies/SeamlessDigitalEngineering#Product_Capability"/>
        <rdfs:comment xml:lang="en">Resources can be CPU, memory, storage, and network devices.</rdfs:comment>
        <rdfs:comment xml:lang="en">Resources can include other software products, the software and hardware configuration of the system, energy, and materials (e.g. print paper, storage media).</rdfs:comment>
        <rdfs:label xml:lang="en">Product Performance Efficiency</rdfs:label>
        <skos:definition xml:lang="en">Capability of a Product to perform its functions within specified time and throughput parameters and be efficient in the use of resources under specified conditions</skos:definition>
        <cco2:ont00001754 xml:lang="en">ISO/IEC 25010:2023</cco2:ont00001754>
    </owl:Class>
    


    <!-- https://hack.cybersystems.engineer/memex/ontologies/SeamlessDigitalEngineering#Product_Quality -->

    <owl:Class rdf:about="https://hack.cybersystems.engineer/memex/ontologies/SeamlessDigitalEngineering#Product_Quality">
        <owl:equivalentClass>
            <owl:Class>
                <owl:intersectionOf rdf:parseType="Collection">
                    <rdf:Description rdf:about="https://hack.cybersystems.engineer/memex/ontologies/SeamlessDigitalEngineering#Quality"/>
                    <owl:Restriction>
                        <owl:onProperty rdf:resource="http://purl.obolibrary.org/obo/BFO_0000195"/>
                        <owl:someValuesFrom rdf:resource="https://hack.cybersystems.engineer/memex/ontologies/SeamlessDigitalEngineering#Product_Capability"/>
                    </owl:Restriction>
                    <owl:Restriction>
                        <owl:onProperty rdf:resource="https://www.commoncoreontologies.org/ont00001947"/>
                        <owl:someValuesFrom rdf:resource="https://hack.cybersystems.engineer/memex/ontologies/SeamlessDigitalEngineering#Product"/>
                    </owl:Restriction>
                </owl:intersectionOf>
            </owl:Class>
        </owl:equivalentClass>
        <rdfs:subClassOf rdf:resource="https://hack.cybersystems.engineer/memex/ontologies/SeamlessDigitalEngineering#Quality"/>
        <rdfs:label xml:lang="en">Product Quality</rdfs:label>
        <skos:definition xml:lang="en">capability of a System or its System Elements (components) to satisfy stated and implied Quality Needs when used under specific conditions</skos:definition>
        <cco2:ont00001754 xml:lang="en">ISO/IEC 25002:2024 Systems and software engineering - Systems and software Quality Requirements and Evaluation (SQuaRE) - Quality model overview and usage</cco2:ont00001754>
    </owl:Class>
    


    <!-- https://hack.cybersystems.engineer/memex/ontologies/SeamlessDigitalEngineering#Product_Quality-in-Use -->

    <owl:Class rdf:about="https://hack.cybersystems.engineer/memex/ontologies/SeamlessDigitalEngineering#Product_Quality-in-Use">
        <owl:equivalentClass>
            <owl:Class>
                <owl:intersectionOf rdf:parseType="Collection">
                    <owl:Restriction>
                        <owl:onProperty rdf:resource="http://purl.obolibrary.org/obo/BFO_0000054"/>
                        <owl:someValuesFrom rdf:resource="https://hack.cybersystems.engineer/memex/ontologies/SeamlessDigitalEngineering#Operation_Process"/>
                    </owl:Restriction>
                    <owl:Restriction>
                        <owl:onProperty rdf:resource="http://purl.obolibrary.org/obo/BFO_0000197"/>
                        <owl:someValuesFrom>
                            <owl:Class>
                                <owl:intersectionOf rdf:parseType="Collection">
                                    <rdf:Description rdf:about="https://hack.cybersystems.engineer/memex/ontologies/SeamlessDigitalEngineering#Context_of_Use"/>
                                    <rdf:Description rdf:about="https://hack.cybersystems.engineer/memex/ontologies/SeamlessDigitalEngineering#System"/>
                                </owl:intersectionOf>
                            </owl:Class>
                        </owl:someValuesFrom>
                    </owl:Restriction>
                </owl:intersectionOf>
            </owl:Class>
        </owl:equivalentClass>
        <rdfs:subClassOf rdf:resource="http://purl.obolibrary.org/obo/BFO_0000017"/>
        <rdfs:label xml:lang="en">Product Quality-in-Use</rdfs:label>
        <skos:definition xml:lang="en">extent to which the System or Product, when it is used in a specified Context of Use satisfies or exceeds Stakeholders&apos; Needs to achieve specified beneficial Goals or Outcomes</skos:definition>
        <cco2:ont00001754 xml:lang="en">ISO/IEC 25002:2024 Systems and software engineering - Systems and software Quality Requirements and Evaluation (SQuaRE) - Quality model overview and usage</cco2:ont00001754>
    </owl:Class>
    


    <!-- https://hack.cybersystems.engineer/memex/ontologies/SeamlessDigitalEngineering#Product_Quality_Model -->

    <owl:Class rdf:about="https://hack.cybersystems.engineer/memex/ontologies/SeamlessDigitalEngineering#Product_Quality_Model">
        <owl:equivalentClass>
            <owl:Class>
                <owl:intersectionOf rdf:parseType="Collection">
                    <rdf:Description rdf:about="https://hack.cybersystems.engineer/memex/ontologies/SeamlessDigitalEngineering#Quality_Model"/>
                    <owl:Restriction>
                        <owl:onProperty rdf:resource="https://www.commoncoreontologies.org/ont00001942"/>
                        <owl:someValuesFrom rdf:resource="https://hack.cybersystems.engineer/memex/ontologies/SeamlessDigitalEngineering#Product_Quality"/>
                    </owl:Restriction>
                </owl:intersectionOf>
            </owl:Class>
        </owl:equivalentClass>
        <rdfs:subClassOf rdf:resource="https://hack.cybersystems.engineer/memex/ontologies/SeamlessDigitalEngineering#Quality_Model"/>
        <rdfs:label xml:lang="en">Product Quality Model</rdfs:label>
    </owl:Class>
    


    <!-- https://hack.cybersystems.engineer/memex/ontologies/SeamlessDigitalEngineering#Product_Recoverability -->

    <owl:Class rdf:about="https://hack.cybersystems.engineer/memex/ontologies/SeamlessDigitalEngineering#Product_Recoverability">
        <rdfs:subClassOf rdf:resource="https://hack.cybersystems.engineer/memex/ontologies/SeamlessDigitalEngineering#Product_Reliability"/>
        <rdfs:comment xml:lang="en">The length of the unavailable period following a failure, during which a product is not available at the same level of use as before the failure, is determined by its recoverability. However, the recoverability of a product depends on the recoverability of the computer system on which the product operates or a subset of its functions.</rdfs:comment>
        <rdfs:label xml:lang="en">Product Recoverability</rdfs:label>
        <skos:definition xml:lang="en">Capability of a Product in the event of an interruption or a failure to recover the Data directly affected and re-establish the desired state of the System</skos:definition>
        <cco2:ont00001754 xml:lang="en">ISO/IEC 25010:2023</cco2:ont00001754>
    </owl:Class>
    


    <!-- https://hack.cybersystems.engineer/memex/ontologies/SeamlessDigitalEngineering#Product_Reliability -->

    <owl:Class rdf:about="https://hack.cybersystems.engineer/memex/ontologies/SeamlessDigitalEngineering#Product_Reliability">
        <rdfs:subClassOf rdf:resource="https://hack.cybersystems.engineer/memex/ontologies/SeamlessDigitalEngineering#Product_Capability"/>
        <rdfs:comment xml:lang="en">Dependability is often used as a synonym for Product Reliability. However, dependability has a larger scope in that it includes Product Security, Product Performance Efficiency, and continuing support and others in addition to the Quality Sub-Characteristics of Product Reliability as discussed in Annex B.</rdfs:comment>
        <rdfs:comment xml:lang="en">Wear does not occur in software. Limitations in reliability are due to results from faults in requirements, design and implementation, or from contextual changes.</rdfs:comment>
        <rdfs:label xml:lang="en">Product Reliability</rdfs:label>
        <skos:definition xml:lang="en">Capability of a Product to perform specified functions under specified conditions for a specified period of time without interruptions and failures</skos:definition>
        <cco2:ont00001754 xml:lang="en">ISO/IEC 25010:2023</cco2:ont00001754>
    </owl:Class>
    


    <!-- https://hack.cybersystems.engineer/memex/ontologies/SeamlessDigitalEngineering#Product_Replaceability -->

    <owl:Class rdf:about="https://hack.cybersystems.engineer/memex/ontologies/SeamlessDigitalEngineering#Product_Replaceability">
        <rdfs:subClassOf rdf:resource="https://hack.cybersystems.engineer/memex/ontologies/SeamlessDigitalEngineering#Product_Flexibility"/>
        <rdfs:comment xml:lang="en">Product Replaceability can include Attributes of both Product Installability and Product Adaptability. The concept has been introduced as a Sub-Characteristic of its own because of its importance.</rdfs:comment>
        <rdfs:comment xml:lang="en">Replaceability reduces lock-in risks, so that other Software Products can be used in place of the present one, for example by the use of standardized file formats.</rdfs:comment>
        <rdfs:comment xml:lang="en">The Product Replaceability of a new version of a Software Product is important to the User when upgrading.</rdfs:comment>
        <rdfs:label xml:lang="en">Product Replaceability</rdfs:label>
        <skos:definition xml:lang="en">Capability of a Product to replace another specified Product for the same Purpose in the same Environment</skos:definition>
        <cco2:ont00001754 xml:lang="en">ISO/IEC 25010:2023</cco2:ont00001754>
    </owl:Class>
    


    <!-- https://hack.cybersystems.engineer/memex/ontologies/SeamlessDigitalEngineering#Product_Resistance -->

    <owl:Class rdf:about="https://hack.cybersystems.engineer/memex/ontologies/SeamlessDigitalEngineering#Product_Resistance">
        <rdfs:subClassOf rdf:resource="https://hack.cybersystems.engineer/memex/ontologies/SeamlessDigitalEngineering#Product_Security"/>
        <rdfs:comment xml:lang="en">A malicious attack can include a denial of service attack, a ransomware attack, or other malicious actions. Then, the following approaches can be applied to improve the Capability of a Product for the Quality Sub-Characteristic:

    — to continuously protect itself from well-known attacks by removing potential flaws or weaknesses of the Product with the use of Product Security tools such as a security weakness diagnostic tool, vulnerability scanner and static analysis tool;
    — to minimize vulnerability of a Product with secure software coding and/or by incorporating security enhancement functions or mechanisms;
    — to maintain Product updates during its life time for security reasons.</rdfs:comment>
        <rdfs:label xml:lang="en">Product Resistance</rdfs:label>
        <skos:definition xml:lang="en">Capability of a Product to sustain operations while under attack from a malicious actor</skos:definition>
        <cco2:ont00001754 xml:lang="en">ISO/IEC 25010:2023</cco2:ont00001754>
    </owl:Class>
    


    <!-- https://hack.cybersystems.engineer/memex/ontologies/SeamlessDigitalEngineering#Product_Resource_Utilization -->

    <owl:Class rdf:about="https://hack.cybersystems.engineer/memex/ontologies/SeamlessDigitalEngineering#Product_Resource_Utilization">
        <rdfs:subClassOf rdf:resource="https://hack.cybersystems.engineer/memex/ontologies/SeamlessDigitalEngineering#Product_Performance_Efficiency"/>
        <rdfs:label xml:lang="en">Product Resource Utilization</rdfs:label>
        <skos:definition xml:lang="en">Capability of a Product to use no more than the specified amount of resources to perform its function under specified conditions</skos:definition>
        <cco2:ont00001754 xml:lang="en">ISO/IEC 25010:2023</cco2:ont00001754>
    </owl:Class>
    


    <!-- https://hack.cybersystems.engineer/memex/ontologies/SeamlessDigitalEngineering#Product_Reusability -->

    <owl:Class rdf:about="https://hack.cybersystems.engineer/memex/ontologies/SeamlessDigitalEngineering#Product_Reusability">
        <rdfs:subClassOf rdf:resource="https://hack.cybersystems.engineer/memex/ontologies/SeamlessDigitalEngineering#Product_Maintainability"/>
        <rdfs:label xml:lang="en">Product Reusability</rdfs:label>
        <skos:definition xml:lang="en">Capability of a Product to be used as assets in more than one System, or in building other assets</skos:definition>
        <cco2:ont00001754 xml:lang="en">ISO/IEC 25010:2023</cco2:ont00001754>
    </owl:Class>
    


    <!-- https://hack.cybersystems.engineer/memex/ontologies/SeamlessDigitalEngineering#Product_Risk_Identification -->

    <owl:Class rdf:about="https://hack.cybersystems.engineer/memex/ontologies/SeamlessDigitalEngineering#Product_Risk_Identification">
        <rdfs:subClassOf rdf:resource="https://hack.cybersystems.engineer/memex/ontologies/SeamlessDigitalEngineering#Product_Safety"/>
        <rdfs:label xml:lang="en">Product Risk Identification</rdfs:label>
        <skos:definition xml:lang="en">Capability of a Product to identify a course of events or operations that can expose life, property or environment to unacceptable Risk</skos:definition>
        <cco2:ont00001754 xml:lang="en">ISO/IEC 25010:2023</cco2:ont00001754>
    </owl:Class>
    


    <!-- https://hack.cybersystems.engineer/memex/ontologies/SeamlessDigitalEngineering#Product_Safe_Integration -->

    <owl:Class rdf:about="https://hack.cybersystems.engineer/memex/ontologies/SeamlessDigitalEngineering#Product_Safe_Integration">
        <rdfs:subClassOf rdf:resource="https://hack.cybersystems.engineer/memex/ontologies/SeamlessDigitalEngineering#Product_Safety"/>
        <rdfs:label xml:lang="en">Product Safe Integration</rdfs:label>
        <skos:definition xml:lang="en">Capability of a Product to maintain Product Safety during and after integration with one or more components</skos:definition>
        <cco2:ont00001754 xml:lang="en">ISO/IEC 25010:2023</cco2:ont00001754>
    </owl:Class>
    


    <!-- https://hack.cybersystems.engineer/memex/ontologies/SeamlessDigitalEngineering#Product_Safety -->

    <owl:Class rdf:about="https://hack.cybersystems.engineer/memex/ontologies/SeamlessDigitalEngineering#Product_Safety">
        <rdfs:subClassOf rdf:resource="https://hack.cybersystems.engineer/memex/ontologies/SeamlessDigitalEngineering#Product_Capability"/>
        <rdfs:comment xml:lang="en">In [ISO/IEC 25010], safety is defined to describe capability of product to be able to avoid exposures which is not tolerable. Then, the definition is different from the other standards relating to safety that define safety as freedom from unacceptable risks.</rdfs:comment>
        <rdfs:label xml:lang="en">Product Safety</rdfs:label>
        <skos:definition xml:lang="en">Capability of a Product under defined conditions to avoid a state in which human life, health, property, or the environment is endangered</skos:definition>
        <cco2:ont00001754 xml:lang="en">ISO/IEC 25010:2023</cco2:ont00001754>
    </owl:Class>
    


    <!-- https://hack.cybersystems.engineer/memex/ontologies/SeamlessDigitalEngineering#Product_Scalability -->

    <owl:Class rdf:about="https://hack.cybersystems.engineer/memex/ontologies/SeamlessDigitalEngineering#Product_Scalability">
        <rdfs:subClassOf rdf:resource="https://hack.cybersystems.engineer/memex/ontologies/SeamlessDigitalEngineering#Product_Flexibility"/>
        <rdfs:label xml:lang="en">Product Scalability</rdfs:label>
        <skos:definition xml:lang="en">Capability of a Product to handle growing or shrinking workloads or to adapt its Product Capacity to handle variability</skos:definition>
        <cco2:ont00001754 xml:lang="en">ISO/IEC 25010:2023</cco2:ont00001754>
    </owl:Class>
    


    <!-- https://hack.cybersystems.engineer/memex/ontologies/SeamlessDigitalEngineering#Product_Security -->

    <owl:Class rdf:about="https://hack.cybersystems.engineer/memex/ontologies/SeamlessDigitalEngineering#Product_Security">
        <rdfs:subClassOf rdf:resource="https://hack.cybersystems.engineer/memex/ontologies/SeamlessDigitalEngineering#Product_Capability"/>
        <rdfs:subClassOf>
            <owl:Restriction>
                <owl:onProperty rdf:resource="http://purl.obolibrary.org/obo/BFO_0000054"/>
                <owl:someValuesFrom rdf:resource="http://www.ontologyrepository.com/CommonCoreOntologies/CybersecurityAct"/>
            </owl:Restriction>
        </rdfs:subClassOf>
        <rdfs:subClassOf>
            <owl:Restriction>
                <owl:onProperty rdf:resource="http://purl.obolibrary.org/obo/BFO_0000054"/>
                <owl:someValuesFrom>
                    <owl:Class>
                        <owl:unionOf rdf:parseType="Collection">
                            <rdf:Description rdf:about="https://www.commoncoreontologies.org/ont00000622"/>
                            <rdf:Description rdf:about="https://www.commoncoreontologies.org/ont00000847"/>
                        </owl:unionOf>
                    </owl:Class>
                </owl:someValuesFrom>
            </owl:Restriction>
        </rdfs:subClassOf>
        <rdfs:comment xml:lang="en">As well as Data stored in or by a Product or System, Product Security also applies to Data in transmission.</rdfs:comment>
        <rdfs:label xml:lang="en">Product Security</rdfs:label>
        <skos:definition xml:lang="en">Capability of a Product to protect Information and Data so that Persons or other Products have the degree of Data access appropriate to their types and levels of authorization, and to defend against attack patterns by malicious actors</skos:definition>
        <cco2:ont00001754 xml:lang="en">ISO/IEC 25010:2023</cco2:ont00001754>
    </owl:Class>
    


    <!-- https://hack.cybersystems.engineer/memex/ontologies/SeamlessDigitalEngineering#Product_Self-Descriptiveness -->

    <owl:Class rdf:about="https://hack.cybersystems.engineer/memex/ontologies/SeamlessDigitalEngineering#Product_Self-Descriptiveness">
        <rdfs:subClassOf rdf:resource="https://hack.cybersystems.engineer/memex/ontologies/SeamlessDigitalEngineering#Product_Interaction_Capability"/>
        <rdfs:comment xml:lang="en">Other resources include user documentation, help desks, other users and other sources of assistance.</rdfs:comment>
        <rdfs:label xml:lang="en">Product Self-Descriptiveness</rdfs:label>
        <skos:definition xml:lang="en">Capability of a Product to present appropriate information, where needed by the User, to make its Capabilities and use immediately obvious to the User without excessive interactions with a Product or other resources</skos:definition>
        <skos:example xml:lang="en">Instructions for user operation are divided and displayed or talked through step-by-step interactively at the helpful timing of operation, in order to help users understand easily what is going on with the system/software and to prevent users from becoming confused by receiving too many instructions at once.</skos:example>
        <cco2:ont00001754 xml:lang="en">ISO/IEC 25010:2023</cco2:ont00001754>
    </owl:Class>
    


    <!-- https://hack.cybersystems.engineer/memex/ontologies/SeamlessDigitalEngineering#Product_Testability -->

    <owl:Class rdf:about="https://hack.cybersystems.engineer/memex/ontologies/SeamlessDigitalEngineering#Product_Testability">
        <rdfs:subClassOf rdf:resource="https://hack.cybersystems.engineer/memex/ontologies/SeamlessDigitalEngineering#Product_Maintainability"/>
        <rdfs:label xml:lang="en">Product Testability</rdfs:label>
        <skos:definition xml:lang="en">Capability of a Product to enable an objective and feasible test to be designed and performed to determine whether a Requirement is met</skos:definition>
        <cco2:ont00001754 xml:lang="en">ISO/IEC 25010:2023</cco2:ont00001754>
    </owl:Class>
    


    <!-- https://hack.cybersystems.engineer/memex/ontologies/SeamlessDigitalEngineering#Product_Time_Behavior -->

    <owl:Class rdf:about="https://hack.cybersystems.engineer/memex/ontologies/SeamlessDigitalEngineering#Product_Time_Behavior">
        <rdfs:subClassOf rdf:resource="https://hack.cybersystems.engineer/memex/ontologies/SeamlessDigitalEngineering#Product_Performance_Efficiency"/>
        <rdfs:label xml:lang="en">Product Time Behavior</rdfs:label>
        <skos:definition xml:lang="en">Capability of a Product to perform its specified function under specified conditions so that the response time and throughput rates meet the Requirements</skos:definition>
        <cco2:ont00001754 xml:lang="en">ISO/IEC 25010:2023</cco2:ont00001754>
    </owl:Class>
    


    <!-- https://hack.cybersystems.engineer/memex/ontologies/SeamlessDigitalEngineering#Product_User_Assistance -->

    <owl:Class rdf:about="https://hack.cybersystems.engineer/memex/ontologies/SeamlessDigitalEngineering#Product_User_Assistance">
        <rdfs:subClassOf rdf:resource="https://hack.cybersystems.engineer/memex/ontologies/SeamlessDigitalEngineering#Product_Interaction_Capability"/>
        <rdfs:comment xml:lang="en">A set of specific rules and methods for software accessibility can be applied to ensure “user assistance” in this document and in ISO/IEC 25019.</rdfs:comment>
        <rdfs:comment xml:lang="en">Inconveniences or less effectiveness for users caused by differences or changes in their actual contexts of use beyond those initially specified in the requirements can be resolved by repeating the quality improvement cycle to find and resolve problems through iterative evaluation and requirements definition from this quality characteristic perspective.
Such differences or changes in the context of use can include, for example, the following cases:

    — when using the system while driving a car or flying in an airplane;
    — when using the system interactively for emergency within short-time use and small screen view due to an accident or a disaster;
    — when a user is a beginner or is changing own task goal of use, usage, or skill and knowledge;
    — when a user having different physical capabilities due to the type of injury or illness, or changes in time due to healing or progression.

Also, other Quality (Sub-)Characteristics, typically such as Product Adaptability or Product Flexibility, can be collaboratively applied to improve Product User Assistance and Product Interaction Capability).</rdfs:comment>
        <rdfs:comment xml:lang="en">The range of capabilities includes language differences and disabilities associated with age, sight, hearing, use of hands, arms and legs, etc.</rdfs:comment>
        <rdfs:label xml:lang="en">Product User Assistance</rdfs:label>
        <skos:definition xml:lang="en">Capability of a Product to be used by people with the widest range of characteristics and Capabilities to achieve specified Goals in a specified Context of Use</skos:definition>
        <skos:example xml:lang="en">A system that can interact with users using multiple input/output methods, such as voice, gaze, and touch, in addition to visual display, in order to accommodate differences in vision, hearing, and body parts that can be moved, or changes in these areas.</skos:example>
        <cco2:ont00001754 xml:lang="en">ISO/IEC 25010:2023</cco2:ont00001754>
    </owl:Class>
    


    <!-- https://hack.cybersystems.engineer/memex/ontologies/SeamlessDigitalEngineering#Product_User_Engagement -->

    <owl:Class rdf:about="https://hack.cybersystems.engineer/memex/ontologies/SeamlessDigitalEngineering#Product_User_Engagement">
        <rdfs:subClassOf rdf:resource="https://hack.cybersystems.engineer/memex/ontologies/SeamlessDigitalEngineering#Product_Interaction_Capability"/>
        <rdfs:comment xml:lang="en">This refers to properties of the product that increase the pleasure and satisfaction of the user, such as harmonious colour, intuitive user interface and friendly voice guidance.</rdfs:comment>
        <rdfs:label xml:lang="en">Product User Engagement</rdfs:label>
        <skos:definition xml:lang="en">Capability of a Product to present functions and information in an inviting and motivating manner encouraging continued interaction</skos:definition>
        <cco2:ont00001754 xml:lang="en">ISO/IEC 25010:2023</cco2:ont00001754>
    </owl:Class>
    


    <!-- https://hack.cybersystems.engineer/memex/ontologies/SeamlessDigitalEngineering#Product_User_Error_Protection -->

    <owl:Class rdf:about="https://hack.cybersystems.engineer/memex/ontologies/SeamlessDigitalEngineering#Product_User_Error_Protection">
        <rdfs:subClassOf rdf:resource="https://hack.cybersystems.engineer/memex/ontologies/SeamlessDigitalEngineering#Product_Interaction_Capability"/>
        <rdfs:label xml:lang="en">Product User Error Protection</rdfs:label>
        <skos:definition xml:lang="en">Capability of a Product to prevent operation errors</skos:definition>
        <cco2:ont00001754 xml:lang="en">ISO/IEC 25010:2023</cco2:ont00001754>
    </owl:Class>
    


    <!-- https://hack.cybersystems.engineer/memex/ontologies/SeamlessDigitalEngineering#Product_Verifiability -->

    <owl:Class rdf:about="https://hack.cybersystems.engineer/memex/ontologies/SeamlessDigitalEngineering#Product_Verifiability">
        <owl:equivalentClass>
            <owl:Class>
                <owl:intersectionOf rdf:parseType="Collection">
                    <rdf:Description rdf:about="https://hack.cybersystems.engineer/memex/ontologies/SeamlessDigitalEngineering#Product_Testability"/>
                    <owl:Restriction>
                        <owl:onProperty rdf:resource="http://purl.obolibrary.org/obo/BFO_0000054"/>
                        <owl:someValuesFrom rdf:resource="https://hack.cybersystems.engineer/memex/ontologies/SeamlessDigitalEngineering#Verification_Process"/>
                    </owl:Restriction>
                </owl:intersectionOf>
            </owl:Class>
        </owl:equivalentClass>
        <rdfs:subClassOf rdf:resource="https://hack.cybersystems.engineer/memex/ontologies/SeamlessDigitalEngineering#Product_Testability"/>
        <rdfs:label xml:lang="en">Product Verifiability</rdfs:label>
        <skos:altLabel xml:lang="en">Verifiability</skos:altLabel>
        <skos:altLabel xml:lang="en">Verifiable</skos:altLabel>
        <skos:definition xml:lang="en">Capability to be checked for Correctness by a Person or Tool</skos:definition>
        <cco2:ont00001754 xml:lang="en">ISO/IEC/IEEE 15289:2019, 3.1.29</cco2:ont00001754>
    </owl:Class>
    


    <!-- https://hack.cybersystems.engineer/memex/ontologies/SeamlessDigitalEngineering#Production_Stage -->

    <owl:Class rdf:about="https://hack.cybersystems.engineer/memex/ontologies/SeamlessDigitalEngineering#Production_Stage">
        <rdfs:subClassOf rdf:resource="https://hack.cybersystems.engineer/memex/ontologies/SeamlessDigitalEngineering#Lifecycle_Stage"/>
        <rdfs:comment xml:lang="en">Purpose: The production stage is executed to produce or manufacture the SoI, test it and produce related enabling systems as needed.</rdfs:comment>
        <rdfs:label xml:lang="en">Production Stage</rdfs:label>
        <cco2:ont00001754>ISO/IEC/IEEE 24748-1:2024</cco2:ont00001754>
    </owl:Class>
    


    <!-- https://hack.cybersystems.engineer/memex/ontologies/SeamlessDigitalEngineering#Program -->

    <owl:Class rdf:about="https://hack.cybersystems.engineer/memex/ontologies/SeamlessDigitalEngineering#Program">
        <owl:equivalentClass>
            <owl:Restriction>
                <owl:onProperty rdf:resource="https://www.commoncoreontologies.org/ont00001777"/>
                <owl:someValuesFrom rdf:resource="https://hack.cybersystems.engineer/memex/ontologies/SeamlessDigitalEngineering#Project"/>
            </owl:Restriction>
        </owl:equivalentClass>
        <rdfs:subClassOf rdf:resource="https://www.commoncoreontologies.org/ont00000228"/>
        <rdfs:label xml:lang="en">Program</rdfs:label>
        <skos:definition xml:lang="en">a group of related Projects, subprograms and program Activities managed in a coordinated way to obtain benefits not available from managing them individually</skos:definition>
        <cco2:ont00001754 xml:lang="en">A Guide to the Project Management Body of Knowledge (PMBOK® Guide) — Fifth Edition</cco2:ont00001754>
    </owl:Class>
    


    <!-- https://hack.cybersystems.engineer/memex/ontologies/SeamlessDigitalEngineering#Progress_Report -->

    <owl:Class rdf:about="https://hack.cybersystems.engineer/memex/ontologies/SeamlessDigitalEngineering#Progress_Report">
        <rdfs:subClassOf rdf:resource="https://www.commoncoreontologies.org/ont00000624"/>
    </owl:Class>
    


    <!-- https://hack.cybersystems.engineer/memex/ontologies/SeamlessDigitalEngineering#Project -->

    <owl:Class rdf:about="https://hack.cybersystems.engineer/memex/ontologies/SeamlessDigitalEngineering#Project">
        <owl:equivalentClass>
            <owl:Class>
                <owl:intersectionOf rdf:parseType="Collection">
                    <owl:Restriction>
                        <owl:onProperty rdf:resource="http://purl.obolibrary.org/obo/BFO_0000066"/>
                        <owl:someValuesFrom rdf:resource="https://www.commoncoreontologies.org/ont00001180"/>
                    </owl:Restriction>
                    <owl:Restriction>
                        <owl:onProperty rdf:resource="https://www.commoncoreontologies.org/ont00001777"/>
                        <owl:someValuesFrom rdf:resource="https://hack.cybersystems.engineer/memex/ontologies/SeamlessDigitalEngineering#Activity"/>
                    </owl:Restriction>
                    <owl:Restriction>
                        <owl:onProperty rdf:resource="https://www.commoncoreontologies.org/ont00001857"/>
                        <owl:someValuesFrom rdf:resource="https://hack.cybersystems.engineer/memex/ontologies/SeamlessDigitalEngineering#Lifecycle"/>
                    </owl:Restriction>
                    <owl:Restriction>
                        <owl:onProperty rdf:resource="https://www.commoncoreontologies.org/ont00001986"/>
                        <owl:someValuesFrom>
                            <owl:Class>
                                <owl:unionOf rdf:parseType="Collection">
                                    <rdf:Description rdf:about="https://hack.cybersystems.engineer/memex/ontologies/SeamlessDigitalEngineering#Product"/>
                                    <rdf:Description rdf:about="https://hack.cybersystems.engineer/memex/ontologies/SeamlessDigitalEngineering#Service"/>
                                </owl:unionOf>
                            </owl:Class>
                        </owl:someValuesFrom>
                    </owl:Restriction>
                </owl:intersectionOf>
            </owl:Class>
        </owl:equivalentClass>
        <rdfs:subClassOf rdf:resource="https://www.commoncoreontologies.org/ont00000228"/>
        <skos:definition xml:lang="en">endeavour with defined start and finish criteria undertaken to create a Product or Service in accordance with specified Resources and Requirements</skos:definition>
        <cco2:ont00001754>ISO/IEC/IEEE 15288:2023</cco2:ont00001754>
    </owl:Class>
    


    <!-- https://hack.cybersystems.engineer/memex/ontologies/SeamlessDigitalEngineering#Project_Assessment_and_Control_Process -->

    <owl:Class rdf:about="https://hack.cybersystems.engineer/memex/ontologies/SeamlessDigitalEngineering#Project_Assessment_and_Control_Process">
        <rdfs:subClassOf rdf:resource="https://hack.cybersystems.engineer/memex/ontologies/SeamlessDigitalEngineering#Technical_Management_Process"/>
        <rdfs:label xml:lang="en">Project Assessment and Control Process</rdfs:label>
        <skos:definition xml:lang="en">The purpose of the project assessment and control process is to assess if the plans are aligned and feasible; determine the status of the project, technical and process performance; and direct execution to help ensure that the performance is according to plans and schedules, within projected budgets, to satisfy project objectives.</skos:definition>
        <cco2:ont00001754>ISO/IEC/IEEE 15288:2023</cco2:ont00001754>
    </owl:Class>
    


    <!-- https://hack.cybersystems.engineer/memex/ontologies/SeamlessDigitalEngineering#Project_Manager -->

    <owl:Class rdf:about="https://hack.cybersystems.engineer/memex/ontologies/SeamlessDigitalEngineering#Project_Manager">
        <rdfs:subClassOf rdf:resource="https://hack.cybersystems.engineer/memex/ontologies/SeamlessDigitalEngineering#Project_Team_Member"/>
        <rdfs:label xml:lang="en">Project Manager</rdfs:label>
    </owl:Class>
    


    <!-- https://hack.cybersystems.engineer/memex/ontologies/SeamlessDigitalEngineering#Project_Plan -->

    <owl:Class rdf:about="https://hack.cybersystems.engineer/memex/ontologies/SeamlessDigitalEngineering#Project_Plan">
        <owl:equivalentClass>
            <owl:Restriction>
                <owl:onProperty rdf:resource="https://www.commoncoreontologies.org/ont00001942"/>
                <owl:someValuesFrom rdf:resource="https://hack.cybersystems.engineer/memex/ontologies/SeamlessDigitalEngineering#Project"/>
            </owl:Restriction>
        </owl:equivalentClass>
        <rdfs:subClassOf rdf:resource="https://www.commoncoreontologies.org/ont00000974"/>
        <rdfs:label xml:lang="en">Project Plan</rdfs:label>
    </owl:Class>
    


    <!-- https://hack.cybersystems.engineer/memex/ontologies/SeamlessDigitalEngineering#Project_Planning_Process -->

    <owl:Class rdf:about="https://hack.cybersystems.engineer/memex/ontologies/SeamlessDigitalEngineering#Project_Planning_Process">
        <rdfs:subClassOf rdf:resource="https://hack.cybersystems.engineer/memex/ontologies/SeamlessDigitalEngineering#Technical_Management_Process"/>
        <rdfs:label xml:lang="en">Project Planning Process</rdfs:label>
        <skos:definition xml:lang="en">The purpose of the project planning process is to produce and coordinate effective and workable plans.</skos:definition>
        <cco2:ont00001754>ISO/IEC/IEEE 15288:2023</cco2:ont00001754>
    </owl:Class>
    


    <!-- https://hack.cybersystems.engineer/memex/ontologies/SeamlessDigitalEngineering#Project_Team -->

    <owl:Class rdf:about="https://hack.cybersystems.engineer/memex/ontologies/SeamlessDigitalEngineering#Project_Team">
        <owl:equivalentClass>
            <owl:Class>
                <owl:intersectionOf rdf:parseType="Collection">
                    <owl:Restriction>
                        <owl:onProperty rdf:resource="http://purl.obolibrary.org/obo/BFO_0000178"/>
                        <owl:someValuesFrom rdf:resource="https://hack.cybersystems.engineer/memex/ontologies/SeamlessDigitalEngineering#Project_Team_Member"/>
                    </owl:Restriction>
                    <owl:Restriction>
                        <owl:onProperty rdf:resource="https://www.commoncoreontologies.org/ont00001787"/>
                        <owl:someValuesFrom rdf:resource="https://hack.cybersystems.engineer/memex/ontologies/SeamlessDigitalEngineering#Project"/>
                    </owl:Restriction>
                </owl:intersectionOf>
            </owl:Class>
        </owl:equivalentClass>
        <rdfs:subClassOf rdf:resource="https://www.commoncoreontologies.org/ont00000914"/>
        <rdfs:label xml:lang="en">Project Team</rdfs:label>
    </owl:Class>
    


    <!-- https://hack.cybersystems.engineer/memex/ontologies/SeamlessDigitalEngineering#Project_Team_Member -->

    <owl:Class rdf:about="https://hack.cybersystems.engineer/memex/ontologies/SeamlessDigitalEngineering#Project_Team_Member">
        <owl:equivalentClass>
            <owl:Class>
                <owl:intersectionOf rdf:parseType="Collection">
                    <rdf:Description rdf:about="https://www.commoncoreontologies.org/ont00000647"/>
                    <owl:Restriction>
                        <owl:onProperty rdf:resource="https://www.commoncoreontologies.org/ont00001787"/>
                        <owl:someValuesFrom rdf:resource="https://hack.cybersystems.engineer/memex/ontologies/SeamlessDigitalEngineering#Project"/>
                    </owl:Restriction>
                </owl:intersectionOf>
            </owl:Class>
        </owl:equivalentClass>
        <rdfs:subClassOf rdf:resource="https://hack.cybersystems.engineer/memex/ontologies/SeamlessDigitalEngineering#Stakeholder"/>
        <rdfs:label xml:lang="en">Project Team Member</rdfs:label>
    </owl:Class>
    


    <!-- https://hack.cybersystems.engineer/memex/ontologies/SeamlessDigitalEngineering#Proof -->

    <owl:Class rdf:about="https://hack.cybersystems.engineer/memex/ontologies/SeamlessDigitalEngineering#Proof">
        <rdfs:subClassOf rdf:resource="http://www.ontologyrepository.com/CommonCoreOntologies/ComputerProgram"/>
        <rdfs:label xml:lang="en">Proof</rdfs:label>
    </owl:Class>
    


    <!-- https://hack.cybersystems.engineer/memex/ontologies/SeamlessDigitalEngineering#Proof_Assistant -->

    <owl:Class rdf:about="https://hack.cybersystems.engineer/memex/ontologies/SeamlessDigitalEngineering#Proof_Assistant">
        <rdfs:subClassOf rdf:resource="https://hack.cybersystems.engineer/memex/ontologies/SeamlessDigitalEngineering#Theorem_Prover"/>
        <rdfs:label xml:lang="en">Proof Assistant</rdfs:label>
        <skos:altLabel xml:lang="en">Interactive Theorem Prover</skos:altLabel>
    </owl:Class>
    


    <!-- https://hack.cybersystems.engineer/memex/ontologies/SeamlessDigitalEngineering#Proof_Certificate -->

    <owl:Class rdf:about="https://hack.cybersystems.engineer/memex/ontologies/SeamlessDigitalEngineering#Proof_Certificate">
        <owl:equivalentClass>
            <owl:Class>
                <owl:intersectionOf rdf:parseType="Collection">
                    <rdf:Description rdf:about="https://www.commoncoreontologies.org/ont00000189"/>
                    <owl:Restriction>
                        <owl:onProperty rdf:resource="https://www.commoncoreontologies.org/ont00001816"/>
                        <owl:someValuesFrom rdf:resource="https://hack.cybersystems.engineer/memex/ontologies/SeamlessDigitalEngineering#Act_of_Computer-Assisted_Theorem_Proving"/>
                    </owl:Restriction>
                </owl:intersectionOf>
            </owl:Class>
        </owl:equivalentClass>
        <rdfs:subClassOf rdf:resource="https://www.commoncoreontologies.org/ont00000189"/>
        <rdfs:label xml:lang="en">Proof Certificate</rdfs:label>
        <skos:definition xml:lang="en">a textual representation of a formal mathematical proof, emitted by the solver for external consumption</skos:definition>
        <cco2:ont00001754 rdf:datatype="http://www.w3.org/2001/XMLSchema#anyURI">https://dx.doi.org/10.1145/3587692</cco2:ont00001754>
    </owl:Class>
    


    <!-- https://hack.cybersystems.engineer/memex/ontologies/SeamlessDigitalEngineering#Proof_Theory_Discipline -->

    <owl:Class rdf:about="https://hack.cybersystems.engineer/memex/ontologies/SeamlessDigitalEngineering#Proof_Theory_Discipline">
        <rdfs:subClassOf rdf:resource="https://hack.cybersystems.engineer/memex/ontologies/SeamlessDigitalEngineering#Mathematical_Logic_Discipline"/>
        <rdfs:label xml:lang="en">Proof Theory Discipline</rdfs:label>
    </owl:Class>
    


    <!-- https://hack.cybersystems.engineer/memex/ontologies/SeamlessDigitalEngineering#Property-of-Interest -->

    <owl:Class rdf:about="https://hack.cybersystems.engineer/memex/ontologies/SeamlessDigitalEngineering#Property-of-Interest">
        <rdfs:subClassOf rdf:resource="http://purl.obolibrary.org/obo/BFO_0000002"/>
        <rdfs:comment xml:lang="en">Assets in the security context, e.g., defined in ISO/IEC 15408-1, can be a Property-of-Interest.</rdfs:comment>
        <rdfs:comment xml:lang="en">In the safety context, human lives and health can be Property-of-Interests.</rdfs:comment>
        <rdfs:comment xml:lang="en">The concept of Property-of-Interest is introduced in order to characterize negative effects of Consequences.</rdfs:comment>
        <rdfs:label xml:lang="en">Property-of-Interest</rdfs:label>
        <skos:definition xml:lang="en">continuant whose loss is considered as a negative effect</skos:definition>
        <cco2:ont00001754 xml:lang="en">derived from ISO/IEC/IEEE 15026-1:2019</cco2:ont00001754>
    </owl:Class>
    


    <!-- https://hack.cybersystems.engineer/memex/ontologies/SeamlessDigitalEngineering#Public_Digital_Infrastructure -->

    <owl:Class rdf:about="https://hack.cybersystems.engineer/memex/ontologies/SeamlessDigitalEngineering#Public_Digital_Infrastructure">
        <owl:equivalentClass>
            <owl:Class>
                <owl:intersectionOf rdf:parseType="Collection">
                    <rdf:Description rdf:about="https://hack.cybersystems.engineer/memex/ontologies/SeamlessDigitalEngineering#Digital_Infrastructure"/>
                    <rdf:Description rdf:about="https://hack.cybersystems.engineer/memex/ontologies/SeamlessDigitalEngineering#Public_Infrastructure"/>
                </owl:intersectionOf>
            </owl:Class>
        </owl:equivalentClass>
        <rdfs:subClassOf rdf:resource="https://hack.cybersystems.engineer/memex/ontologies/SeamlessDigitalEngineering#Digital_Infrastructure"/>
        <rdfs:label xml:lang="en">Public Digital Infrastructure</rdfs:label>
        <skos:altLabel xml:lang="en">internet</skos:altLabel>
        <skos:definition xml:lang="en">global System-of-Systems of inter-connected Digital Networks in the Public Domain</skos:definition>
        <cco2:ont00001754 xml:lang="en">ISO 5127:2017 - Information and documentation - Foundation and vocabulary</cco2:ont00001754>
    </owl:Class>
    


    <!-- https://hack.cybersystems.engineer/memex/ontologies/SeamlessDigitalEngineering#Public_Domain -->

    <owl:Class rdf:about="https://hack.cybersystems.engineer/memex/ontologies/SeamlessDigitalEngineering#Public_Domain">
        <rdfs:subClassOf rdf:resource="http://purl.obolibrary.org/obo/BFO_0000027"/>
        <rdfs:label xml:lang="en">Public Domain</rdfs:label>
        <skos:definition xml:lang="en">totality of intellectual works which may be freely utilized as long as there is no infringement of Moral Rights</skos:definition>
        <cco2:ont00001754 xml:lang="en">ISO 5127:2017 - Information and documentation - Foundation and vocabulary</cco2:ont00001754>
    </owl:Class>
    


    <!-- https://hack.cybersystems.engineer/memex/ontologies/SeamlessDigitalEngineering#Public_Domain_Work -->

    <owl:Class rdf:about="https://hack.cybersystems.engineer/memex/ontologies/SeamlessDigitalEngineering#Public_Domain_Work">
        <rdfs:subClassOf rdf:resource="https://www.commoncoreontologies.org/ont00000253"/>
        <rdfs:label xml:lang="en">Public Domain Work</rdfs:label>
        <skos:definition xml:lang="en">intellectual work which may be freely utilized as long as there is no infringement of Moral Rights</skos:definition>
        <cco2:ont00001754 xml:lang="en">ISO 5127:2017 - Information and documentation - Foundation and vocabulary</cco2:ont00001754>
    </owl:Class>
    


    <!-- https://hack.cybersystems.engineer/memex/ontologies/SeamlessDigitalEngineering#Public_Infrastructure -->

    <owl:Class rdf:about="https://hack.cybersystems.engineer/memex/ontologies/SeamlessDigitalEngineering#Public_Infrastructure">
        <rdfs:subClassOf rdf:resource="https://www.commoncoreontologies.org/ont00000870"/>
        <rdfs:subClassOf>
            <owl:Class>
                <owl:intersectionOf rdf:parseType="Collection">
                    <owl:Restriction>
                        <owl:onProperty rdf:resource="https://www.commoncoreontologies.org/ont00001852"/>
                        <owl:someValuesFrom rdf:resource="https://www.commoncoreontologies.org/ont00000005"/>
                    </owl:Restriction>
                    <owl:Restriction>
                        <owl:onProperty rdf:resource="https://www.commoncoreontologies.org/ont00001925"/>
                        <owl:someValuesFrom rdf:resource="https://www.commoncoreontologies.org/ont00000141"/>
                    </owl:Restriction>
                </owl:intersectionOf>
            </owl:Class>
        </rdfs:subClassOf>
        <rdfs:label xml:lang="en">Public Infrastructure</rdfs:label>
        <skos:definition xml:lang="en">Infrastructure System that is owned or available for use by the Populace (represented by some Government Organizations)</skos:definition>
        <cco2:ont00001754 xml:lang="en">https://en.wikipedia.org/wiki/Infrastructure#Public</cco2:ont00001754>
    </owl:Class>
    


    <!-- https://hack.cybersystems.engineer/memex/ontologies/SeamlessDigitalEngineering#Pure_Functional_Programming_Language -->

    <owl:Class rdf:about="https://hack.cybersystems.engineer/memex/ontologies/SeamlessDigitalEngineering#Pure_Functional_Programming_Language">
        <rdfs:subClassOf rdf:resource="https://hack.cybersystems.engineer/memex/ontologies/SeamlessDigitalEngineering#Functional_Programming_Language"/>
        <rdfs:label xml:lang="en">Pure Functional Programming Language</rdfs:label>
    </owl:Class>
    


    <!-- https://hack.cybersystems.engineer/memex/ontologies/SeamlessDigitalEngineering#Purpose -->

    <owl:Class rdf:about="https://hack.cybersystems.engineer/memex/ontologies/SeamlessDigitalEngineering#Purpose">
        <rdfs:subClassOf rdf:resource="https://hack.cybersystems.engineer/memex/ontologies/SeamlessDigitalEngineering#Need"/>
        <skos:definition xml:lang="en">What the system is for, and why the different stakeholders are willing to participate in the system lifecycle.</skos:definition>
        <cco2:ont00001754 rdf:datatype="http://www.w3.org/2001/XMLSchema#anyURI">https://sebokwiki.org/wiki/Purpose_(glossary)</cco2:ont00001754>
    </owl:Class>
    


    <!-- https://hack.cybersystems.engineer/memex/ontologies/SeamlessDigitalEngineering#Qualification_Process -->

    <owl:Class rdf:about="https://hack.cybersystems.engineer/memex/ontologies/SeamlessDigitalEngineering#Qualification_Process">
        <rdfs:subClassOf rdf:resource="https://hack.cybersystems.engineer/memex/ontologies/SeamlessDigitalEngineering#Validation_Process"/>
        <rdfs:label xml:lang="en">Qualification Process</rdfs:label>
        <skos:definition xml:lang="en">process of demonstrating whether an entity is capable of fulfilling specified Requirements</skos:definition>
        <cco2:ont00001754 xml:lang="en">ISO/IEC TS 24748-1:2024 Systems and software engineering — Life cycle management — Part 1: Guide for life cycle management</cco2:ont00001754>
    </owl:Class>
    


    <!-- https://hack.cybersystems.engineer/memex/ontologies/SeamlessDigitalEngineering#Quality -->

    <owl:Class rdf:about="https://hack.cybersystems.engineer/memex/ontologies/SeamlessDigitalEngineering#Quality">
        <owl:equivalentClass>
            <owl:Class>
                <owl:intersectionOf rdf:parseType="Collection">
                    <rdf:Description rdf:about="http://purl.obolibrary.org/obo/BFO_0000019"/>
                    <owl:Restriction>
                        <owl:onProperty rdf:resource="https://www.commoncoreontologies.org/ont00001947"/>
                        <owl:someValuesFrom rdf:resource="https://hack.cybersystems.engineer/memex/ontologies/SeamlessDigitalEngineering#System"/>
                    </owl:Restriction>
                </owl:intersectionOf>
            </owl:Class>
        </owl:equivalentClass>
        <rdfs:subClassOf rdf:resource="http://purl.obolibrary.org/obo/BFO_0000019"/>
        <rdfs:label xml:lang="en">Quality</rdfs:label>
        <skos:definition xml:lang="en">degree to which the System satisfies the stated and implied Needs of its various Stakeholders, and thus provides Gain of Value</skos:definition>
        <cco2:ont00001754 xml:lang="en">ISO/IEC/IEEE 24765:2017 (ISO/IEC 25010:2011)</cco2:ont00001754>
    </owl:Class>
    


    <!-- https://hack.cybersystems.engineer/memex/ontologies/SeamlessDigitalEngineering#Quality-in-Use_Model -->

    <owl:Class rdf:about="https://hack.cybersystems.engineer/memex/ontologies/SeamlessDigitalEngineering#Quality-in-Use_Model">
        <rdfs:subClassOf rdf:resource="https://hack.cybersystems.engineer/memex/ontologies/SeamlessDigitalEngineering#Quality_Model"/>
        <rdfs:label xml:lang="en">Quality-in-Use Model</rdfs:label>
    </owl:Class>
    


    <!-- https://hack.cybersystems.engineer/memex/ontologies/SeamlessDigitalEngineering#Quality_Assurance -->

    <owl:Class rdf:about="https://hack.cybersystems.engineer/memex/ontologies/SeamlessDigitalEngineering#Quality_Assurance">
        <owl:equivalentClass>
            <owl:Class>
                <owl:intersectionOf rdf:parseType="Collection">
                    <rdf:Description rdf:about="https://hack.cybersystems.engineer/memex/ontologies/SeamlessDigitalEngineering#Assurance"/>
                    <owl:Restriction>
                        <owl:onProperty rdf:resource="https://www.commoncoreontologies.org/ont00001801"/>
                        <owl:someValuesFrom rdf:resource="https://hack.cybersystems.engineer/memex/ontologies/SeamlessDigitalEngineering#Quality_Requirement"/>
                    </owl:Restriction>
                </owl:intersectionOf>
            </owl:Class>
        </owl:equivalentClass>
        <rdfs:subClassOf rdf:resource="https://hack.cybersystems.engineer/memex/ontologies/SeamlessDigitalEngineering#Assurance"/>
        <rdfs:label xml:lang="en">Quality Assurance</rdfs:label>
    </owl:Class>
    


    <!-- https://hack.cybersystems.engineer/memex/ontologies/SeamlessDigitalEngineering#Quality_Assurance_Process -->

    <owl:Class rdf:about="https://hack.cybersystems.engineer/memex/ontologies/SeamlessDigitalEngineering#Quality_Assurance_Process">
        <rdfs:subClassOf rdf:resource="https://hack.cybersystems.engineer/memex/ontologies/SeamlessDigitalEngineering#Technical_Management_Process"/>
        <rdfs:label xml:lang="en">Quality Assurance Process</rdfs:label>
        <skos:definition xml:lang="en">The purpose of the quality assurance process is to help ensure the effective application of the organization’s quality management process to the project.</skos:definition>
        <cco2:ont00001754>ISO/IEC/IEEE 15288:2023</cco2:ont00001754>
    </owl:Class>
    


    <!-- https://hack.cybersystems.engineer/memex/ontologies/SeamlessDigitalEngineering#Quality_Characteristic -->

    <owl:Class rdf:about="https://hack.cybersystems.engineer/memex/ontologies/SeamlessDigitalEngineering#Quality_Characteristic">
        <owl:equivalentClass>
            <owl:Class>
                <owl:intersectionOf rdf:parseType="Collection">
                    <owl:Restriction>
                        <owl:onProperty rdf:resource="http://purl.obolibrary.org/obo/BFO_0000176"/>
                        <owl:someValuesFrom rdf:resource="https://hack.cybersystems.engineer/memex/ontologies/SeamlessDigitalEngineering#Quality_Model"/>
                    </owl:Restriction>
                    <owl:Restriction>
                        <owl:onProperty rdf:resource="https://www.commoncoreontologies.org/ont00001982"/>
                        <owl:someValuesFrom rdf:resource="https://hack.cybersystems.engineer/memex/ontologies/SeamlessDigitalEngineering#Quality_Property"/>
                    </owl:Restriction>
                </owl:intersectionOf>
            </owl:Class>
        </owl:equivalentClass>
        <rdfs:subClassOf rdf:resource="https://www.commoncoreontologies.org/ont00000853"/>
        <rdfs:comment xml:lang="en">Quality Characteristics can be further divided into Quality Sub-characteristics . While [Quality] Characteristics typically represent one aspect of quality that is of interest to Stakeholders, Quality Sub-characteristics can help subdivide Quality Characteristics into individual aspects that help mapping them to Quality Properties.</rdfs:comment>
        <rdfs:label xml:lang="en">Quality Characteristic</rdfs:label>
        <skos:definition xml:lang="en">category of Quality Attributes that bears on the Quality of the [Product or System]</skos:definition>
        <cco2:ont00001754 xml:lang="en">ISO/IEC 25002:2024 Systems and software engineering - Systems and software Quality Requirements and Evaluation (SQuaRE) - Quality model overview and usage</cco2:ont00001754>
    </owl:Class>
    


    <!-- https://hack.cybersystems.engineer/memex/ontologies/SeamlessDigitalEngineering#Quality_Claim -->

    <owl:Class rdf:about="https://hack.cybersystems.engineer/memex/ontologies/SeamlessDigitalEngineering#Quality_Claim">
        <owl:equivalentClass>
            <owl:Class>
                <owl:intersectionOf rdf:parseType="Collection">
                    <rdf:Description rdf:about="https://hack.cybersystems.engineer/memex/ontologies/SeamlessDigitalEngineering#Claim"/>
                    <owl:Restriction>
                        <owl:onProperty rdf:resource="https://www.commoncoreontologies.org/ont00001942"/>
                        <owl:someValuesFrom rdf:resource="https://hack.cybersystems.engineer/memex/ontologies/SeamlessDigitalEngineering#Quality_Property"/>
                    </owl:Restriction>
                </owl:intersectionOf>
            </owl:Class>
        </owl:equivalentClass>
        <rdfs:subClassOf rdf:resource="https://hack.cybersystems.engineer/memex/ontologies/SeamlessDigitalEngineering#Claim"/>
        <rdfs:label xml:lang="en">Quality Claim</rdfs:label>
        <skos:definition xml:lang="en">A Claim that prescribes some verifiable Quality Property</skos:definition>
    </owl:Class>
    


    <!-- https://hack.cybersystems.engineer/memex/ontologies/SeamlessDigitalEngineering#Quality_Engineering_Discipline -->

    <owl:Class rdf:about="https://hack.cybersystems.engineer/memex/ontologies/SeamlessDigitalEngineering#Quality_Engineering_Discipline">
        <owl:equivalentClass>
            <owl:Class>
                <owl:intersectionOf rdf:parseType="Collection">
                    <rdf:Description rdf:about="https://hack.cybersystems.engineer/memex/ontologies/SeamlessDigitalEngineering#Engineering_Discipline"/>
                    <owl:Restriction>
                        <owl:onProperty rdf:resource="https://www.commoncoreontologies.org/ont00001808"/>
                        <owl:someValuesFrom rdf:resource="https://hack.cybersystems.engineer/memex/ontologies/SeamlessDigitalEngineering#Act_of_Quality_Engineering"/>
                    </owl:Restriction>
                </owl:intersectionOf>
            </owl:Class>
        </owl:equivalentClass>
        <rdfs:subClassOf rdf:resource="https://hack.cybersystems.engineer/memex/ontologies/SeamlessDigitalEngineering#Engineering_Discipline"/>
        <rdfs:label xml:lang="en">Quality Engineering Discipline</rdfs:label>
        <skos:definition xml:lang="en">the Engineering Discipline concerned with the Principles and practice of Product and Service Quality Assurance and Quality Control</skos:definition>
        <cco2:ont00001754 rdf:datatype="http://www.w3.org/2001/XMLSchema#anyURI">https://en.wikipedia.org/wiki/Quality_engineering</cco2:ont00001754>
    </owl:Class>
    


    <!-- https://hack.cybersystems.engineer/memex/ontologies/SeamlessDigitalEngineering#Quality_Management_Process -->

    <owl:Class rdf:about="https://hack.cybersystems.engineer/memex/ontologies/SeamlessDigitalEngineering#Quality_Management_Process">
        <rdfs:subClassOf rdf:resource="https://hack.cybersystems.engineer/memex/ontologies/SeamlessDigitalEngineering#Organizational_Project-enabling_Process"/>
        <rdfs:label xml:lang="en">Quality Management Process</rdfs:label>
        <skos:definition xml:lang="en">The purpose of the quality management process is to assure that products, services, and implementations of the quality management process meet organizational and project quality objectives, and achieve customer satisfaction.</skos:definition>
        <cco2:ont00001754>ISO/IEC/IEEE 15288:2023</cco2:ont00001754>
    </owl:Class>
    


    <!-- https://hack.cybersystems.engineer/memex/ontologies/SeamlessDigitalEngineering#Quality_Measure -->

    <owl:Class rdf:about="https://hack.cybersystems.engineer/memex/ontologies/SeamlessDigitalEngineering#Quality_Measure">
        <rdfs:subClassOf rdf:resource="https://hack.cybersystems.engineer/memex/ontologies/SeamlessDigitalEngineering#Measure"/>
        <rdfs:comment xml:lang="en">Inherent (structural) Quality Measures quantify structural properties of the ICT Product or Information System, while behavioral Quality Measures quantify properties that can be identified and measured on the ICT Product or Information System as a whole and its behavior in a Context of Use.</rdfs:comment>
        <rdfs:comment xml:lang="en">Quality Measures can be considered as derived properties of an [Product or System].</rdfs:comment>
        <rdfs:label xml:lang="en">Quality Measure</rdfs:label>
        <skos:definition xml:lang="en">derived measure that is defined as a measurement function of two or more values of Quality Measure Elements</skos:definition>
        <cco2:ont00001754 xml:lang="en">ISO/IEC 25002:2024 Systems and software engineering - Systems and software Quality Requirements and Evaluation (SQuaRE) - Quality model overview and usage</cco2:ont00001754>
    </owl:Class>
    


    <!-- https://hack.cybersystems.engineer/memex/ontologies/SeamlessDigitalEngineering#Quality_Measure_Element -->

    <owl:Class rdf:about="https://hack.cybersystems.engineer/memex/ontologies/SeamlessDigitalEngineering#Quality_Measure_Element">
        <owl:equivalentClass>
            <owl:Restriction>
                <owl:onProperty rdf:resource="https://www.commoncoreontologies.org/ont00001966"/>
                <owl:someValuesFrom rdf:resource="https://hack.cybersystems.engineer/memex/ontologies/SeamlessDigitalEngineering#Quality_Property"/>
            </owl:Restriction>
        </owl:equivalentClass>
        <rdfs:subClassOf rdf:resource="https://hack.cybersystems.engineer/memex/ontologies/SeamlessDigitalEngineering#Quality_Measure"/>
        <rdfs:label xml:lang="en">Quality Measure Element</rdfs:label>
        <skos:definition xml:lang="en">measure defined in terms of a property and the measurement method for quantifying it, including optionally the transformation by a mathematical function.</skos:definition>
        <cco2:ont00001754 xml:lang="en">ISO/IEC 25002:2024 Systems and software engineering - Systems and software Quality Requirements and Evaluation (SQuaRE) - Quality model overview and usage</cco2:ont00001754>
    </owl:Class>
    


    <!-- https://hack.cybersystems.engineer/memex/ontologies/SeamlessDigitalEngineering#Quality_Model -->

    <owl:Class rdf:about="https://hack.cybersystems.engineer/memex/ontologies/SeamlessDigitalEngineering#Quality_Model">
        <owl:equivalentClass>
            <owl:Class>
                <owl:intersectionOf rdf:parseType="Collection">
                    <owl:Restriction>
                        <owl:onProperty rdf:resource="http://purl.obolibrary.org/obo/BFO_0000178"/>
                        <owl:someValuesFrom rdf:resource="https://hack.cybersystems.engineer/memex/ontologies/SeamlessDigitalEngineering#Quality_Characteristic"/>
                    </owl:Restriction>
                    <owl:Restriction>
                        <owl:onProperty rdf:resource="https://www.commoncoreontologies.org/ont00001942"/>
                        <owl:someValuesFrom rdf:resource="https://hack.cybersystems.engineer/memex/ontologies/SeamlessDigitalEngineering#Quality"/>
                    </owl:Restriction>
                </owl:intersectionOf>
            </owl:Class>
        </owl:equivalentClass>
        <rdfs:subClassOf rdf:resource="https://www.commoncoreontologies.org/ont00001045"/>
        <rdfs:label xml:lang="en">Quality Model</rdfs:label>
        <skos:definition xml:lang="en">defined set of Quality Characteristics and of relationships between them, which provides a framework for specifying Quality Requirements and evaluating Quality</skos:definition>
        <cco2:ont00001754 xml:lang="en">ISO/IEC 25000:2014</cco2:ont00001754>
    </owl:Class>
    


    <!-- https://hack.cybersystems.engineer/memex/ontologies/SeamlessDigitalEngineering#Quality_Need -->

    <owl:Class rdf:about="https://hack.cybersystems.engineer/memex/ontologies/SeamlessDigitalEngineering#Quality_Need">
        <owl:equivalentClass>
            <owl:Class>
                <owl:intersectionOf rdf:parseType="Collection">
                    <rdf:Description rdf:about="https://hack.cybersystems.engineer/memex/ontologies/SeamlessDigitalEngineering#Need"/>
                    <owl:Restriction>
                        <owl:onProperty rdf:resource="https://www.commoncoreontologies.org/ont00001942"/>
                        <owl:someValuesFrom>
                            <owl:Class>
                                <owl:unionOf rdf:parseType="Collection">
                                    <rdf:Description rdf:about="https://hack.cybersystems.engineer/memex/ontologies/SeamlessDigitalEngineering#Product_Quality-in-Use"/>
                                    <rdf:Description rdf:about="https://hack.cybersystems.engineer/memex/ontologies/SeamlessDigitalEngineering#Quality"/>
                                </owl:unionOf>
                            </owl:Class>
                        </owl:someValuesFrom>
                    </owl:Restriction>
                </owl:intersectionOf>
            </owl:Class>
        </owl:equivalentClass>
        <rdfs:subClassOf rdf:resource="https://hack.cybersystems.engineer/memex/ontologies/SeamlessDigitalEngineering#Need"/>
        <rdfs:label xml:lang="en">Quality Need</rdfs:label>
        <skos:definition xml:lang="en">the result of a formal transformation of one or more Lifecycle Concepts into an agreed-to expectation for an entity possess some Quality within specified constraints with acceptable risk.</skos:definition>
    </owl:Class>
    


    <!-- https://hack.cybersystems.engineer/memex/ontologies/SeamlessDigitalEngineering#Quality_Property -->

    <owl:Class rdf:about="https://hack.cybersystems.engineer/memex/ontologies/SeamlessDigitalEngineering#Quality_Property">
        <owl:equivalentClass>
            <owl:Class>
                <owl:intersectionOf rdf:parseType="Collection">
                    <rdf:Description rdf:about="https://hack.cybersystems.engineer/memex/ontologies/SeamlessDigitalEngineering#Attribute"/>
                    <owl:Restriction>
                        <owl:onProperty rdf:resource="http://purl.obolibrary.org/obo/BFO_0000195"/>
                        <owl:someValuesFrom rdf:resource="https://hack.cybersystems.engineer/memex/ontologies/SeamlessDigitalEngineering#Quality"/>
                    </owl:Restriction>
                    <owl:Restriction>
                        <owl:onProperty rdf:resource="https://www.commoncoreontologies.org/ont00001904"/>
                        <owl:someValuesFrom rdf:resource="https://hack.cybersystems.engineer/memex/ontologies/SeamlessDigitalEngineering#Quality_Measure_Element"/>
                    </owl:Restriction>
                </owl:intersectionOf>
            </owl:Class>
        </owl:equivalentClass>
        <rdfs:subClassOf rdf:resource="https://hack.cybersystems.engineer/memex/ontologies/SeamlessDigitalEngineering#Attribute"/>
        <rdfs:label xml:lang="en">Quality Property</rdfs:label>
        <skos:altLabel xml:lang="en">Quality Attribute</skos:altLabel>
        <skos:definition xml:lang="en">property of a Target Entity that is related to a Quality Measure Element and which can be quantified by a measurement method</skos:definition>
        <cco2:ont00001754 xml:lang="en">ISO/IEC 25002:2024 Systems and software engineering - Systems and software Quality Requirements and Evaluation (SQuaRE) - Quality model overview and usage</cco2:ont00001754>
    </owl:Class>
    


    <!-- https://hack.cybersystems.engineer/memex/ontologies/SeamlessDigitalEngineering#Quality_Requirement -->

    <owl:Class rdf:about="https://hack.cybersystems.engineer/memex/ontologies/SeamlessDigitalEngineering#Quality_Requirement">
        <owl:equivalentClass>
            <owl:Class>
                <owl:intersectionOf rdf:parseType="Collection">
                    <rdf:Description rdf:about="https://hack.cybersystems.engineer/memex/ontologies/SeamlessDigitalEngineering#Requirement"/>
                    <owl:Restriction>
                        <owl:onProperty rdf:resource="https://www.commoncoreontologies.org/ont00001942"/>
                        <owl:someValuesFrom>
                            <owl:Class>
                                <owl:unionOf rdf:parseType="Collection">
                                    <rdf:Description rdf:about="https://hack.cybersystems.engineer/memex/ontologies/SeamlessDigitalEngineering#Product_Quality-in-Use"/>
                                    <rdf:Description rdf:about="https://hack.cybersystems.engineer/memex/ontologies/SeamlessDigitalEngineering#Quality"/>
                                </owl:unionOf>
                            </owl:Class>
                        </owl:someValuesFrom>
                    </owl:Restriction>
                </owl:intersectionOf>
            </owl:Class>
        </owl:equivalentClass>
        <rdfs:subClassOf rdf:resource="https://www.commoncoreontologies.org/ont00000575"/>
        <rdfs:label xml:lang="en">Quality Requirement</rdfs:label>
        <skos:definition xml:lang="en">Requirement for Quality Properties or Attributes of an Product, Data, or Service that satisfy Needs which ensue from the purpose for which that Product, Data, or Service is to be used</skos:definition>
        <cco2:ont00001754 xml:lang="en">ISO/IEC 25002:2024 Systems and software engineering - Systems and software Quality Requirements and Evaluation (SQuaRE) - Quality model overview and usage</cco2:ont00001754>
    </owl:Class>
    


    <!-- https://hack.cybersystems.engineer/memex/ontologies/SeamlessDigitalEngineering#Quality_Sub-characteristic -->

    <owl:Class rdf:about="https://hack.cybersystems.engineer/memex/ontologies/SeamlessDigitalEngineering#Quality_Sub-characteristic">
        <owl:equivalentClass>
            <owl:Restriction>
                <owl:onProperty rdf:resource="http://purl.obolibrary.org/obo/BFO_0000176"/>
                <owl:someValuesFrom rdf:resource="https://hack.cybersystems.engineer/memex/ontologies/SeamlessDigitalEngineering#Quality_Characteristic"/>
            </owl:Restriction>
        </owl:equivalentClass>
        <rdfs:subClassOf rdf:resource="https://hack.cybersystems.engineer/memex/ontologies/SeamlessDigitalEngineering#Quality_Characteristic"/>
        <rdfs:label xml:lang="en">Quality Sub-characteristic</rdfs:label>
    </owl:Class>
    


    <!-- https://hack.cybersystems.engineer/memex/ontologies/SeamlessDigitalEngineering#Record -->

    <owl:Class rdf:about="https://hack.cybersystems.engineer/memex/ontologies/SeamlessDigitalEngineering#Record">
        <owl:equivalentClass>
            <owl:Class>
                <owl:intersectionOf rdf:parseType="Collection">
                    <rdf:Description rdf:about="http://www.ontologyrepository.com/CommonCoreOntologies/Tuple"/>
                    <owl:Restriction>
                        <owl:onProperty rdf:resource="http://purl.obolibrary.org/obo/BFO_0000115"/>
                        <owl:minQualifiedCardinality rdf:datatype="http://www.w3.org/2001/XMLSchema#nonNegativeInteger">0</owl:minQualifiedCardinality>
                        <owl:onClass rdf:resource="http://www.ontologyrepository.com/CommonCoreOntologies/KeyValuePair"/>
                    </owl:Restriction>
                </owl:intersectionOf>
            </owl:Class>
        </owl:equivalentClass>
        <rdfs:subClassOf rdf:resource="http://www.ontologyrepository.com/CommonCoreOntologies/Tuple"/>
        <rdfs:label xml:lang="en">Record</rdfs:label>
        <skos:altLabel xml:lang="en">Map</skos:altLabel>
        <skos:definition xml:lang="en">Value of a Record Type with possibly empty Set of Field-Value Pairs</skos:definition>
    </owl:Class>
    


    <!-- https://hack.cybersystems.engineer/memex/ontologies/SeamlessDigitalEngineering#Reference_Architecture -->

    <owl:Class rdf:about="https://hack.cybersystems.engineer/memex/ontologies/SeamlessDigitalEngineering#Reference_Architecture">
        <owl:equivalentClass>
            <owl:Restriction>
                <owl:onProperty rdf:resource="https://www.commoncoreontologies.org/ont00001942"/>
                <owl:someValuesFrom rdf:resource="https://hack.cybersystems.engineer/memex/ontologies/SeamlessDigitalEngineering#Architecture"/>
            </owl:Restriction>
        </owl:equivalentClass>
        <rdfs:subClassOf rdf:resource="https://hack.cybersystems.engineer/memex/ontologies/SeamlessDigitalEngineering#Architecture"/>
        <rdfs:comment xml:lang="en">A reference architecture is used by a community of interest as a shared and agreed reference description that can be used for that community’s business purposes. It is usually generic and is instantiated as architectures specific for individual business purposes. Reference architectures are used to:

a) aid understanding of the forms of likely solutions to problems within a particular domain, and
b) maximize the possible commonality in forms of solutions to similar problems within such a domain.</rdfs:comment>
        <rdfs:label xml:lang="en">Reference Architecture</rdfs:label>
        <cco2:ont00001754 xml:lang="en">ISO/IEC/IEEE 42020:2019</cco2:ont00001754>
    </owl:Class>
    


    <!-- https://hack.cybersystems.engineer/memex/ontologies/SeamlessDigitalEngineering#Reference_Material -->

    <owl:Class rdf:about="https://hack.cybersystems.engineer/memex/ontologies/SeamlessDigitalEngineering#Reference_Material">
        <rdfs:subClassOf rdf:resource="https://www.commoncoreontologies.org/ont00000798"/>
        <rdfs:comment xml:lang="en">Reference Material is Information-oriented.</rdfs:comment>
        <rdfs:label xml:lang="en">Reference Material</rdfs:label>
        <skos:definition xml:lang="en">Reference Material is carrier of some ICEs of the System-of-Interest and how to operate it.</skos:definition>
        <cco2:ont00001754 rdf:datatype="http://www.w3.org/2001/XMLSchema#anyURI">https://diataxis.fr/reference/</cco2:ont00001754>
    </owl:Class>
    


    <!-- https://hack.cybersystems.engineer/memex/ontologies/SeamlessDigitalEngineering#Requirement -->

    <owl:Class rdf:about="https://hack.cybersystems.engineer/memex/ontologies/SeamlessDigitalEngineering#Requirement">
        <owl:equivalentClass>
            <owl:Class>
                <owl:intersectionOf rdf:parseType="Collection">
                    <owl:Class>
                        <owl:unionOf rdf:parseType="Collection">
                            <rdf:Description rdf:about="https://www.commoncoreontologies.org/ont00000127"/>
                            <rdf:Description rdf:about="https://www.commoncoreontologies.org/ont00000575"/>
                        </owl:unionOf>
                    </owl:Class>
                    <owl:Restriction>
                        <owl:onProperty rdf:resource="http://purl.obolibrary.org/obo/BFO_0000178"/>
                        <owl:someValuesFrom rdf:resource="http://www.ontologyrepository.com/CommonCoreOntologies/Constraint"/>
                    </owl:Restriction>
                    <owl:Restriction>
                        <owl:onProperty rdf:resource="https://www.commoncoreontologies.org/ont00001942"/>
                        <owl:someValuesFrom rdf:resource="https://hack.cybersystems.engineer/memex/ontologies/SeamlessDigitalEngineering#System"/>
                    </owl:Restriction>
                </owl:intersectionOf>
            </owl:Class>
        </owl:equivalentClass>
        <rdfs:subClassOf rdf:resource="https://www.commoncoreontologies.org/ont00000965"/>
        <skos:definition xml:lang="en">statement which translates or expresses a Need and its associated Constraints and Conditions</skos:definition>
        <cco2:ont00001754>ISO/IEC/IEEE 15288:2023</cco2:ont00001754>
    </owl:Class>
    


    <!-- https://hack.cybersystems.engineer/memex/ontologies/SeamlessDigitalEngineering#Requirement_Attribute -->

    <owl:Class rdf:about="https://hack.cybersystems.engineer/memex/ontologies/SeamlessDigitalEngineering#Requirement_Attribute">
        <rdfs:subClassOf rdf:resource="https://hack.cybersystems.engineer/memex/ontologies/SeamlessDigitalEngineering#Requirement"/>
        <rdfs:label xml:lang="en">Requirement Attribute</rdfs:label>
    </owl:Class>
    


    <!-- https://hack.cybersystems.engineer/memex/ontologies/SeamlessDigitalEngineering#Requirement_Expression -->

    <owl:Class rdf:about="https://hack.cybersystems.engineer/memex/ontologies/SeamlessDigitalEngineering#Requirement_Expression">
        <owl:equivalentClass>
            <owl:Class>
                <owl:intersectionOf rdf:parseType="Collection">
                    <rdf:Description rdf:about="https://hack.cybersystems.engineer/memex/ontologies/SeamlessDigitalEngineering#Requirement"/>
                    <owl:Restriction>
                        <owl:onProperty rdf:resource="http://purl.obolibrary.org/obo/BFO_0000178"/>
                        <owl:someValuesFrom>
                            <owl:Class>
                                <owl:intersectionOf rdf:parseType="Collection">
                                    <rdf:Description rdf:about="https://hack.cybersystems.engineer/memex/ontologies/SeamlessDigitalEngineering#Requirement_Attribute"/>
                                    <rdf:Description rdf:about="https://hack.cybersystems.engineer/memex/ontologies/SeamlessDigitalEngineering#Requirement_Statement"/>
                                </owl:intersectionOf>
                            </owl:Class>
                        </owl:someValuesFrom>
                    </owl:Restriction>
                </owl:intersectionOf>
            </owl:Class>
        </owl:equivalentClass>
        <rdfs:subClassOf rdf:resource="https://hack.cybersystems.engineer/memex/ontologies/SeamlessDigitalEngineering#Requirement"/>
        <rdfs:label xml:lang="en">Requirement Expression</rdfs:label>
        <skos:definition xml:lang="en">includes a Requirement Statement and a set of associated Attributes.</skos:definition>
        <cco2:ont00001754 xml:lang="en">INCOSE Needs and Requirements Manual R1.1 (2022)</cco2:ont00001754>
    </owl:Class>
    


    <!-- https://hack.cybersystems.engineer/memex/ontologies/SeamlessDigitalEngineering#Requirement_Set -->

    <owl:Class rdf:about="https://hack.cybersystems.engineer/memex/ontologies/SeamlessDigitalEngineering#Requirement_Set">
        <owl:equivalentClass>
            <owl:Class>
                <owl:intersectionOf rdf:parseType="Collection">
                    <owl:Restriction>
                        <owl:onProperty rdf:resource="https://www.commoncoreontologies.org/ont00001816"/>
                        <owl:someValuesFrom rdf:resource="https://hack.cybersystems.engineer/memex/ontologies/SeamlessDigitalEngineering#Act_of_Stakeholder_Agreement"/>
                    </owl:Restriction>
                    <owl:Restriction>
                        <owl:onProperty rdf:resource="http://purl.obolibrary.org/obo/BFO_0000178"/>
                        <owl:minQualifiedCardinality rdf:datatype="http://www.w3.org/2001/XMLSchema#nonNegativeInteger">2</owl:minQualifiedCardinality>
                        <owl:onClass rdf:resource="https://hack.cybersystems.engineer/memex/ontologies/SeamlessDigitalEngineering#Requirement_Expression"/>
                    </owl:Restriction>
                </owl:intersectionOf>
            </owl:Class>
        </owl:equivalentClass>
        <rdfs:subClassOf rdf:resource="https://www.commoncoreontologies.org/ont00000965"/>
        <rdfs:label xml:lang="en">Requirement Set</rdfs:label>
        <skos:altLabel xml:lang="en">Design Input Requirements</skos:altLabel>
        <skos:definition xml:lang="en">a structured set of agreed-to Requirement Expressions for the entity (enterprise/business unit/system/subsystem/system element/process) and its external Interfaces</skos:definition>
        <cco2:ont00001754 xml:lang="en">INCOSE Needs and Requirements Manual R1.1 (2022)</cco2:ont00001754>
    </owl:Class>
    


    <!-- https://hack.cybersystems.engineer/memex/ontologies/SeamlessDigitalEngineering#Requirement_Statement -->

    <owl:Class rdf:about="https://hack.cybersystems.engineer/memex/ontologies/SeamlessDigitalEngineering#Requirement_Statement">
        <owl:equivalentClass>
            <owl:Class>
                <owl:intersectionOf rdf:parseType="Collection">
                    <rdf:Description rdf:about="https://hack.cybersystems.engineer/memex/ontologies/SeamlessDigitalEngineering#Requirement"/>
                    <owl:Restriction>
                        <owl:onProperty rdf:resource="https://www.commoncoreontologies.org/ont00001816"/>
                        <owl:someValuesFrom rdf:resource="https://hack.cybersystems.engineer/memex/ontologies/SeamlessDigitalEngineering#Act_of_Formal_Transformation"/>
                    </owl:Restriction>
                    <owl:Restriction>
                        <owl:onProperty rdf:resource="https://www.commoncoreontologies.org/ont00001920"/>
                        <owl:someValuesFrom rdf:resource="https://www.commoncoreontologies.org/ont00000496"/>
                    </owl:Restriction>
                    <owl:Restriction>
                        <owl:onProperty rdf:resource="https://www.commoncoreontologies.org/ont00001942"/>
                        <owl:someValuesFrom>
                            <owl:Class>
                                <owl:unionOf rdf:parseType="Collection">
                                    <rdf:Description rdf:about="http://purl.obolibrary.org/obo/BFO_0000034"/>
                                    <rdf:Description rdf:about="https://hack.cybersystems.engineer/memex/ontologies/SeamlessDigitalEngineering#Quality"/>
                                </owl:unionOf>
                            </owl:Class>
                        </owl:someValuesFrom>
                    </owl:Restriction>
                </owl:intersectionOf>
            </owl:Class>
        </owl:equivalentClass>
        <rdfs:subClassOf rdf:resource="https://hack.cybersystems.engineer/memex/ontologies/SeamlessDigitalEngineering#Requirement"/>
        <rdfs:comment xml:lang="en">For the purpose of high-level Stakeholder Requirements, Requirement Statements may optionally prescribe a Condition.</rdfs:comment>
        <rdfs:label xml:lang="en">Requirement Statement</rdfs:label>
        <skos:definition xml:lang="en">the result of an Act of Formal Transformation of one or more sources, Needs, or higher-level Requirements into an agreed-to obligation for an entity to perform some function or possess some quality within specified Constraints with acceptable Risk.</skos:definition>
        <cco2:ont00001754 xml:lang="en">INCOSE Needs and Requirements Manual R1.1 (2022)</cco2:ont00001754>
    </owl:Class>
    


    <!-- https://hack.cybersystems.engineer/memex/ontologies/SeamlessDigitalEngineering#Requirements_Engineering_Discipline -->

    <owl:Class rdf:about="https://hack.cybersystems.engineer/memex/ontologies/SeamlessDigitalEngineering#Requirements_Engineering_Discipline">
        <owl:equivalentClass>
            <owl:Class>
                <owl:intersectionOf rdf:parseType="Collection">
                    <rdf:Description rdf:about="https://hack.cybersystems.engineer/memex/ontologies/SeamlessDigitalEngineering#Engineering_Discipline"/>
                    <owl:Restriction>
                        <owl:onProperty rdf:resource="https://www.commoncoreontologies.org/ont00001808"/>
                        <owl:someValuesFrom rdf:resource="https://hack.cybersystems.engineer/memex/ontologies/SeamlessDigitalEngineering#Act_of_Requirements_Engineering"/>
                    </owl:Restriction>
                </owl:intersectionOf>
            </owl:Class>
        </owl:equivalentClass>
        <rdfs:subClassOf rdf:resource="https://hack.cybersystems.engineer/memex/ontologies/SeamlessDigitalEngineering#Engineering_Discipline"/>
        <rdfs:label xml:lang="en">Requirements Engineering Discipline</rdfs:label>
    </owl:Class>
    


    <!-- https://hack.cybersystems.engineer/memex/ontologies/SeamlessDigitalEngineering#Retirement_Stage -->

    <owl:Class rdf:about="https://hack.cybersystems.engineer/memex/ontologies/SeamlessDigitalEngineering#Retirement_Stage">
        <rdfs:subClassOf rdf:resource="https://hack.cybersystems.engineer/memex/ontologies/SeamlessDigitalEngineering#Lifecycle_Stage"/>
        <rdfs:comment xml:lang="en">Purpose: The retirement stage is executed to provide for the removal of a SoI and related operational and support services and to operate and support the retirement system itself.</rdfs:comment>
        <rdfs:label xml:lang="en">Retirement Stage</rdfs:label>
        <cco2:ont00001754>ISO/IEC/IEEE 24748-1:2024</cco2:ont00001754>
    </owl:Class>
    


    <!-- https://hack.cybersystems.engineer/memex/ontologies/SeamlessDigitalEngineering#Review_Minutes -->

    <owl:Class rdf:about="https://hack.cybersystems.engineer/memex/ontologies/SeamlessDigitalEngineering#Review_Minutes">
        <rdfs:subClassOf rdf:resource="https://www.commoncoreontologies.org/ont00000624"/>
    </owl:Class>
    


    <!-- https://hack.cybersystems.engineer/memex/ontologies/SeamlessDigitalEngineering#Right -->

    <owl:Class rdf:about="https://hack.cybersystems.engineer/memex/ontologies/SeamlessDigitalEngineering#Right">
        <owl:equivalentClass>
            <owl:Class>
                <owl:intersectionOf rdf:parseType="Collection">
                    <rdf:Description rdf:about="https://www.commoncoreontologies.org/ont00000284"/>
                    <owl:Restriction>
                        <owl:onProperty rdf:resource="http://purl.obolibrary.org/obo/BFO_0000054"/>
                        <owl:someValuesFrom rdf:resource="https://www.commoncoreontologies.org/ont00000005"/>
                    </owl:Restriction>
                </owl:intersectionOf>
            </owl:Class>
        </owl:equivalentClass>
        <rdfs:subClassOf rdf:resource="https://www.commoncoreontologies.org/ont00000284"/>
        <rdfs:comment xml:lang="en">A Right can provide a formal or informal entitlement to own or do something.</rdfs:comment>
        <rdfs:comment xml:lang="en">Rights may be overlapping, or may be in disagreement.</rdfs:comment>
        <rdfs:label xml:lang="en">Right</rdfs:label>
        <skos:definition xml:lang="en">formal or informal entitlement to own or perform an Act</skos:definition>
        <skos:example xml:lang="en">Ownership right, apartment right, tenancy right, possessions, customary right, Islamic right (e.g. miri or milk), Indigenous right, informal right, sovereign rights, rights of innocent passage or rights of transit passage.</skos:example>
        <cco2:ont00001754 xml:lang="en">ISO 19152-1:2024 - Geographic information - Land Administration Domain Model (LAFM) - Part 1: Generic conceptual model</cco2:ont00001754>
    </owl:Class>
    


    <!-- https://hack.cybersystems.engineer/memex/ontologies/SeamlessDigitalEngineering#Right_Declaration -->

    <owl:Class rdf:about="https://hack.cybersystems.engineer/memex/ontologies/SeamlessDigitalEngineering#Right_Declaration">
        <owl:equivalentClass>
            <owl:Class>
                <owl:intersectionOf rdf:parseType="Collection">
                    <rdf:Description rdf:about="https://www.commoncoreontologies.org/ont00000253"/>
                    <owl:Restriction>
                        <owl:onProperty rdf:resource="http://purl.obolibrary.org/obo/BFO_0000101"/>
                        <owl:someValuesFrom rdf:resource="https://hack.cybersystems.engineer/memex/ontologies/SeamlessDigitalEngineering#Human_Rights"/>
                    </owl:Restriction>
                </owl:intersectionOf>
            </owl:Class>
        </owl:equivalentClass>
        <rdfs:subClassOf rdf:resource="https://www.commoncoreontologies.org/ont00000253"/>
        <rdfs:label xml:lang="en">Right Declaration</rdfs:label>
    </owl:Class>
    


    <!-- https://hack.cybersystems.engineer/memex/ontologies/SeamlessDigitalEngineering#Risk -->

    <owl:Class rdf:about="https://hack.cybersystems.engineer/memex/ontologies/SeamlessDigitalEngineering#Risk">
        <owl:equivalentClass>
            <owl:Class>
                <owl:intersectionOf rdf:parseType="Collection">
                    <owl:Restriction>
                        <owl:onProperty rdf:resource="https://www.commoncoreontologies.org/ont00001819"/>
                        <owl:someValuesFrom rdf:resource="https://hack.cybersystems.engineer/memex/ontologies/SeamlessDigitalEngineering#Uncertainty"/>
                    </owl:Restriction>
                    <owl:Restriction>
                        <owl:onProperty rdf:resource="https://www.commoncoreontologies.org/ont00001834"/>
                        <owl:someValuesFrom rdf:resource="https://www.commoncoreontologies.org/ont00000476"/>
                    </owl:Restriction>
                </owl:intersectionOf>
            </owl:Class>
        </owl:equivalentClass>
        <rdfs:subClassOf rdf:resource="https://www.commoncoreontologies.org/ont00000660"/>
        <rdfs:label xml:lang="en">Risk</rdfs:label>
        <skos:definition xml:lang="en">effect of Uncertainty on Objectives</skos:definition>
        <cco2:ont00001754 xml:lang="en">ISO/IEC/IEEE 15288:2023</cco2:ont00001754>
    </owl:Class>
    


    <!-- https://hack.cybersystems.engineer/memex/ontologies/SeamlessDigitalEngineering#Risk_Management_Process -->

    <owl:Class rdf:about="https://hack.cybersystems.engineer/memex/ontologies/SeamlessDigitalEngineering#Risk_Management_Process">
        <rdfs:subClassOf rdf:resource="https://hack.cybersystems.engineer/memex/ontologies/SeamlessDigitalEngineering#Technical_Management_Process"/>
        <rdfs:label xml:lang="en">Risk Management Process</rdfs:label>
        <skos:definition xml:lang="en">The purpose of the risk management process is to identify, analyse, treat, and monitor the risks continually.</skos:definition>
        <cco2:ont00001754>ISO/IEC/IEEE 15288:2023</cco2:ont00001754>
    </owl:Class>
    


    <!-- https://hack.cybersystems.engineer/memex/ontologies/SeamlessDigitalEngineering#Root_of_Trust_Role -->

    <owl:Class rdf:about="https://hack.cybersystems.engineer/memex/ontologies/SeamlessDigitalEngineering#Root_of_Trust_Role">
        <rdfs:subClassOf rdf:resource="https://hack.cybersystems.engineer/memex/ontologies/SeamlessDigitalEngineering#Trusted_Role"/>
        <rdfs:label xml:lang="en">Root of Trust Role</rdfs:label>
        <rdfs:seeAlso rdf:resource="https://hack.cybersystems.engineer/memex/ontologies/SeamlessDigitalEngineering#Auditable_Hex_Seed"/>
        <skos:definition xml:lang="en">A Trusted Role on which all other Trusted Roles depend.</skos:definition>
    </owl:Class>
    


    <!-- https://hack.cybersystems.engineer/memex/ontologies/SeamlessDigitalEngineering#SAT_Solver -->

    <owl:Class rdf:about="https://hack.cybersystems.engineer/memex/ontologies/SeamlessDigitalEngineering#SAT_Solver">
        <rdfs:subClassOf rdf:resource="https://hack.cybersystems.engineer/memex/ontologies/SeamlessDigitalEngineering#Constraint_Solver"/>
        <rdfs:label xml:lang="en">SAT Solver</rdfs:label>
        <rdfs:seeAlso rdf:datatype="http://www.w3.org/2001/XMLSchema#anyURI">https://en.wikipedia.org/wiki/SAT_solver</rdfs:seeAlso>
        <skos:altLabel xml:lang="en">Boolean Satisfiability Solver</skos:altLabel>
    </owl:Class>
    


    <!-- https://hack.cybersystems.engineer/memex/ontologies/SeamlessDigitalEngineering#SMT_Solver -->

    <owl:Class rdf:about="https://hack.cybersystems.engineer/memex/ontologies/SeamlessDigitalEngineering#SMT_Solver">
        <rdfs:subClassOf rdf:resource="https://hack.cybersystems.engineer/memex/ontologies/SeamlessDigitalEngineering#Constraint_Solver"/>
        <rdfs:label xml:lang="en">SMT Solver</rdfs:label>
        <rdfs:seeAlso rdf:datatype="http://www.w3.org/2001/XMLSchema#anyURI">https://en.wikipedia.org/wiki/Satisfiability_modulo_theories</rdfs:seeAlso>
        <skos:altLabel xml:lang="en">Satisfiability Modulo Theories Solver</skos:altLabel>
    </owl:Class>
    


    <!-- https://hack.cybersystems.engineer/memex/ontologies/SeamlessDigitalEngineering#Scientific_Discipline -->

    <owl:Class rdf:about="https://hack.cybersystems.engineer/memex/ontologies/SeamlessDigitalEngineering#Scientific_Discipline">
        <owl:equivalentClass>
            <owl:Class>
                <owl:intersectionOf rdf:parseType="Collection">
                    <rdf:Description rdf:about="https://hack.cybersystems.engineer/memex/ontologies/SeamlessDigitalEngineering#Discipline"/>
                    <owl:Restriction>
                        <owl:onProperty rdf:resource="https://www.commoncoreontologies.org/ont00001808"/>
                        <owl:someValuesFrom rdf:resource="https://hack.cybersystems.engineer/memex/ontologies/SeamlessDigitalEngineering#Act_of_Science"/>
                    </owl:Restriction>
                </owl:intersectionOf>
            </owl:Class>
        </owl:equivalentClass>
        <rdfs:subClassOf rdf:resource="https://hack.cybersystems.engineer/memex/ontologies/SeamlessDigitalEngineering#Discipline"/>
        <rdfs:label xml:lang="en">Scientific Discipline</rdfs:label>
        <skos:definition xml:lang="en">broad domain, branch or area of content covered by an education programme or qualification</skos:definition>
        <cco2:ont00001754 xml:lang="en">ISO/TS 21030:2023
Educational organizations
Requirements for bodies providing audit and certification of educational organizations&apos; management systems</cco2:ont00001754>
    </owl:Class>
    


    <!-- https://hack.cybersystems.engineer/memex/ontologies/SeamlessDigitalEngineering#Scientific_Method -->

    <owl:Class rdf:about="https://hack.cybersystems.engineer/memex/ontologies/SeamlessDigitalEngineering#Scientific_Method">
        <owl:equivalentClass>
            <owl:Class>
                <owl:intersectionOf rdf:parseType="Collection">
                    <rdf:Description rdf:about="https://hack.cybersystems.engineer/memex/ontologies/SeamlessDigitalEngineering#Method"/>
                    <owl:Restriction>
                        <owl:onProperty rdf:resource="https://www.commoncoreontologies.org/ont00001942"/>
                        <owl:someValuesFrom rdf:resource="https://hack.cybersystems.engineer/memex/ontologies/SeamlessDigitalEngineering#Act_of_Science"/>
                    </owl:Restriction>
                </owl:intersectionOf>
            </owl:Class>
        </owl:equivalentClass>
        <rdfs:subClassOf rdf:resource="https://hack.cybersystems.engineer/memex/ontologies/SeamlessDigitalEngineering#Method"/>
        <rdfs:label xml:lang="en">Scientific Method</rdfs:label>
    </owl:Class>
    


    <!-- https://hack.cybersystems.engineer/memex/ontologies/SeamlessDigitalEngineering#Scientific_Principle -->

    <owl:Class rdf:about="https://hack.cybersystems.engineer/memex/ontologies/SeamlessDigitalEngineering#Scientific_Principle">
        <rdfs:subClassOf rdf:resource="https://hack.cybersystems.engineer/memex/ontologies/SeamlessDigitalEngineering#Principle"/>
        <rdfs:label xml:lang="en">Scientific Principle</rdfs:label>
    </owl:Class>
    


    <!-- https://hack.cybersystems.engineer/memex/ontologies/SeamlessDigitalEngineering#Scientist -->

    <owl:Class rdf:about="https://hack.cybersystems.engineer/memex/ontologies/SeamlessDigitalEngineering#Scientist">
        <rdfs:subClassOf rdf:resource="https://hack.cybersystems.engineer/memex/ontologies/SeamlessDigitalEngineering#Project_Team_Member"/>
    </owl:Class>
    


    <!-- https://hack.cybersystems.engineer/memex/ontologies/SeamlessDigitalEngineering#Seamless_Digital_Engineering_Paradigm -->

    <owl:Class rdf:about="https://hack.cybersystems.engineer/memex/ontologies/SeamlessDigitalEngineering#Seamless_Digital_Engineering_Paradigm">
        <owl:equivalentClass>
            <owl:Class>
                <owl:intersectionOf rdf:parseType="Collection">
                    <rdf:Description rdf:about="https://hack.cybersystems.engineer/memex/ontologies/SeamlessDigitalEngineering#Paradigm"/>
                    <owl:Restriction>
                        <owl:onProperty rdf:resource="http://purl.obolibrary.org/obo/BFO_0000178"/>
                        <owl:someValuesFrom rdf:resource="https://hack.cybersystems.engineer/memex/ontologies/SeamlessDigitalEngineering#Digital_Engineering_Approach"/>
                    </owl:Restriction>
                    <owl:Restriction>
                        <owl:onProperty rdf:resource="https://www.commoncoreontologies.org/ont00001808"/>
                        <owl:someValuesFrom rdf:resource="https://hack.cybersystems.engineer/memex/ontologies/SeamlessDigitalEngineering#Correct-by-Construction"/>
                    </owl:Restriction>
                    <owl:Restriction>
                        <owl:onProperty rdf:resource="https://www.commoncoreontologies.org/ont00001942"/>
                        <owl:someValuesFrom rdf:resource="https://hack.cybersystems.engineer/memex/ontologies/SeamlessDigitalEngineering#Seamless_Digital_Engineering_System"/>
                    </owl:Restriction>
                </owl:intersectionOf>
            </owl:Class>
        </owl:equivalentClass>
        <rdfs:subClassOf rdf:resource="https://hack.cybersystems.engineer/memex/ontologies/SeamlessDigitalEngineering#Paradigm"/>
        <rdfs:label xml:lang="en">Seamless Digital Engineering Paradigm</rdfs:label>
        <skos:definition xml:lang="en">A Paradigm of Digital Engineering Environments that guarantees model coherence and integrity by affording an Elegant Human-Computer Interface for Systems modeling that is end-to-end formally verified down thru the Computer Hardware.</skos:definition>
        <cco2:ont00001754 rdf:datatype="http://www.w3.org/2001/XMLSchema#anyURI">https://doi.org/10.2514/6.2024-1053</cco2:ont00001754>
    </owl:Class>
    


    <!-- https://hack.cybersystems.engineer/memex/ontologies/SeamlessDigitalEngineering#Seamless_Digital_Engineering_System -->

    <owl:Class rdf:about="https://hack.cybersystems.engineer/memex/ontologies/SeamlessDigitalEngineering#Seamless_Digital_Engineering_System">
        <owl:equivalentClass>
            <owl:Class>
                <owl:intersectionOf rdf:parseType="Collection">
                    <rdf:Description rdf:about="https://hack.cybersystems.engineer/memex/ontologies/SeamlessDigitalEngineering#Digital_Engineering_Environment"/>
                    <rdf:Description rdf:about="https://hack.cybersystems.engineer/memex/ontologies/SeamlessDigitalEngineering#Engineered_System"/>
                    <owl:Restriction>
                        <owl:onProperty rdf:resource="http://purl.obolibrary.org/obo/BFO_0000101"/>
                        <owl:someValuesFrom>
                            <owl:Class>
                                <owl:intersectionOf rdf:parseType="Collection">
                                    <rdf:Description rdf:about="https://hack.cybersystems.engineer/memex/ontologies/SeamlessDigitalEngineering#High-Integrity_Level_Claim"/>
                                    <rdf:Description rdf:about="https://hack.cybersystems.engineer/memex/ontologies/SeamlessDigitalEngineering#Seamless_Quality_Claim"/>
                                </owl:intersectionOf>
                            </owl:Class>
                        </owl:someValuesFrom>
                    </owl:Restriction>
                    <owl:Restriction>
                        <owl:onProperty rdf:resource="http://purl.obolibrary.org/obo/BFO_0000115"/>
                        <owl:someValuesFrom rdf:resource="https://hack.cybersystems.engineer/memex/ontologies/SeamlessDigitalEngineering#Trustworthy_Computing_Base"/>
                    </owl:Restriction>
                </owl:intersectionOf>
            </owl:Class>
        </owl:equivalentClass>
        <rdfs:subClassOf rdf:resource="https://hack.cybersystems.engineer/memex/ontologies/SeamlessDigitalEngineering#Engineered_System"/>
        <rdfs:label xml:lang="en">Seamless Digital Engineering System</rdfs:label>
        <skos:definition xml:lang="en">An Engineered System and Digital Engineering Environment composed of Trustworthy Computing Base components which carries an independently verifiable Seamless Quality Claim and High-Integrity Level Claim</skos:definition>
    </owl:Class>
    


    <!-- https://hack.cybersystems.engineer/memex/ontologies/SeamlessDigitalEngineering#Seamless_Integration -->

    <owl:Class rdf:about="https://hack.cybersystems.engineer/memex/ontologies/SeamlessDigitalEngineering#Seamless_Integration">
        <owl:equivalentClass>
            <owl:Class>
                <owl:intersectionOf rdf:parseType="Collection">
                    <rdf:Description rdf:about="https://hack.cybersystems.engineer/memex/ontologies/SeamlessDigitalEngineering#Product_Capability"/>
                    <owl:Restriction>
                        <owl:onProperty rdf:resource="http://purl.obolibrary.org/obo/BFO_0000054"/>
                        <owl:someValuesFrom rdf:resource="https://hack.cybersystems.engineer/memex/ontologies/SeamlessDigitalEngineering#Act_of_Formal_Verification"/>
                    </owl:Restriction>
                    <owl:Restriction>
                        <owl:onProperty rdf:resource="http://purl.obolibrary.org/obo/BFO_0000178"/>
                        <owl:someValuesFrom>
                            <owl:Class>
                                <owl:intersectionOf rdf:parseType="Collection">
                                    <rdf:Description rdf:about="https://hack.cybersystems.engineer/memex/ontologies/SeamlessDigitalEngineering#Product_Analysability"/>
                                    <rdf:Description rdf:about="https://hack.cybersystems.engineer/memex/ontologies/SeamlessDigitalEngineering#Product_Faultlessness"/>
                                    <rdf:Description rdf:about="https://hack.cybersystems.engineer/memex/ontologies/SeamlessDigitalEngineering#Product_Functional_Correctness"/>
                                    <rdf:Description rdf:about="https://hack.cybersystems.engineer/memex/ontologies/SeamlessDigitalEngineering#Product_Integrity"/>
                                    <rdf:Description rdf:about="https://hack.cybersystems.engineer/memex/ontologies/SeamlessDigitalEngineering#Product_Safe_Integration"/>
                                </owl:intersectionOf>
                            </owl:Class>
                        </owl:someValuesFrom>
                    </owl:Restriction>
                    <owl:Restriction>
                        <owl:onProperty rdf:resource="http://purl.obolibrary.org/obo/BFO_0000195"/>
                        <owl:someValuesFrom rdf:resource="https://hack.cybersystems.engineer/memex/ontologies/SeamlessDigitalEngineering#Seamless_Interface"/>
                    </owl:Restriction>
                </owl:intersectionOf>
            </owl:Class>
        </owl:equivalentClass>
        <rdfs:subClassOf rdf:resource="https://hack.cybersystems.engineer/memex/ontologies/SeamlessDigitalEngineering#Product_Capability"/>
        <rdfs:label xml:lang="en">Seamless Integration</rdfs:label>
        <skos:definition xml:lang="en">perfectly consistent and coherent and not having or joined by a seam or seams</skos:definition>
        <cco2:ont00001754 xml:lang="en">Princeton WordNet</cco2:ont00001754>
    </owl:Class>
    


    <!-- https://hack.cybersystems.engineer/memex/ontologies/SeamlessDigitalEngineering#Seamless_Interaction_Capability -->

    <owl:Class rdf:about="https://hack.cybersystems.engineer/memex/ontologies/SeamlessDigitalEngineering#Seamless_Interaction_Capability">
        <owl:equivalentClass>
            <owl:Class>
                <owl:intersectionOf rdf:parseType="Collection">
                    <rdf:Description rdf:about="https://hack.cybersystems.engineer/memex/ontologies/SeamlessDigitalEngineering#Product_Interaction_Capability"/>
                    <owl:Restriction>
                        <owl:onProperty rdf:resource="http://purl.obolibrary.org/obo/BFO_0000178"/>
                        <owl:someValuesFrom>
                            <owl:Class>
                                <owl:intersectionOf rdf:parseType="Collection">
                                    <rdf:Description rdf:about="https://hack.cybersystems.engineer/memex/ontologies/SeamlessDigitalEngineering#Product_Compatibility"/>
                                    <rdf:Description rdf:about="https://hack.cybersystems.engineer/memex/ontologies/SeamlessDigitalEngineering#Product_Functional_Appropriateness"/>
                                    <rdf:Description rdf:about="https://hack.cybersystems.engineer/memex/ontologies/SeamlessDigitalEngineering#Product_Functional_Completeness"/>
                                </owl:intersectionOf>
                            </owl:Class>
                        </owl:someValuesFrom>
                    </owl:Restriction>
                    <owl:Restriction>
                        <owl:onProperty rdf:resource="http://purl.obolibrary.org/obo/BFO_0000195"/>
                        <owl:someValuesFrom rdf:resource="https://hack.cybersystems.engineer/memex/ontologies/SeamlessDigitalEngineering#Seamless_Integration"/>
                    </owl:Restriction>
                </owl:intersectionOf>
            </owl:Class>
        </owl:equivalentClass>
        <rdfs:subClassOf rdf:resource="https://hack.cybersystems.engineer/memex/ontologies/SeamlessDigitalEngineering#Product_Capability"/>
        <rdfs:label xml:lang="en">Seamless Interaction Capability</rdfs:label>
        <skos:definition xml:lang="en">perfectly consistent and coherent Product Interaction Capability, to the extent made possible by Seamless Integration</skos:definition>
        <cco2:ont00001754 xml:lang="en">Princeton WordNet</cco2:ont00001754>
    </owl:Class>
    


    <!-- https://hack.cybersystems.engineer/memex/ontologies/SeamlessDigitalEngineering#Seamless_Interface -->

    <owl:Class rdf:about="https://hack.cybersystems.engineer/memex/ontologies/SeamlessDigitalEngineering#Seamless_Interface">
        <owl:equivalentClass>
            <owl:Class>
                <owl:intersectionOf rdf:parseType="Collection">
                    <rdf:Description rdf:about="https://hack.cybersystems.engineer/memex/ontologies/SeamlessDigitalEngineering#Interface"/>
                    <owl:Restriction>
                        <owl:onProperty rdf:resource="http://purl.obolibrary.org/obo/BFO_0000178"/>
                        <owl:someValuesFrom rdf:resource="https://hack.cybersystems.engineer/memex/ontologies/SeamlessDigitalEngineering#Proof_Certificate"/>
                    </owl:Restriction>
                    <owl:Restriction>
                        <owl:onProperty rdf:resource="https://www.commoncoreontologies.org/ont00001920"/>
                        <owl:someValuesFrom rdf:resource="https://hack.cybersystems.engineer/memex/ontologies/SeamlessDigitalEngineering#System_Architecture_Model"/>
                    </owl:Restriction>
                    <owl:Restriction>
                        <owl:onProperty rdf:resource="https://www.commoncoreontologies.org/ont00001936"/>
                        <owl:someValuesFrom rdf:resource="https://hack.cybersystems.engineer/memex/ontologies/SeamlessDigitalEngineering#Act_of_Formal_Verification"/>
                    </owl:Restriction>
                </owl:intersectionOf>
            </owl:Class>
        </owl:equivalentClass>
        <rdfs:subClassOf rdf:resource="https://hack.cybersystems.engineer/memex/ontologies/SeamlessDigitalEngineering#Interface"/>
        <rdfs:comment xml:lang="en">TODO: model secondary &apos;equivalent to&apos; axiom that relates the concept to SysML v2</rdfs:comment>
        <rdfs:label xml:lang="en">Seamless Interface</rdfs:label>
        <skos:definition xml:lang="en">An Interface prescribed by a System Architecture Model which is the object of an Act of Formal Verification that produces a Proof Certificate of its (Product) Functional Correctness.</skos:definition>
    </owl:Class>
    


    <!-- https://hack.cybersystems.engineer/memex/ontologies/SeamlessDigitalEngineering#Seamless_Quality-in-Use -->

    <owl:Class rdf:about="https://hack.cybersystems.engineer/memex/ontologies/SeamlessDigitalEngineering#Seamless_Quality-in-Use">
        <owl:equivalentClass>
            <owl:Class>
                <owl:intersectionOf rdf:parseType="Collection">
                    <rdf:Description rdf:about="https://hack.cybersystems.engineer/memex/ontologies/SeamlessDigitalEngineering#Product_Quality-in-Use"/>
                    <owl:Restriction>
                        <owl:onProperty rdf:resource="http://purl.obolibrary.org/obo/BFO_0000178"/>
                        <owl:someValuesFrom>
                            <owl:Class>
                                <owl:intersectionOf rdf:parseType="Collection">
                                    <rdf:Description rdf:about="https://hack.cybersystems.engineer/memex/ontologies/SeamlessDigitalEngineering#Experience"/>
                                    <rdf:Description rdf:about="https://hack.cybersystems.engineer/memex/ontologies/SeamlessDigitalEngineering#Suitability"/>
                                    <rdf:Description rdf:about="https://hack.cybersystems.engineer/memex/ontologies/SeamlessDigitalEngineering#Trustworthiness"/>
                                    <rdf:Description rdf:about="https://hack.cybersystems.engineer/memex/ontologies/SeamlessDigitalEngineering#Usability"/>
                                </owl:intersectionOf>
                            </owl:Class>
                        </owl:someValuesFrom>
                    </owl:Restriction>
                    <owl:Restriction>
                        <owl:onProperty rdf:resource="http://purl.obolibrary.org/obo/BFO_0000195"/>
                        <owl:someValuesFrom>
                            <owl:Class>
                                <owl:intersectionOf rdf:parseType="Collection">
                                    <rdf:Description rdf:about="https://hack.cybersystems.engineer/memex/ontologies/SeamlessDigitalEngineering#Seamless_Integration"/>
                                    <rdf:Description rdf:about="https://hack.cybersystems.engineer/memex/ontologies/SeamlessDigitalEngineering#Seamless_Interaction_Capability"/>
                                </owl:intersectionOf>
                            </owl:Class>
                        </owl:someValuesFrom>
                    </owl:Restriction>
                </owl:intersectionOf>
            </owl:Class>
        </owl:equivalentClass>
        <rdfs:subClassOf rdf:resource="https://hack.cybersystems.engineer/memex/ontologies/SeamlessDigitalEngineering#Product_Quality-in-Use"/>
        <rdfs:label xml:lang="en">Seamless Quality-in-Use</rdfs:label>
        <skos:definition xml:lang="en">A composite Quality-in-Use comprising Experience, Suitability, Trustworthiness, and Usability, and which specifically depends on Seamless Integration and Seamless Interaction Capability Product Capabilities.</skos:definition>
    </owl:Class>
    


    <!-- https://hack.cybersystems.engineer/memex/ontologies/SeamlessDigitalEngineering#Seamless_Quality_Claim -->

    <owl:Class rdf:about="https://hack.cybersystems.engineer/memex/ontologies/SeamlessDigitalEngineering#Seamless_Quality_Claim">
        <owl:equivalentClass>
            <owl:Class>
                <owl:intersectionOf rdf:parseType="Collection">
                    <rdf:Description rdf:about="https://hack.cybersystems.engineer/memex/ontologies/SeamlessDigitalEngineering#Quality_Claim"/>
                    <owl:Restriction>
                        <owl:onProperty rdf:resource="https://www.commoncoreontologies.org/ont00001942"/>
                        <owl:someValuesFrom rdf:resource="https://hack.cybersystems.engineer/memex/ontologies/SeamlessDigitalEngineering#Seamless_Integration"/>
                    </owl:Restriction>
                    <owl:Restriction>
                        <owl:onProperty rdf:resource="https://www.commoncoreontologies.org/ont00001942"/>
                        <owl:someValuesFrom rdf:resource="https://hack.cybersystems.engineer/memex/ontologies/SeamlessDigitalEngineering#Seamless_Interaction_Capability"/>
                    </owl:Restriction>
                    <owl:Restriction>
                        <owl:onProperty rdf:resource="https://www.commoncoreontologies.org/ont00001942"/>
                        <owl:someValuesFrom rdf:resource="https://hack.cybersystems.engineer/memex/ontologies/SeamlessDigitalEngineering#Seamless_Quality-in-Use"/>
                    </owl:Restriction>
                </owl:intersectionOf>
            </owl:Class>
        </owl:equivalentClass>
        <rdfs:subClassOf rdf:resource="https://hack.cybersystems.engineer/memex/ontologies/SeamlessDigitalEngineering#Quality_Claim"/>
        <rdfs:label xml:lang="en">Seamless Quality Claim</rdfs:label>
        <skos:definition xml:lang="en">A Quality Claim that prescribes Seamless Integration, Seamless Interaction Capability, and Seamless Quality-in-Use of some System-of-Interest</skos:definition>
    </owl:Class>
    


    <!-- https://hack.cybersystems.engineer/memex/ontologies/SeamlessDigitalEngineering#Security_Architecture -->

    <owl:Class rdf:about="https://hack.cybersystems.engineer/memex/ontologies/SeamlessDigitalEngineering#Security_Architecture">
        <rdfs:subClassOf rdf:resource="https://hack.cybersystems.engineer/memex/ontologies/SeamlessDigitalEngineering#Architecture_View"/>
        <rdfs:label xml:lang="en">Security Architecture</rdfs:label>
        <skos:altLabel xml:lang="en">Security (View of) Architecture</skos:altLabel>
        <skos:definition xml:lang="en">when the associated viewpoint is dealing with security</skos:definition>
        <cco2:ont00001754 xml:lang="en">derived from ISO/IEC/IEEE 42020:2019</cco2:ont00001754>
    </owl:Class>
    


    <!-- https://hack.cybersystems.engineer/memex/ontologies/SeamlessDigitalEngineering#Security_Assurance -->

    <owl:Class rdf:about="https://hack.cybersystems.engineer/memex/ontologies/SeamlessDigitalEngineering#Security_Assurance">
        <owl:equivalentClass>
            <owl:Class>
                <owl:intersectionOf rdf:parseType="Collection">
                    <rdf:Description rdf:about="https://hack.cybersystems.engineer/memex/ontologies/SeamlessDigitalEngineering#Assurance"/>
                    <owl:Restriction>
                        <owl:onProperty rdf:resource="https://www.commoncoreontologies.org/ont00001801"/>
                        <owl:someValuesFrom rdf:resource="https://hack.cybersystems.engineer/memex/ontologies/SeamlessDigitalEngineering#Security_Functional_Requirement"/>
                    </owl:Restriction>
                </owl:intersectionOf>
            </owl:Class>
        </owl:equivalentClass>
        <rdfs:subClassOf rdf:resource="https://hack.cybersystems.engineer/memex/ontologies/SeamlessDigitalEngineering#Assurance"/>
        <rdfs:label xml:lang="en">Security Assurance</rdfs:label>
        <skos:definition xml:lang="en">Assurance that a Target of Evaluation meets the Security Functional Requirements</skos:definition>
        <cco2:ont00001754 xml:lang="en">ISO/IEC 15408-1:2022, 3.6
Information security, cybersecurity and privacy protection - Evaluation criteria for IT security - Part 1: Introduction and general model</cco2:ont00001754>
    </owl:Class>
    


    <!-- https://hack.cybersystems.engineer/memex/ontologies/SeamlessDigitalEngineering#Security_Assurance_Requirement -->

    <owl:Class rdf:about="https://hack.cybersystems.engineer/memex/ontologies/SeamlessDigitalEngineering#Security_Assurance_Requirement">
        <owl:equivalentClass>
            <owl:Class>
                <owl:intersectionOf rdf:parseType="Collection">
                    <rdf:Description rdf:about="https://hack.cybersystems.engineer/memex/ontologies/SeamlessDigitalEngineering#Assurance_Requirement"/>
                    <rdf:Description rdf:about="https://hack.cybersystems.engineer/memex/ontologies/SeamlessDigitalEngineering#Security_Requirement"/>
                </owl:intersectionOf>
            </owl:Class>
        </owl:equivalentClass>
        <rdfs:subClassOf rdf:resource="https://hack.cybersystems.engineer/memex/ontologies/SeamlessDigitalEngineering#Assurance_Requirement"/>
        <rdfs:subClassOf rdf:resource="https://hack.cybersystems.engineer/memex/ontologies/SeamlessDigitalEngineering#Security_Requirement"/>
        <rdfs:label xml:lang="en">Security Assurance Requirement</rdfs:label>
        <skos:definition xml:lang="en">Security Requirement that prescribes the Conditions, Supply Process, and Technical Processes of the Target of Evaluation Lifecycle, and the Actions required of Evaluators with respect to Evidence produced from these Conditions and System Lifecycle Processes</skos:definition>
        <cco2:ont00001754 xml:lang="en">ISO/IEC 15408-1:2022</cco2:ont00001754>
    </owl:Class>
    


    <!-- https://hack.cybersystems.engineer/memex/ontologies/SeamlessDigitalEngineering#Security_Functional_Requirement -->

    <owl:Class rdf:about="https://hack.cybersystems.engineer/memex/ontologies/SeamlessDigitalEngineering#Security_Functional_Requirement">
        <owl:equivalentClass>
            <owl:Class>
                <owl:intersectionOf rdf:parseType="Collection">
                    <rdf:Description rdf:about="https://hack.cybersystems.engineer/memex/ontologies/SeamlessDigitalEngineering#Functional_Requirement"/>
                    <rdf:Description rdf:about="https://hack.cybersystems.engineer/memex/ontologies/SeamlessDigitalEngineering#Security_Requirement"/>
                    <owl:Restriction>
                        <owl:onProperty rdf:resource="https://www.commoncoreontologies.org/ont00001808"/>
                        <owl:someValuesFrom rdf:resource="https://hack.cybersystems.engineer/memex/ontologies/SeamlessDigitalEngineering#Security_Problem_Definition"/>
                    </owl:Restriction>
                    <owl:Restriction>
                        <owl:onProperty rdf:resource="https://www.commoncoreontologies.org/ont00001942"/>
                        <owl:someValuesFrom rdf:resource="https://hack.cybersystems.engineer/memex/ontologies/SeamlessDigitalEngineering#Target_of_Evaluation"/>
                    </owl:Restriction>
                </owl:intersectionOf>
            </owl:Class>
        </owl:equivalentClass>
        <rdfs:subClassOf rdf:resource="https://hack.cybersystems.engineer/memex/ontologies/SeamlessDigitalEngineering#Functional_Requirement"/>
        <rdfs:subClassOf rdf:resource="https://hack.cybersystems.engineer/memex/ontologies/SeamlessDigitalEngineering#Security_Requirement"/>
        <rdfs:label xml:lang="en">Security Functional Requirement</rdfs:label>
        <skos:definition xml:lang="en">Security Requirement, which contributes to fulfil the Target of Evaluation Security Problem Definition as defined in a specific Security Target or in a Protection Profile</skos:definition>
        <cco2:ont00001754 xml:lang="en">ISO/IEC 15408-1:2022</cco2:ont00001754>
    </owl:Class>
    


    <!-- https://hack.cybersystems.engineer/memex/ontologies/SeamlessDigitalEngineering#Security_Problem_Definition -->

    <owl:Class rdf:about="https://hack.cybersystems.engineer/memex/ontologies/SeamlessDigitalEngineering#Security_Problem_Definition">
        <owl:equivalentClass>
            <owl:Class>
                <owl:intersectionOf rdf:parseType="Collection">
                    <rdf:Description rdf:about="https://hack.cybersystems.engineer/memex/ontologies/SeamlessDigitalEngineering#Problem_Definition"/>
                    <owl:Restriction>
                        <owl:onProperty rdf:resource="https://www.commoncoreontologies.org/ont00001808"/>
                        <owl:someValuesFrom>
                            <owl:Class>
                                <owl:intersectionOf rdf:parseType="Collection">
                                    <rdf:Description rdf:about="https://hack.cybersystems.engineer/memex/ontologies/SeamlessDigitalEngineering#Operational_Environment"/>
                                    <rdf:Description rdf:about="https://hack.cybersystems.engineer/memex/ontologies/SeamlessDigitalEngineering#Target_of_Evaluation"/>
                                </owl:intersectionOf>
                            </owl:Class>
                        </owl:someValuesFrom>
                    </owl:Restriction>
                    <owl:Restriction>
                        <owl:onProperty rdf:resource="https://www.commoncoreontologies.org/ont00001982"/>
                        <owl:someValuesFrom rdf:resource="https://hack.cybersystems.engineer/memex/ontologies/SeamlessDigitalEngineering#Product_Security"/>
                    </owl:Restriction>
                    <owl:Restriction>
                        <owl:onProperty rdf:resource="https://www.commoncoreontologies.org/ont00001982"/>
                        <owl:someValuesFrom rdf:resource="https://hack.cybersystems.engineer/memex/ontologies/SeamlessDigitalEngineering#Threat"/>
                    </owl:Restriction>
                </owl:intersectionOf>
            </owl:Class>
        </owl:equivalentClass>
        <rdfs:subClassOf rdf:resource="https://hack.cybersystems.engineer/memex/ontologies/SeamlessDigitalEngineering#Problem_Definition"/>
        <rdfs:comment xml:lang="en">This statement consists of a combination of: Threats to be countered by the TOE and its Operational Environment, the Organizational Security Policies enforced by the TOE and its Operational Environment, and the Assumptions that are upheld for the Operational Environment of the TOE.</rdfs:comment>
        <rdfs:label xml:lang="en">Security Problem Definition</rdfs:label>
        <skos:definition xml:lang="en">Problem Definition, which in a formal manner defines the nature and scope of the Product Security that the Target of Evaluation is intended to address</skos:definition>
        <cco2:ont00001754 xml:lang="en">ISO/IEC 15408-1:2022</cco2:ont00001754>
    </owl:Class>
    


    <!-- https://hack.cybersystems.engineer/memex/ontologies/SeamlessDigitalEngineering#Security_Requirement -->

    <owl:Class rdf:about="https://hack.cybersystems.engineer/memex/ontologies/SeamlessDigitalEngineering#Security_Requirement">
        <owl:equivalentClass>
            <owl:Class>
                <owl:intersectionOf rdf:parseType="Collection">
                    <rdf:Description rdf:about="https://hack.cybersystems.engineer/memex/ontologies/SeamlessDigitalEngineering#Quality_Requirement"/>
                    <owl:Restriction>
                        <owl:onProperty rdf:resource="https://www.commoncoreontologies.org/ont00001942"/>
                        <owl:someValuesFrom rdf:resource="https://hack.cybersystems.engineer/memex/ontologies/SeamlessDigitalEngineering#Product_Security"/>
                    </owl:Restriction>
                </owl:intersectionOf>
            </owl:Class>
        </owl:equivalentClass>
        <rdfs:subClassOf rdf:resource="https://hack.cybersystems.engineer/memex/ontologies/SeamlessDigitalEngineering#Quality_Requirement"/>
        <rdfs:label xml:lang="en">Security Requirement</rdfs:label>
        <skos:definition xml:lang="en">Requirement, which is part of a Target of Evaluation security specification as defined in a specific Security Target or in a Protection Profile</skos:definition>
        <cco2:ont00001754 xml:lang="en">ISO/IEC 15408-1:2022</cco2:ont00001754>
    </owl:Class>
    


    <!-- https://hack.cybersystems.engineer/memex/ontologies/SeamlessDigitalEngineering#Security_Target -->

    <owl:Class rdf:about="https://hack.cybersystems.engineer/memex/ontologies/SeamlessDigitalEngineering#Security_Target">
        <rdfs:subClassOf rdf:resource="https://hack.cybersystems.engineer/memex/ontologies/SeamlessDigitalEngineering#Security_Viewpoint"/>
        <rdfs:label xml:lang="en">Security Target</rdfs:label>
        <skos:definition xml:lang="en">implementation-dependent statement of Security Requirements for a Target of Evaluation based on a Security Problem Definition</skos:definition>
        <cco2:ont00001754 xml:lang="en">ISO/IEC 15408-1:2022</cco2:ont00001754>
    </owl:Class>
    


    <!-- https://hack.cybersystems.engineer/memex/ontologies/SeamlessDigitalEngineering#Security_Viewpoint -->

    <owl:Class rdf:about="https://hack.cybersystems.engineer/memex/ontologies/SeamlessDigitalEngineering#Security_Viewpoint">
        <owl:equivalentClass>
            <owl:Class>
                <owl:intersectionOf rdf:parseType="Collection">
                    <rdf:Description rdf:about="https://hack.cybersystems.engineer/memex/ontologies/SeamlessDigitalEngineering#Architecture_Viewpoint"/>
                    <owl:Restriction>
                        <owl:onProperty rdf:resource="https://www.commoncoreontologies.org/ont00001942"/>
                        <owl:someValuesFrom rdf:resource="https://hack.cybersystems.engineer/memex/ontologies/SeamlessDigitalEngineering#Security_Architecture"/>
                    </owl:Restriction>
                </owl:intersectionOf>
            </owl:Class>
        </owl:equivalentClass>
        <rdfs:subClassOf rdf:resource="https://hack.cybersystems.engineer/memex/ontologies/SeamlessDigitalEngineering#Architecture_Viewpoint"/>
        <rdfs:label xml:lang="en">Security Viewpoint</rdfs:label>
        <skos:definition xml:lang="en">An architecture viewpoint focused on &quot;protection against intentional subversion or forced failure&quot;</skos:definition>
        <cco2:ont00001754 xml:lang="en">derived from ISO/IEC/IEEE 15288:2023 definition of &apos;security&apos;</cco2:ont00001754>
    </owl:Class>
    


    <!-- https://hack.cybersystems.engineer/memex/ontologies/SeamlessDigitalEngineering#Service -->

    <owl:Class rdf:about="https://hack.cybersystems.engineer/memex/ontologies/SeamlessDigitalEngineering#Service">
        <owl:equivalentClass>
            <owl:Class>
                <owl:intersectionOf rdf:parseType="Collection">
                    <rdf:Description rdf:about="https://hack.cybersystems.engineer/memex/ontologies/SeamlessDigitalEngineering#Capability"/>
                    <owl:Restriction>
                        <owl:onProperty rdf:resource="https://www.commoncoreontologies.org/ont00001816"/>
                        <owl:someValuesFrom rdf:resource="https://hack.cybersystems.engineer/memex/ontologies/SeamlessDigitalEngineering#Activity"/>
                    </owl:Restriction>
                </owl:intersectionOf>
            </owl:Class>
        </owl:equivalentClass>
        <rdfs:subClassOf rdf:resource="https://hack.cybersystems.engineer/memex/ontologies/SeamlessDigitalEngineering#Capability"/>
        <skos:definition xml:lang="en">[Capability] of an Organization with at least one Activity necessarily performed between the Organization and the Customer</skos:definition>
        <cco2:ont00001754>ISO/IEC/IEEE 15288:2023</cco2:ont00001754>
    </owl:Class>
    


    <!-- https://hack.cybersystems.engineer/memex/ontologies/SeamlessDigitalEngineering#Service_Report -->

    <owl:Class rdf:about="https://hack.cybersystems.engineer/memex/ontologies/SeamlessDigitalEngineering#Service_Report">
        <rdfs:subClassOf rdf:resource="https://www.commoncoreontologies.org/ont00000624"/>
    </owl:Class>
    


    <!-- https://hack.cybersystems.engineer/memex/ontologies/SeamlessDigitalEngineering#Services_Architecture -->

    <owl:Class rdf:about="https://hack.cybersystems.engineer/memex/ontologies/SeamlessDigitalEngineering#Services_Architecture">
        <rdfs:subClassOf rdf:resource="https://hack.cybersystems.engineer/memex/ontologies/SeamlessDigitalEngineering#Architecture_View"/>
        <rdfs:label xml:lang="en">Services Architecture</rdfs:label>
        <skos:altLabel xml:lang="en">Services (View of) Architecture</skos:altLabel>
        <skos:definition xml:lang="en">when the associated viewpoint is dealing with services</skos:definition>
        <cco2:ont00001754 xml:lang="en">ISO/IEC/IEEE 42020:2019</cco2:ont00001754>
    </owl:Class>
    


    <!-- https://hack.cybersystems.engineer/memex/ontologies/SeamlessDigitalEngineering#Services_Viewpoint -->

    <owl:Class rdf:about="https://hack.cybersystems.engineer/memex/ontologies/SeamlessDigitalEngineering#Services_Viewpoint">
        <owl:equivalentClass>
            <owl:Class>
                <owl:intersectionOf rdf:parseType="Collection">
                    <rdf:Description rdf:about="https://hack.cybersystems.engineer/memex/ontologies/SeamlessDigitalEngineering#Architecture_Viewpoint"/>
                    <owl:Restriction>
                        <owl:onProperty rdf:resource="https://www.commoncoreontologies.org/ont00001942"/>
                        <owl:someValuesFrom rdf:resource="https://hack.cybersystems.engineer/memex/ontologies/SeamlessDigitalEngineering#Services_Architecture"/>
                    </owl:Restriction>
                </owl:intersectionOf>
            </owl:Class>
        </owl:equivalentClass>
        <rdfs:subClassOf rdf:resource="https://hack.cybersystems.engineer/memex/ontologies/SeamlessDigitalEngineering#Architecture_Viewpoint"/>
        <rdfs:label xml:lang="en">Services Viewpoint</rdfs:label>
        <skos:definition xml:lang="en">An architecture viewpoint focused on &quot;output of an Organization with at least one Activity necessarily performed between the Organization and the Customer&quot;</skos:definition>
        <cco2:ont00001754 xml:lang="en">derived from ISO/IEC/IEEE 15288:2023 definition of &apos;service&apos;</cco2:ont00001754>
    </owl:Class>
    


    <!-- https://hack.cybersystems.engineer/memex/ontologies/SeamlessDigitalEngineering#Set_Theory_Discipline -->

    <owl:Class rdf:about="https://hack.cybersystems.engineer/memex/ontologies/SeamlessDigitalEngineering#Set_Theory_Discipline">
        <rdfs:subClassOf rdf:resource="https://hack.cybersystems.engineer/memex/ontologies/SeamlessDigitalEngineering#Mathematical_Logic_Discipline"/>
        <rdfs:label xml:lang="en">Set Theory Discipline</rdfs:label>
    </owl:Class>
    


    <!-- https://hack.cybersystems.engineer/memex/ontologies/SeamlessDigitalEngineering#Severity -->

    <owl:Class rdf:about="https://hack.cybersystems.engineer/memex/ontologies/SeamlessDigitalEngineering#Severity">
        <owl:equivalentClass>
            <owl:Class>
                <owl:intersectionOf rdf:parseType="Collection">
                    <rdf:Description rdf:about="https://www.commoncoreontologies.org/ont00001176"/>
                    <owl:Restriction>
                        <owl:onProperty rdf:resource="https://www.commoncoreontologies.org/ont00001966"/>
                        <owl:someValuesFrom>
                            <owl:Class>
                                <owl:unionOf rdf:parseType="Collection">
                                    <rdf:Description rdf:about="https://hack.cybersystems.engineer/memex/ontologies/SeamlessDigitalEngineering#Error"/>
                                    <rdf:Description rdf:about="https://hack.cybersystems.engineer/memex/ontologies/SeamlessDigitalEngineering#Failure"/>
                                </owl:unionOf>
                            </owl:Class>
                        </owl:someValuesFrom>
                    </owl:Restriction>
                </owl:intersectionOf>
            </owl:Class>
        </owl:equivalentClass>
        <rdfs:subClassOf rdf:resource="https://www.commoncoreontologies.org/ont00001176"/>
        <rdfs:label xml:lang="en">Severity</rdfs:label>
        <skos:definition xml:lang="en">measure of a Failure or Error according to the magnitude of its possible Consequences</skos:definition>
        <cco2:ont00001754 xml:lang="en">derived from ISO 10795:2019(en) - Space systems - Programme management and quality - Vocabulary</cco2:ont00001754>
    </owl:Class>
    


    <!-- https://hack.cybersystems.engineer/memex/ontologies/SeamlessDigitalEngineering#Socio-Technical_System -->

    <owl:Class rdf:about="https://hack.cybersystems.engineer/memex/ontologies/SeamlessDigitalEngineering#Socio-Technical_System">
        <rdfs:subClassOf rdf:resource="https://hack.cybersystems.engineer/memex/ontologies/SeamlessDigitalEngineering#System"/>
        <rdfs:label xml:lang="en">Socio-technical System</rdfs:label>
    </owl:Class>
    


    <!-- https://hack.cybersystems.engineer/memex/ontologies/SeamlessDigitalEngineering#Software_Architecture -->

    <owl:Class rdf:about="https://hack.cybersystems.engineer/memex/ontologies/SeamlessDigitalEngineering#Software_Architecture">
        <owl:equivalentClass>
            <owl:Class>
                <owl:intersectionOf rdf:parseType="Collection">
                    <rdf:Description rdf:about="https://hack.cybersystems.engineer/memex/ontologies/SeamlessDigitalEngineering#System_Architecture_Model"/>
                    <owl:Restriction>
                        <owl:onProperty rdf:resource="http://purl.obolibrary.org/obo/BFO_0000178"/>
                        <owl:someValuesFrom rdf:resource="http://www.ontologyrepository.com/CommonCoreOntologies/ComputerProgramArtifactModel"/>
                    </owl:Restriction>
                </owl:intersectionOf>
            </owl:Class>
        </owl:equivalentClass>
        <rdfs:subClassOf rdf:resource="https://hack.cybersystems.engineer/memex/ontologies/SeamlessDigitalEngineering#System_Architecture_Model"/>
        <rdfs:label xml:lang="en">Software Architecture</rdfs:label>
        <skos:definition xml:lang="en">System Architecture of a System-of-Interest where all System Elements are Computer Programs or Software Libraries</skos:definition>
    </owl:Class>
    


    <!-- https://hack.cybersystems.engineer/memex/ontologies/SeamlessDigitalEngineering#Software_Engineer -->

    <owl:Class rdf:about="https://hack.cybersystems.engineer/memex/ontologies/SeamlessDigitalEngineering#Software_Engineer">
        <rdfs:subClassOf rdf:resource="https://hack.cybersystems.engineer/memex/ontologies/SeamlessDigitalEngineering#Engineer"/>
        <rdfs:label xml:lang="en">Software Engineer</rdfs:label>
    </owl:Class>
    


    <!-- https://hack.cybersystems.engineer/memex/ontologies/SeamlessDigitalEngineering#Software_Product -->

    <owl:Class rdf:about="https://hack.cybersystems.engineer/memex/ontologies/SeamlessDigitalEngineering#Software_Product">
        <owl:equivalentClass>
            <owl:Class>
                <owl:intersectionOf rdf:parseType="Collection">
                    <rdf:Description rdf:about="http://www.ontologyrepository.com/CommonCoreOntologies/ComputerProgram"/>
                    <owl:Restriction>
                        <owl:onProperty rdf:resource="http://purl.obolibrary.org/obo/BFO_0000129"/>
                        <owl:someValuesFrom rdf:resource="https://www.commoncoreontologies.org/ont00000420"/>
                    </owl:Restriction>
                </owl:intersectionOf>
            </owl:Class>
        </owl:equivalentClass>
        <rdfs:subClassOf rdf:resource="http://www.ontologyrepository.com/CommonCoreOntologies/ComputerProgram"/>
        <rdfs:subClassOf rdf:resource="https://hack.cybersystems.engineer/memex/ontologies/SeamlessDigitalEngineering#Product"/>
        <rdfs:label xml:lang="en">Software Product</rdfs:label>
    </owl:Class>
    


    <!-- https://hack.cybersystems.engineer/memex/ontologies/SeamlessDigitalEngineering#Software_Unit_Test_Report -->

    <owl:Class rdf:about="https://hack.cybersystems.engineer/memex/ontologies/SeamlessDigitalEngineering#Software_Unit_Test_Report">
        <rdfs:subClassOf rdf:resource="https://hack.cybersystems.engineer/memex/ontologies/SeamlessDigitalEngineering#Integration_and_Test_Report"/>
    </owl:Class>
    


    <!-- https://hack.cybersystems.engineer/memex/ontologies/SeamlessDigitalEngineering#Source_of_Truth_Role -->

    <owl:Class rdf:about="https://hack.cybersystems.engineer/memex/ontologies/SeamlessDigitalEngineering#Source_of_Truth_Role">
        <owl:equivalentClass>
            <owl:Class>
                <owl:intersectionOf rdf:parseType="Collection">
                    <rdf:Description rdf:about="http://purl.obolibrary.org/obo/BFO_0000023"/>
                    <owl:Restriction>
                        <owl:onProperty rdf:resource="http://purl.obolibrary.org/obo/BFO_0000197"/>
                        <owl:someValuesFrom rdf:resource="https://www.commoncoreontologies.org/ont00000798"/>
                    </owl:Restriction>
                </owl:intersectionOf>
            </owl:Class>
        </owl:equivalentClass>
        <rdfs:subClassOf rdf:resource="http://purl.obolibrary.org/obo/BFO_0000023"/>
        <rdfs:label xml:lang="en">Source of Truth Role</rdfs:label>
        <skos:altLabel xml:lang="en">SoT Role</skos:altLabel>
        <skos:definition xml:lang="en">A role that inheres in an Information Bearing Artifact that establishes it as a source of truth for the Information Content Entit(ies) it carries in a particular Context of Use</skos:definition>
        <cco2:ont00001760 rdf:datatype="http://www.w3.org/2001/XMLSchema#anyURI">https://semantic.incose.org/DEIX_Ontology</cco2:ont00001760>
    </owl:Class>
    


    <!-- https://hack.cybersystems.engineer/memex/ontologies/SeamlessDigitalEngineering#Stack_Programming_Language -->

    <owl:Class rdf:about="https://hack.cybersystems.engineer/memex/ontologies/SeamlessDigitalEngineering#Stack_Programming_Language">
        <rdfs:subClassOf rdf:resource="http://www.ontologyrepository.com/CommonCoreOntologies/HighLevelProgrammingLanguage"/>
        <rdfs:label xml:lang="en">Stack Programming Language</rdfs:label>
    </owl:Class>
    


    <!-- https://hack.cybersystems.engineer/memex/ontologies/SeamlessDigitalEngineering#Stakeholder -->

    <owl:Class rdf:about="https://hack.cybersystems.engineer/memex/ontologies/SeamlessDigitalEngineering#Stakeholder">
        <owl:equivalentClass>
            <owl:Class>
                <owl:intersectionOf rdf:parseType="Collection">
                    <owl:Class>
                        <owl:unionOf rdf:parseType="Collection">
                            <rdf:Description rdf:about="https://www.commoncoreontologies.org/ont00001017"/>
                            <rdf:Description rdf:about="https://www.commoncoreontologies.org/ont00001180"/>
                        </owl:unionOf>
                    </owl:Class>
                    <owl:Class>
                        <owl:unionOf rdf:parseType="Collection">
                            <owl:Restriction>
                                <owl:onProperty rdf:resource="https://www.commoncoreontologies.org/ont00001787"/>
                                <owl:someValuesFrom rdf:resource="https://hack.cybersystems.engineer/memex/ontologies/SeamlessDigitalEngineering#Lifecycle"/>
                            </owl:Restriction>
                            <owl:Restriction>
                                <owl:onProperty rdf:resource="https://www.commoncoreontologies.org/ont00001984"/>
                                <owl:someValuesFrom rdf:resource="https://hack.cybersystems.engineer/memex/ontologies/SeamlessDigitalEngineering#Lifecycle"/>
                            </owl:Restriction>
                        </owl:unionOf>
                    </owl:Class>
                    <owl:Restriction>
                        <owl:onProperty rdf:resource="http://purl.obolibrary.org/obo/BFO_0000196"/>
                        <owl:someValuesFrom rdf:resource="https://hack.cybersystems.engineer/memex/ontologies/SeamlessDigitalEngineering#Concern_Disposition"/>
                    </owl:Restriction>
                    <owl:Restriction>
                        <owl:onProperty rdf:resource="http://purl.obolibrary.org/obo/BFO_0000196"/>
                        <owl:someValuesFrom rdf:resource="https://hack.cybersystems.engineer/memex/ontologies/SeamlessDigitalEngineering#Stakeholder_Role"/>
                    </owl:Restriction>
                    <owl:Restriction>
                        <owl:onProperty rdf:resource="https://www.commoncoreontologies.org/ont00001801"/>
                        <owl:someValuesFrom rdf:resource="https://hack.cybersystems.engineer/memex/ontologies/SeamlessDigitalEngineering#Need"/>
                    </owl:Restriction>
                </owl:intersectionOf>
            </owl:Class>
        </owl:equivalentClass>
        <rdfs:subClassOf rdf:resource="https://www.commoncoreontologies.org/ont00001017"/>
        <rdfs:label xml:lang="en">Stakeholder</rdfs:label>
        <skos:definition xml:lang="en">individual or Organization having a right, share, claim, or interest in a System or in its possession of characteristics that meet their Needs and expectations</skos:definition>
        <cco2:ont00001754>ISO/IEC/IEEE 15288:2023</cco2:ont00001754>
        <cco2:ont00001760 rdf:datatype="http://www.w3.org/2001/XMLSchema#anyURI">https://semantic.incose.org/DEIX_Ontology</cco2:ont00001760>
    </owl:Class>
    


    <!-- https://hack.cybersystems.engineer/memex/ontologies/SeamlessDigitalEngineering#Stakeholder_Confidence -->

    <owl:Class rdf:about="https://hack.cybersystems.engineer/memex/ontologies/SeamlessDigitalEngineering#Stakeholder_Confidence">
        <owl:equivalentClass>
            <owl:Class>
                <owl:intersectionOf rdf:parseType="Collection">
                    <rdf:Description rdf:about="https://hack.cybersystems.engineer/memex/ontologies/SeamlessDigitalEngineering#Confidence"/>
                    <owl:Restriction>
                        <owl:onProperty rdf:resource="http://purl.obolibrary.org/obo/BFO_0000197"/>
                        <owl:someValuesFrom rdf:resource="https://hack.cybersystems.engineer/memex/ontologies/SeamlessDigitalEngineering#Stakeholder"/>
                    </owl:Restriction>
                </owl:intersectionOf>
            </owl:Class>
        </owl:equivalentClass>
        <rdfs:subClassOf rdf:resource="https://hack.cybersystems.engineer/memex/ontologies/SeamlessDigitalEngineering#Confidence"/>
        <rdfs:label xml:lang="en">Stakeholder Confidence</rdfs:label>
    </owl:Class>
    


    <!-- https://hack.cybersystems.engineer/memex/ontologies/SeamlessDigitalEngineering#Stakeholder_Needs_and_Requirements_Definition_Process -->

    <owl:Class rdf:about="https://hack.cybersystems.engineer/memex/ontologies/SeamlessDigitalEngineering#Stakeholder_Needs_and_Requirements_Definition_Process">
        <owl:equivalentClass>
            <owl:Restriction>
                <owl:onProperty rdf:resource="https://www.commoncoreontologies.org/ont00001986"/>
                <owl:someValuesFrom>
                    <owl:Class>
                        <owl:intersectionOf rdf:parseType="Collection">
                            <rdf:Description rdf:about="https://hack.cybersystems.engineer/memex/ontologies/SeamlessDigitalEngineering#Need_Set"/>
                            <rdf:Description rdf:about="https://hack.cybersystems.engineer/memex/ontologies/SeamlessDigitalEngineering#Requirement_Set"/>
                        </owl:intersectionOf>
                    </owl:Class>
                </owl:someValuesFrom>
            </owl:Restriction>
        </owl:equivalentClass>
        <rdfs:subClassOf rdf:resource="https://hack.cybersystems.engineer/memex/ontologies/SeamlessDigitalEngineering#Technical_Process"/>
        <rdfs:label xml:lang="en">Stakeholder Needs and Requirements Definition Process</rdfs:label>
        <skos:definition xml:lang="en">The purpose of the stakeholder needs and requirements definition process is to define the stakeholder needs and requirements for a system that can provide the capabilities needed by users and other stakeholders in a defined environment.</skos:definition>
        <cco2:ont00001754>ISO/IEC/IEEE 15288:2023</cco2:ont00001754>
    </owl:Class>
    


    <!-- https://hack.cybersystems.engineer/memex/ontologies/SeamlessDigitalEngineering#Stakeholder_Role -->

    <owl:Class rdf:about="https://hack.cybersystems.engineer/memex/ontologies/SeamlessDigitalEngineering#Stakeholder_Role">
        <rdfs:subClassOf rdf:resource="http://purl.obolibrary.org/obo/BFO_0000023"/>
        <rdfs:label xml:lang="en">Stakeholder Role</rdfs:label>
        <cco2:ont00001760 rdf:datatype="http://www.w3.org/2001/XMLSchema#anyURI">https://semantic.incose.org/DEIX_Ontology</cco2:ont00001760>
    </owl:Class>
    


    <!-- https://hack.cybersystems.engineer/memex/ontologies/SeamlessDigitalEngineering#Standards_Organization -->

    <owl:Class rdf:about="https://hack.cybersystems.engineer/memex/ontologies/SeamlessDigitalEngineering#Standards_Organization">
        <rdfs:subClassOf rdf:resource="https://www.commoncoreontologies.org/ont00001180"/>
        <rdfs:label xml:lang="en">Standards Organization</rdfs:label>
        <skos:altLabel xml:lang="en">standards body</skos:altLabel>
        <skos:altLabel xml:lang="en">standards developing organization (SDO)</skos:altLabel>
        <skos:altLabel xml:lang="en">standards setting organization (SSO)</skos:altLabel>
        <skos:definition xml:lang="en">A standards organization is an organization whose primary function is developing, coordinating, promulgating, revising, amending, reissuing, interpreting, or otherwise contributing to the usefulness of technical standards to those who employ them. Such an organization works to create uniformity across producers, consumers, government agencies, and other relevant parties regarding terminology, product specifications (e.g. size, including units of measure), protocols, and more.</skos:definition>
        <cco2:ont00001754 xml:lang="en">https://en.wikipedia.org/wiki/Standards_organization</cco2:ont00001754>
    </owl:Class>
    


    <!-- https://hack.cybersystems.engineer/memex/ontologies/SeamlessDigitalEngineering#Subsystem -->

    <owl:Class rdf:about="https://hack.cybersystems.engineer/memex/ontologies/SeamlessDigitalEngineering#Subsystem">
        <owl:equivalentClass>
            <owl:Class>
                <owl:intersectionOf rdf:parseType="Collection">
                    <rdf:Description rdf:about="https://hack.cybersystems.engineer/memex/ontologies/SeamlessDigitalEngineering#System"/>
                    <owl:Restriction>
                        <owl:onProperty rdf:resource="http://purl.obolibrary.org/obo/BFO_0000129"/>
                        <owl:someValuesFrom rdf:resource="https://hack.cybersystems.engineer/memex/ontologies/SeamlessDigitalEngineering#System"/>
                    </owl:Restriction>
                </owl:intersectionOf>
            </owl:Class>
        </owl:equivalentClass>
        <rdfs:subClassOf rdf:resource="https://hack.cybersystems.engineer/memex/ontologies/SeamlessDigitalEngineering#System"/>
        <rdfs:label xml:lang="en">Subsystem</rdfs:label>
    </owl:Class>
    


    <!-- https://hack.cybersystems.engineer/memex/ontologies/SeamlessDigitalEngineering#Suitability -->

    <owl:Class rdf:about="https://hack.cybersystems.engineer/memex/ontologies/SeamlessDigitalEngineering#Suitability">
        <rdfs:subClassOf rdf:resource="https://hack.cybersystems.engineer/memex/ontologies/SeamlessDigitalEngineering#Beneficialness"/>
        <rdfs:label xml:lang="en">Suitability</rdfs:label>
        <skos:definition xml:lang="en">extent to which behaviours or outcomes, or both, of a Product meet (satisfy) specified Quality Requirements when used</skos:definition>
        <cco2:ont00001754 xml:lang="en">ISO/IEC 25019:2023(en)
Systems and software engineering — Systems and software Quality Requirements and Evaluation (SQuaRE) — Quality-in-use model</cco2:ont00001754>
    </owl:Class>
    


    <!-- https://hack.cybersystems.engineer/memex/ontologies/SeamlessDigitalEngineering#Supplier -->

    <owl:Class rdf:about="https://hack.cybersystems.engineer/memex/ontologies/SeamlessDigitalEngineering#Supplier">
        <owl:equivalentClass>
            <owl:Class>
                <owl:intersectionOf rdf:parseType="Collection">
                    <rdf:Description rdf:about="https://hack.cybersystems.engineer/memex/ontologies/SeamlessDigitalEngineering#Stakeholder"/>
                    <owl:Restriction>
                        <owl:onProperty rdf:resource="http://purl.obolibrary.org/obo/BFO_0000196"/>
                        <owl:someValuesFrom rdf:resource="https://www.commoncoreontologies.org/ont00000485"/>
                    </owl:Restriction>
                    <owl:Restriction>
                        <owl:onProperty rdf:resource="https://www.commoncoreontologies.org/ont00001787"/>
                        <owl:someValuesFrom rdf:resource="https://hack.cybersystems.engineer/memex/ontologies/SeamlessDigitalEngineering#Agreement_Process"/>
                    </owl:Restriction>
                </owl:intersectionOf>
            </owl:Class>
        </owl:equivalentClass>
        <rdfs:subClassOf rdf:resource="https://hack.cybersystems.engineer/memex/ontologies/SeamlessDigitalEngineering#Stakeholder"/>
        <rdfs:label xml:lang="en">Supplier</rdfs:label>
        <skos:definition xml:lang="en">Stakeholder that enters into an Agreement Process with the Acquirer for the supply of a Product or Service</skos:definition>
        <cco2:ont00001754 xml:lang="en">ISO/IEC/IEEE 24765:2017</cco2:ont00001754>
    </owl:Class>
    


    <!-- https://hack.cybersystems.engineer/memex/ontologies/SeamlessDigitalEngineering#Supply_Process -->

    <owl:Class rdf:about="https://hack.cybersystems.engineer/memex/ontologies/SeamlessDigitalEngineering#Supply_Process">
        <rdfs:subClassOf rdf:resource="https://hack.cybersystems.engineer/memex/ontologies/SeamlessDigitalEngineering#Agreement_Process"/>
        <rdfs:label xml:lang="en">Supply Process</rdfs:label>
        <skos:definition xml:lang="en">The purpose of the Supply Process is to provide an Acquirer with a Product or Service that meets agreed Requirements.</skos:definition>
        <cco2:ont00001754>ISO/IEC/IEEE 15288:2023</cco2:ont00001754>
    </owl:Class>
    


    <!-- https://hack.cybersystems.engineer/memex/ontologies/SeamlessDigitalEngineering#Support_Lifecycle_Stage -->

    <owl:Class rdf:about="https://hack.cybersystems.engineer/memex/ontologies/SeamlessDigitalEngineering#Support_Lifecycle_Stage">
        <rdfs:subClassOf rdf:resource="https://www.commoncoreontologies.org/ont00001191"/>
        <rdfs:label xml:lang="en">Support Lifecycle Stage</rdfs:label>
        <cco2:ont00001754 xml:lang="en">ISO/IEC/IEEE 15288:2023</cco2:ont00001754>
    </owl:Class>
    


    <!-- https://hack.cybersystems.engineer/memex/ontologies/SeamlessDigitalEngineering#Support_Stage -->

    <owl:Class rdf:about="https://hack.cybersystems.engineer/memex/ontologies/SeamlessDigitalEngineering#Support_Stage">
        <rdfs:subClassOf rdf:resource="https://hack.cybersystems.engineer/memex/ontologies/SeamlessDigitalEngineering#Lifecycle_Stage"/>
        <rdfs:comment xml:lang="en">Purpose: The support stage is executed to provide logistics, maintenance and support services that enable continuing SoI operation and a sustainable service.</rdfs:comment>
        <rdfs:label xml:lang="en">Support Stage</rdfs:label>
        <cco2:ont00001754>ISO/IEC/IEEE 24748-1:2024</cco2:ont00001754>
    </owl:Class>
    


    <!-- https://hack.cybersystems.engineer/memex/ontologies/SeamlessDigitalEngineering#Supported_Assurance_Claim -->

    <owl:Class rdf:about="https://hack.cybersystems.engineer/memex/ontologies/SeamlessDigitalEngineering#Supported_Assurance_Claim">
        <owl:equivalentClass>
            <owl:Class>
                <owl:intersectionOf rdf:parseType="Collection">
                    <rdf:Description rdf:about="https://hack.cybersystems.engineer/memex/ontologies/SeamlessDigitalEngineering#Assurance_Claim"/>
                    <rdf:Description rdf:about="https://hack.cybersystems.engineer/memex/ontologies/SeamlessDigitalEngineering#Supported_Claim"/>
                </owl:intersectionOf>
            </owl:Class>
        </owl:equivalentClass>
        <rdfs:subClassOf rdf:resource="https://hack.cybersystems.engineer/memex/ontologies/SeamlessDigitalEngineering#Assurance_Claim"/>
        <rdfs:label xml:lang="en">Supported Assurance Claim</rdfs:label>
        <cco2:ont00001754 xml:lang="en">derived from ISO/IEC/IEEE 15026-1:2019</cco2:ont00001754>
    </owl:Class>
    


    <!-- https://hack.cybersystems.engineer/memex/ontologies/SeamlessDigitalEngineering#Supported_Assurance_Claim_Record -->

    <owl:Class rdf:about="https://hack.cybersystems.engineer/memex/ontologies/SeamlessDigitalEngineering#Supported_Assurance_Claim_Record">
        <owl:equivalentClass>
            <owl:Class>
                <owl:intersectionOf rdf:parseType="Collection">
                    <rdf:Description rdf:about="https://hack.cybersystems.engineer/memex/ontologies/SeamlessDigitalEngineering#Assurance_Claim_Record"/>
                    <owl:Restriction>
                        <owl:onProperty rdf:resource="http://purl.obolibrary.org/obo/BFO_0000101"/>
                        <owl:allValuesFrom rdf:resource="https://hack.cybersystems.engineer/memex/ontologies/SeamlessDigitalEngineering#Supported_Assurance_Claim"/>
                    </owl:Restriction>
                    <owl:Restriction>
                        <owl:onProperty rdf:resource="http://purl.obolibrary.org/obo/BFO_0000115"/>
                        <owl:allValuesFrom rdf:resource="https://hack.cybersystems.engineer/memex/ontologies/SeamlessDigitalEngineering#Developed_Assurance_Argument_Record"/>
                    </owl:Restriction>
                </owl:intersectionOf>
            </owl:Class>
        </owl:equivalentClass>
        <rdfs:subClassOf rdf:resource="https://hack.cybersystems.engineer/memex/ontologies/SeamlessDigitalEngineering#Assurance_Claim_Record"/>
        <rdfs:label xml:lang="en">Supported Assurance Claim Record</rdfs:label>
        <skos:definition xml:lang="en">an Assurance Claim is Supported iff it contains exactly one Developed Assurance Argument Record</skos:definition>
    </owl:Class>
    


    <!-- https://hack.cybersystems.engineer/memex/ontologies/SeamlessDigitalEngineering#Supported_Claim -->

    <owl:Class rdf:about="https://hack.cybersystems.engineer/memex/ontologies/SeamlessDigitalEngineering#Supported_Claim">
        <owl:equivalentClass>
            <owl:Class>
                <owl:intersectionOf rdf:parseType="Collection">
                    <rdf:Description rdf:about="https://hack.cybersystems.engineer/memex/ontologies/SeamlessDigitalEngineering#Claim"/>
                    <owl:Restriction>
                        <owl:onProperty rdf:resource="http://purl.obolibrary.org/obo/BFO_0000178"/>
                        <owl:someValuesFrom rdf:resource="https://hack.cybersystems.engineer/memex/ontologies/SeamlessDigitalEngineering#Evidence_Item"/>
                    </owl:Restriction>
                </owl:intersectionOf>
            </owl:Class>
        </owl:equivalentClass>
        <rdfs:subClassOf rdf:resource="https://hack.cybersystems.engineer/memex/ontologies/SeamlessDigitalEngineering#Claim"/>
        <rdfs:label xml:lang="en">Supported Claim</rdfs:label>
        <cco2:ont00001754 xml:lang="en">derived from ISO/IEC/IEEE 15026-1:2019</cco2:ont00001754>
    </owl:Class>
    


    <!-- https://hack.cybersystems.engineer/memex/ontologies/SeamlessDigitalEngineering#System -->

    <owl:Class rdf:about="https://hack.cybersystems.engineer/memex/ontologies/SeamlessDigitalEngineering#System">
        <owl:equivalentClass>
            <owl:Class>
                <owl:intersectionOf rdf:parseType="Collection">
                    <owl:Restriction>
                        <owl:onProperty rdf:resource="http://purl.obolibrary.org/obo/BFO_0000115"/>
                        <owl:someValuesFrom rdf:resource="https://hack.cybersystems.engineer/memex/ontologies/SeamlessDigitalEngineering#System_Element"/>
                    </owl:Restriction>
                    <owl:Restriction>
                        <owl:onProperty rdf:resource="https://www.commoncoreontologies.org/ont00001787"/>
                        <owl:someValuesFrom rdf:resource="https://www.commoncoreontologies.org/ont00001347"/>
                    </owl:Restriction>
                    <owl:Restriction>
                        <owl:onProperty rdf:resource="https://www.commoncoreontologies.org/ont00001901"/>
                        <owl:someValuesFrom rdf:resource="https://www.commoncoreontologies.org/ont00000038"/>
                    </owl:Restriction>
                </owl:intersectionOf>
            </owl:Class>
        </owl:equivalentClass>
        <rdfs:subClassOf rdf:resource="http://purl.obolibrary.org/obo/BFO_0000027"/>
        <owl:disjointWith rdf:resource="https://hack.cybersystems.engineer/memex/ontologies/SeamlessDigitalEngineering#System_Environment"/>
        <dc:source xml:lang="en">https://sebokwiki.org/wiki/System_(glossary)</dc:source>
        <rdfs:seeAlso rdf:datatype="http://www.w3.org/2001/XMLSchema#anyURI">https://en.wikipedia.org/wiki/System</rdfs:seeAlso>
        <skos:definition xml:lang="en">arrangement of parts or elements that together exhibit a stated behaviour or meaning that the individual constituents do not.</skos:definition>
        <cco2:ont00001754 xml:lang="en">ISO/IEC/IEEE 15288:2023</cco2:ont00001754>
        <cco2:ont00001760 rdf:datatype="http://www.w3.org/2001/XMLSchema#anyURI">https://semantic.incose.org/DEIX_Ontology</cco2:ont00001760>
    </owl:Class>
    


    <!-- https://hack.cybersystems.engineer/memex/ontologies/SeamlessDigitalEngineering#System-of-Interest_Role -->

    <owl:Class rdf:about="https://hack.cybersystems.engineer/memex/ontologies/SeamlessDigitalEngineering#System-of-Interest_Role">
        <rdfs:subClassOf rdf:resource="https://www.commoncoreontologies.org/ont00000038"/>
        <rdfs:label xml:lang="en">System-of-Interest Role</rdfs:label>
        <skos:altLabel>SOI</skos:altLabel>
        <skos:altLabel>SoI</skos:altLabel>
        <skos:definition xml:lang="en">System whose Lifecycle is under consideration</skos:definition>
        <cco2:ont00001754>ISO/IEC/IEEE 15288:2023</cco2:ont00001754>
    </owl:Class>
    


    <!-- https://hack.cybersystems.engineer/memex/ontologies/SeamlessDigitalEngineering#System-of-Systems -->

    <owl:Class rdf:about="https://hack.cybersystems.engineer/memex/ontologies/SeamlessDigitalEngineering#System-of-Systems">
        <owl:equivalentClass>
            <owl:Class>
                <owl:intersectionOf rdf:parseType="Collection">
                    <owl:Restriction>
                        <owl:onProperty rdf:resource="http://purl.obolibrary.org/obo/BFO_0000178"/>
                        <owl:someValuesFrom rdf:resource="https://hack.cybersystems.engineer/memex/ontologies/SeamlessDigitalEngineering#System"/>
                    </owl:Restriction>
                    <owl:Restriction>
                        <owl:onProperty rdf:resource="https://www.commoncoreontologies.org/ont00001898"/>
                        <owl:someValuesFrom rdf:resource="https://hack.cybersystems.engineer/memex/ontologies/SeamlessDigitalEngineering#Capability"/>
                    </owl:Restriction>
                </owl:intersectionOf>
            </owl:Class>
        </owl:equivalentClass>
        <rdfs:subClassOf rdf:resource="https://hack.cybersystems.engineer/memex/ontologies/SeamlessDigitalEngineering#System"/>
        <skos:altLabel>SoS</skos:altLabel>
        <skos:definition xml:lang="en">set of Systems or System Elements that interact to provide a unique Capability that none of the constituent Systems can accomplish on its own</skos:definition>
        <cco2:ont00001754>ISO/IEC/IEEE 15288:2023</cco2:ont00001754>
    </owl:Class>
    


    <!-- https://hack.cybersystems.engineer/memex/ontologies/SeamlessDigitalEngineering#System_Analysis_Process -->

    <owl:Class rdf:about="https://hack.cybersystems.engineer/memex/ontologies/SeamlessDigitalEngineering#System_Analysis_Process">
        <rdfs:subClassOf rdf:resource="https://hack.cybersystems.engineer/memex/ontologies/SeamlessDigitalEngineering#Technical_Process"/>
        <rdfs:label xml:lang="en">System Analysis Process</rdfs:label>
        <skos:definition xml:lang="en">The purpose of the system analysis process is to provide a rigorous basis of data and information for technical understanding to aid decision-making and technical assessments across the life cycle.</skos:definition>
        <cco2:ont00001754>ISO/IEC/IEEE 15288:2023</cco2:ont00001754>
    </owl:Class>
    


    <!-- https://hack.cybersystems.engineer/memex/ontologies/SeamlessDigitalEngineering#System_Architecture_Definition_Process -->

    <owl:Class rdf:about="https://hack.cybersystems.engineer/memex/ontologies/SeamlessDigitalEngineering#System_Architecture_Definition_Process">
        <rdfs:subClassOf rdf:resource="https://hack.cybersystems.engineer/memex/ontologies/SeamlessDigitalEngineering#Technical_Process"/>
        <rdfs:label xml:lang="en">System Architecture Definition Process</rdfs:label>
        <skos:definition xml:lang="en">The purpose of the system architecture definition process is to generate system architecture alternatives, select one or more alternative(s) that address stakeholder concerns and system requirements, and express this in consistent views and models.</skos:definition>
        <cco2:ont00001754>ISO/IEC/IEEE 15288:2023</cco2:ont00001754>
    </owl:Class>
    


    <!-- https://hack.cybersystems.engineer/memex/ontologies/SeamlessDigitalEngineering#System_Architecture_Element -->

    <owl:Class rdf:about="https://hack.cybersystems.engineer/memex/ontologies/SeamlessDigitalEngineering#System_Architecture_Element">
        <rdfs:subClassOf rdf:resource="https://hack.cybersystems.engineer/memex/ontologies/SeamlessDigitalEngineering#System_Architecture_Model"/>
        <rdfs:label xml:lang="en">System Architecture Element</rdfs:label>
    </owl:Class>
    


    <!-- https://hack.cybersystems.engineer/memex/ontologies/SeamlessDigitalEngineering#System_Architecture_Model -->

    <owl:Class rdf:about="https://hack.cybersystems.engineer/memex/ontologies/SeamlessDigitalEngineering#System_Architecture_Model">
        <owl:equivalentClass>
            <owl:Class>
                <owl:intersectionOf rdf:parseType="Collection">
                    <rdf:Description rdf:about="https://hack.cybersystems.engineer/memex/ontologies/SeamlessDigitalEngineering#Architecture"/>
                    <rdf:Description rdf:about="https://hack.cybersystems.engineer/memex/ontologies/SeamlessDigitalEngineering#System_Model"/>
                    <owl:Restriction>
                        <owl:onProperty rdf:resource="http://purl.obolibrary.org/obo/BFO_0000178"/>
                        <owl:someValuesFrom rdf:resource="https://hack.cybersystems.engineer/memex/ontologies/SeamlessDigitalEngineering#System_Architecture_Element"/>
                    </owl:Restriction>
                </owl:intersectionOf>
            </owl:Class>
        </owl:equivalentClass>
        <rdfs:subClassOf rdf:resource="https://www.commoncoreontologies.org/ont00001045"/>
        <rdfs:label xml:lang="en">System Architecture Model</rdfs:label>
        <skos:definition xml:lang="en">The fundamental concepts or properties of a System in its Environment and governing principles for the realization and evolution of this System and its related Lifecycle Processes</skos:definition>
        <cco2:ont00001754 xml:lang="en">ISO/IEC/IEEE 15288:2023</cco2:ont00001754>
    </owl:Class>
    


    <!-- https://hack.cybersystems.engineer/memex/ontologies/SeamlessDigitalEngineering#System_Architecture_Pattern -->

    <owl:Class rdf:about="https://hack.cybersystems.engineer/memex/ontologies/SeamlessDigitalEngineering#System_Architecture_Pattern">
        <rdfs:subClassOf rdf:resource="https://hack.cybersystems.engineer/memex/ontologies/SeamlessDigitalEngineering#System_Architecture_Model"/>
        <rdfs:label xml:lang="en">System Architecture Pattern</rdfs:label>
    </owl:Class>
    


    <!-- https://hack.cybersystems.engineer/memex/ontologies/SeamlessDigitalEngineering#System_Context_Model -->

    <owl:Class rdf:about="https://hack.cybersystems.engineer/memex/ontologies/SeamlessDigitalEngineering#System_Context_Model">
        <owl:equivalentClass>
            <owl:Restriction>
                <owl:onProperty rdf:resource="https://www.commoncoreontologies.org/ont00001942"/>
                <owl:someValuesFrom rdf:resource="https://hack.cybersystems.engineer/memex/ontologies/SeamlessDigitalEngineering#System_Environment"/>
            </owl:Restriction>
        </owl:equivalentClass>
        <rdfs:subClassOf rdf:resource="https://hack.cybersystems.engineer/memex/ontologies/SeamlessDigitalEngineering#Lifecycle_Concept"/>
        <rdfs:label xml:lang="en">System Context Model</rdfs:label>
        <skos:definition xml:lang="en">Describes the system relationships and environment, resolved around a selected system-of-interest.</skos:definition>
    </owl:Class>
    


    <!-- https://hack.cybersystems.engineer/memex/ontologies/SeamlessDigitalEngineering#System_Element -->

    <owl:Class rdf:about="https://hack.cybersystems.engineer/memex/ontologies/SeamlessDigitalEngineering#System_Element">
        <owl:equivalentClass>
            <owl:Restriction>
                <owl:onProperty rdf:resource="https://www.commoncoreontologies.org/ont00001901"/>
                <owl:someValuesFrom rdf:resource="https://www.commoncoreontologies.org/ont00000929"/>
            </owl:Restriction>
        </owl:equivalentClass>
        <rdfs:subClassOf rdf:resource="http://purl.obolibrary.org/obo/BFO_0000027"/>
        <rdfs:label xml:lang="en">System Element</rdfs:label>
        <skos:altLabel xml:lang="en">Component</skos:altLabel>
        <skos:altLabel xml:lang="en">System Part</skos:altLabel>
        <skos:definition xml:lang="en">discrete part of a System that can be implemented to fulfil specified Requirements.</skos:definition>
        <cco2:ont00001754 xml:lang="en">ISO/IEC/IEEE 15288:2023</cco2:ont00001754>
        <cco2:ont00001760 rdf:datatype="http://www.w3.org/2001/XMLSchema#anyURI">https://semantic.incose.org/DEIX_Ontology</cco2:ont00001760>
    </owl:Class>
    


    <!-- https://hack.cybersystems.engineer/memex/ontologies/SeamlessDigitalEngineering#System_Environment -->

    <owl:Class rdf:about="https://hack.cybersystems.engineer/memex/ontologies/SeamlessDigitalEngineering#System_Environment">
        <owl:equivalentClass>
            <owl:Class>
                <owl:intersectionOf rdf:parseType="Collection">
                    <owl:Restriction>
                        <owl:onProperty rdf:resource="http://purl.obolibrary.org/obo/BFO_0000178"/>
                        <owl:someValuesFrom rdf:resource="https://www.commoncoreontologies.org/ont00000574"/>
                    </owl:Restriction>
                    <owl:Restriction>
                        <owl:onProperty rdf:resource="http://purl.obolibrary.org/obo/BFO_0000178"/>
                        <owl:someValuesFrom>
                            <owl:Class>
                                <owl:unionOf rdf:parseType="Collection">
                                    <rdf:Description rdf:about="https://hack.cybersystems.engineer/memex/ontologies/SeamlessDigitalEngineering#Operational_Environment"/>
                                    <rdf:Description rdf:about="https://hack.cybersystems.engineer/memex/ontologies/SeamlessDigitalEngineering#V&amp;V_Environment"/>
                                </owl:unionOf>
                            </owl:Class>
                        </owl:someValuesFrom>
                    </owl:Restriction>
                    <owl:Restriction>
                        <owl:onProperty rdf:resource="http://purl.obolibrary.org/obo/BFO_0000183"/>
                        <owl:someValuesFrom rdf:resource="https://hack.cybersystems.engineer/memex/ontologies/SeamlessDigitalEngineering#Lifecycle"/>
                    </owl:Restriction>
                </owl:intersectionOf>
            </owl:Class>
        </owl:equivalentClass>
        <rdfs:subClassOf rdf:resource="http://purl.obolibrary.org/obo/BFO_0000027"/>
        <rdfs:label>System Environment</rdfs:label>
        <skos:definition xml:lang="en">The surroundings (natural or man‐made) in which the SoI is utilized and supported
or in which the System is being developed, produced, and retired.</skos:definition>
        <skos:definition xml:lang="en">context determining the setting and circumstances of all influences upon System</skos:definition>
        <cco2:ont00001754>INCOSE (2023). Systems Engineering Handbook, Fifth Edition. No. INCOSE-TP-2003-002-05. ISBN: 9781119814306</cco2:ont00001754>
        <cco2:ont00001754>ISO/IEC/IEEE 15288:2023</cco2:ont00001754>
        <cco2:ont00001760 rdf:datatype="http://www.w3.org/2001/XMLSchema#anyURI">https://semantic.incose.org/DEIX_Ontology</cco2:ont00001760>
    </owl:Class>
    


    <!-- https://hack.cybersystems.engineer/memex/ontologies/SeamlessDigitalEngineering#System_Lifecycle_Process -->

    <owl:Class rdf:about="https://hack.cybersystems.engineer/memex/ontologies/SeamlessDigitalEngineering#System_Lifecycle_Process">
        <owl:equivalentClass>
            <owl:Class>
                <owl:intersectionOf rdf:parseType="Collection">
                    <owl:Restriction>
                        <owl:onProperty rdf:resource="https://www.commoncoreontologies.org/ont00001857"/>
                        <owl:someValuesFrom>
                            <owl:Class>
                                <owl:intersectionOf rdf:parseType="Collection">
                                    <rdf:Description rdf:about="https://hack.cybersystems.engineer/memex/ontologies/SeamlessDigitalEngineering#Act_of_Systems_Engineering"/>
                                    <rdf:Description rdf:about="https://hack.cybersystems.engineer/memex/ontologies/SeamlessDigitalEngineering#Lifecycle"/>
                                </owl:intersectionOf>
                            </owl:Class>
                        </owl:someValuesFrom>
                    </owl:Restriction>
                    <owl:Restriction>
                        <owl:onProperty rdf:resource="https://www.commoncoreontologies.org/ont00001920"/>
                        <owl:someValuesFrom rdf:resource="https://hack.cybersystems.engineer/memex/ontologies/SeamlessDigitalEngineering#Technical_Standard"/>
                    </owl:Restriction>
                </owl:intersectionOf>
            </owl:Class>
        </owl:equivalentClass>
        <rdfs:subClassOf rdf:resource="https://hack.cybersystems.engineer/memex/ontologies/SeamlessDigitalEngineering#Act_of_Systems_Engineering"/>
        <rdfs:label xml:lang="en">System Lifecycle Process</rdfs:label>
        <cco2:ont00001754>ISO/IEC/IEEE 15288:2023</cco2:ont00001754>
    </owl:Class>
    


    <!-- https://hack.cybersystems.engineer/memex/ontologies/SeamlessDigitalEngineering#System_Model -->

    <owl:Class rdf:about="https://hack.cybersystems.engineer/memex/ontologies/SeamlessDigitalEngineering#System_Model">
        <owl:equivalentClass>
            <owl:Class>
                <owl:intersectionOf rdf:parseType="Collection">
                    <rdf:Description rdf:about="https://www.commoncoreontologies.org/ont00001045"/>
                    <owl:Restriction>
                        <owl:onProperty rdf:resource="https://www.commoncoreontologies.org/ont00001942"/>
                        <owl:someValuesFrom rdf:resource="https://hack.cybersystems.engineer/memex/ontologies/SeamlessDigitalEngineering#System"/>
                    </owl:Restriction>
                </owl:intersectionOf>
            </owl:Class>
        </owl:equivalentClass>
        <rdfs:subClassOf rdf:resource="https://www.commoncoreontologies.org/ont00001045"/>
        <rdfs:comment xml:lang="en">The provided definition is derived from the INCOSE Systems Engineering Handbook section of prose, 2.3.5.6 System Analysis Process, in lieu of a glossary term. The term is not mentioned in ISO/IEC/IEEE 15288:2023, and not defined in the SEBoK. ISO/IEC/IEEE 24765:2017 has a definition of &apos;system model&apos; that is only applicable to the computer performance evaluation domain.</rdfs:comment>
        <rdfs:label xml:lang="en">System Model</rdfs:label>
        <skos:definition xml:lang="en">Artifact Model that prescribes a System and uses &quot;quantitative (numerical) and qualitative (categorical) variables to represent system attributes along multiple dimensions&quot;</skos:definition>
        <cco2:ont00001754 xml:lang="en">INCOSE Systems Engineering Handbook, Fifth Edition</cco2:ont00001754>
        <cco2:ont00001760 rdf:datatype="http://www.w3.org/2001/XMLSchema#anyURI">https://semantic.incose.org/DEIX_Ontology</cco2:ont00001760>
    </owl:Class>
    


    <!-- https://hack.cybersystems.engineer/memex/ontologies/SeamlessDigitalEngineering#System_Requirements_Definition_Process -->

    <owl:Class rdf:about="https://hack.cybersystems.engineer/memex/ontologies/SeamlessDigitalEngineering#System_Requirements_Definition_Process">
        <owl:equivalentClass>
            <owl:Restriction>
                <owl:onProperty rdf:resource="https://www.commoncoreontologies.org/ont00001986"/>
                <owl:someValuesFrom rdf:resource="https://hack.cybersystems.engineer/memex/ontologies/SeamlessDigitalEngineering#Requirement_Set"/>
            </owl:Restriction>
        </owl:equivalentClass>
        <rdfs:subClassOf rdf:resource="https://hack.cybersystems.engineer/memex/ontologies/SeamlessDigitalEngineering#Technical_Process"/>
        <rdfs:label xml:lang="en">System Requirements Definition Process</rdfs:label>
        <skos:definition xml:lang="en">The purpose of the system requirements definition process is to transform the stakeholder, user-oriented view of desired capabilities into a technical view of a solution that meets the operational needs of the user.</skos:definition>
        <cco2:ont00001754>ISO/IEC/IEEE 15288:2023</cco2:ont00001754>
    </owl:Class>
    


    <!-- https://hack.cybersystems.engineer/memex/ontologies/SeamlessDigitalEngineering#System_View -->

    <owl:Class rdf:about="https://hack.cybersystems.engineer/memex/ontologies/SeamlessDigitalEngineering#System_View">
        <owl:equivalentClass>
            <owl:Class>
                <owl:intersectionOf rdf:parseType="Collection">
                    <rdf:Description rdf:about="https://hack.cybersystems.engineer/memex/ontologies/SeamlessDigitalEngineering#View"/>
                    <owl:Restriction>
                        <owl:onProperty rdf:resource="https://www.commoncoreontologies.org/ont00001938"/>
                        <owl:someValuesFrom rdf:resource="https://hack.cybersystems.engineer/memex/ontologies/SeamlessDigitalEngineering#System"/>
                    </owl:Restriction>
                </owl:intersectionOf>
            </owl:Class>
        </owl:equivalentClass>
        <rdfs:subClassOf rdf:resource="https://hack.cybersystems.engineer/memex/ontologies/SeamlessDigitalEngineering#View"/>
        <rdfs:label xml:lang="en">System View</rdfs:label>
        <skos:definition xml:lang="en">A representation of a System from the perspective of a related set of Concerns</skos:definition>
        <cco2:ont00001754>ISO/IEC/IEEE 15288:2023</cco2:ont00001754>
        <cco2:ont00001760 rdf:datatype="http://www.w3.org/2001/XMLSchema#anyURI">https://semantic.incose.org/DEIX_Ontology</cco2:ont00001760>
    </owl:Class>
    


    <!-- https://hack.cybersystems.engineer/memex/ontologies/SeamlessDigitalEngineering#System_Viewpoint -->

    <owl:Class rdf:about="https://hack.cybersystems.engineer/memex/ontologies/SeamlessDigitalEngineering#System_Viewpoint">
        <owl:equivalentClass>
            <owl:Class>
                <owl:intersectionOf rdf:parseType="Collection">
                    <rdf:Description rdf:about="https://hack.cybersystems.engineer/memex/ontologies/SeamlessDigitalEngineering#Viewpoint"/>
                    <owl:Restriction>
                        <owl:onProperty rdf:resource="https://www.commoncoreontologies.org/ont00001942"/>
                        <owl:someValuesFrom rdf:resource="https://hack.cybersystems.engineer/memex/ontologies/SeamlessDigitalEngineering#System_View"/>
                    </owl:Restriction>
                </owl:intersectionOf>
            </owl:Class>
        </owl:equivalentClass>
        <rdfs:subClassOf rdf:resource="https://hack.cybersystems.engineer/memex/ontologies/SeamlessDigitalEngineering#Viewpoint"/>
        <rdfs:label xml:lang="en">System Viewpoint</rdfs:label>
        <skos:definition xml:lang="en">A specification of the conventions for constructing and using a System View</skos:definition>
        <cco2:ont00001754 xml:lang="en">adapted from ISO/IEC/IEEE 15288:2023</cco2:ont00001754>
        <cco2:ont00001760 rdf:datatype="http://www.w3.org/2001/XMLSchema#anyURI">https://semantic.incose.org/DEIX_Ontology</cco2:ont00001760>
    </owl:Class>
    


    <!-- https://hack.cybersystems.engineer/memex/ontologies/SeamlessDigitalEngineering#Systems_Approach -->

    <owl:Class rdf:about="https://hack.cybersystems.engineer/memex/ontologies/SeamlessDigitalEngineering#Systems_Approach">
        <owl:equivalentClass>
            <owl:Class>
                <owl:intersectionOf rdf:parseType="Collection">
                    <rdf:Description rdf:about="https://hack.cybersystems.engineer/memex/ontologies/SeamlessDigitalEngineering#Approach"/>
                    <owl:Restriction>
                        <owl:onProperty rdf:resource="https://www.commoncoreontologies.org/ont00001808"/>
                        <owl:someValuesFrom rdf:resource="https://hack.cybersystems.engineer/memex/ontologies/SeamlessDigitalEngineering#System"/>
                    </owl:Restriction>
                </owl:intersectionOf>
            </owl:Class>
        </owl:equivalentClass>
        <rdfs:subClassOf rdf:resource="https://hack.cybersystems.engineer/memex/ontologies/SeamlessDigitalEngineering#Approach"/>
        <rdfs:label xml:lang="en">Systems Approach</rdfs:label>
        <skos:definition xml:lang="en">A set of principles for applying systems thinking to engineered system contexts.</skos:definition>
        <cco2:ont00001754 rdf:datatype="http://www.w3.org/2001/XMLSchema#anyURI">https://sebokwiki.org/wiki/Systems_Approach_(glossary)</cco2:ont00001754>
    </owl:Class>
    


    <!-- https://hack.cybersystems.engineer/memex/ontologies/SeamlessDigitalEngineering#Systems_Engineer -->

    <owl:Class rdf:about="https://hack.cybersystems.engineer/memex/ontologies/SeamlessDigitalEngineering#Systems_Engineer">
        <rdfs:subClassOf rdf:resource="https://hack.cybersystems.engineer/memex/ontologies/SeamlessDigitalEngineering#Engineer"/>
        <rdfs:label xml:lang="en">Systems Engineer</rdfs:label>
    </owl:Class>
    


    <!-- https://hack.cybersystems.engineer/memex/ontologies/SeamlessDigitalEngineering#Systems_Engineering_Discipline -->

    <owl:Class rdf:about="https://hack.cybersystems.engineer/memex/ontologies/SeamlessDigitalEngineering#Systems_Engineering_Discipline">
        <owl:equivalentClass>
            <owl:Class>
                <owl:intersectionOf rdf:parseType="Collection">
                    <rdf:Description rdf:about="https://hack.cybersystems.engineer/memex/ontologies/SeamlessDigitalEngineering#Engineering_Discipline"/>
                    <owl:Restriction>
                        <owl:onProperty rdf:resource="https://www.commoncoreontologies.org/ont00001808"/>
                        <owl:someValuesFrom rdf:resource="https://hack.cybersystems.engineer/memex/ontologies/SeamlessDigitalEngineering#Act_of_Systems_Engineering"/>
                    </owl:Restriction>
                </owl:intersectionOf>
            </owl:Class>
        </owl:equivalentClass>
        <rdfs:subClassOf rdf:resource="https://hack.cybersystems.engineer/memex/ontologies/SeamlessDigitalEngineering#Engineering_Discipline"/>
        <rdfs:label xml:lang="en">Systems Engineering Discipline</rdfs:label>
    </owl:Class>
    


    <!-- https://hack.cybersystems.engineer/memex/ontologies/SeamlessDigitalEngineering#Target_Entity -->

    <owl:Class rdf:about="https://hack.cybersystems.engineer/memex/ontologies/SeamlessDigitalEngineering#Target_Entity">
        <owl:equivalentClass>
            <owl:Class>
                <owl:intersectionOf rdf:parseType="Collection">
                    <rdf:Description rdf:about="https://www.commoncoreontologies.org/ont00000544"/>
                    <owl:Restriction>
                        <owl:onProperty rdf:resource="https://www.commoncoreontologies.org/ont00001801"/>
                        <owl:someValuesFrom>
                            <owl:Restriction>
                                <owl:onProperty rdf:resource="http://purl.obolibrary.org/obo/BFO_0000084"/>
                                <owl:someValuesFrom rdf:resource="https://hack.cybersystems.engineer/memex/ontologies/SeamlessDigitalEngineering#Digital_Representation"/>
                            </owl:Restriction>
                        </owl:someValuesFrom>
                    </owl:Restriction>
                </owl:intersectionOf>
            </owl:Class>
        </owl:equivalentClass>
        <rdfs:subClassOf rdf:resource="https://www.commoncoreontologies.org/ont00000544"/>
        <rdfs:comment xml:lang="en">The target entity, which provides some functional purpose in reality, can be either physical or digital under consideration.

Source: ISO/IEC 20924:2024</rdfs:comment>
        <rdfs:label xml:lang="en">Target Entity</rdfs:label>
        <skos:definition xml:lang="en">A Target providing a functional purpose in reality which is the subject of Digital Representation</skos:definition>
        <skos:editorialNote xml:lang="en">TBD: Consider revisiting the equivalence axiom.</skos:editorialNote>
        <cco2:ont00001754 xml:lang="en">derived from ISO/IEC 30173:2023, 3.1.3</cco2:ont00001754>
        <cco2:ont00001760 rdf:datatype="http://www.w3.org/2001/XMLSchema#anyURI">https://semantic.incose.org/DEIX_Ontology</cco2:ont00001760>
    </owl:Class>
    


    <!-- https://hack.cybersystems.engineer/memex/ontologies/SeamlessDigitalEngineering#Target_of_Evaluation -->

    <owl:Class rdf:about="https://hack.cybersystems.engineer/memex/ontologies/SeamlessDigitalEngineering#Target_of_Evaluation">
        <owl:equivalentClass>
            <owl:Class>
                <owl:intersectionOf rdf:parseType="Collection">
                    <rdf:Description rdf:about="https://hack.cybersystems.engineer/memex/ontologies/SeamlessDigitalEngineering#Target_Entity"/>
                    <owl:Restriction>
                        <owl:onProperty rdf:resource="https://www.commoncoreontologies.org/ont00001936"/>
                        <owl:someValuesFrom rdf:resource="https://hack.cybersystems.engineer/memex/ontologies/SeamlessDigitalEngineering#Act_of_Evaluation"/>
                    </owl:Restriction>
                </owl:intersectionOf>
            </owl:Class>
        </owl:equivalentClass>
        <rdfs:subClassOf rdf:resource="https://hack.cybersystems.engineer/memex/ontologies/SeamlessDigitalEngineering#Target_Entity"/>
        <rdfs:label xml:lang="en">Target of Evaluation</rdfs:label>
        <skos:definition xml:lang="en">Target material entity, possibly accompanied by guidance, which is the subject of an Act of Evaluation</skos:definition>
        <cco2:ont00001754 xml:lang="en">derived from ISO/IEC 15408-1:2022
Information security, cybersecurity and privacy protection
Evaluation criteria for IT security
Part 1: Introduction and general model</cco2:ont00001754>
    </owl:Class>
    


    <!-- https://hack.cybersystems.engineer/memex/ontologies/SeamlessDigitalEngineering#Task -->

    <owl:Class rdf:about="https://hack.cybersystems.engineer/memex/ontologies/SeamlessDigitalEngineering#Task">
        <owl:equivalentClass>
            <owl:Restriction>
                <owl:onProperty rdf:resource="https://www.commoncoreontologies.org/ont00001803"/>
                <owl:someValuesFrom rdf:resource="https://hack.cybersystems.engineer/memex/ontologies/SeamlessDigitalEngineering#Process_Outcome"/>
            </owl:Restriction>
        </owl:equivalentClass>
        <rdfs:subClassOf rdf:resource="https://www.commoncoreontologies.org/ont00000228"/>
        <rdfs:label xml:lang="en">Task</rdfs:label>
        <skos:definition xml:lang="en">required, recommended, or permissible action, intended to contribute to the achievement of one or more outcomes of a process</skos:definition>
        <cco2:ont00001754>ISO/IEC/IEEE 15288:2023</cco2:ont00001754>
        <cco2:ont00001760 rdf:datatype="http://www.w3.org/2001/XMLSchema#anyURI">https://semantic.incose.org/DEIX_Ontology</cco2:ont00001760>
    </owl:Class>
    


    <!-- https://hack.cybersystems.engineer/memex/ontologies/SeamlessDigitalEngineering#Task_Plan -->

    <owl:Class rdf:about="https://hack.cybersystems.engineer/memex/ontologies/SeamlessDigitalEngineering#Task_Plan">
        <owl:equivalentClass>
            <owl:Restriction>
                <owl:onProperty rdf:resource="https://www.commoncoreontologies.org/ont00001942"/>
                <owl:someValuesFrom rdf:resource="https://hack.cybersystems.engineer/memex/ontologies/SeamlessDigitalEngineering#Task"/>
            </owl:Restriction>
        </owl:equivalentClass>
        <rdfs:subClassOf rdf:resource="https://www.commoncoreontologies.org/ont00000974"/>
        <rdfs:label xml:lang="en">Task Plan</rdfs:label>
    </owl:Class>
    


    <!-- https://hack.cybersystems.engineer/memex/ontologies/SeamlessDigitalEngineering#Technical_Management_Process -->

    <owl:Class rdf:about="https://hack.cybersystems.engineer/memex/ontologies/SeamlessDigitalEngineering#Technical_Management_Process">
        <rdfs:subClassOf rdf:resource="https://hack.cybersystems.engineer/memex/ontologies/SeamlessDigitalEngineering#System_Lifecycle_Process"/>
        <rdfs:comment xml:lang="en">Technical management is ‘the application of technical and administrative resources to plan, organize, and control engineering functions’ (ISO/IEC/IEEE 24765).</rdfs:comment>
        <rdfs:label xml:lang="en">Technical Management Process</rdfs:label>
        <skos:definition xml:lang="en">The technical management processes are concerned with managing the resources and assets allocated by organization management and with applying them to fulfil the agreements into which the organization or organizations enter. The technical management processes relate to the technical effort of projects, in particular to planning in terms of cost, timescales, and achievements; to the checking of actions to help ensure that they comply with plans and performance criteria; and to the identification and selection of corrective actions that recover shortfalls in progress and achievement. These processes are used to establish and perform technical plans for the project, manage information across the technical team, assess technical progress against the plans for the system products or services, control technical tasks through to completion, and to aid in the decision-making process. Individual technical management processes may be invoked at any time in the life cycle and at any level in a hierarchy of projects, as required by plans or unforeseen events. The technical management processes are applied with a level of rigor and formality that depends on the agreements as well as risk and complexity of the project.</skos:definition>
        <cco2:ont00001754>ISO/IEC/IEEE 15288:2023</cco2:ont00001754>
    </owl:Class>
    


    <!-- https://hack.cybersystems.engineer/memex/ontologies/SeamlessDigitalEngineering#Technical_Process -->

    <owl:Class rdf:about="https://hack.cybersystems.engineer/memex/ontologies/SeamlessDigitalEngineering#Technical_Process">
        <rdfs:subClassOf rdf:resource="https://hack.cybersystems.engineer/memex/ontologies/SeamlessDigitalEngineering#System_Lifecycle_Process"/>
        <rdfs:label xml:lang="en">Technical Process</rdfs:label>
        <skos:definition xml:lang="en">The technical processes are concerned with technical actions throughout the life cycle. Technical processes transform the needs of stakeholders into products or services. By applying that product or operating that service, technical processes provide sustainable performance, when and where needed, to meet the stakeholder requirements and achieve customer satisfaction. The technical processes are applied to create and use a system, whether it is in the form of a model or is a finished product.</skos:definition>
        <cco2:ont00001754>ISO/IEC/IEEE 15288:2023</cco2:ont00001754>
    </owl:Class>
    


    <!-- https://hack.cybersystems.engineer/memex/ontologies/SeamlessDigitalEngineering#Technical_Standard -->

    <owl:Class rdf:about="https://hack.cybersystems.engineer/memex/ontologies/SeamlessDigitalEngineering#Technical_Standard">
        <owl:equivalentClass>
            <owl:Restriction>
                <owl:onProperty rdf:resource="https://www.commoncoreontologies.org/ont00001942"/>
                <owl:someValuesFrom rdf:resource="https://hack.cybersystems.engineer/memex/ontologies/SeamlessDigitalEngineering#Methodology"/>
            </owl:Restriction>
        </owl:equivalentClass>
        <rdfs:subClassOf rdf:resource="https://www.commoncoreontologies.org/ont00000965"/>
        <rdfs:label xml:lang="en">Technical Standard</rdfs:label>
        <skos:definition xml:lang="en">standard that describes the characteristics of applying accumulated technical or management skills and methods in the creation of a product or performing a service</skos:definition>
        <cco2:ont00001754 xml:lang="en">ISO/IEC/IEEE 24765:2017</cco2:ont00001754>
    </owl:Class>
    


    <!-- https://hack.cybersystems.engineer/memex/ontologies/SeamlessDigitalEngineering#Technician -->

    <owl:Class rdf:about="https://hack.cybersystems.engineer/memex/ontologies/SeamlessDigitalEngineering#Technician">
        <rdfs:subClassOf rdf:resource="https://hack.cybersystems.engineer/memex/ontologies/SeamlessDigitalEngineering#Project_Team_Member"/>
        <rdfs:label xml:lang="en">Technician</rdfs:label>
    </owl:Class>
    


    <!-- https://hack.cybersystems.engineer/memex/ontologies/SeamlessDigitalEngineering#Technology_Readiness_Assessment_Report -->

    <owl:Class rdf:about="https://hack.cybersystems.engineer/memex/ontologies/SeamlessDigitalEngineering#Technology_Readiness_Assessment_Report">
        <owl:equivalentClass>
            <owl:Class>
                <owl:intersectionOf rdf:parseType="Collection">
                    <rdf:Description rdf:about="https://hack.cybersystems.engineer/memex/ontologies/SeamlessDigitalEngineering#Evaluation_Report"/>
                    <owl:Restriction>
                        <owl:onProperty rdf:resource="http://purl.obolibrary.org/obo/BFO_0000101"/>
                        <owl:someValuesFrom rdf:resource="https://hack.cybersystems.engineer/memex/ontologies/SeamlessDigitalEngineering#Technology_Readiness_Level"/>
                    </owl:Restriction>
                </owl:intersectionOf>
            </owl:Class>
        </owl:equivalentClass>
        <rdfs:subClassOf rdf:resource="https://hack.cybersystems.engineer/memex/ontologies/SeamlessDigitalEngineering#Evaluation_Report"/>
        <rdfs:label xml:lang="en">Technology Readiness Assessment Report</rdfs:label>
        <skos:definition xml:lang="en">A Report required for transition from Phase B to Phase C/D demonstrating that all systems, subsystems, and components have achieved a level of technological maturity with demonstrated evidence of qualification in a relevant environment.</skos:definition>
        <cco2:ont00001754 xml:lang="en">NASA Systems Engineering Handbook (2016)</cco2:ont00001754>
    </owl:Class>
    


    <!-- https://hack.cybersystems.engineer/memex/ontologies/SeamlessDigitalEngineering#Technology_Readiness_Level -->

    <owl:Class rdf:about="https://hack.cybersystems.engineer/memex/ontologies/SeamlessDigitalEngineering#Technology_Readiness_Level">
        <rdfs:subClassOf rdf:resource="https://www.commoncoreontologies.org/ont00001010"/>
        <rdfs:comment xml:lang="en">Typically, a TRL of 6 (i.e., technology demonstrated in a relevant environment) is required for a technology to be integrated into an SE process.</rdfs:comment>
        <rdfs:label xml:lang="en">Technology Readiness Level</rdfs:label>
        <skos:definition xml:lang="en">Provides a scale against which to measure the maturity of a technology. TRLs range from 1, basic technology research, to 9, systems test, launch, and operations.</skos:definition>
        <cco2:ont00001753 xml:lang="en">TRL</cco2:ont00001753>
        <cco2:ont00001754 xml:lang="en">NASA Systems Engineering Handbook (2016)</cco2:ont00001754>
    </owl:Class>
    


    <!-- https://hack.cybersystems.engineer/memex/ontologies/SeamlessDigitalEngineering#Test_Report -->

    <owl:Class rdf:about="https://hack.cybersystems.engineer/memex/ontologies/SeamlessDigitalEngineering#Test_Report">
        <rdfs:subClassOf rdf:resource="https://www.commoncoreontologies.org/ont00000624"/>
    </owl:Class>
    


    <!-- https://hack.cybersystems.engineer/memex/ontologies/SeamlessDigitalEngineering#Theorem -->

    <owl:Class rdf:about="https://hack.cybersystems.engineer/memex/ontologies/SeamlessDigitalEngineering#Theorem">
        <rdfs:subClassOf rdf:resource="http://www.ontologyrepository.com/CommonCoreOntologies/ComputerProgram"/>
        <rdfs:label xml:lang="en">Theorem</rdfs:label>
    </owl:Class>
    


    <!-- https://hack.cybersystems.engineer/memex/ontologies/SeamlessDigitalEngineering#Theorem_Prover -->

    <owl:Class rdf:about="https://hack.cybersystems.engineer/memex/ontologies/SeamlessDigitalEngineering#Theorem_Prover">
        <owl:equivalentClass>
            <owl:Class>
                <owl:intersectionOf rdf:parseType="Collection">
                    <rdf:Description rdf:about="http://www.ontologyrepository.com/CommonCoreOntologies/ApplicationSoftware"/>
                    <owl:Restriction>
                        <owl:onProperty rdf:resource="https://www.commoncoreontologies.org/ont00001852"/>
                        <owl:someValuesFrom rdf:resource="https://hack.cybersystems.engineer/memex/ontologies/SeamlessDigitalEngineering#Act_of_Formal_Verification"/>
                    </owl:Restriction>
                </owl:intersectionOf>
            </owl:Class>
        </owl:equivalentClass>
        <rdfs:subClassOf rdf:resource="http://www.ontologyrepository.com/CommonCoreOntologies/ApplicationSoftware"/>
        <rdfs:subClassOf>
            <owl:Restriction>
                <owl:onProperty rdf:resource="https://hack.cybersystems.engineer/memex/ontologies/SeamlessDigitalEngineering#correctly_implements_language"/>
                <owl:someValuesFrom rdf:resource="http://www.ontologyrepository.com/CommonCoreOntologies/ProgrammingLanguage"/>
            </owl:Restriction>
        </rdfs:subClassOf>
        <rdfs:label xml:lang="en">Theorem Prover</rdfs:label>
    </owl:Class>
    


    <!-- https://hack.cybersystems.engineer/memex/ontologies/SeamlessDigitalEngineering#Threat -->

    <owl:Class rdf:about="https://hack.cybersystems.engineer/memex/ontologies/SeamlessDigitalEngineering#Threat">
        <owl:equivalentClass>
            <owl:Class>
                <owl:intersectionOf rdf:parseType="Collection">
                    <owl:Restriction>
                        <owl:onProperty rdf:resource="https://www.commoncoreontologies.org/ont00001778"/>
                        <owl:someValuesFrom>
                            <owl:Class>
                                <owl:unionOf rdf:parseType="Collection">
                                    <rdf:Description rdf:about="https://hack.cybersystems.engineer/memex/ontologies/SeamlessDigitalEngineering#System"/>
                                    <rdf:Description rdf:about="https://hack.cybersystems.engineer/memex/ontologies/SeamlessDigitalEngineering#System_Environment"/>
                                </owl:unionOf>
                            </owl:Class>
                        </owl:someValuesFrom>
                    </owl:Restriction>
                    <owl:Restriction>
                        <owl:onProperty rdf:resource="https://www.commoncoreontologies.org/ont00001803"/>
                        <owl:someValuesFrom rdf:resource="https://hack.cybersystems.engineer/memex/ontologies/SeamlessDigitalEngineering#Adverse_Consequence"/>
                    </owl:Restriction>
                </owl:intersectionOf>
            </owl:Class>
        </owl:equivalentClass>
        <rdfs:subClassOf rdf:resource="https://www.commoncoreontologies.org/ont00000004"/>
        <rdfs:label xml:lang="en">Threat</rdfs:label>
        <skos:definition xml:lang="en">state of the System or System Environment which can lead to Adverse Consequences</skos:definition>
        <cco2:ont00001754 xml:lang="en">ISO/IEC/IEEE 24765:2017, 3.4288</cco2:ont00001754>
    </owl:Class>
    


    <!-- https://hack.cybersystems.engineer/memex/ontologies/SeamlessDigitalEngineering#Traceability_Measurement_Information_Content_Entity -->

    <owl:Class rdf:about="https://hack.cybersystems.engineer/memex/ontologies/SeamlessDigitalEngineering#Traceability_Measurement_Information_Content_Entity">
        <owl:equivalentClass>
            <owl:Class>
                <owl:intersectionOf rdf:parseType="Collection">
                    <rdf:Description rdf:about="https://www.commoncoreontologies.org/ont00001163"/>
                    <owl:Restriction>
                        <owl:onProperty rdf:resource="https://www.commoncoreontologies.org/ont00001966"/>
                        <owl:someValuesFrom rdf:resource="https://hack.cybersystems.engineer/memex/ontologies/SeamlessDigitalEngineering#Traceability_Relationship"/>
                    </owl:Restriction>
                </owl:intersectionOf>
            </owl:Class>
        </owl:equivalentClass>
        <rdfs:subClassOf rdf:resource="https://www.commoncoreontologies.org/ont00001163"/>
        <rdfs:label xml:lang="en">Traceability Measurement Information Content Entity</rdfs:label>
        <skos:definition xml:lang="en">A Measurement Information Content Entity that describes the Traceability Relationship among two or more logical entities</skos:definition>
        <cco2:ont00001754>ISO/IEC/IEEE 15288:2023</cco2:ont00001754>
        <cco2:ont00001760 rdf:datatype="http://www.w3.org/2001/XMLSchema#anyURI">https://semantic.incose.org/DEIX_Ontology</cco2:ont00001760>
    </owl:Class>
    


    <!-- https://hack.cybersystems.engineer/memex/ontologies/SeamlessDigitalEngineering#Traceability_Observation_Artifact_Function -->

    <owl:Class rdf:about="https://hack.cybersystems.engineer/memex/ontologies/SeamlessDigitalEngineering#Traceability_Observation_Artifact_Function">
        <owl:equivalentClass>
            <owl:Class>
                <owl:intersectionOf rdf:parseType="Collection">
                    <rdf:Description rdf:about="https://www.commoncoreontologies.org/ont00001306"/>
                    <owl:Restriction>
                        <owl:onProperty rdf:resource="http://purl.obolibrary.org/obo/BFO_0000059"/>
                        <owl:someValuesFrom rdf:resource="https://hack.cybersystems.engineer/memex/ontologies/SeamlessDigitalEngineering#Traceability_Measurement_Information_Content_Entity"/>
                    </owl:Restriction>
                </owl:intersectionOf>
            </owl:Class>
        </owl:equivalentClass>
        <rdfs:subClassOf rdf:resource="https://www.commoncoreontologies.org/ont00001306"/>
        <rdfs:label xml:lang="en">Traceability Observation Artifact Function</rdfs:label>
        <rdfs:seeAlso rdf:resource="https://hack.cybersystems.engineer/memex/ontologies/SeamlessDigitalEngineering#Traceability_Measurement_Information_Content_Entity"/>
        <skos:definition xml:lang="en">An Observation Artifact Function that is realized during events in which an Artifact is used to discern an association among two or more logical entities.</skos:definition>
        <cco2:ont00001754 xml:lang="en">derived from ISO/IEC/IEEE 15288:2023, 3.52</cco2:ont00001754>
        <cco2:ont00001760 rdf:datatype="http://www.w3.org/2001/XMLSchema#anyURI">https://semantic.incose.org/DEIX_Ontology</cco2:ont00001760>
    </owl:Class>
    


    <!-- https://hack.cybersystems.engineer/memex/ontologies/SeamlessDigitalEngineering#Traceability_Relationship -->

    <owl:Class rdf:about="https://hack.cybersystems.engineer/memex/ontologies/SeamlessDigitalEngineering#Traceability_Relationship">
        <owl:equivalentClass>
            <owl:Class>
                <owl:intersectionOf rdf:parseType="Collection">
                    <rdf:Description rdf:about="http://purl.obolibrary.org/obo/BFO_0000145"/>
                    <owl:Restriction>
                        <owl:onProperty rdf:resource="http://purl.obolibrary.org/obo/BFO_0000059"/>
                        <owl:someValuesFrom rdf:resource="https://hack.cybersystems.engineer/memex/ontologies/SeamlessDigitalEngineering#Traceability_Measurement_Information_Content_Entity"/>
                    </owl:Restriction>
                </owl:intersectionOf>
            </owl:Class>
        </owl:equivalentClass>
        <rdfs:subClassOf rdf:resource="http://purl.obolibrary.org/obo/BFO_0000145"/>
        <rdfs:label xml:lang="en">Traceability Relationship</rdfs:label>
        <skos:definition xml:lang="en">A relational quality which is a discernible association among two or more logical entities</skos:definition>
        <skos:example xml:lang="en">Logical entities may include Requirements, System Element, Verifications, or Tasks</skos:example>
        <cco2:ont00001754>ISO/IEC/IEEE 15288:2023, 3.52</cco2:ont00001754>
        <cco2:ont00001760 rdf:datatype="http://www.w3.org/2001/XMLSchema#anyURI">https://semantic.incose.org/DEIX_Ontology</cco2:ont00001760>
    </owl:Class>
    


    <!-- https://hack.cybersystems.engineer/memex/ontologies/SeamlessDigitalEngineering#Trade_Study -->

    <owl:Class rdf:about="https://hack.cybersystems.engineer/memex/ontologies/SeamlessDigitalEngineering#Trade_Study">
        <rdfs:subClassOf rdf:resource="https://hack.cybersystems.engineer/memex/ontologies/SeamlessDigitalEngineering#Decision_Support_Problem_Definition"/>
        <rdfs:label xml:lang="en">Trade Study</rdfs:label>
    </owl:Class>
    


    <!-- https://hack.cybersystems.engineer/memex/ontologies/SeamlessDigitalEngineering#Trade_Study_Process -->

    <owl:Class rdf:about="https://hack.cybersystems.engineer/memex/ontologies/SeamlessDigitalEngineering#Trade_Study_Process">
        <owl:equivalentClass>
            <owl:Class>
                <owl:intersectionOf rdf:parseType="Collection">
                    <rdf:Description rdf:about="https://hack.cybersystems.engineer/memex/ontologies/SeamlessDigitalEngineering#Decision_Management_Process"/>
                    <owl:Restriction>
                        <owl:onProperty rdf:resource="https://www.commoncoreontologies.org/ont00001986"/>
                        <owl:someValuesFrom rdf:resource="https://hack.cybersystems.engineer/memex/ontologies/SeamlessDigitalEngineering#Trade_Study_Report"/>
                    </owl:Restriction>
                </owl:intersectionOf>
            </owl:Class>
        </owl:equivalentClass>
        <rdfs:subClassOf rdf:resource="https://hack.cybersystems.engineer/memex/ontologies/SeamlessDigitalEngineering#Decision_Management_Process"/>
        <rdfs:label xml:lang="en">Trade Study Process</rdfs:label>
        <skos:definition xml:lang="en">A means of evaluating system designs by devising alternative means to meet Functional Requirements, evaluating these alternatives in terms of the Measures of Effectiveness and system cost, ranking the alternatives according to appropriate selection criteria, dropping less promising alternatives, and proceeding to the next level of resolution, if needed.</skos:definition>
        <cco2:ont00001754 xml:lang="en">NASA Systems Engineering Handbook (2016)</cco2:ont00001754>
    </owl:Class>
    


    <!-- https://hack.cybersystems.engineer/memex/ontologies/SeamlessDigitalEngineering#Trade_Study_Report -->

    <owl:Class rdf:about="https://hack.cybersystems.engineer/memex/ontologies/SeamlessDigitalEngineering#Trade_Study_Report">
        <owl:equivalentClass>
            <owl:Class>
                <owl:intersectionOf rdf:parseType="Collection">
                    <rdf:Description rdf:about="https://www.commoncoreontologies.org/ont00000624"/>
                    <owl:Restriction>
                        <owl:onProperty rdf:resource="http://purl.obolibrary.org/obo/BFO_0000101"/>
                        <owl:someValuesFrom rdf:resource="https://hack.cybersystems.engineer/memex/ontologies/SeamlessDigitalEngineering#Trade_Study"/>
                    </owl:Restriction>
                </owl:intersectionOf>
            </owl:Class>
        </owl:equivalentClass>
        <rdfs:subClassOf rdf:resource="https://www.commoncoreontologies.org/ont00000624"/>
        <rdfs:comment xml:lang="en">It should include:

- the system under analysis;
- system goals, objectives (or requirements, as appropriate to the level of resolution), and constraints;
- measures and measurement methods (models) used;
- all data sources used;
- the alternatives chosen for analysis;
- computational results, including uncertainty ranges and sensitivity analyses performed;
- the selection rule used; and
- the recommended alternative.</rdfs:comment>
        <rdfs:label xml:lang="en">Trade Study Report</rdfs:label>
        <skos:definition xml:lang="en">A Report written to document a Trade Study.</skos:definition>
        <cco2:ont00001754 xml:lang="en">NASA Systems Engineering Handbook (2016)</cco2:ont00001754>
    </owl:Class>
    


    <!-- https://hack.cybersystems.engineer/memex/ontologies/SeamlessDigitalEngineering#Transition_Process -->

    <owl:Class rdf:about="https://hack.cybersystems.engineer/memex/ontologies/SeamlessDigitalEngineering#Transition_Process">
        <rdfs:subClassOf rdf:resource="https://hack.cybersystems.engineer/memex/ontologies/SeamlessDigitalEngineering#Technical_Process"/>
        <rdfs:label xml:lang="en">Transition Process</rdfs:label>
        <skos:definition xml:lang="en">The purpose of the transition process is to establish a capability for a system to provide services specified by stakeholder requirements in the operational environment.</skos:definition>
        <cco2:ont00001754>ISO/IEC/IEEE 15288:2023</cco2:ont00001754>
    </owl:Class>
    


    <!-- https://hack.cybersystems.engineer/memex/ontologies/SeamlessDigitalEngineering#Trust -->

    <owl:Class rdf:about="https://hack.cybersystems.engineer/memex/ontologies/SeamlessDigitalEngineering#Trust">
        <owl:equivalentClass>
            <owl:Class>
                <owl:intersectionOf rdf:parseType="Collection">
                    <rdf:Description rdf:about="https://hack.cybersystems.engineer/memex/ontologies/SeamlessDigitalEngineering#Stakeholder_Confidence"/>
                    <owl:Restriction>
                        <owl:onProperty rdf:resource="http://purl.obolibrary.org/obo/BFO_0000195"/>
                        <owl:someValuesFrom rdf:resource="https://hack.cybersystems.engineer/memex/ontologies/SeamlessDigitalEngineering#Trustworthiness"/>
                    </owl:Restriction>
                </owl:intersectionOf>
            </owl:Class>
        </owl:equivalentClass>
        <rdfs:subClassOf rdf:resource="https://hack.cybersystems.engineer/memex/ontologies/SeamlessDigitalEngineering#Stakeholder_Confidence"/>
        <rdfs:comment xml:lang="en">The degree of Trust can vary from one part or aspect of a System to another.</rdfs:comment>
        <rdfs:comment xml:lang="en">Trust can be a function of time and circumstances.</rdfs:comment>
        <rdfs:comment xml:lang="en">Trust requires assessment of Evidence of Trustworthiness combined with levels of Confidence in those assessments.</rdfs:comment>
        <rdfs:label xml:lang="en">Trust</rdfs:label>
        <rdfs:seeAlso xml:lang="en">Fisher, David A., (March 2012), &quot;Principles of Trust for Embedded Systems&quot;, Technical Note No. CMU/SEI-2012-TN-007, Carnegie Mellon University Software Engineering Institute.</rdfs:seeAlso>
        <rdfs:seeAlso xml:lang="en">Fisher, David A., McCune, Jonathan M., Andrews, Archie D., (January 2011), &quot;Trust and Trusted Computing Platforms&quot;, Technical Note No. CMU/SEI-2011-TN-005, Carnegie Mellon University Software Engineering Institute.</rdfs:seeAlso>
        <skos:definition xml:lang="en">degree to which a Stakeholder has Confidence that a Product or System will behave as intended.</skos:definition>
        <cco2:ont00001754 xml:lang="en">ISO/IEC 23643:2020
Software and systems engineering
Capabilities of software safety and security verification tools</cco2:ont00001754>
    </owl:Class>
    


    <!-- https://hack.cybersystems.engineer/memex/ontologies/SeamlessDigitalEngineering#Trusted_Agent -->

    <owl:Class rdf:about="https://hack.cybersystems.engineer/memex/ontologies/SeamlessDigitalEngineering#Trusted_Agent">
        <rdfs:subClassOf rdf:resource="https://www.commoncoreontologies.org/ont00001017"/>
        <rdfs:subClassOf>
            <owl:Restriction>
                <owl:onProperty rdf:resource="http://purl.obolibrary.org/obo/BFO_0000196"/>
                <owl:someValuesFrom rdf:resource="https://hack.cybersystems.engineer/memex/ontologies/SeamlessDigitalEngineering#Trusted_Role"/>
            </owl:Restriction>
        </rdfs:subClassOf>
        <rdfs:label xml:lang="en">Trusted Agent</rdfs:label>
        <skos:definition xml:lang="en">an Agent who is deemed to be Trusted</skos:definition>
    </owl:Class>
    


    <!-- https://hack.cybersystems.engineer/memex/ontologies/SeamlessDigitalEngineering#Trusted_Computing_Base -->

    <owl:Class rdf:about="https://hack.cybersystems.engineer/memex/ontologies/SeamlessDigitalEngineering#Trusted_Computing_Base">
        <owl:equivalentClass>
            <owl:Class>
                <owl:intersectionOf rdf:parseType="Collection">
                    <rdf:Description rdf:about="http://www.ontologyrepository.com/CommonCoreOntologies/ComputerSystem"/>
                    <owl:Restriction>
                        <owl:onProperty rdf:resource="http://purl.obolibrary.org/obo/BFO_0000196"/>
                        <owl:someValuesFrom rdf:resource="https://hack.cybersystems.engineer/memex/ontologies/SeamlessDigitalEngineering#Trusted_Role"/>
                    </owl:Restriction>
                </owl:intersectionOf>
            </owl:Class>
        </owl:equivalentClass>
        <rdfs:subClassOf rdf:resource="http://www.ontologyrepository.com/CommonCoreOntologies/ComputerSystem"/>
        <rdfs:label xml:lang="en">Trusted Computing Base</rdfs:label>
    </owl:Class>
    


    <!-- https://hack.cybersystems.engineer/memex/ontologies/SeamlessDigitalEngineering#Trusted_Role -->

    <owl:Class rdf:about="https://hack.cybersystems.engineer/memex/ontologies/SeamlessDigitalEngineering#Trusted_Role">
        <rdfs:subClassOf rdf:resource="http://purl.obolibrary.org/obo/BFO_0000023"/>
        <rdfs:comment xml:lang="en">A Trusted Role is often an Authority Role.</rdfs:comment>
        <rdfs:label xml:lang="en">Trusted Role</rdfs:label>
        <skos:definition xml:lang="en">a role that performs critical functions which, if performed unsatisfactorily, can have an adverse impact upon the degree of Trustworthiness provided by the System</skos:definition>
        <cco2:ont00001754 xml:lang="en">derived from ISO/IEC 27099:2022, 3.60.</cco2:ont00001754>
    </owl:Class>
    


    <!-- https://hack.cybersystems.engineer/memex/ontologies/SeamlessDigitalEngineering#Trustworthiness -->

    <owl:Class rdf:about="https://hack.cybersystems.engineer/memex/ontologies/SeamlessDigitalEngineering#Trustworthiness">
        <owl:equivalentClass>
            <owl:Class>
                <owl:intersectionOf rdf:parseType="Collection">
                    <rdf:Description rdf:about="https://hack.cybersystems.engineer/memex/ontologies/SeamlessDigitalEngineering#Acceptability"/>
                    <owl:Restriction>
                        <owl:onProperty rdf:resource="http://purl.obolibrary.org/obo/BFO_0000195"/>
                        <owl:someValuesFrom rdf:resource="https://hack.cybersystems.engineer/memex/ontologies/SeamlessDigitalEngineering#Bootstrappability"/>
                    </owl:Restriction>
                    <owl:Restriction>
                        <owl:onProperty rdf:resource="http://purl.obolibrary.org/obo/BFO_0000195"/>
                        <owl:someValuesFrom>
                            <owl:Class>
                                <owl:intersectionOf rdf:parseType="Collection">
                                    <rdf:Description rdf:about="https://hack.cybersystems.engineer/memex/ontologies/SeamlessDigitalEngineering#Complete_Assurance_Case_Report"/>
                                    <owl:Restriction>
                                        <owl:onProperty rdf:resource="http://purl.obolibrary.org/obo/BFO_0000101"/>
                                        <owl:someValuesFrom rdf:resource="https://hack.cybersystems.engineer/memex/ontologies/SeamlessDigitalEngineering#Trustworthiness_Quality_Claim"/>
                                    </owl:Restriction>
                                </owl:intersectionOf>
                            </owl:Class>
                        </owl:someValuesFrom>
                    </owl:Restriction>
                </owl:intersectionOf>
            </owl:Class>
        </owl:equivalentClass>
        <rdfs:subClassOf rdf:resource="https://hack.cybersystems.engineer/memex/ontologies/SeamlessDigitalEngineering#Acceptability"/>
        <rdfs:comment xml:lang="en">Characteristics of Trustworthiness include, for instance, Accountability, Accuracy, Authenticity, Availability, Controllability, Integrity, Privacy, Quality, Reliability, Resilience, Robustness, Safety, Security, Transparency, and Usability.

Source: ISO/IEC TS 5723:2022 - Trustworthiness - Vocabulary</rdfs:comment>
        <rdfs:comment xml:lang="en">Verifiability includes Measurability and demonstrability by means of objective Evidence.

Source: ISO/IEC TS 5723:2022 - Trustworthiness - Vocabulary</rdfs:comment>
        <rdfs:label xml:lang="en">Trustworthiness</rdfs:label>
        <skos:definition xml:lang="en">extent to which Users or Stakeholders have Confidence that their Expectations are met in a verifiable way</skos:definition>
        <cco2:ont00001754 xml:lang="en">ISO/IEC 25019:2023(en)
Systems and software engineering — Systems and software Quality Requirements and Evaluation (SQuaRE) — Quality-in-use model</cco2:ont00001754>
    </owl:Class>
    


    <!-- https://hack.cybersystems.engineer/memex/ontologies/SeamlessDigitalEngineering#Trustworthiness_Quality_Claim -->

    <owl:Class rdf:about="https://hack.cybersystems.engineer/memex/ontologies/SeamlessDigitalEngineering#Trustworthiness_Quality_Claim">
        <owl:equivalentClass>
            <owl:Class>
                <owl:intersectionOf rdf:parseType="Collection">
                    <rdf:Description rdf:about="https://hack.cybersystems.engineer/memex/ontologies/SeamlessDigitalEngineering#Quality_Claim"/>
                    <owl:Restriction>
                        <owl:onProperty rdf:resource="https://www.commoncoreontologies.org/ont00001942"/>
                        <owl:someValuesFrom rdf:resource="https://hack.cybersystems.engineer/memex/ontologies/SeamlessDigitalEngineering#Trustworthiness"/>
                    </owl:Restriction>
                    <owl:Restriction>
                        <owl:onProperty rdf:resource="https://www.commoncoreontologies.org/ont00001942"/>
                        <owl:someValuesFrom rdf:resource="https://hack.cybersystems.engineer/memex/ontologies/SeamlessDigitalEngineering#Trustworthy_Role"/>
                    </owl:Restriction>
                </owl:intersectionOf>
            </owl:Class>
        </owl:equivalentClass>
        <rdfs:subClassOf rdf:resource="https://hack.cybersystems.engineer/memex/ontologies/SeamlessDigitalEngineering#Quality_Claim"/>
        <rdfs:label xml:lang="en">Trustworthiness Quality Claim</rdfs:label>
    </owl:Class>
    


    <!-- https://hack.cybersystems.engineer/memex/ontologies/SeamlessDigitalEngineering#Trustworthy_Computing_Base -->

    <owl:Class rdf:about="https://hack.cybersystems.engineer/memex/ontologies/SeamlessDigitalEngineering#Trustworthy_Computing_Base">
        <owl:equivalentClass>
            <owl:Class>
                <owl:intersectionOf rdf:parseType="Collection">
                    <rdf:Description rdf:about="http://www.ontologyrepository.com/CommonCoreOntologies/ComputerSystem"/>
                    <owl:Restriction>
                        <owl:onProperty rdf:resource="http://purl.obolibrary.org/obo/BFO_0000115"/>
                        <owl:someValuesFrom rdf:resource="https://hack.cybersystems.engineer/memex/ontologies/SeamlessDigitalEngineering#Complete_Assurance_Case_Report"/>
                    </owl:Restriction>
                    <owl:Restriction>
                        <owl:onProperty rdf:resource="http://purl.obolibrary.org/obo/BFO_0000196"/>
                        <owl:someValuesFrom rdf:resource="https://hack.cybersystems.engineer/memex/ontologies/SeamlessDigitalEngineering#Trustworthy_Role"/>
                    </owl:Restriction>
                    <owl:Restriction>
                        <owl:onProperty rdf:resource="https://www.commoncoreontologies.org/ont00001936"/>
                        <owl:someValuesFrom rdf:resource="https://hack.cybersystems.engineer/memex/ontologies/SeamlessDigitalEngineering#Act_of_Assurance_Evaluation"/>
                    </owl:Restriction>
                </owl:intersectionOf>
            </owl:Class>
        </owl:equivalentClass>
        <rdfs:subClassOf rdf:resource="http://www.ontologyrepository.com/CommonCoreOntologies/ComputerSystem"/>
        <rdfs:label xml:lang="en">Trustworthy Computing Base</rdfs:label>
    </owl:Class>
    


    <!-- https://hack.cybersystems.engineer/memex/ontologies/SeamlessDigitalEngineering#Trustworthy_Organization -->

    <owl:Class rdf:about="https://hack.cybersystems.engineer/memex/ontologies/SeamlessDigitalEngineering#Trustworthy_Organization">
        <rdfs:subClassOf rdf:resource="https://www.commoncoreontologies.org/ont00001180"/>
        <rdfs:subClassOf>
            <owl:Restriction>
                <owl:onProperty rdf:resource="http://purl.obolibrary.org/obo/BFO_0000196"/>
                <owl:someValuesFrom rdf:resource="https://hack.cybersystems.engineer/memex/ontologies/SeamlessDigitalEngineering#Trustworthy_Role"/>
            </owl:Restriction>
        </rdfs:subClassOf>
        <rdfs:label xml:lang="en">Trustworthy Organization</rdfs:label>
    </owl:Class>
    


    <!-- https://hack.cybersystems.engineer/memex/ontologies/SeamlessDigitalEngineering#Trustworthy_Person -->

    <owl:Class rdf:about="https://hack.cybersystems.engineer/memex/ontologies/SeamlessDigitalEngineering#Trustworthy_Person">
        <rdfs:subClassOf rdf:resource="https://www.commoncoreontologies.org/ont00001262"/>
        <rdfs:subClassOf>
            <owl:Restriction>
                <owl:onProperty rdf:resource="http://purl.obolibrary.org/obo/BFO_0000196"/>
                <owl:someValuesFrom rdf:resource="https://hack.cybersystems.engineer/memex/ontologies/SeamlessDigitalEngineering#Trustworthy_Role"/>
            </owl:Restriction>
        </rdfs:subClassOf>
        <rdfs:label xml:lang="en">Trustworthy Person</rdfs:label>
    </owl:Class>
    


    <!-- https://hack.cybersystems.engineer/memex/ontologies/SeamlessDigitalEngineering#Trustworthy_Role -->

    <owl:Class rdf:about="https://hack.cybersystems.engineer/memex/ontologies/SeamlessDigitalEngineering#Trustworthy_Role">
        <rdfs:subClassOf rdf:resource="http://purl.obolibrary.org/obo/BFO_0000023"/>
        <rdfs:comment xml:lang="en">a System may also realize the Trustworthy Role</rdfs:comment>
        <rdfs:label xml:lang="en">Trustworthy Role</rdfs:label>
        <rdfs:seeAlso rdf:resource="https://hack.cybersystems.engineer/memex/ontologies/SeamlessDigitalEngineering#Trustworthiness"/>
        <skos:definition xml:lang="en">a role that denotes Evidence-based Trustworthiness</skos:definition>
    </owl:Class>
    


    <!-- https://hack.cybersystems.engineer/memex/ontologies/SeamlessDigitalEngineering#Trustworthy_System -->

    <owl:Class rdf:about="https://hack.cybersystems.engineer/memex/ontologies/SeamlessDigitalEngineering#Trustworthy_System">
        <rdfs:subClassOf rdf:resource="https://hack.cybersystems.engineer/memex/ontologies/SeamlessDigitalEngineering#System"/>
        <rdfs:label xml:lang="en">Trustworthy System</rdfs:label>
        <rdfs:seeAlso rdf:datatype="http://www.w3.org/2001/XMLSchema#anyURI">https://www.it-cisq.org/trustworthy-systems-manifesto</rdfs:seeAlso>
    </owl:Class>
    


    <!-- https://hack.cybersystems.engineer/memex/ontologies/SeamlessDigitalEngineering#Tutorial -->

    <owl:Class rdf:about="https://hack.cybersystems.engineer/memex/ontologies/SeamlessDigitalEngineering#Tutorial">
        <rdfs:subClassOf rdf:resource="https://www.commoncoreontologies.org/ont00000798"/>
        <rdfs:subClassOf>
            <owl:Restriction>
                <owl:onProperty rdf:resource="http://purl.obolibrary.org/obo/BFO_0000101"/>
                <owl:someValuesFrom rdf:resource="https://hack.cybersystems.engineer/memex/ontologies/SeamlessDigitalEngineering#Knowledge"/>
            </owl:Restriction>
        </rdfs:subClassOf>
        <rdfs:comment xml:lang="en">A Tutorial is an experience that takes place under the guidance of a Tutor. A Tutorial is always Learning-oriented.</rdfs:comment>
        <rdfs:label xml:lang="en">Tutorial</rdfs:label>
        <skos:definition xml:lang="en">Information Bearing Artifact which describes a practical Activity, in which the Stakeholder acquires Knowledge by doing something meaningful, towards some achievable Goal.</skos:definition>
        <cco2:ont00001754 rdf:datatype="http://www.w3.org/2001/XMLSchema#anyURI">https://diataxis.fr/tutorials/</cco2:ont00001754>
    </owl:Class>
    


    <!-- https://hack.cybersystems.engineer/memex/ontologies/SeamlessDigitalEngineering#Uncertainty -->

    <owl:Class rdf:about="https://hack.cybersystems.engineer/memex/ontologies/SeamlessDigitalEngineering#Uncertainty">
        <owl:equivalentClass>
            <owl:Class>
                <owl:intersectionOf rdf:parseType="Collection">
                    <owl:Restriction>
                        <owl:onProperty rdf:resource="http://purl.obolibrary.org/obo/BFO_0000059"/>
                        <owl:someValuesFrom rdf:resource="https://hack.cybersystems.engineer/memex/ontologies/SeamlessDigitalEngineering#Knowledge"/>
                    </owl:Restriction>
                    <owl:Restriction>
                        <owl:onProperty rdf:resource="https://www.commoncoreontologies.org/ont00001803"/>
                        <owl:someValuesFrom rdf:resource="https://hack.cybersystems.engineer/memex/ontologies/SeamlessDigitalEngineering#Risk"/>
                    </owl:Restriction>
                    <owl:Restriction>
                        <owl:onProperty rdf:resource="https://www.commoncoreontologies.org/ont00001888"/>
                        <owl:someValuesFrom rdf:resource="http://purl.obolibrary.org/obo/BFO_0000015"/>
                    </owl:Restriction>
                </owl:intersectionOf>
            </owl:Class>
        </owl:equivalentClass>
        <rdfs:subClassOf rdf:resource="https://www.commoncoreontologies.org/ont00001289"/>
        <rdfs:label xml:lang="en">Uncertainty</rdfs:label>
        <skos:definition xml:lang="en">the state, even partial, of deficiency of information related to understanding or knowledge of an event, its consequence, or likelihood.</skos:definition>
        <cco2:ont00001754 xml:lang="en">ISO/IEC/IEEE 15288:2023</cco2:ont00001754>
    </owl:Class>
    


    <!-- https://hack.cybersystems.engineer/memex/ontologies/SeamlessDigitalEngineering#Undeveloped_Assurance_Argument_Record -->

    <owl:Class rdf:about="https://hack.cybersystems.engineer/memex/ontologies/SeamlessDigitalEngineering#Undeveloped_Assurance_Argument_Record">
        <rdfs:subClassOf rdf:resource="https://hack.cybersystems.engineer/memex/ontologies/SeamlessDigitalEngineering#Assurance_Argument_Record"/>
        <rdfs:label xml:lang="en">Undeveloped Assurance Argument Record</rdfs:label>
        <skos:definition xml:lang="en">placeholder Argument to be replaced by a concrete Argument</skos:definition>
        <skos:editorialNote xml:lang="en">Undeveloped Assurance Argument Records contain nothing:

```
&apos;Assurance Argument Record&apos;
 and (&apos;has member part&apos; exactly 0 &apos;Assurance Context List&apos;)
 and (&apos;has member part&apos; exactly 0 &apos;Evidence Report&apos;)
 and (&apos;has member part&apos; exactly 0 &apos;Inference Argument Record&apos;)
```</skos:editorialNote>
        <cco2:ont00001754 xml:lang="en">ISO/IEC/IEEE 15026-2:2022</cco2:ont00001754>
    </owl:Class>
    


    <!-- https://hack.cybersystems.engineer/memex/ontologies/SeamlessDigitalEngineering#Usability -->

    <owl:Class rdf:about="https://hack.cybersystems.engineer/memex/ontologies/SeamlessDigitalEngineering#Usability">
        <rdfs:subClassOf rdf:resource="https://hack.cybersystems.engineer/memex/ontologies/SeamlessDigitalEngineering#Beneficialness"/>
        <rdfs:label xml:lang="en">Usability</rdfs:label>
        <skos:definition xml:lang="en">extent to which a System, Product or Service can be used by specified Users to achieve specified Goals with effectiveness, efficiency, and satisfaction in a specified context of use</skos:definition>
        <cco2:ont00001754 xml:lang="en">ISO/IEC 25019:2023(en)
Systems and software engineering — Systems and software Quality Requirements and Evaluation (SQuaRE) — Quality-in-use model</cco2:ont00001754>
    </owl:Class>
    


    <!-- https://hack.cybersystems.engineer/memex/ontologies/SeamlessDigitalEngineering#User -->

    <owl:Class rdf:about="https://hack.cybersystems.engineer/memex/ontologies/SeamlessDigitalEngineering#User">
        <rdfs:subClassOf rdf:resource="https://hack.cybersystems.engineer/memex/ontologies/SeamlessDigitalEngineering#Customer"/>
        <skos:definition xml:lang="en">individual or group that interacts with a System or benefits from a system during its utilization</skos:definition>
        <cco2:ont00001754>ISO/IEC/IEEE 15288:2023</cco2:ont00001754>
    </owl:Class>
    


    <!-- https://hack.cybersystems.engineer/memex/ontologies/SeamlessDigitalEngineering#Utilization_Lifecycle_Stage -->

    <owl:Class rdf:about="https://hack.cybersystems.engineer/memex/ontologies/SeamlessDigitalEngineering#Utilization_Lifecycle_Stage">
        <rdfs:subClassOf rdf:resource="https://www.commoncoreontologies.org/ont00001191"/>
        <rdfs:label xml:lang="en">Utilization Lifecycle Stage</rdfs:label>
        <cco2:ont00001754 xml:lang="en">ISO/IEC/IEEE 15288:2023</cco2:ont00001754>
    </owl:Class>
    


    <!-- https://hack.cybersystems.engineer/memex/ontologies/SeamlessDigitalEngineering#Utilization_Stage -->

    <owl:Class rdf:about="https://hack.cybersystems.engineer/memex/ontologies/SeamlessDigitalEngineering#Utilization_Stage">
        <rdfs:subClassOf rdf:resource="https://hack.cybersystems.engineer/memex/ontologies/SeamlessDigitalEngineering#Lifecycle_Stage"/>
        <rdfs:comment xml:lang="en">Purpose: The utilization stage is executed to operate the system, to deliver services within intended environments and to help achieve continuing operational effectiveness.</rdfs:comment>
        <rdfs:label xml:lang="en">Utilization Stage</rdfs:label>
        <cco2:ont00001754>ISO/IEC/IEEE 24748-1:2024</cco2:ont00001754>
    </owl:Class>
    


    <!-- https://hack.cybersystems.engineer/memex/ontologies/SeamlessDigitalEngineering#Validation_Process -->

    <owl:Class rdf:about="https://hack.cybersystems.engineer/memex/ontologies/SeamlessDigitalEngineering#Validation_Process">
        <rdfs:subClassOf rdf:resource="https://hack.cybersystems.engineer/memex/ontologies/SeamlessDigitalEngineering#Technical_Process"/>
        <rdfs:label xml:lang="en">Validation Process</rdfs:label>
        <skos:definition xml:lang="en">The purpose of the validation process is to provide objective evidence that the system, when in use, fulfils its business or mission objectives and stakeholder needs and requirements, achieving its intended use in its intended operational environment.</skos:definition>
        <cco2:ont00001754>ISO/IEC/IEEE 15288:2023</cco2:ont00001754>
    </owl:Class>
    


    <!-- https://hack.cybersystems.engineer/memex/ontologies/SeamlessDigitalEngineering#Validation_Report -->

    <owl:Class rdf:about="https://hack.cybersystems.engineer/memex/ontologies/SeamlessDigitalEngineering#Validation_Report">
        <rdfs:subClassOf rdf:resource="https://www.commoncoreontologies.org/ont00000624"/>
        <rdfs:label xml:lang="en">Validation Report</rdfs:label>
    </owl:Class>
    


    <!-- https://hack.cybersystems.engineer/memex/ontologies/SeamlessDigitalEngineering#Verification_Process -->

    <owl:Class rdf:about="https://hack.cybersystems.engineer/memex/ontologies/SeamlessDigitalEngineering#Verification_Process">
        <rdfs:subClassOf rdf:resource="https://hack.cybersystems.engineer/memex/ontologies/SeamlessDigitalEngineering#Technical_Process"/>
        <rdfs:label xml:lang="en">Verification Process</rdfs:label>
        <skos:definition xml:lang="en">The purpose of the Verification Process is to provide objective Evidence that a System, System Element, or Material Artifact fulfils its specified Requirements and Characteristics.</skos:definition>
        <cco2:ont00001754>ISO/IEC/IEEE 15288:2023</cco2:ont00001754>
    </owl:Class>
    


    <!-- https://hack.cybersystems.engineer/memex/ontologies/SeamlessDigitalEngineering#Verification_Report -->

    <owl:Class rdf:about="https://hack.cybersystems.engineer/memex/ontologies/SeamlessDigitalEngineering#Verification_Report">
        <rdfs:subClassOf rdf:resource="https://www.commoncoreontologies.org/ont00000624"/>
    </owl:Class>
    


    <!-- https://hack.cybersystems.engineer/memex/ontologies/SeamlessDigitalEngineering#View -->

    <owl:Class rdf:about="https://hack.cybersystems.engineer/memex/ontologies/SeamlessDigitalEngineering#View">
        <owl:equivalentClass>
            <owl:Class>
                <owl:intersectionOf rdf:parseType="Collection">
                    <rdf:Description rdf:about="https://www.commoncoreontologies.org/ont00001069"/>
                    <owl:Restriction>
                        <owl:onProperty rdf:resource="https://www.commoncoreontologies.org/ont00001920"/>
                        <owl:someValuesFrom rdf:resource="https://hack.cybersystems.engineer/memex/ontologies/SeamlessDigitalEngineering#Viewpoint"/>
                    </owl:Restriction>
                </owl:intersectionOf>
            </owl:Class>
        </owl:equivalentClass>
        <rdfs:subClassOf rdf:resource="https://www.commoncoreontologies.org/ont00001069"/>
        <rdfs:label xml:lang="en">View</rdfs:label>
        <skos:definition xml:lang="en">A representation of an entity from the perspective of a related set of Concerns</skos:definition>
        <cco2:ont00001754 xml:lang="en">adapted from ISO/IEC/IEEE 15288:2023</cco2:ont00001754>
        <cco2:ont00001760 rdf:datatype="http://www.w3.org/2001/XMLSchema#anyURI">https://semantic.incose.org/DEIX_Ontology</cco2:ont00001760>
    </owl:Class>
    


    <!-- https://hack.cybersystems.engineer/memex/ontologies/SeamlessDigitalEngineering#Viewpoint -->

    <owl:Class rdf:about="https://hack.cybersystems.engineer/memex/ontologies/SeamlessDigitalEngineering#Viewpoint">
        <owl:equivalentClass>
            <owl:Class>
                <owl:intersectionOf rdf:parseType="Collection">
                    <rdf:Description rdf:about="https://www.commoncoreontologies.org/ont00000965"/>
                    <owl:Restriction>
                        <owl:onProperty rdf:resource="https://www.commoncoreontologies.org/ont00001808"/>
                        <owl:someValuesFrom rdf:resource="https://hack.cybersystems.engineer/memex/ontologies/SeamlessDigitalEngineering#Concern_Expression"/>
                    </owl:Restriction>
                    <owl:Restriction>
                        <owl:onProperty rdf:resource="https://www.commoncoreontologies.org/ont00001942"/>
                        <owl:someValuesFrom rdf:resource="https://hack.cybersystems.engineer/memex/ontologies/SeamlessDigitalEngineering#View"/>
                    </owl:Restriction>
                </owl:intersectionOf>
            </owl:Class>
        </owl:equivalentClass>
        <rdfs:subClassOf rdf:resource="https://www.commoncoreontologies.org/ont00000965"/>
        <rdfs:comment xml:lang="en">Specification of the conventions for constructing and using a View

Source: ISO/IEC/IEEE 15288:2023</rdfs:comment>
        <rdfs:label xml:lang="en">Viewpoint</rdfs:label>
        <skos:definition xml:lang="en">A set of conventions for the creation, interpretation and use of a View to frame one or more Concerns</skos:definition>
        <cco2:ont00001754 xml:lang="en">derived from ISO/IEC/IEEE 24641:2023 - Systems and Software engineering — Methods and tools for model-based systems and software engineering</cco2:ont00001754>
        <cco2:ont00001760 rdf:datatype="http://www.w3.org/2001/XMLSchema#anyURI">https://semantic.incose.org/DEIX_Ontology</cco2:ont00001760>
    </owl:Class>
    


    <!-- https://hack.cybersystems.engineer/memex/ontologies/SeamlessDigitalEngineering#Virtual_SoS -->

    <owl:Class rdf:about="https://hack.cybersystems.engineer/memex/ontologies/SeamlessDigitalEngineering#Virtual_SoS">
        <rdfs:subClassOf rdf:resource="https://hack.cybersystems.engineer/memex/ontologies/SeamlessDigitalEngineering#System-of-Systems"/>
        <rdfs:label xml:lang="en">Virtual System-of-Systems</rdfs:label>
        <skos:definition xml:lang="en">The SoS lacks a central management authority and a centrally agreed upon purpose for the SoS. Large-scale behavior emerges-and may be desirable-but this type of SoS must rely on relatively invisible mechanisms to maintain it.</skos:definition>
        <cco2:ont00001754 xml:lang="en">ISO/IEC/IEEE 21841 - Systems and software engineering - Taxonomy of systems of systems</cco2:ont00001754>
    </owl:Class>
    


    <!-- https://hack.cybersystems.engineer/memex/ontologies/SeamlessDigitalEngineering#V&amp;V_Environment -->

    <owl:Class rdf:about="https://hack.cybersystems.engineer/memex/ontologies/SeamlessDigitalEngineering#V&amp;V_Environment">
        <owl:equivalentClass>
            <owl:Class>
                <owl:intersectionOf rdf:parseType="Collection">
                    <rdf:Description rdf:about="https://hack.cybersystems.engineer/memex/ontologies/SeamlessDigitalEngineering#System_Environment"/>
                    <owl:Restriction>
                        <owl:onProperty rdf:resource="http://purl.obolibrary.org/obo/BFO_0000183"/>
                        <owl:someValuesFrom>
                            <owl:Class>
                                <owl:unionOf rdf:parseType="Collection">
                                    <rdf:Description rdf:about="https://hack.cybersystems.engineer/memex/ontologies/SeamlessDigitalEngineering#Validation_Process"/>
                                    <rdf:Description rdf:about="https://hack.cybersystems.engineer/memex/ontologies/SeamlessDigitalEngineering#Verification_Process"/>
                                </owl:unionOf>
                            </owl:Class>
                        </owl:someValuesFrom>
                    </owl:Restriction>
                </owl:intersectionOf>
            </owl:Class>
        </owl:equivalentClass>
        <rdfs:subClassOf rdf:resource="https://hack.cybersystems.engineer/memex/ontologies/SeamlessDigitalEngineering#System_Environment"/>
        <rdfs:label xml:lang="en">V&amp;V Environment</rdfs:label>
        <cco2:ont00001760 rdf:datatype="http://www.w3.org/2001/XMLSchema#anyURI">https://semantic.incose.org/DEIX_Ontology</cco2:ont00001760>
    </owl:Class>
    


    <!-- https://www.commoncoreontologies.org/ont00000004 -->

    <owl:Class rdf:about="https://www.commoncoreontologies.org/ont00000004"/>
    


    <!-- https://www.commoncoreontologies.org/ont00000005 -->

    <owl:Class rdf:about="https://www.commoncoreontologies.org/ont00000005"/>
    


    <!-- https://www.commoncoreontologies.org/ont00000038 -->

    <owl:Class rdf:about="https://www.commoncoreontologies.org/ont00000038"/>
    


    <!-- https://www.commoncoreontologies.org/ont00000069 -->

    <owl:Class rdf:about="https://www.commoncoreontologies.org/ont00000069"/>
    


    <!-- https://www.commoncoreontologies.org/ont00000110 -->

    <owl:Class rdf:about="https://www.commoncoreontologies.org/ont00000110"/>
    


    <!-- https://www.commoncoreontologies.org/ont00000118 -->

    <owl:Class rdf:about="https://www.commoncoreontologies.org/ont00000118"/>
    


    <!-- https://www.commoncoreontologies.org/ont00000127 -->

    <owl:Class rdf:about="https://www.commoncoreontologies.org/ont00000127"/>
    


    <!-- https://www.commoncoreontologies.org/ont00000133 -->

    <owl:Class rdf:about="https://www.commoncoreontologies.org/ont00000133"/>
    


    <!-- https://www.commoncoreontologies.org/ont00000146 -->

    <owl:Class rdf:about="https://www.commoncoreontologies.org/ont00000146"/>
    


    <!-- https://www.commoncoreontologies.org/ont00000175 -->

    <owl:Class rdf:about="https://www.commoncoreontologies.org/ont00000175"/>
    


    <!-- https://www.commoncoreontologies.org/ont00000187 -->

    <owl:Class rdf:about="https://www.commoncoreontologies.org/ont00000187"/>
    


    <!-- https://www.commoncoreontologies.org/ont00000189 -->

    <owl:Class rdf:about="https://www.commoncoreontologies.org/ont00000189"/>
    


    <!-- https://www.commoncoreontologies.org/ont00000203 -->

    <owl:Class rdf:about="https://www.commoncoreontologies.org/ont00000203"/>
    


    <!-- https://www.commoncoreontologies.org/ont00000228 -->

    <owl:Class rdf:about="https://www.commoncoreontologies.org/ont00000228"/>
    


    <!-- https://www.commoncoreontologies.org/ont00000314 -->

    <owl:Class rdf:about="https://www.commoncoreontologies.org/ont00000314"/>
    


    <!-- https://www.commoncoreontologies.org/ont00000319 -->

    <owl:Class rdf:about="https://www.commoncoreontologies.org/ont00000319"/>
    


    <!-- https://www.commoncoreontologies.org/ont00000345 -->

    <owl:Class rdf:about="https://www.commoncoreontologies.org/ont00000345"/>
    


    <!-- https://www.commoncoreontologies.org/ont00000379 -->

    <owl:Class rdf:about="https://www.commoncoreontologies.org/ont00000379"/>
    


    <!-- https://www.commoncoreontologies.org/ont00000402 -->

    <owl:Class rdf:about="https://www.commoncoreontologies.org/ont00000402"/>
    


    <!-- https://www.commoncoreontologies.org/ont00000408 -->

    <owl:Class rdf:about="https://www.commoncoreontologies.org/ont00000408"/>
    


    <!-- https://www.commoncoreontologies.org/ont00000420 -->

    <owl:Class rdf:about="https://www.commoncoreontologies.org/ont00000420"/>
    


    <!-- https://www.commoncoreontologies.org/ont00000443 -->

    <owl:Class rdf:about="https://www.commoncoreontologies.org/ont00000443"/>
    


    <!-- https://www.commoncoreontologies.org/ont00000476 -->

    <owl:Class rdf:about="https://www.commoncoreontologies.org/ont00000476">
        <owl:equivalentClass>
            <owl:Class>
                <owl:intersectionOf rdf:parseType="Collection">
                    <rdf:Description rdf:about="https://hack.cybersystems.engineer/memex/ontologies/SeamlessDigitalEngineering#Need"/>
                    <owl:Restriction>
                        <owl:onProperty rdf:resource="http://purl.obolibrary.org/obo/BFO_0000176"/>
                        <owl:someValuesFrom rdf:resource="https://hack.cybersystems.engineer/memex/ontologies/SeamlessDigitalEngineering#Goal"/>
                    </owl:Restriction>
                </owl:intersectionOf>
            </owl:Class>
        </owl:equivalentClass>
        <skos:definition xml:lang="en">Objectives are upper-level Needs that form the third level of the hierarchy of the Integrated Set of Needs. Objectives are elaborated from the Goals providing more details concerning what must be done to meet the Goals that will result in the Mission to be achieved i.e., what the Project Team and the System to be developed need to achieve so the System can fulfill its intended Purpose (Mission) in its Operational Environment when operated by its intended Users.</skos:definition>
        <cco2:ont00001754>INCOSE Needs and Requirements Manual R1.1 (2022)</cco2:ont00001754>
    </owl:Class>
    


    <!-- https://www.commoncoreontologies.org/ont00000485 -->

    <owl:Class rdf:about="https://www.commoncoreontologies.org/ont00000485"/>
    


    <!-- https://www.commoncoreontologies.org/ont00000496 -->

    <owl:Class rdf:about="https://www.commoncoreontologies.org/ont00000496"/>
    


    <!-- https://www.commoncoreontologies.org/ont00000509 -->

    <owl:Class rdf:about="https://www.commoncoreontologies.org/ont00000509">
        <owl:equivalentClass>
            <owl:Restriction>
                <owl:onProperty rdf:resource="https://www.commoncoreontologies.org/ont00001898"/>
                <owl:someValuesFrom rdf:resource="https://hack.cybersystems.engineer/memex/ontologies/SeamlessDigitalEngineering#Service"/>
            </owl:Restriction>
        </owl:equivalentClass>
    </owl:Class>
    


    <!-- https://www.commoncoreontologies.org/ont00000513 -->

    <owl:Class rdf:about="https://www.commoncoreontologies.org/ont00000513"/>
    


    <!-- https://www.commoncoreontologies.org/ont00000517 -->

    <owl:Class rdf:about="https://www.commoncoreontologies.org/ont00000517"/>
    


    <!-- https://www.commoncoreontologies.org/ont00000544 -->

    <owl:Class rdf:about="https://www.commoncoreontologies.org/ont00000544"/>
    


    <!-- https://www.commoncoreontologies.org/ont00000555 -->

    <owl:Class rdf:about="https://www.commoncoreontologies.org/ont00000555"/>
    


    <!-- https://www.commoncoreontologies.org/ont00000564 -->

    <owl:Class rdf:about="https://www.commoncoreontologies.org/ont00000564"/>
    


    <!-- https://www.commoncoreontologies.org/ont00000566 -->

    <owl:Class rdf:about="https://www.commoncoreontologies.org/ont00000566"/>
    


    <!-- https://www.commoncoreontologies.org/ont00000574 -->

    <owl:Class rdf:about="https://www.commoncoreontologies.org/ont00000574"/>
    


    <!-- https://www.commoncoreontologies.org/ont00000575 -->

    <owl:Class rdf:about="https://www.commoncoreontologies.org/ont00000575"/>
    


    <!-- https://www.commoncoreontologies.org/ont00000581 -->

    <owl:Class rdf:about="https://www.commoncoreontologies.org/ont00000581"/>
    


    <!-- https://www.commoncoreontologies.org/ont00000604 -->

    <owl:Class rdf:about="https://www.commoncoreontologies.org/ont00000604"/>
    


    <!-- https://www.commoncoreontologies.org/ont00000622 -->

    <owl:Class rdf:about="https://www.commoncoreontologies.org/ont00000622"/>
    


    <!-- https://www.commoncoreontologies.org/ont00000624 -->

    <owl:Class rdf:about="https://www.commoncoreontologies.org/ont00000624">
        <rdfs:comment xml:lang="en">A Report communicates decisions.</rdfs:comment>
        <rdfs:comment xml:lang="en">A Report shall include the following Information Parts:

a) date of issue and status;
b) scope;
c) issuing organization;
d) contributors;
e) summary;
f) introduction, including the purpose, audience and scope of the report;
g) context (assumptions);
h) body (including methods of obtaining results);
i) conclusions and recommendations;
j) references;
k) bibliography;
l) glossary; and
m) change history.</rdfs:comment>
        <rdfs:comment xml:lang="en">The Purpose of a Report is to describe the results of Activities such as investigations, assessments, and tests.</rdfs:comment>
        <cco2:ont00001754 xml:lang="en">ISO/IEC/IEEE 15289:2019</cco2:ont00001754>
    </owl:Class>
    


    <!-- https://www.commoncoreontologies.org/ont00000636 -->

    <owl:Class rdf:about="https://www.commoncoreontologies.org/ont00000636"/>
    


    <!-- https://www.commoncoreontologies.org/ont00000647 -->

    <owl:Class rdf:about="https://www.commoncoreontologies.org/ont00000647"/>
    


    <!-- https://www.commoncoreontologies.org/ont00000660 -->

    <owl:Class rdf:about="https://www.commoncoreontologies.org/ont00000660"/>
    


    <!-- https://www.commoncoreontologies.org/ont00000696 -->

    <owl:Class rdf:about="https://www.commoncoreontologies.org/ont00000696"/>
    


    <!-- https://www.commoncoreontologies.org/ont00000700 -->

    <owl:Class rdf:about="https://www.commoncoreontologies.org/ont00000700">
        <skos:altLabel xml:lang="en">Digital Network</skos:altLabel>
    </owl:Class>
    


    <!-- https://www.commoncoreontologies.org/ont00000731 -->

    <owl:Class rdf:about="https://www.commoncoreontologies.org/ont00000731"/>
    


    <!-- https://www.commoncoreontologies.org/ont00000740 -->

    <owl:Class rdf:about="https://www.commoncoreontologies.org/ont00000740"/>
    


    <!-- https://www.commoncoreontologies.org/ont00000756 -->

    <owl:Class rdf:about="https://www.commoncoreontologies.org/ont00000756"/>
    


    <!-- https://www.commoncoreontologies.org/ont00000768 -->

    <owl:Class rdf:about="https://www.commoncoreontologies.org/ont00000768"/>
    


    <!-- https://www.commoncoreontologies.org/ont00000798 -->

    <owl:Class rdf:about="https://www.commoncoreontologies.org/ont00000798"/>
    


    <!-- https://www.commoncoreontologies.org/ont00000836 -->

    <owl:Class rdf:about="https://www.commoncoreontologies.org/ont00000836"/>
    


    <!-- https://www.commoncoreontologies.org/ont00000847 -->

    <owl:Class rdf:about="https://www.commoncoreontologies.org/ont00000847"/>
    


    <!-- https://www.commoncoreontologies.org/ont00000853 -->

    <owl:Class rdf:about="https://www.commoncoreontologies.org/ont00000853"/>
    


    <!-- https://www.commoncoreontologies.org/ont00000856 -->

    <owl:Class rdf:about="https://www.commoncoreontologies.org/ont00000856"/>
    


    <!-- https://www.commoncoreontologies.org/ont00000908 -->

    <owl:Class rdf:about="https://www.commoncoreontologies.org/ont00000908"/>
    


    <!-- https://www.commoncoreontologies.org/ont00000914 -->

    <owl:Class rdf:about="https://www.commoncoreontologies.org/ont00000914"/>
    


    <!-- https://www.commoncoreontologies.org/ont00000929 -->

    <owl:Class rdf:about="https://www.commoncoreontologies.org/ont00000929"/>
    


    <!-- https://www.commoncoreontologies.org/ont00000932 -->

    <owl:Class rdf:about="https://www.commoncoreontologies.org/ont00000932"/>
    


    <!-- https://www.commoncoreontologies.org/ont00000958 -->

    <owl:Class rdf:about="https://www.commoncoreontologies.org/ont00000958">
        <rdfs:comment xml:lang="en">information:
facts, concepts or instructions

Source: ISO 10303-2:2024 Industrial automation systems and integration - Product data representation and exchange - Part 2: Vocabulary, 3.1.227</rdfs:comment>
    </owl:Class>
    


    <!-- https://www.commoncoreontologies.org/ont00000965 -->

    <owl:Class rdf:about="https://www.commoncoreontologies.org/ont00000965"/>
    


    <!-- https://www.commoncoreontologies.org/ont00000970 -->

    <owl:Class rdf:about="https://www.commoncoreontologies.org/ont00000970"/>
    


    <!-- https://www.commoncoreontologies.org/ont00000974 -->

    <owl:Class rdf:about="https://www.commoncoreontologies.org/ont00000974"/>
    


    <!-- https://www.commoncoreontologies.org/ont00000995 -->

    <owl:Class rdf:about="https://www.commoncoreontologies.org/ont00000995">
        <skos:definition xml:lang="en">Work product that is produced and used during a project to capture and convey information.</skos:definition>
        <cco2:ont00001754>ISO/IEC/IEEE 15288:2023</cco2:ont00001754>
    </owl:Class>
    


    <!-- https://www.commoncoreontologies.org/ont00000997 -->

    <owl:Class rdf:about="https://www.commoncoreontologies.org/ont00000997"/>
    


    <!-- https://www.commoncoreontologies.org/ont00001006 -->

    <owl:Class rdf:about="https://www.commoncoreontologies.org/ont00001006"/>
    


    <!-- https://www.commoncoreontologies.org/ont00001010 -->

    <owl:Class rdf:about="https://www.commoncoreontologies.org/ont00001010"/>
    


    <!-- https://www.commoncoreontologies.org/ont00001017 -->

    <owl:Class rdf:about="https://www.commoncoreontologies.org/ont00001017"/>
    


    <!-- https://www.commoncoreontologies.org/ont00001032 -->

    <owl:Class rdf:about="https://www.commoncoreontologies.org/ont00001032"/>
    


    <!-- https://www.commoncoreontologies.org/ont00001045 -->

    <owl:Class rdf:about="https://www.commoncoreontologies.org/ont00001045"/>
    


    <!-- https://www.commoncoreontologies.org/ont00001066 -->

    <owl:Class rdf:about="https://www.commoncoreontologies.org/ont00001066"/>
    


    <!-- https://www.commoncoreontologies.org/ont00001069 -->

    <owl:Class rdf:about="https://www.commoncoreontologies.org/ont00001069"/>
    


    <!-- https://www.commoncoreontologies.org/ont00001100 -->

    <owl:Class rdf:about="https://www.commoncoreontologies.org/ont00001100"/>
    


    <!-- https://www.commoncoreontologies.org/ont00001119 -->

    <owl:Class rdf:about="https://www.commoncoreontologies.org/ont00001119"/>
    


    <!-- https://www.commoncoreontologies.org/ont00001163 -->

    <owl:Class rdf:about="https://www.commoncoreontologies.org/ont00001163"/>
    


    <!-- https://www.commoncoreontologies.org/ont00001180 -->

    <owl:Class rdf:about="https://www.commoncoreontologies.org/ont00001180">
        <skos:definition xml:lang="en">person or group of people that has its own functions with responsibilities, authorities, and relationships to achieve its Objectives.</skos:definition>
        <skos:example xml:lang="en">Company, corporation, firm, enterprise, manufacturer, institution, charity, sole trader, association, or parts or combination thereof.</skos:example>
        <cco2:ont00001754>ISO/IEC/IEEE 15288:2023</cco2:ont00001754>
    </owl:Class>
    


    <!-- https://www.commoncoreontologies.org/ont00001191 -->

    <owl:Class rdf:about="https://www.commoncoreontologies.org/ont00001191"/>
    


    <!-- https://www.commoncoreontologies.org/ont00001262 -->

    <owl:Class rdf:about="https://www.commoncoreontologies.org/ont00001262"/>
    


    <!-- https://www.commoncoreontologies.org/ont00001289 -->

    <owl:Class rdf:about="https://www.commoncoreontologies.org/ont00001289"/>
    


    <!-- https://www.commoncoreontologies.org/ont00001298 -->

    <owl:Class rdf:about="https://www.commoncoreontologies.org/ont00001298"/>
    


    <!-- https://www.commoncoreontologies.org/ont00001324 -->

    <owl:Class rdf:about="https://www.commoncoreontologies.org/ont00001324"/>
    


    <!-- https://www.commoncoreontologies.org/ont00001334 -->

    <owl:Class rdf:about="https://www.commoncoreontologies.org/ont00001334"/>
    


    <!-- https://www.commoncoreontologies.org/ont00001347 -->

    <owl:Class rdf:about="https://www.commoncoreontologies.org/ont00001347">
        <owl:equivalentClass>
            <owl:Class>
                <owl:intersectionOf rdf:parseType="Collection">
                    <rdf:Description rdf:about="https://www.commoncoreontologies.org/ont00000005"/>
                    <owl:Restriction>
                        <owl:onProperty rdf:resource="https://www.commoncoreontologies.org/ont00001833"/>
                        <owl:someValuesFrom rdf:resource="https://hack.cybersystems.engineer/memex/ontologies/SeamlessDigitalEngineering#System"/>
                    </owl:Restriction>
                </owl:intersectionOf>
            </owl:Class>
        </owl:equivalentClass>
        <rdfs:comment xml:lang="en">observable activity of a system, measurable in terms of quantifiable effects on the environment whether arising from internal or external stimulus

Source: ISO/IEC/IEEE 24765:2017</rdfs:comment>
    </owl:Class>
    


    <!-- https://www.commoncoreontologies.org/ont00001359 -->

    <owl:Class rdf:about="https://www.commoncoreontologies.org/ont00001359"/>
    


    <!-- https://www.commoncoreontologies.org/ont00001379 -->

    <owl:Class rdf:about="https://www.commoncoreontologies.org/ont00001379"/>
    


    <!-- 
    ///////////////////////////////////////////////////////////////////////////////////////
    //
    // Individuals
    //
    ///////////////////////////////////////////////////////////////////////////////////////
     -->

    


    <!-- https://hack.cybersystems.engineer/memex/ontologies/SeamlessDigitalEngineering#AFRL_Digital_Laboratory_Environment -->

    <owl:NamedIndividual rdf:about="https://hack.cybersystems.engineer/memex/ontologies/SeamlessDigitalEngineering#AFRL_Digital_Laboratory_Environment">
        <rdf:type rdf:resource="https://hack.cybersystems.engineer/memex/ontologies/SeamlessDigitalEngineering#Digital_Laboratory_Environment"/>
        <obo:BFO_0000176 rdf:resource="https://hack.cybersystems.engineer/memex/ontologies/SeamlessDigitalEngineering#United_States_Air_Force_Research_Laboratory"/>
        <rdfs:label xml:lang="en">AFRL Digital Laboratory Environment</rdfs:label>
        <rdfs:seeAlso rdf:datatype="http://www.w3.org/2001/XMLSchema#anyURI">https://afresearchlab.com/news/afrl-digital-transformation-progresses-enterprise-communications/</rdfs:seeAlso>
        <skos:altLabel xml:lang="en">AFRL DLE</skos:altLabel>
    </owl:NamedIndividual>
    


    <!-- https://hack.cybersystems.engineer/memex/ontologies/SeamlessDigitalEngineering#Accessibility_Cyber_Right -->

    <owl:NamedIndividual rdf:about="https://hack.cybersystems.engineer/memex/ontologies/SeamlessDigitalEngineering#Accessibility_Cyber_Right">
        <rdf:type rdf:resource="https://hack.cybersystems.engineer/memex/ontologies/SeamlessDigitalEngineering#Human_Cyber_Right"/>
        <rdfs:label xml:lang="en">Accessibility Cyber Right</rdfs:label>
        <skos:definition xml:lang="en">Every Person has an equal Right to access and use a secure and open Cyberspace.</skos:definition>
        <cco2:ont00001754 rdf:resource="https://hack.cybersystems.engineer/memex/ontologies/SeamlessDigitalEngineering#Charter_of_Human_Rights_and_Principles_for_the_Internet"/>
    </owl:NamedIndividual>
    


    <!-- https://hack.cybersystems.engineer/memex/ontologies/SeamlessDigitalEngineering#Bootstrappable_KQA -->

    <owl:NamedIndividual rdf:about="https://hack.cybersystems.engineer/memex/ontologies/SeamlessDigitalEngineering#Bootstrappable_KQA">
        <rdf:type rdf:resource="https://hack.cybersystems.engineer/memex/ontologies/SeamlessDigitalEngineering#Key_Quality_Attribute"/>
        <rdf:type>
            <owl:Restriction>
                <owl:onProperty rdf:resource="http://purl.obolibrary.org/obo/BFO_0000195"/>
                <owl:someValuesFrom rdf:resource="https://hack.cybersystems.engineer/memex/ontologies/SeamlessDigitalEngineering#Bootstrappability"/>
            </owl:Restriction>
        </rdf:type>
        <rdfs:label xml:lang="en">Bootstrappable KQA</rdfs:label>
    </owl:NamedIndividual>
    


    <!-- https://hack.cybersystems.engineer/memex/ontologies/SeamlessDigitalEngineering#CATIA_Magic_Cyber-Systems_Engineer -->

    <owl:NamedIndividual rdf:about="https://hack.cybersystems.engineer/memex/ontologies/SeamlessDigitalEngineering#CATIA_Magic_Cyber-Systems_Engineer">
        <rdf:type rdf:resource="https://hack.cybersystems.engineer/memex/ontologies/SeamlessDigitalEngineering#Digital_Tool"/>
        <obo:BFO_0000176 rdf:resource="https://hack.cybersystems.engineer/memex/ontologies/SeamlessDigitalEngineering#Dassault_Systemes"/>
        <cco2:ont00001976 rdf:resource="https://hack.cybersystems.engineer/memex/ontologies/SeamlessDigitalEngineering#Systems_Modeling_Language"/>
        <rdfs:label xml:lang="en">CATIA Magic Cyber-Systems Engineer</rdfs:label>
        <skos:definition xml:lang="en">The ‘Magic Cyber-Systems Engineer’ product is an industry leading cross-platform collaborative Model-Based Systems Engineering (MBSE) environment. It provides smart, robust, and intuitive tools to define, track, and visualize all aspects of systems in the most standard-compliant SysML models and diagrams.</skos:definition>
        <cco2:ont00001754 rdf:datatype="http://www.w3.org/2001/XMLSchema#anyURI">https://www.3ds.com/products/catia/catia-magic</cco2:ont00001754>
    </owl:NamedIndividual>
    


    <!-- https://hack.cybersystems.engineer/memex/ontologies/SeamlessDigitalEngineering#Charter_of_Human_Rights_and_Principles_for_the_Internet -->

    <owl:NamedIndividual rdf:about="https://hack.cybersystems.engineer/memex/ontologies/SeamlessDigitalEngineering#Charter_of_Human_Rights_and_Principles_for_the_Internet">
        <rdf:type>
            <owl:Class>
                <owl:intersectionOf rdf:parseType="Collection">
                    <rdf:Description rdf:about="https://www.commoncoreontologies.org/ont00001298"/>
                    <owl:Restriction>
                        <owl:onProperty rdf:resource="http://purl.obolibrary.org/obo/BFO_0000178"/>
                        <owl:someValuesFrom rdf:resource="https://hack.cybersystems.engineer/memex/ontologies/SeamlessDigitalEngineering#Right_Declaration"/>
                    </owl:Restriction>
                </owl:intersectionOf>
            </owl:Class>
        </rdf:type>
        <obo:BFO_0000101 rdf:resource="https://hack.cybersystems.engineer/memex/ontologies/SeamlessDigitalEngineering#Accessibility_Cyber_Right"/>
        <obo:BFO_0000101 rdf:resource="https://hack.cybersystems.engineer/memex/ontologies/SeamlessDigitalEngineering#Diversity_Cyber_Right"/>
        <obo:BFO_0000101 rdf:resource="https://hack.cybersystems.engineer/memex/ontologies/SeamlessDigitalEngineering#Expression_and_Association_Cyber_Right"/>
        <obo:BFO_0000101 rdf:resource="https://hack.cybersystems.engineer/memex/ontologies/SeamlessDigitalEngineering#Governance_Cyber_Right"/>
        <obo:BFO_0000101 rdf:resource="https://hack.cybersystems.engineer/memex/ontologies/SeamlessDigitalEngineering#Network_Equality_Cyber_Right"/>
        <obo:BFO_0000101 rdf:resource="https://hack.cybersystems.engineer/memex/ontologies/SeamlessDigitalEngineering#Privacy_and_Data_Protection_Cyber_Right"/>
        <obo:BFO_0000101 rdf:resource="https://hack.cybersystems.engineer/memex/ontologies/SeamlessDigitalEngineering#Rights_and_Social_Justice_Cyber_Right"/>
        <obo:BFO_0000101 rdf:resource="https://hack.cybersystems.engineer/memex/ontologies/SeamlessDigitalEngineering#Standards_and_Regulation_Cyber_Right"/>
        <obo:BFO_0000101 rdf:resource="https://hack.cybersystems.engineer/memex/ontologies/SeamlessDigitalEngineering#Universality_and_Equality_Cyber_Right"/>
        <obo:BFO_0000101 rdf:resource="https://hack.cybersystems.engineer/memex/ontologies/SeamlessDigitalEngineering#Life,_Libery_and_Security_Cyber_Right"/>
        <rdfs:label xml:lang="en">Charter of Human Rights and Principles for the Internet</rdfs:label>
        <rdfs:seeAlso rdf:datatype="http://www.w3.org/2001/XMLSchema#anyURI">https://internetrightsandprinciples.org/campaign/</rdfs:seeAlso>
    </owl:NamedIndividual>
    


    <!-- https://hack.cybersystems.engineer/memex/ontologies/SeamlessDigitalEngineering#Common_Criteria -->

    <owl:NamedIndividual rdf:about="https://hack.cybersystems.engineer/memex/ontologies/SeamlessDigitalEngineering#Common_Criteria"/>
    


    <!-- https://hack.cybersystems.engineer/memex/ontologies/SeamlessDigitalEngineering#Convivial_KQA -->

    <owl:NamedIndividual rdf:about="https://hack.cybersystems.engineer/memex/ontologies/SeamlessDigitalEngineering#Convivial_KQA">
        <rdf:type rdf:resource="https://hack.cybersystems.engineer/memex/ontologies/SeamlessDigitalEngineering#Key_Quality_Attribute"/>
        <rdf:type>
            <owl:Restriction>
                <owl:onProperty rdf:resource="http://purl.obolibrary.org/obo/BFO_0000195"/>
                <owl:someValuesFrom>
                    <owl:Class>
                        <owl:intersectionOf rdf:parseType="Collection">
                            <rdf:Description rdf:about="https://hack.cybersystems.engineer/memex/ontologies/SeamlessDigitalEngineering#Product_Capability"/>
                            <rdf:Description rdf:about="https://hack.cybersystems.engineer/memex/ontologies/SeamlessDigitalEngineering#Product_Quality-in-Use"/>
                        </owl:intersectionOf>
                    </owl:Class>
                </owl:someValuesFrom>
            </owl:Restriction>
        </rdf:type>
        <obo:BFO_0000195 rdf:resource="https://hack.cybersystems.engineer/memex/ontologies/SeamlessDigitalEngineering#Elegant_KQA"/>
        <obo:BFO_0000195 rdf:resource="https://hack.cybersystems.engineer/memex/ontologies/SeamlessDigitalEngineering#Seamless_KQA"/>
        <obo:BFO_0000195 rdf:resource="https://hack.cybersystems.engineer/memex/ontologies/SeamlessDigitalEngineering#Trustworthy_KQA"/>
        <rdfs:label xml:lang="en">Convivial KQA</rdfs:label>
        <skos:altLabel xml:lang="en">Conviviality</skos:altLabel>
        <skos:definition xml:lang="en">the Capability of Persons to interact creatively and autonomously with others and their environment to satisfy their own Needs.</skos:definition>
        <cco2:ont00001754 xml:lang="en">derived from https://en.wikipedia.org/Conviviality</cco2:ont00001754>
    </owl:NamedIndividual>
    


    <!-- https://hack.cybersystems.engineer/memex/ontologies/SeamlessDigitalEngineering#Dassault_Systemes -->

    <owl:NamedIndividual rdf:about="https://hack.cybersystems.engineer/memex/ontologies/SeamlessDigitalEngineering#Dassault_Systemes">
        <rdf:type rdf:resource="https://www.commoncoreontologies.org/ont00000443"/>
        <obo:BFO_0000178 rdf:resource="https://hack.cybersystems.engineer/memex/ontologies/SeamlessDigitalEngineering#CATIA_Magic_Cyber-Systems_Engineer"/>
        <rdfs:label xml:lang="en">Dassault Systemes</rdfs:label>
        <rdfs:label xml:lang="fr">Dassault Systèmes</rdfs:label>
        <rdfs:seeAlso rdf:datatype="http://www.w3.org/2001/XMLSchema#anyURI">http://3ds.com/</rdfs:seeAlso>
        <skos:definition xml:lang="en">Dassault Systèmes SE (French pronunciation: [daso sistɛm]) (abbreviated 3DS) is a French multinational software corporation which develops software for 3D product design, simulation, manufacturing and other 3D related products.</skos:definition>
        <cco2:ont00001754 rdf:datatype="http://www.w3.org/2001/XMLSchema#anyURI">https://en.wikipedia.org/wiki/Dassault_Syst%C3%A8mes</cco2:ont00001754>
    </owl:NamedIndividual>
    


    <!-- https://hack.cybersystems.engineer/memex/ontologies/SeamlessDigitalEngineering#Diversity_Cyber_Right -->

    <owl:NamedIndividual rdf:about="https://hack.cybersystems.engineer/memex/ontologies/SeamlessDigitalEngineering#Diversity_Cyber_Right">
        <rdf:type rdf:resource="https://hack.cybersystems.engineer/memex/ontologies/SeamlessDigitalEngineering#Human_Cyber_Right"/>
        <rdfs:label xml:lang="en">Diversity Cyber Right</rdfs:label>
        <skos:definition xml:lang="en">Cultural and linguistic diversity in Cyberspace must be promoted, and technical and policy innovation should be encouraged to facilitate plurality of expression.</skos:definition>
        <cco2:ont00001754 rdf:resource="https://hack.cybersystems.engineer/memex/ontologies/SeamlessDigitalEngineering#Charter_of_Human_Rights_and_Principles_for_the_Internet"/>
    </owl:NamedIndividual>
    


    <!-- https://hack.cybersystems.engineer/memex/ontologies/SeamlessDigitalEngineering#EAL_1 -->

    <owl:NamedIndividual rdf:about="https://hack.cybersystems.engineer/memex/ontologies/SeamlessDigitalEngineering#EAL_1">
        <rdf:type rdf:resource="https://hack.cybersystems.engineer/memex/ontologies/SeamlessDigitalEngineering#Evaluation_Assurance_Level"/>
        <rdfs:label>EAL 1</rdfs:label>
        <skos:definition xml:lang="en">Functionally tested</skos:definition>
        <cco2:ont00001754 xml:lang="en">ISO/IEC 15408-5:2022</cco2:ont00001754>
    </owl:NamedIndividual>
    


    <!-- https://hack.cybersystems.engineer/memex/ontologies/SeamlessDigitalEngineering#EAL_2 -->

    <owl:NamedIndividual rdf:about="https://hack.cybersystems.engineer/memex/ontologies/SeamlessDigitalEngineering#EAL_2">
        <rdf:type rdf:resource="https://hack.cybersystems.engineer/memex/ontologies/SeamlessDigitalEngineering#Evaluation_Assurance_Level"/>
        <rdfs:label>EAL 2</rdfs:label>
        <skos:definition xml:lang="en">Structurally tested</skos:definition>
        <cco2:ont00001754 xml:lang="en">ISO/IEC 15408-5:2022</cco2:ont00001754>
    </owl:NamedIndividual>
    


    <!-- https://hack.cybersystems.engineer/memex/ontologies/SeamlessDigitalEngineering#EAL_3 -->

    <owl:NamedIndividual rdf:about="https://hack.cybersystems.engineer/memex/ontologies/SeamlessDigitalEngineering#EAL_3">
        <rdf:type rdf:resource="https://hack.cybersystems.engineer/memex/ontologies/SeamlessDigitalEngineering#Evaluation_Assurance_Level"/>
        <rdfs:label>EAL 3</rdfs:label>
        <skos:definition xml:lang="en">Methodically tested and checked</skos:definition>
        <cco2:ont00001754 xml:lang="en">ISO/IEC 15408-5:2022</cco2:ont00001754>
    </owl:NamedIndividual>
    


    <!-- https://hack.cybersystems.engineer/memex/ontologies/SeamlessDigitalEngineering#EAL_4 -->

    <owl:NamedIndividual rdf:about="https://hack.cybersystems.engineer/memex/ontologies/SeamlessDigitalEngineering#EAL_4">
        <rdf:type rdf:resource="https://hack.cybersystems.engineer/memex/ontologies/SeamlessDigitalEngineering#Evaluation_Assurance_Level"/>
        <rdfs:label>EAL 4</rdfs:label>
        <skos:definition xml:lang="en">Methodically designed, tested and reviewed</skos:definition>
        <cco2:ont00001754 xml:lang="en">ISO/IEC 15408-5:2022</cco2:ont00001754>
    </owl:NamedIndividual>
    


    <!-- https://hack.cybersystems.engineer/memex/ontologies/SeamlessDigitalEngineering#EAL_5 -->

    <owl:NamedIndividual rdf:about="https://hack.cybersystems.engineer/memex/ontologies/SeamlessDigitalEngineering#EAL_5">
        <rdf:type rdf:resource="https://hack.cybersystems.engineer/memex/ontologies/SeamlessDigitalEngineering#Evaluation_Assurance_Level"/>
        <rdfs:label>EAL 5</rdfs:label>
        <skos:definition xml:lang="en">Semi-formally verified designed and tested</skos:definition>
        <cco2:ont00001754 xml:lang="en">ISO/IEC 15408-5:2022</cco2:ont00001754>
    </owl:NamedIndividual>
    


    <!-- https://hack.cybersystems.engineer/memex/ontologies/SeamlessDigitalEngineering#EAL_6 -->

    <owl:NamedIndividual rdf:about="https://hack.cybersystems.engineer/memex/ontologies/SeamlessDigitalEngineering#EAL_6">
        <rdf:type rdf:resource="https://hack.cybersystems.engineer/memex/ontologies/SeamlessDigitalEngineering#Evaluation_Assurance_Level"/>
        <rdfs:label>EAL 6</rdfs:label>
        <skos:definition xml:lang="en">Semi-formally verified design and tested</skos:definition>
        <cco2:ont00001754 xml:lang="en">ISO/IEC 15408-5:2022</cco2:ont00001754>
    </owl:NamedIndividual>
    


    <!-- https://hack.cybersystems.engineer/memex/ontologies/SeamlessDigitalEngineering#EAL_7 -->

    <owl:NamedIndividual rdf:about="https://hack.cybersystems.engineer/memex/ontologies/SeamlessDigitalEngineering#EAL_7">
        <rdf:type rdf:resource="https://hack.cybersystems.engineer/memex/ontologies/SeamlessDigitalEngineering#Evaluation_Assurance_Level"/>
        <rdfs:label>EAL 7</rdfs:label>
        <skos:definition xml:lang="en">Formally-verified design and tested</skos:definition>
        <cco2:ont00001754 xml:lang="en">ISO/IEC 15408-5:2022</cco2:ont00001754>
    </owl:NamedIndividual>
    


    <!-- https://hack.cybersystems.engineer/memex/ontologies/SeamlessDigitalEngineering#Elegant_KQA -->

    <owl:NamedIndividual rdf:about="https://hack.cybersystems.engineer/memex/ontologies/SeamlessDigitalEngineering#Elegant_KQA">
        <rdf:type rdf:resource="https://hack.cybersystems.engineer/memex/ontologies/SeamlessDigitalEngineering#Key_Quality_Attribute"/>
        <rdf:type>
            <owl:Restriction>
                <owl:onProperty rdf:resource="http://purl.obolibrary.org/obo/BFO_0000195"/>
                <owl:someValuesFrom>
                    <owl:Class>
                        <owl:intersectionOf rdf:parseType="Collection">
                            <rdf:Description rdf:about="https://hack.cybersystems.engineer/memex/ontologies/SeamlessDigitalEngineering#Product_Interaction_Capability"/>
                            <rdf:Description rdf:about="https://hack.cybersystems.engineer/memex/ontologies/SeamlessDigitalEngineering#Product_Performance_Efficiency"/>
                            <rdf:Description rdf:about="https://hack.cybersystems.engineer/memex/ontologies/SeamlessDigitalEngineering#Product_Safety"/>
                            <owl:Class>
                                <owl:intersectionOf rdf:parseType="Collection">
                                    <rdf:Description rdf:about="https://hack.cybersystems.engineer/memex/ontologies/SeamlessDigitalEngineering#Product_Flexibility"/>
                                    <rdf:Description rdf:about="https://hack.cybersystems.engineer/memex/ontologies/SeamlessDigitalEngineering#Product_Reliability"/>
                                </owl:intersectionOf>
                            </owl:Class>
                        </owl:intersectionOf>
                    </owl:Class>
                </owl:someValuesFrom>
            </owl:Restriction>
        </rdf:type>
        <rdfs:comment xml:lang="en">The cited attributes of Elegant Systems are equivalent to the following ISO/IEC 25010:2023 SQuaRE product quality (sub-)characteristics:

System efficacy = Product Interaction Capability
System efficiency = Product Performance Efficiency
System robustness = Product Flexibility and Product Reliability
Minimizing unintended consequences = Product Safety</rdfs:comment>
        <rdfs:label xml:lang="en">Elegant KQA</rdfs:label>
        <cco2:ont00001754 rdf:datatype="http://www.w3.org/2001/XMLSchema#anyURI">https://dx.doi.org/10.1007/978-3-030-00114-8_40</cco2:ont00001754>
    </owl:NamedIndividual>
    


    <!-- https://hack.cybersystems.engineer/memex/ontologies/SeamlessDigitalEngineering#Expression_and_Association_Cyber_Right -->

    <owl:NamedIndividual rdf:about="https://hack.cybersystems.engineer/memex/ontologies/SeamlessDigitalEngineering#Expression_and_Association_Cyber_Right">
        <rdf:type rdf:resource="https://hack.cybersystems.engineer/memex/ontologies/SeamlessDigitalEngineering#Human_Cyber_Right"/>
        <rdfs:label xml:lang="en">Expression and Association Cyber Right</rdfs:label>
        <skos:definition xml:lang="en">Every Person has the Right to seek, receive, and impart Information freely in Cyberspace without censorship or other interference. Everyone also has the Right to associate freely through Cyberspace, for social, political, cultural or other purposes.</skos:definition>
        <cco2:ont00001754 rdf:resource="https://hack.cybersystems.engineer/memex/ontologies/SeamlessDigitalEngineering#Charter_of_Human_Rights_and_Principles_for_the_Internet"/>
    </owl:NamedIndividual>
    


    <!-- https://hack.cybersystems.engineer/memex/ontologies/SeamlessDigitalEngineering#Governance_Cyber_Right -->

    <owl:NamedIndividual rdf:about="https://hack.cybersystems.engineer/memex/ontologies/SeamlessDigitalEngineering#Governance_Cyber_Right">
        <rdf:type rdf:resource="https://hack.cybersystems.engineer/memex/ontologies/SeamlessDigitalEngineering#Human_Cyber_Right"/>
        <rdfs:label xml:lang="en">Governance Cyber Right</rdfs:label>
        <skos:definition xml:lang="en">Human Rights and social justice must form the legal and normative foundations upon which Cyberspace operates and is governed. This shall happen in a transparent and multilateral manner, based on principles of openness, inclusive participation and accountability.</skos:definition>
        <cco2:ont00001754 rdf:resource="https://hack.cybersystems.engineer/memex/ontologies/SeamlessDigitalEngineering#Charter_of_Human_Rights_and_Principles_for_the_Internet"/>
    </owl:NamedIndividual>
    


    <!-- https://hack.cybersystems.engineer/memex/ontologies/SeamlessDigitalEngineering#HACK_Assurance_Case_Report -->

    <owl:NamedIndividual rdf:about="https://hack.cybersystems.engineer/memex/ontologies/SeamlessDigitalEngineering#HACK_Assurance_Case_Report">
        <rdf:type rdf:resource="https://hack.cybersystems.engineer/memex/ontologies/SeamlessDigitalEngineering#Assurance_Case_Report"/>
        <obo:BFO_0000115 rdf:resource="https://hack.cybersystems.engineer/memex/ontologies/SeamlessDigitalEngineering#HACK_High-Assurance_Claim_Record"/>
        <rdfs:label xml:lang="en">HACK Assurance Case Report</rdfs:label>
    </owl:NamedIndividual>
    


    <!-- https://hack.cybersystems.engineer/memex/ontologies/SeamlessDigitalEngineering#HACK_Conviviality_Claim -->

    <owl:NamedIndividual rdf:about="https://hack.cybersystems.engineer/memex/ontologies/SeamlessDigitalEngineering#HACK_Conviviality_Claim">
        <rdf:type rdf:resource="https://hack.cybersystems.engineer/memex/ontologies/SeamlessDigitalEngineering#Quality_Claim"/>
        <cco2:ont00001942 rdf:resource="https://hack.cybersystems.engineer/memex/ontologies/SeamlessDigitalEngineering#Convivial_KQA"/>
        <rdfs:label xml:lang="en">HACK Conviviality Claim</rdfs:label>
    </owl:NamedIndividual>
    


    <!-- https://hack.cybersystems.engineer/memex/ontologies/SeamlessDigitalEngineering#HACK_Digital_Twin -->

    <owl:NamedIndividual rdf:about="https://hack.cybersystems.engineer/memex/ontologies/SeamlessDigitalEngineering#HACK_Digital_Twin">
        <rdf:type rdf:resource="https://hack.cybersystems.engineer/memex/ontologies/SeamlessDigitalEngineering#Digital_Twin"/>
        <obo:BFO_0000176 rdf:resource="https://hack.cybersystems.engineer/memex/ontologies/SeamlessDigitalEngineering#High-Assurance_Computing_Kit"/>
        <rdfs:label xml:lang="en">HACK Digital Twin</rdfs:label>
    </owl:NamedIndividual>
    


    <!-- https://hack.cybersystems.engineer/memex/ontologies/SeamlessDigitalEngineering#HACK_Elegant_Claim -->

    <owl:NamedIndividual rdf:about="https://hack.cybersystems.engineer/memex/ontologies/SeamlessDigitalEngineering#HACK_Elegant_Claim">
        <rdf:type rdf:resource="https://hack.cybersystems.engineer/memex/ontologies/SeamlessDigitalEngineering#Quality_Claim"/>
        <cco2:ont00001942 rdf:resource="https://hack.cybersystems.engineer/memex/ontologies/SeamlessDigitalEngineering#Elegant_KQA"/>
        <rdfs:label xml:lang="en">HACK Elegant Claim</rdfs:label>
    </owl:NamedIndividual>
    


    <!-- https://hack.cybersystems.engineer/memex/ontologies/SeamlessDigitalEngineering#HACK_High-Assurance_Argument_Record -->

    <owl:NamedIndividual rdf:about="https://hack.cybersystems.engineer/memex/ontologies/SeamlessDigitalEngineering#HACK_High-Assurance_Argument_Record">
        <rdf:type rdf:resource="https://hack.cybersystems.engineer/memex/ontologies/SeamlessDigitalEngineering#Undeveloped_Assurance_Argument_Record"/>
        <rdfs:label xml:lang="en">HACK High-Assurance Argument Record</rdfs:label>
    </owl:NamedIndividual>
    


    <!-- https://hack.cybersystems.engineer/memex/ontologies/SeamlessDigitalEngineering#HACK_High-Assurance_Claim -->

    <owl:NamedIndividual rdf:about="https://hack.cybersystems.engineer/memex/ontologies/SeamlessDigitalEngineering#HACK_High-Assurance_Claim">
        <rdf:type rdf:resource="https://hack.cybersystems.engineer/memex/ontologies/SeamlessDigitalEngineering#Assurance_Claim"/>
        <rdfs:label xml:lang="en">HACK High-Assurance Claim</rdfs:label>
    </owl:NamedIndividual>
    


    <!-- https://hack.cybersystems.engineer/memex/ontologies/SeamlessDigitalEngineering#HACK_High-Assurance_Claim_Record -->

    <owl:NamedIndividual rdf:about="https://hack.cybersystems.engineer/memex/ontologies/SeamlessDigitalEngineering#HACK_High-Assurance_Claim_Record">
        <rdf:type rdf:resource="https://hack.cybersystems.engineer/memex/ontologies/SeamlessDigitalEngineering#Assurance_Claim_Record"/>
        <obo:BFO_0000101 rdf:resource="https://hack.cybersystems.engineer/memex/ontologies/SeamlessDigitalEngineering#HACK_High-Assurance_Claim"/>
        <obo:BFO_0000115 rdf:resource="https://hack.cybersystems.engineer/memex/ontologies/SeamlessDigitalEngineering#HACK_High-Assurance_Argument_Record"/>
        <obo:BFO_0000115 rdf:resource="https://hack.cybersystems.engineer/memex/ontologies/SeamlessDigitalEngineering#HACK_High-Assurance_Context"/>
        <rdfs:label xml:lang="en">HACK High-Assurance Claim Record</rdfs:label>
    </owl:NamedIndividual>
    


    <!-- https://hack.cybersystems.engineer/memex/ontologies/SeamlessDigitalEngineering#HACK_High-Assurance_Context -->

    <owl:NamedIndividual rdf:about="https://hack.cybersystems.engineer/memex/ontologies/SeamlessDigitalEngineering#HACK_High-Assurance_Context">
        <rdf:type rdf:resource="https://hack.cybersystems.engineer/memex/ontologies/SeamlessDigitalEngineering#Assurance_Context_List"/>
        <rdfs:label xml:lang="en">HACK High-Assurance Context</rdfs:label>
    </owl:NamedIndividual>
    


    <!-- https://hack.cybersystems.engineer/memex/ontologies/SeamlessDigitalEngineering#HACK_Seamless_Claim -->

    <owl:NamedIndividual rdf:about="https://hack.cybersystems.engineer/memex/ontologies/SeamlessDigitalEngineering#HACK_Seamless_Claim">
        <rdf:type rdf:resource="https://hack.cybersystems.engineer/memex/ontologies/SeamlessDigitalEngineering#Seamless_Quality_Claim"/>
        <cco2:ont00001942 rdf:resource="https://hack.cybersystems.engineer/memex/ontologies/SeamlessDigitalEngineering#Seamless_KQA"/>
        <rdfs:label xml:lang="en">HACK Seamless Claim</rdfs:label>
    </owl:NamedIndividual>
    


    <!-- https://hack.cybersystems.engineer/memex/ontologies/SeamlessDigitalEngineering#HACK_Trustworthiness_Claim -->

    <owl:NamedIndividual rdf:about="https://hack.cybersystems.engineer/memex/ontologies/SeamlessDigitalEngineering#HACK_Trustworthiness_Claim"/>
    


    <!-- https://hack.cybersystems.engineer/memex/ontologies/SeamlessDigitalEngineering#High-Assurance_Computing_Kit -->

    <owl:NamedIndividual rdf:about="https://hack.cybersystems.engineer/memex/ontologies/SeamlessDigitalEngineering#High-Assurance_Computing_Kit">
        <rdf:type rdf:resource="https://hack.cybersystems.engineer/memex/ontologies/SeamlessDigitalEngineering#Information_Appliance"/>
        <rdf:type rdf:resource="https://hack.cybersystems.engineer/memex/ontologies/SeamlessDigitalEngineering#Seamless_Digital_Engineering_System"/>
        <rdf:type rdf:resource="https://hack.cybersystems.engineer/memex/ontologies/SeamlessDigitalEngineering#Trustworthy_System"/>
        <rdf:type rdf:resource="https://www.commoncoreontologies.org/ont00000870"/>
        <obo:BFO_0000101 rdf:resource="https://hack.cybersystems.engineer/memex/ontologies/SeamlessDigitalEngineering#HACK_Conviviality_Claim"/>
        <obo:BFO_0000101 rdf:resource="https://hack.cybersystems.engineer/memex/ontologies/SeamlessDigitalEngineering#HACK_Elegant_Claim"/>
        <obo:BFO_0000101 rdf:resource="https://hack.cybersystems.engineer/memex/ontologies/SeamlessDigitalEngineering#HACK_High-Assurance_Claim"/>
        <obo:BFO_0000101 rdf:resource="https://hack.cybersystems.engineer/memex/ontologies/SeamlessDigitalEngineering#HACK_Seamless_Claim"/>
        <obo:BFO_0000101 rdf:resource="https://hack.cybersystems.engineer/memex/ontologies/SeamlessDigitalEngineering#HACK_Trustworthiness_Claim"/>
        <rdfs:label xml:lang="en">High-Assurance Computing Kit</rdfs:label>
        <skos:altLabel xml:lang="en">HACK</skos:altLabel>
        <skos:definition xml:lang="en">Information Appliance that implements the Seamless Digital Engineering Environment Reference Architecture and is bearer of Seamless, Trustworthy, Elegant, and Convivial Key Quality Attributes</skos:definition>
    </owl:NamedIndividual>
    


    <!-- https://hack.cybersystems.engineer/memex/ontologies/SeamlessDigitalEngineering#High-Assurance_Computing_Kit_System_Architecture -->

    <owl:NamedIndividual rdf:about="https://hack.cybersystems.engineer/memex/ontologies/SeamlessDigitalEngineering#High-Assurance_Computing_Kit_System_Architecture">
        <rdf:type rdf:resource="https://hack.cybersystems.engineer/memex/ontologies/SeamlessDigitalEngineering#System_Architecture_Model"/>
        <cco2:ont00001920 rdf:resource="https://hack.cybersystems.engineer/memex/ontologies/SeamlessDigitalEngineering#Seamless_Digital_Engineering_Environment_Reference_Architecture"/>
        <cco2:ont00001942 rdf:resource="https://hack.cybersystems.engineer/memex/ontologies/SeamlessDigitalEngineering#HACK_Digital_Twin"/>
        <cco2:ont00001942 rdf:resource="https://hack.cybersystems.engineer/memex/ontologies/SeamlessDigitalEngineering#High-Assurance_Computing_Kit"/>
        <rdfs:label xml:lang="en">High-Assurance Computing Kit (HACK) System Architecture</rdfs:label>
    </owl:NamedIndividual>
    


    <!-- https://hack.cybersystems.engineer/memex/ontologies/SeamlessDigitalEngineering#MATLAB -->

    <owl:NamedIndividual rdf:about="https://hack.cybersystems.engineer/memex/ontologies/SeamlessDigitalEngineering#MATLAB">
        <rdf:type rdf:resource="https://hack.cybersystems.engineer/memex/ontologies/SeamlessDigitalEngineering#Digital_Tool"/>
        <obo:BFO_0000176 rdf:resource="https://hack.cybersystems.engineer/memex/ontologies/SeamlessDigitalEngineering#MathWorks"/>
        <rdfs:isDefinedBy rdf:datatype="http://www.w3.org/2001/XMLSchema#anyURI">https://www.wikidata.org/entity/Q169478</rdfs:isDefinedBy>
        <rdfs:label xml:lang="en">MATLAB</rdfs:label>
        <rdfs:seeAlso rdf:datatype="http://www.w3.org/2001/XMLSchema#anyURI">https://www.mathworks.com/products/matlab.html</rdfs:seeAlso>
        <skos:definition xml:lang="en">MATLAB (an abbreviation of &quot;MATrix LABoratory&quot;) is a proprietary multi-paradigm programming language and numeric computing environment developed by MathWorks. MATLAB allows matrix manipulations, plotting of functions and data, implementation of algorithms, creation of user interfaces, and interfacing with programs written in other languages.

Although MATLAB is intended primarily for numeric computing, an optional toolbox uses the MuPAD symbolic engine allowing access to symbolic computing abilities. An additional package, Simulink, adds graphical multi-domain simulation and model-based design for dynamic and embedded systems.</skos:definition>
        <cco2:ont00001754 rdf:datatype="http://www.w3.org/2001/XMLSchema#anyURI">https://en.wikipedia.org/wiki/MATLAB</cco2:ont00001754>
    </owl:NamedIndividual>
    


    <!-- https://hack.cybersystems.engineer/memex/ontologies/SeamlessDigitalEngineering#ManTech_Digital_Engineering_Environment_Reference_Model -->

    <owl:NamedIndividual rdf:about="https://hack.cybersystems.engineer/memex/ontologies/SeamlessDigitalEngineering#ManTech_Digital_Engineering_Environment_Reference_Model">
        <rdf:type rdf:resource="https://hack.cybersystems.engineer/memex/ontologies/SeamlessDigitalEngineering#Digital_Engineering_Environment_Reference_Architecture"/>
        <obo:BFO_0000084 rdf:resource="https://hack.cybersystems.engineer/memex/ontologies/SeamlessDigitalEngineering#ManTech_International_Corporation"/>
        <rdfs:label xml:lang="en">ManTech Digital Engineering Environment Reference Model</rdfs:label>
    </owl:NamedIndividual>
    


    <!-- https://hack.cybersystems.engineer/memex/ontologies/SeamlessDigitalEngineering#ManTech_International_Corporation -->

    <owl:NamedIndividual rdf:about="https://hack.cybersystems.engineer/memex/ontologies/SeamlessDigitalEngineering#ManTech_International_Corporation">
        <rdf:type rdf:resource="https://hack.cybersystems.engineer/memex/ontologies/SeamlessDigitalEngineering#Contractor"/>
        <obo:BFO_0000101 rdf:resource="https://hack.cybersystems.engineer/memex/ontologies/SeamlessDigitalEngineering#ManTech_Digital_Engineering_Environment_Reference_Model"/>
        <rdfs:label xml:lang="en">ManTech International Corporation</rdfs:label>
        <rdfs:seeAlso rdf:datatype="http://www.w3.org/2001/XMLSchema#anyURI">https://en.wikipedia.org/wiki/ManTech_International</rdfs:seeAlso>
        <rdfs:seeAlso rdf:datatype="http://www.w3.org/2001/XMLSchema#anyURI">https://www.mantech.com/</rdfs:seeAlso>
    </owl:NamedIndividual>
    


    <!-- https://hack.cybersystems.engineer/memex/ontologies/SeamlessDigitalEngineering#MathWorks -->

    <owl:NamedIndividual rdf:about="https://hack.cybersystems.engineer/memex/ontologies/SeamlessDigitalEngineering#MathWorks">
        <rdf:type>
            <owl:Class>
                <owl:intersectionOf rdf:parseType="Collection">
                    <rdf:Description rdf:about="https://hack.cybersystems.engineer/memex/ontologies/SeamlessDigitalEngineering#Supplier"/>
                    <rdf:Description rdf:about="https://www.commoncoreontologies.org/ont00000443"/>
                </owl:intersectionOf>
            </owl:Class>
        </rdf:type>
        <obo:BFO_0000178 rdf:resource="https://hack.cybersystems.engineer/memex/ontologies/SeamlessDigitalEngineering#MATLAB"/>
        <rdfs:isDefinedBy rdf:datatype="http://www.w3.org/2001/XMLSchema#anyURI">http://www.wikidata.org/entity/Q1518683</rdfs:isDefinedBy>
        <rdfs:label xml:lang="en">MathWorks</rdfs:label>
        <rdfs:seeAlso rdf:datatype="http://www.w3.org/2001/XMLSchema#anyURI">https://mathworks.com/</rdfs:seeAlso>
        <skos:definition xml:lang="en">The MathWorks, Inc. is an American privately held corporation that specializes in mathematical computing software. Its major products include MATLAB and Simulink, which support data analysis and simulation.</skos:definition>
        <cco2:ont00001754 rdf:datatype="http://www.w3.org/2001/XMLSchema#anyURI">https://en.wikipedia.org/wiki/MathWorks</cco2:ont00001754>
    </owl:NamedIndividual>
    


    <!-- https://hack.cybersystems.engineer/memex/ontologies/SeamlessDigitalEngineering#Microsoft -->

    <owl:NamedIndividual rdf:about="https://hack.cybersystems.engineer/memex/ontologies/SeamlessDigitalEngineering#Microsoft">
        <rdf:type rdf:resource="https://www.commoncoreontologies.org/ont00000443"/>
        <obo:BFO_0000178 rdf:resource="https://hack.cybersystems.engineer/memex/ontologies/SeamlessDigitalEngineering#MicrosoftProject"/>
        <rdfs:isDefinedBy rdf:datatype="http://www.w3.org/2001/XMLSchema#anyURI">https://www.wikidata.org/entity/Q2283</rdfs:isDefinedBy>
        <rdfs:label xml:lang="en">Microsoft</rdfs:label>
        <skos:definition xml:lang="en">Microsoft Corporation is an American multinational corporation and technology company headquartered in Redmond, Washington.[2] Its best-known software products are the Windows line of operating systems, the Microsoft 365 suite of productivity applications, the Azure cloud computing platform and the Edge web browser.</skos:definition>
        <cco2:ont00001754 rdf:datatype="http://www.w3.org/2001/XMLSchema#anyURI">https://en.wikipedia.org/wiki/Microsoft</cco2:ont00001754>
    </owl:NamedIndividual>
    


    <!-- https://hack.cybersystems.engineer/memex/ontologies/SeamlessDigitalEngineering#MicrosoftProject -->

    <owl:NamedIndividual rdf:about="https://hack.cybersystems.engineer/memex/ontologies/SeamlessDigitalEngineering#MicrosoftProject">
        <rdf:type rdf:resource="https://hack.cybersystems.engineer/memex/ontologies/SeamlessDigitalEngineering#Digital_Tool"/>
        <obo:BFO_0000176 rdf:resource="https://hack.cybersystems.engineer/memex/ontologies/SeamlessDigitalEngineering#Microsoft"/>
        <rdfs:isDefinedBy rdf:datatype="http://www.w3.org/2001/XMLSchema#anyURI">https://www.wikidata.org/entity/Q80336</rdfs:isDefinedBy>
        <rdfs:label xml:lang="en">Microsoft Project</rdfs:label>
        <rdfs:seeAlso rdf:datatype="http://www.w3.org/2001/XMLSchema#anyURI">http://www.microsoft.com/en-us/microsoft-365/project/project-management-software</rdfs:seeAlso>
        <skos:definition xml:lang="en">Microsoft Project is project management software product, developed and sold by Microsoft. It is designed to assist a project manager in developing a schedule, assigning resources to tasks, tracking progress, managing the budget, and analyzing workloads.</skos:definition>
        <cco2:ont00001754 rdf:datatype="http://www.w3.org/2001/XMLSchema#anyURI">https://en.wikipedia.org/wiki/Microsoft_Project</cco2:ont00001754>
    </owl:NamedIndividual>
    


    <!-- https://hack.cybersystems.engineer/memex/ontologies/SeamlessDigitalEngineering#Network_Equality_Cyber_Right -->

    <owl:NamedIndividual rdf:about="https://hack.cybersystems.engineer/memex/ontologies/SeamlessDigitalEngineering#Network_Equality_Cyber_Right">
        <rdf:type rdf:resource="https://hack.cybersystems.engineer/memex/ontologies/SeamlessDigitalEngineering#Human_Cyber_Right"/>
        <rdfs:label xml:lang="en">Network Equality Cyber Right</rdfs:label>
        <skos:definition xml:lang="en">Every Person shall have universal and open access to Cyberspace content, free from discriminatory prioritisation, filtering or traffic control on commercial, political or other grounds.</skos:definition>
        <cco2:ont00001754 rdf:resource="https://hack.cybersystems.engineer/memex/ontologies/SeamlessDigitalEngineering#Charter_of_Human_Rights_and_Principles_for_the_Internet"/>
    </owl:NamedIndividual>
    


    <!-- https://hack.cybersystems.engineer/memex/ontologies/SeamlessDigitalEngineering#Object_Management_Group -->

    <owl:NamedIndividual rdf:about="https://hack.cybersystems.engineer/memex/ontologies/SeamlessDigitalEngineering#Object_Management_Group">
        <rdf:type rdf:resource="https://hack.cybersystems.engineer/memex/ontologies/SeamlessDigitalEngineering#Standards_Organization"/>
        <obo:BFO_0000101 rdf:resource="https://hack.cybersystems.engineer/memex/ontologies/SeamlessDigitalEngineering#Systems_Modeling_Language"/>
        <rdfs:label xml:lang="en">Object Management Group</rdfs:label>
        <rdfs:seeAlso rdf:datatype="http://www.w3.org/2001/XMLSchema#anyURI">https://www.omg.org/</rdfs:seeAlso>
        <skos:altLabel xml:lang="en">OMG</skos:altLabel>
        <skos:definition xml:lang="en">The Object Management Group (OMG) is a computer industry standards consortium. OMG Task Forces develop enterprise integration standards for a range of technologies.</skos:definition>
        <cco2:ont00001754 rdf:datatype="http://www.w3.org/2001/XMLSchema#anyURI">https://en.wikipedia.org/wiki/Object_Management_Group</cco2:ont00001754>
    </owl:NamedIndividual>
    


    <!-- https://hack.cybersystems.engineer/memex/ontologies/SeamlessDigitalEngineering#Privacy_and_Data_Protection_Cyber_Right -->

    <owl:NamedIndividual rdf:about="https://hack.cybersystems.engineer/memex/ontologies/SeamlessDigitalEngineering#Privacy_and_Data_Protection_Cyber_Right">
        <rdf:type rdf:resource="https://hack.cybersystems.engineer/memex/ontologies/SeamlessDigitalEngineering#Human_Cyber_Right"/>
        <rdfs:label xml:lang="en">Privacy and Data Protection Cyber Right</rdfs:label>
        <skos:definition xml:lang="en">Every Person has the Right to privacy in Cyberspace. This includes freedom from surveillance, the Right to use encryption, and the Right to online anonymity. Everyone also has the Right to data protection, including control over personal Data collection, retention, processing, disposal and disclosure.</skos:definition>
        <cco2:ont00001754 rdf:resource="https://hack.cybersystems.engineer/memex/ontologies/SeamlessDigitalEngineering#Charter_of_Human_Rights_and_Principles_for_the_Internet"/>
    </owl:NamedIndividual>
    


    <!-- https://hack.cybersystems.engineer/memex/ontologies/SeamlessDigitalEngineering#Protege -->

    <owl:NamedIndividual rdf:about="https://hack.cybersystems.engineer/memex/ontologies/SeamlessDigitalEngineering#Protege">
        <rdf:type rdf:resource="https://hack.cybersystems.engineer/memex/ontologies/SeamlessDigitalEngineering#Digital_Tool"/>
        <rdfs:label xml:lang="en">Protégé</rdfs:label>
        <rdfs:seeAlso rdf:datatype="http://www.w3.org/2001/XMLSchema#anyURI">https://protege.stanford.edu/</rdfs:seeAlso>
    </owl:NamedIndividual>
    


    <!-- https://hack.cybersystems.engineer/memex/ontologies/SeamlessDigitalEngineering#Rights_and_Social_Justice_Cyber_Right -->

    <owl:NamedIndividual rdf:about="https://hack.cybersystems.engineer/memex/ontologies/SeamlessDigitalEngineering#Rights_and_Social_Justice_Cyber_Right">
        <rdf:type rdf:resource="https://hack.cybersystems.engineer/memex/ontologies/SeamlessDigitalEngineering#Human_Cyber_Right"/>
        <rdfs:label xml:lang="en">Rights and Social Justice Cyber Right</rdfs:label>
        <skos:definition xml:lang="en">Cyberspace is a space for the promotion, protection and fulfilment of Human Rights and the advancement of social justice. Every Person has the duty to respect the Human Rights of all others in Cyberspace.</skos:definition>
        <cco2:ont00001754 rdf:resource="https://hack.cybersystems.engineer/memex/ontologies/SeamlessDigitalEngineering#Charter_of_Human_Rights_and_Principles_for_the_Internet"/>
    </owl:NamedIndividual>
    


    <!-- https://hack.cybersystems.engineer/memex/ontologies/SeamlessDigitalEngineering#Seamless_Digital_Engineering_Environment_Reference_Architecture -->

    <owl:NamedIndividual rdf:about="https://hack.cybersystems.engineer/memex/ontologies/SeamlessDigitalEngineering#Seamless_Digital_Engineering_Environment_Reference_Architecture">
        <rdf:type rdf:resource="https://hack.cybersystems.engineer/memex/ontologies/SeamlessDigitalEngineering#Reference_Architecture"/>
        <rdf:type>
            <owl:Restriction>
                <owl:onProperty rdf:resource="https://www.commoncoreontologies.org/ont00001942"/>
                <owl:someValuesFrom rdf:resource="https://hack.cybersystems.engineer/memex/ontologies/SeamlessDigitalEngineering#Seamless_Digital_Engineering_System"/>
            </owl:Restriction>
        </rdf:type>
        <cco2:ont00001942 rdf:resource="https://hack.cybersystems.engineer/memex/ontologies/SeamlessDigitalEngineering#Seamless_Digital_Engineering_Ontology"/>
        <rdfs:label xml:lang="en">Seamless Digital Engineering Environment Reference Architecture</rdfs:label>
        <skos:altLabel xml:lang="en">Seamless DE Environment RA</skos:altLabel>
    </owl:NamedIndividual>
    


    <!-- https://hack.cybersystems.engineer/memex/ontologies/SeamlessDigitalEngineering#Seamless_Digital_Engineering_Ontology -->

    <owl:NamedIndividual rdf:about="https://hack.cybersystems.engineer/memex/ontologies/SeamlessDigitalEngineering#Seamless_Digital_Engineering_Ontology">
        <rdf:type>
            <owl:Class>
                <owl:intersectionOf rdf:parseType="Collection">
                    <rdf:Description rdf:about="http://www.ontologyrepository.com/CommonCoreOntologies/Ontology"/>
                    <owl:Restriction>
                        <owl:onProperty rdf:resource="http://purl.obolibrary.org/obo/BFO_0000101"/>
                        <owl:someValuesFrom rdf:resource="https://hack.cybersystems.engineer/memex/ontologies/SeamlessDigitalEngineering#Seamless_Digital_Engineering_Paradigm"/>
                    </owl:Restriction>
                </owl:intersectionOf>
            </owl:Class>
        </rdf:type>
        <cco2:ont00001920 rdf:resource="https://hack.cybersystems.engineer/memex/ontologies/SeamlessDigitalEngineering#Seamless_Digital_Engineering_Environment_Reference_Architecture"/>
        <rdfs:label xml:lang="en">Seamless Digital Engineering Ontology</rdfs:label>
    </owl:NamedIndividual>
    


    <!-- https://hack.cybersystems.engineer/memex/ontologies/SeamlessDigitalEngineering#Seamless_KQA -->

    <owl:NamedIndividual rdf:about="https://hack.cybersystems.engineer/memex/ontologies/SeamlessDigitalEngineering#Seamless_KQA">
        <rdf:type rdf:resource="https://hack.cybersystems.engineer/memex/ontologies/SeamlessDigitalEngineering#Key_Quality_Attribute"/>
        <rdf:type>
            <owl:Restriction>
                <owl:onProperty rdf:resource="http://purl.obolibrary.org/obo/BFO_0000195"/>
                <owl:someValuesFrom>
                    <owl:Class>
                        <owl:intersectionOf rdf:parseType="Collection">
                            <rdf:Description rdf:about="https://hack.cybersystems.engineer/memex/ontologies/SeamlessDigitalEngineering#Seamless_Integration"/>
                            <rdf:Description rdf:about="https://hack.cybersystems.engineer/memex/ontologies/SeamlessDigitalEngineering#Seamless_Interaction_Capability"/>
                            <rdf:Description rdf:about="https://hack.cybersystems.engineer/memex/ontologies/SeamlessDigitalEngineering#Seamless_Quality-in-Use"/>
                        </owl:intersectionOf>
                    </owl:Class>
                </owl:someValuesFrom>
            </owl:Restriction>
        </rdf:type>
        <rdfs:label xml:lang="en">Seamless KQA</rdfs:label>
    </owl:NamedIndividual>
    


    <!-- https://hack.cybersystems.engineer/memex/ontologies/SeamlessDigitalEngineering#Standards_and_Regulation_Cyber_Right -->

    <owl:NamedIndividual rdf:about="https://hack.cybersystems.engineer/memex/ontologies/SeamlessDigitalEngineering#Standards_and_Regulation_Cyber_Right">
        <rdf:type rdf:resource="https://hack.cybersystems.engineer/memex/ontologies/SeamlessDigitalEngineering#Human_Cyber_Right"/>
        <rdfs:label xml:lang="en">Standards and Regulation Cyber Right</rdfs:label>
        <skos:definition xml:lang="en">Cyberspace’s architecture, communication systems, and document and data formats shall be based on open standards that ensure complete interoperability, inclusion and equal opportunity for all.</skos:definition>
        <cco2:ont00001754 rdf:resource="https://hack.cybersystems.engineer/memex/ontologies/SeamlessDigitalEngineering#Charter_of_Human_Rights_and_Principles_for_the_Internet"/>
    </owl:NamedIndividual>
    


    <!-- https://hack.cybersystems.engineer/memex/ontologies/SeamlessDigitalEngineering#System_Architecture_Framework -->

    <owl:NamedIndividual rdf:about="https://hack.cybersystems.engineer/memex/ontologies/SeamlessDigitalEngineering#System_Architecture_Framework">
        <rdf:type rdf:resource="https://hack.cybersystems.engineer/memex/ontologies/SeamlessDigitalEngineering#Architecture_Description_Framework"/>
        <rdfs:label xml:lang="en">System Architecture Framework</rdfs:label>
        <rdfs:seeAlso rdf:datatype="http://www.w3.org/2001/XMLSchema#anyURI">https://saf.gfse.org/</rdfs:seeAlso>
        <cco2:ont00001753 xml:lang="en">SAF</cco2:ont00001753>
    </owl:NamedIndividual>
    


    <!-- https://hack.cybersystems.engineer/memex/ontologies/SeamlessDigitalEngineering#Systems_Modeling_Language -->

    <owl:NamedIndividual rdf:about="https://hack.cybersystems.engineer/memex/ontologies/SeamlessDigitalEngineering#Systems_Modeling_Language">
        <rdf:type rdf:resource="https://hack.cybersystems.engineer/memex/ontologies/SeamlessDigitalEngineering#Architecture_Description_Language"/>
        <rdf:type rdf:resource="https://hack.cybersystems.engineer/memex/ontologies/SeamlessDigitalEngineering#Technical_Standard"/>
        <obo:BFO_0000084 rdf:resource="https://hack.cybersystems.engineer/memex/ontologies/SeamlessDigitalEngineering#Object_Management_Group"/>
        <rdfs:label xml:lang="en">Systems Modeling Language</rdfs:label>
        <rdfs:seeAlso rdf:datatype="http://www.w3.org/2001/XMLSchema#anyURI">https://sysml.org/</rdfs:seeAlso>
        <rdfs:seeAlso rdf:datatype="http://www.w3.org/2001/XMLSchema#anyURI">https://www.omg.org/spec/SysML/1.7/About-SysML/</rdfs:seeAlso>
        <skos:altLabel xml:lang="en">SysML</skos:altLabel>
        <skos:definition xml:lang="en">The systems modeling language (SysML) is a general-purpose modeling language for systems engineering applications. It supports the specification, analysis, design, verification and validation of a broad range of systems and systems-of-systems.</skos:definition>
        <cco2:ont00001754 rdf:datatype="http://www.w3.org/2001/XMLSchema#anyURI">https://en.wikipedia.org/wiki/Systems_modeling_language</cco2:ont00001754>
    </owl:NamedIndividual>
    


    <!-- https://hack.cybersystems.engineer/memex/ontologies/SeamlessDigitalEngineering#TRL_1 -->

    <owl:NamedIndividual rdf:about="https://hack.cybersystems.engineer/memex/ontologies/SeamlessDigitalEngineering#TRL_1">
        <rdf:type rdf:resource="https://hack.cybersystems.engineer/memex/ontologies/SeamlessDigitalEngineering#Technology_Readiness_Level"/>
        <rdfs:comment xml:lang="en">Basic technology research</rdfs:comment>
        <rdfs:label xml:lang="en">TRL 1</rdfs:label>
        <skos:definition xml:lang="en">Basic principles observed and reported</skos:definition>
        <cco2:ont00001754 xml:lang="en">NASA Systems Engineering Handbook (2016)</cco2:ont00001754>
    </owl:NamedIndividual>
    


    <!-- https://hack.cybersystems.engineer/memex/ontologies/SeamlessDigitalEngineering#TRL_2 -->

    <owl:NamedIndividual rdf:about="https://hack.cybersystems.engineer/memex/ontologies/SeamlessDigitalEngineering#TRL_2">
        <rdf:type rdf:resource="https://hack.cybersystems.engineer/memex/ontologies/SeamlessDigitalEngineering#Technology_Readiness_Level"/>
        <rdfs:comment xml:lang="en">Research to prove feasibility, and
Basic technology research</rdfs:comment>
        <rdfs:label xml:lang="en">TRL 2</rdfs:label>
        <skos:definition xml:lang="en">Technology concept and/or application formulated</skos:definition>
        <cco2:ont00001754 xml:lang="en">NASA Systems Engineering Handbook (2016)</cco2:ont00001754>
    </owl:NamedIndividual>
    


    <!-- https://hack.cybersystems.engineer/memex/ontologies/SeamlessDigitalEngineering#TRL_3 -->

    <owl:NamedIndividual rdf:about="https://hack.cybersystems.engineer/memex/ontologies/SeamlessDigitalEngineering#TRL_3">
        <rdf:type rdf:resource="https://hack.cybersystems.engineer/memex/ontologies/SeamlessDigitalEngineering#Technology_Readiness_Level"/>
        <rdfs:comment xml:lang="en">Research to prove feasibility, and
Basic technology research</rdfs:comment>
        <rdfs:label xml:lang="en">TRL 3</rdfs:label>
        <skos:definition xml:lang="en">Analytical and experimental critical function and/or characteristic proof-of-concept</skos:definition>
        <cco2:ont00001754 xml:lang="en">NASA Systems Engineering Handbook (2016)</cco2:ont00001754>
    </owl:NamedIndividual>
    


    <!-- https://hack.cybersystems.engineer/memex/ontologies/SeamlessDigitalEngineering#TRL_4 -->

    <owl:NamedIndividual rdf:about="https://hack.cybersystems.engineer/memex/ontologies/SeamlessDigitalEngineering#TRL_4">
        <rdf:type rdf:resource="https://hack.cybersystems.engineer/memex/ontologies/SeamlessDigitalEngineering#Technology_Readiness_Level"/>
        <rdfs:comment xml:lang="en">Technology development, and
Research to prove feasibility</rdfs:comment>
        <rdfs:label xml:lang="en">TRL 4</rdfs:label>
        <skos:definition xml:lang="en">Component and/or breadboard validation in laboratory environment</skos:definition>
        <cco2:ont00001754 xml:lang="en">NASA Systems Engineering Handbook (2016)</cco2:ont00001754>
    </owl:NamedIndividual>
    


    <!-- https://hack.cybersystems.engineer/memex/ontologies/SeamlessDigitalEngineering#TRL_5 -->

    <owl:NamedIndividual rdf:about="https://hack.cybersystems.engineer/memex/ontologies/SeamlessDigitalEngineering#TRL_5">
        <rdf:type rdf:resource="https://hack.cybersystems.engineer/memex/ontologies/SeamlessDigitalEngineering#Technology_Readiness_Level"/>
        <rdfs:comment xml:lang="en">Technology demonstration, and
Technology development</rdfs:comment>
        <rdfs:label xml:lang="en">TRL 5</rdfs:label>
        <skos:definition xml:lang="en">Component and/or breadboard validation in relevant environment</skos:definition>
        <cco2:ont00001754 xml:lang="en">NASA Systems Engineering Handbook (2016)</cco2:ont00001754>
    </owl:NamedIndividual>
    


    <!-- https://hack.cybersystems.engineer/memex/ontologies/SeamlessDigitalEngineering#TRL_6 -->

    <owl:NamedIndividual rdf:about="https://hack.cybersystems.engineer/memex/ontologies/SeamlessDigitalEngineering#TRL_6">
        <rdf:type rdf:resource="https://hack.cybersystems.engineer/memex/ontologies/SeamlessDigitalEngineering#Technology_Readiness_Level"/>
        <rdfs:comment xml:lang="en">Technology demonstration, and in-between
System/subsystem development and Technology development</rdfs:comment>
        <rdfs:label xml:lang="en">TRL 6</rdfs:label>
        <skos:definition xml:lang="en">System/subsystem model or prototype demonstration in a relevant environment (ground or space)</skos:definition>
        <cco2:ont00001754 xml:lang="en">NASA Systems Engineering Handbook (2016)</cco2:ont00001754>
    </owl:NamedIndividual>
    


    <!-- https://hack.cybersystems.engineer/memex/ontologies/SeamlessDigitalEngineering#TRL_7 -->

    <owl:NamedIndividual rdf:about="https://hack.cybersystems.engineer/memex/ontologies/SeamlessDigitalEngineering#TRL_7">
        <rdf:type rdf:resource="https://hack.cybersystems.engineer/memex/ontologies/SeamlessDigitalEngineering#Technology_Readiness_Level"/>
        <rdfs:comment xml:lang="en">System/subsystem development, and
Technology demonstration</rdfs:comment>
        <rdfs:label xml:lang="en">TRL 7</rdfs:label>
        <skos:definition xml:lang="en">System prototype demonstration in a target/space environment</skos:definition>
        <cco2:ont00001754 xml:lang="en">NASA Systems Engineering Handbook (2016)</cco2:ont00001754>
    </owl:NamedIndividual>
    


    <!-- https://hack.cybersystems.engineer/memex/ontologies/SeamlessDigitalEngineering#TRL_8 -->

    <owl:NamedIndividual rdf:about="https://hack.cybersystems.engineer/memex/ontologies/SeamlessDigitalEngineering#TRL_8">
        <rdf:type rdf:resource="https://hack.cybersystems.engineer/memex/ontologies/SeamlessDigitalEngineering#Technology_Readiness_Level"/>
        <rdfs:comment xml:lang="en">System test, launch, and operations, and
System/subsystem development</rdfs:comment>
        <rdfs:label xml:lang="en">TRL 8</rdfs:label>
        <skos:definition xml:lang="en">Actual system completed and &quot;flight-qualified&quot; through test and demonstration (ground or flight)</skos:definition>
        <cco2:ont00001754 xml:lang="en">NASA Systems Engineering Handbook (2016)</cco2:ont00001754>
    </owl:NamedIndividual>
    


    <!-- https://hack.cybersystems.engineer/memex/ontologies/SeamlessDigitalEngineering#TRL_9 -->

    <owl:NamedIndividual rdf:about="https://hack.cybersystems.engineer/memex/ontologies/SeamlessDigitalEngineering#TRL_9">
        <rdf:type rdf:resource="https://hack.cybersystems.engineer/memex/ontologies/SeamlessDigitalEngineering#Technology_Readiness_Level"/>
        <rdfs:comment xml:lang="en">System test, launch, and operations</rdfs:comment>
        <rdfs:label xml:lang="en">TRL 9</rdfs:label>
        <skos:definition xml:lang="en">Actual system &quot;flight-proven&quot; through successful mission operations</skos:definition>
        <cco2:ont00001754 xml:lang="en">NASA Systems Engineering Handbook (2016)</cco2:ont00001754>
    </owl:NamedIndividual>
    


    <!-- https://hack.cybersystems.engineer/memex/ontologies/SeamlessDigitalEngineering#Trustworthy_KQA -->

    <owl:NamedIndividual rdf:about="https://hack.cybersystems.engineer/memex/ontologies/SeamlessDigitalEngineering#Trustworthy_KQA">
        <rdf:type rdf:resource="https://hack.cybersystems.engineer/memex/ontologies/SeamlessDigitalEngineering#Key_Quality_Attribute"/>
        <rdf:type>
            <owl:Restriction>
                <owl:onProperty rdf:resource="http://purl.obolibrary.org/obo/BFO_0000195"/>
                <owl:someValuesFrom rdf:resource="https://hack.cybersystems.engineer/memex/ontologies/SeamlessDigitalEngineering#Trustworthiness"/>
            </owl:Restriction>
        </rdf:type>
        <rdfs:label xml:lang="en">Trustworthy KQA</rdfs:label>
    </owl:NamedIndividual>
    


    <!-- https://hack.cybersystems.engineer/memex/ontologies/SeamlessDigitalEngineering#Unified_Architecture_Framework -->

    <owl:NamedIndividual rdf:about="https://hack.cybersystems.engineer/memex/ontologies/SeamlessDigitalEngineering#Unified_Architecture_Framework">
        <rdf:type rdf:resource="https://hack.cybersystems.engineer/memex/ontologies/SeamlessDigitalEngineering#Architecture_Description_Framework"/>
        <obo:BFO_0000084 rdf:resource="https://hack.cybersystems.engineer/memex/ontologies/SeamlessDigitalEngineering#Object_Management_Group"/>
        <obo:BFO_0000178 rdf:resource="https://hack.cybersystems.engineer/memex/ontologies/SeamlessDigitalEngineering#Systems_Modeling_Language"/>
        <rdfs:label xml:lang="en">Unified Architecture Framework</rdfs:label>
        <rdfs:seeAlso rdf:datatype="http://www.w3.org/2001/XMLSchema#anyURI">https://www.omg.org/spec/UAF</rdfs:seeAlso>
        <rdfs:seeAlso rdf:datatype="http://www.w3.org/2001/XMLSchema#anyURI">https://www.omg.org/uaf/</rdfs:seeAlso>
        <cco2:ont00001753 xml:lang="en">UAF</cco2:ont00001753>
    </owl:NamedIndividual>
    


    <!-- https://hack.cybersystems.engineer/memex/ontologies/SeamlessDigitalEngineering#United_States_Air_Force_Research_Laboratory -->

    <owl:NamedIndividual rdf:about="https://hack.cybersystems.engineer/memex/ontologies/SeamlessDigitalEngineering#United_States_Air_Force_Research_Laboratory">
        <rdf:type rdf:resource="https://www.commoncoreontologies.org/ont00000408"/>
        <obo:BFO_0000178 rdf:resource="https://hack.cybersystems.engineer/memex/ontologies/SeamlessDigitalEngineering#AFRL_Digital_Laboratory_Environment"/>
        <rdfs:label xml:lang="en">US Air Force Research Laboratory</rdfs:label>
        <skos:altLabel xml:lang="en">AFRL</skos:altLabel>
    </owl:NamedIndividual>
    


    <!-- https://hack.cybersystems.engineer/memex/ontologies/SeamlessDigitalEngineering#Universal_Declaration_of_Human_Rights -->

    <owl:NamedIndividual rdf:about="https://hack.cybersystems.engineer/memex/ontologies/SeamlessDigitalEngineering#Universal_Declaration_of_Human_Rights">
        <rdf:type>
            <owl:Class>
                <owl:intersectionOf rdf:parseType="Collection">
                    <rdf:Description rdf:about="https://www.commoncoreontologies.org/ont00001298"/>
                    <owl:Restriction>
                        <owl:onProperty rdf:resource="http://purl.obolibrary.org/obo/BFO_0000178"/>
                        <owl:someValuesFrom rdf:resource="https://hack.cybersystems.engineer/memex/ontologies/SeamlessDigitalEngineering#Right_Declaration"/>
                    </owl:Restriction>
                </owl:intersectionOf>
            </owl:Class>
        </rdf:type>
        <rdfs:label xml:lang="en">Universal Declaration of Human Rights</rdfs:label>
        <rdfs:seeAlso rdf:datatype="http://www.w3.org/2001/XMLSchema#anyURI">https://en.wikisource.org/wiki/Universal_Declaration_of_Human_Rights</rdfs:seeAlso>
    </owl:NamedIndividual>
    


    <!-- https://hack.cybersystems.engineer/memex/ontologies/SeamlessDigitalEngineering#Universality_and_Equality_Cyber_Right -->

    <owl:NamedIndividual rdf:about="https://hack.cybersystems.engineer/memex/ontologies/SeamlessDigitalEngineering#Universality_and_Equality_Cyber_Right">
        <rdf:type rdf:resource="https://hack.cybersystems.engineer/memex/ontologies/SeamlessDigitalEngineering#Human_Cyber_Right"/>
        <rdfs:label xml:lang="en">Universality and Equality Cyber Right</rdfs:label>
        <skos:definition xml:lang="en">All Persons are born free and equal in dignity and Rights, which must be respected, protected and fulfilled in Cyberspace.</skos:definition>
        <cco2:ont00001754 rdf:resource="https://hack.cybersystems.engineer/memex/ontologies/SeamlessDigitalEngineering#Charter_of_Human_Rights_and_Principles_for_the_Internet"/>
    </owl:NamedIndividual>
    


    <!-- https://hack.cybersystems.engineer/memex/ontologies/SeamlessDigitalEngineering#University_of_Arizona -->

    <owl:NamedIndividual rdf:about="https://hack.cybersystems.engineer/memex/ontologies/SeamlessDigitalEngineering#University_of_Arizona">
        <rdf:type rdf:resource="https://www.commoncoreontologies.org/ont00000564"/>
        <obo:BFO_0000178 rdf:resource="https://hack.cybersystems.engineer/memex/ontologies/SeamlessDigitalEngineering#University_of_Arizona_Digital_Engineering_Factory"/>
        <rdfs:isDefinedBy rdf:datatype="http://www.w3.org/2001/XMLSchema#anyURI">https://www.wikidata.org/entity/Q503419</rdfs:isDefinedBy>
        <rdfs:label xml:lang="en">University of Arizona</rdfs:label>
        <rdfs:seeAlso rdf:datatype="http://www.w3.org/2001/XMLSchema#anyURI">https://en.wikipedia.org/wiki/University_of_Arizona</rdfs:seeAlso>
        <rdfs:seeAlso rdf:datatype="http://www.w3.org/2001/XMLSchema#anyURI">https://www.arizona.edu/</rdfs:seeAlso>
        <skos:altLabel xml:lang="en">UA</skos:altLabel>
    </owl:NamedIndividual>
    


    <!-- https://hack.cybersystems.engineer/memex/ontologies/SeamlessDigitalEngineering#University_of_Arizona_Digital_Engineering_Factory -->

    <owl:NamedIndividual rdf:about="https://hack.cybersystems.engineer/memex/ontologies/SeamlessDigitalEngineering#University_of_Arizona_Digital_Engineering_Factory">
        <rdf:type rdf:resource="https://hack.cybersystems.engineer/memex/ontologies/SeamlessDigitalEngineering#Digital_Engineering_Environment"/>
        <obo:BFO_0000176 rdf:resource="https://hack.cybersystems.engineer/memex/ontologies/SeamlessDigitalEngineering#University_of_Arizona"/>
        <rdfs:label xml:lang="en">UA Digital Engineering Factory</rdfs:label>
        <rdfs:seeAlso rdf:datatype="http://www.w3.org/2001/XMLSchema#anyURI">https://doi.org/10.1007/978-3-031-62554-1_18</rdfs:seeAlso>
        <skos:altLabel xml:lang="en">UA DEF</skos:altLabel>
    </owl:NamedIndividual>
    


    <!-- https://hack.cybersystems.engineer/memex/ontologies/SeamlessDigitalEngineering#EAL_7+ -->

    <owl:NamedIndividual rdf:about="https://hack.cybersystems.engineer/memex/ontologies/SeamlessDigitalEngineering#EAL_7+">
        <rdf:type rdf:resource="https://hack.cybersystems.engineer/memex/ontologies/SeamlessDigitalEngineering#Evaluation_Assurance_Level"/>
        <rdfs:label>EAL 7+</rdfs:label>
        <skos:definition xml:lang="en">Formally-verified design and tested, augmented</skos:definition>
        <cco2:ont00001754 xml:lang="en">ISO/IEC 15408-5:2022</cco2:ont00001754>
    </owl:NamedIndividual>
    


    <!-- https://hack.cybersystems.engineer/memex/ontologies/SeamlessDigitalEngineering#How_is_an_Evidence-based_Claim_supported? -->

    <owl:NamedIndividual rdf:about="https://hack.cybersystems.engineer/memex/ontologies/SeamlessDigitalEngineering#How_is_an_Evidence-based_Claim_supported?">
        <rdf:type rdf:resource="https://hack.cybersystems.engineer/memex/ontologies/SeamlessDigitalEngineering#Concern_Disposition"/>
        <rdfs:label xml:lang="en">How is an Evidence-based Claim supported?</rdfs:label>
        <cco2:ont00001754 rdf:datatype="http://www.w3.org/2001/XMLSchema#anyURI">https://saf.gfse.org/userdoc/Common%20Domain/Argumentation%20Assurance%20Viewpoint.html</cco2:ont00001754>
    </owl:NamedIndividual>
    


    <!-- https://hack.cybersystems.engineer/memex/ontologies/SeamlessDigitalEngineering#Life,_Libery_and_Security_Cyber_Right -->

    <owl:NamedIndividual rdf:about="https://hack.cybersystems.engineer/memex/ontologies/SeamlessDigitalEngineering#Life,_Libery_and_Security_Cyber_Right">
        <rdf:type rdf:resource="https://hack.cybersystems.engineer/memex/ontologies/SeamlessDigitalEngineering#Human_Cyber_Right"/>
        <rdfs:label xml:lang="en">Life, Liberty and Security Cyber Right</rdfs:label>
        <skos:definition xml:lang="en">The Rights to life, liberty, and security must be respected, protected and fulfilled in Cyberspace. These Rights must not be infringed upon, or used to infringe other Rights, in Cyberspace.</skos:definition>
        <cco2:ont00001754 rdf:resource="https://hack.cybersystems.engineer/memex/ontologies/SeamlessDigitalEngineering#Charter_of_Human_Rights_and_Principles_for_the_Internet"/>
    </owl:NamedIndividual>
    <rdf:Description>
        <owl:qualifiedCardinality rdf:datatype="http://www.w3.org/2001/XMLSchema#nonNegativeInteger">1</owl:qualifiedCardinality>
    </rdf:Description>
    <rdf:Description>
        <owl:qualifiedCardinality rdf:datatype="http://www.w3.org/2001/XMLSchema#nonNegativeInteger">1</owl:qualifiedCardinality>
    </rdf:Description>
    <rdf:Description>
        <owl:qualifiedCardinality rdf:datatype="http://www.w3.org/2001/XMLSchema#nonNegativeInteger">1</owl:qualifiedCardinality>
    </rdf:Description>
    <rdf:Description>
        <owl:qualifiedCardinality rdf:datatype="http://www.w3.org/2001/XMLSchema#nonNegativeInteger">1</owl:qualifiedCardinality>
    </rdf:Description>
    <rdf:Description>
        <owl:qualifiedCardinality rdf:datatype="http://www.w3.org/2001/XMLSchema#nonNegativeInteger">1</owl:qualifiedCardinality>
    </rdf:Description>
    


    <!-- 
    ///////////////////////////////////////////////////////////////////////////////////////
    //
    // Annotations
    //
    ///////////////////////////////////////////////////////////////////////////////////////
     -->

    <rdf:Description rdf:about="http://purl.obolibrary.org/obo/BFO_0000001">
        <skos:definition xml:lang="en">An entity is a single item to which a concept, need, or requirement applies: an organization, business unit, project, supplier, service, procedure, SOI (system, subsystem, system element), product, process, or stakeholder class (user, operator, tester, maintainer, etc.)</skos:definition>
        <cco2:ont00001754>INCOSE Needs and Requirements Manual R1.1 (2022)</cco2:ont00001754>
    </rdf:Description>
    <rdf:Description rdf:about="http://www.ontologyrepository.com/CommonCoreOntologies/CentralProcessingUnit">
        <cco2:ont00001753 xml:lang="en">CPU</cco2:ont00001753>
    </rdf:Description>
    <rdf:Description rdf:about="http://www.ontologyrepository.com/CommonCoreOntologies/GraphicsProcessingUnit">
        <cco2:ont00001753 xml:lang="en">GPU</cco2:ont00001753>
    </rdf:Description>
    <rdf:Description rdf:about="http://www.ontologyrepository.com/CommonCoreOntologies/ProcessingUnit">
        <skos:altLabel xml:lang="en">Processor</skos:altLabel>
    </rdf:Description>
    <rdf:Description rdf:about="https://www.commoncoreontologies.org/ont00000010">
        <skos:altLabel xml:lang="en">business</skos:altLabel>
    </rdf:Description>
    


    <!-- 
    ///////////////////////////////////////////////////////////////////////////////////////
    //
    // General axioms
    //
    ///////////////////////////////////////////////////////////////////////////////////////
     -->

    <rdf:Description>
        <rdf:type rdf:resource="http://www.w3.org/2002/07/owl#AllDisjointClasses"/>
        <owl:members rdf:parseType="Collection">
            <rdf:Description rdf:about="https://hack.cybersystems.engineer/memex/ontologies/SeamlessDigitalEngineering#Acceptance_Report"/>
            <rdf:Description rdf:about="https://hack.cybersystems.engineer/memex/ontologies/SeamlessDigitalEngineering#Configuration_Status_Report"/>
            <rdf:Description rdf:about="https://hack.cybersystems.engineer/memex/ontologies/SeamlessDigitalEngineering#Evaluation_Report"/>
            <rdf:Description rdf:about="https://hack.cybersystems.engineer/memex/ontologies/SeamlessDigitalEngineering#Incident_Report"/>
            <rdf:Description rdf:about="https://hack.cybersystems.engineer/memex/ontologies/SeamlessDigitalEngineering#Installation_Report"/>
            <rdf:Description rdf:about="https://hack.cybersystems.engineer/memex/ontologies/SeamlessDigitalEngineering#Integration_and_Test_Report"/>
            <rdf:Description rdf:about="https://hack.cybersystems.engineer/memex/ontologies/SeamlessDigitalEngineering#Monitoring_and_Control_Report"/>
            <rdf:Description rdf:about="https://hack.cybersystems.engineer/memex/ontologies/SeamlessDigitalEngineering#Narrative_Introduction_Report"/>
            <rdf:Description rdf:about="https://hack.cybersystems.engineer/memex/ontologies/SeamlessDigitalEngineering#Problem_Report"/>
            <rdf:Description rdf:about="https://hack.cybersystems.engineer/memex/ontologies/SeamlessDigitalEngineering#Process_Improvement_Report"/>
            <rdf:Description rdf:about="https://hack.cybersystems.engineer/memex/ontologies/SeamlessDigitalEngineering#Product_Need_Assessment"/>
            <rdf:Description rdf:about="https://hack.cybersystems.engineer/memex/ontologies/SeamlessDigitalEngineering#Progress_Report"/>
            <rdf:Description rdf:about="https://hack.cybersystems.engineer/memex/ontologies/SeamlessDigitalEngineering#Review_Minutes"/>
            <rdf:Description rdf:about="https://hack.cybersystems.engineer/memex/ontologies/SeamlessDigitalEngineering#Service_Report"/>
            <rdf:Description rdf:about="https://hack.cybersystems.engineer/memex/ontologies/SeamlessDigitalEngineering#Test_Report"/>
            <rdf:Description rdf:about="https://hack.cybersystems.engineer/memex/ontologies/SeamlessDigitalEngineering#Validation_Report"/>
            <rdf:Description rdf:about="https://hack.cybersystems.engineer/memex/ontologies/SeamlessDigitalEngineering#Verification_Report"/>
        </owl:members>
    </rdf:Description>
    <rdf:Description>
        <rdf:type rdf:resource="http://www.w3.org/2002/07/owl#AllDisjointClasses"/>
        <owl:members rdf:parseType="Collection">
            <rdf:Description rdf:about="https://hack.cybersystems.engineer/memex/ontologies/SeamlessDigitalEngineering#Computability_Theory_Discipline"/>
            <rdf:Description rdf:about="https://hack.cybersystems.engineer/memex/ontologies/SeamlessDigitalEngineering#Model_Theory_Discipline"/>
            <rdf:Description rdf:about="https://hack.cybersystems.engineer/memex/ontologies/SeamlessDigitalEngineering#Proof_Theory_Discipline"/>
            <rdf:Description rdf:about="https://hack.cybersystems.engineer/memex/ontologies/SeamlessDigitalEngineering#Set_Theory_Discipline"/>
        </owl:members>
    </rdf:Description>
    <rdf:Description>
        <rdf:type rdf:resource="http://www.w3.org/2002/07/owl#AllDisjointClasses"/>
        <owl:members rdf:parseType="Collection">
            <rdf:Description rdf:about="https://hack.cybersystems.engineer/memex/ontologies/SeamlessDigitalEngineering#Concept_Stage"/>
            <rdf:Description rdf:about="https://hack.cybersystems.engineer/memex/ontologies/SeamlessDigitalEngineering#Development_Stage"/>
            <rdf:Description rdf:about="https://hack.cybersystems.engineer/memex/ontologies/SeamlessDigitalEngineering#Production_Stage"/>
            <rdf:Description rdf:about="https://hack.cybersystems.engineer/memex/ontologies/SeamlessDigitalEngineering#Retirement_Stage"/>
        </owl:members>
    </rdf:Description>
    <rdf:Description>
        <rdf:type rdf:resource="http://www.w3.org/2002/07/owl#AllDisjointClasses"/>
        <owl:members rdf:parseType="Collection">
            <rdf:Description rdf:about="https://hack.cybersystems.engineer/memex/ontologies/SeamlessDigitalEngineering#Explanation_Material"/>
            <rdf:Description rdf:about="https://hack.cybersystems.engineer/memex/ontologies/SeamlessDigitalEngineering#How-to_Guide"/>
            <rdf:Description rdf:about="https://hack.cybersystems.engineer/memex/ontologies/SeamlessDigitalEngineering#Reference_Material"/>
            <rdf:Description rdf:about="https://hack.cybersystems.engineer/memex/ontologies/SeamlessDigitalEngineering#Tutorial"/>
        </owl:members>
    </rdf:Description>
</rdf:RDF>



<!-- Generated by the OWL API (version 4.5.29.2024-05-13T12:11:03Z) https://github.com/owlcs/owlapi -->

